@prefix :     <http://www.prostep.org/ontologies/ecad/2024/03/vec#> .
@prefix owl:  <http://www.w3.org/2002/07/owl#> .
@prefix rdf:  <http://www.w3.org/1999/02/22-rdf-syntax-ns#> .
@prefix rdfs: <http://www.w3.org/2000/01/rdf-schema#> .
@prefix vec:  <http://www.prostep.org/ontologies/ecad/2024/03/vec#> .
@prefix xs:   <http://www.w3.org/2001/XMLSchema#> .

vec:WireLengthType_Production
        rdf:type         vec:WireLengthType , owl:NamedIndividiual;
        rdfs:comment     "The cutting length for the used in production environments.\n"@en;
        vec:enumLiteral  "Production" .

vec:LanguageCode_Ar  rdf:type  vec:LanguageCode , owl:NamedIndividiual;
        vec:enumLiteral  "Ar" .

vec:SignalSubType_LIN
        rdf:type         vec:SignalSubType , owl:NamedIndividiual;
        rdfs:comment     "Local Interconnect Network"@en;
        vec:enumLiteral  "LIN" .

vec:TypeOfPermission_Seen
        rdf:type         vec:TypeOfPermission , owl:NamedIndividiual;
        vec:enumLiteral  "Seen" .

vec:documentVersionFileName
        rdf:type      owl:DatatypeProperty;
        rdfs:comment  "The name of the file as it appears in the VEC-Package, including the folder structure (fully qualified name) that contains this DocumentVersion . If this DocumentVersion is a link to an external document (e.g. a ComponentSymbol), then the fileName attribute points to the file containing the original document. The usage of this attribute is only valid, if the original document is distributed along with the VEC-file in a VEC-Package. It must not point to any file location which is not part of the VEC-Package (e.g. a File on a central server file share).\n"@en;
        rdfs:domain   vec:DocumentVersion;
        rdfs:label    "fileName"@en;
        rdfs:range    xs:string .

vec:PrimaryPartType_CavityAccessory
        rdf:type         vec:PrimaryPartType , owl:NamedIndividiual;
        vec:enumLiteral  "CavityAccessory" .

vec:housingComponentSegmentConnectionPoint
        rdf:type            owl:ObjectProperty;
        rdfs:comment        "Specifies the SegmentConnectionPoints the HousingComponent .\n"@en;
        rdfs:domain         vec:HousingComponent;
        rdfs:label          "segmentConnectionPoint"@en;
        rdfs:range          vec:SegmentConnectionPointHC;
        rdfs:subPropertyOf  vec:contains .

vec:SiUnitName_Kelvin
        rdf:type         vec:SiUnitName , owl:NamedIndividiual;
        vec:enumLiteral  "Kelvin" .

vec:SealState_Sealed  rdf:type  vec:SealState , owl:NamedIndividiual;
        rdfs:comment     "The splice is waterproof.\n"@en;
        vec:enumLiteral  "Sealed" .

vec:internalComponentConnectionPins
        rdf:type     owl:ObjectProperty;
        rdfs:domain  vec:InternalComponentConnection;
        rdfs:label   "pins"@en;
        rdfs:range   vec:PinComponent .

vec:LanguageCode_Cs  rdf:type  vec:LanguageCode , owl:NamedIndividiual;
        vec:enumLiteral  "Cs" .

vec:LanguageCode_Yo  rdf:type  vec:LanguageCode , owl:NamedIndividiual;
        vec:enumLiteral  "Yo" .

vec:SiUnitName_Newton
        rdf:type         vec:SiUnitName , owl:NamedIndividiual;
        vec:enumLiteral  "Newton" .

vec:approvalDescription
        rdf:type            owl:ObjectProperty;
        rdfs:comment        "Room for additional information about the item.\n"@en;
        rdfs:domain         vec:Approval;
        rdfs:label          "description"@en;
        rdfs:range          vec:AbstractLocalizedString;
        rdfs:subPropertyOf  vec:contains .

vec:LanguageCode_Sq  rdf:type  vec:LanguageCode , owl:NamedIndividiual;
        vec:enumLiteral  "Sq" .

vec:LanguageCode_Et  rdf:type  vec:LanguageCode , owl:NamedIndividiual;
        vec:enumLiteral  "Et" .

vec:onWayPlacementStartLocation
        rdf:type            owl:ObjectProperty;
        rdfs:comment        "References the Location where OnWayPlacement starts. \n"@en;
        rdfs:domain         vec:OnWayPlacement;
        rdfs:label          "startLocation"@en;
        rdfs:range          vec:Location;
        rdfs:subPropertyOf  vec:contains .

vec:SiUnitName_Weber  rdf:type  vec:SiUnitName , owl:NamedIndividiual;
        vec:enumLiteral  "Weber" .

vec:CurrentType_ACTwoPhase
        rdf:type         vec:CurrentType , owl:NamedIndividiual;
        vec:enumLiteral  "ACTwoPhase" .

vec:netTypeDescription
        rdf:type            owl:ObjectProperty;
        rdfs:comment        "Room for additional, human readable information about the NetType .\n"@en;
        rdfs:domain         vec:NetType;
        rdfs:label          "description"@en;
        rdfs:range          vec:AbstractLocalizedString;
        rdfs:subPropertyOf  vec:contains .

vec:LanguageCode_Ms  rdf:type  vec:LanguageCode , owl:NamedIndividiual;
        vec:enumLiteral  "Ms" .

vec:SiUnitName_Candela
        rdf:type         vec:SiUnitName , owl:NamedIndividiual;
        vec:enumLiteral  "Candela" .

vec:PrimaryPartType_EEComponent
        rdf:type         vec:PrimaryPartType , owl:NamedIndividiual;
        vec:enumLiteral  "EEComponent" .

vec:TransmissionMediumType_Pneumatic
        rdf:type         vec:TransmissionMediumType , owl:NamedIndividiual;
        vec:enumLiteral  "Pneumatic" .

vec:componentPortSignal
        rdf:type      owl:ObjectProperty;
        rdfs:comment  "References the Signal that is associated with the ComponentPort .\n"@en;
        rdfs:domain   vec:ComponentPort;
        rdfs:label    "signal"@en;
        rdfs:range    vec:Signal .

vec:configurableElementAssociatedAssignmentGroups
        rdf:type     owl:ObjectProperty;
        rdfs:domain  vec:ConfigurableElement;
        rdfs:label   "associatedAssignmentGroups"@en;
        rdfs:range   vec:AssignmentGroup .

vec:LanguageCode_Ur  rdf:type  vec:LanguageCode , owl:NamedIndividiual;
        vec:enumLiteral  "Ur" .

vec:InsulationSpecification
        rdf:type         owl:Class;
        rdfs:comment     "Specification for the definition of insulation properties of a WireElement.\n"@en;
        rdfs:label       "InsulationSpecification"@en;
        rdfs:subClassOf  vec:Specification .

vec:LanguageCode_Gu  rdf:type  vec:LanguageCode , owl:NamedIndividiual;
        vec:enumLiteral  "Gu" .

vec:PinCurrentType_ClippingCurrent
        rdf:type         vec:PinCurrentType , owl:NamedIndividiual;
        rdfs:comment     "Current at which the output driver of an ECU turns off or limits the current on an output in (a behavior similar to a fuse).\n"@en;
        vec:enumLiteral  "clippingCurrent" .

vec:conductorSpecificationPlatingMaterial
        rdf:type            owl:ObjectProperty;
        rdfs:comment        "Specifies the plating material of the conductor.\n"@en;
        rdfs:domain         vec:ConductorSpecification;
        rdfs:label          "platingMaterial"@en;
        rdfs:range          vec:Material;
        rdfs:subPropertyOf  vec:contains .

vec:ImperialUnitName_Chain
        rdf:type         vec:ImperialUnitName , owl:NamedIndividiual;
        vec:enumLiteral  "Chain" .

vec:boundingBoxZ  rdf:type  owl:ObjectProperty;
        rdfs:comment        "Defines the extent of the bounding box in the direction of z (height).\n"@en;
        rdfs:domain         vec:BoundingBox;
        rdfs:label          "z"@en;
        rdfs:range          vec:NumericalValue;
        rdfs:subPropertyOf  vec:contains .

vec:TerminalType  rdf:type  owl:Class;
        rdfs:comment     "Defines the type (system) of a terminal. The type is specified by a combination of a name for the system and an optional nominalSize.\nIn some processes the terminal type is referred as cavity system, because the system of cavities, terminals, seals, plugs and other cavity accessories must match┬á/┬ábe compatible.\nHowever, since a terminal has only one since type and a cavity can be compatible to more than one it is named TerminalType in the VEC.\n"@en;
        rdfs:label       "TerminalType"@en;
        rdfs:subClassOf  vec:ExtendableElement .

vec:wireElementSpecificationType
        rdf:type            owl:ObjectProperty;
        rdfs:comment        "Defines the type of the wire. A wire must not have more than one type. This attribute allows more than one value for the reason, that the same type can be expressed in multiple reference systems.\n"@en;
        rdfs:domain         vec:WireElementSpecification;
        rdfs:label          "type"@en;
        rdfs:range          vec:WireType;
        rdfs:subPropertyOf  vec:contains .

vec:PartOccurrence  rdf:type  owl:Class;
        rdfs:comment     "A PartOccurrence is an instance of a component with a specified part number (PartVersion).\n"@en;
        rdfs:label       "PartOccurrence"@en;
        rdfs:subClassOf  vec:OccurrenceOrUsage .

vec:MassInformationSource
        rdf:type         owl:Class;
        rdfs:comment     "Defines possible sources for MassInformations .\n"@en;
        rdfs:label       "MassInformationSource"@en;
        rdfs:subClassOf  vec:OpenEnumeration .

vec:placeableElementSpecificationMeasurementPoint
        rdf:type            owl:ObjectProperty;
        rdfs:comment        "Specifies the MeasurementPoints of a PlaceableElement .\n"@en;
        rdfs:domain         vec:PlaceableElementSpecification;
        rdfs:label          "measurementPoint"@en;
        rdfs:range          vec:MeasurementPoint;
        rdfs:subPropertyOf  vec:contains .

vec:GeneralTechnicalPartSpecification
        rdf:type         owl:Class;
        rdfs:comment     "Specification for the definition of common properties for technical parts.\n"@en;
        rdfs:label       "GeneralTechnicalPartSpecification"@en;
        rdfs:subClassOf  vec:PartOrUsageRelatedSpecification .

vec:measurementPointReferenceIdentification
        rdf:type      owl:DatatypeProperty;
        rdfs:comment  "Specifies a unique identification of the MeasurementPointReference. The identification is guaranteed to be unique within the containing PlaceableElementRole.\n"@en;
        rdfs:domain   vec:MeasurementPointReference;
        rdfs:label    "identification"@en;
        rdfs:range    xs:string .

vec:TerminalBoltType_Plain
        rdf:type         vec:TerminalBoltType , owl:NamedIndividiual;
        rdfs:comment     "A plain bolt without an special features.\n"@en;
        vec:enumLiteral  "Plain" .

vec:Size  rdf:type    owl:Class;
        rdfs:comment  "Defines the size of an element by width & height. Per definition is width > height.\n"@en;
        rdfs:label    "Size"@en .

vec:LanguageCode_Qu  rdf:type  vec:LanguageCode , owl:NamedIndividiual;
        vec:enumLiteral  "Qu" .

vec:sizeWidth  rdf:type     owl:ObjectProperty;
        rdfs:comment        "The width of the element.\n"@en;
        rdfs:domain         vec:Size;
        rdfs:label          "width"@en;
        rdfs:range          vec:NumericalValue;
        rdfs:subPropertyOf  vec:contains .

vec:contains  rdf:type  owl:ObjectProperty;
        rdfs:comment  "This is the representation of the containment modeled in the UML. All associations that are a \"containment\" in the UML model are subproperties of this property."@en;
        rdfs:label    "contains"@en .

vec:PartRelationType_Custom
        rdf:type         vec:PartRelationType , owl:NamedIndividiual;
        rdfs:comment     "Custom means, that there is some kind of custom constraints /┬álogic between referenced PartVersions that has to be evaluated to determine the selected accessories.\n"@en;
        vec:enumLiteral  "Custom" .

vec:multiCavityPlugSpecificationAssignment
        rdf:type            owl:ObjectProperty;
        rdfs:comment        "References the SealedCavitiesAssignments that are valid for this MultiCavityPlug . One individual SealedCavitiesAssignment is used for each connector housing that matches witch this MultiCavityPlug.\n"@en;
        rdfs:domain         vec:MultiCavityPlugSpecification;
        rdfs:label          "assignment"@en;
        rdfs:range          vec:SealedCavitiesAssignment;
        rdfs:subPropertyOf  vec:contains .

vec:BoltTerminalRole  rdf:type  owl:Class;
        rdfs:comment     "A BoltTerminalRole defines the instance specific properties and relationships of a ring terminal.\n"@en;
        rdfs:label       "BoltTerminalRole"@en;
        rdfs:subClassOf  vec:TerminalRole .

vec:partUsageInstanciatedUsage
        rdf:type     owl:ObjectProperty;
        rdfs:domain  vec:PartUsage;
        rdfs:label   "instanciatedUsage"@en;
        rdfs:range   vec:PartUsage .

vec:NetworkNodeType_Ground
        rdf:type         vec:NetworkNodeType , owl:NamedIndividiual;
        rdfs:comment     "Defines that this NetworkNode is a grounding point.\n"@en;
        vec:enumLiteral  "Ground" .

vec:TopologyBendingRestriction
        rdf:type      owl:Class;
        rdfs:comment  "As the name implies, a TopologyBendingRestriction defines restrictions on the bendability a path in the Topology. There are multiple reasons, why such restrictions exist, for example: There is a bending restriction for a wire in the segment. The number of wires and the segment diameter is such, that excessive bending causes intolerable torsion forces on wires in the segment. Other technical reasons Since these restrictions can be determined using a variety of methods the VEC provides a concept to store this information for later use. This makes the information available in the downstream processes, without detailed knowledge of the determination procedure (e.g. during form board design, packaging or installation).\nThe restriction applies to a path of segments as this can cover different case: a single segment two adjacent segments at a node the complete path of a wire "@en;
        rdfs:label    "TopologyBendingRestriction"@en .

vec:slotCouplingIdentification
        rdf:type     owl:DatatypeProperty;
        rdfs:domain  vec:SlotCoupling;
        rdfs:label   "identification"@en;
        rdfs:range   xs:string .

vec:CartesianPoint2DWrapper
        rdf:type      owl:Class;
        rdfs:comment  "Container class for CartesianPoint2D to participate in non-unique and/or ordered associations." .

vec:ConnectionGroupType_Shielded
        rdf:type         vec:ConnectionGroupType , owl:NamedIndividiual;
        vec:enumLiteral  "Shielded" .

vec:tubeSpecificationShape
        rdf:type            owl:ObjectProperty;
        rdfs:comment        "Specifies the shape of the cross section of the tube.\nThis attribute is defined as an OpenEnumeration\n"@en;
        rdfs:domain         vec:TubeSpecification;
        rdfs:label          "shape"@en;
        rdfs:range          vec:TubeShape;
        rdfs:subPropertyOf  vec:contains .

vec:pinComponentBehaviorApplianceType
        rdf:type            owl:ObjectProperty;
        rdfs:comment        "Classifies the appliance of a Pin in terms of the duration of the appliance (see PinApplianceType).\n"@en;
        rdfs:domain         vec:PinComponentBehavior;
        rdfs:label          "applianceType"@en;
        rdfs:range          vec:PinApplianceType;
        rdfs:subPropertyOf  vec:contains .

vec:tubeSpecificationWidth
        rdf:type            owl:ObjectProperty;
        rdfs:comment        "Specifies the width of the tube. If the width is defined, a height shall be defined, too. The height and width of a tube shall only be used for tubes that are not circular (shape != Circular). For circular shapes, the outside diameter shall be used.\n"@en;
        rdfs:domain         vec:TubeSpecification;
        rdfs:label          "width"@en;
        rdfs:range          vec:NumericalValue;
        rdfs:subPropertyOf  vec:contains .

vec:LanguageCode_Sv  rdf:type  vec:LanguageCode , owl:NamedIndividiual;
        vec:enumLiteral  "Sv" .

vec:PrimaryLockingType_Lance
        rdf:type         vec:PrimaryLockingType , owl:NamedIndividiual;
        vec:enumLiteral  "Lance" .

vec:ImperialUnitName_Mile
        rdf:type         vec:ImperialUnitName , owl:NamedIndividiual;
        vec:enumLiteral  "Mile" .

vec:transformation2DA11
        rdf:type     owl:DatatypeProperty;
        rdfs:domain  vec:Transformation2D;
        rdfs:label   "a11"@en;
        rdfs:range   xs:double .

vec:cavityAddOnCavity
        rdf:type     owl:ObjectProperty;
        rdfs:domain  vec:CavityAddOn;
        rdfs:label   "cavity"@en;
        rdfs:range   vec:Cavity .

vec:OpenCavitiesAssignment
        rdf:type      owl:Class;
        rdfs:comment  "An OpenCavitiesAssignment groups the cavities of ONE connector that are open in a MultiCavitySeal. If a MultiCavitySeal fits into more than one connector, than there are as many OpenCavitiesAssignments.\n"@en;
        rdfs:label    "OpenCavitiesAssignment"@en .

vec:NetworkPortViewItemSide_Left
        rdf:type         vec:NetworkPortViewItemSide , owl:NamedIndividiual;
        vec:enumLiteral  "Left" .

vec:PrimaryPartType_CableTie
        rdf:type         vec:PrimaryPartType , owl:NamedIndividiual;
        vec:enumLiteral  "CableTie" .

vec:itemVersionContract
        rdf:type      owl:ObjectProperty;
        rdfs:comment  "References the contracts that apply to an ItemVersion.\n"@en;
        rdfs:domain   vec:ItemVersion;
        rdfs:label    "contract"@en;
        rdfs:range    vec:Contract .

vec:wireElementReferenceLabelPosition
        rdf:type            owl:ObjectProperty;
        rdfs:comment        "Specifies the position of label, if this WireElementReference is labled."@en;
        rdfs:domain         vec:WireElementReference;
        rdfs:label          "labelPosition"@en;
        rdfs:range          vec:LabelPosition;
        rdfs:subPropertyOf  vec:contains .

vec:PinTimingType_OverrunTime
        rdf:type         vec:PinTimingType , owl:NamedIndividiual;
        vec:enumLiteral  "overrunTime" .

vec:SignalCurve_ContinuousSignal
        rdf:type         vec:SignalCurve , owl:NamedIndividiual;
        vec:enumLiteral  "continuousSignal" .

vec:MassInformationSource_Prototype
        rdf:type         vec:MassInformationSource , owl:NamedIndividiual;
        rdfs:comment     "A MassInformation with this valueSource has been determined based on a preproduction part.\n"@en;
        vec:enumLiteral  "Prototype" .

vec:cartesianDimensionWidth
        rdf:type      owl:DatatypeProperty;
        rdfs:comment  "Specifies the width of the object. The unit of this value is the baseUnit of containing BuildingBlockSpecification2D.\n"@en;
        rdfs:domain   vec:CartesianDimension;
        rdfs:label    "width"@en;
        rdfs:range    xs:double .

vec:RingTerminalRole  rdf:type  owl:Class;
        rdfs:comment     "A RingTerminalRole defines the instance specific properties and relationships of a ring terminal.\n"@en;
        rdfs:label       "RingTerminalRole"@en;
        rdfs:subClassOf  vec:TerminalRole .

vec:UsageNodeType_CableDuct
        rdf:type         vec:UsageNodeType , owl:NamedIndividiual;
        vec:enumLiteral  "CableDuct" .

vec:insulationSpecificationLabelIdentificationColor
        rdf:type            owl:ObjectProperty;
        rdfs:comment        "Specifies the color of a label printed on the insulation of the wire.\n"@en;
        rdfs:domain         vec:InsulationSpecification;
        rdfs:label          "labelIdentificationColor"@en;
        rdfs:range          vec:Color;
        rdfs:subPropertyOf  vec:contains .

vec:housingComponentHousingSpecification
        rdf:type      owl:ObjectProperty;
        rdfs:comment  "References the ConnectorHousingSpecification that is describing the connector interface of the HousingComponent (e.g. Slots, Cavities, Design, Coding).\n"@en;
        rdfs:domain   vec:HousingComponent;
        rdfs:label    "housingSpecification"@en;
        rdfs:range    vec:ConnectorHousingSpecification .

vec:moduleFamilyDescription
        rdf:type            owl:ObjectProperty;
        rdfs:comment        "Room for additional, human readable information about the ModuleFamily.\n"@en;
        rdfs:domain         vec:ModuleFamily;
        rdfs:label          "description"@en;
        rdfs:range          vec:AbstractLocalizedString;
        rdfs:subPropertyOf  vec:contains .

vec:terminalReceptionSpecificationPrimaryLockingType
        rdf:type            owl:ObjectProperty;
        rdfs:comment        "Specifies if the terminal reception has a primary locking and of what type it is.\n"@en;
        rdfs:domain         vec:TerminalReceptionSpecification;
        rdfs:label          "primaryLockingType"@en;
        rdfs:range          vec:PrimaryLockingType;
        rdfs:subPropertyOf  vec:contains .

vec:IECPrefix_Zebi  rdf:type  vec:IECPrefix , owl:NamedIndividiual;
        vec:enumLiteral  "Zebi" .

vec:slotSealingType  rdf:type  owl:ObjectProperty;
        rdfs:comment        "Specifies the type of the sealing of the slot, if sealed. The values are defined in an OpenEnumeration .\n"@en;
        rdfs:domain         vec:Slot;
        rdfs:label          "sealingType"@en;
        rdfs:range          vec:SlotSealingType;
        rdfs:subPropertyOf  vec:contains .

vec:SiUnitName  rdf:type     owl:Class;
        rdfs:comment         "Enumeration for the definition of SI unit names. In difference to the SI-System gram is used as literal for the measurement of mass, instead of kilogram. Since a unit is formed with prefix and unit name gram would have to be defined as milli kilogram otherwise.\n"@en;
        rdfs:label           "SiUnitName"@en;
        rdfs:subClassOf      vec:ClosedEnumeration;
        owl:equivalentClass  [ rdf:type   owl:Class;
                               owl:oneOf  ( vec:SiUnitName_Metre vec:SiUnitName_Gram vec:SiUnitName_Second vec:SiUnitName_Ampere vec:SiUnitName_Kelvin vec:SiUnitName_Mole vec:SiUnitName_Candela vec:SiUnitName_Radian vec:SiUnitName_Steradian vec:SiUnitName_Hertz vec:SiUnitName_Newton vec:SiUnitName_Pascal vec:SiUnitName_Joule vec:SiUnitName_Watt vec:SiUnitName_Coulomb vec:SiUnitName_Volt vec:SiUnitName_Farad vec:SiUnitName_Ohm vec:SiUnitName_Siemens vec:SiUnitName_Weber vec:SiUnitName_Tesla vec:SiUnitName_Henry vec:SiUnitName_DegreeCelsius vec:SiUnitName_Lumen vec:SiUnitName_Lux vec:SiUnitName_Becquerel vec:SiUnitName_Gray vec:SiUnitName_Sievert vec:SiUnitName_Katal )
                             ] .

vec:shrinkableTubeSpecificationResin
        rdf:type            owl:ObjectProperty;
        rdfs:comment        "Defines the material of the resin usable for this shrinkable tube.\n"@en;
        rdfs:domain         vec:ShrinkableTubeSpecification;
        rdfs:label          "resin"@en;
        rdfs:range          vec:Material;
        rdfs:subPropertyOf  vec:contains .

vec:TerminalBoltNominalSize_M10
        rdf:type         vec:TerminalBoltNominalSize , owl:NamedIndividiual;
        vec:enumLiteral  "M10" .

vec:matingPointMatingDetail
        rdf:type            owl:ObjectProperty;
        rdfs:comment        "Specifies the MatingDetails, if a detailed description of the relationships between TerminalReceptions and TerminalReceptions is needed. \n"@en;
        rdfs:domain         vec:MatingPoint;
        rdfs:label          "matingDetail"@en;
        rdfs:range          vec:MatingDetail;
        rdfs:subPropertyOf  vec:contains .

vec:MultiFuseType_Welded
        rdf:type         vec:MultiFuseType , owl:NamedIndividiual;
        vec:enumLiteral  "Welded" .

vec:PartRelationType_Mandatory
        rdf:type         vec:PartRelationType , owl:NamedIndividiual;
        rdfs:comment     " Mandatory means that in a usage of a component all referenced acessoryParts must be used.\n"@en;
        vec:enumLiteral  "Mandatory" .

vec:FunctionalAssignmentGroup
        rdf:type         owl:Class;
        rdfs:comment     "The FunctionalAssignmentGroup clusters elements that contribute to a specific function or a functional aspect. With such a group, certain functional requirements can be associated.\n"@en;
        rdfs:label       "FunctionalAssignmentGroup"@en;
        rdfs:subClassOf  vec:AssignmentGroup .

vec:ImperialUnitName_Inch
        rdf:type         vec:ImperialUnitName , owl:NamedIndividiual;
        vec:enumLiteral  "Inch" .

vec:pinWireMappingPointContactPoint
        rdf:type     owl:ObjectProperty;
        rdfs:domain  vec:PinWireMappingPoint;
        rdfs:label   "contactPoint"@en;
        rdfs:range   vec:ContactPoint .

vec:personPhoneNumber
        rdf:type      owl:DatatypeProperty;
        rdfs:comment  "Specifies the person's phone number.\n"@en;
        rdfs:domain   vec:Person;
        rdfs:label    "phoneNumber"@en;
        rdfs:range    xs:string .

vec:topologyZoneType  rdf:type  owl:ObjectProperty;
        rdfs:comment        "The type of the TopologyZone. Valid values are defined in an OpenEnumeration.\n"@en;
        rdfs:domain         vec:TopologyZone;
        rdfs:label          "type"@en;
        rdfs:range          vec:TopologyZoneType;
        rdfs:subPropertyOf  vec:contains .

vec:wireMountingWireEndAccessory
        rdf:type     owl:ObjectProperty;
        rdfs:domain  vec:WireMounting;
        rdfs:label   "wireEndAccessory"@en;
        rdfs:range   vec:WireEndAccessoryRole .

vec:cavityAccessorySpecificationWireReceptionType
        rdf:type            owl:ObjectProperty;
        rdfs:comment        "Specifies the wireReceptionType to which the cavity accessory fits.\n"@en;
        rdfs:domain         vec:CavityAccessorySpecification;
        rdfs:label          "wireReceptionType"@en;
        rdfs:range          vec:WireReceptionType;
        rdfs:subPropertyOf  vec:contains .

vec:cableLeadThroughSpecificationMaxSegmentOutsideDiameter
        rdf:type            owl:ObjectProperty;
        rdfs:comment        "Specifies the maximum diameter a segment can have to fit into the cable lead through.\n"@en;
        rdfs:domain         vec:CableLeadThroughSpecification;
        rdfs:label          "maxSegmentOutsideDiameter"@en;
        rdfs:range          vec:NumericalValue;
        rdfs:subPropertyOf  vec:contains .

vec:TemperatureType_StorageTemperature
        rdf:type         vec:TemperatureType , owl:NamedIndividiual;
        vec:enumLiteral  "StorageTemperature" .

vec:sheetOrChapterSpecification
        rdf:type            owl:ObjectProperty;
        rdfs:comment        "Specifies the Specifications contained in the SheetOrChapter. All structured, technical information in the VEC is described by such Specifications. \n"@en;
        rdfs:domain         vec:SheetOrChapter;
        rdfs:label          "specification"@en;
        rdfs:range          vec:Specification;
        rdfs:subPropertyOf  vec:contains .

vec:ringTerminalSpecificationBoltNominalSize
        rdf:type            owl:ObjectProperty;
        rdfs:comment        "Defines the size (diameter) of the bolt for which the ring terminal is designed for in a nominal way (e.g. \"M8\").\n"@en;
        rdfs:domain         vec:RingTerminalSpecification;
        rdfs:label          "boltNominalSize"@en;
        rdfs:range          vec:TerminalBoltNominalSize;
        rdfs:subPropertyOf  vec:contains .

vec:housingComponentReferenceConnectorHousingRole
        rdf:type            owl:ObjectProperty;
        rdfs:domain         vec:HousingComponentReference;
        rdfs:label          "connectorHousingRole"@en;
        rdfs:range          vec:ConnectorHousingRole;
        rdfs:subPropertyOf  vec:contains .

vec:ComponentPortViewItemSide
        rdf:type             owl:Class;
        rdfs:label           "ComponentPortViewItemSide"@en;
        rdfs:subClassOf      vec:ClosedEnumeration;
        owl:equivalentClass  [ rdf:type   owl:Class;
                               owl:oneOf  ( vec:ComponentPortViewItemSide_Top vec:ComponentPortViewItemSide_Bottom vec:ComponentPortViewItemSide_Left vec:ComponentPortViewItemSide_Right )
                             ] .

vec:TerminalBoltNominalSize_M52
        rdf:type         vec:TerminalBoltNominalSize , owl:NamedIndividiual;
        vec:enumLiteral  "M52" .

vec:SiPrefix_Giga  rdf:type  vec:SiPrefix , owl:NamedIndividiual;
        vec:enumLiteral  "Giga" .

vec:changeDescriptionChangeDate
        rdf:type      owl:DatatypeProperty;
        rdfs:comment  "Specifies the date when the change was performed.\n"@en;
        rdfs:domain   vec:ChangeDescription;
        rdfs:label    "changeDate"@en;
        rdfs:range    xs:dateTime .

[ rdf:type     owl:AllDisjointClasses;
  owl:members  ( vec:CoreSpecification vec:ShieldSpecification vec:FlatCoreSpecification )
] .

vec:TopologyBendingRestrictionSpecification
        rdf:type         owl:Class;
        rdfs:comment     "A TopologyBendingRestrictionSpecification can be used to define TopologyBendingRestrictions.\n"@en;
        rdfs:label       "TopologyBendingRestrictionSpecification"@en;
        rdfs:subClassOf  vec:Specification .

vec:NominalVoltage_HV
        rdf:type         vec:NominalVoltage , owl:NamedIndividiual;
        rdfs:comment     "HV defines all voltages that are dangerous to health or life, regardless if alternating (AC) or direct current (DC). This literal should be used if the concrete class is not known, not defined or not specified.\n"@en;
        vec:enumLiteral  "HV" .

vec:wireProtectionRoleProtectionLength
        rdf:type            owl:ObjectProperty;
        rdfs:comment        "The ProtectionLength specifies the length of the area covered by the protection. As a consequence, the ProtectionLength may differ from the real length of the material (e.g. for tapes).\n"@en;
        rdfs:domain         vec:WireProtectionRole;
        rdfs:label          "protectionLength"@en;
        rdfs:range          vec:NumericalValue;
        rdfs:subPropertyOf  vec:contains .

vec:PrimaryPartType  rdf:type  owl:Class;
        rdfs:comment         "The primary type of the part defines the type of the part (e.g. ConnectorHousing, Fixing, etc.) Since the VEC supports dual use parts (e.g. Fixing & WireProtection) the primary part type is necessary to define which specification associated to part is the primary character of the part. Therefore, all primary part types correspond to a PartOrUsageRelatedSpecification (e.g. ConnectorHousing --> ConnectorHousingSpecification).\nThe primary part type 'Other' is used if the PartVersion is not further specified by the VEC, which means it has no PartOrUsageRelatedSpecification, only a GeneralTechnicalPartSpecification or a direct instance of PartOrUsageRelatedSpecification.\n"@en;
        rdfs:label           "PrimaryPartType"@en;
        rdfs:subClassOf      vec:ClosedEnumeration;
        owl:equivalentClass  [ rdf:type   owl:Class;
                               owl:oneOf  ( vec:PrimaryPartType_Antenna vec:PrimaryPartType_Battery vec:PrimaryPartType_BoltMountedFixing vec:PrimaryPartType_BoltTerminal vec:PrimaryPartType_CableDuct vec:PrimaryPartType_CableTie vec:PrimaryPartType_Capacitor vec:PrimaryPartType_CavityAccessory vec:PrimaryPartType_CavityPlug vec:PrimaryPartType_CavitySeal vec:PrimaryPartType_ConnectorHousing vec:PrimaryPartType_ConnectorHousingCap vec:PrimaryPartType_CorrugatedPipe vec:PrimaryPartType_Diode vec:PrimaryPartType_EdgeMountedFixing vec:PrimaryPartType_EEComponent vec:PrimaryPartType_Ferrite vec:PrimaryPartType_Fitting vec:PrimaryPartType_Fixing vec:PrimaryPartType_Fuse vec:PrimaryPartType_Grommet vec:PrimaryPartType_HoleMountedFixing vec:PrimaryPartType_MultiCavityPlug vec:PrimaryPartType_MultiCavitySeal vec:PrimaryPartType_MultiFuse vec:PrimaryPartType_Other vec:PrimaryPartType_OpenWireEnd vec:PrimaryPartType_PartStructure vec:PrimaryPartType_PluggableTerminal vec:PrimaryPartType_PotentialDistributor vec:PrimaryPartType_Relay vec:PrimaryPartType_RingTerminal vec:PrimaryPartType_ShrinkableTube vec:PrimaryPartType_SpliceTerminal vec:PrimaryPartType_Stripe vec:PrimaryPartType_Tape vec:PrimaryPartType_Terminal vec:PrimaryPartType_Tube vec:PrimaryPartType_Wire vec:PrimaryPartType_WireEndAccessory vec:PrimaryPartType_WireProtection )
                             ] .

vec:occurrenceOrUsageInstallationInstruction
        rdf:type            owl:ObjectProperty;
        rdfs:comment        "Room to specify InstallationInstruction(s) for the OccurrenceOrUsage. \n"@en;
        rdfs:domain         vec:OccurrenceOrUsage;
        rdfs:label          "installationInstruction"@en;
        rdfs:range          vec:Instruction;
        rdfs:subPropertyOf  vec:contains .

vec:SiUnitName_DegreeCelsius
        rdf:type         vec:SiUnitName , owl:NamedIndividiual;
        vec:enumLiteral  "DegreeCelsius" .

vec:TextBasedInstruction
        rdf:type         owl:Class;
        rdfs:comment     "A TextBasedInstruction is used to specify human readable instructions in text.\n"@en;
        rdfs:label       "TextBasedInstruction"@en;
        rdfs:subClassOf  vec:Instruction .

vec:connectionEndIsExternalEnd
        rdf:type      owl:DatatypeProperty;
        rdfs:comment  "Specifies if the ConnectionEnd is connected to the internal or the external side of the ComponentPort.\n"@en;
        rdfs:domain   vec:ConnectionEnd;
        rdfs:label    "isExternalEnd"@en;
        rdfs:range    xs:boolean .

vec:conductorSpecificationResistance
        rdf:type            owl:ObjectProperty;
        rdfs:comment        "Specifies the electrical resistance of the conductor. In most cases this is specified as resistance per length (e.g. Ohm per meter).\n"@en;
        rdfs:domain         vec:ConductorSpecification;
        rdfs:label          "resistance"@en;
        rdfs:range          vec:NumericalValue;
        rdfs:subPropertyOf  vec:contains .

vec:GeometryType_Formboard
        rdf:type         vec:GeometryType , owl:NamedIndividiual;
        rdfs:comment     "The Geometry is a model of a Formboard.\n"@en;
        vec:enumLiteral  "Formboard" .

vec:powerConsumptionValue
        rdf:type            owl:ObjectProperty;
        rdfs:comment        "Specifies the power consumption for this type of PowerConsumption .\n"@en;
        rdfs:domain         vec:PowerConsumption;
        rdfs:label          "value"@en;
        rdfs:range          vec:NumericalValue;
        rdfs:subPropertyOf  vec:contains .

vec:matingDetailFirstTerminalReception
        rdf:type      owl:ObjectProperty;
        rdfs:comment  "References the first terminal reception that is mated.\n"@en;
        rdfs:domain   vec:MatingDetail;
        rdfs:label    "firstTerminalReception"@en;
        rdfs:range    vec:TerminalReceptionReference .

vec:ringTerminalSpecificationBoltType
        rdf:type            owl:ObjectProperty;
        rdfs:comment        "Specifies the type of the bolt to which the ring terminal is compatible.\n"@en;
        rdfs:domain         vec:RingTerminalSpecification;
        rdfs:label          "boltType"@en;
        rdfs:range          vec:TerminalBoltType;
        rdfs:subPropertyOf  vec:contains .

<http://www.prostep.org/ontologies/ecad/2024/03/vec#TerminalBoltNominalSize_7%2F8>
        rdf:type         vec:TerminalBoltNominalSize , owl:NamedIndividiual;
        vec:enumLiteral  "7/8" .

vec:approvalPermission
        rdf:type            owl:ObjectProperty;
        rdfs:comment        "Specifies the permission issued with the approval.\n"@en;
        rdfs:domain         vec:Approval;
        rdfs:label          "permission"@en;
        rdfs:range          vec:Permission;
        rdfs:subPropertyOf  vec:contains .

[ rdf:type     owl:AllDisjointClasses;
  owl:members  ( vec:NodeLocation vec:SegmentLocation )
] .

vec:LanguageCode_Ja  rdf:type  vec:LanguageCode , owl:NamedIndividiual;
        vec:enumLiteral  "Ja" .

vec:ExternalMapping  rdf:type  owl:Class;
        rdfs:comment     "An ExternalMapping is used to relate an ExtendableElement in the VEC with an element located in an external data source. The element in the VEC┬áis referenced by the mappedElement , the external element is identified by the attribute externalReference.\n"@en;
        rdfs:label       "ExternalMapping"@en;
        rdfs:subClassOf  vec:ExtendableElement .

vec:slotReferenceUsedSupplementaryParts
        rdf:type      owl:ObjectProperty;
        rdfs:comment  "This is the relationship of the supplementary parts actually used in this SlotReference. This is the actual selection of the potential supplementary parts defined in the corresponding Slot.supplementaryParts association.\n"@en;
        rdfs:domain   vec:SlotReference;
        rdfs:label    "usedSupplementaryParts"@en;
        rdfs:range    vec:OccurrenceOrUsage .

vec:LabelingTechnology_Printed
        rdf:type         vec:LabelingTechnology , owl:NamedIndividiual;
        vec:enumLiteral  "Printed" .

vec:ValueDetermination
        rdf:type             owl:Class;
        rdfs:comment         "Enumeration for the definition of a value determination. (see KBLFRM-316)\n"@en;
        rdfs:label           "ValueDetermination"@en;
        rdfs:subClassOf      vec:ClosedEnumeration;
        owl:equivalentClass  [ rdf:type   owl:Class;
                               owl:oneOf  ( vec:ValueDetermination_Calculated vec:ValueDetermination_Measured vec:ValueDetermination_Estimated )
                             ] .

vec:NetworkPort  rdf:type  owl:Class;
        rdfs:comment     "NetworkPort is the source or the receiver of a of a Net.\n"@en;
        rdfs:label       "NetworkPort"@en;
        rdfs:subClassOf  vec:ConfigurableElement .

vec:generalTechnicalPartSpecificationBoundingBox
        rdf:type            owl:ObjectProperty;
        rdfs:comment        "Defines the bounding box of the part.\n"@en;
        rdfs:domain         vec:GeneralTechnicalPartSpecification;
        rdfs:label          "boundingBox"@en;
        rdfs:range          vec:BoundingBox;
        rdfs:subPropertyOf  vec:contains .

vec:TerminalBoltNominalSize_M1.4
        rdf:type         vec:TerminalBoltNominalSize , owl:NamedIndividiual;
        vec:enumLiteral  "M1.4" .

vec:PinCurrentType_LeakageCurrent
        rdf:type         vec:PinCurrentType , owl:NamedIndividiual;
        rdfs:comment     "Defines the current that leaks at this pin.\n"@en;
        vec:enumLiteral  "leakageCurrent" .

vec:TerminalBoltNominalSize_M36
        rdf:type         vec:TerminalBoltNominalSize , owl:NamedIndividiual;
        vec:enumLiteral  "M36" .

vec:extensionSlotReferenceUsedInserts
        rdf:type      owl:ObjectProperty;
        rdfs:comment  "Defines the inserts used for extension slot in a defined instance. These can be more than one EEComponentRole, because of variance in a 150% specification. "@en;
        rdfs:domain   vec:ExtensionSlotReference;
        rdfs:label    "usedInserts"@en;
        rdfs:range    vec:EEComponentRole .

vec:itemVersionCompanyName
        rdf:type      owl:DatatypeProperty;
        rdfs:comment  "Defines the publishing company of the ItemVersion. The companyName is part of the main identifier of an ItemVersion together with the corresponding number (partNumber or documentNumber) and version (partVersion or documentVersion).\n"@en;
        rdfs:domain   vec:ItemVersion;
        rdfs:label    "companyName"@en;
        rdfs:range    xs:string .

vec:LanguageCode_Ta  rdf:type  vec:LanguageCode , owl:NamedIndividiual;
        vec:enumLiteral  "Ta" .

vec:WireLength  rdf:type  owl:Class;
        rdfs:comment     "Defines the length of a WireElementReference. A WireElementReference can have multiple lengths of different types but must not have more than one length of the same type.\n"@en;
        rdfs:label       "WireLength"@en;
        rdfs:subClassOf  vec:ExtendableElement .

vec:topologySegmentCrossSectionAreaInformation
        rdf:type            owl:ObjectProperty;
        rdfs:comment        "Specifies the different SegmentCrossSectionAreas of the TopologySegment. \n"@en;
        rdfs:domain         vec:TopologySegment;
        rdfs:label          "crossSectionAreaInformation"@en;
        rdfs:range          vec:SegmentCrossSectionArea;
        rdfs:subPropertyOf  vec:contains .

vec:terminalSpecificationWireReception
        rdf:type            owl:ObjectProperty;
        rdfs:comment        "Specifies the WireReceptions of the terminal described by the TerminalSpecification.\n"@en;
        rdfs:domain         vec:TerminalSpecification;
        rdfs:label          "wireReception"@en;
        rdfs:range          vec:WireReception;
        rdfs:subPropertyOf  vec:contains .

vec:PowerConsumptionType_Minimum
        rdf:type         vec:PowerConsumptionType , owl:NamedIndividiual;
        vec:enumLiteral  "Minimum" .

vec:tapeRoleGradient  rdf:type  owl:ObjectProperty;
        rdfs:comment        "Specifies the gradient of the taping.\n"@en;
        rdfs:domain         vec:TapeRole;
        rdfs:label          "gradient"@en;
        rdfs:range          vec:ValueWithUnit;
        rdfs:subPropertyOf  vec:contains .

vec:ConnectionEndGender_Female
        rdf:type         vec:ConnectionEndGender , owl:NamedIndividiual;
        vec:enumLiteral  "Female" .

vec:PrimaryPartType_CableDuct
        rdf:type         vec:PrimaryPartType , owl:NamedIndividiual;
        vec:enumLiteral  "CableDuct" .

vec:FunctionalRequirementType_Function
        rdf:type         vec:FunctionalRequirementType , owl:NamedIndividiual;
        rdfs:comment     "Requirements from a functional point of view (e.g. standby current).\n┬á\n"@en;
        vec:enumLiteral  "Function" .

vec:ImperialUnitName  rdf:type  owl:Class;
        rdfs:comment         "Enumeration for the definition of imperial unit names.\n"@en;
        rdfs:label           "ImperialUnitName"@en;
        rdfs:subClassOf      vec:ClosedEnumeration;
        owl:equivalentClass  [ rdf:type   owl:Class;
                               owl:oneOf  ( vec:ImperialUnitName_Thou vec:ImperialUnitName_Inch vec:ImperialUnitName_Foot vec:ImperialUnitName_Yard vec:ImperialUnitName_Chain vec:ImperialUnitName_Furlong vec:ImperialUnitName_Mile vec:ImperialUnitName_League vec:ImperialUnitName_FluidOunce vec:ImperialUnitName_Gill vec:ImperialUnitName_Pint vec:ImperialUnitName_Quart vec:ImperialUnitName_Gallon vec:ImperialUnitName_Grain vec:ImperialUnitName_Drachm vec:ImperialUnitName_Ounce vec:ImperialUnitName_Pound vec:ImperialUnitName_Stone vec:ImperialUnitName_Quarter vec:ImperialUnitName_HundredWeight vec:ImperialUnitName_Ton vec:ImperialUnitName_Perch vec:ImperialUnitName_Rood vec:ImperialUnitName_Acre )
                             ] .

vec:connectionNodeViewItemGridSquare
        rdf:type      owl:DatatypeProperty;
        rdfs:comment  "Specifies the grid square in which the ComponentNodeViewIt em is placed (e.g. E/40).\n"@en;
        rdfs:domain   vec:ConnectionNodeViewItem;
        rdfs:label    "gridSquare"@en;
        rdfs:range    xs:string .

vec:multiFuseSpecificationIMaxTotal
        rdf:type            owl:ObjectProperty;
        rdfs:comment        "Specifies the maximum electric current tolerated by the multifuse in total.\n"@en;
        rdfs:domain         vec:MultiFuseSpecification;
        rdfs:label          "iMaxTotal"@en;
        rdfs:range          vec:NumericalValue;
        rdfs:subPropertyOf  vec:contains .

vec:BuildingBlockPositioning2D
        rdf:type         owl:Class;
        rdfs:comment     "Defines the position of a BuildingBlock2D on a HarnessDrawing.\n"@en;
        rdfs:label       "BuildingBlockPositioning2D"@en;
        rdfs:subClassOf  vec:ConfigurableElement .

vec:WireEndAccessorySpecification
        rdf:type         owl:Class;
        rdfs:comment     " WireEndAccessorySpecifications are describing parts that are used for a treatment of a wire end before the actual terminal is attached to the WireEnd (e.g. a ferrule).\nThe actual specification is done by the referenced WireReceptionSpecification since a WireEndAccessory is basically just a single WireReception .\n"@en;
        rdfs:label       "WireEndAccessorySpecification"@en;
        rdfs:subClassOf  vec:PartOrUsageRelatedSpecification .

vec:LanguageCode_He  rdf:type  vec:LanguageCode , owl:NamedIndividiual;
        vec:enumLiteral  "He" .

vec:VariantCodeType  rdf:type  owl:Class;
        rdfs:comment     "OpenEnumeration for the available types of the variant codes.\n"@en;
        rdfs:label       "VariantCodeType"@en;
        rdfs:subClassOf  vec:OpenEnumeration .

vec:Path  rdf:type       owl:Class;
        rdfs:comment     "Describes a path in the topology. A Path is a continuous way through a topology without interruptions, defined by an ordered list of TopologySegments .\n"@en;
        rdfs:label       "Path"@en;
        rdfs:subClassOf  vec:ExtendableElement .

vec:terminalReceptionSpecificationTerminalType
        rdf:type            owl:ObjectProperty;
        rdfs:comment        "Specifies the terminal type that is associated with the terminal reception.\n"@en;
        rdfs:domain         vec:TerminalReceptionSpecification;
        rdfs:label          "terminalType"@en;
        rdfs:range          vec:TerminalType;
        rdfs:subPropertyOf  vec:contains .

vec:variantStructureNodeAbbreviation
        rdf:type            owl:ObjectProperty;
        rdfs:comment        "Room for a human readable short name, title etc. of the VariantStructureNode .\n"@en;
        rdfs:domain         vec:VariantStructureNode;
        rdfs:label          "abbreviation"@en;
        rdfs:range          vec:LocalizedString;
        rdfs:subPropertyOf  vec:contains .

vec:LabelingTechnology
        rdf:type         owl:Class;
        rdfs:comment     "OpenEnumeration of standard labeling technologies."@en;
        rdfs:label       "LabelingTechnology"@en;
        rdfs:subClassOf  vec:OpenEnumeration .

vec:valueWithUnitUnitComponent
        rdf:type      owl:ObjectProperty;
        rdfs:comment  "References the unit of the value. \n"@en;
        rdfs:domain   vec:ValueWithUnit;
        rdfs:label    "unitComponent"@en;
        rdfs:range    vec:Unit .

vec:ConductorStructure_Asymmetric
        rdf:type         vec:ConductorStructure , owl:NamedIndividiual;
        rdfs:comment     "Asymmetric conductor structure in accordance with ISO 6722-1 (Type B)\n"@en;
        vec:enumLiteral  "Asymmetric" .

vec:LanguageCode_Bg  rdf:type  vec:LanguageCode , owl:NamedIndividiual;
        vec:enumLiteral  "Bg" .

vec:MeasurementPoint  rdf:type  owl:Class;
        rdfs:comment     "Defines a reference point on a component that can be used to apply a Dimension. This is normally a significant point of the component e.g. an edge, a hole, a bolt or something similar.\n"@en;
        rdfs:label       "MeasurementPoint"@en;
        rdfs:subClassOf  vec:ExtendableElement .

vec:FuseType_Type_A1  rdf:type  vec:FuseType , owl:NamedIndividiual;
        rdfs:comment     "also known as: jcase\n"@en;
        vec:enumLiteral  "Type_A1" .

vec:FlatCoreSpecification
        rdf:type         owl:Class;
        rdfs:comment     "Defines the properties of a flat (rectangular)┬áconductor which are specific for them.\n"@en;
        rdfs:label       "FlatCoreSpecification"@en;
        rdfs:subClassOf  vec:ConductorSpecification .

vec:MeasurePointPosition
        rdf:type         owl:Class;
        rdfs:comment     "Defines the position of a MeasurementPoint within the coordinate system of the component. MeasurementPoint onto which dimension can be defined .\n"@en;
        rdfs:label       "MeasurePointPosition"@en;
        rdfs:subClassOf  vec:LocalPosition .

vec:fixingSpecificationOffset
        rdf:type            owl:ObjectProperty;
        rdfs:domain         vec:FixingSpecification;
        rdfs:label          "offset"@en;
        rdfs:range          vec:NumericalValue;
        rdfs:subPropertyOf  vec:contains .

vec:LabelingTechnology_Codeable
        rdf:type         vec:LabelingTechnology , owl:NamedIndividiual;
        rdfs:comment     "In case of labels that can be coded at a later stage┬á(e.g. RFID)."@en;
        vec:enumLiteral  "Codeable" .

vec:localGeometrySpecificationBoundingBoxPositioning
        rdf:type            owl:ObjectProperty;
        rdfs:comment        "The transformation that defines the positioning of the bounding box in coordinate system of the component.\n"@en;
        rdfs:domain         vec:LocalGeometrySpecification;
        rdfs:label          "boundingBoxPositioning"@en;
        rdfs:range          vec:Transformation3D;
        rdfs:subPropertyOf  vec:contains .

vec:UsageNodeType_Fuse
        rdf:type         vec:UsageNodeType , owl:NamedIndividiual;
        vec:enumLiteral  "Fuse" .

vec:topologySpecificationTopologyNode
        rdf:type            owl:ObjectProperty;
        rdfs:comment        "Specifies the TopologyNodes defined by the TopologySpecification.\n"@en;
        rdfs:domain         vec:TopologySpecification;
        rdfs:label          "topologyNode"@en;
        rdfs:range          vec:TopologyNode;
        rdfs:subPropertyOf  vec:contains .

vec:colorDescription  rdf:type  owl:ObjectProperty;
        rdfs:comment        "On optional human readable description of the color (e.g. the name).\n"@en;
        rdfs:domain         vec:Color;
        rdfs:label          "description"@en;
        rdfs:range          vec:LocalizedString;
        rdfs:subPropertyOf  vec:contains .

vec:FuseType_Type_SF30
        rdf:type         vec:FuseType , owl:NamedIndividiual;
        rdfs:comment     "also known as: midi\n"@en;
        vec:enumLiteral  "Type_SF30" .

vec:topologyBendingRestrictionSpecificationTopologyBendingRestriction
        rdf:type            owl:ObjectProperty;
        rdfs:domain         vec:TopologyBendingRestrictionSpecification;
        rdfs:label          "topologyBendingRestriction"@en;
        rdfs:range          vec:TopologyBendingRestriction;
        rdfs:subPropertyOf  vec:contains .

vec:WindingFirmness_Tight
        rdf:type         vec:WindingFirmness , owl:NamedIndividiual;
        rdfs:comment     "The taping is applied tight.\n"@en;
        vec:enumLiteral  "Tight" .

vec:generalTechnicalPartSpecificationMaterialInformation
        rdf:type            owl:ObjectProperty;
        rdfs:comment        "Specifies the material of a part.\n"@en;
        rdfs:domain         vec:GeneralTechnicalPartSpecification;
        rdfs:label          "materialInformation"@en;
        rdfs:range          vec:Material;
        rdfs:subPropertyOf  vec:contains .

vec:UsageConstraintType_Deny
        rdf:type         vec:UsageConstraintType , owl:NamedIndividiual;
        vec:enumLiteral  "Deny" .

vec:HoleMountedFixingHoleShape_Oval
        rdf:type         vec:HoleMountedFixingHoleShape , owl:NamedIndividiual;
        vec:enumLiteral  "Oval" .

vec:parent  rdf:type   owl:ObjectProperty;
        rdfs:comment   "The inverse of 'contains'."@en;
        rdfs:label     "parent"@en;
        owl:inverseOf  vec:contains .

vec:PowerConsumptionType
        rdf:type         owl:Class;
        rdfs:comment     "OpenEnumeration for predefined PowerConsumptionTypes. "@en;
        rdfs:label       "PowerConsumptionType"@en;
        rdfs:subClassOf  vec:OpenEnumeration .

vec:abstractSlotReferenceIdentification
        rdf:type      owl:DatatypeProperty;
        rdfs:comment  "Specifies a unique identification of the SlotReference. The identification is guaranteed to be unique within the ConnectorHousingRole. The cavity & slot number is defined by the associated cavity and slot.\n"@en;
        rdfs:domain   vec:AbstractSlotReference;
        rdfs:label    "identification"@en;
        rdfs:range    xs:string .

vec:matingPointIdentification
        rdf:type      owl:DatatypeProperty;
        rdfs:comment  "Specifies a unique identification of the MatingPoint . The identification is guaranteed to be unique within a CouplingPoint .\n"@en;
        rdfs:domain   vec:MatingPoint;
        rdfs:label    "identification"@en;
        rdfs:range    xs:string .

vec:FuseType_Type_SF51
        rdf:type         vec:FuseType , owl:NamedIndividiual;
        rdfs:comment     "also known as: mega\n"@en;
        vec:enumLiteral  "Type_SF51" .

vec:slotSpecificationSlotLayout
        rdf:type            owl:ObjectProperty;
        rdfs:comment        "References the layout associated with this slot.\n"@en;
        rdfs:domain         vec:SlotSpecification;
        rdfs:label          "slotLayout"@en;
        rdfs:range          vec:SlotLayout;
        rdfs:subPropertyOf  vec:contains .

vec:buildingBlockPositioning2DReferenced2DBuildingBlock
        rdf:type      owl:ObjectProperty;
        rdfs:comment  "References the building block which is placed on the harness drawing. \n"@en;
        rdfs:domain   vec:BuildingBlockPositioning2D;
        rdfs:label    "referenced2DBuildingBlock"@en;
        rdfs:range    vec:BuildingBlockSpecification2D .

vec:connectorHousingRoleSealState
        rdf:type            owl:ObjectProperty;
        rdfs:comment        "Specifies if this instance of a connector housing should be sealed (waterproof).\n"@en;
        rdfs:domain         vec:ConnectorHousingRole;
        rdfs:label          "sealState"@en;
        rdfs:range          vec:SealState;
        rdfs:subPropertyOf  vec:contains .

vec:GeometryType  rdf:type  owl:Class;
        rdfs:comment     "Enumeration for the definition of the GeometryType.\n"@en;
        rdfs:label       "GeometryType"@en;
        rdfs:subClassOf  vec:OpenEnumeration .

vec:internalTerminalConnectionTerminalReception
        rdf:type      owl:ObjectProperty;
        rdfs:comment  "References the TerminalReceptions that participate in the InternalTerminalConnection.\n"@en;
        rdfs:domain   vec:InternalTerminalConnection;
        rdfs:label    "terminalReception"@en;
        rdfs:range    vec:TerminalReception .

vec:itemEquivalenceItem
        rdf:type      owl:ObjectProperty;
        rdfs:comment  "References all ItemVersion that are considered to be equivalent by the ItemEquivalence. A single ItemEquivalence shall only reference ItemVersions of the same class (either DocumentVersions or PartVersions ).\n"@en;
        rdfs:domain   vec:ItemEquivalence;
        rdfs:label    "item"@en;
        rdfs:range    vec:ItemVersion .

vec:NetworkNodeSubType_Lamp
        rdf:type         vec:NetworkNodeSubType , owl:NamedIndividiual;
        vec:enumLiteral  "Lamp" .

vec:LanguageCode_Fi  rdf:type  vec:LanguageCode , owl:NamedIndividiual;
        vec:enumLiteral  "Fi" .

vec:mappingSpecificationMapping
        rdf:type            owl:ObjectProperty;
        rdfs:comment        ""@en;
        rdfs:domain         vec:MappingSpecification;
        rdfs:label          "mapping"@en;
        rdfs:range          vec:Mapping;
        rdfs:subPropertyOf  vec:contains .

vec:applicationConstraintSpecificationApplicationConstraint
        rdf:type            owl:ObjectProperty;
        rdfs:comment        "Specifies the UsageConstraints that apply to the PartVersion or PartUsages described by the UsageConstraintSpecification. \n"@en;
        rdfs:domain         vec:ApplicationConstraintSpecification;
        rdfs:label          "applicationConstraint"@en;
        rdfs:range          vec:ApplicationConstraint;
        rdfs:subPropertyOf  vec:contains .

vec:cartesianVector3DZ
        rdf:type      owl:DatatypeProperty;
        rdfs:comment  "Specifies the z-coordinate in 3D space.\n"@en;
        rdfs:domain   vec:CartesianVector3D;
        rdfs:label    "z"@en;
        rdfs:range    xs:double .

vec:PrimaryPartType_CavityPlug
        rdf:type         vec:PrimaryPartType , owl:NamedIndividiual;
        vec:enumLiteral  "CavityPlug" .

vec:HousingComponentType
        rdf:type         owl:Class;
        rdfs:comment     "Defines the valid HousingComponentTypes. The values in this Enumeration are matching the relevant PrimaryPartTypes. For a description of the values see PrimaryPartType.\n"@en;
        rdfs:label       "HousingComponentType"@en;
        rdfs:subClassOf  vec:OpenEnumeration .

vec:Signal  rdf:type     owl:Class;
        rdfs:comment     "Specifies a signal.\n"@en;
        rdfs:label       "Signal"@en;
        rdfs:subClassOf  vec:ExtendableElement .

<http://www.prostep.org/ontologies/ecad/2024/03/vec#TerminalBoltNominalSize_7%2F16>
        rdf:type         vec:TerminalBoltNominalSize , owl:NamedIndividiual;
        vec:enumLiteral  "7/16" .

vec:variantGroupAliasId
        rdf:type            owl:ObjectProperty;
        rdfs:comment        "Room to specify additional identifiers for the VariantGroup.\n"@en;
        rdfs:domain         vec:VariantGroup;
        rdfs:label          "aliasId"@en;
        rdfs:range          vec:AliasIdentification;
        rdfs:subPropertyOf  vec:contains .

vec:terminalReceptionSpecificationCavityDesign
        rdf:type        owl:DatatypeProperty;
        rdfs:comment    ""@en , "Deprecated (since Version 1.1.4): This attribute has been marked as deprecated, as it has been replaced by the more meaningful mechanism with TerminalTypes.\n"@en;
        rdfs:domain     vec:TerminalReceptionSpecification;
        rdfs:label      "cavityDesign"@en;
        rdfs:range      xs:string;
        owl:deprecated  true .

vec:configurableElementConfigInfo
        rdf:type        owl:ObjectProperty;
        rdfs:comment    ""@en , " Deprecated since VEC┬áV2.0.0. Use ConfigurationConstraints instead.\nReferences the configuration information that applies to the ConfigurableElement.\n"@en;
        rdfs:domain     vec:ConfigurableElement;
        rdfs:label      "configInfo"@en;
        rdfs:range      vec:VariantConfiguration;
        owl:deprecated  true .

vec:pinComponentReferenceIdentification
        rdf:type      owl:DatatypeProperty;
        rdfs:comment  "Specifies a unique identification of the PinComponentReference. The identification is guaranteed to be unique within the HousingComponentReference.\n"@en;
        rdfs:domain   vec:PinComponentReference;
        rdfs:label    "identification"@en;
        rdfs:range    xs:string .

vec:IECPrefix_Kibi  rdf:type  vec:IECPrefix , owl:NamedIndividiual;
        vec:enumLiteral  "Kibi" .

vec:topologyNodeMatchingPointId
        rdf:type      owl:DatatypeProperty;
        rdfs:comment  "Specifies an identifier that can be used for matching TopologyNodes that belong to different TopologySpecifications and are actually representing the same node. Example: There are two TopologySpecif ications, each specifying the topology of a certain zone of the car. If the zones are adjacent, it is possible that there are TopologyNodes in both zones where the two topologies are connected /┬áhave contact. These \"connection-nodes\" would then define the same matchingPointId .\n"@en;
        rdfs:domain   vec:TopologyNode;
        rdfs:label    "matchingPointId"@en;
        rdfs:range    xs:string .

vec:partWithSubComponentsRoleSubComponent
        rdf:type      owl:ObjectProperty;
        rdfs:comment  "References the subcomponents that belong to this instance of a PartWithSubComponents.\n"@en;
        rdfs:domain   vec:PartWithSubComponentsRole;
        rdfs:label    "subComponent"@en;
        rdfs:range    vec:OccurrenceOrUsage .

vec:NominalVoltage_48V
        rdf:type         vec:NominalVoltage , owl:NamedIndividiual;
        vec:enumLiteral  "48V" .

vec:SignalSubType_BTLE
        rdf:type         vec:SignalSubType , owl:NamedIndividiual;
        rdfs:comment     "Bluetooth Low Energy\n"@en;
        vec:enumLiteral  "BTLE" .

vec:SpliceTerminalSpecification
        rdf:type         owl:Class;
        rdfs:comment     "Specification for the definition of splice terminals.\n"@en;
        rdfs:label       "SpliceTerminalSpecification"@en;
        rdfs:subClassOf  vec:TerminalSpecification .

vec:CableLeadThroughType_ShrinkingTubeWithSealingGlue
        rdf:type         vec:CableLeadThroughType , owl:NamedIndividiual;
        vec:enumLiteral  "ShrinkingTubeWithSealingGlue" .

vec:VariantGroupType_OptionalFamily
        rdf:type         vec:VariantGroupType , owl:NamedIndividiual;
        rdfs:comment     "A group with the type \"OptionalFamily\" defines a set of variant codes that are mutually exclusive, and a valid configuration can, but does not have to contain one variant code from the group.\n"@en;
        vec:enumLiteral  "OptionalFamily" .

vec:connectorHousingSpecificationSegmentConnectionPoint
        rdf:type            owl:ObjectProperty;
        rdfs:comment        "Specifies the SegmentConnectionPoints the connector housing.\n"@en;
        rdfs:domain         vec:ConnectorHousingSpecification;
        rdfs:label          "segmentConnectionPoint"@en;
        rdfs:range          vec:SegmentConnectionPoint;
        rdfs:subPropertyOf  vec:contains .

vec:conductorCurrentInformationMaxCurrent
        rdf:type            owl:ObjectProperty;
        rdfs:comment        "The maximum current value.\n"@en;
        rdfs:domain         vec:ConductorCurrentInformation;
        rdfs:label          "maxCurrent"@en;
        rdfs:range          vec:NumericalValue;
        rdfs:subPropertyOf  vec:contains .

vec:batterySpecificationICool
        rdf:type            owl:ObjectProperty;
        rdfs:comment        "Specifies the battery's current in cool state.\n"@en;
        rdfs:domain         vec:BatterySpecification;
        rdfs:label          "iCool"@en;
        rdfs:range          vec:NumericalValue;
        rdfs:subPropertyOf  vec:contains .

vec:LanguageCode_Xh  rdf:type  vec:LanguageCode , owl:NamedIndividiual;
        vec:enumLiteral  "Xh" .

[ rdf:type     owl:AllDisjointClasses;
  owl:members  ( vec:DocumentRelatedAssignmentGroup vec:FunctionalAssignmentGroup )
] .

vec:VecVersion_1.1.1  rdf:type  vec:VecVersion , owl:NamedIndividiual;
        vec:enumLiteral  "1.1.1" .

vec:partStructureSpecificationContent
        rdf:type            owl:ObjectProperty;
        rdfs:comment        "Specifies the type of content of the bill of material (e.g. module, harness complete set)\n"@en;
        rdfs:domain         vec:PartStructureSpecification;
        rdfs:label          "content"@en;
        rdfs:range          vec:PartStructureContentType;
        rdfs:subPropertyOf  vec:contains .

vec:sheetOrChapterDescription
        rdf:type            owl:ObjectProperty;
        rdfs:comment        "Room for additional, human readable information about the SheetOrChapter.\n"@en;
        rdfs:domain         vec:SheetOrChapter;
        rdfs:label          "description"@en;
        rdfs:range          vec:AbstractLocalizedString;
        rdfs:subPropertyOf  vec:contains .

vec:PinComponentReference
        rdf:type         owl:Class;
        rdfs:comment     "A PinComponentReference represents the usage of a PinComponent in the context of a PartUsage or PartOccurrence. (KBLFRM-401)\n"@en;
        rdfs:label       "PinComponentReference"@en;
        rdfs:subClassOf  vec:ConfigurableElement .

vec:connectionViewSpecificationCartesianPoint
        rdf:type            owl:ObjectProperty;
        rdfs:comment        "Specifies all the CartesianPoint2Ds that are used within the ConnectionViewSpecification . "@en;
        rdfs:domain         vec:ConnectionViewSpecification;
        rdfs:label          "cartesianPoint"@en;
        rdfs:range          vec:CartesianPoint2D;
        rdfs:subPropertyOf  vec:contains .

vec:LanguageCode_Zi  rdf:type  vec:LanguageCode , owl:NamedIndividiual;
        vec:enumLiteral  "Zi" .

vec:WireProtectionSpecification
        rdf:type         owl:Class;
        rdfs:comment     "Specification for the description of wire protections.\n"@en;
        rdfs:label       "WireProtectionSpecification"@en;
        rdfs:subClassOf  vec:PartOrUsageRelatedSpecification .

vec:nodeMappingInnerNode
        rdf:type     owl:ObjectProperty;
        rdfs:domain  vec:NodeMapping;
        rdfs:label   "innerNode"@en;
        rdfs:range   vec:TopologyNode .

vec:insulationSpecificationLabelingTechnology
        rdf:type            owl:ObjectProperty;
        rdfs:comment        "Specifies used labeling technology if the label is already defined in this specification."@en;
        rdfs:domain         vec:InsulationSpecification;
        rdfs:label          "labelingTechnology"@en;
        rdfs:range          vec:LabelingTechnology;
        rdfs:subPropertyOf  vec:contains .

<http://www.prostep.org/ontologies/ecad/2024/03/vec#TerminalBoltNominalSize_3%2F8>
        rdf:type         vec:TerminalBoltNominalSize , owl:NamedIndividiual;
        vec:enumLiteral  "3/8" .

vec:segmentConnectionPointHCIdentification
        rdf:type     owl:DatatypeProperty;
        rdfs:domain  vec:SegmentConnectionPointHC;
        rdfs:label   "identification"@en;
        rdfs:range   xs:string .

vec:SpliceType_InlineSplice
        rdf:type         vec:SpliceType , owl:NamedIndividiual;
        rdfs:comment     "An inlineSplice is a splice where wires from both sides are connected.\n"@en;
        vec:enumLiteral  "InlineSplice" .

vec:WireReceptionType_FrictionWelding
        rdf:type         vec:WireReceptionType , owl:NamedIndividiual;
        vec:enumLiteral  "FrictionWelding" .

vec:PinApplianceType_LongTerm
        rdf:type         vec:PinApplianceType , owl:NamedIndividiual;
        vec:enumLiteral  "longTerm" .

vec:LanguageCode_Tk  rdf:type  vec:LanguageCode , owl:NamedIndividiual;
        vec:enumLiteral  "Tk" .

vec:slotReferenceCavityReference
        rdf:type            owl:ObjectProperty;
        rdfs:comment        "Specifies the CavityReferences used in the SlotReference.\n"@en;
        rdfs:domain         vec:SlotReference;
        rdfs:label          "cavityReference"@en;
        rdfs:range          vec:CavityReference;
        rdfs:subPropertyOf  vec:contains .

vec:pinComponentDescription
        rdf:type            owl:ObjectProperty;
        rdfs:comment        "Specifies additional, human readable information about the PinComponent .\n"@en;
        rdfs:domain         vec:PinComponent;
        rdfs:label          "description"@en;
        rdfs:range          vec:AbstractLocalizedString;
        rdfs:subPropertyOf  vec:contains .

vec:ColorReferenceSystem
        rdf:type         owl:Class;
        rdfs:comment     "Defines the literals that shall be used for specific color reference systems.\n"@en;
        rdfs:label       "ColorReferenceSystem"@en;
        rdfs:subClassOf  vec:OpenEnumeration .

vec:SiUnitName_Volt  rdf:type  vec:SiUnitName , owl:NamedIndividiual;
        vec:enumLiteral  "Volt" .

vec:SlotSealingType_SingleSealing
        rdf:type         vec:SlotSealingType , owl:NamedIndividiual;
        rdfs:comment     "The Slot is sealed with a single Seal per Cavity e.g. a CavitySeal or a CavityPlug.\n"@en;
        vec:enumLiteral  "SingleSealing" .

vec:contactPointMountedTerminal
        rdf:type      owl:ObjectProperty;
        rdfs:comment  "References the terminal that is used for contacting defined by the ContactPoint. \n"@en;
        rdfs:domain   vec:ContactPoint;
        rdfs:label    "mountedTerminal"@en;
        rdfs:range    vec:TerminalRole .

vec:BoltMountedFixingBoltType_Regular
        rdf:type         vec:BoltMountedFixingBoltType , owl:NamedIndividiual;
        rdfs:comment     "A bolt with some kind of corrugation for fixing to lock on."@en;
        vec:enumLiteral  "Regular" .

vec:PowerConsumptionType_Maximum
        rdf:type         vec:PowerConsumptionType , owl:NamedIndividiual;
        vec:enumLiteral  "Maximum" .

vec:ExtensionSlot  rdf:type  owl:Class;
        rdfs:comment     "An ExtensionSlot defines a slot within an EE-Component where other EE-Components can be plugged into (modular extension). This is necessary for example for modular power distributions.\n"@en;
        rdfs:label       "ExtensionSlot"@en;
        rdfs:subClassOf  vec:ConfigurableElement .

<http://www.prostep.org/ontologies/ecad/2024/03/vec#TerminalBoltNominalSize_%231>
        rdf:type         vec:TerminalBoltNominalSize , owl:NamedIndividiual;
        vec:enumLiteral  "#1" .

vec:DocumentType_GeometryModel
        rdf:type         vec:DocumentType , owl:NamedIndividiual;
        rdfs:comment     "Documents of this type represent a geometry model (3D), which is normally an external file (e.g. a JT┬áFile or some native file of a 3D modelling tool). Typical use cases are for example the models of components (e.g. connectors) used in a 3D model or the 3D visualization of a Harness.\n"@en;
        vec:enumLiteral  "GeometryModel" .

[ rdf:type     owl:AllDisjointClasses;
  owl:members  ( vec:NumericalValueProperty vec:SimpleValueProperty vec:ValueRangeProperty vec:LocalizedStringProperty vec:BooleanValueProperty vec:DateValueProperty vec:DoubleValueProperty vec:IntegerValueProperty vec:ComplexProperty )
] .

vec:occurrenceOrUsageAbbreviation
        rdf:type            owl:ObjectProperty;
        rdfs:comment        "Specifies an abbreviation of the OccurrenceOrUsage . Normally this a human readable short name.\n"@en;
        rdfs:domain         vec:OccurrenceOrUsage;
        rdfs:label          "abbreviation"@en;
        rdfs:range          vec:LocalizedString;
        rdfs:subPropertyOf  vec:contains .

vec:ValueDetermination_Estimated
        rdf:type         vec:ValueDetermination , owl:NamedIndividiual;
        rdfs:comment     "The value is estimated by a person.\n"@en;
        vec:enumLiteral  "Estimated" .

vec:TerminalBoltNominalSize_M3.5
        rdf:type         vec:TerminalBoltNominalSize , owl:NamedIndividiual;
        vec:enumLiteral  "M3.5" .

vec:netNetType  rdf:type  owl:ObjectProperty;
        rdfs:domain  vec:Net;
        rdfs:label   "netType"@en;
        rdfs:range   vec:NetType .

vec:terminalSpecificationSealingType
        rdf:type            owl:ObjectProperty;
        rdfs:comment        "Defines the SealingType of the Terminal. This type always refers to the sealing of the terminal itself. However, even a terminal which is not sealable can be used in sealed locations with additional measures (e.g. on the slot).\n"@en;
        rdfs:domain         vec:TerminalSpecification;
        rdfs:label          "sealingType"@en;
        rdfs:range          vec:TerminalSealingType;
        rdfs:subPropertyOf  vec:contains .

vec:fillerSpecificationDiameter
        rdf:type            owl:ObjectProperty;
        rdfs:comment        "Specifies the diameter of the filler.\n"@en;
        rdfs:domain         vec:FillerSpecification;
        rdfs:label          "diameter"@en;
        rdfs:range          vec:NumericalValue;
        rdfs:subPropertyOf  vec:contains .

vec:terminalSpecificationVoltageRange
        rdf:type            owl:ObjectProperty;
        rdfs:comment        "Specifies the allowed voltage range for the connector housing.\n"@en;
        rdfs:domain         vec:TerminalSpecification;
        rdfs:label          "voltageRange"@en;
        rdfs:range          vec:ValueRange;
        rdfs:subPropertyOf  vec:contains .

vec:buildingBlockPositioning2DCenterPoint
        rdf:type            owl:ObjectProperty;
        rdfs:comment        "Specifies the center point of the BuildingBlock in the coordinate system of the harness drawing. \n"@en;
        rdfs:domain         vec:BuildingBlockPositioning2D;
        rdfs:label          "centerPoint"@en;
        rdfs:range          vec:CartesianPoint2D;
        rdfs:subPropertyOf  vec:contains .

vec:PinVoltageType_TypicalVoltage
        rdf:type         vec:PinVoltageType , owl:NamedIndividiual;
        vec:enumLiteral  "typicalVoltage" .

vec:cavityCouplingSecondCavity
        rdf:type     owl:ObjectProperty;
        rdfs:domain  vec:CavityCoupling;
        rdfs:label   "secondCavity"@en;
        rdfs:range   vec:CavityReference .

vec:TopologySegment  rdf:type  owl:Class;
        rdfs:comment     "A TopologySegment is a distance in the Topology where no intermediate electrical contacts appear. If a Topology contains routed wires, then the wire at the beginning of a TopologySegment must be the same as in the ending. TopologySegments are a logical construct to describe the physical representation of a wiring harness topology. Therefore, a TopologySegment is only valid if it has a physical manifestation. TopologySegments with a length of 0 or less do not have a physical manifestation and are therefore not valid.\nAdditionally, the usage of TopologySegments with a length of 0 create problems in the overall process. For example, the synchronization of 3D /┬á2D┬ásystems becomes harder or even impossible and the handling of wire protections on those TopologySegment is also unclear.\n"@en;
        rdfs:label       "TopologySegment"@en;
        rdfs:subClassOf  vec:ConfigurableElement .

vec:matingPointConnection
        rdf:type      owl:ObjectProperty;
        rdfs:comment  "References the Connection that is realized by this MatingPoint . For example, when a connection is realized by directly plugging or screwing two E/E components together.\n"@en;
        rdfs:domain   vec:MatingPoint;
        rdfs:label    "connection"@en;
        rdfs:range    vec:Connection .

vec:BaselineSpecification
        rdf:type         owl:Class;
        rdfs:comment     "A BaselineSpecification defines a set of ItemVersion s ( Document- and PartVersions ) that relate to each other in a certain way e.g. all parts and documents in their specific versions that contributed to a specific manufactured result.\nBaselines are a standard mechanism to support change, release and configuration management.\n"@en;
        rdfs:label       "BaselineSpecification"@en;
        rdfs:subClassOf  vec:Specification .

vec:matingDetailSecondTerminalReception
        rdf:type      owl:ObjectProperty;
        rdfs:comment  "References the second terminal reception that is mated.\n"@en;
        rdfs:domain   vec:MatingDetail;
        rdfs:label    "secondTerminalReception"@en;
        rdfs:range    vec:TerminalReceptionReference .

vec:wireLengthLengthValue
        rdf:type            owl:ObjectProperty;
        rdfs:comment        "The length value for the type.\n"@en;
        rdfs:domain         vec:WireLength;
        rdfs:label          "lengthValue"@en;
        rdfs:range          vec:NumericalValue;
        rdfs:subPropertyOf  vec:contains .

vec:LanguageCode_Ro  rdf:type  vec:LanguageCode , owl:NamedIndividiual;
        vec:enumLiteral  "Ro" .

vec:WireGroupType  rdf:type  owl:Class;
        rdfs:comment     "OpenEnumeration for the types of wire groups.\n"@en;
        rdfs:label       "WireGroupType"@en;
        rdfs:subClassOf  vec:OpenEnumeration .

vec:IECPrefix  rdf:type      owl:Class;
        rdfs:comment         "Enumeration for the definition of IEC unit prefixes.\n"@en;
        rdfs:label           "IECPrefix"@en;
        rdfs:subClassOf      vec:ClosedEnumeration;
        owl:equivalentClass  [ rdf:type   owl:Class;
                               owl:oneOf  ( vec:IECPrefix_Yobi vec:IECPrefix_Zebi vec:IECPrefix_Exbi vec:IECPrefix_Pebi vec:IECPrefix_Tebi vec:IECPrefix_Gibi vec:IECPrefix_Mebi vec:IECPrefix_Kibi )
                             ] .

vec:AliasIdentificationType_UUID
        rdf:type         vec:AliasIdentificationType , owl:NamedIndividiual;
        rdfs:comment     "Defines that this AliasIdentification represents a \"Universally Unique Identifier\". Although a UUID┬áis technical definition of a 128-Bit number, the primary relevance of this type is not its technical representation, but it's other properties. An┬áAliasIdentification with the type \"UUID\" of an element is its unique identifier, that is constant over time, never changes and is never reused for other elements. Such an AliasIdentification can be used to trace elements through different systems, companies and processes.\n"@en;
        vec:enumLiteral  "UUID" .

vec:UsageNodeType_Splice
        rdf:type         vec:UsageNodeType , owl:NamedIndividiual;
        vec:enumLiteral  "Splice" .

vec:LengthClassification_Designed
        rdf:type         vec:LengthClassification , owl:NamedIndividiual;
        rdfs:comment     "A designed length means that the value is derived automatically in a CAD Tool (e.g. from a 3D Geometry).\n"@en;
        vec:enumLiteral  "Designed" .

vec:topologyZoneIdentification
        rdf:type      owl:DatatypeProperty;
        rdfs:comment  "Specifies a unique identification of the Zone (normally the name). The identification is guaranteed to be unique within the TopologySpecification. For all VEC-documents a Zone-instance can be trusted to be the same if the TopologySpecification-instance is the same (see TopologySpecification) and the identification of the Zone is the same.\n"@en;
        rdfs:domain   vec:TopologyZone;
        rdfs:label    "identification"@en;
        rdfs:range    xs:string .

vec:powerConsumptionType
        rdf:type            owl:ObjectProperty;
        rdfs:comment        "The type of a PowerConsumption . This should be an enumeration of values defined in a conformance class.\n"@en;
        rdfs:domain         vec:PowerConsumption;
        rdfs:label          "type"@en;
        rdfs:range          vec:PowerConsumptionType;
        rdfs:subPropertyOf  vec:contains .

vec:itemHistoryEntrySuccessorVersion
        rdf:type      owl:ObjectProperty;
        rdfs:comment  "References the ItemVersion that is the successor in the ItemHistoryEntry. \n"@en;
        rdfs:domain   vec:ItemHistoryEntry;
        rdfs:label    "successorVersion"@en;
        rdfs:range    vec:ItemVersion .

vec:RequirementsConformanceSpecification
        rdf:type         owl:Class;
        rdfs:comment     "A RequirementsConformanceSpecification can be used to express the conformance of a PartVersion (or a group of PartVersions ). The PartVersions to which this RequirementsConformanceSpecification applies are expressed through the describedPart reference.\n"@en;
        rdfs:label       "RequirementsConformanceSpecification"@en;
        rdfs:subClassOf  vec:PartOrUsageRelatedSpecification .

vec:ApplicationConstraint
        rdf:type         owl:Class;
        rdfs:comment     "An ApplicationConstraint defines a condition with which it is possible to express the inclusion or exclusion of ConfigurableElements in different variants of a product. The ApplicationConstraint is focused to express validity rules based on time periods or elements of the product hierarchy in a concise way (attributes and relationships). It is complementary to the VariantConfiguration which expresses validity rules based on control strings.\nAn ApplicationConstraint can reference another ApplicationConstraint as baseInclusion . In this case, an ApplicationConstraint can only be satisfied if its baseInclusion is also satisfied.\n"@en;
        rdfs:label       "ApplicationConstraint"@en;
        rdfs:subClassOf  vec:ExtendableElement .

vec:TerminalBoltNominalSize_M2
        rdf:type         vec:TerminalBoltNominalSize , owl:NamedIndividiual;
        vec:enumLiteral  "M2" .

vec:partRelationRelationType
        rdf:type            owl:ObjectProperty;
        rdfs:comment        "Specifies the type of the relation.\n"@en;
        rdfs:domain         vec:PartRelation;
        rdfs:label          "relationType"@en;
        rdfs:range          vec:PartRelationType;
        rdfs:subPropertyOf  vec:contains .

vec:materialKey  rdf:type  owl:DatatypeProperty;
        rdfs:comment  "The key of the material in the corresponding material reference system.\n"@en;
        rdfs:domain   vec:Material;
        rdfs:label    "key"@en;
        rdfs:range    xs:string .

vec:grommetSpecificationHardness
        rdf:type            owl:ObjectProperty;
        rdfs:comment        "Specifies the hardness of the grommet.\n"@en;
        rdfs:domain         vec:GrommetSpecification;
        rdfs:label          "hardness"@en;
        rdfs:range          vec:NumericalValue;
        rdfs:subPropertyOf  vec:contains .

vec:FittingForm_Straight
        rdf:type         vec:FittingForm , owl:NamedIndividiual;
        rdfs:comment     "Straight 1:1 coupling e.g. used for the coupling of different pipe sections.\n"@en;
        vec:enumLiteral  "Straight" .

vec:wireReceptionWireReceptionSpecification
        rdf:type      owl:ObjectProperty;
        rdfs:comment  "References the WireReceptionSpecification that specifies the WireReception. \n"@en;
        rdfs:domain   vec:WireReception;
        rdfs:label    "wireReceptionSpecification"@en;
        rdfs:range    vec:WireReceptionSpecification .

vec:ComponentNodeType_CouplingDevice
        rdf:type         vec:ComponentNodeType , owl:NamedIndividiual;
        rdfs:comment     "A CouplingDevice is the (virtual) device that separates / connects two or more wiring harnesses. \"Virtual\" because it can be interpreted as a device / interface definition between the harnesses, where one harness behaves like an E/E component form the point of view of the other harness.\n"@en;
        vec:enumLiteral  "CouplingDevice" .

vec:DocumentRelatedAssignmentGroup
        rdf:type         owl:Class;
        rdfs:comment     "A DocumentRelatedAssignmentGroup allows the creation of traceability links to elements in a DocumentVersion for a set of VEC┬áobjects. The semantic of the traceability link is defined by the DocumentRelationType.\n"@en;
        rdfs:label       "DocumentRelatedAssignmentGroup"@en;
        rdfs:subClassOf  vec:AssignmentGroup .

<http://www.prostep.org/ontologies/ecad/2024/03/vec#TerminalBoltNominalSize_%236>
        rdf:type         vec:TerminalBoltNominalSize , owl:NamedIndividiual;
        vec:enumLiteral  "#6" .

vec:netViewSpecificationCartesianPoint
        rdf:type            owl:ObjectProperty;
        rdfs:comment        "Specifies all the CartesianPoint2Ds that are used within the NetViewSpecification. "@en;
        rdfs:domain         vec:NetViewSpecification;
        rdfs:label          "cartesianPoint"@en;
        rdfs:range          vec:CartesianPoint2D;
        rdfs:subPropertyOf  vec:contains .

vec:wireElementSpecificationWireGroupSpecification
        rdf:type      owl:ObjectProperty;
        rdfs:comment  "If the WireElementSpecification is representing a wire group, then the specification of the wire group is referenced here. That means as well, that the WireElementSpecification shall have subWireElementSpecifications .\n"@en;
        rdfs:domain   vec:WireElementSpecification;
        rdfs:label    "wireGroupSpecification"@en;
        rdfs:range    vec:WireGroupSpecification .

vec:PinTimingType_Duration
        rdf:type         vec:PinTimingType , owl:NamedIndividiual;
        vec:enumLiteral  "duration" .

vec:LanguageCode_Ps  rdf:type  vec:LanguageCode , owl:NamedIndividiual;
        vec:enumLiteral  "Ps" .

vec:generalTechnicalPartSpecificationTemperatureInformation
        rdf:type            owl:ObjectProperty;
        rdfs:comment        "Specifies valid temperatures for a part.\n"@en;
        rdfs:domain         vec:GeneralTechnicalPartSpecification;
        rdfs:label          "temperatureInformation"@en;
        rdfs:range          vec:TemperatureInformation;
        rdfs:subPropertyOf  vec:contains .

vec:TubeSlitStyle_Slit
        rdf:type         vec:TubeSlitStyle , owl:NamedIndividiual;
        rdfs:comment     "The tube has just a simple slit.\n"@en;
        vec:enumLiteral  "Slit" .

vec:SealingGeometry_Segmented
        rdf:type         vec:SealingGeometry , owl:NamedIndividiual;
        vec:enumLiteral  "Segmented" .

vec:PathSegment  rdf:type  owl:Class;
        rdfs:comment     "A PathSegment is a part of the 2D presentation of a GeometrySegment2D. The complete presentation of a GeometrySegment2D is built from an ordered list of PathSegments. Each PathSegment has an ordered list of control points through which the path goes. If no curveRadius is specified the control points are connected by a direct straight line. If a curveRadius is specified, the PathSegment can be drawn by a segment of a circle which touches all control points and has the radius specified.\n"@en;
        rdfs:label       "PathSegment"@en;
        rdfs:subClassOf  vec:ExtendableElement .

vec:USUnitName_Quart  rdf:type  vec:USUnitName , owl:NamedIndividiual;
        vec:enumLiteral  "Quart" .

vec:Connection  rdf:type  owl:Class;
        rdfs:comment     "A Connection is an electrological connection between two or more ComponentPorts.\n"@en;
        rdfs:label       "Connection"@en;
        rdfs:subClassOf  vec:RoutableElement .

vec:TapingDirection_FromEnd
        rdf:type         vec:TapingDirection , owl:NamedIndividiual;
        vec:enumLiteral  "FromEnd" .

vec:cableLeadThroughSpecificationSealable
        rdf:type      owl:DatatypeProperty;
        rdfs:comment  "Specifies if the cable lead through is sealable.\n"@en;
        rdfs:domain   vec:CableLeadThroughSpecification;
        rdfs:label    "sealable"@en;
        rdfs:range    xs:boolean .

vec:defaultDimensionDimensionValueRange
        rdf:type            owl:ObjectProperty;
        rdfs:comment        "dimensionValueRange defines the magnitude of measurements for which the tolerance applies (e.g. length from 500mm - 1500mm).\n"@en;
        rdfs:domain         vec:DefaultDimension;
        rdfs:label          "dimensionValueRange"@en;
        rdfs:range          vec:ValueRange;
        rdfs:subPropertyOf  vec:contains .

vec:wireReceptionAddOnType
        rdf:type            owl:ObjectProperty;
        rdfs:comment        "Defines the type of the add-on.\n"@en;
        rdfs:domain         vec:WireReceptionAddOn;
        rdfs:label          "type"@en;
        rdfs:range          vec:WireAddOnType;
        rdfs:subPropertyOf  vec:contains .

vec:materialDescription
        rdf:type            owl:ObjectProperty;
        rdfs:comment        "On optional human readable description of the material (e.g. the name).\n"@en;
        rdfs:domain         vec:Material;
        rdfs:label          "description"@en;
        rdfs:range          vec:LocalizedString;
        rdfs:subPropertyOf  vec:contains .

vec:cavityPositionDetailRotation
        rdf:type            owl:ObjectProperty;
        rdfs:comment        "The rotation of the cavity is defined as the angle between the primary locking of the cavity and the Y-axis of the connector housing coordinate system.\n"@en;
        rdfs:domain         vec:CavityPositionDetail;
        rdfs:label          "rotation"@en;
        rdfs:range          vec:NumericalValue;
        rdfs:subPropertyOf  vec:contains .

vec:DateValueProperty
        rdf:type         owl:Class;
        rdfs:comment     "A custom property with a date value.\n"@en;
        rdfs:label       "DateValueProperty"@en;
        rdfs:subClassOf  vec:CustomProperty .

vec:capacitorSpecificationCapacity
        rdf:type            owl:ObjectProperty;
        rdfs:domain         vec:CapacitorSpecification;
        rdfs:label          "capacity"@en;
        rdfs:range          vec:NumericalValue;
        rdfs:subPropertyOf  vec:contains .

vec:SlotLayoutType_USBTypeBSuperSpeed
        rdf:type         vec:SlotLayoutType , owl:NamedIndividiual;
        vec:enumLiteral  "USBTypeBSuperSpeed" .

vec:sheetOrChapterSheetSize
        rdf:type            owl:ObjectProperty;
        rdfs:comment        "Defines the size of the sheet with numerical values. This is the size of the \"paper\", the actual drawing area might be smaller for example due to drawing frames."@en;
        rdfs:domain         vec:SheetOrChapter;
        rdfs:label          "sheetSize"@en;
        rdfs:range          vec:Size;
        rdfs:subPropertyOf  vec:contains .

vec:WindingType_Spiral
        rdf:type         vec:WindingType , owl:NamedIndividiual;
        rdfs:comment     " Spiral defines a taping with the least overlapping (German: Spiral).\n"@en;
        vec:enumLiteral  "Spiral" .

vec:PinComponentType_NotConnected
        rdf:type         vec:PinComponentType , owl:NamedIndividiual;
        vec:enumLiteral  "NotConnected" .

vec:LanguageCode_Lv  rdf:type  vec:LanguageCode , owl:NamedIndividiual;
        vec:enumLiteral  "Lv" .

vec:VariantGroup  rdf:type  owl:Class;
        rdfs:comment     "With a VariantGroup it is possible to group VariantCodes. The semantic of this grouping should be defined with the groupType (e.g. composition, choice, etc.).\n"@en;
        rdfs:label       "VariantGroup"@en;
        rdfs:subClassOf  vec:ExtendableElement .

vec:PinType_Filament  rdf:type  vec:PinType , owl:NamedIndividiual;
        vec:enumLiteral  "filament" .

vec:TubeSlitStyle_Overlapping
        rdf:type         vec:TubeSlitStyle , owl:NamedIndividiual;
        rdfs:comment     "The edges of the slit are overlapping.\n"@en;
        vec:enumLiteral  "Overlapping" .

vec:connectorHousingSpecificationConnectorPositionAssurance
        rdf:type      owl:DatatypeProperty;
        rdfs:comment  "If true the ConnectorHousing has a connector position assurance (CPA).\nA CPA is some sort of feature of a connector, that secures the connector in its correctly assembled position with its mating part.\n"@en;
        rdfs:domain   vec:ConnectorHousingSpecification;
        rdfs:label    "connectorPositionAssurance"@en;
        rdfs:range    xs:boolean .

vec:LevelOfApproval_Invalid
        rdf:type         vec:LevelOfApproval , owl:NamedIndividiual;
        rdfs:comment     "The ItemVersion shall not be used anymore.\n"@en;
        vec:enumLiteral  "Invalid" .

vec:boltMountedFixingSpecificationBoltDiameter
        rdf:type            owl:ObjectProperty;
        rdfs:comment        "Specifies the diameter of the bolt on which the fixing can be mounted.\n"@en;
        rdfs:domain         vec:BoltMountedFixingSpecification;
        rdfs:label          "boltDiameter"@en;
        rdfs:range          vec:NumericalValue;
        rdfs:subPropertyOf  vec:contains .

vec:TerminalBoltNominalSize_M7
        rdf:type         vec:TerminalBoltNominalSize , owl:NamedIndividiual;
        vec:enumLiteral  "M7" .

vec:PrimaryPartType_WireProtection
        rdf:type         vec:PrimaryPartType , owl:NamedIndividiual;
        vec:enumLiteral  "WireProtection" .

vec:robustnessPropertiesHasRobustness
        rdf:type      owl:DatatypeProperty;
        rdfs:comment  "Specifies if the described element has a robustness in the specified robustness class. (see KBLFRM-260)\n"@en;
        rdfs:domain   vec:RobustnessProperties;
        rdfs:label    "hasRobustness"@en;
        rdfs:range    xs:boolean .

vec:MassInformationSource_IMDS
        rdf:type         vec:MassInformationSource , owl:NamedIndividiual;
        rdfs:comment     "A MassInformation with this valueSource has been retrieved from the IMDS (see http://www.mdsystem.com ).\n"@en;
        vec:enumLiteral  "IMDS" .

vec:WireLengthType_Contract
        rdf:type         vec:WireLengthType , owl:NamedIndividiual;
        rdfs:comment     "The agreed length for any negotiations and calculations.\n"@en;
        vec:enumLiteral  "Contract" .

vec:abstractSlotSlotSpecification
        rdf:type      owl:ObjectProperty;
        rdfs:comment  "References the SlotSpecification that is satisfied by the slot.\n"@en;
        rdfs:domain   vec:AbstractSlot;
        rdfs:label    "slotSpecification"@en;
        rdfs:range    vec:SlotSpecification .

vec:colorReferenceSystem
        rdf:type            owl:ObjectProperty;
        rdfs:comment        "The identification of the color reference system, which is defining possible values and the semantic of color keys. (see KBLFRM-315). For common color reference systems the literals defined in the open enumeration ColorReferenceSystem shall be used.\n"@en;
        rdfs:domain         vec:Color;
        rdfs:label          "referenceSystem"@en;
        rdfs:range          vec:ColorReferenceSystem;
        rdfs:subPropertyOf  vec:contains .

vec:OccurrenceOrUsageViewItem3D
        rdf:type         owl:Class;
        rdfs:comment     "An OccurrenceOrUsageViewItem3D specifies the existence and representation of an OccurrenceOrUsage in a 3D-model.\nThe definition of the existence is necessary because a 150% model of a harness might contain different geometric variants and not all of them must be represented in the same BuildingBlockSpecification3D .\nThere are two different cases for the representation of OccurrenceOrUsage s in a 3D model. There are components that can be represented explicitly by a 3D model of the component (e.g. connectors, cable ducts, fixings) and there are components that are represented implicitly by a generic visualization and their placement on the topology (e.g. tapes, tubes). If an OccurrenceOrUsage has a 3D┬ámodel and it shall be placed explicitly in 3D space, the OccurrenceOrUsageViewItem3D defines a Transformation3D in the orientation role. If no orientation is defined the OccurrenceOrUsage is represented implicitly.\n"@en;
        rdfs:label       "OccurrenceOrUsageViewItem3D"@en;
        rdfs:subClassOf  vec:ExtendableElement .

vec:ComponentPortViewItem
        rdf:type      owl:Class;
        rdfs:comment  "A ComponentPortViewItem represents a ComponentPort within a ComponentNodeViewItem and defines its position on the node."@en;
        rdfs:label    "ComponentPortViewItem"@en .

vec:UsageNodeType_Sensor
        rdf:type         vec:UsageNodeType , owl:NamedIndividiual;
        vec:enumLiteral  "Sensor" .

vec:geometrySegmentAliasId
        rdf:type            owl:ObjectProperty;
        rdfs:comment        "Specifies additional identifiers for the GeometrySegment.\n"@en;
        rdfs:domain         vec:GeometrySegment;
        rdfs:label          "aliasId"@en;
        rdfs:range          vec:AliasIdentification;
        rdfs:subPropertyOf  vec:contains .

vec:HousingComponentType_RingTerminal
        rdf:type         vec:HousingComponentType , owl:NamedIndividiual;
        vec:enumLiteral  "RingTerminal" .

vec:usageNodeUsedInProject
        rdf:type      owl:ObjectProperty;
        rdfs:comment  "Specifies the Projects in which the UsageNode can be used.\n"@en;
        rdfs:domain   vec:UsageNode;
        rdfs:label    "usedInProject"@en;
        rdfs:range    vec:Project .

vec:placementSpecificationDimension
        rdf:type            owl:ObjectProperty;
        rdfs:comment        "Specifies the Dimensions defined by the PlacementSpecification.\n"@en;
        rdfs:domain         vec:PlacementSpecification;
        rdfs:label          "dimension"@en;
        rdfs:range          vec:Dimension;
        rdfs:subPropertyOf  vec:contains .

vec:LanguageCode_Hy  rdf:type  vec:LanguageCode , owl:NamedIndividiual;
        vec:enumLiteral  "Hy" .

vec:cavityMountingEquippedCavityRef
        rdf:type      owl:ObjectProperty;
        rdfs:comment  "References the cavities that are used for the cavity mounting. \n"@en;
        rdfs:domain   vec:CavityMounting;
        rdfs:label    "equippedCavityRef"@en;
        rdfs:range    vec:CavityReference .

vec:PrimaryPartType_BoltMountedFixing
        rdf:type         vec:PrimaryPartType , owl:NamedIndividiual;
        vec:enumLiteral  "BoltMountedFixing" .

vec:ferriteRoleFerriteSpecification
        rdf:type     owl:ObjectProperty;
        rdfs:domain  vec:FerriteRole;
        rdfs:label   "ferriteSpecification"@en;
        rdfs:range   vec:FerriteSpecification .

vec:cavityAccessorySpecificationWireElementOutsideDiameter
        rdf:type            owl:ObjectProperty;
        rdfs:comment        "Specifies a range of valid wire diameters to which the cavity accessory fits.\n"@en;
        rdfs:domain         vec:CavityAccessorySpecification;
        rdfs:label          "wireElementOutsideDiameter"@en;
        rdfs:range          vec:ValueRange;
        rdfs:subPropertyOf  vec:contains .

vec:cavityPartSpecificationCavityDimension
        rdf:type            owl:ObjectProperty;
        rdfs:comment        "Specifies a valid cavity dimensions to which the cavity part fits. The dimension defines the size of the sealing area of the cavity (crimp end), not in the contacting area (box end).\nNote: CavityDimension is of type Size which is defined as x &┬áy with type NumericalValue. NumericalValue can define tolerances. So, a cavity dimension is not necessarily a single fixed value.\n"@en;
        rdfs:domain         vec:CavityPartSpecification;
        rdfs:label          "cavityDimension"@en;
        rdfs:range          vec:Size;
        rdfs:subPropertyOf  vec:contains .

vec:onWayPlacementPath
        rdf:type            owl:ObjectProperty;
        rdfs:comment        "Specifies the topology path defining the way the OnWayPlacement takes in the topology. \n"@en;
        rdfs:domain         vec:OnWayPlacement;
        rdfs:label          "path"@en;
        rdfs:range          vec:Path;
        rdfs:subPropertyOf  vec:contains .

vec:TransmissionMediumType_Hydraulic
        rdf:type         vec:TransmissionMediumType , owl:NamedIndividiual;
        vec:enumLiteral  "Hydraulic" .

vec:DocumentBasedInstruction
        rdf:type         owl:Class;
        rdfs:comment     "A DocumentBasedInstruction is an Instruction to a SheetOrChapter in a DocumentVersion or to a complete DocumentVersion.\n"@en;
        rdfs:label       "DocumentBasedInstruction"@en;
        rdfs:subClassOf  vec:Instruction .

vec:tubeSpecificationSlitStyle
        rdf:type            owl:ObjectProperty;
        rdfs:comment        "Specifies the style of the slitting of the tube. If a slitStyle is defined, it implies that isSlit=true .\nThis attribute is defined as an OpenEnumeration.\n"@en;
        rdfs:domain         vec:TubeSpecification;
        rdfs:label          "slitStyle"@en;
        rdfs:range          vec:TubeSlitStyle;
        rdfs:subPropertyOf  vec:contains .

vec:SignalType  rdf:type  owl:Class;
        rdfs:label       "SignalType"@en;
        rdfs:subClassOf  vec:OpenEnumeration .

vec:connectionViewSpecificationPlacedViewItems
        rdf:type            owl:ObjectProperty;
        rdfs:comment        "Specifies all ComponentNodeViewItems that are displayed within a ConnectionViewSpecification ."@en;
        rdfs:domain         vec:ConnectionViewSpecification;
        rdfs:label          "placedViewItems"@en;
        rdfs:range          vec:ConnectionNodeViewItem;
        rdfs:subPropertyOf  vec:contains .

vec:terminalSpecificationConnectionALength
        rdf:type            owl:ObjectProperty;
        rdfs:comment        "Specifies the length of the terminal between the contact area (terminal reception) and the crimp are (wire reception, see diagram \"Terminal Dimensions\").\n"@en;
        rdfs:domain         vec:TerminalSpecification;
        rdfs:label          "connectionALength"@en;
        rdfs:range          vec:NumericalValue;
        rdfs:subPropertyOf  vec:contains .

vec:onWayPlacementEndLocation
        rdf:type            owl:ObjectProperty;
        rdfs:comment        "References the Location where OnWayPlacement ends. \n"@en;
        rdfs:domain         vec:OnWayPlacement;
        rdfs:label          "endLocation"@en;
        rdfs:range          vec:Location;
        rdfs:subPropertyOf  vec:contains .

vec:ImperialUnitName_Ounce
        rdf:type         vec:ImperialUnitName , owl:NamedIndividiual;
        vec:enumLiteral  "Ounce" .

vec:UsageNodeSpecification
        rdf:type         owl:Class;
        rdfs:comment     "A UsageNodeSpecification is a container for the specification of UsageNodes.\n"@en;
        rdfs:label       "UsageNodeSpecification"@en;
        rdfs:subClassOf  vec:Specification .

vec:BuildingBlockSpecification2D
        rdf:type         owl:Class;
        rdfs:comment     "Specification for the description of a two-dimensional building block. A building block is a reusable section of a geometry.\n"@en;
        rdfs:label       "BuildingBlockSpecification2D"@en;
        rdfs:subClassOf  vec:Specification .

vec:variantStructureNodeContainedGroups
        rdf:type     owl:ObjectProperty;
        rdfs:domain  vec:VariantStructureNode;
        rdfs:label   "containedGroups"@en;
        rdfs:range   vec:VariantGroup .

vec:CableDuctSpecification
        rdf:type         owl:Class;
        rdfs:comment     "Specification for cable ducts. A cable duct can have one or more outlets.\n"@en;
        rdfs:label       "CableDuctSpecification"@en;
        rdfs:subClassOf  vec:PartOrUsageRelatedSpecification .

vec:specificRoleSpecification
        rdf:type      owl:ObjectProperty;
        rdfs:comment  "References the PartOrUsageRelatedSpecification that is instantiated by this SpecificRole.\n"@en;
        rdfs:domain   vec:SpecificRole;
        rdfs:label    "specification"@en;
        rdfs:range    vec:PartOrUsageRelatedSpecification .

vec:MassInformation  rdf:type  owl:Class;
        rdfs:comment  "Allows the definition of mass information. Attributes of the type MassInformation normally have the multiplicity [0..*]. This means that such an attribute can have mass values for different determinationTypes and valueSources. It must not have multiple values for the same determinationType and valueSource.\n"@en;
        rdfs:label    "MassInformation"@en .

vec:pinCurrentInformationCurrent
        rdf:type            owl:ObjectProperty;
        rdfs:comment        "The current of the pin.\n"@en;
        rdfs:domain         vec:PinCurrentInformation;
        rdfs:label          "current"@en;
        rdfs:range          vec:NumericalValue;
        rdfs:subPropertyOf  vec:contains .

vec:geometryNodeIdentification
        rdf:type      owl:DatatypeProperty;
        rdfs:comment  "Specifies a unique identification of the GeometryNode. The identification is guaranteed to be unique within the corresponding BuildingBlockSpecification. For all VEC-documents a GeometryNode-instance can be trusted to be the same if the BuildingBlockSpecification-instance is the same (see BuildingBlockSpecification) and the identification of the GeometryNode is the same.\n"@en;
        rdfs:domain   vec:GeometryNode;
        rdfs:label    "identification"@en;
        rdfs:range    xs:string .

vec:RobustnessClass  rdf:type  owl:Class;
        rdfs:comment     "Defines the literals that shall be used for specific robustness classes.\n"@en;
        rdfs:label       "RobustnessClass"@en;
        rdfs:subClassOf  vec:OpenEnumeration .

vec:cartesianPoint3DY
        rdf:type      owl:DatatypeProperty;
        rdfs:comment  "Specifies the value of y-coordinate of the Cartesian point. The unit of this value is the baseUnit of containing BuildingBlockSpecification3D.\n"@en;
        rdfs:domain   vec:CartesianPoint3D;
        rdfs:label    "y"@en;
        rdfs:range    xs:double .

vec:GeometrySegment  rdf:type  owl:Class;
        rdfs:comment     "A GeometrySegment is the geometric representation of a TopologySegment. A TopologySegment may be represented by more than one GeometrySegments, but only within different BuildingBlockSpecification2D/3D. That means, in a single BuildingBlockSpecification a TopologySegment shall only be represent once┬á(or not).\nFurthermore, the definition of the GeometrySegment shall be consistent to the definition in the TopologySpecification. That means, that a GeometrySegment shall have those GeometryNodes as start- &┬áendNode that represent the TopologyNodes referenced from the corresponding TopologySegment .\nA GeometrySegment is either a GeometrySegment2D or a GeometrySegment3D.\n"@en;
        rdfs:label       "GeometrySegment"@en;
        rdfs:subClassOf  vec:ConfigurableElement .

vec:FittingForm  rdf:type  owl:Class;
        rdfs:comment     "OpenEnumeration to define different fitting forms.\n"@en;
        rdfs:label       "FittingForm"@en;
        rdfs:subClassOf  vec:OpenEnumeration .

vec:SiUnitName_Joule  rdf:type  vec:SiUnitName , owl:NamedIndividiual;
        vec:enumLiteral  "Joule" .

vec:SealingGeometry  rdf:type  owl:Class;
        rdfs:comment     "Defines valid values of the geometry of a cavity sealing. It defines the cross-section geometry.\n"@en;
        rdfs:label       "SealingGeometry"@en;
        rdfs:subClassOf  vec:OpenEnumeration .

vec:SiUnitName_Lux  rdf:type  vec:SiUnitName , owl:NamedIndividiual;
        vec:enumLiteral  "Lux" .

vec:wireEndIdentification
        rdf:type      owl:DatatypeProperty;
        rdfs:comment  "Specifies a unique identification of the WireEnd. The identification is guaranteed to be unique within the WireElementReference.\n"@en;
        rdfs:domain   vec:WireEnd;
        rdfs:label    "identification"@en;
        rdfs:range    xs:string .

vec:WireMounting  rdf:type  owl:Class;
        rdfs:comment     "A WireMounting defines the mounting of a wire end to terminal. If the contacting is required to be waterproof a cavity seal can be mounted additionally.\n"@en;
        rdfs:label       "WireMounting"@en;
        rdfs:subClassOf  vec:ExtendableElement .

vec:moduleListIdentification
        rdf:type      owl:DatatypeProperty;
        rdfs:comment  "Specifies a unique identification of the ModuleList. The identification is guaranteed to be unique within the ModuleListSpecification. For all VEC-documents a ModuleList-instance can be trusted to be the same if the ModuleListSpecification-instance is the same and the identification of the ModuleList is the same.\n"@en;
        rdfs:domain   vec:ModuleList;
        rdfs:label    "identification"@en;
        rdfs:range    xs:string .

vec:LabelType_RFID  rdf:type  vec:LabelType , owl:NamedIndividiual;
        vec:enumLiteral  "RFID" .

vec:PinComponentType  rdf:type  owl:Class;
        rdfs:comment     "Specifies the type of a PinComponent .\n"@en;
        rdfs:label       "PinComponentType"@en;
        rdfs:subClassOf  vec:OpenEnumeration .

vec:slotSpecificationGender
        rdf:type            owl:ObjectProperty;
        rdfs:comment        "Specifies the gender of the slot. Valid values are defined in an open enumeration.\n"@en;
        rdfs:domain         vec:SlotSpecification;
        rdfs:label          "gender"@en;
        rdfs:range          vec:SlotGender;
        rdfs:subPropertyOf  vec:contains .

vec:cableTieRoleCableTieSpecification
        rdf:type     owl:ObjectProperty;
        rdfs:domain  vec:CableTieRole;
        rdfs:label   "cableTieSpecification"@en;
        rdfs:range   vec:CableTieSpecification .

vec:buildingBlockPositioning3DIdentification
        rdf:type      owl:DatatypeProperty;
        rdfs:comment  "Specifies a unique (optional) identification of the BuildingBlockPositioning3D. The identification is guaranteed to be unique within the HarnessGeometrySpecification3D.\n"@en;
        rdfs:domain   vec:BuildingBlockPositioning3D;
        rdfs:label    "identification"@en;
        rdfs:range    xs:string .

vec:wireReceptionSpecificationAddOns
        rdf:type            owl:ObjectProperty;
        rdfs:domain         vec:WireReceptionSpecification;
        rdfs:label          "addOns"@en;
        rdfs:range          vec:WireReceptionAddOn;
        rdfs:subPropertyOf  vec:contains .

vec:buildingBlockSpecification3DGeometrySegment
        rdf:type            owl:ObjectProperty;
        rdfs:comment        "Specifies the GeometrySegment3Ds defined by the BuildingBlockSpecification3D.\n"@en;
        rdfs:domain         vec:BuildingBlockSpecification3D;
        rdfs:label          "geometrySegment"@en;
        rdfs:range          vec:GeometrySegment3D;
        rdfs:subPropertyOf  vec:contains .

vec:PartStructureContentType
        rdf:type         owl:Class;
        rdfs:comment     "OpenEnumeration that defines standard content types for the PartStructureSpecification.\n"@en;
        rdfs:label       "PartStructureContentType"@en;
        rdfs:subClassOf  vec:OpenEnumeration .

vec:variantCodeIdentification
        rdf:type      owl:DatatypeProperty;
        rdfs:comment  "Specifies a unique identification of the variant code. This is also the literal value for the VariantCode, which shall be used in the logisticControlExpressions of VariantConfigurations.\n"@en;
        rdfs:domain   vec:VariantCode;
        rdfs:label    "identification"@en;
        rdfs:range    xs:string .

vec:FuseType_Type_F  rdf:type  vec:FuseType , owl:NamedIndividiual;
        rdfs:comment     "also known as: mini\n"@en;
        vec:enumLiteral  "Type_F" .

vec:NominalVoltage_HV1
        rdf:type         vec:NominalVoltage , owl:NamedIndividiual;
        rdfs:comment     "HV Class 1 (200V┬áDC)\n"@en;
        vec:enumLiteral  "HV1" .

vec:RelaySpecification
        rdf:type         owl:Class;
        rdfs:comment     "Specification of the electrological aspects of a relay.\n"@en;
        rdfs:label       "RelaySpecification"@en;
        rdfs:subClassOf  vec:EEComponentSpecification .

[ rdf:type     owl:AllDisjointClasses;
  owl:members  ( vec:MultiCavitySealSpecification )
] .

vec:LanguageCode_Ca  rdf:type  vec:LanguageCode , owl:NamedIndividiual;
        vec:enumLiteral  "Ca" .

vec:TemperatureInformation
        rdf:type      owl:Class;
        rdfs:comment  "Defines valid temperature ranges for a general technical part. A part can have different valid temperature ranges in different scenarios e.g. operating temperature, storage temperature, processing temperature, environment temperature. A class can own multiple TemperatureInformations but must not have more than one TemperatureInformations of the same temperatureType.\n"@en;
        rdfs:label    "TemperatureInformation"@en .

vec:usageNodeSubUsageNodes
        rdf:type            owl:ObjectProperty;
        rdfs:comment        ""@en;
        rdfs:domain         vec:UsageNode;
        rdfs:label          "subUsageNodes"@en;
        rdfs:range          vec:UsageNode;
        rdfs:subPropertyOf  vec:contains .

vec:partVersionPartVersion
        rdf:type      owl:DatatypeProperty;
        rdfs:comment  "The partVersion specifies the version index of a part (see also partNumber).\n"@en;
        rdfs:domain   vec:PartVersion;
        rdfs:label    "partVersion"@en;
        rdfs:range    xs:string .

vec:OtherUnit  rdf:type  owl:Class;
        rdfs:comment     "The OtherUnit class can be used to define a unit, which is necessary in the context of data exchange but not contained in the standard systems (e.g. Piece).\n"@en;
        rdfs:label       "OtherUnit"@en;
        rdfs:subClassOf  vec:Unit .

vec:TerminalBoltNominalSize_M24
        rdf:type         vec:TerminalBoltNominalSize , owl:NamedIndividiual;
        vec:enumLiteral  "M24" .

vec:IECUnit  rdf:type    owl:Class;
        rdfs:comment     "The IECUnit class can define quantities in the terms of the IEC-Unit-System by specifying the corresponding IEC prefix (optional) and an IEC unit name.\n"@en;
        rdfs:label       "IECUnit"@en;
        rdfs:subClassOf  vec:Unit .

vec:wireElementSpecificationMinBendRadiusStatic
        rdf:type            owl:ObjectProperty;
        rdfs:comment        "Specifies the minimum bend radius for wire element, if it is used in a static environment, where it is bended once during installation. After that it remains unchanged in its bended position during usage. (see KLBFRM-311)\n"@en;
        rdfs:domain         vec:WireElementSpecification;
        rdfs:label          "minBendRadiusStatic"@en;
        rdfs:range          vec:NumericalValue;
        rdfs:subPropertyOf  vec:contains .

vec:cavityIntegratedTerminalSpecification
        rdf:type      owl:ObjectProperty;
        rdfs:comment  "Specifies the terminal, if the cavity has an integrated terminal (e.g. an IDC).\n"@en;
        rdfs:domain   vec:Cavity;
        rdfs:label    "integratedTerminalSpecification"@en;
        rdfs:range    vec:TerminalSpecification .

vec:SlotLayoutType_USBMicroAB
        rdf:type         vec:SlotLayoutType , owl:NamedIndividiual;
        vec:enumLiteral  "USBMicroAB" .

vec:cartesianVector2DX
        rdf:type      owl:DatatypeProperty;
        rdfs:comment  "Specifies the x-coordinate in 2D space.\n"@en;
        rdfs:domain   vec:CartesianVector2D;
        rdfs:label    "x"@en;
        rdfs:range    xs:double .

vec:segmentConnectionPointModularSlotAddOns
        rdf:type            owl:ObjectProperty;
        rdfs:domain         vec:SegmentConnectionPoint;
        rdfs:label          "ModularSlotAddOns"@en;
        rdfs:range          vec:ModularSlotAddOn;
        rdfs:subPropertyOf  vec:contains .

vec:WireGrouping  rdf:type  owl:Class;
        rdfs:comment     "A WireGrouping is the definition of a multi core wire in its usage.┬áThe elements of a WireGrouping are well defined wires (e.g. with a part number). The grouping itself is only created in its concrete usage. The most common use case is the individual definition of unshielded twisted pair wires without creating the full combinatorics of every possible core / insulation / twist combination in a part master data system (and by this creating part numbers for all of them). However, there are other use cases as well.\nA WireGrouping groups the relatedWireElementReferences on an equal level containedWireGroupings are on a lower level. So, in order to create something like a shielded twisted pair, one WireGrouping \"A\" that references two WireElementReferences is required to represent the twisted pair and another WireGrouping \" B\" that contains WireGrouping \"A\" and references the \"shield wire element\".\n┬áThe referenced WireGroupSpecification defines the handling of the WireGrouping during its assembly (e.g. twist).\n"@en;
        rdfs:label       "WireGrouping"@en;
        rdfs:subClassOf  vec:ExtendableElement .

vec:HoleMountedFixingSpecification
        rdf:type         owl:Class;
        rdfs:comment     "Specification for fixings that are mounted into a hole. This means the fixing has got a bolt which is mounted into a hole of the surrounding.\n"@en;
        rdfs:label       "HoleMountedFixingSpecification"@en;
        rdfs:subClassOf  vec:FixingSpecification .

vec:USUnitName_Stone  rdf:type  vec:USUnitName , owl:NamedIndividiual;
        vec:enumLiteral  "Stone" .

vec:TopologyZoneType  rdf:type  owl:Class;
        rdfs:comment     "There can be various reasons to define TopologyZones. These can be differentiated with these type literals.\n"@en;
        rdfs:label       "TopologyZoneType"@en;
        rdfs:subClassOf  vec:OpenEnumeration .

vec:TerminalBoltNominalSize_M45
        rdf:type         vec:TerminalBoltNominalSize , owl:NamedIndividiual;
        vec:enumLiteral  "M45" .

vec:SiUnitName_Farad  rdf:type  vec:SiUnitName , owl:NamedIndividiual;
        vec:enumLiteral  "Farad" .

vec:codingCoding  rdf:type  owl:DatatypeProperty;
        rdfs:comment  "Specifies the name of the coding.\n"@en;
        rdfs:domain   vec:Coding;
        rdfs:label    "coding"@en;
        rdfs:range    xs:string .

vec:LocalPosition  rdf:type  owl:Class;
        rdfs:comment  "A LocalPosition defines the position of a relevant point of component within the coordinate system of the component.\n"@en;
        rdfs:label    "LocalPosition"@en .

vec:variantCodeAbbreviation
        rdf:type            owl:ObjectProperty;
        rdfs:comment        "Room for a human readable short name, title etc. of the VariantConfiguration.\n"@en;
        rdfs:domain         vec:VariantCode;
        rdfs:label          "abbreviation"@en;
        rdfs:range          vec:LocalizedString;
        rdfs:subPropertyOf  vec:contains .

vec:HistoryEntryType_Sequence
        rdf:type         vec:HistoryEntryType , owl:NamedIndividiual;
        vec:enumLiteral  "Sequence" .

vec:partOrUsageRelatedSpecificationSpecialPartType
        rdf:type      owl:DatatypeProperty;
        rdfs:comment  "The specialPartType allows the specification of subclassifications for a PartOrUsageRelatedSpecification (e.g. different types of connector housings).\n"@en;
        rdfs:domain   vec:PartOrUsageRelatedSpecification;
        rdfs:label    "specialPartType"@en;
        rdfs:range    xs:string .

vec:FittingForm_Reducer
        rdf:type         vec:FittingForm , owl:NamedIndividiual;
        rdfs:comment     "Straight 1:1 coupling used for changes of the nominal size.\n"@en;
        vec:enumLiteral  "Reducer" .

vec:SlotLayoutType_Form_CB15_CatE
        rdf:type         vec:SlotLayoutType , owl:NamedIndividiual;
        rdfs:comment     "Fuse type according to ISO8820, also known as: auto\n"@en;
        vec:enumLiteral  "Form_CB15_CatE" .

vec:terminalRoleTerminalReceptionReference
        rdf:type            owl:ObjectProperty;
        rdfs:comment        "Specifies the TerminalReceptionReferences of this TerminalRole.\n"@en;
        rdfs:domain         vec:TerminalRole;
        rdfs:label          "terminalReceptionReference"@en;
        rdfs:range          vec:TerminalReceptionReference;
        rdfs:subPropertyOf  vec:contains .

vec:SlotLayoutType_USBTypeC
        rdf:type         vec:SlotLayoutType , owl:NamedIndividiual;
        vec:enumLiteral  "USBTypeC" .

vec:textBasedInstructionInstallationInstruction
        rdf:type            owl:ObjectProperty;
        rdfs:comment        "Specifies the instruction in a human readable form. Different languages are possible.\n"@en;
        rdfs:domain         vec:TextBasedInstruction;
        rdfs:label          "installationInstruction"@en;
        rdfs:range          vec:LocalizedString;
        rdfs:subPropertyOf  vec:contains .

vec:applicationConstraintFromEffectivityControlKey
        rdf:type      owl:DatatypeProperty;
        rdfs:comment  "In the production logistics of complex products (like vehicles), the control of operation and cancellation dates of changes, features, components or the like is usually not carried out via concrete dates but via \"date keys\". These keys are then mapped in planning systems with concrete time specifications for certain plants or production steps. In the VEC┬áthese keys are called EffectivityControlKey.\nWith the FromEffectivityControlKey and To EffectivityControlKey a validity interval can be defined. If one of the two values is defined and the other is omitted, the meaning shall be \"unbounded\".\n"@en;
        rdfs:domain   vec:ApplicationConstraint;
        rdfs:label    "fromEffectivityControlKey"@en;
        rdfs:range    xs:string .

vec:Curve3D  rdf:type    owl:Class;
        rdfs:comment     "The Curve3D is an abstract representation of a curve, that defines the three-dimensional appearance of the centreline of a segment. The concrete type of the curve (e.g. NURBSCurve) defines the mathematical function that applies to curve and stores the required parameter set for this function in the VEC.\n"@en;
        rdfs:label       "Curve3D"@en;
        rdfs:subClassOf  vec:ExtendableElement .

vec:LanguageCode_Id  rdf:type  vec:LanguageCode , owl:NamedIndividiual;
        vec:enumLiteral  "Id" .

vec:partVersionPrimaryPartType
        rdf:type            owl:ObjectProperty;
        rdfs:comment        "The primary type of the part defines the type of the part (e.g. ConnectorHousing, Fixing, etc.) Since the VEC supports dual use parts (e.g. Fixing & WireProtection) the primary part type is necessary to define which specification associated to part is the primary character of the part. Therefore, all primary part types correspond to a PartOrUsageRelatedSpecification (e.g. ConnectorHousing --> ConnectorHousingSpecification).\n"@en;
        rdfs:domain         vec:PartVersion;
        rdfs:label          "primaryPartType"@en;
        rdfs:range          vec:PrimaryPartType;
        rdfs:subPropertyOf  vec:contains .

vec:variantGroupGroupType
        rdf:type            owl:ObjectProperty;
        rdfs:comment        "Allows the classification of a VariantGroups into different types. For example: - composition (e.g. winter package) - choice (e.g. right hand / left hand driving). Agreed literals for this attribute are defined in the OpenEnumeration VariantGroupType.\n"@en;
        rdfs:domain         vec:VariantGroup;
        rdfs:label          "groupType"@en;
        rdfs:range          vec:VariantGroupType;
        rdfs:subPropertyOf  vec:contains .

vec:boltTerminalSpecificationBoltDiameter
        rdf:type            owl:ObjectProperty;
        rdfs:comment        "Specifies the diameter of the bolt in a nominal way.\n"@en;
        rdfs:domain         vec:BoltTerminalSpecification;
        rdfs:label          "boltDiameter"@en;
        rdfs:range          vec:NumericalValue;
        rdfs:subPropertyOf  vec:contains .

vec:WireTupleTermination
        rdf:type      owl:Class;
        rdfs:comment  "A WireTupleTermination is to define the handling of wire ends in a tuple (group). This is mostly relevant for twisted pairs┬á/┬átriple / tuple to define the handling of untwisting.\n"@en;
        rdfs:label    "WireTupleTermination"@en .

vec:insulationSpecificationThickness
        rdf:type            owl:ObjectProperty;
        rdfs:comment        "Specifies the thickness of the insulation.\n"@en;
        rdfs:domain         vec:InsulationSpecification;
        rdfs:label          "thickness"@en;
        rdfs:range          vec:NumericalValue;
        rdfs:subPropertyOf  vec:contains .

vec:wireTupleSpecificationFixationRequired
        rdf:type      owl:DatatypeProperty;
        rdfs:comment  "Specifies if a fixation to prevent untwisting is required."@en;
        rdfs:domain   vec:WireTupleSpecification;
        rdfs:label    "fixationRequired"@en;
        rdfs:range    xs:boolean .

vec:TemperatureType_AmbientTemperature
        rdf:type         vec:TemperatureType , owl:NamedIndividiual;
        vec:enumLiteral  "AmbientTemperature" .

vec:wireEndAccessorySpecificationWireReceptionSpecification
        rdf:type      owl:ObjectProperty;
        rdfs:comment  "References the single WireReceptionSpecification that is specifying the properties of the WireEndAccessory that are related to wire.\n"@en;
        rdfs:domain   vec:WireEndAccessorySpecification;
        rdfs:label    "wireReceptionSpecification"@en;
        rdfs:range    vec:WireReceptionSpecification .

vec:wireElementReferenceWireLength
        rdf:type            owl:ObjectProperty;
        rdfs:comment        "Specifies the different length of a wire. \n"@en;
        rdfs:domain         vec:WireElementReference;
        rdfs:label          "wireLength"@en;
        rdfs:range          vec:WireLength;
        rdfs:subPropertyOf  vec:contains .

vec:SiPrefix_Tera  rdf:type  vec:SiPrefix , owl:NamedIndividiual;
        vec:enumLiteral  "Tera" .

vec:TubeSlitStyle_Closable
        rdf:type         vec:TubeSlitStyle , owl:NamedIndividiual;
        rdfs:comment     "The slit can be closed manually.\n"@en;
        vec:enumLiteral  "Closable" .

vec:transformation3DA13
        rdf:type     owl:DatatypeProperty;
        rdfs:domain  vec:Transformation3D;
        rdfs:label   "a13"@en;
        rdfs:range   xs:double .

vec:GeometryNode3D  rdf:type  owl:Class;
        rdfs:comment     "A GeometryNode3D is the geometric representation of a TopologyNode in 3D-space.\n"@en;
        rdfs:label       "GeometryNode3D"@en;
        rdfs:subClassOf  vec:GeometryNode .

vec:NetworkNodeSubType_Motor
        rdf:type         vec:NetworkNodeSubType , owl:NamedIndividiual;
        vec:enumLiteral  "Motor" .

vec:wireProtectionRoleWireProtectionSpecification
        rdf:type      owl:ObjectProperty;
        rdfs:comment  "References the WireProtectionSpecification that is instanced by this WireProtectionRole.\n"@en;
        rdfs:domain   vec:WireProtectionRole;
        rdfs:label    "wireProtectionSpecification"@en;
        rdfs:range    vec:WireProtectionSpecification .

vec:cableDuctOutletPlacementPoint
        rdf:type      owl:ObjectProperty;
        rdfs:comment  "Specifies the PlacementPoint that represents this CableDuctOutlet in a PlaceableElementSpecification.\n"@en;
        rdfs:domain   vec:CableDuctOutlet;
        rdfs:label    "placementPoint"@en;
        rdfs:range    vec:PlacementPoint .

vec:CompositionSpecification
        rdf:type         owl:Class;
        rdfs:comment     "The CompositionSpecificiation is used to define a set of occurrences required to describe unambiguously the design of a composite part. This does not have to be necessarily the same occurrences which are building the bill of material. Example: A company might want to regard an antenna cable as one part out of a bill of material perspective. However, at the same time it may be useful for the company to be able to describe the contacting of the antenna cable within the VEC. (see also PartStructureSpecification)\n"@en;
        rdfs:label       "CompositionSpecification"@en;
        rdfs:subClassOf  vec:Specification .

vec:ValueRangeProperty
        rdf:type         owl:Class;
        rdfs:comment     "A custom property with a value range. (see KBLFRM-319)\n"@en;
        rdfs:label       "ValueRangeProperty"@en;
        rdfs:subClassOf  vec:CustomProperty .

vec:SignalTransmissionMediumType
        rdf:type         owl:Class;
        rdfs:label       "SignalTransmissionMediumType"@en;
        rdfs:subClassOf  vec:OpenEnumeration .

vec:LanguageCode_Sd  rdf:type  vec:LanguageCode , owl:NamedIndividiual;
        vec:enumLiteral  "Sd" .

vec:WireReceptionType_Crimp
        rdf:type         vec:WireReceptionType , owl:NamedIndividiual;
        vec:enumLiteral  "Crimp" .

vec:usageConstraintUsageNode
        rdf:type      owl:ObjectProperty;
        rdfs:comment  "References the UsageNode to which the UsageConstraint applies. This means the described PartVersion is allowed / denied in the referenced UsageNode.\n"@en;
        rdfs:domain   vec:UsageConstraint;
        rdfs:label    "usageNode"@en;
        rdfs:range    vec:UsageNode .

vec:SignalSubType_IEEE802.11
        rdf:type         vec:SignalSubType , owl:NamedIndividiual;
        rdfs:comment     "also: Wi-Fi, Wireless LAN"@en;
        vec:enumLiteral  "IEEE802.11" .

vec:networkNodeSubType
        rdf:type            owl:ObjectProperty;
        rdfs:comment        "Specifies the sub type of a NetworkNode. The sub type allows a differentiation within a specific type. E.g. an actuator can be differentiated into lamps, speakers, motors.\n"@en;
        rdfs:domain         vec:NetworkNode;
        rdfs:label          "subType"@en;
        rdfs:range          vec:NetworkNodeSubType;
        rdfs:subPropertyOf  vec:contains .

vec:topologySpecificationTopologySegment
        rdf:type            owl:ObjectProperty;
        rdfs:comment        "Specifies the TopologySegments defined by the TopologySpecification.\n"@en;
        rdfs:domain         vec:TopologySpecification;
        rdfs:label          "topologySegment"@en;
        rdfs:range          vec:TopologySegment;
        rdfs:subPropertyOf  vec:contains .

vec:ComponentNodeSubType
        rdf:type         owl:Class;
        rdfs:comment     "Defines agreed values for ComponentNodeSubTypes . Not all combinations of ComponentNodeSubTypes and ComponentNodeTypes are semantically correct (e.g.┬áLamp, Microphone, Speaker, Motor are all Actuators).\n"@en;
        rdfs:label       "ComponentNodeSubType"@en;
        rdfs:subClassOf  vec:OpenEnumeration .

vec:OpenWireEndTerminalRole
        rdf:type         owl:Class;
        rdfs:comment     "An OpenWireEndTerminalRole defines the instance specific properties and relationships of an open wire end.\n"@en;
        rdfs:label       "OpenWireEndTerminalRole"@en;
        rdfs:subClassOf  vec:TerminalRole .

vec:connectorHousingRoleComponentConnector
        rdf:type      owl:ObjectProperty;
        rdfs:comment  "References the ComponentConnector that is realized by the referenced ConnectorHousing (OccurrenceOrUsage with ConnectorHousingRole). This can especially be relevant for inliners. KBLFRM-341.\n"@en;
        rdfs:domain   vec:ConnectorHousingRole;
        rdfs:label    "componentConnector"@en;
        rdfs:range    vec:ComponentConnector .

vec:CavityAccessoryRole
        rdf:type         owl:Class;
        rdfs:comment     "A CavityAccessoryRole defines the instance specific properties and relationships of a cavity accessory.\n"@en;
        rdfs:label       "CavityAccessoryRole"@en;
        rdfs:subClassOf  vec:Role .

<http://www.prostep.org/ontologies/ecad/2024/03/vec#RobustnessClassReferenceSystem_LV%20214>
        rdf:type         vec:RobustnessClassReferenceSystem , owl:NamedIndividiual;
        rdfs:comment     "OEM┬áConnector Test Specification\n"@en;
        vec:enumLiteral  "LV 214" .

vec:PinCurrentType  rdf:type  owl:Class;
        rdfs:comment     "Defines the different available current types of a pin.\n"@en;
        rdfs:label       "PinCurrentType"@en;
        rdfs:subClassOf  vec:OpenEnumeration .

vec:networkNodeDescription
        rdf:type            owl:ObjectProperty;
        rdfs:comment        "Room for additional, human readable information about the NetworkNode.\n"@en;
        rdfs:domain         vec:NetworkNode;
        rdfs:label          "description"@en;
        rdfs:range          vec:AbstractLocalizedString;
        rdfs:subPropertyOf  vec:contains .

<http://www.prostep.org/ontologies/ecad/2024/03/vec#RobustnessClassReferenceSystem_ISO%2020653>
        rdf:type         vec:RobustnessClassReferenceSystem , owl:NamedIndividiual;
        rdfs:comment     "The literal that shall be used for the ISO 20653 \"Road vehicles - Degrees of protection┬á(IP code) - Protection of electrical equipment against foreign objects, water and access\".\n"@en;
        vec:enumLiteral  "ISO 20653" .

vec:abstractLocalizedStringValue
        rdf:type      owl:DatatypeProperty;
        rdfs:comment  "The value of the LocalizedString in language defined by the languageCode.\n"@en;
        rdfs:domain   vec:AbstractLocalizedString;
        rdfs:label    "value"@en;
        rdfs:range    xs:string .

vec:SegmentCrossSectionAreaType_Real
        rdf:type         vec:SegmentCrossSectionAreaType , owl:NamedIndividiual;
        rdfs:comment     " Real is the type for cross section areas that can be observed for TopologySegments with variants of a Harness that are producible.\n"@en;
        vec:enumLiteral  "Real" .

vec:terminalRoleComponentPort
        rdf:type      owl:ObjectProperty;
        rdfs:comment  "References the ComponentPort that is realized by the referenced Terminal (OccurrenceOrUsage with TerminalRole).\nKBLFRM-341\n"@en;
        rdfs:domain   vec:TerminalRole;
        rdfs:label    "componentPort"@en;
        rdfs:range    vec:ComponentPort .

vec:PinOpticalInformation
        rdf:type      owl:Class;
        rdfs:comment  "Allows the specification of optical information in a PinComponentBehavior.\n"@en;
        rdfs:label    "PinOpticalInformation"@en .

vec:CableLeadThroughType_SealingGlue
        rdf:type         vec:CableLeadThroughType , owl:NamedIndividiual;
        vec:enumLiteral  "SealingGlue" .

vec:occurrenceOrUsageRealizedUsageNode
        rdf:type      owl:ObjectProperty;
        rdfs:comment  "References the UsageNode that is realized by this OccurrenceOrUsage .\n"@en;
        rdfs:domain   vec:OccurrenceOrUsage;
        rdfs:label    "realizedUsageNode"@en;
        rdfs:range    vec:UsageNode .

vec:Ordered  rdf:type  owl:Class;
        rdfs:comment  "Class of elements that are ordered within their containment."@en;
        rdfs:label    "Ordered"@en .

vec:ComponentNodeType_Generator
        rdf:type         vec:ComponentNodeType , owl:NamedIndividiual;
        rdfs:comment     "A device that can generate energy.\n"@en;
        vec:enumLiteral  "Generator" .

vec:PinCurrentType_MaxCurrent
        rdf:type         vec:PinCurrentType , owl:NamedIndividiual;
        vec:enumLiteral  "maxCurrent" .

vec:buildingBlockSpecification2DGeometryNode
        rdf:type            owl:ObjectProperty;
        rdfs:comment        "Specifies the GeometryNode2Ds defined by the BuildingBlockSpecification2D.\n"@en;
        rdfs:domain         vec:BuildingBlockSpecification2D;
        rdfs:label          "geometryNode"@en;
        rdfs:range          vec:GeometryNode2D;
        rdfs:subPropertyOf  vec:contains .

vec:flatCoreSpecificationSize
        rdf:type            owl:ObjectProperty;
        rdfs:comment        "Defines the size (width &┬áheight) of the flat core.\n"@en;
        rdfs:domain         vec:FlatCoreSpecification;
        rdfs:label          "size"@en;
        rdfs:range          vec:Size;
        rdfs:subPropertyOf  vec:contains .

vec:RoutableElement  rdf:type  owl:Class;
        rdfs:comment     "A RoutableElement is an element that can be routed, which mean it is possible to assign it to a Path in the Topology.\n"@en;
        rdfs:label       "RoutableElement"@en;
        rdfs:subClassOf  vec:ConfigurableElement .

vec:MultiFuseSpecification
        rdf:type         owl:Class;
        rdfs:label       "MultiFuseSpecification"@en;
        rdfs:subClassOf  vec:EEComponentSpecification .

vec:LevelOfApproval_Free
        rdf:type         vec:LevelOfApproval , owl:NamedIndividiual;
        rdfs:comment     "The ItemVersion can be used without restriction.\n"@en;
        vec:enumLiteral  "Free" .

vec:extensionSlotAllowedInserts
        rdf:type      owl:ObjectProperty;
        rdfs:comment  "References the PartRelations that are valid inserts for this ExtensionSlot.\nThis reference points to PartRelations in order to allow referencing indirectly a PartVersion if the description of individual PartVersions is done with one physical VEC file per PartVersion and to allow the expression of optional inserts, choices etc. However, inserts for an ExtensionSlot are always EEComponents by itself. Therefore, the referenced PartVersion shall have a PrimaryPartType =┬áEEComponent.\n"@en;
        rdfs:domain   vec:ExtensionSlot;
        rdfs:label    "allowedInserts"@en;
        rdfs:range    vec:PartRelation .

vec:requirementsConformanceSpecificationConformanceStatement
        rdf:type            owl:ObjectProperty;
        rdfs:domain         vec:RequirementsConformanceSpecification;
        rdfs:label          "conformanceStatement"@en;
        rdfs:range          vec:RequirementsConformanceStatement;
        rdfs:subPropertyOf  vec:contains .

vec:wireReceptionAddOnWireAddOn
        rdf:type            owl:ObjectProperty;
        rdfs:comment        "Specifies the wire length add on needed for the wire reception.\n"@en;
        rdfs:domain         vec:WireReceptionAddOn;
        rdfs:label          "wireAddOn"@en;
        rdfs:range          vec:NumericalValue;
        rdfs:subPropertyOf  vec:contains .

[ rdf:type     owl:AllDisjointClasses;
  owl:members  ( vec:WireElementReference vec:Connection )
] .

vec:labelingSpecificationLabelType
        rdf:type            owl:ObjectProperty;
        rdfs:comment        "Specifies the type of a label printed, stamped or integrated on or in component (e.g. alpha numerical, bar code).\n"@en;
        rdfs:domain         vec:LabelingSpecification;
        rdfs:label          "labelType"@en;
        rdfs:range          vec:LabelType;
        rdfs:subPropertyOf  vec:contains .

vec:PluggableTerminalSpecification
        rdf:type         owl:Class;
        rdfs:comment     "Specification for the definition of pluggable terminals.\n"@en;
        rdfs:label       "PluggableTerminalSpecification"@en;
        rdfs:subClassOf  vec:TerminalSpecification .

vec:NetworkNodeSubType_Microphone
        rdf:type         vec:NetworkNodeSubType , owl:NamedIndividiual;
        vec:enumLiteral  "Microphone" .

vec:contactPointIdentification
        rdf:type      owl:DatatypeProperty;
        rdfs:comment  "Specifies a unique identification of the ContactPoint. The identification is guaranteed to be unique within the ContactingSpecification.\n"@en;
        rdfs:domain   vec:ContactPoint;
        rdfs:label    "identification"@en;
        rdfs:range    xs:string .

vec:CustomUnit  rdf:type  owl:Class;
        rdfs:comment     "A CustomUnit can be used to define \"FreeText\"-Units. Custom units must not be used for units that can be expressed by any of the other subclasses of Unit. Custom units are only allowed if a unit is needed that cannot be handled by any of the other classes.\n"@en;
        rdfs:label       "CustomUnit"@en;
        rdfs:subClassOf  vec:Unit .

vec:CavityCoupling  rdf:type  owl:Class;
        rdfs:comment     "A CavityCoupling defines the mapping between two cavities of the ConnectorHousingRoles associated with the CouplingPoint .\n"@en;
        rdfs:label       "CavityCoupling"@en;
        rdfs:subClassOf  vec:ConfigurableElement .

vec:wireReceptionSpecificationConnectionBLength
        rdf:type            owl:ObjectProperty;
        rdfs:comment        "Specifies the length of the connection between the conductor and the insulation crimp (wire reception, see diagram \"Terminal Dimensions\").\n"@en;
        rdfs:domain         vec:WireReceptionSpecification;
        rdfs:label          "connectionBLength"@en;
        rdfs:range          vec:NumericalValue;
        rdfs:subPropertyOf  vec:contains .

vec:numericalValuePropertyValue
        rdf:type            owl:ObjectProperty;
        rdfs:comment        "Defines the value of the CustomProperty.\n"@en;
        rdfs:domain         vec:NumericalValueProperty;
        rdfs:label          "value"@en;
        rdfs:range          vec:NumericalValue;
        rdfs:subPropertyOf  vec:contains .

vec:UsageNode  rdf:type  owl:Class;
        rdfs:comment     "A UsageNode represents a position in an abstract vehicle. For example, the \"Head Light Left\". UsageNodes belong to the master data and they are defined on some companywide level. They can be used to enforce consistent naming over different projects and different development streams (e.g. between Geometry and Electrologic).\nA UsageNode can be realized by different elements in the VEC (e.g. NetworkNode, OccurrenceOrUsage, TopologyNode, ComponentNode ).\n"@en;
        rdfs:label       "UsageNode"@en;
        rdfs:subClassOf  vec:ConfigurableElement .

vec:shieldSpecificationOpticalTissueDensity
        rdf:type            owl:ObjectProperty;
        rdfs:comment        "Defines the optical tissue density of the strands of a shield. This is defined as a value in percentage. Should only be used for ShieldSpecifications with type=Braided.\n┬á\n"@en;
        rdfs:domain         vec:ShieldSpecification;
        rdfs:label          "opticalTissueDensity"@en;
        rdfs:range          vec:NumericalValue;
        rdfs:subPropertyOf  vec:contains .

vec:cavityPartSpecificationGeometry
        rdf:type            owl:ObjectProperty;
        rdfs:comment        "Defines the geometry of the cavity sealing.\n┬á\nThis attribute is defined as an OpenEnumeration.\n"@en;
        rdfs:domain         vec:CavityPartSpecification;
        rdfs:label          "geometry"@en;
        rdfs:range          vec:SealingGeometry;
        rdfs:subPropertyOf  vec:contains .

vec:LanguageCode_Si  rdf:type  vec:LanguageCode , owl:NamedIndividiual;
        vec:enumLiteral  "Si" .

vec:spliceTerminalRoleSpliceType
        rdf:type            owl:ObjectProperty;
        rdfs:comment        "Specifies the type of splice (inline, end).\n"@en;
        rdfs:domain         vec:SpliceTerminalRole;
        rdfs:label          "spliceType"@en;
        rdfs:range          vec:SpliceType;
        rdfs:subPropertyOf  vec:contains .

vec:pinVoltageInformationType
        rdf:type            owl:ObjectProperty;
        rdfs:comment        "Defines the type of the voltage.\n"@en;
        rdfs:domain         vec:PinVoltageInformation;
        rdfs:label          "type"@en;
        rdfs:range          vec:PinVoltageType;
        rdfs:subPropertyOf  vec:contains .

vec:SiUnitName_Metre  rdf:type  vec:SiUnitName , owl:NamedIndividiual;
        vec:enumLiteral  "Metre" .

vec:SignalSubType_MOST
        rdf:type         vec:SignalSubType , owl:NamedIndividiual;
        vec:enumLiteral  "MOST" .

vec:LanguageCode_El  rdf:type  vec:LanguageCode , owl:NamedIndividiual;
        vec:enumLiteral  "El" .

vec:GrommetType_LeadThrough
        rdf:type         vec:GrommetType , owl:NamedIndividiual;
        vec:enumLiteral  "LeadThrough" .

vec:LocalizedTypedStringType_SupplementaryTitle
        rdf:type         vec:LocalizedTypedStringType , owl:NamedIndividiual;
        rdfs:comment     "The LocalizedTypedString represents a SupplementaryTitle in accordance to ISO 7200.\n"@en;
        vec:enumLiteral  "SupplementaryTitle" .

vec:wireTypeType  rdf:type  owl:DatatypeProperty;
        rdfs:comment  "Specifies the type of the wire (e.g. FLRY, NYFAZw). Valid values are defined by the wireTypeReferenceSystem.\n"@en;
        rdfs:domain   vec:WireType;
        rdfs:label    "type"@en;
        rdfs:range    xs:string .

vec:LanguageCode_Mk  rdf:type  vec:LanguageCode , owl:NamedIndividiual;
        vec:enumLiteral  "Mk" .

vec:assignmentGroupSpecificationAssignmentGroup
        rdf:type            owl:ObjectProperty;
        rdfs:comment        "Contains the AssignmentGroups that are defined by this AssignmentGroupSpecification.\n"@en;
        rdfs:domain         vec:AssignmentGroupSpecification;
        rdfs:label          "assignmentGroup"@en;
        rdfs:range          vec:AssignmentGroup;
        rdfs:subPropertyOf  vec:contains .

vec:configurationConstraintIdentification
        rdf:type      owl:DatatypeProperty;
        rdfs:comment  "Specifies a unique identification of the ConfigurationConstraint . The identification is guaranteed to be unique within the ConfigurableElement and does not change over the time.\n"@en;
        rdfs:domain   vec:ConfigurationConstraint;
        rdfs:label    "identification"@en;
        rdfs:range    xs:string .

vec:PluggableTerminalType_Coax
        rdf:type         vec:PluggableTerminalType , owl:NamedIndividiual;
        vec:enumLiteral  "Coax" .

vec:externalMappingSpecificationMappedDocument
        rdf:type      owl:ObjectProperty;
        rdfs:comment  "Reference to the DocumentVersion that represents the external data source that connected to the VEC content by the ExternalMappingSpecification .\n"@en;
        rdfs:domain   vec:ExternalMappingSpecification;
        rdfs:label    "mappedDocument"@en;
        rdfs:range    vec:DocumentVersion .

vec:networkNodeNetworkNodeType
        rdf:type            owl:ObjectProperty;
        rdfs:comment        "Specifies the type of a NetworkNode. Common values are agreed as an OpenEnumeration .\n"@en;
        rdfs:domain         vec:NetworkNode;
        rdfs:label          "networkNodeType"@en;
        rdfs:range          vec:NetworkNodeType;
        rdfs:subPropertyOf  vec:contains .

vec:WindingType_Longitudinal
        rdf:type         vec:WindingType , owl:NamedIndividiual;
        rdfs:comment     " Longitudinal defines a taping with where the tape is folded around a segment.\n"@en;
        vec:enumLiteral  "Longitudinal" .

vec:applicationConstraintToEffectivityControlKey
        rdf:type      owl:DatatypeProperty;
        rdfs:comment  "See FromEffectivityControlKey.\n"@en;
        rdfs:domain   vec:ApplicationConstraint;
        rdfs:label    "toEffectivityControlKey"@en;
        rdfs:range    xs:string .

vec:WireReceptionType
        rdf:type         owl:Class;
        rdfs:comment     "The WireReceptionType defines in an OpenEnumeration how a wire is joined with a wire reception.\n"@en;
        rdfs:label       "WireReceptionType"@en;
        rdfs:subClassOf  vec:OpenEnumeration .

vec:SlotLayoutType_Fakra
        rdf:type         vec:SlotLayoutType , owl:NamedIndividiual;
        rdfs:comment     "Fakra (ISO-20860)"@en;
        vec:enumLiteral  "Fakra" .

vec:ChangeDescription
        rdf:type         owl:Class;
        rdfs:comment     "A ChangeDescription describes the implemented issues that are reason for the aggregating ItemVersion to be either an initial or successor version. A ChangeDescription can optionally define the person who has approved the change.\n"@en;
        rdfs:label       "ChangeDescription"@en;
        rdfs:subClassOf  vec:ExtendableElement .

vec:CavityMounting  rdf:type  owl:Class;
        rdfs:comment     "A CavityMounting defines the cavities (CavityReference) where the contacted elements (Terminal) will be mounted.\n"@en;
        rdfs:label       "CavityMounting"@en;
        rdfs:subClassOf  vec:ExtendableElement .

vec:variantConfigurationSpecificationVariantConfiguration
        rdf:type            owl:ObjectProperty;
        rdfs:comment        "Specifies the individual VariantConfigurations defined in the VariantConfigurationSpecification.\n"@en;
        rdfs:domain         vec:VariantConfigurationSpecification;
        rdfs:label          "variantConfiguration"@en;
        rdfs:range          vec:VariantConfiguration;
        rdfs:subPropertyOf  vec:contains .

vec:componentNodeIdentification
        rdf:type      owl:DatatypeProperty;
        rdfs:comment  "Specifies a unique identification of the ComponentNode. The identification is guaranteed to be unique within the ConnectionSpecification.\n"@en;
        rdfs:domain   vec:ComponentNode;
        rdfs:label    "identification"@en;
        rdfs:range    xs:string .

vec:PrimaryPartType_Other
        rdf:type         vec:PrimaryPartType , owl:NamedIndividiual;
        vec:enumLiteral  "Other" .

vec:documentVersionRelatedDocument
        rdf:type      owl:ObjectProperty;
        rdfs:comment  "The association is an informative link which DocumentVersion are related to each other (e.g. by derivation, A Harness-Drawing is related to a 3D-Model). \n"@en;
        rdfs:domain   vec:DocumentVersion;
        rdfs:label    "relatedDocument"@en;
        rdfs:range    vec:DocumentVersion .

vec:HoleMountedFixingHoleType_Through
        rdf:type         vec:HoleMountedFixingHoleType , owl:NamedIndividiual;
        rdfs:comment     "The hole is in some kind metal sheet or simialar. The fixing is stuck through the hole and expands in some way on the other side to reach a fixation."@en;
        vec:enumLiteral  "Through" .

vec:networkNodeViewItemGridSquare
        rdf:type      owl:DatatypeProperty;
        rdfs:comment  "Specifies the grid square in which the NodeViewItem is placed (e.g. E/40).\n"@en;
        rdfs:domain   vec:NetworkNodeViewItem;
        rdfs:label    "gridSquare"@en;
        rdfs:range    xs:string .

vec:DocumentRelationType_RequirementsLink
        rdf:type         vec:DocumentRelationType , owl:NamedIndividiual;
        vec:enumLiteral  "RequirementsLink" .

vec:Net  rdf:type        owl:Class;
        rdfs:comment     "A Net is an undirected link between NetworkPorts .┬áIt defines that the NetworkPorts are related to each other with the Net .\nA Net is normally an instance of a NetType. ┬áE.g. if \"CAN-BUS\" is defined as a NetType typical Nets would be \"BODY-CAN\", \"AUDIO-CAN\".\n"@en;
        rdfs:label       "Net"@en;
        rdfs:subClassOf  vec:ConfigurableElement .

vec:wireMountingDetailReferencedWireEnd
        rdf:type      owl:ObjectProperty;
        rdfs:comment  "References the WireEnds that are mounted to referenced WireReception. A cardinality of more than one is allowed in order support parallel connectors, where multiple wire ends are placed on one side of the connector (one wire reception) and the other wire ends are placed on the other side of the connector (the other wire reception).\n"@en;
        rdfs:domain   vec:WireMountingDetail;
        rdfs:label    "referencedWireEnd"@en;
        rdfs:range    vec:WireEnd .

vec:labelingRoleLabelingTechnology
        rdf:type            owl:ObjectProperty;
        rdfs:comment        "Specifies the used labeling technology."@en;
        rdfs:domain         vec:LabelingRole;
        rdfs:label          "labelingTechnology"@en;
        rdfs:range          vec:LabelingTechnology;
        rdfs:subPropertyOf  vec:contains .

vec:BaselineState  rdf:type  owl:Class;
        rdfs:comment     "Enumeration the define the valid states of a baseline.\n"@en;
        rdfs:label       "BaselineState"@en;
        rdfs:subClassOf  vec:OpenEnumeration .

vec:LanguageCode_In  rdf:type  vec:LanguageCode , owl:NamedIndividiual;
        vec:enumLiteral  "In" .

vec:cavityCavitySpecification
        rdf:type      owl:ObjectProperty;
        rdfs:comment  "References the CavitySpecification that is satisfied by the cavity.\n"@en;
        rdfs:domain   vec:Cavity;
        rdfs:label    "cavitySpecification"@en;
        rdfs:range    vec:CavitySpecification .

vec:holeMountedFixingSpecificationHoleShape
        rdf:type            owl:ObjectProperty;
        rdfs:comment        "Specifies the shape of the hole in horizontal direction┬á(the plain on which the fixing is fixated)."@en;
        rdfs:domain         vec:HoleMountedFixingSpecification;
        rdfs:label          "holeShape"@en;
        rdfs:range          vec:HoleMountedFixingHoleShape;
        rdfs:subPropertyOf  vec:contains .

vec:NodeType_Inliner  rdf:type  vec:NodeType , owl:NamedIndividiual;
        rdfs:comment     "An Inliner is a TopologyNode where one section of the electrical system is connected to another section.\n"@en;
        vec:enumLiteral  "Inliner" .

vec:ComponentNodeType_Sensor
        rdf:type         vec:ComponentNodeType , owl:NamedIndividiual;
        rdfs:comment     "A sensor is a device that detects changes to the environment and sends them as information to other devices (e.g. an ECU).\n"@en;
        vec:enumLiteral  "Sensor" .

vec:geometrySegment2DEndVector
        rdf:type            owl:ObjectProperty;
        rdfs:comment        "Specifies the end vector of the geometry segment. The end vector is a tangent to the segment at the end position.\n"@en;
        rdfs:domain         vec:GeometrySegment2D;
        rdfs:label          "endVector"@en;
        rdfs:range          vec:CartesianVector2D;
        rdfs:subPropertyOf  vec:contains .

vec:LocalGeometrySpecification
        rdf:type         owl:Class;
        rdfs:comment     "A LocalGeometrySpecification is responsible to create a relationship between the 3D model of a component (e.g. a connector, a cable duct or a fixing)┬áand entities of the VEC. The 'Local' in the name refers to the fact that all definitions within this specification are 'local' to the 3D model of a specific component (a component in a library, not in a specific usage).\nSpecifically, it defines a transformation to transform the BoundingBox of a component into to coordinate system of the component and it defines the positions of Placement- and MeasurementPoints in this coordinate system.\n"@en;
        rdfs:label       "LocalGeometrySpecification"@en;
        rdfs:subClassOf  vec:PartOrUsageRelatedSpecification .

vec:fuseComponentConnectedPins
        rdf:type     owl:ObjectProperty;
        rdfs:domain  vec:FuseComponent;
        rdfs:label   "connectedPins"@en;
        rdfs:range   vec:PinComponent .

vec:nURBSControlPointWeight
        rdf:type      owl:DatatypeProperty;
        rdfs:comment  "┬áThe weight of the NURBSControlPoint.\n"@en;
        rdfs:domain   vec:NURBSControlPoint;
        rdfs:label    "weight"@en;
        rdfs:range    xs:double .

vec:LanguageCode_Ko  rdf:type  vec:LanguageCode , owl:NamedIndividiual;
        vec:enumLiteral  "Ko" .

vec:functionalRequirementValue
        rdf:type      owl:DatatypeProperty;
        rdfs:comment  "The value that represents the functional requirement (e.g. ASIL┬áD).\n┬á\n"@en;
        rdfs:domain   vec:FunctionalRequirement;
        rdfs:label    "value"@en;
        rdfs:range    xs:string .

vec:TerminalSealingType_Neutral
        rdf:type         vec:TerminalSealingType , owl:NamedIndividiual;
        rdfs:comment     "The terminal can be sealed (with a cavity seal), but a seal is not mandatory for this terminal.\n"@en;
        vec:enumLiteral  "Neutral" .

vec:terminalPairingUnmatingForce
        rdf:type            owl:ObjectProperty;
        rdfs:comment        "Specifies the force required to unmate the two terminals.\n"@en;
        rdfs:domain         vec:TerminalPairing;
        rdfs:label          "unmatingForce"@en;
        rdfs:range          vec:NumericalValue;
        rdfs:subPropertyOf  vec:contains .

vec:UsageConstraintType
        rdf:type             owl:Class;
        rdfs:comment         "Enumeration for the definition of the type of a UsageConstraint. Valid values are allow and deny.\n"@en;
        rdfs:label           "UsageConstraintType"@en;
        rdfs:subClassOf      vec:ClosedEnumeration;
        owl:equivalentClass  [ rdf:type   owl:Class;
                               owl:oneOf  ( vec:UsageConstraintType_Allow vec:UsageConstraintType_Deny )
                             ] .

vec:LanguageCode_Sn  rdf:type  vec:LanguageCode , owl:NamedIndividiual;
        vec:enumLiteral  "Sn" .

vec:VecVersion_1.2.0  rdf:type  vec:VecVersion , owl:NamedIndividiual;
        vec:enumLiteral  "1.2.0" .

vec:aliasIdentificationScope
        rdf:type      owl:DatatypeProperty;
        rdfs:comment  "The scope in which the AliasIdentification is valid /┬áor the issuer of the alias id. This could be for example a certain process, a company or an IT-System.\n"@en;
        rdfs:domain   vec:AliasIdentification;
        rdfs:label    "scope"@en;
        rdfs:range    xs:string .

vec:signalIdentification
        rdf:type      owl:DatatypeProperty;
        rdfs:comment  "Specifies a unique identification of the Signal. The identification is guaranteed to be unique within the SignalSpecification.\n"@en;
        rdfs:domain   vec:Signal;
        rdfs:label    "identification"@en;
        rdfs:range    xs:string .

<http://www.prostep.org/ontologies/ecad/2024/03/vec#RobustnessClassReferenceSystem_ISO%206722>
        rdf:type         vec:RobustnessClassReferenceSystem , owl:NamedIndividiual;
        rdfs:comment     "The literal that shall be used for the ISO 6722 \"Road vehicles -- 60 V and 600 V single-core cables\".\n"@en;
        vec:enumLiteral  "ISO 6722" .

vec:StatusOfApproval  rdf:type  owl:Class;
        rdfs:comment     "Enumeration for the definition of the state of an approval.\n"@en;
        rdfs:label       "StatusOfApproval"@en;
        rdfs:subClassOf  vec:OpenEnumeration .

vec:componentNodeSubType
        rdf:type            owl:ObjectProperty;
        rdfs:comment        "Specifies the sub type of a ComponentNode. The sub type allows a differentiation within a specific type. E.g. an actuator can be differentiated into lamps, speakers, motors.┬á\n"@en;
        rdfs:domain         vec:ComponentNode;
        rdfs:label          "subType"@en;
        rdfs:range          vec:ComponentNodeSubType;
        rdfs:subPropertyOf  vec:contains .

vec:WindingType_Overlap
        rdf:type         vec:WindingType , owl:NamedIndividiual;
        rdfs:comment     " Overlap describes a taping where each round overlaps the preceeding round.\n"@en;
        vec:enumLiteral  "Overlap" .

vec:otherUnitOtherUnitName
        rdf:type            owl:ObjectProperty;
        rdfs:comment        "Specifies the name of the unit.\n"@en;
        rdfs:domain         vec:OtherUnit;
        rdfs:label          "otherUnitName"@en;
        rdfs:range          vec:OtherUnitName;
        rdfs:subPropertyOf  vec:contains .

vec:PinTimingType_StartStopTime
        rdf:type         vec:PinTimingType , owl:NamedIndividiual;
        vec:enumLiteral  "startStopTime" .

vec:SegmentForm_NonCircular
        rdf:type         vec:SegmentForm , owl:NamedIndividiual;
        vec:enumLiteral  "NonCircular" .

vec:geometryNode2DCartesianPoint
        rdf:type      owl:ObjectProperty;
        rdfs:comment  "References the CartesianPoint2D where the GeometryNode2D is located. \n"@en;
        rdfs:domain   vec:GeometryNode2D;
        rdfs:label    "cartesianPoint"@en;
        rdfs:range    vec:CartesianPoint2D .

vec:CableDuctRole  rdf:type  owl:Class;
        rdfs:comment     "A CableDuctRole defines the instance specific properties and relationships of a cable duct.\n"@en;
        rdfs:label       "CableDuctRole"@en;
        rdfs:subClassOf  vec:Role .

vec:wireMountingMountedCavitySeal
        rdf:type      owl:ObjectProperty;
        rdfs:comment  "References the cavity seal that is used for the wire mounting.\n"@en;
        rdfs:domain   vec:WireMounting;
        rdfs:label    "mountedCavitySeal"@en;
        rdfs:range    vec:CavitySealRole .

[ rdf:type     owl:AllDisjointClasses;
  owl:members  ( vec:NURBSCurve )
] .

vec:Tolerance  rdf:type  owl:Class;
        rdfs:comment     "Enables the specification of value ranges which can be tolerated.\n"@en;
        rdfs:label       "Tolerance"@en;
        rdfs:subClassOf  vec:ExtendableElement .

vec:cableTieSpecificationThickness
        rdf:type            owl:ObjectProperty;
        rdfs:domain         vec:CableTieSpecification;
        rdfs:label          "thickness"@en;
        rdfs:range          vec:NumericalValue;
        rdfs:subPropertyOf  vec:contains .

vec:CavityMapping  rdf:type  owl:Class;
        rdfs:comment  "Defines the mapping of two cavities contained Slot A & B of the containing SlotMapping-object.\n"@en;
        rdfs:label    "CavityMapping"@en .

vec:projectCarClassificationLevel3
        rdf:type      owl:DatatypeProperty;
        rdfs:comment  "Provides a classification according to \"CC8 Recommended Practices Specification and Configuration, Product Structures\". Car classification is the identification of a set of similar cars to be offered to the market. Level 3 stands for \"Configuration information / product family\" where all variant control mechanisms are attached.\n"@en;
        rdfs:domain   vec:Project;
        rdfs:label    "carClassificationLevel3"@en;
        rdfs:range    xs:string .

vec:wireElementSpecificationFillerSpecification
        rdf:type      owl:ObjectProperty;
        rdfs:comment  "If the WireElement is a filler then the specification of the filler is referenced here.\n"@en;
        rdfs:domain   vec:WireElementSpecification;
        rdfs:label    "fillerSpecification"@en;
        rdfs:range    vec:FillerSpecification .

vec:componentNodeNetworkNode
        rdf:type      owl:ObjectProperty;
        rdfs:comment  "References the NetworkNode that is realized by the ComponentNode.\n"@en;
        rdfs:domain   vec:ComponentNode;
        rdfs:label    "networkNode"@en;
        rdfs:range    vec:NetworkNode .

vec:SiPrefix_Femto  rdf:type  vec:SiPrefix , owl:NamedIndividiual;
        vec:enumLiteral  "Femto" .

vec:USUnitName_HundredWeight
        rdf:type         vec:USUnitName , owl:NamedIndividiual;
        vec:enumLiteral  "HundredWeight" .

vec:geometrySegment3DCurve
        rdf:type            owl:ObjectProperty;
        rdfs:comment        "Specifies an ordered list of curves which describe the centerline of the segment. If a segment is described by more than one curve, the centrelines of the individual curves are aligned in the order of this association.\n"@en;
        rdfs:domain         vec:GeometrySegment3D;
        rdfs:label          "curve"@en;
        rdfs:range          vec:Curve3D , vec:Ordered;
        rdfs:subPropertyOf  vec:contains .

vec:CustomProperty  rdf:type  owl:Class;
        rdfs:comment  "Abstract base class for custom properties. Basically, a custom property is key / value pair. The key (propertyType) defines the meaning of the value. A custom property can either be a simple value (string), a numerical value or a value range.\n"@en;
        rdfs:label    "CustomProperty"@en .

vec:wireReceptionSpecificationFrontBellMouthLength
        rdf:type            owl:ObjectProperty;
        rdfs:comment        "Specifies the length of the front (facing the terminal reception) bell mouth of the conductor crimp (wire reception, see diagram \"Terminal Dimensions\").\n"@en;
        rdfs:domain         vec:WireReceptionSpecification;
        rdfs:label          "frontBellMouthLength"@en;
        rdfs:range          vec:NumericalValue;
        rdfs:subPropertyOf  vec:contains .

vec:PartRelation  rdf:type  owl:Class;
        rdfs:comment  "A PartRelation defines additional parts (e.g. accessories) for a specific part. These parts are in some way or usage scenario required for the part itself to be used. However, they are not included with the part number and have to ordered separately. This can be used for example for caps, cable ties etc.\nThe associated PartRelations of a GeneralTechnicalPartSpecification represent a configurable bill of material that can/must be ordered together with the part, when it is used. Each PartRelation represents an item /┬áline in this bill of material. The semantic by which a PartRelation is resolved to PartVersions is defined by the PartRelationType. If multiple PartRelations resolve to the same PartVersions the resulting bill of material is the sum of them.\nIf a PartRelation references more than one accessoryPart the PartRelationType defines the semantic to resolve this reference for a resulting bill of material. If the type is Mandatory all referenced PartVersions shall be in the resulting bill of material. If the type is Optional , the referenced PartVersions can be selected by choice into the resulting bill of material. However, the choice applies to all PartVersion s of one PartRelation. For Mandatory it is semantically equivalent to have one PartRelation referencing N PartVersions or to have N PartRelations , each referencing one PartVersion. The PartRelationType OneOfAll defines, that exactly one of the referenced PartVersions shall be chosen for the resulting bill of material.\nIf the same PartVersion is referenced multiple times, each reference counts as its own position. Example: To express that a PartVersion shall be used at least three times and with a maximum of 6 times, three mandatory and three optional PartRelations to this PartVersion would be created.\nWith these concepts, simple yes/no decisions can be represented. However, there cases where there are constraints between accessory parts (e.g. if part A, then choice of 2 x B┬áor 1 x C). To express such logic in a static object model is not very feasible and inflexible. For such cases, the relationType 'Custom' was introduced. In this case, the relationships and constraints between all referenced accessoryPart can be expressed with some custom expression language in the customRelationExpression attribute. Even if it is custom, the expression shall only refer to elements that are contained in the accessoryPart relation and shall not influence other PartRelations of the same GeneralTechnicalPartSpecification .\n┬á\n"@en;
        rdfs:label    "PartRelation"@en .

vec:LanguageCode_Is  rdf:type  vec:LanguageCode , owl:NamedIndividiual;
        vec:enumLiteral  "Is" .

vec:topologySegmentEndNode
        rdf:type      owl:ObjectProperty;
        rdfs:comment  "References the TopologyNode where the TopologySegment ends. \n"@en;
        rdfs:domain   vec:TopologySegment;
        rdfs:label    "endNode"@en;
        rdfs:range    vec:TopologyNode .

vec:functionalStructureSpecificationRootNode
        rdf:type            owl:ObjectProperty;
        rdfs:comment        ""@en;
        rdfs:domain         vec:FunctionalStructureSpecification;
        rdfs:label          "rootNode"@en;
        rdfs:range          vec:FunctionalStructureNode;
        rdfs:subPropertyOf  vec:contains .

vec:TerminalSealingType_None
        rdf:type         vec:TerminalSealingType , owl:NamedIndividiual;
        rdfs:comment     "The Terminal cannot be sealed by itself (e.g. a CavitySeal)\n"@en;
        vec:enumLiteral  "None" .

vec:ConnectionGroupType_Twisted
        rdf:type         vec:ConnectionGroupType , owl:NamedIndividiual;
        vec:enumLiteral  "Twisted" .

vec:conductorSpecificationStructure
        rdf:type            owl:ObjectProperty;
        rdfs:comment        "Specifies the structure of the conductor according to ISO 6722-1 for ConductorSpecifications with Type = Stranded. Should only be used for ConductorSpecifications with type=Stranded.\n┬á\n"@en;
        rdfs:domain         vec:ConductorSpecification;
        rdfs:label          "structure"@en;
        rdfs:range          vec:ConductorStructure;
        rdfs:subPropertyOf  vec:contains .

vec:SiUnitName_Sievert
        rdf:type         vec:SiUnitName , owl:NamedIndividiual;
        vec:enumLiteral  "Sievert" .

vec:VariantConfigurationType
        rdf:type         owl:Class;
        rdfs:comment     "Defines an OpenEnumeration for VariantConfigurationTypes. The configuration type defines in which \"variant code universe\" the logistic control expression is defined."@en;
        rdfs:label       "VariantConfigurationType"@en;
        rdfs:subClassOf  vec:OpenEnumeration .

vec:routingRoutedElement
        rdf:type      owl:ObjectProperty;
        rdfs:comment  "Specifies the Element that is routed. \n"@en;
        rdfs:domain   vec:Routing;
        rdfs:label    "routedElement"@en;
        rdfs:range    vec:RoutableElement .

vec:ImperialUnitName_Quart
        rdf:type         vec:ImperialUnitName , owl:NamedIndividiual;
        vec:enumLiteral  "Quart" .

vec:PinVoltageType  rdf:type  owl:Class;
        rdfs:comment     "Defines the different available voltage types of a pin.\n"@en;
        rdfs:label       "PinVoltageType"@en;
        rdfs:subClassOf  vec:OpenEnumeration .

vec:NURBSControlPoint
        rdf:type      owl:Class;
        rdfs:comment  "Represents a control point of a NURBSCurve. It consists of a referenced CartesianPoint3D for the position and a weight .\n"@en;
        rdfs:label    "NURBSControlPoint"@en .

vec:Approval  rdf:type   owl:Class;
        rdfs:comment     "Defines the approval of an ItemVersion. This consists of the StatusOfApproval and the Permissions issued for the approval.\n"@en;
        rdfs:label       "Approval"@en;
        rdfs:subClassOf  vec:ExtendableElement .

vec:geometrySegment3DStartNode
        rdf:type      owl:ObjectProperty;
        rdfs:comment  "References the GeometryNode3D where the GeometrySegment3D starts. \n"@en;
        rdfs:domain   vec:GeometrySegment3D;
        rdfs:label    "startNode"@en;
        rdfs:range    vec:GeometryNode3D .

vec:cavityMountingCavityAccessory
        rdf:type     owl:ObjectProperty;
        rdfs:domain  vec:CavityMounting;
        rdfs:label   "cavityAccessory"@en;
        rdfs:range   vec:CavityAccessoryRole .

vec:AnchorType_FromEndNode
        rdf:type         vec:AnchorType , owl:NamedIndividiual;
        rdfs:comment     "The offset of the location is measured from the endNode of the TopologySegment.\n"@en;
        vec:enumLiteral  "FromEndNode" .

vec:LanguageCode_Ss  rdf:type  vec:LanguageCode , owl:NamedIndividiual;
        vec:enumLiteral  "Ss" .

vec:functionalRequirementType
        rdf:type            owl:ObjectProperty;
        rdfs:comment        "The type defines to which category a requirement belongs (e.g. ┬áFunctional┬áSafety).\n"@en;
        rdfs:domain         vec:FunctionalRequirement;
        rdfs:label          "type"@en;
        rdfs:range          vec:FunctionalRequirementType;
        rdfs:subPropertyOf  vec:contains .

vec:SignalTransmissionMediumType_Inductive
        rdf:type         vec:SignalTransmissionMediumType , owl:NamedIndividiual;
        vec:enumLiteral  "inductive" .

vec:cableLeadThroughOutletPlacementPoint
        rdf:type      owl:ObjectProperty;
        rdfs:comment  "Specifies the PlacementPoint that represents this CableLeadThroughOutlet in a PlaceableElementSpecification.\n"@en;
        rdfs:domain   vec:CableLeadThroughOutlet;
        rdfs:label    "placementPoint"@en;
        rdfs:range    vec:PlacementPoint .

vec:terminalSpecificationInternalTerminalConnection
        rdf:type            owl:ObjectProperty;
        rdfs:comment        "Specifies the InternalTerminalConnections of the terminal. \n"@en;
        rdfs:domain         vec:TerminalSpecification;
        rdfs:label          "internalTerminalConnection"@en;
        rdfs:range          vec:InternalTerminalConnection;
        rdfs:subPropertyOf  vec:contains .

vec:buildingBlockSpecification3DTopologyZone
        rdf:type      owl:ObjectProperty;
        rdfs:comment  "References the Zone that is building block represents. This shall be a TopologyZone with the type \"DmuZone\".\n"@en;
        rdfs:domain   vec:BuildingBlockSpecification3D;
        rdfs:label    "topologyZone"@en;
        rdfs:range    vec:TopologyZone .

vec:locationIdentification
        rdf:type      owl:DatatypeProperty;
        rdfs:comment  "Specifies a unique identification of the Location. The identification is guaranteed to be unique within the PlacementSpecification.\n"@en;
        rdfs:domain   vec:Location;
        rdfs:label    "identification"@en;
        rdfs:range    xs:string .

vec:segmentLocationAnchor
        rdf:type            owl:ObjectProperty;
        rdfs:comment        "Specifies if the location on the TopologySegment is defined as on offset relative to the startNode of the TopologySegment or the endNode.\n"@en;
        rdfs:domain         vec:SegmentLocation;
        rdfs:label          "anchor"@en;
        rdfs:range          vec:AnchorType;
        rdfs:subPropertyOf  vec:contains .

vec:moduleListDescription
        rdf:type            owl:ObjectProperty;
        rdfs:comment        "Room for additional, human readable information about the ModuleList.\n"@en;
        rdfs:domain         vec:ModuleList;
        rdfs:label          "description"@en;
        rdfs:range          vec:AbstractLocalizedString;
        rdfs:subPropertyOf  vec:contains .

vec:corrugatedPipeSpecificationCorrugationGradient
        rdf:type            owl:ObjectProperty;
        rdfs:comment        "Specifies the gradient of a corrugation of the pipe.\n"@en;
        rdfs:domain         vec:CorrugatedPipeSpecification;
        rdfs:label          "corrugationGradient"@en;
        rdfs:range          vec:NumericalValue;
        rdfs:subPropertyOf  vec:contains .

vec:nURBSControlPointCartesianPoint3D
        rdf:type      owl:ObjectProperty;
        rdfs:comment  "The CartesionPoint3D that defines the position of this NURBSControlPoint. ┬á\n"@en;
        rdfs:domain   vec:NURBSControlPoint;
        rdfs:label    "cartesianPoint3D"@en;
        rdfs:range    vec:CartesianPoint3D .

vec:RobustnessProperties
        rdf:type      owl:Class;
        rdfs:comment  "Allows the definition of robustness properties. Robustness of component is specified as a level of robustness against a specific influence (e.g. oil, water, UV-light). The influence is specified by the class and the level is specified by the classKey . Valid robustness classes and keys are specified by the reference system. Attributes of the type RobustnessProperties normally have the multiplicity [0..*]. This means that such an attribute can have RobustnessProperties entries for different classReferenceSystems and classes . It must not have multiple entries for the same class and classReferenceSystem .\nNote: Most reference systems just define one class or at least some of the possible classes, but not all (e.g. the ISO 20653 defines \"Solid Particle Protection\" and \"Liquid┬áIngress┬áProtection\", whereas the ISO 6722 defines \"Ambient┬áTemperature\" among others).\n"@en;
        rdfs:label    "RobustnessProperties"@en .

vec:topologyNodeRealizedUsageNode
        rdf:type      owl:ObjectProperty;
        rdfs:comment  "References the UsageNode that is realized by this TopologyNode .\n"@en;
        rdfs:domain   vec:TopologyNode;
        rdfs:label    "realizedUsageNode"@en;
        rdfs:range    vec:UsageNode .

vec:pluggableTerminalSpecificationTerminalType
        rdf:type            owl:ObjectProperty;
        rdfs:comment        "Defines the type of the terminal. The type defines constraints about the numbers of wire and┬áterminal receptions and their relations.\n"@en;
        rdfs:domain         vec:PluggableTerminalSpecification;
        rdfs:label          "terminalType"@en;
        rdfs:range          vec:PluggableTerminalType;
        rdfs:subPropertyOf  vec:contains .

vec:PinVoltageType_StartStopVoltage
        rdf:type         vec:PinVoltageType , owl:NamedIndividiual;
        vec:enumLiteral  "startStopVoltage" .

vec:wireElementReferenceConnection
        rdf:type      owl:ObjectProperty;
        rdfs:comment  "References the Connection that is realized by the referenced WireElement (WireElementReference).\nKBLFRM-341\n"@en;
        rdfs:domain   vec:WireElementReference;
        rdfs:label    "connection"@en;
        rdfs:range    vec:Connection .

vec:partUsagePartSubstitution
        rdf:type     owl:ObjectProperty;
        rdfs:domain  vec:PartUsage;
        rdfs:label   "partSubstitution"@en;
        rdfs:range   vec:PartSubstitutionSpecification .

vec:cavityMappingIdentificationA
        rdf:type      owl:DatatypeProperty;
        rdfs:comment  "The identification of the Cavity on side A\n"@en;
        rdfs:domain   vec:CavityMapping;
        rdfs:label    "identificationA"@en;
        rdfs:range    xs:string .

vec:SpliceType  rdf:type  owl:Class;
        rdfs:comment     "Enumeration for the definition of type of splice.\n"@en;
        rdfs:label       "SpliceType"@en;
        rdfs:subClassOf  vec:OpenEnumeration .

vec:TapingDirection_FromStart
        rdf:type         vec:TapingDirection , owl:NamedIndividiual;
        vec:enumLiteral  "FromStart" .

vec:LanguageCode_Ay  rdf:type  vec:LanguageCode , owl:NamedIndividiual;
        vec:enumLiteral  "Ay" .

vec:SlotLayoutType_USBMiniA
        rdf:type         vec:SlotLayoutType , owl:NamedIndividiual;
        vec:enumLiteral  "USBMiniA" .

vec:BoltMountedFixingBoltShape
        rdf:type         owl:Class;
        rdfs:comment     "OpenEnumeration for the shapes of the bolts on which the fixing can be mounted.\n"@en;
        rdfs:label       "BoltMountedFixingBoltShape"@en;
        rdfs:subClassOf  vec:OpenEnumeration .

vec:PartNature  rdf:type  owl:Class;
        rdfs:comment     " OpenEnumeration that defines the nature of a PartVersion . The nature specifies how the PartVersion can be used in the different processes or the significance of the PartVersion in the process.\n"@en;
        rdfs:label       "PartNature"@en;
        rdfs:subClassOf  vec:OpenEnumeration .

vec:ModularSlotReference
        rdf:type         owl:Class;
        rdfs:comment     "A ModularSlotReference represents the usage of a ModularSlot in the context of PartUsage or PartOccurrence.\n"@en;
        rdfs:label       "ModularSlotReference"@en;
        rdfs:subClassOf  vec:AbstractSlotReference .

vec:PinTimingType_BlockTime
        rdf:type         vec:PinTimingType , owl:NamedIndividiual;
        vec:enumLiteral  "blockTime" .

vec:routingIdentification
        rdf:type      owl:DatatypeProperty;
        rdfs:comment  "Specifies a unique identification of the Routing. The identification is guaranteed to be unique within the RoutingSpecification.\n"@en;
        rdfs:domain   vec:Routing;
        rdfs:label    "identification"@en;
        rdfs:range    xs:string .

vec:IECPrefix_Exbi  rdf:type  vec:IECPrefix , owl:NamedIndividiual;
        vec:enumLiteral  "Exbi" .

vec:usageConstraintFromEffectivityControlKey
        rdf:type      owl:DatatypeProperty;
        rdfs:comment  "In the production logistics of complex products (like vehicles), the control of operation and cancellation dates of changes, features, components or the like is usually not carried out via concrete dates but via \"date keys\". These keys are then mapped in planning systems with concrete time specifications for certain plants or production steps. In the VEC┬áthese keys are called EffectivityControlKey.\nWith the FromEffectivityControlKey and To EffectivityControlKey a validity interval can be defined. If one of the two values is defined and the other is omitted, the meaning shall be \"unbounded\".\n"@en;
        rdfs:domain   vec:UsageConstraint;
        rdfs:label    "fromEffectivityControlKey"@en;
        rdfs:range    xs:string .

vec:wireReceptionSpecificationValidConductorMaterials
        rdf:type            owl:ObjectProperty;
        rdfs:comment        "Specifies the materials of a conductor, that are valid to use with this WireReceptionSpecification . This material shall be matched against the ConductorSpecification.material.\n"@en;
        rdfs:domain         vec:WireReceptionSpecification;
        rdfs:label          "validConductorMaterials"@en;
        rdfs:range          vec:ConductorMaterial;
        rdfs:subPropertyOf  vec:contains .

vec:topologyZoneSubZone
        rdf:type            owl:ObjectProperty;
        rdfs:comment        "Specifies the sub TopologyZones that are part the TopologyZone . All ZoneAssignments defined for subZones are automatically inherited by the parent zone.\n"@en;
        rdfs:domain         vec:TopologyZone;
        rdfs:label          "subZone"@en;
        rdfs:range          vec:TopologyZone;
        rdfs:subPropertyOf  vec:contains .

vec:TerminalSealingType_Moulded
        rdf:type         vec:TerminalSealingType , owl:NamedIndividiual;
        rdfs:comment     "The terminal can be used in a moulded slot.\n"@en;
        vec:enumLiteral  "Moulded" .

vec:segmentConnectionPointCavityAddOns
        rdf:type            owl:ObjectProperty;
        rdfs:domain         vec:SegmentConnectionPoint;
        rdfs:label          "cavityAddOns"@en;
        rdfs:range          vec:CavityAddOn;
        rdfs:subPropertyOf  vec:contains .

vec:partStructureSpecificationInBillOfMaterial
        rdf:type      owl:ObjectProperty;
        rdfs:comment  "References the PartOccurrences that are building the bill of material of a composite part.\n"@en;
        rdfs:domain   vec:PartStructureSpecification;
        rdfs:label    "inBillOfMaterial"@en;
        rdfs:range    vec:OccurrenceOrUsage .

vec:LanguageCode_Ky  rdf:type  vec:LanguageCode , owl:NamedIndividiual;
        vec:enumLiteral  "Ky" .

vec:cavitySpecificationCavityDesign
        rdf:type        owl:DatatypeProperty;
        rdfs:comment    ""@en , "Deprecated (since Version 1.1.4): This attribute has been marked as deprecated, as it has been replaced by the more meaningful mechanism with TerminalTypes.\n"@en;
        rdfs:domain     vec:CavitySpecification;
        rdfs:label      "cavityDesign"@en;
        rdfs:range      xs:string;
        owl:deprecated  true .

vec:locationMatchingId
        rdf:type      owl:DatatypeProperty;
        rdfs:comment  "Specifies an identification for matching the location with a reference point of component (e.g. a cable channel).\n"@en;
        rdfs:domain   vec:Location;
        rdfs:label    "matchingId"@en;
        rdfs:range    xs:string .

vec:ConductorStructure_MultiStrand
        rdf:type         vec:ConductorStructure , owl:NamedIndividiual;
        rdfs:comment     "Multi-Strand conductor structure in accordance with ISO 6722-1 (Type C)\n"@en;
        vec:enumLiteral  "MultiStrand" .

vec:internalTerminalConnectionIdentification
        rdf:type      owl:DatatypeProperty;
        rdfs:comment  "Specifies a unique identification of the InternalTerminalConnection. The identification is guaranteed to be unique within the TerminalSpecification (this might be for example an internal connection number).\n"@en;
        rdfs:domain   vec:InternalTerminalConnection;
        rdfs:label    "identification"@en;
        rdfs:range    xs:string .

vec:ConductorType_Braided
        rdf:type         vec:ConductorType , owl:NamedIndividiual;
        rdfs:comment     "Used for conductors that are made of multiple individual strands that are braided together┬á(often used for shields).\n"@en;
        vec:enumLiteral  "Braided" .

vec:ComponentPortViewItemSide_Bottom
        rdf:type         vec:ComponentPortViewItemSide , owl:NamedIndividiual;
        vec:enumLiteral  "Bottom" .

vec:CurrentType_ACOnePhase
        rdf:type         vec:CurrentType , owl:NamedIndividiual;
        vec:enumLiteral  "ACOnePhase" .

vec:pinComponentBehaviorVoltageInformation
        rdf:type            owl:ObjectProperty;
        rdfs:comment        "Specifies the voltage information of the PinComponent in this PinComponentBehavior . Since the voltage values of a pin can be defined for different types and times it is possible to define multiple PinVoltageInformations for a PinComponentBehavior .\n"@en;
        rdfs:domain         vec:PinComponentBehavior;
        rdfs:label          "voltageInformation"@en;
        rdfs:range          vec:PinVoltageInformation;
        rdfs:subPropertyOf  vec:contains .

vec:SiUnitName_Second
        rdf:type         vec:SiUnitName , owl:NamedIndividiual;
        vec:enumLiteral  "Second" .

vec:USUnitName_Furlong
        rdf:type         vec:USUnitName , owl:NamedIndividiual;
        vec:enumLiteral  "Furlong" .

vec:SlotLayoutType_USBMicroBSuperSpeed
        rdf:type         vec:SlotLayoutType , owl:NamedIndividiual;
        vec:enumLiteral  "USBMicroBSuperSpeed" .

vec:DocumentVersion  rdf:type  owl:Class;
        rdfs:comment     "The DocumentVersion is one of the two anchors for PDM information in the VEC. All technical information about a PartVersion is contained in one or more documents. The documents are containing the actual content of the VEC since all Specifications are an element of a document.\n"@en;
        rdfs:label       "DocumentVersion"@en;
        rdfs:subClassOf  vec:ItemVersion .

vec:SignalSubType_USB
        rdf:type         vec:SignalSubType , owl:NamedIndividiual;
        rdfs:comment     "Universal Serial┬áBus Version 1.X: The \"USB\" literal represents all USB 1.X Versions for USB 2.0 or USB 3.X the corresponding literals shall be used.\n"@en;
        vec:enumLiteral  "USB" .

vec:slotColorInformation
        rdf:type            owl:ObjectProperty;
        rdfs:comment        "Specifies the color of the slot.\n"@en;
        rdfs:domain         vec:Slot;
        rdfs:label          "colorInformation"@en;
        rdfs:range          vec:Color;
        rdfs:subPropertyOf  vec:contains .

vec:GrommetMountingType_Slit
        rdf:type         vec:GrommetMountingType , owl:NamedIndividiual;
        rdfs:comment     "The grommet has a longitudinal slit through which the wires can be inserted.\n"@en;
        vec:enumLiteral  "Slit" .

vec:modularSlotAllowedInserts
        rdf:type      owl:ObjectProperty;
        rdfs:comment  "References the PartRelations that are valid inserts for this ModularSlot.\nThis reference points to PartRelations in order to allow referencing indirectly a PartVersion if the description of individual PartVersions is done with one physical VEC file per PartVersion and to allow the expression of optional inserts, choices etc. However, inserts for a ModularSlot are always ConnectorHousings by itself. Therefore, the referenced PartVersion shall have a PrimaryPartType =┬áConnectorHousing\n"@en;
        rdfs:domain   vec:ModularSlot;
        rdfs:label    "allowedInserts"@en;
        rdfs:range    vec:PartRelation .

vec:UsageNodeType_Switch
        rdf:type         vec:UsageNodeType , owl:NamedIndividiual;
        vec:enumLiteral  "Switch" .

vec:CavitySpecification
        rdf:type         owl:Class;
        rdfs:comment     "Specification for the definition of cavities.\n"@en;
        rdfs:label       "CavitySpecification"@en;
        rdfs:subClassOf  vec:Specification .

vec:modularSlotAddOnWireAddOn
        rdf:type            owl:ObjectProperty;
        rdfs:comment        "Specifies the wire length add on needed for the modular slot.\n"@en;
        rdfs:domain         vec:ModularSlotAddOn;
        rdfs:label          "wireAddOn"@en;
        rdfs:range          vec:NumericalValue;
        rdfs:subPropertyOf  vec:contains .

vec:AssignmentGroupSpecification
        rdf:type         owl:Class;
        rdfs:comment     "Specification that contains AssignmentGroups .\n"@en;
        rdfs:label       "AssignmentGroupSpecification"@en;
        rdfs:subClassOf  vec:Specification .

vec:wireElementSpecificationSubWireElementSpecification
        rdf:type      owl:ObjectProperty;
        rdfs:comment  "Specifies the contained subWireElements if the WireElement has sub elements. If a WireElementSpecification contains the same WireElementSpecification multiple times, then it shall be referenced as often as it occurs in the reality. Otherwise the WireElementSpecification wouldn't specify a wire element unambiguously, because the representation in the model would be the same, regardless of the number of sub elements. Therefore, this association must not be realized with a \"set\" semantic.\n┬á\n"@en;
        rdfs:domain   vec:WireElementSpecification;
        rdfs:label    "subWireElementSpecification"@en;
        rdfs:range    vec:WireElementSpecification .

vec:buildingBlockSpecification2DBoundingBox
        rdf:type            owl:ObjectProperty;
        rdfs:comment        "Specifies the size of the area described by the BuildingBlockSpecification2D in Cartesian dimensions. \n"@en;
        rdfs:domain         vec:BuildingBlockSpecification2D;
        rdfs:label          "boundingBox"@en;
        rdfs:range          vec:CartesianDimension;
        rdfs:subPropertyOf  vec:contains .

vec:SegmentForm  rdf:type  owl:Class;
        rdfs:comment     "Enumeration for the definition of the SegmentForm.\n"@en;
        rdfs:label       "SegmentForm"@en;
        rdfs:subClassOf  vec:OpenEnumeration .

vec:partRelationCustomRelationExpression
        rdf:type      owl:DatatypeProperty;
        rdfs:comment  "Defines the relationship between the accessory parts in a proprietary expression language. This attribute shall only be used, if the relationType =┬á'Custom'.\n"@en;
        rdfs:domain   vec:PartRelation;
        rdfs:label    "customRelationExpression"@en;
        rdfs:range    xs:string .

vec:variantGroupAbbreviation
        rdf:type            owl:ObjectProperty;
        rdfs:comment        "Room for a human readable short name, title etc. of the VariantGroup.\n"@en;
        rdfs:domain         vec:VariantGroup;
        rdfs:label          "abbreviation"@en;
        rdfs:range          vec:LocalizedString;
        rdfs:subPropertyOf  vec:contains .

vec:terminalReceptionTerminalReceptionSpecification
        rdf:type      owl:ObjectProperty;
        rdfs:comment  "References the TerminalReceptionSpecification that specifies the TerminalReception.\n"@en;
        rdfs:domain   vec:TerminalReception;
        rdfs:label    "terminalReceptionSpecification"@en;
        rdfs:range    vec:TerminalReceptionSpecification .

vec:soundDampingClassReferenceSystem
        rdf:type      owl:DatatypeProperty;
        rdfs:comment  "The identification of the sound damping class reference system, which is defining possible values and the semantic of sound damping keys.\n"@en;
        rdfs:domain   vec:SoundDampingClass;
        rdfs:label    "referenceSystem"@en;
        rdfs:range    xs:string .

vec:buildingBlockSpecification3DGeometryNode
        rdf:type            owl:ObjectProperty;
        rdfs:comment        "Specifies the GeometryNode3Ds defined by the BuildingBlockSpecification3D.\n"@en;
        rdfs:domain         vec:BuildingBlockSpecification3D;
        rdfs:label          "geometryNode"@en;
        rdfs:range          vec:GeometryNode3D;
        rdfs:subPropertyOf  vec:contains .

vec:topologyMappingSpecificationNodeMapping
        rdf:type            owl:ObjectProperty;
        rdfs:domain         vec:TopologyMappingSpecification;
        rdfs:label          "nodeMapping"@en;
        rdfs:range          vec:NodeMapping;
        rdfs:subPropertyOf  vec:contains .

vec:partUsagePartOrUsageRelatedSpecification
        rdf:type      owl:ObjectProperty;
        rdfs:comment  "References the PartOrUsageRelatedSpecification(s) that describe the PartOrUsageRelatedSpecification. \nKBLFRM-399\n"@en;
        rdfs:domain   vec:PartUsage;
        rdfs:label    "partOrUsageRelatedSpecification"@en;
        rdfs:range    vec:PartOrUsageRelatedSpecification .

vec:connectorHousingSpecificationAverageWireLengthAddOn
        rdf:type            owl:ObjectProperty;
        rdfs:comment        "Specifies the average wire length add on for this connector.\n"@en;
        rdfs:domain         vec:ConnectorHousingSpecification;
        rdfs:label          "averageWireLengthAddOn"@en;
        rdfs:range          vec:NumericalValue;
        rdfs:subPropertyOf  vec:contains .

vec:changeDescriptionResponsibleDesigner
        rdf:type            owl:ObjectProperty;
        rdfs:comment        "Specifies the design engineer who is/was responsible to perform the change.\n"@en;
        rdfs:domain         vec:ChangeDescription;
        rdfs:label          "responsibleDesigner"@en;
        rdfs:range          vec:Person;
        rdfs:subPropertyOf  vec:contains .

vec:ComponentNodeSubType_Motor
        rdf:type         vec:ComponentNodeSubType , owl:NamedIndividiual;
        vec:enumLiteral  "Motor" .

vec:TerminalBoltNominalSize_M12
        rdf:type         vec:TerminalBoltNominalSize , owl:NamedIndividiual;
        vec:enumLiteral  "M12" .

[ rdf:type     owl:AllDisjointClasses;
  owl:members  ( vec:LocalizedString vec:LocalizedTypedString )
] .

vec:LevelOfApproval_Planned
        rdf:type         vec:LevelOfApproval , owl:NamedIndividiual;
        rdfs:comment     "The ItemVersion has been created.\n"@en;
        vec:enumLiteral  "Planned" .

vec:approvalCompanyInScope
        rdf:type      owl:DatatypeProperty;
        rdfs:comment  "Room to specify for which companies the Approval is valid. It might be e.g. that an approved Item may only be delivered by some specific company.\n"@en;
        rdfs:domain   vec:Approval;
        rdfs:label    "companyInScope"@en;
        rdfs:range    xs:string .

vec:PrimaryPartType_RingTerminal
        rdf:type         vec:PrimaryPartType , owl:NamedIndividiual;
        vec:enumLiteral  "RingTerminal" .

vec:topologyNodeProcessingInstruction
        rdf:type            owl:ObjectProperty;
        rdfs:comment        "Specifies processing instructions for the TopologyNode.\n"@en;
        rdfs:domain         vec:TopologyNode;
        rdfs:label          "processingInstruction"@en;
        rdfs:range          vec:LocalizedString;
        rdfs:subPropertyOf  vec:contains .

<http://www.prostep.org/ontologies/ecad/2024/03/vec#RobustnessClassReferenceSystem_LV%20112>
        rdf:type         vec:RobustnessClassReferenceSystem , owl:NamedIndividiual;
        rdfs:comment     "The literal that shall be used for the LV 112.\n"@en;
        vec:enumLiteral  "LV 112" .

vec:numericalValueTolerance
        rdf:type            owl:ObjectProperty;
        rdfs:comment        "Specifies the tolerance for the dimension. \n"@en;
        rdfs:domain         vec:NumericalValue;
        rdfs:label          "tolerance"@en;
        rdfs:range          vec:Tolerance;
        rdfs:subPropertyOf  vec:contains .

vec:changeDescriptionRelatedChangeRequest
        rdf:type      owl:DatatypeProperty;
        rdfs:comment  "Specifies the identification of a corresponding change request. (see KBLFRM-249)\n"@en;
        rdfs:domain   vec:ChangeDescription;
        rdfs:label    "relatedChangeRequest"@en;
        rdfs:range    xs:string .

vec:DocumentType_RequirementsDescription
        rdf:type         vec:DocumentType , owl:NamedIndividiual;
        rdfs:comment     "A requirements description is some kind of document that contains requirements for a certain part or a group of parts, their design or their properties. A requirements description can be a requirements specification (e.g. REQ-IF) or any other document containing requirements (e.g. a norm).\n"@en;
        vec:enumLiteral  "RequirementsDescription" .

vec:shrinkableTubeSpecificationShrinkingFactor
        rdf:type      owl:DatatypeProperty;
        rdfs:comment  "Defines the factor of shrinking for the tube.\n"@en;
        rdfs:domain   vec:ShrinkableTubeSpecification;
        rdfs:label    "shrinkingFactor"@en;
        rdfs:range    xs:double .

vec:PinComponentType_PowerDistribution
        rdf:type         vec:PinComponentType , owl:NamedIndividiual;
        rdfs:comment     " PowerDistribution defines a PinComponent that is used to distribute power to other components (in contrast to PowerSupply ). The semantic of this type depends on the SignalDirection . In means, that this PinComponent is used to supply power to the EEComponent for further distribution to other components. Out means that the PinComponent is a source of power for other EEComponents.\n"@en;
        vec:enumLiteral  "PowerDistribution" .

vec:TerminalBoltNominalSize_M33
        rdf:type         vec:TerminalBoltNominalSize , owl:NamedIndividiual;
        vec:enumLiteral  "M33" .

[ rdf:type     owl:AllDisjointClasses;
  owl:members  ( vec:ConnectorHousingSpecification vec:EEComponentSpecification vec:GeneralTechnicalPartSpecification vec:TerminalSpecification vec:WireSpecification vec:ConnectorHousingCapSpecification vec:CavityPartSpecification vec:WireEndAccessorySpecification vec:LabelingSpecification vec:CableDuctSpecification vec:FixingSpecification vec:GrommetSpecification vec:WireProtectionSpecification vec:CableTieSpecification vec:FerriteSpecification vec:PartStructureSpecification vec:PlaceableElementSpecification vec:RequirementsConformanceSpecification vec:LocalGeometrySpecification )
] .

vec:geometrySegment3DStartVector
        rdf:type            owl:ObjectProperty;
        rdfs:comment        "Specifies the start vector of the geometry segment. The start vector is a tangent to the segment at the start position.\n"@en;
        rdfs:domain         vec:GeometrySegment3D;
        rdfs:label          "startVector"@en;
        rdfs:range          vec:CartesianVector3D;
        rdfs:subPropertyOf  vec:contains .

vec:SlotLayoutType_USBMicroB
        rdf:type         vec:SlotLayoutType , owl:NamedIndividiual;
        vec:enumLiteral  "USBMicroB" .

vec:fixingRoleFixingSpecification
        rdf:type      owl:ObjectProperty;
        rdfs:comment  "References the FixingSpecification that is instanced by this FixingRole.\n"@en;
        rdfs:domain   vec:FixingRole;
        rdfs:label    "fixingSpecification"@en;
        rdfs:range    vec:FixingSpecification .

vec:SlotLayoutType_AMEC
        rdf:type         vec:SlotLayoutType , owl:NamedIndividiual;
        vec:enumLiteral  "AMEC" .

vec:LanguageCode_Fa  rdf:type  vec:LanguageCode , owl:NamedIndividiual;
        vec:enumLiteral  "Fa" .

vec:placeableElementSpecificationValidPlacementTypes
        rdf:type            owl:ObjectProperty;
        rdfs:comment        "Defines the PlacementTypes that are valid for this element.\n"@en;
        rdfs:domain         vec:PlaceableElementSpecification;
        rdfs:label          "validPlacementTypes"@en;
        rdfs:range          vec:PlacementType;
        rdfs:subPropertyOf  vec:contains .

vec:ImperialUnitName_Stone
        rdf:type         vec:ImperialUnitName , owl:NamedIndividiual;
        vec:enumLiteral  "Stone" .

[ rdf:type     owl:AllDisjointClasses;
  owl:members  ( vec:TerminalPairing vec:CavityMounting vec:CavityMountingDetail vec:WireMounting vec:WireMountingDetail vec:ConfigurableElement vec:ItemVersion vec:SheetOrChapter vec:Specification vec:VecContent vec:ConfigurationConstraint vec:AbstractSlot vec:Cavity vec:Coding vec:InternalTerminalConnection vec:SegmentConnectionPoint vec:TerminalReception vec:TerminalType vec:WireElement vec:WireReception vec:SegmentConnectionPointHC vec:ExternalMapping vec:CartesianDimension vec:CartesianPoint2D vec:OccurrenceOrUsageViewItem2D vec:PathSegment vec:Transformation2D vec:CartesianPoint3D vec:OccurrenceOrUsageViewItem3D vec:Transformation3D vec:Curve3D vec:Role vec:AbstractSlotReference vec:CavityReference vec:WireEnd vec:WireGrouping vec:WireLength vec:Instruction vec:Mapping vec:MatingDetail vec:ModuleFamily vec:ModuleList vec:CableDuctOutlet vec:CableLeadThrough vec:FittingOutlet vec:Approval vec:ChangeDescription vec:Contract vec:CopyrightInformation vec:Creation vec:ItemEquivalence vec:ItemHistoryEntry vec:Permission vec:Project vec:Tolerance vec:MeasurementPoint vec:PlacementPoint vec:DimensionAnchor vec:PlacementPointReference vec:Signal vec:SegmentCrossSectionArea vec:SegmentLength vec:Path vec:UsageConstraint vec:VariantCode vec:VariantConfiguration vec:VariantGroup vec:ApplicationConstraint vec:VariantStructureNode vec:AssignmentGroup )
] .

vec:SlotGender_Female
        rdf:type         vec:SlotGender , owl:NamedIndividiual;
        vec:enumLiteral  "Female" .

vec:NetworkNodeSubType_Relay
        rdf:type         vec:NetworkNodeSubType , owl:NamedIndividiual;
        vec:enumLiteral  "Relay" .

vec:PinTiming  rdf:type  owl:Class;
        rdfs:comment  "Specifies the timing for a PinCurrentInformation or a PinVoltageInformation .\n"@en;
        rdfs:label    "PinTiming"@en .

vec:Role  rdf:type       owl:Class;
        rdfs:comment     "A Role is the corresponding mechanism for OccurrenceOrUsages to the PartOrUsageRelatedSpecifcations for PartVersions or PartUsages. The PartOrUsageRelatedSpecifcations are describing a certain aspect of the master data of a part. A Role describes the corresponding properties and relationships for instances of a part (e.g. the usage specific properties of a wire occurrence like the length or the contacting).\n"@en;
        rdfs:label       "Role"@en;
        rdfs:subClassOf  vec:ExtendableElement .

vec:personCompanyName
        rdf:type      owl:DatatypeProperty;
        rdfs:comment  "Specifies the name of the company the person belongs to.\n"@en;
        rdfs:domain   vec:Person;
        rdfs:label    "companyName"@en;
        rdfs:range    xs:string .

vec:SoundDampingClass
        rdf:type      owl:Class;
        rdfs:comment  "Allows the definition of a sound damping class. The sound damping class of a component is specified as a level of sound damping. The level is specified by the classKey . Valid keys are specified by the referenceSystem . Attributes of the type SoundDampingClass normally have the multiplicity [0..*]. This means that such an attribute can have SoundDampingClass entries for different referenceSystems . It must not have multiple entries for the same referenceSystem .\n"@en;
        rdfs:label    "SoundDampingClass"@en .

vec:usageConstraintSpecificationConstrainedParts
        rdf:type      owl:ObjectProperty;
        rdfs:comment  "References the PartVersions to which this UsageConstraintSpecification applies.\n"@en;
        rdfs:domain   vec:UsageConstraintSpecification;
        rdfs:label    "constrainedParts"@en;
        rdfs:range    vec:PartVersion .

vec:PlacementPointReference
        rdf:type         owl:Class;
        rdfs:comment     "A PlacementPointReference is the instance of a PlacementPoint in the context of an OccurrenceOrUsage .\n"@en;
        rdfs:label       "PlacementPointReference"@en;
        rdfs:subClassOf  vec:ExtendableElement .

vec:WireRole  rdf:type   owl:Class;
        rdfs:comment     "A WireRole defines the instance specific properties and relationships of a wire.\n"@en;
        rdfs:label       "WireRole"@en;
        rdfs:subClassOf  vec:Role .

vec:geometrySegment2DStartVector
        rdf:type            owl:ObjectProperty;
        rdfs:comment        "Specifies the start vector of the geometry segment. The start vector is a tangent to the segment at the start position.\n"@en;
        rdfs:domain         vec:GeometrySegment2D;
        rdfs:label          "startVector"@en;
        rdfs:range          vec:CartesianVector2D;
        rdfs:subPropertyOf  vec:contains .

vec:netTypeSignalType
        rdf:type            owl:ObjectProperty;
        rdfs:domain         vec:NetType;
        rdfs:label          "signalType"@en;
        rdfs:range          vec:SignalType;
        rdfs:subPropertyOf  vec:contains .

vec:LanguageCode_Pa  rdf:type  vec:LanguageCode , owl:NamedIndividiual;
        vec:enumLiteral  "Pa" .

vec:DocumentType_SchematicSymbol
        rdf:type         vec:DocumentType , owl:NamedIndividiual;
        rdfs:comment     "Documents of this type represent a graphical symbol (2D), which is normally an external file (e.g. an SVG, PNG). The use case for this document type are symbols that are used in schematic diagrams.\n"@en;
        vec:enumLiteral  "SchematicSymbol" .

vec:PrimaryLockingType
        rdf:type         owl:Class;
        rdfs:comment     "Defines the valid primary locking types for terminals.\n"@en;
        rdfs:label       "PrimaryLockingType"@en;
        rdfs:subClassOf  vec:OpenEnumeration .

vec:FoilShieldWindingType_Overlap
        rdf:type         vec:FoilShieldWindingType , owl:NamedIndividiual;
        rdfs:comment     "Spirally wound around the shielded elements with minimal overlap (i.e. without gaps)"@en;
        vec:enumLiteral  "Overlap" .

vec:slotCouplingCavityCoupling
        rdf:type            owl:ObjectProperty;
        rdfs:domain         vec:SlotCoupling;
        rdfs:label          "cavityCoupling"@en;
        rdfs:range          vec:CavityCoupling;
        rdfs:subPropertyOf  vec:contains .

vec:AliasIdentificationType
        rdf:type         owl:Class;
        rdfs:label       "AliasIdentificationType"@en;
        rdfs:subClassOf  vec:OpenEnumeration .

vec:SpliceType_EndSplice
        rdf:type         vec:SpliceType , owl:NamedIndividiual;
        rdfs:comment     "An endSplice is a splice where wires only from one side are connected.\n"@en;
        vec:enumLiteral  "EndSplice" .

vec:PlacementType  rdf:type  owl:Class;
        rdfs:comment         "Defines the type for which a PlaceableElement can be used.\n"@en;
        rdfs:label           "PlacementType"@en;
        rdfs:subClassOf      vec:ClosedEnumeration;
        owl:equivalentClass  [ rdf:type   owl:Class;
                               owl:oneOf  ( vec:PlacementType_OnWay vec:PlacementType_OnPoint )
                             ] .

vec:wireElementSpecificationSize
        rdf:type            owl:ObjectProperty;
        rdfs:comment        "Defines the size of a WireElement if it has not the shape of circle. If it has the shape of a circle the size is normally defined by its outside diameter.\n"@en;
        rdfs:domain         vec:WireElementSpecification;
        rdfs:label          "size"@en;
        rdfs:range          vec:Size;
        rdfs:subPropertyOf  vec:contains .

vec:LabelType  rdf:type  owl:Class;
        rdfs:comment     "OpenEnumeration of different labeling types. This refers to the way the information is encoded."@en;
        rdfs:label       "LabelType"@en;
        rdfs:subClassOf  vec:OpenEnumeration .

vec:wireTupleTerminationWireTupleSpecification
        rdf:type     owl:ObjectProperty;
        rdfs:domain  vec:WireTupleTermination;
        rdfs:label   "wireTupleSpecification"@en;
        rdfs:range   vec:WireTupleSpecification .

vec:RobustnessClassReferenceSystem
        rdf:type         owl:Class;
        rdfs:comment     "Defines the literals that shall be used for specific robustness class reference systems.\n"@en;
        rdfs:label       "RobustnessClassReferenceSystem"@en;
        rdfs:subClassOf  vec:OpenEnumeration .

vec:slotSupplementaryParts
        rdf:type      owl:ObjectProperty;
        rdfs:comment  "References the PartRelations that specify supplementary parts for this slot.\n"@en;
        rdfs:domain   vec:Slot;
        rdfs:label    "supplementaryParts"@en;
        rdfs:range    vec:PartRelation .

vec:topologyZoneAmbientTemperature
        rdf:type            owl:ObjectProperty;
        rdfs:comment        "Defines the ambient temperature that can occur in this zone. This can result in specific requirements for the used components.\n"@en;
        rdfs:domain         vec:TopologyZone;
        rdfs:label          "ambientTemperature"@en;
        rdfs:range          vec:TemperatureInformation;
        rdfs:subPropertyOf  vec:contains .

vec:SlotLayoutType_HMTD
        rdf:type         vec:SlotLayoutType , owl:NamedIndividiual;
        rdfs:comment     "High-Speed Modular Twisted-Pair Data"@en;
        vec:enumLiteral  "HMTD" .

vec:UsageNodeType_Ground
        rdf:type         vec:UsageNodeType , owl:NamedIndividiual;
        rdfs:comment     "Defines that this ComponentNode is a grounding point.\n"@en;
        vec:enumLiteral  "Ground" .

vec:NetworkNodeType_PowerDistribution
        rdf:type         vec:NetworkNodeType , owl:NamedIndividiual;
        rdfs:comment     "A device that distributes power to other devices (e.g. a fuse box).\n"@en;
        vec:enumLiteral  "PowerDistribution" .

vec:signalSignalType  rdf:type  owl:ObjectProperty;
        rdfs:domain         vec:Signal;
        rdfs:label          "signalType"@en;
        rdfs:range          vec:SignalType;
        rdfs:subPropertyOf  vec:contains .

vec:LanguageCode_De  rdf:type  vec:LanguageCode , owl:NamedIndividiual;
        vec:enumLiteral  "De" .

vec:LanguageCode_Za  rdf:type  vec:LanguageCode , owl:NamedIndividiual;
        vec:enumLiteral  "Za" .

vec:PinCurrentType_BlockCurrent
        rdf:type         vec:PinCurrentType , owl:NamedIndividiual;
        vec:enumLiteral  "blockCurrent" .

vec:transformation3DA22
        rdf:type     owl:DatatypeProperty;
        rdfs:domain  vec:Transformation3D;
        rdfs:label   "a22"@en;
        rdfs:range   xs:double .

vec:TerminalBoltNominalSize_M1.6
        rdf:type         vec:TerminalBoltNominalSize , owl:NamedIndividiual;
        vec:enumLiteral  "M1.6" .

vec:signalDescription
        rdf:type            owl:ObjectProperty;
        rdfs:comment        "A human readable description of the signal.\n"@en;
        rdfs:domain         vec:Signal;
        rdfs:label          "description"@en;
        rdfs:range          vec:AbstractLocalizedString;
        rdfs:subPropertyOf  vec:contains .

vec:ComponentNode  rdf:type  owl:Class;
        rdfs:comment     "A ComponentNode is a node where an electrological component is located. It is a representative for an element in the electric system, e.g. an actuator, a sensor, an ECU. In this way it is quite similar to a NetworkNode and may even reference the corresponding NetworkNode in this case. However, a ComponentNode is more likely to be used as a representative of an inliner or a splice. Moreover, a ComponentNode can define childNodes in order to describe its internal structure.\n"@en;
        rdfs:label       "ComponentNode"@en;
        rdfs:subClassOf  vec:ConfigurableElement .

vec:pinComponentBehaviorOpticalInformation
        rdf:type            owl:ObjectProperty;
        rdfs:comment        "Specifies the optical information of the pin, if it has the type optical.\n"@en;
        rdfs:domain         vec:PinComponentBehavior;
        rdfs:label          "opticalInformation"@en;
        rdfs:range          vec:PinOpticalInformation;
        rdfs:subPropertyOf  vec:contains .

vec:specificationIdentification
        rdf:type      owl:DatatypeProperty;
        rdfs:comment  "Specifies a unique identification of the specification. The identification is guaranteed to be unique within the document containing the specification. For all VEC-documents a Specification-instance can be trusted to be identical if the DocumentVersion-instance is the same (see DocumentVersion) and the identification of the Specification is the same.\n"@en;
        rdfs:domain   vec:Specification;
        rdfs:label    "identification"@en;
        rdfs:range    xs:string .

vec:LanguageCode_Ne  rdf:type  vec:LanguageCode , owl:NamedIndividiual;
        vec:enumLiteral  "Ne" .

vec:baselineSpecificationValidVersions
        rdf:type      owl:ObjectProperty;
        rdfs:comment  "References the ItemVersions that are the content of the baseline.\n┬á\n"@en;
        rdfs:domain   vec:BaselineSpecification;
        rdfs:label    "validVersions"@en;
        rdfs:range    vec:ItemVersion .

vec:DocumentType_InstallationDescription
        rdf:type         vec:DocumentType , owl:NamedIndividiual;
        rdfs:comment     ""@en;
        vec:enumLiteral  "InstallationDescription" .

vec:SignalSpecification
        rdf:type         owl:Class;
        rdfs:comment     "Specification for the definition of a list of valid signals.\n"@en;
        rdfs:label       "SignalSpecification"@en;
        rdfs:subClassOf  vec:Specification .

vec:TerminalPairing  rdf:type  owl:Class;
        rdfs:comment     "A TerminalPairing is a standard reference setup of exactly two terminals and a defined length of a core contacted to both terminals. The TerminalPairing defines physical properties that apply to this combination.\n┬á\n"@en;
        rdfs:label       "TerminalPairing"@en;
        rdfs:subClassOf  vec:ExtendableElement .

vec:ConnectionEndGender_Unspecified
        rdf:type         vec:ConnectionEndGender , owl:NamedIndividiual;
        rdfs:comment     ""@en;
        vec:enumLiteral  "Unspecified" .

vec:SignalSubType_APIX2
        rdf:type         vec:SignalSubType , owl:NamedIndividiual;
        vec:enumLiteral  "APIX2" .

vec:conductorSpecificationCurrentInformation
        rdf:type            owl:ObjectProperty;
        rdfs:comment        "Specifies the current information of the conductor. These are the maximum currents for which the conductor is approved.\n"@en;
        rdfs:domain         vec:ConductorSpecification;
        rdfs:label          "currentInformation"@en;
        rdfs:range          vec:ConductorCurrentInformation;
        rdfs:subPropertyOf  vec:contains .

vec:insulationSpecificationSecondIdentificationColor
        rdf:type            owl:ObjectProperty;
        rdfs:comment        "Specifies the second identification color of the insulation.\n"@en;
        rdfs:domain         vec:InsulationSpecification;
        rdfs:label          "secondIdentificationColor"@en;
        rdfs:range          vec:Color;
        rdfs:subPropertyOf  vec:contains .

vec:LanguageCode_Bi  rdf:type  vec:LanguageCode , owl:NamedIndividiual;
        vec:enumLiteral  "Bi" .

vec:MultiFuseType  rdf:type  owl:Class;
        rdfs:comment     "OpenEnumeration for the manufacturing types of the multi-fuses.\n"@en;
        rdfs:label       "MultiFuseType"@en;
        rdfs:subClassOf  vec:OpenEnumeration .

vec:localizedStringPropertyValue
        rdf:type            owl:ObjectProperty;
        rdfs:comment        "Defines the value of the CustomProperty.\n"@en;
        rdfs:domain         vec:LocalizedStringProperty;
        rdfs:label          "value"@en;
        rdfs:range          vec:LocalizedString;
        rdfs:subPropertyOf  vec:contains .

vec:Specification  rdf:type  owl:Class;
        rdfs:comment     "Abstract super-class for all specifications. Every technical information exchanged with the VEC is contained in the different specializations of a specification.\n"@en;
        rdfs:label       "Specification"@en;
        rdfs:subClassOf  vec:ExtendableElement .

vec:Routing  rdf:type    owl:Class;
        rdfs:comment     "A Routing is the assignment of a RoutableElement (Connection or WireElementReference) to a path in the topology.\n"@en;
        rdfs:label       "Routing"@en;
        rdfs:subClassOf  vec:ConfigurableElement .

vec:PlacementType_OnWay
        rdf:type         vec:PlacementType , owl:NamedIndividiual;
        rdfs:comment     " OnWay refers to an OnWayPlacement .\n"@en;
        vec:enumLiteral  "OnWay" .

vec:internalComponentConnectionConductorSpecification
        rdf:type     owl:ObjectProperty;
        rdfs:domain  vec:InternalComponentConnection;
        rdfs:label   "conductorSpecification"@en;
        rdfs:range   vec:ConductorSpecification .

vec:SiPrefix_Centi  rdf:type  vec:SiPrefix , owl:NamedIndividiual;
        vec:enumLiteral  "Centi" .

vec:pinOpticalInformationFrequency
        rdf:type            owl:ObjectProperty;
        rdfs:comment        "The frequency of the optical signal.\n"@en;
        rdfs:domain         vec:PinOpticalInformation;
        rdfs:label          "frequency"@en;
        rdfs:range          vec:NumericalValue;
        rdfs:subPropertyOf  vec:contains .

vec:labelingRoleLabelType
        rdf:type            owl:ObjectProperty;
        rdfs:comment        "Specifies the type of a label printed, stamped or integrated on or in component (e.g. alpha numerical, bar code).\n"@en;
        rdfs:domain         vec:LabelingRole;
        rdfs:label          "labelType"@en;
        rdfs:range          vec:LabelType;
        rdfs:subPropertyOf  vec:contains .

vec:TopologySegmentWrapper
        rdf:type      owl:Class;
        rdfs:comment  "Container class for TopologySegment to participate in non-unique and/or ordered associations." .

vec:temperatureInformationTemperatureRange
        rdf:type            owl:ObjectProperty;
        rdfs:comment        "Specifies the allowed temperature range for this type of temperature.\n"@en;
        rdfs:domain         vec:TemperatureInformation;
        rdfs:label          "temperatureRange"@en;
        rdfs:range          vec:ValueRange;
        rdfs:subPropertyOf  vec:contains .

vec:WireElementShape_Elliptical
        rdf:type         vec:WireElementShape , owl:NamedIndividiual;
        vec:enumLiteral  "Elliptical" .

vec:eEComponentRoleComponentNode
        rdf:type      owl:ObjectProperty;
        rdfs:comment  "References the ComponentNode that is realized by the referenced EEComponent (OccurrenceOrUsage with EEComponentRole).\nKBLFRM-341\n"@en;
        rdfs:domain   vec:EEComponentRole;
        rdfs:label    "componentNode"@en;
        rdfs:range    vec:ComponentNode .

vec:IntegerValueProperty
        rdf:type         owl:Class;
        rdfs:comment     "A custom property with an integer value.\n"@en;
        rdfs:label       "IntegerValueProperty"@en;
        rdfs:subClassOf  vec:CustomProperty .

vec:temperatureInformationTemperatureType
        rdf:type            owl:ObjectProperty;
        rdfs:comment        "The type of a TemperatureInformation.\n"@en;
        rdfs:domain         vec:TemperatureInformation;
        rdfs:label          "temperatureType"@en;
        rdfs:range          vec:TemperatureType;
        rdfs:subPropertyOf  vec:contains .

vec:SealingGeometry_Sectored
        rdf:type         vec:SealingGeometry , owl:NamedIndividiual;
        vec:enumLiteral  "Sectored" .

vec:robustnessPropertiesClassReferenceSystem
        rdf:type            owl:ObjectProperty;
        rdfs:comment        "The identification of the robustness class reference system, which is defining possible values and the semantic of robustness classes and robustness class keys. Specific known and used reference systems are defined in an open enumeration.\n"@en;
        rdfs:domain         vec:RobustnessProperties;
        rdfs:label          "classReferenceSystem"@en;
        rdfs:range          vec:RobustnessClassReferenceSystem;
        rdfs:subPropertyOf  vec:contains .

vec:housingComponentReferenceHousingComponent
        rdf:type      owl:ObjectProperty;
        rdfs:comment  "Points to the HousingComponent referenced by the HousingComponent reference. \n(KBLFRM-401)\n"@en;
        rdfs:domain   vec:HousingComponentReference;
        rdfs:label    "housingComponent"@en;
        rdfs:range    vec:HousingComponent .

vec:wireElementSpecificationConductorSpecification
        rdf:type      owl:ObjectProperty;
        rdfs:comment  "If the WireElement has a core then the specification of the core is referenced here.\n"@en;
        rdfs:domain   vec:WireElementSpecification;
        rdfs:label    "conductorSpecification"@en;
        rdfs:range    vec:ConductorSpecification .

vec:LanguageCode_Th  rdf:type  vec:LanguageCode , owl:NamedIndividiual;
        vec:enumLiteral  "Th" .

vec:FittingForm_Plug  rdf:type  vec:FittingForm , owl:NamedIndividiual;
        rdfs:comment     "Plug for the closure of tubes and pipes.\n"@en;
        vec:enumLiteral  "Plug" .

vec:enumLiteral  rdf:type   owl:DatatypeProperty;
        rdfs:comment        "Defines the literal value of an enumeration as represented in the model."@en;
        rdfs:domain         vec:Enumeration;
        rdfs:label          "enumLiteral"@en;
        rdfs:range          xs:string;
        rdfs:subPropertyOf  rdfs:label .

vec:connectorHousingRoleConnectorHousingSpecification
        rdf:type      owl:ObjectProperty;
        rdfs:comment  "References the ConnectorHousingSpecification that is instanced by this ConnectorHousingRole.\n"@en;
        rdfs:domain   vec:ConnectorHousingRole;
        rdfs:label    "connectorHousingSpecification"@en;
        rdfs:range    vec:ConnectorHousingSpecification .

vec:ContractRole  rdf:type  owl:Class;
        rdfs:comment     "Enumeration for the definition of roles a contractor has in a contract.\n"@en;
        rdfs:label       "ContractRole"@en;
        rdfs:subClassOf  vec:OpenEnumeration .

vec:IECUnitName_Byte  rdf:type  vec:IECUnitName , owl:NamedIndividiual;
        vec:enumLiteral  "Byte" .

vec:DocumentType_BaselineDefinition
        rdf:type         vec:DocumentType , owl:NamedIndividiual;
        rdfs:comment     "The DocumentVersion represents the definition of a baseline (see BaselineSpecification ).\n"@en;
        vec:enumLiteral  "BaselineDefinition" .

vec:HousingComponentType_ConnectorHousing
        rdf:type         vec:HousingComponentType , owl:NamedIndividiual;
        vec:enumLiteral  "ConnectorHousing" .

vec:fittingOutletInnerDiameter
        rdf:type            owl:ObjectProperty;
        rdfs:comment        "Specifies the inner diameter of the outlet.\n"@en;
        rdfs:domain         vec:FittingOutlet;
        rdfs:label          "innerDiameter"@en;
        rdfs:range          vec:NumericalValue;
        rdfs:subPropertyOf  vec:contains .

vec:partOccurrenceIsSecondaryAlternative
        rdf:type      owl:DatatypeProperty;
        rdfs:comment  "If a PartUsage is realized by more than one PartOccurrence it is possible to specify which one is the preferred. (see KBLFRM-264)\n"@en;
        rdfs:domain   vec:PartOccurrence;
        rdfs:label    "isSecondaryAlternative"@en;
        rdfs:range    xs:boolean .

[ rdf:type     owl:AllDisjointClasses;
  owl:members  ( vec:PluggableTerminalSpecification vec:RingTerminalSpecification vec:SpliceTerminalSpecification vec:BoltTerminalSpecification vec:OpenWireEndTerminalSpecification vec:BridgeTerminalSpecification )
] .

vec:USUnitName_Foot  rdf:type  vec:USUnitName , owl:NamedIndividiual;
        vec:enumLiteral  "Foot" .

vec:LanguageCode_Vi  rdf:type  vec:LanguageCode , owl:NamedIndividiual;
        vec:enumLiteral  "Vi" .

vec:grommetRoleGrommetSpecification
        rdf:type      owl:ObjectProperty;
        rdfs:comment  "References the GrommetSpecification that is instanced by this GrommetRole.\n"@en;
        rdfs:domain   vec:GrommetRole;
        rdfs:label    "grommetSpecification"@en;
        rdfs:range    vec:GrommetSpecification .

vec:SpliceTerminalRole
        rdf:type         owl:Class;
        rdfs:comment     "A SpliceTerminalRole defines the instance specific properties and relationships of a splice terminal.\n"@en;
        rdfs:label       "SpliceTerminalRole"@en;
        rdfs:subClassOf  vec:TerminalRole .

vec:vecContentItemHistoryEntry
        rdf:type            owl:ObjectProperty;
        rdfs:comment        "Specifies the ItemVersionHistoryEntries for ItemVersions contained in the VEC-file. \n"@en;
        rdfs:domain         vec:VecContent;
        rdfs:label          "itemHistoryEntry"@en;
        rdfs:range          vec:ItemHistoryEntry;
        rdfs:subPropertyOf  vec:contains .

vec:slotLayoutGridY  rdf:type  owl:ObjectProperty;
        rdfs:comment        "The vertical distance between the center points of two cavities.\n"@en;
        rdfs:domain         vec:SlotLayout;
        rdfs:label          "gridY"@en;
        rdfs:range          vec:NumericalValue;
        rdfs:subPropertyOf  vec:contains .

vec:vecContentPartVersion
        rdf:type            owl:ObjectProperty;
        rdfs:comment        "Specifies the PartVersions contained in the VEC-file. \n"@en;
        rdfs:domain         vec:VecContent;
        rdfs:label          "partVersion"@en;
        rdfs:range          vec:PartVersion;
        rdfs:subPropertyOf  vec:contains .

vec:FittingForm_Elbow
        rdf:type         vec:FittingForm , owl:NamedIndividiual;
        rdfs:comment     "Angled 1:1 coupling.\n"@en;
        vec:enumLiteral  "Elbow" .

vec:signalSignalName  rdf:type  owl:DatatypeProperty;
        rdfs:comment  "Name of the Signal, which is not guaranteed to be unique and is normally function oriented.\n"@en;
        rdfs:domain   vec:Signal;
        rdfs:label    "signalName"@en;
        rdfs:range    xs:string .

vec:HoleMountedFixingHoleType_ImperialThread
        rdf:type         vec:HoleMountedFixingHoleType , owl:NamedIndividiual;
        rdfs:comment     "The hole provides an imperial thread for fixation."@en;
        vec:enumLiteral  "ImperialThread" .

vec:LanguageCode_Bn  rdf:type  vec:LanguageCode , owl:NamedIndividiual;
        vec:enumLiteral  "Bn" .

vec:PartNature_CustomerOrder
        rdf:type         vec:PartNature , owl:NamedIndividiual;
        rdfs:comment     " CustomerOrder PartVersions represent part numbers that are not regularly used in serial production. They are only used to fulfil special customer orders (e.g. an adapter connector for equipment of a special purpose vehicle).\n"@en;
        vec:enumLiteral  "CustomerOrder" .

vec:HoleMountedFixingHoleType_Plain
        rdf:type         vec:HoleMountedFixingHoleType , owl:NamedIndividiual;
        rdfs:comment     "The hol itself is plain and provides no special features."@en;
        vec:enumLiteral  "Plain" .

vec:componentNodeChildNode
        rdf:type            owl:ObjectProperty;
        rdfs:comment        "Specifies the ComponentNodes that are a child of this ComponentNode.\n"@en;
        rdfs:domain         vec:ComponentNode;
        rdfs:label          "childNode"@en;
        rdfs:range          vec:ComponentNode;
        rdfs:subPropertyOf  vec:contains .

vec:partVersionProject
        rdf:type      owl:ObjectProperty;
        rdfs:comment  "References the project that develops the PartVersion. \n"@en;
        rdfs:domain   vec:PartVersion;
        rdfs:label    "project"@en;
        rdfs:range    vec:Project .

vec:FittingForm_Lateral
        rdf:type         vec:FittingForm , owl:NamedIndividiual;
        rdfs:comment     "A \"wye\"┬áwith one straight and one lateral outlet.\n"@en;
        vec:enumLiteral  "Lateral" .

vec:PowerConsumptionType_Sleep
        rdf:type         vec:PowerConsumptionType , owl:NamedIndividiual;
        vec:enumLiteral  "Sleep" .

vec:relaySpecificationApplianceType
        rdf:type            owl:ObjectProperty;
        rdfs:comment        "Specifies the appliance type of a relais.\n"@en;
        rdfs:domain         vec:RelaySpecification;
        rdfs:label          "applianceType"@en;
        rdfs:range          vec:RelaisApplianceType;
        rdfs:subPropertyOf  vec:contains .

vec:signalRecommendedInsulationSpecification
        rdf:type      owl:ObjectProperty;
        rdfs:comment  "Defines a recommended Specification for the insulation (e.g. the color) that implements this signal.\n"@en;
        rdfs:domain   vec:Signal;
        rdfs:label    "recommendedInsulationSpecification"@en;
        rdfs:range    vec:InsulationSpecification .

vec:DimensionAnchor  rdf:type  owl:Class;
        rdfs:comment     "A DimensionAnchor represents an abstract anchor onto which a Dimension can be specified.\n"@en;
        rdfs:label       "DimensionAnchor"@en;
        rdfs:subClassOf  vec:ExtendableElement .

vec:ImperialUnitName_Pint
        rdf:type         vec:ImperialUnitName , owl:NamedIndividiual;
        vec:enumLiteral  "Pint" .

vec:PrimaryPartType_HoleMountedFixing
        rdf:type         vec:PrimaryPartType , owl:NamedIndividiual;
        vec:enumLiteral  "HoleMountedFixing" .

vec:networkPortViewItemNetworkPort
        rdf:type      owl:ObjectProperty;
        rdfs:comment  "References the NetworkPort that is represented by this NetworkPortViewItem. "@en;
        rdfs:domain   vec:NetworkPortViewItem;
        rdfs:label    "networkPort"@en;
        rdfs:range    vec:NetworkPort .

vec:VecVersion_1.1.3  rdf:type  vec:VecVersion , owl:NamedIndividiual;
        vec:enumLiteral  "1.1.3" .

vec:NetworkNodeType_Actuator
        rdf:type         vec:NetworkNodeType , owl:NamedIndividiual;
        rdfs:comment     "An actuator is a device that is responsible for controlling or moving a mechanism.\n"@en;
        vec:enumLiteral  "Actuator" .

vec:VariantCodeSpecification
        rdf:type         owl:Class;
        rdfs:comment     "Specification for the definition of variant codes.\n"@en;
        rdfs:label       "VariantCodeSpecification"@en;
        rdfs:subClassOf  vec:Specification .

vec:netIdentification
        rdf:type      owl:DatatypeProperty;
        rdfs:comment  "Specifies a unique identification of the Net. The identification is guaranteed to be unique within the NetSpecification.\n"@en;
        rdfs:domain   vec:Net;
        rdfs:label    "identification"@en;
        rdfs:range    xs:string .

vec:MassInformationSource_Series
        rdf:type         vec:MassInformationSource , owl:NamedIndividiual;
        rdfs:comment     "A MassInformation with this valueSource has been determined based on a serial production part.\n"@en;
        vec:enumLiteral  "Series" .

vec:Unit  rdf:type    owl:Class;
        rdfs:comment  "A precisely specified quantity in terms of which the magnitudes of other quantities of the same kind can be stated. The different systems to define units are represented by the subclasses of this class (e.g. SIUnit, ImperialUnit).\n"@en;
        rdfs:label    "Unit"@en .

vec:tubeSpecificationSecondaryNominalSize
        rdf:type      owl:DatatypeProperty;
        rdfs:comment  "Defines the secondary nominal size of a tube. The nominal size is a name for the size of the tube that is somehow related to the inner diameter of the tube. However, it is not the inner diameter (e.g. \"10.5\").\nThe secondary nominal size shall only be used for two-parted tubes (see┬áTubeSlitStyle = TwoParts). The secondary nominal size defines the size of the outer (larger) tube of a two-parted tube.\n"@en;
        rdfs:domain   vec:TubeSpecification;
        rdfs:label    "secondaryNominalSize"@en;
        rdfs:range    xs:string .

vec:SignalSubType_APIX
        rdf:type         vec:SignalSubType , owl:NamedIndividiual;
        rdfs:comment     "Automotive Pixel Link\n"@en;
        vec:enumLiteral  "APIX" .

vec:LanguageCode_Ln  rdf:type  vec:LanguageCode , owl:NamedIndividiual;
        vec:enumLiteral  "Ln" .

vec:ShieldSpecification
        rdf:type         owl:Class;
        rdfs:comment     "Specifies the properties of a shield.\n"@en;
        rdfs:label       "ShieldSpecification"@en;
        rdfs:subClassOf  vec:ConductorSpecification .

vec:SlotLayoutType_Type_A1
        rdf:type         vec:SlotLayoutType , owl:NamedIndividiual;
        rdfs:comment     "Fuse type according to ISO8820, also known as: jcase\n"@en;
        vec:enumLiteral  "Type_A1" .

[ rdf:type     owl:AllDisjointClasses;
  owl:members  ( vec:GeometryNode2D vec:GeometryNode3D )
] .

vec:PrimaryPartType_ShrinkableTube
        rdf:type         vec:PrimaryPartType , owl:NamedIndividiual;
        vec:enumLiteral  "ShrinkableTube" .

vec:LanguageCode_No  rdf:type  vec:LanguageCode , owl:NamedIndividiual;
        vec:enumLiteral  "No" .

vec:SignalSubType_FlexRay
        rdf:type         vec:SignalSubType , owl:NamedIndividiual;
        vec:enumLiteral  "FlexRay" .

vec:LevelOfApproval  rdf:type  owl:Class;
        rdfs:comment     "The┬áLevelOfApproval standardizes the approval levels most engineering processes have in common. See Approval.levelOfApproval for more details.\n"@en;
        rdfs:label       "LevelOfApproval"@en;
        rdfs:subClassOf  vec:OpenEnumeration .

vec:NominalVoltage  rdf:type  owl:Class;
        rdfs:label       "NominalVoltage"@en;
        rdfs:subClassOf  vec:OpenEnumeration .

vec:ConnectionGroup  rdf:type  owl:Class;
        rdfs:comment     "A ConnectionGroup references two or more Connections expressing that the physical realization of the referenced Connection shall be somehow grouped e.g. twisted. For complex structures a ConnectionGroup can specify subgroups.\n"@en;
        rdfs:label       "ConnectionGroup"@en;
        rdfs:subClassOf  vec:ConfigurableElement .

vec:ConnectorOutletDirection_Straight
        rdf:type         vec:ConnectorOutletDirection , owl:NamedIndividiual;
        vec:enumLiteral  "Straight" .

vec:routingSpecificationRouting
        rdf:type            owl:ObjectProperty;
        rdfs:comment        "Specifies the Routings described by the RoutingSpecification.\n"@en;
        rdfs:domain         vec:RoutingSpecification;
        rdfs:label          "routing"@en;
        rdfs:range          vec:Routing;
        rdfs:subPropertyOf  vec:contains .

vec:TapeSpecification
        rdf:type         owl:Class;
        rdfs:comment     "Specification for the description of tapes.\n"@en;
        rdfs:label       "TapeSpecification"@en;
        rdfs:subClassOf  vec:WireProtectionSpecification .

vec:PartVersionWrapper
        rdf:type      owl:Class;
        rdfs:comment  "Container class for PartVersion to participate in non-unique and/or ordered associations." .

<http://www.prostep.org/ontologies/ecad/2024/03/vec#TerminalBoltNominalSize_%233>
        rdf:type         vec:TerminalBoltNominalSize , owl:NamedIndividiual;
        vec:enumLiteral  "#3" .

vec:TopologySpecification
        rdf:type         owl:Class;
        rdfs:comment     "Specification for the definition of a topology. A topology consists of TopologyNodes, TopologySegments.\n"@en;
        rdfs:label       "TopologySpecification"@en;
        rdfs:subClassOf  vec:Specification .

vec:cableLeadThroughReferenceIdentification
        rdf:type      owl:DatatypeProperty;
        rdfs:comment  "Specifies a unique identification of the CableLeadThroughReference. The identification is guaranteed to be unique within the GrommetRole.\n"@en;
        rdfs:domain   vec:CableLeadThroughReference;
        rdfs:label    "identification"@en;
        rdfs:range    xs:string .

vec:HousingComponentType_Fuse
        rdf:type         vec:HousingComponentType , owl:NamedIndividiual;
        vec:enumLiteral  "Fuse" .

vec:switchingStateIdentification
        rdf:type      owl:DatatypeProperty;
        rdfs:comment  "Identification of the SwitchingState, which must be distinct for all SwitchingStates of an EEComponent.\n"@en;
        rdfs:domain   vec:SwitchingState;
        rdfs:label    "identification"@en;
        rdfs:range    xs:string .

vec:connectorHousingSpecificationSlot
        rdf:type            owl:ObjectProperty;
        rdfs:comment        "Specifies the slots forming the ConnectorHousing. \n"@en;
        rdfs:domain         vec:ConnectorHousingSpecification;
        rdfs:label          "slot"@en;
        rdfs:range          vec:AbstractSlot;
        rdfs:subPropertyOf  vec:contains .

vec:PrimaryPartType_Stripe
        rdf:type         vec:PrimaryPartType , owl:NamedIndividiual;
        vec:enumLiteral  "Stripe" .

vec:itemVersionDescription
        rdf:type            owl:ObjectProperty;
        rdfs:comment        "Room for additional, human readable information about the ItemVersion. e.g. Buchsengeh├ñuse 26-polig\n"@en;
        rdfs:domain         vec:ItemVersion;
        rdfs:label          "description"@en;
        rdfs:range          vec:AbstractLocalizedString;
        rdfs:subPropertyOf  vec:contains .

vec:projectDescription
        rdf:type            owl:ObjectProperty;
        rdfs:comment        "Room for additional information about the item.\n"@en;
        rdfs:domain         vec:Project;
        rdfs:label          "description"@en;
        rdfs:range          vec:AbstractLocalizedString;
        rdfs:subPropertyOf  vec:contains .

vec:SignalSubType_BroadR-Reach
        rdf:type         vec:SignalSubType , owl:NamedIndividiual;
        vec:enumLiteral  "BroadR-Reach" .

vec:WireElementSpecification
        rdf:type         owl:Class;
        rdfs:comment     "A WireElementSpecification is the basic element to describe a wire in the VEC. A WireElementSpecification can be atomic or composed recursively out of other WireElementSpecifications. A WireElementSpecification can reference an InsulationSpecification, if it has an insulation, a CoreSpecification, if it has a core or a WireGroupSpecification if it is a grouping of other WireElementSpecifications in the Wire (e.g. a multi-core wire with twisted pairs).\n"@en;
        rdfs:label       "WireElementSpecification"@en;
        rdfs:subClassOf  vec:Specification .

vec:BoltMountedFixingSpecification
        rdf:type         owl:Class;
        rdfs:comment     "Specification for fixings that are mounted onto a bolt. This means the fixing itself has got a hole, which is mounted onto a bolt of the surrounding.┬á\n"@en;
        rdfs:label       "BoltMountedFixingSpecification"@en;
        rdfs:subClassOf  vec:FixingSpecification .

vec:BridgeTerminalSpecification
        rdf:type         owl:Class;
        rdfs:comment     "A bridge terminal is a part that behaves like terminal but has no WireReceptions. It is used to create short circuit between different pins in a connector. In its use, it can realize a schematic connection on its own and independently of other components.\n"@en;
        rdfs:label       "BridgeTerminalSpecification"@en;
        rdfs:subClassOf  vec:TerminalSpecification .

vec:CavitySealRole  rdf:type  owl:Class;
        rdfs:comment     "A CavitySealRole defines the instance specific properties and relationships of a cavity seal.\n"@en;
        rdfs:label       "CavitySealRole"@en;
        rdfs:subClassOf  vec:Role .

vec:SiPrefix_Nano  rdf:type  vec:SiPrefix , owl:NamedIndividiual;
        vec:enumLiteral  "Nano" .

vec:insulationSpecificationMaterial
        rdf:type            owl:ObjectProperty;
        rdfs:comment        "Specifies the material of the insulation.\n"@en;
        rdfs:domain         vec:InsulationSpecification;
        rdfs:label          "material"@en;
        rdfs:range          vec:Material;
        rdfs:subPropertyOf  vec:contains .

vec:ComponentNodeType_Switch
        rdf:type         vec:ComponentNodeType , owl:NamedIndividiual;
        rdfs:comment     "A \"Switch\" is a device that can change its internal connectivity in reaction to some external action (e.g. connect /┬ádisconnect┬ásome pins). A switch has no \"active\" logic (in contrast to an ECU).\n"@en;
        vec:enumLiteral  "Switch" .

vec:insulationSpecificationAllowedLabelingTechnology
        rdf:type            owl:ObjectProperty;
        rdfs:comment        "Specifies the allowed labeling technologies if the insulation is not yet labeled, but support labeling in its usage."@en;
        rdfs:domain         vec:InsulationSpecification;
        rdfs:label          "allowedLabelingTechnology"@en;
        rdfs:range          vec:LabelingTechnology;
        rdfs:subPropertyOf  vec:contains .

vec:PartOrUsageRelatedSpecification
        rdf:type         owl:Class;
        rdfs:comment     "Base class for all specifications which are describing a PartVersion or a PartUsage . A PartOrUsageRelatedSpecification specifies a certain aspect of the described part or usage (e.g. general technical part information, connector housing aspects or wire aspects).\n"@en;
        rdfs:label       "PartOrUsageRelatedSpecification"@en;
        rdfs:subClassOf  vec:Specification .

vec:dimensionReferenceAnchor
        rdf:type      owl:ObjectProperty;
        rdfs:comment  "References the location that is used as reference point for the dimensioning (e.g. the location of a fixing as this relates to a fixpoint of the body in white).\nSee KBLFRM-329 and KBLFRM-391.\n"@en;
        rdfs:domain   vec:Dimension;
        rdfs:label    "referenceAnchor"@en;
        rdfs:range    vec:DimensionAnchor .

vec:USUnitName_Perch  rdf:type  vec:USUnitName , owl:NamedIndividiual;
        vec:enumLiteral  "Perch" .

vec:PowerConsumptionType_StartStop
        rdf:type         vec:PowerConsumptionType , owl:NamedIndividiual;
        vec:enumLiteral  "StartStop" .

vec:netNetworkPort  rdf:type  owl:ObjectProperty;
        rdfs:comment  "References the NetworkPorts that are connected by the Net. \n"@en;
        rdfs:domain   vec:Net;
        rdfs:label    "networkPort"@en;
        rdfs:range    vec:NetworkPort .

vec:SiUnitName_Katal  rdf:type  vec:SiUnitName , owl:NamedIndividiual;
        vec:enumLiteral  "Katal" .

vec:ConnectorHousingRole
        rdf:type         owl:Class;
        rdfs:comment     "A ConnectorHousingRole defines the instance specific properties and relationships of a connector housing.\n"@en;
        rdfs:label       "ConnectorHousingRole"@en;
        rdfs:subClassOf  vec:Role .

vec:insulationSpecificationBaseColor
        rdf:type            owl:ObjectProperty;
        rdfs:comment        "Specifies the base color of the insulation.\n"@en;
        rdfs:domain         vec:InsulationSpecification;
        rdfs:label          "baseColor"@en;
        rdfs:range          vec:Color;
        rdfs:subPropertyOf  vec:contains .

vec:capacitorSpecificationImpedance
        rdf:type            owl:ObjectProperty;
        rdfs:domain         vec:CapacitorSpecification;
        rdfs:label          "impedance"@en;
        rdfs:range          vec:NumericalValue;
        rdfs:subPropertyOf  vec:contains .

vec:SegmentCrossSectionArea
        rdf:type         owl:Class;
        rdfs:comment     "Specifies the cross-section area of a segment. For the data exchange the cross-section area is used and not the diameter, because the diameter is only a valid measure for circular segments. For circular segments, the diameter and the cross-section area can be translated into each other without the loss of information. Attributes of the type SegmentCrossSectionArea normally have the multiplicity [0..*]. This means that such an attribute can have SegmentCrossSectionArea entries for different crossSectionAreaTypes and valueDeterminations. It must not have multiple entries with the same crossSectionAreaType and valueDetermination.\n"@en;
        rdfs:label       "SegmentCrossSectionArea"@en;
        rdfs:subClassOf  vec:ExtendableElement .

vec:BridgeTerminalRole
        rdf:type         owl:Class;
        rdfs:comment     "A BridgeTerminalRole defines the instance specific properties and relationships of a bridge terminal (see BridgeTerminalSpecification).\nA bridge terminal is a part that behaves like terminal but has no WireReceptions. It is used to create short circuit between different pins in a connector. In its use, it can realize a schematic connection on its own and independently of other components.\n"@en;
        rdfs:label       "BridgeTerminalRole"@en;
        rdfs:subClassOf  vec:TerminalRole .

vec:FuseType_Form_CB15_CatE
        rdf:type         vec:FuseType , owl:NamedIndividiual;
        rdfs:comment     "also known as: auto\n"@en;
        vec:enumLiteral  "Form_CB15_CatE" .

vec:LanguageCode_Tr  rdf:type  vec:LanguageCode , owl:NamedIndividiual;
        vec:enumLiteral  "Tr" .

vec:wireLengthLengthType
        rdf:type            owl:ObjectProperty;
        rdfs:comment        "The type of the length.┬áPossible values are defined in an open enumeration (see WireLengthType).\n"@en;
        rdfs:domain         vec:WireLength;
        rdfs:label          "lengthType"@en;
        rdfs:range          vec:WireLengthType;
        rdfs:subPropertyOf  vec:contains .

vec:TerminalBoltNominalSize_M4
        rdf:type         vec:TerminalBoltNominalSize , owl:NamedIndividiual;
        vec:enumLiteral  "M4" .

vec:PlacementPointPosition
        rdf:type         owl:Class;
        rdfs:comment     "Defines the position of a PlacementPoint within the coordinate system of the component. PlacementPoints are points where a component is attached to a TopologySegment. Therefor a PlacementPointPosition can define a tangent vector (in the coordinate system of the component) for a segment that is connected to the PlacementPoint.\n"@en;
        rdfs:label       "PlacementPointPosition"@en;
        rdfs:subClassOf  vec:LocalPosition .

vec:signalCurrentType
        rdf:type            owl:ObjectProperty;
        rdfs:domain         vec:Signal;
        rdfs:label          "currentType"@en;
        rdfs:range          vec:CurrentType;
        rdfs:subPropertyOf  vec:contains .

vec:CavityPositionDetail
        rdf:type      owl:Class;
        rdfs:comment  " CavityPositionDetail is an aggregator class for all geometric properties of a cavity within the connector (e.g. rotation, position)."@en;
        rdfs:label    "CavityPositionDetail"@en .

vec:geometrySegment2DEndNode
        rdf:type      owl:ObjectProperty;
        rdfs:comment  "References the GeometryNode2D where the GeometrySegment2D ends. \n"@en;
        rdfs:domain   vec:GeometrySegment2D;
        rdfs:label    "endNode"@en;
        rdfs:range    vec:GeometryNode2D .

vec:valueRangeMinimum
        rdf:type      owl:DatatypeProperty;
        rdfs:comment  "Lower bound of the value range.\n"@en;
        rdfs:domain   vec:ValueRange;
        rdfs:label    "minimum"@en;
        rdfs:range    xs:double .

vec:USUnitName_Gill  rdf:type  vec:USUnitName , owl:NamedIndividiual;
        vec:enumLiteral  "Gill" .

vec:WireReceptionSpecification
        rdf:type         owl:Class;
        rdfs:comment     "Specification for the definition of wire receptions. A WireReception is the area of a terminal where the contacting with a wire element (e.g. by crimping) takes place.\n"@en;
        rdfs:label       "WireReceptionSpecification"@en;
        rdfs:subClassOf  vec:Specification .

vec:topologyNodeIdentification
        rdf:type      owl:DatatypeProperty;
        rdfs:comment  "Specifies a unique identification of the TopologyNode. The identification is guaranteed to be unique within the TopologySpecification. For all VEC-documents a TopologyNode-instance can be trusted to be the same if the TopologySpecification-instance is the same (see TopologySpecification) and the identification of the TopologyNode is the same.\n"@en;
        rdfs:domain   vec:TopologyNode;
        rdfs:label    "identification"@en;
        rdfs:range    xs:string .

vec:placementType  rdf:type  owl:DatatypeProperty;
        rdfs:comment  "Room to specify additional type information of the placement.\n"@en;
        rdfs:domain   vec:Placement;
        rdfs:label    "type"@en;
        rdfs:range    xs:string .

vec:wireElementSpecificationShape
        rdf:type            owl:ObjectProperty;
        rdfs:comment        "Defines the shape of a WireElement. Circular wire elements are defined by their outsideDiameter, all others are defined by their size.\n"@en;
        rdfs:domain         vec:WireElementSpecification;
        rdfs:label          "shape"@en;
        rdfs:range          vec:WireElementShape;
        rdfs:subPropertyOf  vec:contains .

<http://www.prostep.org/ontologies/ecad/2024/03/vec#TerminalBoltNominalSize_%238>
        rdf:type         vec:TerminalBoltNominalSize , owl:NamedIndividiual;
        vec:enumLiteral  "#8" .

vec:documentRelatedAssignmentGroupRelatedDocumentVersion
        rdf:type      owl:ObjectProperty;
        rdfs:comment  "References the DocumentVersion to which this group relates.\n"@en;
        rdfs:domain   vec:DocumentRelatedAssignmentGroup;
        rdfs:label    "relatedDocumentVersion"@en;
        rdfs:range    vec:DocumentVersion .

[ rdf:type     owl:AllDisjointClasses;
  owl:members  ( vec:AntennaSpecification vec:BatterySpecification vec:FuseSpecification vec:RelaySpecification vec:MultiFuseSpecification vec:PotentialDistributorSpecification vec:DiodeSpecification vec:CapacitorSpecification )
] .

vec:buildingBlockSpecification2DBaseUnit
        rdf:type      owl:ObjectProperty;
        rdfs:comment  ""@en;
        rdfs:domain   vec:BuildingBlockSpecification2D;
        rdfs:label    "baseUnit"@en;
        rdfs:range    vec:Unit .

vec:ContactPoint  rdf:type  owl:Class;
        rdfs:comment     "A contact point defines the relationship between Terminals, Seals, Plugs, Cavities and Wires. It specifies a single contacting variant. This means that the contacting is manufactured, as specified by the Contact Point. Either all participants (Cavities, Terminals, Seals, Wires) set into a relationship by the ContactPoint exist in a specific harness or none. There is no requirement, to filter the participants of a contacting situation with information derived from VariantConfigurations or assembly /┬ámodule associations in order to create a manufacturing variant.\nThe ContactPoint represents a single potential. Consequently, all cavities and wires referencing / being referenced by a ContactPoint are short-circuited and have the same potential (even if the signals on the wires are named differently. If a contacting of a terminal has more than one potential (e.g. a coax-contact) one contact point for each potential is needed.\n"@en;
        rdfs:label       "ContactPoint"@en;
        rdfs:subClassOf  vec:ConfigurableElement .

vec:capacitorSpecificationUMax
        rdf:type            owl:ObjectProperty;
        rdfs:comment        "┬áThe breakdown voltage of the capacitor.\n"@en;
        rdfs:domain         vec:CapacitorSpecification;
        rdfs:label          "uMax"@en;
        rdfs:range          vec:NumericalValue;
        rdfs:subPropertyOf  vec:contains .

vec:SignalForm_SinusWave
        rdf:type         vec:SignalForm , owl:NamedIndividiual;
        vec:enumLiteral  "sinusWave" .

vec:ConductorMaterial
        rdf:type      owl:Class;
        rdfs:comment  " ConductorMaterial is a helper class to specify validConductorMaterials. This is necessary, since all attributes of the type Material have a multiplicity of * with the semantics that it always defines one Material with the possibility to define it in different reference systems.\nSince a wire reception can have more than one validConductorMaterial this container class is necessary to keep the semantics clear.\n"@en;
        rdfs:label    "ConductorMaterial"@en .

vec:topologySegmentLengthInformation
        rdf:type            owl:ObjectProperty;
        rdfs:comment        "Specifies the different SegmentLengths of the TopologySegment. \n"@en;
        rdfs:domain         vec:TopologySegment;
        rdfs:label          "lengthInformation"@en;
        rdfs:range          vec:SegmentLength;
        rdfs:subPropertyOf  vec:contains .

vec:variantConfigurationBaseInclusion
        rdf:type      owl:ObjectProperty;
        rdfs:comment  "A VariantConfiguration can only be satisfied if its baseInclusion is satisfied as well.\n"@en;
        rdfs:domain   vec:VariantConfiguration;
        rdfs:label    "baseInclusion"@en;
        rdfs:range    vec:VariantConfiguration .

vec:RoutingSpecification
        rdf:type         owl:Class;
        rdfs:comment     "Specification for the description of Routings.\n"@en;
        rdfs:label       "RoutingSpecification"@en;
        rdfs:subClassOf  vec:Specification .

vec:LanguageCode_Jw  rdf:type  vec:LanguageCode , owl:NamedIndividiual;
        vec:enumLiteral  "Jw" .

<http://www.prostep.org/ontologies/ecad/2024/03/vec#TerminalBoltNominalSize_9%2F16>
        rdf:type         vec:TerminalBoltNominalSize , owl:NamedIndividiual;
        vec:enumLiteral  "9/16" .

vec:Cavity  rdf:type     owl:Class;
        rdfs:comment     "A cavity is a defined space in a connector housing for location of an electrical terminal or cavity plug or seal. A cavity may also be empty.\n"@en;
        rdfs:label       "Cavity"@en;
        rdfs:subClassOf  vec:ExtendableElement .

vec:signalSpecificationSignal
        rdf:type            owl:ObjectProperty;
        rdfs:comment        "Specifies the signals.\n"@en;
        rdfs:domain         vec:SignalSpecification;
        rdfs:label          "signal"@en;
        rdfs:range          vec:Signal;
        rdfs:subPropertyOf  vec:contains .

vec:LanguageCode_Zu  rdf:type  vec:LanguageCode , owl:NamedIndividiual;
        rdfs:comment     "Zulu\n"@en;
        vec:enumLiteral  "Zu" .

vec:PinCurrentType_InitCurrent
        rdf:type         vec:PinCurrentType , owl:NamedIndividiual;
        vec:enumLiteral  "initCurrent" .

vec:CableTieSpecification
        rdf:type         owl:Class;
        rdfs:comment     "Specification for the definition of cable ties.\n"@en;
        rdfs:label       "CableTieSpecification"@en;
        rdfs:subClassOf  vec:PartOrUsageRelatedSpecification .

vec:ApplicationConstraintType
        rdf:type             owl:Class;
        rdfs:comment         "Enumeration for the definition of the type of an ApplicationConstraints. Valid values are allow and deny.\n"@en;
        rdfs:label           "ApplicationConstraintType"@en;
        rdfs:subClassOf      vec:ClosedEnumeration;
        owl:equivalentClass  [ rdf:type   owl:Class;
                               owl:oneOf  ( vec:ApplicationConstraintType_Allow vec:ApplicationConstraintType_Deny )
                             ] .

vec:ComponentNodeSubType_Relay
        rdf:type         vec:ComponentNodeSubType , owl:NamedIndividiual;
        vec:enumLiteral  "Relay" .

vec:segmentConnectionPointIdentification
        rdf:type      owl:DatatypeProperty;
        rdfs:comment  "Specifies a unique identification of the SegmentConnectionPoint. The identification is guaranteed to be unique within the ConnectorHousingSpecification.\n"@en;
        rdfs:domain   vec:SegmentConnectionPoint;
        rdfs:label    "identification"@en;
        rdfs:range    xs:string .

vec:LanguageCode_Tw  rdf:type  vec:LanguageCode , owl:NamedIndividiual;
        vec:enumLiteral  "Tw" .

vec:cableLeadThroughReferenceUsedPlugs
        rdf:type      owl:ObjectProperty;
        rdfs:comment  "References the plugs that are used with this CableLeadThroughReference. This association might be a 150% selection.\n"@en;
        rdfs:domain   vec:CableLeadThroughReference;
        rdfs:label    "usedPlugs"@en;
        rdfs:range    vec:CavityPlugRole .

vec:componentPortViewItemSide
        rdf:type            owl:ObjectProperty;
        rdfs:comment        "Specifies the side of the ComponentNodeViewItem on which the port should be displayed."@en;
        rdfs:domain         vec:ComponentPortViewItem;
        rdfs:label          "side"@en;
        rdfs:range          vec:ComponentPortViewItemSide;
        rdfs:subPropertyOf  vec:contains .

vec:ComponentNodeType_Ground
        rdf:type         vec:ComponentNodeType , owl:NamedIndividiual;
        rdfs:comment     "Defines that this ComponentNode is a grounding point.\n"@en;
        vec:enumLiteral  "Ground" .

vec:SealingGeometry_Circular
        rdf:type         vec:SealingGeometry , owl:NamedIndividiual;
        vec:enumLiteral  "Circular" .

vec:sheetOrChapterChangeDescription
        rdf:type            owl:ObjectProperty;
        rdfs:comment        "Specifies the change history of the SheetOrChapter."@en;
        rdfs:domain         vec:SheetOrChapter;
        rdfs:label          "changeDescription"@en;
        rdfs:range          vec:ChangeDescription;
        rdfs:subPropertyOf  vec:contains .

vec:WireReceptionType_Soldering
        rdf:type         vec:WireReceptionType , owl:NamedIndividiual;
        vec:enumLiteral  "Soldering" .

vec:itemVersionApproval
        rdf:type            owl:ObjectProperty;
        rdfs:comment        "Specifies the approval information of the ItemVersion. \n"@en;
        rdfs:domain         vec:ItemVersion;
        rdfs:label          "approval"@en;
        rdfs:range          vec:Approval;
        rdfs:subPropertyOf  vec:contains .

vec:wireReceptionSpecificationWireReceptionType
        rdf:type            owl:ObjectProperty;
        rdfs:comment        "Specifies the type of the wire reception. The wireReceptionType defines how the wire is joined with the wire reception.\nThis attribute is defined in an OpenEnumeration.\n"@en;
        rdfs:domain         vec:WireReceptionSpecification;
        rdfs:label          "wireReceptionType"@en;
        rdfs:range          vec:WireReceptionType;
        rdfs:subPropertyOf  vec:contains .

vec:PinCurrentType_DeepSleepCurrent
        rdf:type         vec:PinCurrentType , owl:NamedIndividiual;
        rdfs:comment     "Defines the current on the pin, when the EEComponent is in deep sleep mode.\n"@en;
        vec:enumLiteral  "deepSleepCurrent" .

vec:PinCurrentType_StartStopCurrent
        rdf:type         vec:PinCurrentType , owl:NamedIndividiual;
        vec:enumLiteral  "startStopCurrent" .

vec:transformation2DA22
        rdf:type     owl:DatatypeProperty;
        rdfs:domain  vec:Transformation2D;
        rdfs:label   "a22"@en;
        rdfs:range   xs:double .

vec:documentVersionSheetOrChapter
        rdf:type            owl:ObjectProperty;
        rdfs:comment        "Specifies SheetOrChapters defined in this DocumentVersion. These are especially useful if the DocumentVersion represents an external reference. \n"@en;
        rdfs:domain         vec:DocumentVersion;
        rdfs:label          "sheetOrChapter"@en;
        rdfs:range          vec:SheetOrChapter;
        rdfs:subPropertyOf  vec:contains .

vec:NetworkNodeType  rdf:type  owl:Class;
        rdfs:comment     "Defines the common agreed values for the Types of a NetworkNode.\n"@en;
        rdfs:label       "NetworkNodeType"@en;
        rdfs:subClassOf  vec:OpenEnumeration .

vec:NodeLocation  rdf:type  owl:Class;
        rdfs:comment     "Specifies a TopologyNode as a Location.\n"@en;
        rdfs:label       "NodeLocation"@en;
        rdfs:subClassOf  vec:Location .

vec:NetworkPortViewItemSide_Top
        rdf:type         vec:NetworkPortViewItemSide , owl:NamedIndividiual;
        vec:enumLiteral  "Top" .

vec:cavityMountingCavityMountingDetail
        rdf:type            owl:ObjectProperty;
        rdfs:comment        "Specifies the CavityMoutingDetails, if a detailed description of the relationships between Cavities and TerminalReceptions is needed.\n"@en;
        rdfs:domain         vec:CavityMounting;
        rdfs:label          "cavityMountingDetail"@en;
        rdfs:range          vec:CavityMountingDetail;
        rdfs:subPropertyOf  vec:contains .

vec:ConnectionNodeViewItem
        rdf:type      owl:Class;
        rdfs:comment  "A ComponentNodeViewItem represents a ComponentNode within a ConnectionViewSpecification and defines its position within the layout."@en;
        rdfs:label    "ConnectionNodeViewItem"@en .

vec:SegmentForm_Circular
        rdf:type         vec:SegmentForm , owl:NamedIndividiual;
        vec:enumLiteral  "Circular" .

vec:occurrenceOrUsageIdentification
        rdf:type      owl:DatatypeProperty;
        rdfs:comment  "Specifies a unique identification of the OccurrenceOrUsage. The identification is guaranteed to be unique within the context. For all VEC-documents an OccurrenceOrUsage-instance can be trusted to be the same if the context-instance is the same and the identification of the OccurrenceOrUsage is the same.\n"@en;
        rdfs:domain   vec:OccurrenceOrUsage;
        rdfs:label    "identification"@en;
        rdfs:range    xs:string .

vec:aliasIdentificationType
        rdf:type            owl:ObjectProperty;
        rdfs:comment        "Defines the type (or the role)┬áof the AliasIdentification. Defined literals are contained in an OpenEnumeration.\n"@en;
        rdfs:domain         vec:AliasIdentification;
        rdfs:label          "type"@en;
        rdfs:range          vec:AliasIdentificationType;
        rdfs:subPropertyOf  vec:contains .

vec:pinCurrentInformationType
        rdf:type            owl:ObjectProperty;
        rdfs:comment        "Defines the type of the current.\n"@en;
        rdfs:domain         vec:PinCurrentInformation;
        rdfs:label          "type"@en;
        rdfs:range          vec:PinCurrentType;
        rdfs:subPropertyOf  vec:contains .

vec:ComponentNodeSubType_Lamp
        rdf:type         vec:ComponentNodeSubType , owl:NamedIndividiual;
        vec:enumLiteral  "Lamp" .

vec:GrommetMountingType
        rdf:type         owl:Class;
        rdfs:comment     "OpenEnumeration to define different mounting possibilites of a grommet onto a wiring harness."@en;
        rdfs:label       "GrommetMountingType"@en;
        rdfs:subClassOf  vec:OpenEnumeration .

vec:ModuleList  rdf:type  owl:Class;
        rdfs:comment     "A ModuleList is a mechanism to control additional / completion PartOccurrences. This means for a car configuration, if at least one of the modules in the list participates in the configuration, the \"completionComponent\" participates, too.\n"@en;
        rdfs:label       "ModuleList"@en;
        rdfs:subClassOf  vec:ExtendableElement .

vec:VariantGroupSpecification
        rdf:type         owl:Class;
        rdfs:comment     "Specification for the definition of variant groups.\n"@en;
        rdfs:label       "VariantGroupSpecification"@en;
        rdfs:subClassOf  vec:Specification .

vec:SignalInformationType
        rdf:type         owl:Class;
        rdfs:label       "SignalInformationType"@en;
        rdfs:subClassOf  vec:OpenEnumeration .

vec:FuseType_Type_C  rdf:type  vec:FuseType , owl:NamedIndividiual;
        rdfs:comment     "also known as: ato\n"@en;
        vec:enumLiteral  "Type_C" .

vec:LabelingTechnology_Imprinted
        rdf:type         vec:LabelingTechnology , owl:NamedIndividiual;
        vec:enumLiteral  "Imprinted" .

vec:generalTechnicalPartSpecificationMassInformation
        rdf:type            owl:ObjectProperty;
        rdfs:comment        "Specifies the mass of the part.\n"@en;
        rdfs:domain         vec:GeneralTechnicalPartSpecification;
        rdfs:label          "massInformation"@en;
        rdfs:range          vec:MassInformation;
        rdfs:subPropertyOf  vec:contains .

vec:PinType_Resistive
        rdf:type         vec:PinType , owl:NamedIndividiual;
        vec:enumLiteral  "resistive" .

vec:wireReceptionAngle
        rdf:type            owl:ObjectProperty;
        rdfs:comment        "Specifies the angles against two planes of the connector housing a wire reception can be buckled. The planes are defined in a way, that angles of ┬á[0.0, 0.0] specify an unbuckled (regular)┬áterminal. The two planes are perpendicular to each other and parallel to the plugging direction of the terminal (the direction of the pin).\nThe plane for the first angle is the plane in which the uncrimped wire reception would be, if the terminal has not been buckled. Since most terminals are cut or punched in some way out of a sheet of metal, this plane would be the same as metal sheet before further deformation.\nFor ring terminals the first plane is perpendicular to the bolt direction.\nWith a viewing direction from the wire reception to the terminal reception and the intended wire position above the terminal, buckling directions up and right are expressed by positive angles, down and left by negative angles.\n"@en;
        rdfs:domain         vec:WireReception;
        rdfs:label          "angle"@en;
        rdfs:range          vec:NumericalValue , vec:Ordered;
        rdfs:subPropertyOf  vec:contains .

vec:housingComponentReferenceIdentification
        rdf:type      owl:DatatypeProperty;
        rdfs:comment  "Specifies a unique identification of the HousingComponentReference. The identification is guaranteed to be unique within the EEComponentRole.\n"@en;
        rdfs:domain   vec:HousingComponentReference;
        rdfs:label    "identification"@en;
        rdfs:range    xs:string .

vec:WireReceptionReference
        rdf:type      owl:Class;
        rdfs:comment  "A WireReceptionReference is an instance of a WireReception .\n"@en;
        rdfs:label    "WireReceptionReference"@en .

vec:measurementPointReferenceMeasurementPoint
        rdf:type      owl:ObjectProperty;
        rdfs:comment  "References the MeasurementPoint that is instanced by this MeasurementPointReference.\n"@en;
        rdfs:domain   vec:MeasurementPointReference;
        rdfs:label    "measurementPoint"@en;
        rdfs:range    vec:MeasurementPoint .

vec:connectionSpecificationConnectionGroup
        rdf:type            owl:ObjectProperty;
        rdfs:comment        "Specifies the ConnectionGroup defined by the ConnectionSpecification.\n"@en;
        rdfs:domain         vec:ConnectionSpecification;
        rdfs:label          "connectionGroup"@en;
        rdfs:range          vec:ConnectionGroup;
        rdfs:subPropertyOf  vec:contains .

vec:ExtensionSlotReference
        rdf:type         owl:Class;
        rdfs:comment     "An ExtensionSlotReference represents the usage of an ExtensionSlot in the context of a PartUsage or PartOccurrence.\n"@en;
        rdfs:label       "ExtensionSlotReference"@en;
        rdfs:subClassOf  vec:ConfigurableElement .

vec:HoleMountedFixingHoleShape_Square
        rdf:type         vec:HoleMountedFixingHoleShape , owl:NamedIndividiual;
        vec:enumLiteral  "Square" .

vec:PinVoltageType_MinVoltage
        rdf:type         vec:PinVoltageType , owl:NamedIndividiual;
        vec:enumLiteral  "minVoltage" .

vec:CableLeadThroughGeometry_Circular
        rdf:type         vec:CableLeadThroughGeometry , owl:NamedIndividiual;
        vec:enumLiteral  "Circular" .

vec:SignalSubType_USB3.X
        rdf:type         vec:SignalSubType , owl:NamedIndividiual;
        rdfs:comment     "Universal Serial┬áBus Version 3.X\n"@en;
        vec:enumLiteral  "USB3.X" .

vec:FoilShieldWindingType_Longitudinal
        rdf:type         vec:FoilShieldWindingType , owl:NamedIndividiual;
        rdfs:comment     "Folded lengthwise around the shielded elements (like a cigarette paper)."@en;
        vec:enumLiteral  "Longitudinal" .

vec:wireGroupingRelatedWireElementReference
        rdf:type      owl:ObjectProperty;
        rdfs:comment  "References the concrete wire elements ( WireElementReference ) that are grouped by the WireGrouping.\n"@en;
        rdfs:domain   vec:WireGrouping;
        rdfs:label    "relatedWireElementReference"@en;
        rdfs:range    vec:WireElementReference .

vec:localPositionCartesianPoint
        rdf:type     owl:ObjectProperty;
        rdfs:domain  vec:LocalPosition;
        rdfs:label   "cartesianPoint"@en;
        rdfs:range   vec:CartesianPoint3D .

vec:DefaultDimensionType_MeasurementChains
        rdf:type         vec:DefaultDimensionType , owl:NamedIndividiual;
        rdfs:comment     "Applies to all measurements without specific tolerance definitions or a more specific DefaultDimensionType. Sums of individual dimensions must also not exceed these tolerances.\n"@en;
        vec:enumLiteral  "MeasurementChains" .

vec:SiPrefix_Milli  rdf:type  vec:SiPrefix , owl:NamedIndividiual;
        vec:enumLiteral  "Milli" .

vec:FittingForm_A  rdf:type  vec:FittingForm , owl:NamedIndividiual;
        rdfs:comment     "A pipe /┬átube connector (1:1) with an additional outlet for wires (without a pipe /┬átube).\n"@en;
        vec:enumLiteral  "A" .

vec:wireProtectionRoleMaterialLength
        rdf:type            owl:ObjectProperty;
        rdfs:domain         vec:WireProtectionRole;
        rdfs:label          "materialLength"@en;
        rdfs:range          vec:ProtectionMaterialLength;
        rdfs:subPropertyOf  vec:contains .

vec:TerminalBoltNominalSize_M42
        rdf:type         vec:TerminalBoltNominalSize , owl:NamedIndividiual;
        vec:enumLiteral  "M42" .

vec:CurrentType  rdf:type  owl:Class;
        rdfs:label       "CurrentType"@en;
        rdfs:subClassOf  vec:OpenEnumeration .

vec:FuseType_Type_SF  rdf:type  vec:FuseType , owl:NamedIndividiual;
        rdfs:comment     "also known as: strip\n"@en;
        vec:enumLiteral  "Type_SF" .

vec:fittingSpecificationForm
        rdf:type            owl:ObjectProperty;
        rdfs:comment        "Specifies the form of the fitting (e.g. Y, T).\n"@en;
        rdfs:domain         vec:FittingSpecification;
        rdfs:label          "form"@en;
        rdfs:range          vec:FittingForm;
        rdfs:subPropertyOf  vec:contains .

vec:FuseType_Type_A1S
        rdf:type         vec:FuseType , owl:NamedIndividiual;
        rdfs:comment     "also known as: flat\n"@en;
        vec:enumLiteral  "Type_A1S" .

vec:terminalCurrentInformationCoreCrossSectionArea
        rdf:type            owl:ObjectProperty;
        rdfs:comment        "Specifies the coreCrossSectionArea for which the CurrentRangeInformation is valid. The coreCrossSectionArea is a relevant information, because the thermal absorption of the core depends on the cross-section area and thus is an influence factor for the valid current range.\n"@en;
        rdfs:domain         vec:TerminalCurrentInformation;
        rdfs:label          "coreCrossSectionArea"@en;
        rdfs:range          vec:NumericalValue;
        rdfs:subPropertyOf  vec:contains .

vec:Project  rdf:type    owl:Class;
        rdfs:comment     "Specifies a certain vehicle project. Instances of this class are assumed to be constant. Thus, this is located directly under VEC-root element.\nA vehicle project can be some abstract or concrete node in the product structure, addressed by the car classification levels.\n"@en;
        rdfs:label       "Project"@en;
        rdfs:subClassOf  vec:ExtendableElement .

vec:RelaisApplianceType_Screwed
        rdf:type         vec:RelaisApplianceType , owl:NamedIndividiual;
        vec:enumLiteral  "screwed" .

vec:fuseComponentFuseSpecification
        rdf:type     owl:ObjectProperty;
        rdfs:domain  vec:FuseComponent;
        rdfs:label   "fuseSpecification"@en;
        rdfs:range   vec:FuseSpecification .

vec:couplingPointSlotCoupling
        rdf:type            owl:ObjectProperty;
        rdfs:domain         vec:CouplingPoint;
        rdfs:label          "slotCoupling"@en;
        rdfs:range          vec:SlotCoupling;
        rdfs:subPropertyOf  vec:contains .

vec:SegmentCrossSectionAreaType_Reserved
        rdf:type         vec:SegmentCrossSectionAreaType , owl:NamedIndividiual;
        rdfs:comment     " Reserved is the type for cross section areas that define a reserved space in the DMU┬áfor the┬á TopologySegment.\n"@en;
        vec:enumLiteral  "Reserved" .

vec:Material  rdf:type  owl:Class;
        rdfs:comment  "Allows the definition of material information. Attributes of the type Material normally have the multiplicity [0..*]. This means that such an attribute can have material values for different referenceSystems . It must not have multiple values for the same referenceSystems .\n"@en;
        rdfs:label    "Material"@en .

[ rdf:type     owl:AllDisjointClasses;
  owl:members  ( vec:NumericalValue vec:ValueRange )
] .

vec:CableLeadThrough  rdf:type  owl:Class;
        rdfs:comment     "A CableLeadThrough specifies a hole in the grommet through which wires can pass through the grommet. There can be different technical realizations of a lead through, e.g. it can be realized with a shrinking material or an additional seal. The properties of a CableLeadThrough are defined in the referenced CableLeadThroughSpecification .\nFor a precise placement in topology, a CableLeadThrough specifies outlets.\n"@en;
        rdfs:label       "CableLeadThrough"@en;
        rdfs:subClassOf  vec:ExtendableElement .

vec:LanguageCode_Ab  rdf:type  vec:LanguageCode , owl:NamedIndividiual;
        rdfs:comment     "Abkhazian\n"@en;
        vec:enumLiteral  "Ab" .

vec:RobustnessClass_ImpactProtection
        rdf:type         vec:RobustnessClass , owl:NamedIndividiual;
        vec:enumLiteral  "ImpactProtection" .

vec:harnessGeometrySpecification3DGeometryType
        rdf:type      owl:ObjectProperty;
        rdfs:comment  "Specifies the type of geometry. Valid values are Dmu, Formboard.\n"@en;
        rdfs:domain   vec:HarnessGeometrySpecification3D;
        rdfs:label    "geometryType"@en;
        rdfs:range    vec:GeometryType .

vec:SignalType_Energy
        rdf:type         vec:SignalType , owl:NamedIndividiual;
        vec:enumLiteral  "energy" .

vec:LanguageCode_Ia  rdf:type  vec:LanguageCode , owl:NamedIndividiual;
        vec:enumLiteral  "Ia" .

vec:USUnitName_Grain  rdf:type  vec:USUnitName , owl:NamedIndividiual;
        vec:enumLiteral  "Grain" .

vec:valueRangeMaximum
        rdf:type      owl:DatatypeProperty;
        rdfs:comment  "Upper bound of the value range.\n"@en;
        rdfs:domain   vec:ValueRange;
        rdfs:label    "maximum"@en;
        rdfs:range    xs:double .

vec:TopologyZoneType_DmuZone
        rdf:type         vec:TopologyZoneType , owl:NamedIndividiual;
        vec:enumLiteral  "DmuZone" .

vec:FoilShieldWindingType
        rdf:type         owl:Class;
        rdfs:comment     "Defines the type of winding for foil shields. It can be folded around and along the inner wire elements like a cigarette paper or it can be wound around them in a spiral. Both types result in different manufacturing and EMC properties.\n"@en;
        rdfs:label       "FoilShieldWindingType"@en;
        rdfs:subClassOf  vec:OpenEnumeration .

vec:NominalVoltage_HV3
        rdf:type         vec:NominalVoltage , owl:NamedIndividiual;
        rdfs:comment     "HV Class 3 (600V┬áDC)\n"@en;
        vec:enumLiteral  "HV3" .

vec:topologyBendingRestrictionMinBendRadiusStatic
        rdf:type            owl:ObjectProperty;
        rdfs:comment        "Specifies the minimum bend radius for the restricted path, if it is used in a static environment, where it is bended once during installation. After that it remains unchanged in its bended position during usage.\n"@en;
        rdfs:domain         vec:TopologyBendingRestriction;
        rdfs:label          "minBendRadiusStatic"@en;
        rdfs:range          vec:NumericalValue;
        rdfs:subPropertyOf  vec:contains .

vec:cavityPlugRoleCavityPlugSpecification
        rdf:type      owl:ObjectProperty;
        rdfs:comment  "References the CavityPlugSpecification that is instanced by this CavityPlugRole.\n"@en;
        rdfs:domain   vec:CavityPlugRole;
        rdfs:label    "cavityPlugSpecification"@en;
        rdfs:range    vec:CavityPlugSpecification .

vec:VecContent  rdf:type  owl:Class;
        rdfs:comment     "The VecContent is the XML-Root node for any VEC-Document.\n"@en;
        rdfs:label       "VecContent"@en;
        rdfs:subClassOf  vec:ExtendableElement .

vec:wireTupleTerminationSpecificationWireTupleTermination
        rdf:type            owl:ObjectProperty;
        rdfs:domain         vec:WireTupleTerminationSpecification;
        rdfs:label          "wireTupleTermination"@en;
        rdfs:range          vec:WireTupleTermination;
        rdfs:subPropertyOf  vec:contains .

vec:wireEndConnectionEnd
        rdf:type     owl:ObjectProperty;
        rdfs:domain  vec:WireEnd;
        rdfs:label   "connectionEnd"@en;
        rdfs:range   vec:ConnectionEnd .

vec:placeableElementRolePlaceableElementSpecification
        rdf:type      owl:ObjectProperty;
        rdfs:comment  "References the PlaceableElementSpecification that is instanced by this PlaceableElementRole.\n"@en;
        rdfs:domain   vec:PlaceableElementRole;
        rdfs:label    "placeableElementSpecification"@en;
        rdfs:range    vec:PlaceableElementSpecification .

vec:LanguageCode_Sa  rdf:type  vec:LanguageCode , owl:NamedIndividiual;
        vec:enumLiteral  "Sa" .

vec:PluggableTerminalType_Bridge
        rdf:type         vec:PluggableTerminalType , owl:NamedIndividiual;
        vec:enumLiteral  "Bridge" .

vec:functionalAssignmentGroupFunctionalRequirements
        rdf:type            owl:ObjectProperty;
        rdfs:comment        "Functional requirements that apply to the members of this group.\n┬á\n"@en;
        rdfs:domain         vec:FunctionalAssignmentGroup;
        rdfs:label          "functionalRequirements"@en;
        rdfs:range          vec:FunctionalRequirement;
        rdfs:subPropertyOf  vec:contains .

vec:DefaultDimensionType
        rdf:type         owl:Class;
        rdfs:comment     "The dimensionType defines to which measurements this DefaultDimension applies.\n"@en;
        rdfs:label       "DefaultDimensionType"@en;
        rdfs:subClassOf  vec:OpenEnumeration .

vec:occurrenceOrUsageViewItem3DOccurrenceOrUsage
        rdf:type      owl:ObjectProperty;
        rdfs:comment  "Specifies the OccurrenceOrUsages which are represented by the view item. Important: To use one OccurenceOrUsageViewItem for multiple OccurrenceOrUsages is only valid, if the referenced items are true alternatives to each other. That means, they must have an identical placement, the geometrical models used for each item must be substitutable and the item must be mutually exclusive to each other.\n"@en;
        rdfs:domain   vec:OccurrenceOrUsageViewItem3D;
        rdfs:label    "occurrenceOrUsage"@en;
        rdfs:range    vec:OccurrenceOrUsage .

vec:TubeShape  rdf:type  owl:Class;
        rdfs:comment     "Defines valid shapes of the cross section of a tube.\n"@en;
        rdfs:label       "TubeShape"@en;
        rdfs:subClassOf  vec:OpenEnumeration .

vec:USUnitName_Acre  rdf:type  vec:USUnitName , owl:NamedIndividiual;
        vec:enumLiteral  "Acre" .

vec:transformation3DA31
        rdf:type     owl:DatatypeProperty;
        rdfs:domain  vec:Transformation3D;
        rdfs:label   "a31"@en;
        rdfs:range   xs:double .

vec:orderedIndex  rdf:type  owl:DataProperty;
        rdfs:comment  "Defines the order of Ordered elements. Lower indices are further forward in a list. 0 is the lowest index, i.e. the first element."@en;
        rdfs:domain   vec:Ordered;
        rdfs:range    xs:nonNegativeInteger .

vec:wireSpecificationWireElement
        rdf:type            owl:ObjectProperty;
        rdfs:comment        "Specifies the WireElement that represents the root of the WireSpecification .\n"@en;
        rdfs:domain         vec:WireSpecification;
        rdfs:label          "wireElement"@en;
        rdfs:range          vec:WireElement;
        rdfs:subPropertyOf  vec:contains .

vec:TerminalSealingType_Sealed
        rdf:type         vec:TerminalSealingType , owl:NamedIndividiual;
        rdfs:comment     "The Terminal can be sealed and can only be used together with a cavity seal. It is not allowed to be used unsealed.\n"@en;
        vec:enumLiteral  "Sealed" .

vec:componentConnectorDescription
        rdf:type            owl:ObjectProperty;
        rdfs:domain         vec:ComponentConnector;
        rdfs:label          "description"@en;
        rdfs:range          vec:AbstractLocalizedString;
        rdfs:subPropertyOf  vec:contains .

vec:CompositeUnit  rdf:type  owl:Class;
        rdfs:comment     "Defines a unit as a composition of other units. The composition is done by multiplying the different other units. By this way combined units like kg/m can be formed.\n"@en;
        rdfs:label       "CompositeUnit"@en;
        rdfs:subClassOf  vec:Unit .

vec:CableLeadThroughSpecification
        rdf:type         owl:Class;
        rdfs:comment     "A CableLeadThrough specifies a hole in the grommet through which wires can pass through the grommet. The CableLeadThroughSpecification defines the technical properties of a CableLeadThrough (or a set of similar ones).\n"@en;
        rdfs:label       "CableLeadThroughSpecification"@en;
        rdfs:subClassOf  vec:Specification .

vec:GrommetRole  rdf:type  owl:Class;
        rdfs:comment     "A GrommetRole defines the instance specific properties and relationships of a grommet.\n"@en;
        rdfs:label       "GrommetRole"@en;
        rdfs:subClassOf  vec:Role .

vec:connectionEndConnectedComponentPort
        rdf:type      owl:ObjectProperty;
        rdfs:comment  "References the ComponentPort that is connected by the ConnectionEnd. \n"@en;
        rdfs:domain   vec:ConnectionEnd;
        rdfs:label    "connectedComponentPort"@en;
        rdfs:range    vec:ComponentPort .

vec:PinTimingType_CurrentPeakDistances
        rdf:type         vec:PinTimingType , owl:NamedIndividiual;
        vec:enumLiteral  "currentPeakDistances" .

vec:pinComponentBehaviorPinType
        rdf:type            owl:ObjectProperty;
        rdfs:comment        "Specifies the PinType of the PinComponent .\n"@en;
        rdfs:domain         vec:PinComponentBehavior;
        rdfs:label          "pinType"@en;
        rdfs:range          vec:PinType;
        rdfs:subPropertyOf  vec:contains .

vec:BaselineState_Draft
        rdf:type         vec:BaselineState , owl:NamedIndividiual;
        rdfs:comment     "Draft means that the baseline is not finalized yet and new ItemVersions can be added without the necessity to create a new version of the baseline itself.\n"@en;
        vec:enumLiteral  "Draft" .

<http://www.prostep.org/ontologies/ecad/2024/03/vec#TerminalBoltNominalSize_1%2F2>
        rdf:type         vec:TerminalBoltNominalSize , owl:NamedIndividiual;
        vec:enumLiteral  "1/2" .

vec:fillerSpecificationMaterial
        rdf:type            owl:ObjectProperty;
        rdfs:comment        "Specifies the material of the filler.\n"@en;
        rdfs:domain         vec:FillerSpecification;
        rdfs:label          "material"@en;
        rdfs:range          vec:Material;
        rdfs:subPropertyOf  vec:contains .

vec:cavityCouplingIdentification
        rdf:type     owl:DatatypeProperty;
        rdfs:domain  vec:CavityCoupling;
        rdfs:label   "identification"@en;
        rdfs:range   xs:string .

vec:usageNodeSpecificationUsageNodes
        rdf:type            owl:ObjectProperty;
        rdfs:comment        "Specifies the UsageNodes defined by this UsageNodeSpecification.\n"@en;
        rdfs:domain         vec:UsageNodeSpecification;
        rdfs:label          "usageNodes"@en;
        rdfs:range          vec:UsageNode;
        rdfs:subPropertyOf  vec:contains .

vec:contractContractRole
        rdf:type            owl:ObjectProperty;
        rdfs:comment        "The role the company takes in reference to the associated ItemVersion. Predefined are the values: OEM, Supplier and Manufacturer.\n"@en;
        rdfs:domain         vec:Contract;
        rdfs:label          "contractRole"@en;
        rdfs:range          vec:ContractRole;
        rdfs:subPropertyOf  vec:contains .

vec:connectionConnectionEnd
        rdf:type            owl:ObjectProperty;
        rdfs:comment        "Specifies the ConnectionEnds of the Connection. "@en;
        rdfs:domain         vec:Connection;
        rdfs:label          "connectionEnd"@en;
        rdfs:range          vec:ConnectionEnd;
        rdfs:subPropertyOf  vec:contains .

vec:ComponentNodeType_Actuator
        rdf:type         vec:ComponentNodeType , owl:NamedIndividiual;
        rdfs:comment     "An actuator is a device that is responsible for controlling or moving a mechanism.\n"@en;
        vec:enumLiteral  "Actuator" .

vec:variantCodeSpecificationVariantCode
        rdf:type            owl:ObjectProperty;
        rdfs:comment        "Specifies the individual VariantCodes defined in the VariantCodeSpecification.\n"@en;
        rdfs:domain         vec:VariantCodeSpecification;
        rdfs:label          "variantCode"@en;
        rdfs:range          vec:VariantCode;
        rdfs:subPropertyOf  vec:contains .

vec:usageConstraintToDate
        rdf:type      owl:DatatypeProperty;
        rdfs:comment  "Specifies the upper bound of the time period to which the usage constraint applies.\n"@en;
        rdfs:domain   vec:UsageConstraint;
        rdfs:label    "toDate"@en;
        rdfs:range    xs:dateTime .

vec:usageConstraintProject
        rdf:type      owl:ObjectProperty;
        rdfs:comment  "References the Projects to which the UsageConstraint applies. This means the described PartVersion is allowed / denied in the referenced UsageConstraint.\n"@en;
        rdfs:domain   vec:UsageConstraint;
        rdfs:label    "project"@en;
        rdfs:range    vec:Project .

vec:partOccurrenceRealizedPartUsage
        rdf:type      owl:ObjectProperty;
        rdfs:comment  "References the PartUsages that are realized by the PartOccurrence. \n"@en;
        rdfs:domain   vec:PartOccurrence;
        rdfs:label    "realizedPartUsage"@en;
        rdfs:range    vec:PartUsage .

vec:SlotLayoutType_Type_F
        rdf:type         vec:SlotLayoutType , owl:NamedIndividiual;
        rdfs:comment     "Fuse type according to ISO8820, also known as: mini\n"@en;
        vec:enumLiteral  "Type_F" .

vec:PinTimingType  rdf:type  owl:Class;
        rdfs:comment     "Defines the different available timing types of a pin.\n"@en;
        rdfs:label       "PinTimingType"@en;
        rdfs:subClassOf  vec:OpenEnumeration .

vec:shieldSpecificationWindingType
        rdf:type            owl:ObjectProperty;
        rdfs:comment        "Defines the type of winding of the shield. Should only be used for ShieldSpecifications with type=Foil.\n"@en;
        rdfs:domain         vec:ShieldSpecification;
        rdfs:label          "windingType"@en;
        rdfs:range          vec:FoilShieldWindingType;
        rdfs:subPropertyOf  vec:contains .

vec:FittingForm_Tee  rdf:type  vec:FittingForm , owl:NamedIndividiual;
        vec:enumLiteral  "Tee" .

vec:usageNodeIdentification
        rdf:type      owl:DatatypeProperty;
        rdfs:comment  "Specifies a unique identification of the UsageNode . The identification is guaranteed to be unique within the context. For all VEC-documents a UsageNode-instance can be trusted to be the same if the context-instance is the same and the identification of the UsageNode is the same.\n"@en;
        rdfs:domain   vec:UsageNode;
        rdfs:label    "identification"@en;
        rdfs:range    xs:string .

vec:antennaSpecificationFMax
        rdf:type            owl:ObjectProperty;
        rdfs:comment        "Specifies the maximum operating frequency of the antenna.\n"@en;
        rdfs:domain         vec:AntennaSpecification;
        rdfs:label          "fMax"@en;
        rdfs:range          vec:NumericalValue;
        rdfs:subPropertyOf  vec:contains .

vec:CapacitorSpecification
        rdf:type         owl:Class;
        rdfs:comment     "Specification of the electrological aspects of a capacitor.┬á\n"@en;
        rdfs:label       "CapacitorSpecification"@en;
        rdfs:subClassOf  vec:EEComponentSpecification .

vec:MultiFuseType_Stamped
        rdf:type         vec:MultiFuseType , owl:NamedIndividiual;
        vec:enumLiteral  "Stamped" .

vec:netTypeSignalInformationType
        rdf:type            owl:ObjectProperty;
        rdfs:domain         vec:NetType;
        rdfs:label          "signalInformationType"@en;
        rdfs:range          vec:SignalInformationType;
        rdfs:subPropertyOf  vec:contains .

vec:WindingType_Spare
        rdf:type         vec:WindingType , owl:NamedIndividiual;
        rdfs:comment     " Spare describes a taping with larger gaps between the rounds (German: Spar)\n"@en;
        vec:enumLiteral  "Spare" .

vec:CavityGeometry_Circular
        rdf:type         vec:CavityGeometry , owl:NamedIndividiual;
        rdfs:comment     ""@en;
        vec:enumLiteral  "Circular" .

vec:eEComponentRoleExtensionSlotRef
        rdf:type            owl:ObjectProperty;
        rdfs:comment        "Specifies the ExtensionSlotReferences used in the EEComponentRole. "@en;
        rdfs:domain         vec:EEComponentRole;
        rdfs:label          "extensionSlotRef"@en;
        rdfs:range          vec:ExtensionSlotReference;
        rdfs:subPropertyOf  vec:contains .

vec:partVersionIsPreferredPart
        rdf:type      owl:DatatypeProperty;
        rdfs:comment  "Flags a part as \"preferred\" by the means of being a preferred part out of a group of parts with identical technical properties. The preferred part should be used, if the other properties of a couple of parts do not allow a distinct decision.\nEven though the name suggests a boolean value, this attribute has the type \"string\". The way in which preference is expressed varies greatly between the process and usually it is a multi-value flag and not just a yes/no answer.\n"@en;
        rdfs:domain   vec:PartVersion;
        rdfs:label    "isPreferredPart"@en;
        rdfs:range    xs:string .

vec:connectionGroupDescription
        rdf:type            owl:ObjectProperty;
        rdfs:comment        "Room for additional, human readable information about the ConnectionGroup.\n"@en;
        rdfs:domain         vec:ConnectionGroup;
        rdfs:label          "description"@en;
        rdfs:range          vec:AbstractLocalizedString;
        rdfs:subPropertyOf  vec:contains .

vec:LocalizedTypedString
        rdf:type         owl:Class;
        rdfs:comment     "Allows the internationalization of text contents in a typed way. Attributes of the type LocalizedTypedString normally have the multiplicity [0..*]. This means that such an attribute can have multiple values for different locales and types. It must not have multiple values for the same locale and type."@en;
        rdfs:label       "LocalizedTypedString"@en;
        rdfs:subClassOf  vec:AbstractLocalizedString .

vec:variantCodeCodeType
        rdf:type            owl:ObjectProperty;
        rdfs:comment        "Allows the classification of a VariantCodes.\n"@en;
        rdfs:domain         vec:VariantCode;
        rdfs:label          "codeType"@en;
        rdfs:range          vec:VariantCodeType;
        rdfs:subPropertyOf  vec:contains .

vec:uSUnitUsUnitName  rdf:type  owl:ObjectProperty;
        rdfs:comment        "Specifies the name of the USUnit .\n"@en;
        rdfs:domain         vec:USUnit;
        rdfs:label          "usUnitName"@en;
        rdfs:range          vec:USUnitName;
        rdfs:subPropertyOf  vec:contains .

vec:PrimaryPartType_ConnectorHousing
        rdf:type         vec:PrimaryPartType , owl:NamedIndividiual;
        vec:enumLiteral  "ConnectorHousing" .

vec:TerminalBoltNominalSize_M2.5
        rdf:type         vec:TerminalBoltNominalSize , owl:NamedIndividiual;
        vec:enumLiteral  "M2.5" .

vec:LanguageCode_Ug  rdf:type  vec:LanguageCode , owl:NamedIndividiual;
        vec:enumLiteral  "Ug" .

vec:housingComponentPinComponent
        rdf:type            owl:ObjectProperty;
        rdfs:comment        "Specifies the PinComponents of HousingComponent. \n\n(see KBLFRM-300)\n"@en;
        rdfs:domain         vec:HousingComponent;
        rdfs:label          "pinComponent"@en;
        rdfs:range          vec:PinComponent;
        rdfs:subPropertyOf  vec:contains .

vec:segmentMappingInnerSegment
        rdf:type     owl:ObjectProperty;
        rdfs:domain  vec:SegmentMapping;
        rdfs:label   "innerSegment"@en;
        rdfs:range   vec:TopologySegment .

vec:OpenEnumeration  rdf:type  owl:Class;
        rdfs:comment     "Classes in the model where some value can be enumerated, but not all values are known (Open)."@en;
        rdfs:label       "OpenEnumeration"@en;
        rdfs:subClassOf  vec:Enumeration .

vec:ferriteRoleNumberOfWindings
        rdf:type      owl:DatatypeProperty;
        rdfs:comment  "Defines the of windings that the wires are wound around the ferrite.\n"@en;
        rdfs:domain   vec:FerriteRole;
        rdfs:label    "numberOfWindings"@en;
        rdfs:range    xs:integer .

vec:wireEndAccessoryRoleWireEndAccessorySpecification
        rdf:type      owl:ObjectProperty;
        rdfs:comment  "References the WireEndAccessorySpecification that is instanced by this WireEndAccessoryRole.\n"@en;
        rdfs:domain   vec:WireEndAccessoryRole;
        rdfs:label    "wireEndAccessorySpecification"@en;
        rdfs:range    vec:WireEndAccessorySpecification .

vec:SiPrefix_Deci  rdf:type  vec:SiPrefix , owl:NamedIndividiual;
        vec:enumLiteral  "Deci" .

vec:SlotSpecification
        rdf:type         owl:Class;
        rdfs:comment     "Specification for the definition of slots.\n"@en;
        rdfs:label       "SlotSpecification"@en;
        rdfs:subClassOf  vec:Specification .

vec:NetworkPortViewItemSide_Right
        rdf:type         vec:NetworkPortViewItemSide , owl:NamedIndividiual;
        vec:enumLiteral  "Right" .

vec:PinVoltageInformation
        rdf:type      owl:Class;
        rdfs:comment  "Allows the definition of voltages for a pin of an EEComponent . A current can be further specified by a duration. Attributes of the type PinVoltageInformation normally have the multiplicity [0..*]. This means that such an attribute can have PinVoltageInformation entries for different types and durations. It must not have multiple entries for the same type and duration.\n"@en;
        rdfs:label    "PinVoltageInformation"@en .

vec:SignalForm_SquareWave
        rdf:type         vec:SignalForm , owl:NamedIndividiual;
        vec:enumLiteral  "squareWave" .

vec:SiPrefix_Yotta  rdf:type  vec:SiPrefix , owl:NamedIndividiual;
        vec:enumLiteral  "Yotta" .

vec:modularSlotReferenceUsedInserts
        rdf:type      owl:ObjectProperty;
        rdfs:comment  "References the inserts that are used in this ModularSlotReference. More than one insert is valid in the case variant dependent equipment of the slot.\n"@en;
        rdfs:domain   vec:ModularSlotReference;
        rdfs:label    "usedInserts"@en;
        rdfs:range    vec:ConnectorHousingRole .

vec:NetworkNodeSubType_Fuse
        rdf:type         vec:NetworkNodeSubType , owl:NamedIndividiual;
        vec:enumLiteral  "Fuse" .

vec:tapeSpecificationWidth
        rdf:type            owl:ObjectProperty;
        rdfs:comment        "Specifies the width of the tape.\n"@en;
        rdfs:domain         vec:TapeSpecification;
        rdfs:label          "width"@en;
        rdfs:range          vec:NumericalValue;
        rdfs:subPropertyOf  vec:contains .

vec:LanguageCode_Ik  rdf:type  vec:LanguageCode , owl:NamedIndividiual;
        vec:enumLiteral  "Ik" .

vec:abstractSlotCoding
        rdf:type            owl:ObjectProperty;
        rdfs:comment        "Defines coding of the slot that is satisfied by the Slot.\n"@en;
        rdfs:domain         vec:AbstractSlot;
        rdfs:label          "coding"@en;
        rdfs:range          vec:Coding;
        rdfs:subPropertyOf  vec:contains .

vec:topologySegmentIdentification
        rdf:type      owl:DatatypeProperty;
        rdfs:comment  "Specifies a unique identification of the TopologySegment. The identification is guaranteed to be unique within the TopologySpecification. For all VEC-documents a TopologySegment-instance can be trusted to be the same if the TopologySpecification-instance is the same (see TopologySpecification) and the identification of the TopologySegment is the same.\n"@en;
        rdfs:domain   vec:TopologySegment;
        rdfs:label    "identification"@en;
        rdfs:range    xs:string .

vec:MultiFuseType_Clinched
        rdf:type         vec:MultiFuseType , owl:NamedIndividiual;
        vec:enumLiteral  "Clinched" .

vec:CableLeadThroughType_Overmolded
        rdf:type         vec:CableLeadThroughType , owl:NamedIndividiual;
        vec:enumLiteral  "Overmolded" .

vec:ringTerminalSpecificationBoltDiameter
        rdf:type            owl:ObjectProperty;
        rdfs:comment        "Specifies the diameter of the bolt for which the ring terminal is designed for in a numerical way.\n"@en;
        rdfs:domain         vec:RingTerminalSpecification;
        rdfs:label          "boltDiameter"@en;
        rdfs:range          vec:NumericalValue;
        rdfs:subPropertyOf  vec:contains .

vec:wireMountingDetailContactedWireReception
        rdf:type      owl:ObjectProperty;
        rdfs:comment  "References the WireReception that is used for the WireMounting. \n"@en;
        rdfs:domain   vec:WireMountingDetail;
        rdfs:label    "contactedWireReception"@en;
        rdfs:range    vec:WireReceptionReference .

vec:LanguageCode_Yi  rdf:type  vec:LanguageCode , owl:NamedIndividiual;
        vec:enumLiteral  "Yi" .

vec:wireElementReferenceLabelingTechnology
        rdf:type            owl:ObjectProperty;
        rdfs:comment        "Specifies the used LabelingTechnology , if this WireElementReference is labled."@en;
        rdfs:domain         vec:WireElementReference;
        rdfs:label          "labelingTechnology"@en;
        rdfs:range          vec:LabelingTechnology;
        rdfs:subPropertyOf  vec:contains .

vec:geometrySegment2DStartNode
        rdf:type      owl:ObjectProperty;
        rdfs:comment  "References the GeometryNode2D where the GeometrySegment2D starts. \n"@en;
        rdfs:domain   vec:GeometrySegment2D;
        rdfs:label    "startNode"@en;
        rdfs:range    vec:GeometryNode2D .

vec:NodeType  rdf:type   owl:Class;
        rdfs:comment     "Enumeration for the definition of the type of a TopologyNode.\n"@en;
        rdfs:label       "NodeType"@en;
        rdfs:subClassOf  vec:OpenEnumeration .

vec:NumericalValue  rdf:type  owl:Class;
        rdfs:comment     "A quantity expressed with a numerical value and a unit.\n"@en;
        rdfs:label       "NumericalValue"@en;
        rdfs:subClassOf  vec:ValueWithUnit .

vec:personFirstName  rdf:type  owl:DatatypeProperty;
        rdfs:comment  "Specifies the person's first name.\n"@en;
        rdfs:domain   vec:Person;
        rdfs:label    "firstName"@en;
        rdfs:range    xs:string .

vec:occurrenceOrUsageViewItem2DGridSquare
        rdf:type      owl:DatatypeProperty;
        rdfs:comment  "Specifies the grid square in which the OccurrenceOrUsageViewItem2D is placed (e.g. E/40).\n"@en;
        rdfs:domain   vec:OccurrenceOrUsageViewItem2D;
        rdfs:label    "gridSquare"@en;
        rdfs:range    xs:string .

vec:LanguageCode_Kl  rdf:type  vec:LanguageCode , owl:NamedIndividiual;
        vec:enumLiteral  "Kl" .

vec:SignalDirection_Out
        rdf:type         vec:SignalDirection , owl:NamedIndividiual;
        vec:enumLiteral  "Out" .

vec:grommetSpecificationGrommetType
        rdf:type            owl:ObjectProperty;
        rdfs:comment        "Specifies the type of the grommet.\n"@en;
        rdfs:domain         vec:GrommetSpecification;
        rdfs:label          "grommetType"@en;
        rdfs:range          vec:GrommetType;
        rdfs:subPropertyOf  vec:contains .

vec:UsageConstraint  rdf:type  owl:Class;
        rdfs:comment     "Specifies a constraint of the possible usages for PartVersion or PartUsages. UsageConstraints are of part master data information. UsageConstraints specify general restrictions for the application of a PartVersion or PartUsage (e.g. a certain period of time in which the part is allowed to be used). (see KBLFRM-229)\n"@en;
        rdfs:label       "UsageConstraint"@en;
        rdfs:subClassOf  vec:ExtendableElement .

vec:LanguageCode_Sk  rdf:type  vec:LanguageCode , owl:NamedIndividiual;
        vec:enumLiteral  "Sk" .

vec:variantStructureNodeAliasId
        rdf:type            owl:ObjectProperty;
        rdfs:comment        "Room to specify additional identifiers for the VariantStructureNode .\n"@en;
        rdfs:domain         vec:VariantStructureNode;
        rdfs:label          "aliasId"@en;
        rdfs:range          vec:AliasIdentification;
        rdfs:subPropertyOf  vec:contains .

vec:corrugatedPipeSpecificationCorrugationHeight
        rdf:type            owl:ObjectProperty;
        rdfs:comment        "Specifies the height of a corrugation of the pipe.\n"@en;
        rdfs:domain         vec:CorrugatedPipeSpecification;
        rdfs:label          "corrugationHeight"@en;
        rdfs:range          vec:NumericalValue;
        rdfs:subPropertyOf  vec:contains .

vec:WireTupleSpecification
        rdf:type         owl:Class;
        rdfs:comment     "A Specification to define requirements for the handling of wire / wire element tuples (pairs, triple,...) with the focus on twisting. More precisely, the allowed untwisting at the wire ends and required measures against it.\nThis definition is made independent from the WireGroup , as the might be defined for the part master data (the wire on the roller). The specifications for untwisting are based on the concrete usage.\n"@en;
        rdfs:label       "WireTupleSpecification"@en;
        rdfs:subClassOf  vec:Specification .

vec:PluggableTerminalRole
        rdf:type         owl:Class;
        rdfs:comment     "A PluggableTerminalRole defines the instance specific properties and relationships of a pluggable terminal.\n"@en;
        rdfs:label       "PluggableTerminalRole"@en;
        rdfs:subClassOf  vec:TerminalRole .

vec:LanguageCode_En  rdf:type  vec:LanguageCode , owl:NamedIndividiual;
        vec:enumLiteral  "En" .

vec:itemVersionChangeDescription
        rdf:type            owl:ObjectProperty;
        rdfs:comment        "Specifies the change history of the ItemVersion. \n"@en;
        rdfs:domain         vec:ItemVersion;
        rdfs:label          "changeDescription"@en;
        rdfs:range          vec:ChangeDescription;
        rdfs:subPropertyOf  vec:contains .

vec:TransmissionMediumType
        rdf:type         owl:Class;
        rdfs:comment     "OpenEnumeration of the different transmission mediums in wire elements."@en;
        rdfs:label       "TransmissionMediumType"@en;
        rdfs:subClassOf  vec:OpenEnumeration .

vec:GrommetType_BendProtection
        rdf:type         vec:GrommetType , owl:NamedIndividiual;
        vec:enumLiteral  "BendProtection" .

vec:PinComponentBehavior
        rdf:type         owl:Class;
        rdfs:comment     "A PinComponentBehavior specifies the electrical behavior of a PinComponent. Since the behavior of a pin is configuration dependent (e.g. the software deployed on an ECU) the PinComponentBehavior inherits from ConfigurableElement. Therefore, a PinComponent can specify multiple PinComponentBehavior.\n"@en;
        rdfs:label       "PinComponentBehavior"@en;
        rdfs:subClassOf  vec:ConfigurableElement .

vec:CavityGeometry_Octagon
        rdf:type         vec:CavityGeometry , owl:NamedIndividiual;
        vec:enumLiteral  "Octagon" .

vec:ringTerminalSpecificationTorsionProtection
        rdf:type      owl:DatatypeProperty;
        rdfs:comment  "Specifies if the ring terminal is torsion protected or not. (see KBLFRM-311)\n"@en;
        rdfs:domain   vec:RingTerminalSpecification;
        rdfs:label    "torsionProtection"@en;
        rdfs:range    xs:boolean .

vec:ComponentPortViewItemSide_Top
        rdf:type         vec:ComponentPortViewItemSide , owl:NamedIndividiual;
        vec:enumLiteral  "Top" .

vec:wireElementReferenceIdentification
        rdf:type      owl:DatatypeProperty;
        rdfs:comment  "Specifies a unique identification of the WireElementReference. The identification is guaranteed to be unique within the WireRole.\n"@en;
        rdfs:domain   vec:WireElementReference;
        rdfs:label    "identification"@en;
        rdfs:range    xs:string .

vec:SiUnitName_Coulomb
        rdf:type         vec:SiUnitName , owl:NamedIndividiual;
        vec:enumLiteral  "Coulomb" .

vec:PartStructureContentType_Harness
        rdf:type         vec:PartStructureContentType , owl:NamedIndividiual;
        rdfs:comment     "A definition of harness, containing variance (150%)."@en;
        vec:enumLiteral  "Harness" .

vec:occurrenceOrUsageViewItem2DIdentification
        rdf:type      owl:DatatypeProperty;
        rdfs:comment  "Specifies a unique identification of the OccurrenceOrUsageViewItem2D. The identification is guaranteed to be unique within the BuildingBlockSpecification2D.\n"@en;
        rdfs:domain   vec:OccurrenceOrUsageViewItem2D;
        rdfs:label    "identification"@en;
        rdfs:range    xs:string .

vec:documentVersionDataFormat
        rdf:type      owl:DatatypeProperty;
        rdfs:comment  "The dataFormat specifies the convention that was used to structure the information in the document. This is useful if the DocumentVersion is a pointer to an external document, which is not contained in the VEC or if the content of this DocumentVersion was automatically generated by the extraction of the information out of the original document.\n"@en;
        rdfs:domain   vec:DocumentVersion;
        rdfs:label    "dataFormat"@en;
        rdfs:range    xs:string .

vec:buildingBlockSpecification3DCartesianPoint
        rdf:type            owl:ObjectProperty;
        rdfs:comment        "Specifies the CartesianPoint3Ds that are used in the BuildingBlockSpecification3D.\n"@en;
        rdfs:domain         vec:BuildingBlockSpecification3D;
        rdfs:label          "cartesianPoint"@en;
        rdfs:range          vec:CartesianPoint3D;
        rdfs:subPropertyOf  vec:contains .

vec:signalSignalSubType
        rdf:type            owl:ObjectProperty;
        rdfs:domain         vec:Signal;
        rdfs:label          "signalSubType"@en;
        rdfs:range          vec:SignalSubType;
        rdfs:subPropertyOf  vec:contains .

vec:UsageConstraintType_Allow
        rdf:type         vec:UsageConstraintType , owl:NamedIndividiual;
        vec:enumLiteral  "Allow" .

vec:PartUsage  rdf:type  owl:Class;
        rdfs:comment     "PartUsages shall be used for the specification of the elements on an electrical system wiring plan and for the specification of the elements on a pure geometry description. PartUsages shall more than ever be used in cases where it is necessary to describe a certain instance of a part or part group, possibly together with certain technical properties, but where it is at the same time yet not possible to define a concrete part number.\n"@en;
        rdfs:label       "PartUsage"@en;
        rdfs:subClassOf  vec:OccurrenceOrUsage .

vec:MultiFuseType_OverMolded
        rdf:type         vec:MultiFuseType , owl:NamedIndividiual;
        vec:enumLiteral  "OverMolded" .

vec:RequirementsConformanceStatement
        rdf:type      owl:Class;
        rdfs:comment  "A RequirementsConformanceStatement states that the PartVersions referenced by the parent RequirementsConformanceSpecification satisfy or do not satisfy the requirements defined in the associated DocumentVersion (via the requirementsSpecification association) .\n"@en;
        rdfs:label    "RequirementsConformanceStatement"@en .

vec:WireElementReference
        rdf:type         owl:Class;
        rdfs:comment     "A WireElementReference represents the usage of a WireElement in the context of a PartUsage or PartOccurrence. For contacting purposes, a WireElementReference has WireEnds. KBLFRM-384\n"@en;
        rdfs:label       "WireElementReference"@en;
        rdfs:subClassOf  vec:RoutableElement .

vec:placementIsOnTopOf
        rdf:type      owl:ObjectProperty;
        rdfs:comment  "Specifies constraints on ordering of Placements. All referenced Placements must be below (nearer to the center of the Segment) this Placement. \n(see KBLFRM-171)\n"@en;
        rdfs:domain   vec:Placement;
        rdfs:label    "isOnTopOf"@en;
        rdfs:range    vec:Placement .

vec:netSpecificationNet
        rdf:type            owl:ObjectProperty;
        rdfs:comment        "Specifies the Nets defined in the NetSpecification.\n"@en;
        rdfs:domain         vec:NetSpecification;
        rdfs:label          "net"@en;
        rdfs:range          vec:Net;
        rdfs:subPropertyOf  vec:contains .

vec:generalTechnicalPartSpecificationFitRate
        rdf:type      owl:DatatypeProperty;
        rdfs:comment  "The Failures In Time (FIT) rate of a device is the number of failures that can be expected in one billion (109) device-hours of operation.[14]┬á(E.g. 1000 devices for 1 million hours, or 1 million devices for 1000 hours each, or some other combination.) (see https://en.wikipedia.org/wiki/Failure_rate#Units )\n"@en;
        rdfs:domain   vec:GeneralTechnicalPartSpecification;
        rdfs:label    "fitRate"@en;
        rdfs:range    xs:double .

vec:SlotLayoutType_USBMicroABSuperSpeed
        rdf:type         vec:SlotLayoutType , owl:NamedIndividiual;
        vec:enumLiteral  "USBMicroABSuperSpeed" .

vec:variantGroupDescription
        rdf:type            owl:ObjectProperty;
        rdfs:comment        "On optional human readable description of the variant group.\n"@en;
        rdfs:domain         vec:VariantGroup;
        rdfs:label          "description"@en;
        rdfs:range          vec:AbstractLocalizedString;
        rdfs:subPropertyOf  vec:contains .

vec:wireSpecificationWireElementSpecification
        rdf:type      owl:ObjectProperty;
        rdfs:comment  "References the WireElementSpecification that defines the properties of the top-most WireElement.\n"@en;
        rdfs:domain   vec:WireSpecification;
        rdfs:label    "wireElementSpecification"@en;
        rdfs:range    vec:WireElementSpecification .

vec:CableLeadThroughGeometry
        rdf:type         owl:Class;
        rdfs:comment     "Defines valid values for the geometry of a CableLeadThrough in the sealing area.\n"@en;
        rdfs:label       "CableLeadThroughGeometry"@en;
        rdfs:subClassOf  vec:OpenEnumeration .

vec:applicationConstraintBaseInclusion
        rdf:type      owl:ObjectProperty;
        rdfs:comment  "An ApplicationConstraint can only be satisfied if its baseInclusion is satisfied as well.┬á\n"@en;
        rdfs:domain   vec:ApplicationConstraint;
        rdfs:label    "baseInclusion"@en;
        rdfs:range    vec:ApplicationConstraint .

vec:wireElementIdentification
        rdf:type      owl:DatatypeProperty;
        rdfs:comment  "The identification of the WireElement. The identification is guaranteed to be unique within a wire and immutable. The identification is guaranteed to be the same for the same WireElement over different VEC documents.\n"@en;
        rdfs:domain   vec:WireElement;
        rdfs:label    "identification"@en;
        rdfs:range    xs:string .

vec:moduleListSpecificationModuleListConfiguration
        rdf:type            owl:ObjectProperty;
        rdfs:comment        "Specifies the ModuleLists defined in the ModuleListSpecification.\n"@en;
        rdfs:domain         vec:ModuleListSpecification;
        rdfs:label          "moduleListConfiguration"@en;
        rdfs:range          vec:ModuleList;
        rdfs:subPropertyOf  vec:contains .

vec:GeometrySegment3D
        rdf:type         owl:Class;
        rdfs:comment     "A GeometrySegment3D is the geometric representation of a TopologySegment in 3D-space.\n"@en;
        rdfs:label       "GeometrySegment3D"@en;
        rdfs:subClassOf  vec:GeometrySegment .

vec:PrimaryPartType_OpenWireEnd
        rdf:type         vec:PrimaryPartType , owl:NamedIndividiual;
        vec:enumLiteral  "OpenWireEnd" .

vec:AbstractLocalizedString
        rdf:type      owl:Class;
        rdfs:comment  "Abstract super-class for Localized text values. "@en;
        rdfs:label    "AbstractLocalizedString"@en .

vec:AliasIdentification
        rdf:type      owl:Class;
        rdfs:comment  "Class for the definition of alias identifications. Alias identifications are additional identifications for VEC-elements, which are valid in a certain scope (e.g. PPS-ID's).\n"@en;
        rdfs:label    "AliasIdentification"@en .

vec:documentBasedInstructionReferencedSheetOrChapter
        rdf:type      owl:ObjectProperty;
        rdfs:comment  "References the SheetOrChapter that is used as an Instruction.\n"@en;
        rdfs:domain   vec:DocumentBasedInstruction;
        rdfs:label    "referencedSheetOrChapter"@en;
        rdfs:range    vec:SheetOrChapter .

vec:VecVersion_1.2.2  rdf:type  vec:VecVersion , owl:NamedIndividiual;
        vec:enumLiteral  "1.2.2" .

vec:relaySpecificationIMax
        rdf:type            owl:ObjectProperty;
        rdfs:comment        "Specifies the maximum current allowed for the relais.\n"@en;
        rdfs:domain         vec:RelaySpecification;
        rdfs:label          "iMax"@en;
        rdfs:range          vec:NumericalValue;
        rdfs:subPropertyOf  vec:contains .

vec:SlotLayoutType_USBMicroASuperSpeed
        rdf:type         vec:SlotLayoutType , owl:NamedIndividiual;
        vec:enumLiteral  "USBMicroASuperSpeed" .

vec:LanguageCode_Es  rdf:type  vec:LanguageCode , owl:NamedIndividiual;
        vec:enumLiteral  "Es" .

vec:LabelPosition  rdf:type  owl:Class;
        rdfs:comment     "Open Enumeration of standard label positions on WireElementReferences. "@en;
        rdfs:label       "LabelPosition"@en;
        rdfs:subClassOf  vec:OpenEnumeration .

vec:PinCurrentType_OverrunCurrent
        rdf:type         vec:PinCurrentType , owl:NamedIndividiual;
        vec:enumLiteral  "overrunCurrent" .

vec:NetworkNodeType_OpenEnd
        rdf:type         vec:NetworkNodeType , owl:NamedIndividiual;
        rdfs:comment     "Defines that this NetworkNode is the end point for some unconnected nets that require wires and routings in the resulting harness (e.g. an antenna). A NetworkNode of this type is used whenever nets shall not be connected (on one side).\n"@en;
        vec:enumLiteral  "OpenEnd" .

vec:LabelingTechnology_Lasered
        rdf:type         vec:LabelingTechnology , owl:NamedIndividiual;
        vec:enumLiteral  "Lasered" .

vec:approvalStatus  rdf:type  owl:ObjectProperty;
        rdfs:comment        "The approval level concerning approval status. Predefined are the values: NotYetApproved, Approved and Withdrawn. The status refers to the status of the Approval , not the status of the ItemVersion. So, e.g. withdrawn means the approval (with its corresponding level) has been withdrawn, not the ItemVersion itself.\n"@en;
        rdfs:domain         vec:Approval;
        rdfs:label          "status"@en;
        rdfs:range          vec:StatusOfApproval;
        rdfs:subPropertyOf  vec:contains .

vec:LanguageCode_Mr  rdf:type  vec:LanguageCode , owl:NamedIndividiual;
        vec:enumLiteral  "Mr" .

vec:stripeSpecificationSegmentDiameter
        rdf:type            owl:ObjectProperty;
        rdfs:comment        "Specifies the valid segment diameter range for which the stripe can be used.\n"@en;
        rdfs:domain         vec:StripeSpecification;
        rdfs:label          "segmentDiameter"@en;
        rdfs:range          vec:ValueRange;
        rdfs:subPropertyOf  vec:contains .

vec:cableLeadThroughIdentification
        rdf:type      owl:DatatypeProperty;
        rdfs:comment  "Specifies the identification of the CableLeadThrough. This must be unique within a GrommetSpecification.\n"@en;
        rdfs:domain   vec:CableLeadThrough;
        rdfs:label    "identification"@en;
        rdfs:range    xs:string .

vec:ConnectionEndGender
        rdf:type         owl:Class;
        rdfs:comment     "Defines the gender of a connetion end.\n"@en;
        rdfs:label       "ConnectionEndGender"@en;
        rdfs:subClassOf  vec:OpenEnumeration .

vec:AntennaSpecification
        rdf:type         owl:Class;
        rdfs:comment     "Specification of the electrological aspects of an antenna.\n"@en;
        rdfs:label       "AntennaSpecification"@en;
        rdfs:subClassOf  vec:EEComponentSpecification .

vec:SlotLayoutType_Type_A1S
        rdf:type         vec:SlotLayoutType , owl:NamedIndividiual;
        rdfs:comment     "Fuse type according to ISO8820, also known as: flat\n"@en;
        vec:enumLiteral  "Type_A1S" .

vec:occurrenceOrUsageViewItem2DAliasId
        rdf:type            owl:ObjectProperty;
        rdfs:comment        "Specifies additional identifiers for the OccurrenceOrUsageViewItem2D.\n"@en;
        rdfs:domain         vec:OccurrenceOrUsageViewItem2D;
        rdfs:label          "aliasId"@en;
        rdfs:range          vec:AliasIdentification;
        rdfs:subPropertyOf  vec:contains .

vec:harnessDrawingSpecification2DBuildingBlockPositionings
        rdf:type            owl:ObjectProperty;
        rdfs:comment        "Specifies the BuildingBlockPositioning2Ds that are forming the 2D harness drawing. \n"@en;
        rdfs:domain         vec:HarnessDrawingSpecification2D;
        rdfs:label          "buildingBlockPositionings"@en;
        rdfs:range          vec:BuildingBlockPositioning2D;
        rdfs:subPropertyOf  vec:contains .

vec:connectionNodeViewItemIdentification
        rdf:type      owl:DatatypeProperty;
        rdfs:comment  "Specifies a unique identification of the ComponentNodeViewItem . The identification is guaranteed to be unique within the ConnectionViewSpecification .\n"@en;
        rdfs:domain   vec:ConnectionNodeViewItem;
        rdfs:label    "identification"@en;
        rdfs:range    xs:string .

vec:tapeRoleTapeOverlapRelative
        rdf:type      owl:DatatypeProperty;
        rdfs:comment  "Specifies the amount of overlap two rounds of taping around a segment have, as a relative value. A negative value means, that there is a gap between two rounds. Values are defined as a factor, not as a percentage. Values can be between 1.0 and negative \"infinity\". Examples: An overlap of 1.0 defines that the second round is placed exactly on top of the first one. An overlap of 0.5 specifies that one half of the second round is on top of the first round (50% overlapping), a value of 0 specifies, that there is no overlap, but also no gap. A value of -2.0 specifies that there is a gap twice the width of the tape between two rounds.\n"@en;
        rdfs:domain   vec:TapeRole;
        rdfs:label    "tapeOverlapRelative"@en;
        rdfs:range    xs:double .

vec:SiPrefix_Zepto  rdf:type  vec:SiPrefix , owl:NamedIndividiual;
        vec:enumLiteral  "Zepto" .

vec:LocalizedTypedStringType_AdditionalDescription
        rdf:type         vec:LocalizedTypedStringType , owl:NamedIndividiual;
        rdfs:comment     "An additional description that is an extension or a detailing of the MainDescription .\n"@en;
        vec:enumLiteral  "AdditionalDescription" .

vec:netTypeIdentification
        rdf:type      owl:DatatypeProperty;
        rdfs:comment  "Specifies a unique identification of the NetType. The identification is guaranteed to be unique within the NetSpecification.\n"@en;
        rdfs:domain   vec:NetType;
        rdfs:label    "identification"@en;
        rdfs:range    xs:string .

vec:TopologyZoneSpecification
        rdf:type         owl:Class;
        rdfs:comment     "Specification for the definition of TopologyZones.\n"@en;
        rdfs:label       "TopologyZoneSpecification"@en;
        rdfs:subClassOf  vec:Specification .

vec:partUsagePrimaryPartUsageType
        rdf:type            owl:ObjectProperty;
        rdfs:comment        "The primary type of the PartUsage defines the type of the described part (e.g. ConnectorHousing, Fixing, etc.) Since the VEC supports dual use parts (e.g. Fixing & WireProtection) there is no direct connection between the primaryPartUsageType and the allowed specifications for the description of a PartUsage.\n"@en;
        rdfs:domain         vec:PartUsage;
        rdfs:label          "primaryPartUsageType"@en;
        rdfs:range          vec:PrimaryPartType;
        rdfs:subPropertyOf  vec:contains .

vec:boundingBoxY  rdf:type  owl:ObjectProperty;
        rdfs:comment        "Defines the extent of the bounding box in the direction of y (width).\n"@en;
        rdfs:domain         vec:BoundingBox;
        rdfs:label          "y"@en;
        rdfs:range          vec:NumericalValue;
        rdfs:subPropertyOf  vec:contains .

vec:USUnitName_Ton  rdf:type  vec:USUnitName , owl:NamedIndividiual;
        vec:enumLiteral  "Ton" .

vec:compositionSpecificationComponent
        rdf:type            owl:ObjectProperty;
        rdfs:comment        "Specifies the PartOccurrences defined in the CompositionSpecification.\n"@en;
        rdfs:domain         vec:CompositionSpecification;
        rdfs:label          "component"@en;
        rdfs:range          vec:PartOccurrence;
        rdfs:subPropertyOf  vec:contains .

vec:componentPortNetworkPort
        rdf:type      owl:ObjectProperty;
        rdfs:comment  "References the NetworkPort that is realized by the ComponentPort.\n"@en;
        rdfs:domain   vec:ComponentPort;
        rdfs:label    "networkPort"@en;
        rdfs:range    vec:NetworkPort .

vec:LanguageCode_Iu  rdf:type  vec:LanguageCode , owl:NamedIndividiual;
        vec:enumLiteral  "Iu" .

vec:USUnitName_Thou  rdf:type  vec:USUnitName , owl:NamedIndividiual;
        vec:enumLiteral  "Thou" .

vec:tapeSpecificationThickness
        rdf:type            owl:ObjectProperty;
        rdfs:comment        "Specifies the thickness of the tape (adhesive + backing).\n"@en;
        rdfs:domain         vec:TapeSpecification;
        rdfs:label          "thickness"@en;
        rdfs:range          vec:NumericalValue;
        rdfs:subPropertyOf  vec:contains .

vec:topologySegmentStartNode
        rdf:type      owl:ObjectProperty;
        rdfs:comment  "References the TopologyNode where the TopologySegment starts. \n"@en;
        rdfs:domain   vec:TopologySegment;
        rdfs:label    "startNode"@en;
        rdfs:range    vec:TopologyNode .

vec:personLastName  rdf:type  owl:DatatypeProperty;
        rdfs:comment  "Specifies the person's last name.\n"@en;
        rdfs:domain   vec:Person;
        rdfs:label    "lastName"@en;
        rdfs:range    xs:string .

vec:wireElementReferenceWireEnd
        rdf:type            owl:ObjectProperty;
        rdfs:comment        "Specifies the ends of the WireElementReference for contacting purposes. \n"@en;
        rdfs:domain         vec:WireElementReference;
        rdfs:label          "wireEnd"@en;
        rdfs:range          vec:WireEnd;
        rdfs:subPropertyOf  vec:contains .

vec:grommetSpecificationCableLeadThrough
        rdf:type            owl:ObjectProperty;
        rdfs:comment        "Specifies the CableLeadThroughs of the Grommet. \n"@en;
        rdfs:domain         vec:GrommetSpecification;
        rdfs:label          "cableLeadThrough"@en;
        rdfs:range          vec:CableLeadThrough;
        rdfs:subPropertyOf  vec:contains .

vec:PrimaryPartType_Tube
        rdf:type         vec:PrimaryPartType , owl:NamedIndividiual;
        vec:enumLiteral  "Tube" .

vec:MultiCavitySealSpecification
        rdf:type         owl:Class;
        rdfs:comment     "Specification for cavity seals that apply to more than one cavity. A CavitySeal is a watertight non-electrical object to fill a populated Cavity. MultiCavitySeals are formed to fit into one connector / slot and to seal more than one cavity at once.\nThere are existing two types of MultiCavitySeals: In first type the MultiCavitySeal has an opening for all cavities of the connector. Each opening can be filled either with a wire (without an individual seal) or with a CavityPlug (e.g. a synthetic pin) or a MultiCavityPlug. In the second type, the MultiCavitySeal has a specific configuration of openings for some cavities of the connector. These MultiCavitySeals are sealing all cavities with an opening and a wire in it and all cavities where no opening in the MultiCavitySeal exists. For each opening that has no wire it an additional CavityPlug is needed.┬á The cavities that are left open by a MultiCavitySeal are defined with a SealedCavitiesAssignment.\n"@en;
        rdfs:label       "MultiCavitySealSpecification"@en;
        rdfs:subClassOf  vec:CavitySealSpecification .

vec:HoleMountedFixingHoleType
        rdf:type         owl:Class;
        rdfs:comment     "Open Enumeration of standard hole types (see HoleMountedFixingSpecification.holeType)."@en;
        rdfs:label       "HoleMountedFixingHoleType"@en;
        rdfs:subClassOf  vec:OpenEnumeration .

vec:PinApplianceType_ShortTerm
        rdf:type         vec:PinApplianceType , owl:NamedIndividiual;
        vec:enumLiteral  "shortTerm" .

vec:sheetOrChapterSheetVersion
        rdf:type      owl:DatatypeProperty;
        rdfs:comment  "The sheetVersion specifies the version index of a sheet (see also sheetNumber)\n"@en;
        rdfs:domain   vec:SheetOrChapter;
        rdfs:label    "sheetVersion"@en;
        rdfs:range    xs:string .

vec:WireProtectionRole
        rdf:type         owl:Class;
        rdfs:comment     "A WireProtectionRole defines the instance specific properties and relationships of a wire protection. This is a general-purpose role for instances of all types of WireProtectionSpecifications that do not have specific instance attributes. For TapeSpecifications the more specific TapeRole shall be used.\n"@en;
        rdfs:label       "WireProtectionRole"@en;
        rdfs:subClassOf  vec:Role .

vec:wireReceptionSpecificationInsulationDisplacementLength
        rdf:type            owl:ObjectProperty;
        rdfs:comment        "Specifies the length of the insulation which must be stripped off to fit to this wire reception.\n"@en;
        rdfs:domain         vec:WireReceptionSpecification;
        rdfs:label          "insulationDisplacementLength"@en;
        rdfs:range          vec:NumericalValue;
        rdfs:subPropertyOf  vec:contains .

vec:cartesianPoint2DY
        rdf:type      owl:DatatypeProperty;
        rdfs:comment  "Specifies the value of y-coordinate of the Cartesian point. The unit of this value is the baseUnit of containing BuildingBlockSpecification2D.\n"@en;
        rdfs:domain   vec:CartesianPoint2D;
        rdfs:label    "y"@en;
        rdfs:range    xs:double .

vec:tubeSpecificationWallThickness
        rdf:type            owl:ObjectProperty;
        rdfs:comment        "Specifies the thickness of the wall of the tube.\n"@en;
        rdfs:domain         vec:TubeSpecification;
        rdfs:label          "wallThickness"@en;
        rdfs:range          vec:NumericalValue;
        rdfs:subPropertyOf  vec:contains .

vec:variantConfigurationLogisticControlExpression
        rdf:type      owl:DatatypeProperty;
        rdfs:comment  "Specifies a logisticControlExpression expressed as boolean term.\n"@en;
        rdfs:domain   vec:VariantConfiguration;
        rdfs:label    "logisticControlExpression"@en;
        rdfs:range    xs:string .

vec:LanguageCode_Su  rdf:type  vec:LanguageCode , owl:NamedIndividiual;
        vec:enumLiteral  "Su" .

vec:vecContentGeneratingSystemName
        rdf:type      owl:DatatypeProperty;
        rdfs:comment  "Specifies the name of the system that has generated the VEC-file.\n"@en;
        rdfs:domain   vec:VecContent;
        rdfs:label    "generatingSystemName"@en;
        rdfs:range    xs:string .

vec:topologyMappingSpecificationOuterTopology
        rdf:type     owl:ObjectProperty;
        rdfs:domain  vec:TopologyMappingSpecification;
        rdfs:label   "outerTopology"@en;
        rdfs:range   vec:TopologySpecification .

vec:pinVoltageInformationTiming
        rdf:type            owl:ObjectProperty;
        rdfs:comment        "Specifies the timing of the PinVoltageInformation .\n"@en;
        rdfs:domain         vec:PinVoltageInformation;
        rdfs:label          "timing"@en;
        rdfs:range          vec:PinTiming;
        rdfs:subPropertyOf  vec:contains .

vec:USUnitName_AWG  rdf:type  vec:USUnitName , owl:NamedIndividiual;
        rdfs:comment     "American wire gauge (AWG), also known as the Brown & Sharpe wire gauge, is a standardized wire gauge system used in the United States and Canada.\n"@en;
        vec:enumLiteral  "AWG" .

vec:LabelPosition_End
        rdf:type         vec:LabelPosition , owl:NamedIndividiual;
        vec:enumLiteral  "End" .

vec:OccurrenceOrUsageViewItem2D
        rdf:type         owl:Class;
        rdfs:comment     "An OccurrenceOrUsageViewItem2D specifies the representation of an OccurrenceOrUsage in a 2DDrawing.\n"@en;
        rdfs:label       "OccurrenceOrUsageViewItem2D"@en;
        rdfs:subClassOf  vec:ExtendableElement .

vec:PlacementPoint  rdf:type  owl:Class;
        rdfs:comment     "Defines a point on the component which can be placed explicitly in the topology (e.g. opening in a grommet, the entry point of a connector housing). If a PlacementPoint requires further specification for a certain component type (e.g. the entry point of a connector housing), this is done by an element specific for the component type, which related to the placement point.\n"@en;
        rdfs:label       "PlacementPoint"@en;
        rdfs:subClassOf  vec:ExtendableElement .

vec:CavityPlugRole  rdf:type  owl:Class;
        rdfs:comment     "A CavityPlugRole defines the instance specific properties and relationships of a cavity plug.\n"@en;
        rdfs:label       "CavityPlugRole"@en;
        rdfs:subClassOf  vec:Role .

vec:nodeLocationReferencedNode
        rdf:type      owl:ObjectProperty;
        rdfs:comment  "References the TopologyNode on which the Location is located.\n"@en;
        rdfs:domain   vec:NodeLocation;
        rdfs:label    "referencedNode"@en;
        rdfs:range    vec:TopologyNode .

vec:CouplingSpecification
        rdf:type         owl:Class;
        rdfs:comment     "Specification for the description of a Coupling. A coupling allows the mapping between independent harness sections or EEComponents of the electrical system. This is done by the mapping of either-or both, ConnectorHousingRoles &┬áTerminalRoles of one side to the other.\n"@en;
        rdfs:label       "CouplingSpecification"@en;
        rdfs:subClassOf  vec:Specification .

vec:WireReceptionAddOn
        rdf:type      owl:Class;
        rdfs:comment  "Specifies the wire addon required for this wire reception.\n"@en;
        rdfs:label    "WireReceptionAddOn"@en .

vec:placeableElementRoleMeasurementPointReference
        rdf:type            owl:ObjectProperty;
        rdfs:comment        ""@en;
        rdfs:domain         vec:PlaceableElementRole;
        rdfs:label          "measurementPointReference"@en;
        rdfs:range          vec:MeasurementPointReference;
        rdfs:subPropertyOf  vec:contains .

vec:zoneCoverageFirstLocation
        rdf:type            owl:ObjectProperty;
        rdfs:domain         vec:ZoneCoverage;
        rdfs:label          "firstLocation"@en;
        rdfs:range          vec:Location;
        rdfs:subPropertyOf  vec:contains .

vec:ConnectionViewSpecification
        rdf:type         owl:Class;
        rdfs:comment     "The ConnectionViewSpecification supports the exchange of a basic layout for a ConnectionSpecification .\n"@en;
        rdfs:label       "ConnectionViewSpecification"@en;
        rdfs:subClassOf  vec:Specification .

vec:labelingSpecificationLabelValue
        rdf:type      owl:DatatypeProperty;
        rdfs:comment  "Specifies the value of a label printed on the component. This value applies to all components that satisfy this specification, so all instances share the same label value (e.g. a part number).\nIf instances of a component require individual labeling it has to be defined on the LabelingRole.\n"@en;
        rdfs:domain   vec:LabelingSpecification;
        rdfs:label    "labelValue"@en;
        rdfs:range    xs:string .

vec:USUnitName_FluidOunce
        rdf:type         vec:USUnitName , owl:NamedIndividiual;
        vec:enumLiteral  "FluidOunce" .

vec:partVersionWrapperItem
        rdf:type      owl:ObjectProperty;
        rdfs:comment  "References the actual item for a Wrapper.";
        rdfs:domain   vec:PartVersionWrapper;
        rdfs:range    vec:PartVersion .

vec:terminalPairingFirstTerminal
        rdf:type      owl:ObjectProperty;
        rdfs:comment  "References the first terminal of the TerminalPairing.\n"@en;
        rdfs:domain   vec:TerminalPairing;
        rdfs:label    "firstTerminal"@en;
        rdfs:range    vec:PartVersion .

vec:shrinkableTubeSpecificationMaximumLongitudinalShrinkage
        rdf:type            owl:ObjectProperty;
        rdfs:comment        "Defines the shrinkage in longitudinal direction.\n"@en;
        rdfs:domain         vec:ShrinkableTubeSpecification;
        rdfs:label          "maximumLongitudinalShrinkage"@en;
        rdfs:range          vec:NumericalValue;
        rdfs:subPropertyOf  vec:contains .

vec:SealState  rdf:type  owl:Class;
        rdfs:comment     "Enumeration for the definition of the sealing state of the splice.\n"@en;
        rdfs:label       "SealState"@en;
        rdfs:subClassOf  vec:OpenEnumeration .

vec:corrugatedPipeSpecificationCorrugationWidth
        rdf:type            owl:ObjectProperty;
        rdfs:comment        "Specifies the width of a corrugation of the pipe.\n"@en;
        rdfs:domain         vec:CorrugatedPipeSpecification;
        rdfs:label          "corrugationWidth"@en;
        rdfs:range          vec:NumericalValue;
        rdfs:subPropertyOf  vec:contains .

vec:partVersionAliasId
        rdf:type            owl:ObjectProperty;
        rdfs:comment        "Room to specify additional identifiers for the PartVersion. This field must not be used for alternative PartNumbers. It is intended for identifiers others than PartNumbers, such as human readable identifiers printed on the part e.g. a number of fuse or a relay. Therefore, it does not have to be strictly unique.\n"@en;
        rdfs:domain         vec:PartVersion;
        rdfs:label          "aliasId"@en;
        rdfs:range          vec:AliasIdentification;
        rdfs:subPropertyOf  vec:contains .

vec:topologyNodeAliasId
        rdf:type            owl:ObjectProperty;
        rdfs:comment        "Specifies additional identifiers for the TopologyNode.\nExample: TopologyNode Ids may vary from one CAD system export to another. Therefore, the CAD system Id is improper for identification attribute. The identification shall have a value which is unique within the Topology. AliasId may be used for the CAD system Id.\n"@en;
        rdfs:domain         vec:TopologyNode;
        rdfs:label          "aliasId"@en;
        rdfs:range          vec:AliasIdentification;
        rdfs:subPropertyOf  vec:contains .

vec:cartesianPoint2DWrapperItem
        rdf:type      owl:ObjectProperty;
        rdfs:comment  "References the actual item for a Wrapper.";
        rdfs:domain   vec:CartesianPoint2DWrapper;
        rdfs:range    vec:CartesianPoint2D .

vec:pinTimingType  rdf:type  owl:ObjectProperty;
        rdfs:comment        "Specifies the type of the timing.\n"@en;
        rdfs:domain         vec:PinTiming;
        rdfs:label          "type"@en;
        rdfs:range          vec:PinTimingType;
        rdfs:subPropertyOf  vec:contains .

vec:antennaSpecificationImpedance
        rdf:type            owl:ObjectProperty;
        rdfs:comment        "Specifies the impedance of the antenna.\n"@en;
        rdfs:domain         vec:AntennaSpecification;
        rdfs:label          "impedance"@en;
        rdfs:range          vec:NumericalValue;
        rdfs:subPropertyOf  vec:contains .

[ rdf:type     owl:AllDisjointClasses;
  owl:members  ( vec:OnPointPlacement vec:OnWayPlacement )
] .

vec:cavityMountingDetailTerminalReceptionReference
        rdf:type      owl:ObjectProperty;
        rdfs:comment  "References the TerminalReception that is used for the detailed description of the cavity mounting. \n"@en;
        rdfs:domain   vec:CavityMountingDetail;
        rdfs:label    "terminalReceptionReference"@en;
        rdfs:range    vec:TerminalReceptionReference .

vec:BaselineContent_Partial
        rdf:type         vec:BaselineContent , owl:NamedIndividiual;
        rdfs:comment     "A partial baseline does not contain all elements of the final scope of the baseline (e.g. it is a baseline created during the development process).\n"@en;
        vec:enumLiteral  "Partial" .

vec:ImperialUnitName_Quarter
        rdf:type         vec:ImperialUnitName , owl:NamedIndividiual;
        vec:enumLiteral  "Quarter" .

vec:ValueRange  rdf:type  owl:Class;
        rdfs:comment     "A pair of numerical values representing a value range.\n"@en;
        rdfs:label       "ValueRange"@en;
        rdfs:subClassOf  vec:ValueWithUnit .

vec:OccurrenceOrUsage
        rdf:type         owl:Class;
        rdfs:comment     "An OccurrenceOrUsage is an abstract appearance of a part in the harness. This can either be a concrete part (with a part number or something similar) or the description (specification / requirements) of a part that should be used at that position. In the first case it would be a PartOccurrence in the second case a PartUsage.\n"@en;
        rdfs:label       "OccurrenceOrUsage"@en;
        rdfs:subClassOf  vec:ConfigurableElement .

vec:labelingSpecificationAllowedLabelingTechnology
        rdf:type            owl:ObjectProperty;
        rdfs:comment        "Specifies the allowed labeling technologies if the component is not yet labeled, but support labeling in its usage."@en;
        rdfs:domain         vec:LabelingSpecification;
        rdfs:label          "allowedLabelingTechnology"@en;
        rdfs:range          vec:LabelingTechnology;
        rdfs:subPropertyOf  vec:contains .

vec:CavityAddOn  rdf:type  owl:Class;
        rdfs:comment  "Specifies the wire addon needed to reach a Cavity from a specific SegmentConnectionPoint . More specifically, it is the addon required to calculate the cutting length of a wire. It is not a measured distance between the segment connection point and the insertion point of the cavity. For each SegmentConnectionPoint there shall be no more than one add-on value per cavity and type.\n"@en;
        rdfs:label    "CavityAddOn"@en .

vec:FittingOutlet  rdf:type  owl:Class;
        rdfs:comment     "Specifies one outlet of the fitting.\n"@en;
        rdfs:label       "FittingOutlet"@en;
        rdfs:subClassOf  vec:ExtendableElement .

vec:connectionSpecificationComponentNode
        rdf:type            owl:ObjectProperty;
        rdfs:comment        "Specifies the ComponentNodes defined by the ConnectionSpecification.\n"@en;
        rdfs:domain         vec:ConnectionSpecification;
        rdfs:label          "componentNode"@en;
        rdfs:range          vec:ComponentNode;
        rdfs:subPropertyOf  vec:contains .

vec:FunctionalRequirementType_Legal
        rdf:type         vec:FunctionalRequirementType , owl:NamedIndividiual;
        rdfs:comment     "Legal Requirements.\n┬á\n"@en;
        vec:enumLiteral  "Legal" .

vec:SlotLayoutType_MITOX
        rdf:type         vec:SlotLayoutType , owl:NamedIndividiual;
        rdfs:comment     "Fuse type according to ISO8820\n"@en;
        vec:enumLiteral  "MITOX" .

vec:protectionMaterialLengthValueDetermination
        rdf:type            owl:ObjectProperty;
        rdfs:domain         vec:ProtectionMaterialLength;
        rdfs:label          "valueDetermination"@en;
        rdfs:range          vec:ValueDetermination;
        rdfs:subPropertyOf  vec:contains .

vec:SlotLayoutType_HSD
        rdf:type         vec:SlotLayoutType , owl:NamedIndividiual;
        rdfs:comment     "High Speed Data Connectors"@en;
        vec:enumLiteral  "HSD" .

vec:TerminalBoltNominalSize_M30
        rdf:type         vec:TerminalBoltNominalSize , owl:NamedIndividiual;
        vec:enumLiteral  "M30" .

vec:UsageNodeType_Generator
        rdf:type         vec:UsageNodeType , owl:NamedIndividiual;
        vec:enumLiteral  "Generator" .

vec:TubeShape_NonCircular
        rdf:type         vec:TubeShape , owl:NamedIndividiual;
        rdfs:comment     "The tube has a cross section that is not circular.\n"@en;
        vec:enumLiteral  "NonCircular" .

vec:UsageNodeType_ECU
        rdf:type         vec:UsageNodeType , owl:NamedIndividiual;
        vec:enumLiteral  "ECU" .

vec:topologyMappingSpecificationSegmentMapping
        rdf:type            owl:ObjectProperty;
        rdfs:domain         vec:TopologyMappingSpecification;
        rdfs:label          "segmentMapping"@en;
        rdfs:range          vec:SegmentMapping;
        rdfs:subPropertyOf  vec:contains .

vec:HoleMountedFixingHoleShape_Slotted
        rdf:type         vec:HoleMountedFixingHoleShape , owl:NamedIndividiual;
        vec:enumLiteral  "Slotted" .

vec:openCavitiesAssignmentOpenCavities
        rdf:type      owl:ObjectProperty;
        rdfs:comment  "Specifies the cavities that are open.\n"@en;
        rdfs:domain   vec:OpenCavitiesAssignment;
        rdfs:label    "openCavities"@en;
        rdfs:range    vec:Cavity .

<http://www.prostep.org/ontologies/ecad/2024/03/vec#ColorReferenceSystem_IEC%2060757>
        rdf:type         vec:ColorReferenceSystem , owl:NamedIndividiual;
        rdfs:comment     "The literal shall be used for the IEC┬á60757 \"Electrotechnical engineering; code for designation of colours\"\n"@en;
        vec:enumLiteral  "IEC 60757" .

vec:connectionInstallationInstruction
        rdf:type            owl:ObjectProperty;
        rdfs:comment        "Specifies installation instruction for the connection.\n"@en;
        rdfs:domain         vec:Connection;
        rdfs:label          "installationInstruction"@en;
        rdfs:range          vec:Instruction;
        rdfs:subPropertyOf  vec:contains .

vec:fittingOutletOuterDiameter
        rdf:type            owl:ObjectProperty;
        rdfs:comment        "Specifies the outer diameter of the outlet.\n"@en;
        rdfs:domain         vec:FittingOutlet;
        rdfs:label          "outerDiameter"@en;
        rdfs:range          vec:NumericalValue;
        rdfs:subPropertyOf  vec:contains .

vec:changeDescriptionLabel
        rdf:type      owl:DatatypeProperty;
        rdfs:comment  "Specifies the label of the change on a drawing for example. If more than one change is issued with one ItemVersion (e.g. change 0001, 0002), in some cases the different changes are labelled on the drawing (e.g. A, B, C).\n"@en;
        rdfs:domain   vec:ChangeDescription;
        rdfs:label    "label"@en;
        rdfs:range    xs:string .

vec:dimensionTolerance
        rdf:type            owl:ObjectProperty;
        rdfs:domain         vec:Dimension;
        rdfs:label          "tolerance"@en;
        rdfs:range          vec:Tolerance;
        rdfs:subPropertyOf  vec:contains .

vec:terminalReceptionReferenceTerminalReception
        rdf:type      owl:ObjectProperty;
        rdfs:comment  "References the TerminalReception that is instanced by this TerminalReceptionReference.\n"@en;
        rdfs:domain   vec:TerminalReceptionReference;
        rdfs:label    "terminalReception"@en;
        rdfs:range    vec:TerminalReception .

vec:PrimaryPartType_Relay
        rdf:type         vec:PrimaryPartType , owl:NamedIndividiual;
        vec:enumLiteral  "Relay" .

vec:InternalComponentConnection
        rdf:type         owl:Class;
        rdfs:comment     "An InternalComponentConnection defines a conductive connection between PinComponents within an EEComponent . Such a connection can be statically permanent or dynamically switch (e.g. by a relais). This behaviour can be defined with a SwitchingState .\nThe electrical behaviour of an InternalComponentConnection can be further specified by a referenced ConductorSpecification.\n"@en;
        rdfs:label       "InternalComponentConnection"@en;
        rdfs:subClassOf  vec:ConfigurableElement .

vec:booleanValuePropertyValue
        rdf:type      owl:DatatypeProperty;
        rdfs:comment  "Defines the value of the CustomProperty.\n"@en;
        rdfs:domain   vec:BooleanValueProperty;
        rdfs:label    "value"@en;
        rdfs:range    xs:boolean .

vec:LanguageCode_Ba  rdf:type  vec:LanguageCode , owl:NamedIndividiual;
        vec:enumLiteral  "Ba" .

vec:contactingSpecificationContactPoint
        rdf:type            owl:ObjectProperty;
        rdfs:comment        "Specifies the ContactPoints defined by the ContactingSpecification.\n"@en;
        rdfs:domain         vec:ContactingSpecification;
        rdfs:label          "contactPoint"@en;
        rdfs:range          vec:ContactPoint;
        rdfs:subPropertyOf  vec:contains .

[ rdf:type     owl:AllDisjointClasses;
  owl:members  ( vec:AliasIdentification vec:ExtendableElement vec:AbstractLocalizedString vec:CustomProperty vec:ConductorCurrentInformation vec:PartRelation vec:PinCurrentInformation vec:PinOpticalInformation vec:PinTiming vec:PinVoltageInformation vec:SealedCavitiesAssignment vec:SlotLayout vec:TerminalCurrentInformation vec:WireType vec:OpenCavitiesAssignment vec:PowerConsumption vec:ModularSlotAddOn vec:CavityAddOn vec:FuseComponent vec:ConductorMaterial vec:WireReceptionAddOn vec:CavityPositionDetail vec:NURBSControlPoint vec:WireReceptionReference vec:TerminalReceptionReference vec:WireTupleTermination vec:CableLeadThroughReference vec:CavityMapping vec:SlotMapping vec:NetType vec:NetworkNodeViewItem vec:NetworkPortViewItem vec:CableLeadThroughOutlet vec:ProtectionMaterialLength vec:Person vec:Color vec:MassInformation vec:Material vec:RobustnessProperties vec:Size vec:SoundDampingClass vec:TemperatureInformation vec:Unit vec:ValueWithUnit vec:BoundingBox vec:DefaultDimension vec:ComponentPortViewItem vec:ConnectionNodeViewItem vec:CartesianVector vec:ZoneAssignment vec:ZoneCoverage vec:NodeMapping vec:SegmentMapping vec:TopologyBendingRestriction vec:RequirementsConformanceStatement vec:LocalPosition vec:PinWireMappingPoint vec:FunctionalRequirement vec:FunctionalStructureNode )
] .

vec:conductorSpecificationCrossSectionArea
        rdf:type            owl:ObjectProperty;
        rdfs:comment        "Specifies the cross-section area of the conductor (e.g. 0,5 mm┬▓). The cross-section area is a nominal value, which refers to the conducting properties of the conductor normalized to the properties of a full material core.\n"@en;
        rdfs:domain         vec:ConductorSpecification;
        rdfs:label          "crossSectionArea"@en;
        rdfs:range          vec:NumericalValue;
        rdfs:subPropertyOf  vec:contains .

vec:TerminalBoltNominalSize_M14
        rdf:type         vec:TerminalBoltNominalSize , owl:NamedIndividiual;
        vec:enumLiteral  "M14" .

vec:ImperialUnitName_Grain
        rdf:type         vec:ImperialUnitName , owl:NamedIndividiual;
        vec:enumLiteral  "Grain" .

vec:applicationConstraintProject
        rdf:type      owl:ObjectProperty;
        rdfs:comment  "┬áDefines the projects for which the application constraint applies.\n"@en;
        rdfs:domain   vec:ApplicationConstraint;
        rdfs:label    "project"@en;
        rdfs:range    vec:Project .

vec:SealState_Unsealed
        rdf:type         vec:SealState , owl:NamedIndividiual;
        rdfs:comment     "The splice is not waterproof.\n"@en;
        vec:enumLiteral  "Unsealed" .

vec:componentPortSignalDirection
        rdf:type            owl:ObjectProperty;
        rdfs:comment        "Specifies the direction of the signal on this ComponentPort.\n"@en;
        rdfs:domain         vec:ComponentPort;
        rdfs:label          "signalDirection"@en;
        rdfs:range          vec:SignalDirection;
        rdfs:subPropertyOf  vec:contains .

vec:compositeUnitFactors
        rdf:type      owl:ObjectProperty;
        rdfs:comment  "References the Units that are used as factors to create the CompositeUnit.\n"@en;
        rdfs:domain   vec:CompositeUnit;
        rdfs:label    "factors"@en;
        rdfs:range    vec:Unit .

vec:SignalDirection_InOut
        rdf:type         vec:SignalDirection , owl:NamedIndividiual;
        vec:enumLiteral  "InOut" .

vec:LanguageCode_La  rdf:type  vec:LanguageCode , owl:NamedIndividiual;
        vec:enumLiteral  "La" .

vec:aliasIdentificationDescription
        rdf:type            owl:ObjectProperty;
        rdfs:comment        "On optional human readable description of the AliasIdentification.\n"@en;
        rdfs:domain         vec:AliasIdentification;
        rdfs:label          "description"@en;
        rdfs:range          vec:AbstractLocalizedString;
        rdfs:subPropertyOf  vec:contains .

vec:fittingOutletPlacementPoint
        rdf:type      owl:ObjectProperty;
        rdfs:comment  "Specifies the PlacementPoint that represents this FittingOutlet in a PlaceableElementSpecification.\n"@en;
        rdfs:domain   vec:FittingOutlet;
        rdfs:label    "placementPoint"@en;
        rdfs:range    vec:PlacementPoint .

vec:WireElementShape  rdf:type  owl:Class;
        rdfs:comment     "Defines the shape of a wire element.\n"@en;
        rdfs:label       "WireElementShape"@en;
        rdfs:subClassOf  vec:OpenEnumeration .

vec:ComponentNodeType
        rdf:type         owl:Class;
        rdfs:comment     "Defines the common agreed values for the types of a ComponentNode.\n"@en;
        rdfs:label       "ComponentNodeType"@en;
        rdfs:subClassOf  vec:OpenEnumeration .

vec:wireTupleSpecificationFixationOffset
        rdf:type            owl:ObjectProperty;
        rdfs:comment        "The offset from the wire end, at which the fixation has to be placed."@en;
        rdfs:domain         vec:WireTupleSpecification;
        rdfs:label          "fixationOffset"@en;
        rdfs:range          vec:NumericalValue;
        rdfs:subPropertyOf  vec:contains .

[ rdf:type     owl:AllDisjointClasses;
  owl:members  ( vec:ModularSlot vec:Slot )
] .

vec:ContractRole_Supplier
        rdf:type         vec:ContractRole , owl:NamedIndividiual;
        vec:enumLiteral  "Supplier" .

vec:mappingB  rdf:type  owl:ObjectProperty;
        rdfs:comment  ""@en;
        rdfs:domain   vec:Mapping;
        rdfs:label    "B"@en;
        rdfs:range    vec:PartVersion .

vec:ConfigurableElement
        rdf:type         owl:Class;
        rdfs:comment     "Abstract base class for all elements which can be configured with a VariantConfiguration.\n"@en;
        rdfs:label       "ConfigurableElement"@en;
        rdfs:subClassOf  vec:ExtendableElement .

vec:usageConstraintToSerialNumber
        rdf:type      owl:DatatypeProperty;
        rdfs:comment  "Specifies the upper bound of a serial number range to which the usage constraint applies.\n"@en;
        rdfs:domain   vec:UsageConstraint;
        rdfs:label    "toSerialNumber"@en;
        rdfs:range    xs:string .

vec:Enumeration  rdf:type  owl:Class;
        rdfs:comment  "Classes in the model that can be enumerated, either closed or open (see VEC Specicification)"@en;
        rdfs:label    "Enumeration"@en .

vec:TerminalBoltType_ImperialThread
        rdf:type         vec:TerminalBoltType , owl:NamedIndividiual;
        rdfs:comment     "A bolt with a imperial scale thread.\n"@en;
        vec:enumLiteral  "ImperialThread" .

vec:cableLeadThroughCableLeadThroughSpecification
        rdf:type      owl:ObjectProperty;
        rdfs:comment  "References the CableLeadThroughSpecification that defines the technical properties of this CableLeadThrough.\n"@en;
        rdfs:domain   vec:CableLeadThrough;
        rdfs:label    "cableLeadThroughSpecification"@en;
        rdfs:range    vec:CableLeadThroughSpecification .

vec:TerminalBoltNominalSize_M56
        rdf:type         vec:TerminalBoltNominalSize , owl:NamedIndividiual;
        vec:enumLiteral  "M56" .

vec:DocumentType_ComponentDrawing
        rdf:type         vec:DocumentType , owl:NamedIndividiual;
        rdfs:comment     " DocumentVersion of this type represent the drawing of a component (Deutsch: Einzelteilezeichnung). Those DocumentVersion are normally used as external reference to the document containing the graphical representation of the component and do not contain Specifications . DocumentVersion describing a component in terms of the VEC┬á(with Specifications ) shall have the DocumentType PartMaster.\n"@en;
        vec:enumLiteral  "ComponentDrawing" .

vec:variantStructureNodeChildNodes
        rdf:type            owl:ObjectProperty;
        rdfs:domain         vec:VariantStructureNode;
        rdfs:label          "childNodes"@en;
        rdfs:range          vec:VariantStructureNode;
        rdfs:subPropertyOf  vec:contains .

vec:UsageNodeType  rdf:type  owl:Class;
        rdfs:comment     "Enumeration for the different types of UsageNodes.\n"@en;
        rdfs:label       "UsageNodeType"@en;
        rdfs:subClassOf  vec:OpenEnumeration .

vec:cableLeadThroughOutlet
        rdf:type            owl:ObjectProperty;
        rdfs:comment        "Specfies the outlets of a CableLeadThrough. "@en;
        rdfs:domain         vec:CableLeadThrough;
        rdfs:label          "outlet"@en;
        rdfs:range          vec:CableLeadThroughOutlet;
        rdfs:subPropertyOf  vec:contains .

vec:PluggableTerminalType_MultiContact
        rdf:type         vec:PluggableTerminalType , owl:NamedIndividiual;
        vec:enumLiteral  "MultiContact" .

vec:creationResponsibleDesigner
        rdf:type            owl:ObjectProperty;
        rdfs:comment        "Specifies the person, which is the responsible designer for the ItemVersion at the point of creation.\n"@en;
        rdfs:domain         vec:Creation;
        rdfs:label          "responsibleDesigner"@en;
        rdfs:range          vec:Person;
        rdfs:subPropertyOf  vec:contains .

vec:personAliasId  rdf:type  owl:ObjectProperty;
        rdfs:comment        "Specifies identifiers for the Person in different contexts.\n"@en;
        rdfs:domain         vec:Person;
        rdfs:label          "aliasId"@en;
        rdfs:range          vec:AliasIdentification;
        rdfs:subPropertyOf  vec:contains .

vec:BaselineContent_Complete
        rdf:type         vec:BaselineContent , owl:NamedIndividiual;
        rdfs:comment     "A complete baseline contains all elements of the final scope of the baseline.\n"@en;
        vec:enumLiteral  "Complete" .

vec:GeometryNode2D  rdf:type  owl:Class;
        rdfs:comment     "A GeometryNode2D is the geometric representation of a TopologyNode in 2D-space.\n"@en;
        rdfs:label       "GeometryNode2D"@en;
        rdfs:subClassOf  vec:GeometryNode .

vec:ConductorStructure_Symmetric
        rdf:type         vec:ConductorStructure , owl:NamedIndividiual;
        rdfs:comment     "Symmetric conductor structure in accordance with ISO 6722-1 (Type A)\n"@en;
        vec:enumLiteral  "Symmetric" .

vec:CavityGeometry_Oval
        rdf:type         vec:CavityGeometry , owl:NamedIndividiual;
        rdfs:comment     ""@en;
        vec:enumLiteral  "Oval" .

vec:coreSpecificationOutsideDiameter
        rdf:type            owl:ObjectProperty;
        rdfs:comment        "Specifies the outside diameter of the core.\n"@en;
        rdfs:domain         vec:CoreSpecification;
        rdfs:label          "outsideDiameter"@en;
        rdfs:range          vec:NumericalValue;
        rdfs:subPropertyOf  vec:contains .

vec:usageConstraintSpecificationPartUsageConstraint
        rdf:type            owl:ObjectProperty;
        rdfs:comment        "Specifies the UsageConstraints that apply to the PartVersion or PartUsages described by the UsageConstraintSpecification. The ordering of this association is relevant. The elements shall arranged in the order of ascending priority.┬áThat means, elements further back in the collection have a higher priority.\n"@en;
        rdfs:domain         vec:UsageConstraintSpecification;
        rdfs:label          "partUsageConstraint"@en;
        rdfs:range          vec:UsageConstraint , vec:Ordered;
        rdfs:subPropertyOf  vec:contains .

vec:CartesianPoint3D  rdf:type  owl:Class;
        rdfs:comment     "A CartesianPoint3D is a point that is defined by its coordinates in a rectangular three-dimensional Cartesian coordinate system.\n"@en;
        rdfs:label       "CartesianPoint3D"@en;
        rdfs:subClassOf  vec:ExtendableElement .

[ rdf:type     owl:AllDisjointClasses;
  owl:members  ( vec:CompositeUnit vec:CustomUnit vec:IECUnit vec:ImperialUnit vec:OtherUnit vec:SIUnit vec:USUnit )
] .

vec:TerminalBoltNominalSize_M1.8
        rdf:type         vec:TerminalBoltNominalSize , owl:NamedIndividiual;
        vec:enumLiteral  "M1.8" .

vec:PrimaryPartType_WireEndAccessory
        rdf:type         vec:PrimaryPartType , owl:NamedIndividiual;
        vec:enumLiteral  "WireEndAccessory" .

vec:abstractSlotReferenceReferencedSlot
        rdf:type      owl:ObjectProperty;
        rdfs:comment  "Points to the slot referenced by the slot reference. \n"@en;
        rdfs:domain   vec:AbstractSlotReference;
        rdfs:label    "referencedSlot"@en;
        rdfs:range    vec:AbstractSlot .

vec:CavitySealSpecification
        rdf:type         owl:Class;
        rdfs:comment     "Specification for the definition of cavity seals. A CavitySeal is a watertight non-electrical object to fill a populated Cavity.\n"@en;
        rdfs:label       "CavitySealSpecification"@en;
        rdfs:subClassOf  vec:CavityPartSpecification .

vec:LanguageCode_Te  rdf:type  vec:LanguageCode , owl:NamedIndividiual;
        vec:enumLiteral  "Te" .

vec:NetworkNodeType_Generator
        rdf:type         vec:NetworkNodeType , owl:NamedIndividiual;
        rdfs:comment     "A device that can generate energy.\n"@en;
        vec:enumLiteral  "Generator" .

vec:USUnitName_Pound  rdf:type  vec:USUnitName , owl:NamedIndividiual;
        vec:enumLiteral  "Pound" .

vec:modularSlotAddOnSlot
        rdf:type     owl:ObjectProperty;
        rdfs:domain  vec:ModularSlotAddOn;
        rdfs:label   "slot"@en;
        rdfs:range   vec:ModularSlot .

vec:CorrugatedPipeSpecification
        rdf:type         owl:Class;
        rdfs:comment     "Specification for the definition of corrugated pipes.\n"@en;
        rdfs:label       "CorrugatedPipeSpecification"@en;
        rdfs:subClassOf  vec:TubeSpecification .

vec:zoneAssignmentCoverage
        rdf:type            owl:ObjectProperty;
        rdfs:comment        "Contains a set of ZoneCoverages that define the areas of a TopologySegment that is affected by the TopologyZone.┬áIf no coverage is defined, the complete segment is affected. Multiple coverages can be necessary if the TopologySegment zigzags in and out of the TopologyZone.\n"@en;
        rdfs:domain         vec:ZoneAssignment;
        rdfs:label          "coverage"@en;
        rdfs:range          vec:ZoneCoverage;
        rdfs:subPropertyOf  vec:contains .

vec:ApplicationConstraintSpecification
        rdf:type         owl:Class;
        rdfs:comment     "Specification for the definition of application constraints. The associated ApplicationConstraints are restricting the possible usages of the associated ConfigurableElements .\n"@en;
        rdfs:label       "ApplicationConstraintSpecification"@en;
        rdfs:subClassOf  vec:Specification .

vec:cartesianVector3DY
        rdf:type      owl:DatatypeProperty;
        rdfs:comment  "Specifies the y-coordinate in 3D space.\n"@en;
        rdfs:domain   vec:CartesianVector3D;
        rdfs:label    "y"@en;
        rdfs:range    xs:double .

vec:PlacementSpecification
        rdf:type         owl:Class;
        rdfs:comment     "Specification for the description of placements. Placements are used to connect OccurrenceOrUsages with a topology.\n"@en;
        rdfs:label       "PlacementSpecification"@en;
        rdfs:subClassOf  vec:Specification .

vec:grommetRoleCableLeadThroughReference
        rdf:type            owl:ObjectProperty;
        rdfs:domain         vec:GrommetRole;
        rdfs:label          "cableLeadThroughReference"@en;
        rdfs:range          vec:CableLeadThroughReference;
        rdfs:subPropertyOf  vec:contains .

vec:stripeSpecificationWidth
        rdf:type            owl:ObjectProperty;
        rdfs:comment        "Specifies the width of the stripe.\n"@en;
        rdfs:domain         vec:StripeSpecification;
        rdfs:label          "width"@en;
        rdfs:range          vec:NumericalValue;
        rdfs:subPropertyOf  vec:contains .

vec:EEComponentRole  rdf:type  owl:Class;
        rdfs:comment     "An EEComponentRole defines the instance specific properties and relationships of an EE-component.\n"@en;
        rdfs:label       "EEComponentRole"@en;
        rdfs:subClassOf  vec:Role .

vec:FunctionalStructureSpecification
        rdf:type         owl:Class;
        rdfs:comment     "Specification to define any hierarchical structure on functional assignment groups (e.g. by the means of a functional organization).┬áThe hierarchy starts with a single root node.\n"@en;
        rdfs:label       "FunctionalStructureSpecification"@en;
        rdfs:subClassOf  vec:Specification .

vec:housingComponentReferencePinComponentRef
        rdf:type            owl:ObjectProperty;
        rdfs:comment        "Specifies the PinComponentReferences used in the HousingComponentReference. \n(KBLFRM-401)\n"@en;
        rdfs:domain         vec:HousingComponentReference;
        rdfs:label          "pinComponentRef"@en;
        rdfs:range          vec:PinComponentReference;
        rdfs:subPropertyOf  vec:contains .

vec:PrimaryPartType_MultiCavitySeal
        rdf:type         vec:PrimaryPartType , owl:NamedIndividiual;
        vec:enumLiteral  "MultiCavitySeal" .

vec:slotLayoutRowCount
        rdf:type      owl:DatatypeProperty;
        rdfs:comment  "The number of cavity rows of the slot.\n"@en;
        rdfs:domain   vec:SlotLayout;
        rdfs:label    "rowCount"@en;
        rdfs:range    xs:integer .

vec:LanguageCode_Hi  rdf:type  vec:LanguageCode , owl:NamedIndividiual;
        vec:enumLiteral  "Hi" .

vec:ComponentNodeType_EnergyStorage
        rdf:type         vec:ComponentNodeType , owl:NamedIndividiual;
        rdfs:comment     "A device that stores energy in some kind of way (e.g. a battery).\n"@en;
        vec:enumLiteral  "EnergyStorage" .

vec:cavityPlugRolePluggedCavityRef
        rdf:type      owl:ObjectProperty;
        rdfs:comment  "Defines which cavity / cavities in a connector instance is sealed by the plug. \n"@en;
        rdfs:domain   vec:CavityPlugRole;
        rdfs:label    "pluggedCavityRef"@en;
        rdfs:range    vec:CavityReference .

vec:PlaceableElementSpecification
        rdf:type         owl:Class;
        rdfs:comment     "Specification for the general aspects of a component that are enabling the component to be placed in a topology. All components that should have the ability to be placed on a certain position in the topology must have a PlaceableElementSpecification\n"@en;
        rdfs:label       "PlaceableElementSpecification"@en;
        rdfs:subClassOf  vec:PartOrUsageRelatedSpecification .

vec:SlotLayout  rdf:type  owl:Class;
        rdfs:comment  "For regularly laid out slots the slot layout describes the positions of the cavities\n"@en;
        rdfs:label    "SlotLayout"@en .

vec:vecContentContract
        rdf:type            owl:ObjectProperty;
        rdfs:comment        "Specifies the contracts used in the VEC-file. \n"@en;
        rdfs:domain         vec:VecContent;
        rdfs:label          "contract"@en;
        rdfs:range          vec:Contract;
        rdfs:subPropertyOf  vec:contains .

vec:NetworkNodeType_CouplingDevice
        rdf:type         vec:NetworkNodeType , owl:NamedIndividiual;
        rdfs:comment     "A CouplingDevice is the (virtual)┬ádevice that separates / connects two or more wiring harnesses. \"Virtual\" because it can be interpreted as a device /┬áinterface definition between the harnesses, where one harness behaves like an E/E┬ácomponent form the point of view of the other harness.\n"@en;
        vec:enumLiteral  "CouplingDevice" .

vec:baselineSpecificationState
        rdf:type            owl:ObjectProperty;
        rdfs:comment        "Defines the state of the baseline itself (e.g. if it is finalized or work in progress).\n┬á\n"@en;
        rdfs:domain         vec:BaselineSpecification;
        rdfs:label          "state"@en;
        rdfs:range          vec:BaselineState;
        rdfs:subPropertyOf  vec:contains .

vec:cavitySpecificationAngle
        rdf:type            owl:ObjectProperty;
        rdfs:comment        "Specifies the angle against two planes of the connector housing a terminal used in this cavity can be buckled.\n"@en;
        rdfs:domain         vec:CavitySpecification;
        rdfs:label          "angle"@en;
        rdfs:range          vec:NumericalValue , vec:Ordered;
        rdfs:subPropertyOf  vec:contains .

vec:SiPrefix_Peta  rdf:type  vec:SiPrefix , owl:NamedIndividiual;
        vec:enumLiteral  "Peta" .

vec:OpenWireEndTerminalSpecification
        rdf:type         owl:Class;
        rdfs:comment     "Specification for the definition of open wire ends. An open wire end is an end of wire located at a specific location in the harness. Open wire ends are not connected to some other component, in contrast to regular connectors or ring terminals. Only one wire is ending at a single open wire end, otherwise it would be a splice.\n"@en;
        rdfs:label       "OpenWireEndTerminalSpecification"@en;
        rdfs:subClassOf  vec:TerminalSpecification .

vec:USUnitName_Mile  rdf:type  vec:USUnitName , owl:NamedIndividiual;
        vec:enumLiteral  "Mile" .

vec:SegmentConnectionPointHC
        rdf:type         owl:Class;
        rdfs:comment     "Specifies a point where the HousingComponent can be attached to the topology [if required] (sometimes called bundle position point or insertion point).\n┬á Note: The suffix HC is justified by the fact that class names must be unique within the model and the name SegmentConnectionPoint is already used within the ConnectorHousingSpecification. However, the represented semantics of the two connection points are so similar that the use of actually different names for both would rather have led to confusion. So SegmentConnectionPointHC┬áactually is short hand for \"SegmentConnectionPoint within HousingComponent\".\n"@en;
        rdfs:label       "SegmentConnectionPointHC"@en;
        rdfs:subClassOf  vec:ExtendableElement .

vec:measurePointPositionMeasurementPoint
        rdf:type     owl:ObjectProperty;
        rdfs:domain  vec:MeasurePointPosition;
        rdfs:label   "measurementPoint"@en;
        rdfs:range   vec:MeasurementPoint .

vec:externalMappingMappedElement
        rdf:type      owl:ObjectProperty;
        rdfs:comment  ""@en;
        rdfs:domain   vec:ExternalMapping;
        rdfs:label    "mappedElement"@en;
        rdfs:range    vec:ExtendableElement .

vec:slotMappingIdentificationB
        rdf:type      owl:DatatypeProperty;
        rdfs:comment  "The identification of the Slot on side B\n"@en;
        rdfs:domain   vec:SlotMapping;
        rdfs:label    "identificationB"@en;
        rdfs:range    xs:string .

vec:pathSegmentControlPoint
        rdf:type            owl:ObjectProperty;
        rdfs:comment        "This association is defined as unique='false' and ordered='true'. This can not be represented efficiently directly in RDF/OWL. Therefore, this association references Wrappers as proxies to the actual elements, instead of the actual elements itself (like a regular association)." , "The ordered list of control points through which the PathSegment goes. \n"@en;
        rdfs:domain         vec:PathSegment;
        rdfs:label          "controlPoint"@en;
        rdfs:range          vec:CartesianPoint2DWrapper , vec:Ordered;
        rdfs:subPropertyOf  vec:contains .

vec:fuseSpecificationIMax
        rdf:type            owl:ObjectProperty;
        rdfs:comment        "Specifies the maximum electric current tolerated by the fuse.\n"@en;
        rdfs:domain         vec:FuseSpecification;
        rdfs:label          "iMax"@en;
        rdfs:range          vec:NumericalValue;
        rdfs:subPropertyOf  vec:contains .

vec:LanguageCode_Zh  rdf:type  vec:LanguageCode , owl:NamedIndividiual;
        rdfs:comment     "Chinese\n"@en;
        vec:enumLiteral  "Zh" .

vec:cableLeadThroughReferenceCableLeadThrough
        rdf:type     owl:ObjectProperty;
        rdfs:domain  vec:CableLeadThroughReference;
        rdfs:label   "cableLeadThrough"@en;
        rdfs:range   vec:CableLeadThrough .

vec:itemVersionProcessingInstruction
        rdf:type            owl:ObjectProperty;
        rdfs:comment        "Processing instructions for the application of the part or the document.\n"@en;
        rdfs:domain         vec:ItemVersion;
        rdfs:label          "processingInstruction"@en;
        rdfs:range          vec:Instruction;
        rdfs:subPropertyOf  vec:contains .

vec:BaselineContent  rdf:type  owl:Class;
        rdfs:comment     "Enumeration to define the state of the content of the baseline in regard of its defined scope.\n"@en;
        rdfs:label       "BaselineContent"@en;
        rdfs:subClassOf  vec:OpenEnumeration .

vec:DocumentType_MasterDataDefinition
        rdf:type         vec:DocumentType , owl:NamedIndividiual;
        rdfs:comment     "Documents of this type master data definition e.g. list valid UsageNodes or list valid Signals .\n"@en;
        vec:enumLiteral  "MasterDataDefinition" .

vec:cavityPartSpecificationCompatibleCavityGeometry
        rdf:type            owl:ObjectProperty;
        rdfs:comment        "Defines a list of CavityGeometries that are compatible with this cavity part.\n"@en;
        rdfs:domain         vec:CavityPartSpecification;
        rdfs:label          "compatibleCavityGeometry"@en;
        rdfs:range          vec:CavityGeometry;
        rdfs:subPropertyOf  vec:contains .

vec:SiUnitName_Gram  rdf:type  vec:SiUnitName , owl:NamedIndividiual;
        vec:enumLiteral  "Gram" .

vec:terminalReceptionSpecificationContactRangeLength
        rdf:type            owl:ObjectProperty;
        rdfs:comment        "Specifies the length of the contact area (see diagram \"Terminal Dimensions\").\n"@en;
        rdfs:domain         vec:TerminalReceptionSpecification;
        rdfs:label          "contactRangeLength"@en;
        rdfs:range          vec:NumericalValue;
        rdfs:subPropertyOf  vec:contains .

vec:TerminalRole  rdf:type  owl:Class;
        rdfs:comment     "A TerminalRole defines the instance specific properties and relationships of a terminal.\n"@en;
        rdfs:label       "TerminalRole"@en;
        rdfs:subClassOf  vec:Role .

vec:LanguageCode_Nl  rdf:type  vec:LanguageCode , owl:NamedIndividiual;
        vec:enumLiteral  "Nl" .

vec:wireGroupingSpecificationWireGrouping
        rdf:type            owl:ObjectProperty;
        rdfs:comment        "Specifies the WireGroupings described by the WireGroupingSpecification.\n"@en;
        rdfs:domain         vec:WireGroupingSpecification;
        rdfs:label          "wireGrouping"@en;
        rdfs:range          vec:WireGrouping;
        rdfs:subPropertyOf  vec:contains .

vec:ContractRole_Manufacturer
        rdf:type         vec:ContractRole , owl:NamedIndividiual;
        vec:enumLiteral  "Manufacturer" .

vec:TerminalPairingSpecification
        rdf:type         owl:Class;
        rdfs:comment     "Specification for the definition of TerminalPairings.\n"@en;
        rdfs:label       "TerminalPairingSpecification"@en;
        rdfs:subClassOf  vec:Specification .

vec:boltTerminalSpecificationMaxTerminalCount
        rdf:type      owl:DatatypeProperty;
        rdfs:comment  "┬áDefines the maximum number of (ring) terminals that can be attached to this bolt at the same time.\n"@en;
        rdfs:domain   vec:BoltTerminalSpecification;
        rdfs:label    "maxTerminalCount"@en;
        rdfs:range    xs:integer .

vec:ImperialUnitName_Drachm
        rdf:type         vec:ImperialUnitName , owl:NamedIndividiual;
        vec:enumLiteral  "Drachm" .

vec:batterySpecificationI
        rdf:type            owl:ObjectProperty;
        rdfs:comment        "Specifies the current the battery provides.\n"@en;
        rdfs:domain         vec:BatterySpecification;
        rdfs:label          "i"@en;
        rdfs:range          vec:NumericalValue;
        rdfs:subPropertyOf  vec:contains .

<http://www.prostep.org/ontologies/ecad/2024/03/vec#TerminalBoltNominalSize_%230>
        rdf:type         vec:TerminalBoltNominalSize , owl:NamedIndividiual;
        vec:enumLiteral  "#0" .

vec:LocalizedTypedStringType_MainDescription
        rdf:type         vec:LocalizedTypedStringType , owl:NamedIndividiual;
        rdfs:comment     "The primary description of an element, possibly inherited from a parent element (e.g. a ComponentNode might inherit its description from the assigned UsageNode ).\n"@en;
        vec:enumLiteral  "MainDescription" .

vec:CartesianVector  rdf:type  owl:Class;
        rdfs:comment  "Abstract super class for vectors, either 2D or 3D.\n"@en;
        rdfs:label    "CartesianVector"@en .

vec:applicationConstraintFromSerialNumber
        rdf:type      owl:DatatypeProperty;
        rdfs:comment  "Specifies the lower bound of a serial number range to which the application constraint applies.\n"@en;
        rdfs:domain   vec:ApplicationConstraint;
        rdfs:label    "fromSerialNumber"@en;
        rdfs:range    xs:string .

vec:SignalTransmissionMediumType_Pneumatic
        rdf:type         vec:SignalTransmissionMediumType , owl:NamedIndividiual;
        vec:enumLiteral  "pneumatic" .

vec:nURBSCurveDegree  rdf:type  owl:DatatypeProperty;
        rdfs:comment  "Defines the degree of the NURBS (for details see the class description of NURBSCurve).\n"@en;
        rdfs:domain   vec:NURBSCurve;
        rdfs:label    "degree"@en;
        rdfs:range    xs:integer .

vec:Creation  rdf:type   owl:Class;
        rdfs:comment     "A Creation-instance provides additional information to the owning ItemVersion stating personal information on the creator and the creation date.\n"@en;
        rdfs:label       "Creation"@en;
        rdfs:subClassOf  vec:ExtendableElement .

vec:cableLeadThroughOutletIdentification
        rdf:type      owl:DatatypeProperty;
        rdfs:comment  "Specifies the identification of the CableLe adThroughOutlet. This must be unique within a CableLeadThrough .\n"@en;
        rdfs:domain   vec:CableLeadThroughOutlet;
        rdfs:label    "identification"@en;
        rdfs:range    xs:string .

vec:zoneCoverageSecondLocation
        rdf:type            owl:ObjectProperty;
        rdfs:domain         vec:ZoneCoverage;
        rdfs:label          "secondLocation"@en;
        rdfs:range          vec:Location;
        rdfs:subPropertyOf  vec:contains .

vec:SlotSealingType_MultiSealing
        rdf:type         vec:SlotSealingType , owl:NamedIndividiual;
        rdfs:comment     "The Slot is sealed with a more complex sealing variant, typically sealing multiple cavities with a single seal (e.g. a MultiCavityPlug or a combination of those).\n"@en;
        vec:enumLiteral  "MultiSealing" .

vec:LanguageCode_Rn  rdf:type  vec:LanguageCode , owl:NamedIndividiual;
        vec:enumLiteral  "Rn" .

vec:DocumentRelationType_ResponsibilityLink
        rdf:type         vec:DocumentRelationType , owl:NamedIndividiual;
        vec:enumLiteral  "ResponsibilityLink" .

vec:ModuleFamily  rdf:type  owl:Class;
        rdfs:comment     "A ModuleFamily is a mechanism to group mutually exclusive modules. This could be for example something like \"audio equipment\", \"diesel engine\".\nIn other words, a module family groups different variants of the same basic feature. In a real car configuration only one member of the family can participate. For the example module family \"audio equipment\" the members may be named: \"Basic Audio Equipment\", \"Standard Audio Equipment\", \"Premium / High End Audio Equipment\".\n"@en;
        rdfs:label       "ModuleFamily"@en;
        rdfs:subClassOf  vec:ExtendableElement .

vec:switchingStateSwitchedConnections
        rdf:type      owl:ObjectProperty;
        rdfs:comment  "Specifies the InternalComponentConnections that are switched by this SwitchingState.\n"@en;
        rdfs:domain   vec:SwitchingState;
        rdfs:label    "switchedConnections"@en;
        rdfs:range    vec:InternalComponentConnection .

vec:ringTerminalSpecificationOutsideDimension
        rdf:type            owl:ObjectProperty;
        rdfs:comment        "Specifies the diameter of the circle around the center of the bolt which passes through the farthest outside point of the contact surface of the ring terminal. (see KBLFRM-311)\n"@en;
        rdfs:domain         vec:RingTerminalSpecification;
        rdfs:label          "outsideDimension"@en;
        rdfs:range          vec:NumericalValue;
        rdfs:subPropertyOf  vec:contains .

vec:FerriteRole  rdf:type  owl:Class;
        rdfs:comment     "A FerriteRole defines the instance specific properties and relationships of a ferrite.\n"@en;
        rdfs:label       "FerriteRole"@en;
        rdfs:subClassOf  vec:Role .

vec:wireReceptionSpecificationWireElementOutsideDiameter
        rdf:type            owl:ObjectProperty;
        rdfs:comment        "Specifies a value range for valid diameters a WireElement must have to fit to the wire reception.\n"@en;
        rdfs:domain         vec:WireReceptionSpecification;
        rdfs:label          "wireElementOutsideDiameter"@en;
        rdfs:range          vec:ValueRange;
        rdfs:subPropertyOf  vec:contains .

vec:TapeRole  rdf:type   owl:Class;
        rdfs:comment     "Specific WireProtectionRole for instances of TapeSpecification.\n"@en;
        rdfs:label       "TapeRole"@en;
        rdfs:subClassOf  vec:WireProtectionRole .

vec:usageConstraintFromSerialNumber
        rdf:type      owl:DatatypeProperty;
        rdfs:comment  "Specifies the lower bound of a serial number range to which the usage constraint applies.\n"@en;
        rdfs:domain   vec:UsageConstraint;
        rdfs:label    "fromSerialNumber"@en;
        rdfs:range    xs:string .

vec:dateValuePropertyValue
        rdf:type      owl:DatatypeProperty;
        rdfs:comment  "Defines the value of the CustomProperty.\n"@en;
        rdfs:domain   vec:DateValueProperty;
        rdfs:label    "value"@en;
        rdfs:range    xs:dateTime .

vec:LanguageCode_To  rdf:type  vec:LanguageCode , owl:NamedIndividiual;
        vec:enumLiteral  "To" .

vec:topologyZoneRequiredRobustnessProperties
        rdf:type            owl:ObjectProperty;
        rdfs:comment        "Defines the robustness properties that are required in this zone. This can result in specific requirements for the used components (e.g. the ability for sealing).\n"@en;
        rdfs:domain         vec:TopologyZone;
        rdfs:label          "requiredRobustnessProperties"@en;
        rdfs:range          vec:RobustnessProperties;
        rdfs:subPropertyOf  vec:contains .

vec:LanguageCode_Fr  rdf:type  vec:LanguageCode , owl:NamedIndividiual;
        vec:enumLiteral  "Fr" .

vec:TerminalBoltNominalSize_M1
        rdf:type         vec:TerminalBoltNominalSize , owl:NamedIndividiual;
        vec:enumLiteral  "M1" .

vec:partWithSubComponentsRolePartStructureSpecification
        rdf:type      owl:ObjectProperty;
        rdfs:comment  "References the PartStructureSpecification that is instantiated by this PartWithSubComponentsRole .\n"@en;
        rdfs:domain   vec:PartWithSubComponentsRole;
        rdfs:label    "partStructureSpecification"@en;
        rdfs:range    vec:PartStructureSpecification .

vec:cavityPositionDetailCavitySealingOffset
        rdf:type            owl:ObjectProperty;
        rdfs:comment        "Defines the offset (length) by which the starting point of the sealing area is displaced insertionPosition in insertion direction."@en;
        rdfs:domain         vec:CavityPositionDetail;
        rdfs:label          "cavitySealingOffset"@en;
        rdfs:range          vec:NumericalValue;
        rdfs:subPropertyOf  vec:contains .

vec:PinType_Inductive
        rdf:type         vec:PinType , owl:NamedIndividiual;
        vec:enumLiteral  "inductive" .

vec:insulationSpecificationFirstIdentificationColor
        rdf:type            owl:ObjectProperty;
        rdfs:comment        "Specifies the first identification color of the insulation.\n"@en;
        rdfs:domain         vec:InsulationSpecification;
        rdfs:label          "firstIdentificationColor"@en;
        rdfs:range          vec:Color;
        rdfs:subPropertyOf  vec:contains .

vec:multiFuseSpecificationFuseComponents
        rdf:type            owl:ObjectProperty;
        rdfs:domain         vec:MultiFuseSpecification;
        rdfs:label          "fuseComponents"@en;
        rdfs:range          vec:FuseComponent;
        rdfs:subPropertyOf  vec:contains .

vec:Permission  rdf:type  owl:Class;
        rdfs:comment     "Describes an act of acceptance together with information about the responsible person, department and company who directly provoked the approval level and status as described in the referenced Approval-instance. (see KBLFRM-229)\n"@en;
        rdfs:label       "Permission"@en;
        rdfs:subClassOf  vec:ExtendableElement .

<http://www.prostep.org/ontologies/ecad/2024/03/vec#TerminalBoltNominalSize_%235>
        rdf:type         vec:TerminalBoltNominalSize , owl:NamedIndividiual;
        vec:enumLiteral  "#5" .

vec:topologyZoneSpecificationZone
        rdf:type            owl:ObjectProperty;
        rdfs:comment        "Specifies the TopologyZones that are part of the TopologyZoneSpecification .\n"@en;
        rdfs:domain         vec:TopologyZoneSpecification;
        rdfs:label          "zone"@en;
        rdfs:range          vec:TopologyZone;
        rdfs:subPropertyOf  vec:contains .

vec:PrimaryPartType_MultiFuse
        rdf:type         vec:PrimaryPartType , owl:NamedIndividiual;
        vec:enumLiteral  "MultiFuse" .

vec:occurrenceOrUsageDescription
        rdf:type            owl:ObjectProperty;
        rdfs:comment        "Specifies additional, human readable information about the OccurrenceOrUsage.\n"@en;
        rdfs:domain         vec:OccurrenceOrUsage;
        rdfs:label          "description"@en;
        rdfs:range          vec:AbstractLocalizedString;
        rdfs:subPropertyOf  vec:contains .

vec:PinTimingType_InitTime
        rdf:type         vec:PinTimingType , owl:NamedIndividiual;
        vec:enumLiteral  "initTime" .

vec:connectorHousingSpecificationCoupleable
        rdf:type      owl:DatatypeProperty;
        rdfs:comment  "Defines whether the connector is coupleable or not. Connectors that are coupleable can be used in an inline position. Connectors that are not coupleable can be connected only to an ECU or something similar.\n"@en;
        rdfs:domain   vec:ConnectorHousingSpecification;
        rdfs:label    "coupleable"@en;
        rdfs:range    xs:boolean .

vec:specificRoleSpecificRoleType
        rdf:type      owl:DatatypeProperty;
        rdfs:comment  "Specifies the type for role.\n"@en;
        rdfs:domain   vec:SpecificRole;
        rdfs:label    "specificRoleType"@en;
        rdfs:range    xs:string .

vec:PlacementType_OnPoint
        rdf:type         vec:PlacementType , owl:NamedIndividiual;
        rdfs:comment     " OnPoint refers to an OnPointPlacement .\n"@en;
        vec:enumLiteral  "OnPoint" .

vec:LocalizedString  rdf:type  owl:Class;
        rdfs:comment     "Allows the internationalization of text contents. Attributes of the type LocalizedString normally have the multiplicity [0..*]. This means that such an attribute can have multiple values for different locales. It must not have multiple values for the same locale.\n"@en;
        rdfs:label       "LocalizedString"@en;
        rdfs:subClassOf  vec:AbstractLocalizedString .

vec:DocumentType_WiringDescription
        rdf:type         vec:DocumentType , owl:NamedIndividiual;
        rdfs:comment     ""@en;
        vec:enumLiteral  "WiringDescription" .

vec:occurrenceOrUsageViewItem2DOccurrenceOrUsage
        rdf:type      owl:ObjectProperty;
        rdfs:comment  "Specifies the OccurrenceOrUsages which are represented by the view item. Important: To use one OccurenceOrUsageViewItem for multiple OccurrenceOrUsages is only valid, if the referenced items are true alternatives to each other. That means, they must have an identical placement, the geometrical models used for each item must be substitutable and the item must be mutually exclusive to each other.\n"@en;
        rdfs:domain   vec:OccurrenceOrUsageViewItem2D;
        rdfs:label    "occurrenceOrUsage"@en;
        rdfs:range    vec:OccurrenceOrUsage .

vec:localGeometrySpecificationCartesianPoint
        rdf:type            owl:ObjectProperty;
        rdfs:comment        "All CartesianPoint3Ds that are used in this LocalGeometrySpecification. All CartesianPoint3Ds are defined in relation to the coordinate system of the component.\n"@en;
        rdfs:domain         vec:LocalGeometrySpecification;
        rdfs:label          "cartesianPoint"@en;
        rdfs:range          vec:CartesianPoint3D;
        rdfs:subPropertyOf  vec:contains .

vec:networkPortSignalDirection
        rdf:type            owl:ObjectProperty;
        rdfs:comment        "Specifies the direction of the signal on this NetworkPort.\n"@en;
        rdfs:domain         vec:NetworkPort;
        rdfs:label          "signalDirection"@en;
        rdfs:range          vec:SignalDirection;
        rdfs:subPropertyOf  vec:contains .

vec:NetworkPortViewItem
        rdf:type      owl:Class;
        rdfs:comment  "A NetworkPortViewItem represents a NetworkPort within a NetworkNodeViewItem and defines its position on the node."@en;
        rdfs:label    "NetworkPortViewItem"@en .

vec:pinWireMappingSpecificationPinWireMappingPoint
        rdf:type            owl:ObjectProperty;
        rdfs:domain         vec:PinWireMappingSpecification;
        rdfs:label          "pinWireMappingPoint"@en;
        rdfs:range          vec:PinWireMappingPoint;
        rdfs:subPropertyOf  vec:contains .

vec:netGroupNetGroupType
        rdf:type      owl:DatatypeProperty;
        rdfs:comment  "Specifies the type of the group.\n"@en;
        rdfs:domain   vec:NetGroup;
        rdfs:label    "netGroupType"@en;
        rdfs:range    xs:string .

vec:Slot  rdf:type       owl:Class;
        rdfs:comment     "A slot is a group of cavities in a connector housing with own properties. The design of a slot is described in a SlotSpecification.\n"@en;
        rdfs:label       "Slot"@en;
        rdfs:subClassOf  vec:AbstractSlot .

vec:routingPath  rdf:type   owl:ObjectProperty;
        rdfs:comment        "Specifies a Path on the topology that is used for the routing. \n"@en;
        rdfs:domain         vec:Routing;
        rdfs:label          "path"@en;
        rdfs:range          vec:Path;
        rdfs:subPropertyOf  vec:contains .

vec:UsageNodeType_Lamp
        rdf:type         vec:UsageNodeType , owl:NamedIndividiual;
        vec:enumLiteral  "Lamp" .

vec:diodeSpecificationBreakDownVoltage
        rdf:type            owl:ObjectProperty;
        rdfs:comment        "Voltage at which the diode starts conducting in reverse direction.\n"@en;
        rdfs:domain         vec:DiodeSpecification;
        rdfs:label          "breakDownVoltage"@en;
        rdfs:range          vec:NumericalValue;
        rdfs:subPropertyOf  vec:contains .

vec:LanguageCode_Tt  rdf:type  vec:LanguageCode , owl:NamedIndividiual;
        vec:enumLiteral  "Tt" .

vec:CartesianVector3D
        rdf:type         owl:Class;
        rdfs:comment     "A Cartesian vector in three-dimensional space.\n"@en;
        rdfs:label       "CartesianVector3D"@en;
        rdfs:subClassOf  vec:CartesianVector .

vec:moduleFamilySpecificationModuleFamily
        rdf:type            owl:ObjectProperty;
        rdfs:comment        "Specifies the ModuleFamilies defined in the ModuleFamilySpecification.\n"@en;
        rdfs:domain         vec:ModuleFamilySpecification;
        rdfs:label          "moduleFamily"@en;
        rdfs:range          vec:ModuleFamily;
        rdfs:subPropertyOf  vec:contains .

vec:diodeSpecificationThresholdVoltage
        rdf:type            owl:ObjectProperty;
        rdfs:comment        "Voltage at which the diode starts conducting in forward direction.\n"@en;
        rdfs:domain         vec:DiodeSpecification;
        rdfs:label          "thresholdVoltage"@en;
        rdfs:range          vec:NumericalValue;
        rdfs:subPropertyOf  vec:contains .

vec:WireEnd  rdf:type    owl:Class;
        rdfs:comment     "A WireEnd is the end of a wire. This class mainly needed for the definition of a contacting. As a wire can be contacted on more than two ends (e.g. IDC) the WireEnd has a position on the wire.\n"@en;
        rdfs:label       "WireEnd"@en;
        rdfs:subClassOf  vec:ExtendableElement .

vec:vecContentStandardCopyrightInformation
        rdf:type      owl:ObjectProperty;
        rdfs:comment  "References the CopyrightInformation that is in effect for the complete content of this VecContent . It is applied to all ItemVersions that do not references their own individual CopyrightInformation.\n"@en;
        rdfs:domain   vec:VecContent;
        rdfs:label    "standardCopyrightInformation"@en;
        rdfs:range    vec:CopyrightInformation .

vec:sheetOrChapterReferencedPart
        rdf:type      owl:ObjectProperty;
        rdfs:comment  "The association is an informative link which PartVersions are described by the SheetOrChapter. \n"@en;
        rdfs:domain   vec:SheetOrChapter;
        rdfs:label    "referencedPart"@en;
        rdfs:range    vec:PartVersion .

vec:SheetOrChapter  rdf:type  owl:Class;
        rdfs:comment     "Documents can be structured into sheets or chapters. Since it is possible, that one document describes a couple of parts it is necessary to be able to specify which sheet or chapter contains the description of which part. (see KBLFRM-308)\n"@en;
        rdfs:label       "SheetOrChapter"@en;
        rdfs:subClassOf  vec:ExtendableElement .

vec:TerminalBoltNominalSize_M6
        rdf:type         vec:TerminalBoltNominalSize , owl:NamedIndividiual;
        vec:enumLiteral  "M6" .

vec:PrimaryPartType_BoltTerminal
        rdf:type         vec:PrimaryPartType , owl:NamedIndividiual;
        vec:enumLiteral  "BoltTerminal" .

vec:TransmissionMediumType_Electrical
        rdf:type         vec:TransmissionMediumType , owl:NamedIndividiual;
        vec:enumLiteral  "Electrical" .

vec:FunctionalRequirementType_FunctionalSafety
        rdf:type         vec:FunctionalRequirementType , owl:NamedIndividiual;
        rdfs:comment     "Functional safety requirements e.g. ASIL Level.\n┬á\n"@en;
        vec:enumLiteral  "FunctionalSafety" .

vec:Color  rdf:type   owl:Class;
        rdfs:comment  "Specifies a color value. A color is always defined by a key value. What color is meant by this key value is defined by a standard reference system (e.g. RAL).\nFor example, if a RAL color should be expressed in the terms of the VEC the referenceSystem would be \"RAL\", the key would be the RAL number defined by the standard (e.g. \"1003\" for signal yellow).\nAttributes of the type Color normally have the multiplicity [0..*]. This means that such an attribute can have a value for different referenceSystems (e.g. RAL, RGB,...). It must not have multiple values for the same ReferenceSystem.\n"@en;
        rdfs:label    "Color"@en .

vec:tubeSpecificationInnerDiameter
        rdf:type            owl:ObjectProperty;
        rdfs:comment        "Defines the inner diameter of a tube. In the case of a shrinkable tube, it is the diameter of the tube in the unshrinked state.\n"@en;
        rdfs:domain         vec:TubeSpecification;
        rdfs:label          "innerDiameter"@en;
        rdfs:range          vec:NumericalValue;
        rdfs:subPropertyOf  vec:contains .

vec:functionalStructureNodeChildNodes
        rdf:type            owl:ObjectProperty;
        rdfs:domain         vec:FunctionalStructureNode;
        rdfs:label          "childNodes"@en;
        rdfs:range          vec:FunctionalStructureNode;
        rdfs:subPropertyOf  vec:contains .

vec:PartNature_Preliminary
        rdf:type         vec:PartNature , owl:NamedIndividiual;
        rdfs:comment     " Preliminary PartVersion represent part numbers which are used as place holders for parts that are not yet developed, or which are representing prototype parts that are not allowed in serial production.\n"@en;
        vec:enumLiteral  "Preliminary" .

vec:placementPlacedElement
        rdf:type      owl:ObjectProperty;
        rdfs:comment  "References the PlaceableElementRoles placed by the Placement. \n"@en;
        rdfs:domain   vec:Placement;
        rdfs:label    "placedElement"@en;
        rdfs:range    vec:PlaceableElementRole .

vec:approvalLevelOfApproval
        rdf:type            owl:ObjectProperty;
        rdfs:comment        "Relates to activities that are allowed with the ItemVersion after release for example building pilot tools or production tools. The levelOfApproval applies to the ItemVersion itself without further detailing or additional context. So, for example \"Free\" means, that from a component's perspective the corresponding PartVersion has satisfied all qualification procedures and can be used within its specified limits without restriction.\nThe levels Planned , Free , Invalid refer to a single approval level. The levels Develop and Restricted refer to a category of approval levels in the lifecycle of an ItemVersion that all belong to the same phase but are highly company specific. For example, Develop approvals might be a \"a start of construction approval\" or a \"building of prototypes or tools allowed approval\". \"Restricted\" approvals might be \"only for special purpose vehicles\", \"spare part only\" or \"residual parts may be used up\".\nIn these cases, the additionalLevelInformation can be used to provide further information (e.g. a company specific approval level).\n"@en;
        rdfs:domain         vec:Approval;
        rdfs:label          "levelOfApproval"@en;
        rdfs:range          vec:LevelOfApproval;
        rdfs:subPropertyOf  vec:contains .

vec:placementPointPositionTangent
        rdf:type            owl:ObjectProperty;
        rdfs:comment        "A vector in the direction of the tangent on the TopologySegment that is attached to the PlacementPoint represented by this instance. The vector is defined in the coordinate system of the 3D model of the component.\n"@en;
        rdfs:domain         vec:PlacementPointPosition;
        rdfs:label          "tangent"@en;
        rdfs:range          vec:CartesianVector3D;
        rdfs:subPropertyOf  vec:contains .

vec:componentConnectorIdentification
        rdf:type      owl:DatatypeProperty;
        rdfs:comment  "Specifies a unique identification of the ComponentConnector. The identification is guaranteed to be unique within the ComponentNode."@en;
        rdfs:domain   vec:ComponentConnector;
        rdfs:label    "identification"@en;
        rdfs:range    xs:string .

vec:moduleFamilyModuleInFamily
        rdf:type      owl:ObjectProperty;
        rdfs:comment  "References the Modules that belong to the ModuleFamily. \n"@en;
        rdfs:domain   vec:ModuleFamily;
        rdfs:label    "moduleInFamily"@en;
        rdfs:range    vec:PartWithSubComponentsRole .

vec:BoltMountedFixingBoltShape_Circular
        rdf:type         vec:BoltMountedFixingBoltShape , owl:NamedIndividiual;
        vec:enumLiteral  "Circular" .

vec:terminalReceptionIdentification
        rdf:type      owl:DatatypeProperty;
        rdfs:comment  "Specifies a unique identification of the TerminalReception. The identification is guaranteed to be unique within the TerminalSpecification (this might be for example a reception number).\n"@en;
        rdfs:domain   vec:TerminalReception;
        rdfs:label    "identification"@en;
        rdfs:range    xs:string .

vec:couplingPointMatingPoint
        rdf:type            owl:ObjectProperty;
        rdfs:comment        "Specifies the MatingPoints defined within the CouplingPoint .\n"@en;
        rdfs:domain         vec:CouplingPoint;
        rdfs:label          "matingPoint"@en;
        rdfs:range          vec:MatingPoint;
        rdfs:subPropertyOf  vec:contains .

vec:SlotLayoutType_USBTypeASuperSpeed
        rdf:type         vec:SlotLayoutType , owl:NamedIndividiual;
        vec:enumLiteral  "USBTypeASuperSpeed" .

vec:TerminalBoltNominalSize_M5.5
        rdf:type         vec:TerminalBoltNominalSize , owl:NamedIndividiual;
        vec:enumLiteral  "M5.5" .

vec:documentVersionDocumentType
        rdf:type            owl:ObjectProperty;
        rdfs:comment        "The type of the document, that is defined in an OpenEnumeration and gives a hint about the content of the document. Values for typical types of documents in the process are predefined (e.g. a part master document for the specification of a PartVersion ).\nAt later point, further constraint might be attached to documentType defining a minimum content for certain types of documents.\n"@en;
        rdfs:domain         vec:DocumentVersion;
        rdfs:label          "documentType"@en;
        rdfs:range          vec:DocumentType;
        rdfs:subPropertyOf  vec:contains .

vec:multiCavitySealSpecificationAssignment
        rdf:type            owl:ObjectProperty;
        rdfs:comment        "References the OpenCavitiesAssignments that are valid for this MultiCavitySeal . One individual OpenCavitiesAssignment is used for each connector housing that matches witch this MultiCavitySeal.\n"@en;
        rdfs:domain         vec:MultiCavitySealSpecification;
        rdfs:label          "assignment"@en;
        rdfs:range          vec:OpenCavitiesAssignment;
        rdfs:subPropertyOf  vec:contains .

vec:HousingComponentReference
        rdf:type         owl:Class;
        rdfs:comment     "A HousingComponentReference represents the usage of a HousingComponent in the context of a PartUsage or PartOccurrence. (KBLFRM-401)\n"@en;
        rdfs:label       "HousingComponentReference"@en;
        rdfs:subClassOf  vec:ConfigurableElement .

vec:connectorHousingCapSpecificationWireAddOn
        rdf:type            owl:ObjectProperty;
        rdfs:comment        "Specifies the wire length add on needed for the cap.\n"@en;
        rdfs:domain         vec:ConnectorHousingCapSpecification;
        rdfs:label          "wireAddOn"@en;
        rdfs:range          vec:NumericalValue;
        rdfs:subPropertyOf  vec:contains .

vec:componentPortIdentification
        rdf:type      owl:DatatypeProperty;
        rdfs:comment  "Specifies a unique identification of the ComponentPort. The identification is guaranteed to be unique within the ComponentConnector.\n"@en;
        rdfs:domain   vec:ComponentPort;
        rdfs:label    "identification"@en;
        rdfs:range    xs:string .

vec:TerminalReception
        rdf:type         owl:Class;
        rdfs:comment     "A TerminalReception is the area of a terminal where the contacting with another terminal (e.g. between a connector housing and a control unit) takes place. Normally the terminal reception is placed in a cavity of a connector housing.\nThis class represents such an area on the terminal.\n"@en;
        rdfs:label       "TerminalReception"@en;
        rdfs:subClassOf  vec:ExtendableElement .

vec:cartesianPoint3DX
        rdf:type      owl:DatatypeProperty;
        rdfs:comment  "Specifies the value of x-coordinate of the Cartesian point. The unit of this value is the baseUnit of containing BuildingBlockSpecification3D.\n"@en;
        rdfs:domain   vec:CartesianPoint3D;
        rdfs:label    "x"@en;
        rdfs:range    xs:double .

vec:HoleMountedFixingHoleType_MetricThread
        rdf:type         vec:HoleMountedFixingHoleType , owl:NamedIndividiual;
        rdfs:comment     "The hole provides a metric thread for fixation."@en;
        vec:enumLiteral  "MetricThread" .

vec:LabelType_BarCode
        rdf:type         vec:LabelType , owl:NamedIndividiual;
        vec:enumLiteral  "BarCode" .

vec:PinType_Capacitive
        rdf:type         vec:PinType , owl:NamedIndividiual;
        vec:enumLiteral  "capacitive" .

vec:wireReceptionSpecificationCutOffTabLength
        rdf:type            owl:ObjectProperty;
        rdfs:comment        "Specifies the length of the cut off tab (wire reception, see diagram \"Terminal Dimensions\").\n"@en;
        rdfs:domain         vec:WireReceptionSpecification;
        rdfs:label          "cutOffTabLength"@en;
        rdfs:range          vec:NumericalValue;
        rdfs:subPropertyOf  vec:contains .

vec:variantStructureNodeIdentification
        rdf:type      owl:DatatypeProperty;
        rdfs:comment  "Specifies a unique identification of the VariantStructureNode .\n"@en;
        rdfs:domain   vec:VariantStructureNode;
        rdfs:label    "identification"@en;
        rdfs:range    xs:string .

vec:valueRangePropertyValue
        rdf:type            owl:ObjectProperty;
        rdfs:comment        "Defines the value of the CustomProperty.\n"@en;
        rdfs:domain         vec:ValueRangeProperty;
        rdfs:label          "value"@en;
        rdfs:range          vec:ValueRange;
        rdfs:subPropertyOf  vec:contains .

vec:ValueDetermination_Measured
        rdf:type         vec:ValueDetermination , owl:NamedIndividiual;
        rdfs:comment     "The value is determined by an exact measurement.\n"@en;
        vec:enumLiteral  "Measured" .

vec:TerminalBoltNominalSize_M60
        rdf:type         vec:TerminalBoltNominalSize , owl:NamedIndividiual;
        vec:enumLiteral  "M60" .

vec:FittingForm_Wye  rdf:type  vec:FittingForm , owl:NamedIndividiual;
        rdfs:comment     "Symetric division (2 ways).\n"@en;
        vec:enumLiteral  "Wye" .

vec:SlotLayoutType_USBMiniAB
        rdf:type         vec:SlotLayoutType , owl:NamedIndividiual;
        vec:enumLiteral  "USBMiniAB" .

vec:dimensionValueCalculated
        rdf:type      owl:DatatypeProperty;
        rdfs:comment  "Defines if the value of the Dimension was calculated (e.g. the sum of segment lengths in the topology) or if it was defined manually.\n"@en;
        rdfs:domain   vec:Dimension;
        rdfs:label    "valueCalculated"@en;
        rdfs:range    xs:boolean .

vec:documentVersionReferencedPart
        rdf:type      owl:ObjectProperty;
        rdfs:comment  "The association is an informative link which PartVersions are described by the DocumentVersion. \n"@en;
        rdfs:domain   vec:DocumentVersion;
        rdfs:label    "referencedPart"@en;
        rdfs:range    vec:PartVersion .

vec:PrimaryPartType_Grommet
        rdf:type         vec:PrimaryPartType , owl:NamedIndividiual;
        vec:enumLiteral  "Grommet" .

vec:EdgeMountedFixingSpecification
        rdf:type         owl:Class;
        rdfs:comment     "Specification for fixings that are mounted onto an edge.\n"@en;
        rdfs:label       "EdgeMountedFixingSpecification"@en;
        rdfs:subClassOf  vec:FixingSpecification .

vec:wireElementReferenceLabelType
        rdf:type            owl:ObjectProperty;
        rdfs:domain         vec:WireElementReference;
        rdfs:label          "labelType"@en;
        rdfs:range          vec:LabelType;
        rdfs:subPropertyOf  vec:contains .

vec:FuseType_Type_E  rdf:type  vec:FuseType , owl:NamedIndividiual;
        rdfs:comment     "also known as: maxi\n"@en;
        vec:enumLiteral  "Type_E" .

vec:measurementPointIdentification
        rdf:type      owl:DatatypeProperty;
        rdfs:comment  "Specifies a unique identification of the MeasurementPoint. The identification is guaranteed to be unique within a component.\n"@en;
        rdfs:domain   vec:MeasurementPoint;
        rdfs:label    "identification"@en;
        rdfs:range    xs:string .

vec:localizedTypedStringType
        rdf:type            owl:ObjectProperty;
        rdfs:comment        "Defines the type of the LocalizedTypedString . This allows the definition of a more detailed semantic than the semantic of the attribute itself with the type LocalizedTypedString. Agreed type values are defined in an OpenEnumeration.\n"@en;
        rdfs:domain         vec:LocalizedTypedString;
        rdfs:label          "type"@en;
        rdfs:range          vec:LocalizedTypedStringType;
        rdfs:subPropertyOf  vec:contains .

vec:NetworkPortViewItemSide
        rdf:type             owl:Class;
        rdfs:label           "NetworkPortViewItemSide"@en;
        rdfs:subClassOf      vec:ClosedEnumeration;
        owl:equivalentClass  [ rdf:type   owl:Class;
                               owl:oneOf  ( vec:NetworkPortViewItemSide_Top vec:NetworkPortViewItemSide_Bottom vec:NetworkPortViewItemSide_Left vec:NetworkPortViewItemSide_Right )
                             ] .

vec:FittingForm_Cross
        rdf:type         vec:FittingForm , owl:NamedIndividiual;
        vec:enumLiteral  "Cross" .

vec:conductorSpecificationNumberOfStrands
        rdf:type            owl:ObjectProperty;
        rdfs:comment        "Specifies the number of strands in one conductor. If the conductor is solid than the number of strands would be one.\n"@en;
        rdfs:domain         vec:ConductorSpecification;
        rdfs:label          "numberOfStrands"@en;
        rdfs:range          vec:NumericalValue;
        rdfs:subPropertyOf  vec:contains .

vec:copyrightInformationCopyrightNote
        rdf:type            owl:ObjectProperty;
        rdfs:comment        "An informal text which specifies copyright information.\n"@en;
        rdfs:domain         vec:CopyrightInformation;
        rdfs:label          "copyrightNote"@en;
        rdfs:range          vec:LocalizedString;
        rdfs:subPropertyOf  vec:contains .

vec:wireReceptionSpecificationConductorCrimpLength
        rdf:type            owl:ObjectProperty;
        rdfs:comment        "Specifies the length of the conductor crimp (wire reception, see diagram \"Terminal Dimensions\").\n"@en;
        rdfs:domain         vec:WireReceptionSpecification;
        rdfs:label          "conductorCrimpLength"@en;
        rdfs:range          vec:NumericalValue;
        rdfs:subPropertyOf  vec:contains .

vec:HarnessDrawingSpecification2D
        rdf:type         owl:Class;
        rdfs:comment     "The HarnessDrawingSpecification2D specifies a two-dimensional drawing of a harness. A harness drawing is composed of one or more BuildingBlockSpecifaction2D which are placed on the drawing.\n"@en;
        rdfs:label       "HarnessDrawingSpecification2D"@en;
        rdfs:subClassOf  vec:Specification .

vec:SignalTransmissionMediumType_Electrical
        rdf:type         vec:SignalTransmissionMediumType , owl:NamedIndividiual;
        vec:enumLiteral  "electrical" .

vec:terminalRoleWireReceptionReference
        rdf:type            owl:ObjectProperty;
        rdfs:comment        "Specifies the WireReceptionReferences of this TerminalRole.\n"@en;
        rdfs:domain         vec:TerminalRole;
        rdfs:label          "wireReceptionReference"@en;
        rdfs:range          vec:WireReceptionReference;
        rdfs:subPropertyOf  vec:contains .

vec:NetType  rdf:type  owl:Class;
        rdfs:comment  "A NetType defines the different types of Nets used in the NetSpecification . The level of detail of the NetTypes for the can be process dependent.\nA NetType could be just used to differentiate between conventional (analogue) communication and bus communication (digital), it can also already define the different types of digital communication (e.g. CAN, MOST, Ethernet).\n"@en;
        rdfs:label    "NetType"@en .

vec:netDescription  rdf:type  owl:ObjectProperty;
        rdfs:comment        "Room for additional, human readable information about the Net.\n"@en;
        rdfs:domain         vec:Net;
        rdfs:label          "description"@en;
        rdfs:range          vec:AbstractLocalizedString;
        rdfs:subPropertyOf  vec:contains .

vec:PrimaryLockingType_None
        rdf:type         vec:PrimaryLockingType , owl:NamedIndividiual;
        vec:enumLiteral  "None" .

vec:UsageNodeType_Relay
        rdf:type         vec:UsageNodeType , owl:NamedIndividiual;
        vec:enumLiteral  "Relay" .

vec:PinVoltageType_MaxVoltage
        rdf:type         vec:PinVoltageType , owl:NamedIndividiual;
        vec:enumLiteral  "maxVoltage" .

vec:boltTerminalSpecificationBoltType
        rdf:type            owl:ObjectProperty;
        rdfs:comment        "Specifies the type of the bolt.\n"@en;
        rdfs:domain         vec:BoltTerminalSpecification;
        rdfs:label          "boltType"@en;
        rdfs:range          vec:TerminalBoltType;
        rdfs:subPropertyOf  vec:contains .

vec:fileBasedInstructionDataFormat
        rdf:type      owl:DatatypeProperty;
        rdfs:comment  "The dataFormat specifies the format of the FileReference. The dataFormat has to be a valid \"Internet Media Type\" (see https://www.iana.org/assignments/media-types/media-types.xhtml ).\n"@en;
        rdfs:domain   vec:FileBasedInstruction;
        rdfs:label    "dataFormat"@en;
        rdfs:range    xs:string .

vec:occurrenceOrUsageAliasId
        rdf:type            owl:ObjectProperty;
        rdfs:comment        "Room to specify additional identifiers for the OccurrenceOrUsage.\n"@en;
        rdfs:domain         vec:OccurrenceOrUsage;
        rdfs:label          "aliasId"@en;
        rdfs:range          vec:AliasIdentification;
        rdfs:subPropertyOf  vec:contains .

vec:documentBasedInstructionReferencedDocument
        rdf:type      owl:ObjectProperty;
        rdfs:comment  "References the DocumentVersion that is used as an Instruction.\n"@en;
        rdfs:domain   vec:DocumentBasedInstruction;
        rdfs:label    "referencedDocument"@en;
        rdfs:range    vec:DocumentVersion .

vec:TapingDirection  rdf:type  owl:Class;
        rdfs:comment         "Defines the direction in relation to the start┬á&┬áend-Location of the corresponding placement. If no TapingDirection is defined it is arbitrary.\n"@en;
        rdfs:label           "TapingDirection"@en;
        rdfs:subClassOf      vec:ClosedEnumeration;
        owl:equivalentClass  [ rdf:type   owl:Class;
                               owl:oneOf  ( vec:TapingDirection_FromStart vec:TapingDirection_FromEnd )
                             ] .

vec:segmentCrossSectionAreaCrossSectionAreaType
        rdf:type            owl:ObjectProperty;
        rdfs:comment        "Specifies the type of the cross-section area of the segment. Different types are for example needed to differentiate between the designed space of a segment and the required space (e.g. calculated from the wires going through the segment).\nAttribute is defined as an OpenEnumeration.\n"@en;
        rdfs:domain         vec:SegmentCrossSectionArea;
        rdfs:label          "crossSectionAreaType"@en;
        rdfs:range          vec:SegmentCrossSectionAreaType;
        rdfs:subPropertyOf  vec:contains .

vec:FittingForm_EndPiece
        rdf:type         vec:FittingForm , owl:NamedIndividiual;
        rdfs:comment     "For covering pipe ends when no screw fitting is used. Allows cables to be inserted level to avoid damage.\n"@en;
        vec:enumLiteral  "EndPiece" .

vec:PinWireMappingSpecification
        rdf:type         owl:Class;
        rdfs:comment     "A PinWireMappingSpecification can be used create variance free mappings between a wire (represented by the contact point) and the pin of an E/E component. This is a possibility to create a shortcut in the model between a wire and its connected E/E-component (e.g. a fuse) that might be only indirectly connected to a wire (e.g. via a fuse and relay carrier). This is a relevant information for e.g. the validation of fusing. See the Pin Wire Mapping Diagram for more details.\n"@en;
        rdfs:label       "PinWireMappingSpecification"@en;
        rdfs:subClassOf  vec:Specification .

vec:PinApplianceType  rdf:type  owl:Class;
        rdfs:comment     "Classifies the appliance of a Pin in terms of the duration of the appliance.\nE.g. the power supply pin of a power window has \"shortTerm\" PinApplianceType, in contrast to the head light which is a \"long term\".\n"@en;
        rdfs:label       "PinApplianceType"@en;
        rdfs:subClassOf  vec:OpenEnumeration .

vec:SiUnitName_Ohm  rdf:type  vec:SiUnitName , owl:NamedIndividiual;
        vec:enumLiteral  "Ohm" .

vec:diodeSpecificationIMax
        rdf:type            owl:ObjectProperty;
        rdfs:comment        "Specifies the maximum electric current tolerated by the diode.\n"@en;
        rdfs:domain         vec:DiodeSpecification;
        rdfs:label          "iMax"@en;
        rdfs:range          vec:NumericalValue;
        rdfs:subPropertyOf  vec:contains .

vec:UsageNodeType_Fixing
        rdf:type         vec:UsageNodeType , owl:NamedIndividiual;
        vec:enumLiteral  "Fixing" .

vec:LanguageCode  rdf:type   owl:Class;
        rdfs:comment         "Enumeration for the definition of ISO language codes. (see KBLFRM-317)\n"@en;
        rdfs:label           "LanguageCode"@en;
        rdfs:subClassOf      vec:ClosedEnumeration;
        owl:equivalentClass  [ rdf:type   owl:Class;
                               owl:oneOf  ( vec:LanguageCode_Aa vec:LanguageCode_Ab vec:LanguageCode_Af vec:LanguageCode_Am vec:LanguageCode_Ar vec:LanguageCode_As vec:LanguageCode_Ay vec:LanguageCode_Az vec:LanguageCode_Ba vec:LanguageCode_Be vec:LanguageCode_Bg vec:LanguageCode_Bh vec:LanguageCode_Bi vec:LanguageCode_Bn vec:LanguageCode_Bo vec:LanguageCode_Br vec:LanguageCode_Ca vec:LanguageCode_Co vec:LanguageCode_Cs vec:LanguageCode_Cy vec:LanguageCode_Da vec:LanguageCode_De vec:LanguageCode_Dz vec:LanguageCode_El vec:LanguageCode_En vec:LanguageCode_Eo vec:LanguageCode_Es vec:LanguageCode_Et vec:LanguageCode_Eu vec:LanguageCode_Fa vec:LanguageCode_Fi vec:LanguageCode_Fj vec:LanguageCode_Fo vec:LanguageCode_Fr vec:LanguageCode_Fy vec:LanguageCode_Ga vec:LanguageCode_Gd vec:LanguageCode_Gl vec:LanguageCode_Gn vec:LanguageCode_Gu vec:LanguageCode_Ha vec:LanguageCode_Hi vec:LanguageCode_He vec:LanguageCode_Hr vec:LanguageCode_Hu vec:LanguageCode_Hy vec:LanguageCode_Ia vec:LanguageCode_Id vec:LanguageCode_Ie vec:LanguageCode_Ik vec:LanguageCode_In vec:LanguageCode_Is vec:LanguageCode_It vec:LanguageCode_Iu vec:LanguageCode_Iw vec:LanguageCode_Ja vec:LanguageCode_Ji vec:LanguageCode_Jw vec:LanguageCode_Ka vec:LanguageCode_Kk vec:LanguageCode_Kl vec:LanguageCode_Km vec:LanguageCode_Kn vec:LanguageCode_Ko vec:LanguageCode_Ks vec:LanguageCode_Ku vec:LanguageCode_Ky vec:LanguageCode_La vec:LanguageCode_Ln vec:LanguageCode_Lo vec:LanguageCode_Lt vec:LanguageCode_Lv vec:LanguageCode_Mg vec:LanguageCode_Mi vec:LanguageCode_Mk vec:LanguageCode_Ml vec:LanguageCode_Mn vec:LanguageCode_Mo vec:LanguageCode_Mr vec:LanguageCode_Ms vec:LanguageCode_Mt vec:LanguageCode_My vec:LanguageCode_Na vec:LanguageCode_Ne vec:LanguageCode_Nl vec:LanguageCode_No vec:LanguageCode_Oc vec:LanguageCode_Om vec:LanguageCode_Or vec:LanguageCode_Pa vec:LanguageCode_Pl vec:LanguageCode_Ps vec:LanguageCode_Pt vec:LanguageCode_Qu vec:LanguageCode_Rm vec:LanguageCode_Rn vec:LanguageCode_Ro vec:LanguageCode_Ru vec:LanguageCode_Rw vec:LanguageCode_Sa vec:LanguageCode_Sd vec:LanguageCode_Sg vec:LanguageCode_Sh vec:LanguageCode_Si vec:LanguageCode_Sk vec:LanguageCode_Sl vec:LanguageCode_Sm vec:LanguageCode_Sn vec:LanguageCode_So vec:LanguageCode_Sq vec:LanguageCode_Sr vec:LanguageCode_Ss vec:LanguageCode_St vec:LanguageCode_Su vec:LanguageCode_Sv vec:LanguageCode_Sw vec:LanguageCode_Ta vec:LanguageCode_Te vec:LanguageCode_Tg vec:LanguageCode_Th vec:LanguageCode_Zi vec:LanguageCode_Tk vec:LanguageCode_Tl vec:LanguageCode_Tn vec:LanguageCode_To vec:LanguageCode_Tr vec:LanguageCode_Ts vec:LanguageCode_Tt vec:LanguageCode_Tw vec:LanguageCode_Ug vec:LanguageCode_Uk vec:LanguageCode_Ur vec:LanguageCode_Uz vec:LanguageCode_Vi vec:LanguageCode_Vo vec:LanguageCode_Wo vec:LanguageCode_Xh vec:LanguageCode_Yi vec:LanguageCode_Yo vec:LanguageCode_Za vec:LanguageCode_Zh vec:LanguageCode_Zu )
                             ] .

vec:DocumentType_DeviationTable
        rdf:type         vec:DocumentType , owl:NamedIndividiual;
        rdfs:comment     "Documents that define allowed deviations from specified part numbers.\n"@en;
        vec:enumLiteral  "DeviationTable" .

vec:netTypeSignalSubType
        rdf:type            owl:ObjectProperty;
        rdfs:domain         vec:NetType;
        rdfs:label          "signalSubType"@en;
        rdfs:range          vec:SignalSubType;
        rdfs:subPropertyOf  vec:contains .

vec:usageConstraintFromDate
        rdf:type      owl:DatatypeProperty;
        rdfs:comment  "Specifies the lower bound of the time period to which the usage constraint applies.\n"@en;
        rdfs:domain   vec:UsageConstraint;
        rdfs:label    "fromDate"@en;
        rdfs:range    xs:dateTime .

vec:SignalDirection_In
        rdf:type         vec:SignalDirection , owl:NamedIndividiual;
        vec:enumLiteral  "In" .

vec:signalSignalInformationType
        rdf:type            owl:ObjectProperty;
        rdfs:comment        "Specifies the information type of the signal.\n"@en;
        rdfs:domain         vec:Signal;
        rdfs:label          "signalInformationType"@en;
        rdfs:range          vec:SignalInformationType;
        rdfs:subPropertyOf  vec:contains .

vec:SiPrefix_Deca  rdf:type  vec:SiPrefix , owl:NamedIndividiual;
        vec:enumLiteral  "Deca" .

vec:topologySegmentAliasId
        rdf:type            owl:ObjectProperty;
        rdfs:comment        "Specifies additional identifiers for the TopologySegment.\nExample: TopologySegment Ids may vary from one CAD system export to another. Therefore, the CAD system Id is improper for identification attribute. The identification shall have a value which is unique within the Topology. AliasId may be used for the CAD system Id.\n"@en;
        rdfs:domain         vec:TopologySegment;
        rdfs:label          "aliasId"@en;
        rdfs:range          vec:AliasIdentification;
        rdfs:subPropertyOf  vec:contains .

vec:documentVersionItemEquivalence
        rdf:type            owl:ObjectProperty;
        rdfs:comment        "Specifies ItemEquivalances defined by the DocumentVersion.\n"@en;
        rdfs:domain         vec:DocumentVersion;
        rdfs:label          "itemEquivalence"@en;
        rdfs:range          vec:ItemEquivalence;
        rdfs:subPropertyOf  vec:contains .

vec:PartStructureContentType_ConfigurableAssembly
        rdf:type         vec:PartStructureContentType , owl:NamedIndividiual;
        rdfs:comment     "Definition of part / component that has variance, that has a bill of material (150%).\n"@en;
        vec:enumLiteral  "ConfigurableAssembly" .

vec:SlotLayoutType_USBTypeB
        rdf:type         vec:SlotLayoutType , owl:NamedIndividiual;
        vec:enumLiteral  "USBTypeB" .

vec:tapeRoleTapingDirection
        rdf:type            owl:ObjectProperty;
        rdfs:comment        "Specifies the direction of the taping.\n"@en;
        rdfs:domain         vec:TapeRole;
        rdfs:label          "tapingDirection"@en;
        rdfs:range          vec:TapingDirection;
        rdfs:subPropertyOf  vec:contains .

vec:RingTerminalSpecification
        rdf:type         owl:Class;
        rdfs:comment     "Specification for the definition of ring terminals. These are the counterparts to bolt terminals.\n"@en;
        rdfs:label       "RingTerminalSpecification"@en;
        rdfs:subClassOf  vec:TerminalSpecification .

vec:pinComponentPinSpecification
        rdf:type      owl:ObjectProperty;
        rdfs:comment  "References the TerminalSpecification describing the electrical connectivity aspect of the PinComponent. \n(see KBLFRM-300)\n"@en;
        rdfs:domain   vec:PinComponent;
        rdfs:label    "pinSpecification"@en;
        rdfs:range    vec:TerminalSpecification .

vec:SiPrefix_Mega  rdf:type  vec:SiPrefix , owl:NamedIndividiual;
        vec:enumLiteral  "Mega" .

vec:iECUnitIecUnitName
        rdf:type            owl:ObjectProperty;
        rdfs:comment        "Specifies the name of the IEC unit.\n"@en;
        rdfs:domain         vec:IECUnit;
        rdfs:label          "iecUnitName"@en;
        rdfs:range          vec:IECUnitName;
        rdfs:subPropertyOf  vec:contains .

vec:WireReception  rdf:type  owl:Class;
        rdfs:comment     "A WireReception is the area of a terminal where the contacting with a wire element (e.g. by crimping) takes place. This class represents such an area on the terminal. Its description is done with a WireReceptionSpecification, which is independent from the TerminalSpecification. This allows the reuse of the specification of similar WireReception on different terminals.\n"@en;
        rdfs:label       "WireReception"@en;
        rdfs:subClassOf  vec:ExtendableElement .

[ rdf:type     owl:AllDisjointClasses;
  owl:members  ( vec:BoltMountedFixingSpecification vec:EdgeMountedFixingSpecification vec:HoleMountedFixingSpecification )
] .

vec:PrimaryPartType_CorrugatedPipe
        rdf:type         vec:PrimaryPartType , owl:NamedIndividiual;
        vec:enumLiteral  "CorrugatedPipe" .

vec:NominalVoltage_HV5
        rdf:type         vec:NominalVoltage , owl:NamedIndividiual;
        rdfs:comment     "HV Class 5 (1200V┬áDC)\n"@en;
        vec:enumLiteral  "HV5" .

vec:defaultDimensionDimensionType
        rdf:type            owl:ObjectProperty;
        rdfs:comment        "The dimensionType defines to which measurements this DefaultDimension applies.\n"@en;
        rdfs:domain         vec:DefaultDimension;
        rdfs:label          "dimensionType"@en;
        rdfs:range          vec:DefaultDimensionType;
        rdfs:subPropertyOf  vec:contains .

vec:relaySpecificationRelaisType
        rdf:type            owl:ObjectProperty;
        rdfs:comment        "The type of the relay (switching behaviour). This is an OpenEnumeration, for values see RelaisType.\n"@en;
        rdfs:domain         vec:RelaySpecification;
        rdfs:label          "relaisType"@en;
        rdfs:range          vec:RelaisType;
        rdfs:subPropertyOf  vec:contains .

vec:cavityPartSpecificationHardness
        rdf:type            owl:ObjectProperty;
        rdfs:comment        "Specifies the hardness of the cavity seal.\n"@en;
        rdfs:domain         vec:CavityPartSpecification;
        rdfs:label          "hardness"@en;
        rdfs:range          vec:NumericalValue;
        rdfs:subPropertyOf  vec:contains .

vec:TransmissionMediumType_Optical
        rdf:type         vec:TransmissionMediumType , owl:NamedIndividiual;
        vec:enumLiteral  "Optical" .

vec:AbstractSlotReference
        rdf:type         owl:Class;
        rdfs:comment     "An AbstractSlotReference represents the usage of an AbstractSlot in the context of PartUsage or PartOccurrence.\n"@en;
        rdfs:label       "AbstractSlotReference"@en;
        rdfs:subClassOf  vec:ExtendableElement .

vec:RelaisApplianceType_Plugged
        rdf:type         vec:RelaisApplianceType , owl:NamedIndividiual;
        vec:enumLiteral  "plugged" .

vec:SlotReference  rdf:type  owl:Class;
        rdfs:comment     "A SlotReference represents the usage of a Slot in the context of PartUsage or PartOccurrence.\n"@en;
        rdfs:label       "SlotReference"@en;
        rdfs:subClassOf  vec:AbstractSlotReference .

vec:PinComponentType_Signal
        rdf:type         vec:PinComponentType , owl:NamedIndividiual;
        vec:enumLiteral  "Signal" .

vec:transformation3DA12
        rdf:type     owl:DatatypeProperty;
        rdfs:domain  vec:Transformation3D;
        rdfs:label   "a12"@en;
        rdfs:range   xs:double .

vec:SlotLayoutType_Type_C
        rdf:type         vec:SlotLayoutType , owl:NamedIndividiual;
        rdfs:comment     "Fuse type according to ISO8820, also known as: ato\n"@en;
        vec:enumLiteral  "Type_C" .

vec:netSpecificationNetworkNode
        rdf:type            owl:ObjectProperty;
        rdfs:comment        "Specifies the NetworkNodes defined in the NetSpecification.\n"@en;
        rdfs:domain         vec:NetSpecification;
        rdfs:label          "networkNode"@en;
        rdfs:range          vec:NetworkNode;
        rdfs:subPropertyOf  vec:contains .

vec:diodeSpecificationAnode
        rdf:type     owl:ObjectProperty;
        rdfs:domain  vec:DiodeSpecification;
        rdfs:label   "anode"@en;
        rdfs:range   vec:PinComponent .

vec:ImperialUnitName_FluidOunce
        rdf:type         vec:ImperialUnitName , owl:NamedIndividiual;
        vec:enumLiteral  "FluidOunce" .

vec:IECPrefix_Pebi  rdf:type  vec:IECPrefix , owl:NamedIndividiual;
        vec:enumLiteral  "Pebi" .

vec:UsageNodeType_CouplingDevice
        rdf:type         vec:UsageNodeType , owl:NamedIndividiual;
        vec:enumLiteral  "CouplingDevice" .

vec:PluggableTerminalType_Standard
        rdf:type         vec:PluggableTerminalType , owl:NamedIndividiual;
        vec:enumLiteral  "Standard" .

vec:placementPointReferencePlacementPoint
        rdf:type      owl:ObjectProperty;
        rdfs:comment  "References the PlacementPoint that is instanced by this PlacementPointReference.\n"@en;
        rdfs:domain   vec:PlacementPointReference;
        rdfs:label    "placementPoint"@en;
        rdfs:range    vec:PlacementPoint .

vec:segmentLengthClassification
        rdf:type            owl:ObjectProperty;
        rdfs:comment        "Specifies the classification of the segment length.\n"@en;
        rdfs:domain         vec:SegmentLength;
        rdfs:label          "classification"@en;
        rdfs:range          vec:LengthClassification;
        rdfs:subPropertyOf  vec:contains .

vec:functionalStructureNodeAbbreviation
        rdf:type            owl:ObjectProperty;
        rdfs:comment        "Room for a human readable short name, title etc. of the FunctionalStructureNode .\n"@en;
        rdfs:domain         vec:FunctionalStructureNode;
        rdfs:label          "abbreviation"@en;
        rdfs:range          vec:LocalizedString;
        rdfs:subPropertyOf  vec:contains .

vec:Mapping  rdf:type    owl:Class;
        rdfs:comment     "The Mapping defines the concrete mapping two parts aliased as A & B. For performance reasons the roles PartSideA and PartSideB are abbreviated to A & B.\n"@en;
        rdfs:label       "Mapping"@en;
        rdfs:subClassOf  vec:ExtendableElement .

vec:SlotCoupling  rdf:type  owl:Class;
        rdfs:comment     "A SlotCoupling defines the mapping between two slots of the ConnectorHousingRoles associated with the CouplingPoint .\n"@en;
        rdfs:label       "SlotCoupling"@en;
        rdfs:subClassOf  vec:ConfigurableElement .

vec:PinVoltageType_InitVoltage
        rdf:type         vec:PinVoltageType , owl:NamedIndividiual;
        vec:enumLiteral  "initVoltage" .

[ rdf:type     owl:AllDisjointClasses;
  owl:members  ( vec:TapeRole )
] .

vec:eEComponentRoleEEComponentSpecification
        rdf:type      owl:ObjectProperty;
        rdfs:comment  "References the EEComponentSpecification that is instanced by this EEComponentRole.\n"@en;
        rdfs:domain   vec:EEComponentRole;
        rdfs:label    "EEComponentSpecification"@en;
        rdfs:range    vec:EEComponentSpecification .

vec:BoltMountedFixingBoltType_MetricThread
        rdf:type         vec:BoltMountedFixingBoltType , owl:NamedIndividiual;
        rdfs:comment     "A bolt with a metric scale thread.\n"@en;
        vec:enumLiteral  "MetricThread" .

vec:terminalSpecificationCurrentInformation
        rdf:type            owl:ObjectProperty;
        rdfs:comment        "Specifies the TerminalCurrentInformation that is applicable for the terminal.\n"@en;
        rdfs:domain         vec:TerminalSpecification;
        rdfs:label          "currentInformation"@en;
        rdfs:range          vec:TerminalCurrentInformation;
        rdfs:subPropertyOf  vec:contains .

vec:transformation3DA33
        rdf:type     owl:DatatypeProperty;
        rdfs:domain  vec:Transformation3D;
        rdfs:label   "a33"@en;
        rdfs:range   xs:double .

vec:VariantGroupType_Family
        rdf:type         vec:VariantGroupType , owl:NamedIndividiual;
        rdfs:comment     "A group with the type \"Family\" defines a set of variant codes that are mutually exclusive, and a valid configuration must contain one variant code from the group.\n"@en;
        vec:enumLiteral  "Family" .

vec:cavitySealSpecificationInsideDiameter
        rdf:type            owl:ObjectProperty;
        rdfs:comment        "Defines the inside diameter in the relaxed state for a cavity seal.\n"@en;
        rdfs:domain         vec:CavitySealSpecification;
        rdfs:label          "insideDiameter"@en;
        rdfs:range          vec:NumericalValue;
        rdfs:subPropertyOf  vec:contains .

vec:cavityReferenceComponentPort
        rdf:type      owl:ObjectProperty;
        rdfs:comment  "References the ComponentPort that is implemented by this CavityReference .\n"@en;
        rdfs:domain   vec:CavityReference;
        rdfs:label    "componentPort"@en;
        rdfs:range    vec:ComponentPort .

vec:terminalPairingSecondTerminal
        rdf:type      owl:ObjectProperty;
        rdfs:comment  "References the second terminal of the TerminalPairing (first and second does not imply any specific order).\n"@en;
        rdfs:domain   vec:TerminalPairing;
        rdfs:label    "secondTerminal"@en;
        rdfs:range    vec:PartVersion .

vec:cavityMountingReplacedPlug
        rdf:type      owl:ObjectProperty;
        rdfs:comment  "References the cavity plugs that are obsolete if the cavity mounting is realized. \n"@en;
        rdfs:domain   vec:CavityMounting;
        rdfs:label    "replacedPlug"@en;
        rdfs:range    vec:CavityPlugRole .

vec:ImperialUnitName_Pound
        rdf:type         vec:ImperialUnitName , owl:NamedIndividiual;
        vec:enumLiteral  "Pound" .

<http://www.prostep.org/ontologies/ecad/2024/03/vec#TerminalBoltNominalSize_%2310>
        rdf:type         vec:TerminalBoltNominalSize , owl:NamedIndividiual;
        vec:enumLiteral  "#10" .

vec:UsageNodeType_Protection
        rdf:type         vec:UsageNodeType , owl:NamedIndividiual;
        vec:enumLiteral  "Protection" .

vec:cavitySpecificationCompatibleTerminalType
        rdf:type            owl:ObjectProperty;
        rdfs:comment        "Defines a list of terminal types that are compatible to this CavitySpecification.\n"@en;
        rdfs:domain         vec:CavitySpecification;
        rdfs:label          "compatibleTerminalType"@en;
        rdfs:range          vec:TerminalType;
        rdfs:subPropertyOf  vec:contains .

vec:itemHistoryEntryType
        rdf:type            owl:ObjectProperty;
        rdfs:comment        "Specifies the type of relationship between the ItemVersions.\n"@en;
        rdfs:domain         vec:ItemHistoryEntry;
        rdfs:label          "type"@en;
        rdfs:range          vec:HistoryEntryType;
        rdfs:subPropertyOf  vec:contains .

vec:nURBSCurveControlPoint
        rdf:type            owl:ObjectProperty;
        rdfs:comment        "Defines the control points of the NURBS curve (for details see the class description of NURBSCurve)\n"@en;
        rdfs:domain         vec:NURBSCurve;
        rdfs:label          "controlPoint"@en;
        rdfs:range          vec:NURBSControlPoint , vec:Ordered;
        rdfs:subPropertyOf  vec:contains .

vec:netGroupIdentification
        rdf:type      owl:DatatypeProperty;
        rdfs:comment  "Specifies a unique identification of the NetGroup. The identification is guaranteed to be unique within the NetSpecification.\n"@en;
        rdfs:domain   vec:NetGroup;
        rdfs:label    "identification"@en;
        rdfs:range    xs:string .

vec:terminalCurrentInformationNominalVoltage
        rdf:type            owl:ObjectProperty;
        rdfs:comment        "Specifies the nominalVoltage for which the CurrentRangeInformation is valid.\n"@en;
        rdfs:domain         vec:TerminalCurrentInformation;
        rdfs:label          "nominalVoltage"@en;
        rdfs:range          vec:NumericalValue;
        rdfs:subPropertyOf  vec:contains .

vec:terminalReceptionReferenceIdentification
        rdf:type      owl:DatatypeProperty;
        rdfs:comment  "Specifies a unique identification of the TerminalReceptionReference . The identification is guaranteed to be unique within the TerminalRole (this might be for example a reception number).\n"@en;
        rdfs:domain   vec:TerminalReceptionReference;
        rdfs:label    "identification"@en;
        rdfs:range    xs:string .

vec:CableTieRole  rdf:type  owl:Class;
        rdfs:comment     "A CableTieRole defines the instance specific properties and relationships of a cable tie.\n"@en;
        rdfs:label       "CableTieRole"@en;
        rdfs:subClassOf  vec:Role .

vec:documentRelatedAssignmentGroupType
        rdf:type            owl:ObjectProperty;
        rdfs:domain         vec:DocumentRelatedAssignmentGroup;
        rdfs:label          "type"@en;
        rdfs:range          vec:DocumentRelationType;
        rdfs:subPropertyOf  vec:contains .

vec:topologySegmentProcessingInstruction
        rdf:type            owl:ObjectProperty;
        rdfs:comment        "Specifies processing instructions for the TopologySegment.\n"@en;
        rdfs:domain         vec:TopologySegment;
        rdfs:label          "processingInstruction"@en;
        rdfs:range          vec:LocalizedString;
        rdfs:subPropertyOf  vec:contains .

vec:shrinkableTubeSpecificationWaterAbsorbtion
        rdf:type            owl:ObjectProperty;
        rdfs:comment        "Defines the water absorption of the shrinkable tube specification.\n"@en;
        rdfs:domain         vec:ShrinkableTubeSpecification;
        rdfs:label          "waterAbsorbtion"@en;
        rdfs:range          vec:NumericalValue;
        rdfs:subPropertyOf  vec:contains .

vec:cavityAvailable  rdf:type  owl:DatatypeProperty;
        rdfs:comment  "Defines whether the cavity is available for contacting. If the cavity is not available, it means that it is completely closed.\n"@en;
        rdfs:domain   vec:Cavity;
        rdfs:label    "available"@en;
        rdfs:range    xs:boolean .

vec:DoubleValueProperty
        rdf:type         owl:Class;
        rdfs:comment     "A custom property with a double value.\n"@en;
        rdfs:label       "DoubleValueProperty"@en;
        rdfs:subClassOf  vec:CustomProperty .

<http://www.prostep.org/ontologies/ecad/2024/03/vec#TerminalBoltNominalSize_1%2F4>
        rdf:type         vec:TerminalBoltNominalSize , owl:NamedIndividiual;
        vec:enumLiteral  "1/4" .

vec:housingComponentReferenceComponentConnector
        rdf:type      owl:ObjectProperty;
        rdfs:comment  "References the ComponentConnector that is realized by the referenced HousingComponentReference."@en;
        rdfs:domain   vec:HousingComponentReference;
        rdfs:label    "componentConnector"@en;
        rdfs:range    vec:ComponentConnector .

vec:CavityGeometry_Square
        rdf:type         vec:CavityGeometry , owl:NamedIndividiual;
        rdfs:comment     ""@en;
        vec:enumLiteral  "Square" .

vec:ConnectorHousingCapSpecification
        rdf:type         owl:Class;
        rdfs:comment     "Specification for the definition of caps (backshells) of connectors. Different caps can add additional wire length addons to a connector housing.\nA 'cap' which already defines the number of cavities, coding etc. is in the┬áVEC┬ádefined by ConnectorHousingSpecification with ModularSlots and not by a ConnectorHousingCapSpecification .\n"@en;
        rdfs:label       "ConnectorHousingCapSpecification"@en;
        rdfs:subClassOf  vec:PartOrUsageRelatedSpecification .

vec:netViewSpecificationPlacedViewItems
        rdf:type            owl:ObjectProperty;
        rdfs:comment        "Specifies all NetworkNodeViewItems that are displayed within a NetViewSpecification ."@en;
        rdfs:domain         vec:NetViewSpecification;
        rdfs:label          "placedViewItems"@en;
        rdfs:range          vec:NetworkNodeViewItem;
        rdfs:subPropertyOf  vec:contains .

vec:terminalPairingSpecificationTerminalPairing
        rdf:type            owl:ObjectProperty;
        rdfs:comment        "Specifies the TerminalPairings described by this TerminalPairingSpecification.\n"@en;
        rdfs:domain         vec:TerminalPairingSpecification;
        rdfs:label          "terminalPairing"@en;
        rdfs:range          vec:TerminalPairing;
        rdfs:subPropertyOf  vec:contains .

vec:SlotLayoutType_Type_SF
        rdf:type         vec:SlotLayoutType , owl:NamedIndividiual;
        rdfs:comment     "Fuse type according to ISO8820, also known as: strip\n"@en;
        vec:enumLiteral  "Type_SF" .

vec:PowerConsumption  rdf:type  owl:Class;
        rdfs:comment  "Defines the power consumption of an EEComponent . An EEComponent can have multiple different PowerConsumptions e.g. standby, maximum. An EEComponent can have multiple PowerConsumptions but must not have more than one PowerConsumptions of the same type .\n"@en;
        rdfs:label    "PowerConsumption"@en .

vec:ColorReferenceSystem_RAL
        rdf:type         vec:ColorReferenceSystem , owl:NamedIndividiual;
        vec:enumLiteral  "RAL" .

vec:NURBSCurve  rdf:type  owl:Class;
        rdfs:comment     "The NURBSCurve represents the parameter set of a NURBS (Non-Uniform rational B-Spline)┬áin the VEC.┬áFor a complete definition of NURBS┬ásee for example ( https://en.wikipedia.org/wiki/Non-uniform_rational_B-spline ).\n┬á\nBasically, a NURBS curve is defined by: a degree a list of control points : with at least degree + 1 points. a weight for each control point. a knots vector: a list of numbers, with ( degree + #controlpoints +1) elements. Every number must be equal or greater than its predecessor, and the same value must not be repeated more than degree times. It seems that modern NURBS algorithms just require ( degree + #controlpoints -1) control points. Commonly used default assignments for the parameters are: weight = 1 for all control points: In this case the curve is called \"non-rational\". knot vector: equidistant and increasing values in the knot vector (e.g. 1,2,3,4,5,6,7) means the curve is \"uniform\"┬áwhich exists in two variants. clamped (or pinned): If the knot vector starts and ends with degree times the same value (e.g. degree = 3, knots = [0,0,0,1,2,3,4,5,5,5], then it is clamped. This has the effect, that the first and last control point coincide with the start and end point of the curve. unclamped (or unpinned): If there are no repeated values in the knot vector (e.g. 1,2,3,4,5,6,7) it is unclamped. The VEC┬á NURBSCurve corresponds to removed BSplineCurve (VEC┬áVersion <= 1.1.3 and KBL). However, the BSplineCurve did not define weight and knot vector, so default assignments where assumed. Existing implementations are using \"uniform non-rational b splines\", unfortunately some implementations use \"uniform clamped\" and some \"unclamped\".\nSince a NURBS cannot be rendered correctly without the knowledge of all parameters and to avoid further misconceptions the VEC allows the definition of all parameters of a NURBS. Furthermore, it requires the specification of all parameters, even if some known default assignment (e.g. non-rational)┬áis used.┬á\n"@en;
        rdfs:label       "NURBSCurve"@en;
        rdfs:subClassOf  vec:Curve3D .

vec:MultiCavityPlugSpecification
        rdf:type         owl:Class;
        rdfs:comment     "Specification for the definition of cavity plugs that apply to more than one cavity. A cavity plug is a watertight non-electrical object to fill an empty cavity. MultiCavityPlugs are formed to fit into one connector / slot and to seal more than one cavity at once. Normally there are different variants of these MultiCavityPlugs that can seal a connector in different pinning scenarios. The cavities that are plugged by a MultiCavityPlug are defined with a SealedCavitiesAssignment.\n"@en;
        rdfs:label       "MultiCavityPlugSpecification"@en;
        rdfs:subClassOf  vec:CavityPlugSpecification .

vec:LanguageCode_Sh  rdf:type  vec:LanguageCode , owl:NamedIndividiual;
        vec:enumLiteral  "Sh" .

vec:BoltMountedFixingBoltType
        rdf:type         owl:Class;
        rdfs:comment     "OpenEnumeration for the types of the bolts on which the fixing can be mounted.\n"@en;
        rdfs:label       "BoltMountedFixingBoltType"@en;
        rdfs:subClassOf  vec:OpenEnumeration .

vec:placementPointIdentification
        rdf:type      owl:DatatypeProperty;
        rdfs:comment  "Specifies a unique identification of the PlacementPoint. The identification is guaranteed to be unique within a component.\n"@en;
        rdfs:domain   vec:PlacementPoint;
        rdfs:label    "identification"@en;
        rdfs:range    xs:string .

vec:SlotLayoutType_RS-453
        rdf:type         vec:SlotLayoutType , owl:NamedIndividiual;
        rdfs:comment     "IEC 60603-11"@en;
        vec:enumLiteral  "RS-453" .

vec:ImperialUnitName_League
        rdf:type         vec:ImperialUnitName , owl:NamedIndividiual;
        vec:enumLiteral  "League" .

vec:SlotLayoutType  rdf:type  owl:Class;
        rdfs:comment     "OpenEnumeration that defines standard slot layouts. A slot layout represents the mechanical /┬ágeometrical properties /┬álayout of the slot, not the electrical properties.\n"@en;
        rdfs:label       "SlotLayoutType"@en;
        rdfs:subClassOf  vec:OpenEnumeration .

vec:defaultDimensionToleranceIndication
        rdf:type            owl:ObjectProperty;
        rdfs:domain         vec:DefaultDimension;
        rdfs:label          "toleranceIndication"@en;
        rdfs:range          vec:Tolerance;
        rdfs:subPropertyOf  vec:contains .

vec:variantConfigurationConfigurationType
        rdf:type            owl:ObjectProperty;
        rdfs:comment        "Allows the classification of a VariantConfiguration.\n(see KBLFRM-250, KBLFRM-314, KBLFRM-290)\n"@en;
        rdfs:domain         vec:VariantConfiguration;
        rdfs:label          "configurationType"@en;
        rdfs:range          vec:VariantConfigurationType;
        rdfs:subPropertyOf  vec:contains .

vec:LengthClassification_Adapted
        rdf:type         vec:LengthClassification , owl:NamedIndividiual;
        rdfs:comment     "An adapted length means that the value is not the exact value taken from the CAD tool but is adapted in some way. Adapted values are supposed for further use in the process, especially as basis for the product specification. Adapted values are normally created for example by rounding the designed values.\n"@en;
        vec:enumLiteral  "Adapted" .

vec:FittingForm_M  rdf:type  vec:FittingForm , owl:NamedIndividiual;
        rdfs:comment     "A┬á\"wye\" with more than 2 outlets (one inlet).\n"@en;
        vec:enumLiteral  "M" .

vec:networkNodeRealizedUsageNode
        rdf:type      owl:ObjectProperty;
        rdfs:comment  "References the UsageNode that is realized by this NetworkNode .\n"@en;
        rdfs:domain   vec:NetworkNode;
        rdfs:label    "realizedUsageNode"@en;
        rdfs:range    vec:UsageNode .

vec:terminalSpecificationTerminalReception
        rdf:type            owl:ObjectProperty;
        rdfs:comment        "Specifies the TerminalReceptions of the terminal described by the TerminalSpecification.\n"@en;
        rdfs:domain         vec:TerminalSpecification;
        rdfs:label          "terminalReception"@en;
        rdfs:range          vec:TerminalReception;
        rdfs:subPropertyOf  vec:contains .

vec:TypeOfPermission  rdf:type  owl:Class;
        rdfs:comment     "Enumeration for the definition of the type of a permission.\n"@en;
        rdfs:label       "TypeOfPermission"@en;
        rdfs:subClassOf  vec:OpenEnumeration .

vec:LanguageCode_Gl  rdf:type  vec:LanguageCode , owl:NamedIndividiual;
        vec:enumLiteral  "Gl" .

vec:FuseComponent  rdf:type  owl:Class;
        rdfs:label  "FuseComponent"@en .

vec:approvalAdditionalLevelInformation
        rdf:type      owl:DatatypeProperty;
        rdfs:comment  "Additional potentially company specific information about the level of approval (e.g. further detailing of a \"Restricted\" approval.\n"@en;
        rdfs:domain   vec:Approval;
        rdfs:label    "additionalLevelInformation"@en;
        rdfs:range    xs:string .

vec:ConnectionGroupType_Coaxial
        rdf:type         vec:ConnectionGroupType , owl:NamedIndividiual;
        vec:enumLiteral  "Coaxial" .

vec:pinCurrentInformationTiming
        rdf:type            owl:ObjectProperty;
        rdfs:comment        "Specifies the timing of the PinCurrentInformation.\n"@en;
        rdfs:domain         vec:PinCurrentInformation;
        rdfs:label          "timing"@en;
        rdfs:range          vec:PinTiming;
        rdfs:subPropertyOf  vec:contains .

vec:WindingType_OnSpace
        rdf:type         vec:WindingType , owl:NamedIndividiual;
        rdfs:comment     " OnSpace describes a taping with gaps between the rounds (German: Luecke)\n"@en;
        vec:enumLiteral  "OnSpace" .

vec:conductorSpecificationMaterial
        rdf:type            owl:ObjectProperty;
        rdfs:comment        "Specifies the material of the conductor.\n"@en;
        rdfs:domain         vec:ConductorSpecification;
        rdfs:label          "material"@en;
        rdfs:range          vec:Material;
        rdfs:subPropertyOf  vec:contains .

vec:netSpecificationNetGroup
        rdf:type            owl:ObjectProperty;
        rdfs:comment        "Specifies the NetGroup defined in the NetSpecification.\n"@en;
        rdfs:domain         vec:NetSpecification;
        rdfs:label          "netGroup"@en;
        rdfs:range          vec:NetGroup;
        rdfs:subPropertyOf  vec:contains .

vec:wireGroupSpecificationGroupType
        rdf:type            owl:ObjectProperty;
        rdfs:comment        "Specifies the type of the group (e.g. twisted pair, ...).\n"@en;
        rdfs:domain         vec:WireGroupSpecification;
        rdfs:label          "groupType"@en;
        rdfs:range          vec:WireGroupType;
        rdfs:subPropertyOf  vec:contains .

<http://www.prostep.org/ontologies/ecad/2024/03/vec#TerminalBoltNominalSize_5%2F16>
        rdf:type         vec:TerminalBoltNominalSize , owl:NamedIndividiual;
        vec:enumLiteral  "5/16" .

vec:ImperialUnitName_Foot
        rdf:type         vec:ImperialUnitName , owl:NamedIndividiual;
        vec:enumLiteral  "Foot" .

vec:OnWayPlacement  rdf:type  owl:Class;
        rdfs:comment     "An OnWayPlacement places an OccurrenceOrUsage onto an area of the Topology (e.g. a tape or a tube). The area is defined by a startLocation and an endLocation. If startLocation and endLocation are not located on the same TopologySegment it is possible to specify a Path of TopologySegments over which the OnWayPlacement goes.\nThe names start- and endLocation are used to distinguish between the two ends. It does not indicate a direction as property of the product (e.g. for tapes).\n"@en;
        rdfs:label       "OnWayPlacement"@en;
        rdfs:subClassOf  vec:Placement .

vec:CableLeadThroughGeometry_Oval
        rdf:type         vec:CableLeadThroughGeometry , owl:NamedIndividiual;
        vec:enumLiteral  "Oval" .

vec:WireEndAccessoryRole
        rdf:type         owl:Class;
        rdfs:comment     "A WireEndAccessoryRole defines the instance specific properties and relationships of a WireEndAccessory .\n"@en;
        rdfs:label       "WireEndAccessoryRole"@en;
        rdfs:subClassOf  vec:Role .

vec:USUnitName_Yard  rdf:type  vec:USUnitName , owl:NamedIndividiual;
        vec:enumLiteral  "Yard" .

vec:cavityPositionDetail
        rdf:type            owl:ObjectProperty;
        rdfs:comment        "Optional details for geometric properties of the cavity in the connector."@en;
        rdfs:domain         vec:Cavity;
        rdfs:label          "positionDetail"@en;
        rdfs:range          vec:CavityPositionDetail;
        rdfs:subPropertyOf  vec:contains .

vec:ComponentPortViewItemSide_Left
        rdf:type         vec:ComponentPortViewItemSide , owl:NamedIndividiual;
        vec:enumLiteral  "Left" .

vec:signalClampName  rdf:type  owl:DatatypeProperty;
        rdfs:comment  "Specifies the name of the clamp e.g. KL15, KL30, KL31.\n"@en;
        rdfs:domain   vec:Signal;
        rdfs:label    "clampName"@en;
        rdfs:range    xs:string .

vec:LanguageCode_Co  rdf:type  vec:LanguageCode , owl:NamedIndividiual;
        vec:enumLiteral  "Co" .

vec:connectionNodeViewItemDisplayedPort
        rdf:type            owl:ObjectProperty;
        rdfs:comment        "Specifies all ComponentPortViewItems that are displayed on this ComponentNodeViewItem . The order of this association defines the clockwise arrangement of the ports on the node. As each ComponentPortViewItem can also define the side on which it is placed, side definitions take precedence over order. ┬á Caution: This association is ordered ! ┬á\n"@en;
        rdfs:domain         vec:ConnectionNodeViewItem;
        rdfs:label          "displayedPort"@en;
        rdfs:range          vec:ComponentPortViewItem , vec:Ordered;
        rdfs:subPropertyOf  vec:contains .

vec:conductorSpecificationVoltageRange
        rdf:type            owl:ObjectProperty;
        rdfs:comment        "Specifies the voltageRange for which the conductor is approved.\n"@en;
        rdfs:domain         vec:ConductorSpecification;
        rdfs:label          "voltageRange"@en;
        rdfs:range          vec:NumericalValue;
        rdfs:subPropertyOf  vec:contains .

vec:ApplicationConstraintType_Deny
        rdf:type         vec:ApplicationConstraintType , owl:NamedIndividiual;
        vec:enumLiteral  "Deny" .

vec:SegmentLocation  rdf:type  owl:Class;
        rdfs:comment     "Specifies a point on a TopologySegment as a Location.\n"@en;
        rdfs:label       "SegmentLocation"@en;
        rdfs:subClassOf  vec:Location .

vec:extendableElementCustomProperty
        rdf:type            owl:ObjectProperty;
        rdfs:comment        "Specifies the CustomProperties of the ExtendableElement. \n"@en;
        rdfs:domain         vec:ExtendableElement;
        rdfs:label          "customProperty"@en;
        rdfs:range          vec:CustomProperty;
        rdfs:subPropertyOf  vec:contains .

vec:tubeSpecificationBendRadius
        rdf:type            owl:ObjectProperty;
        rdfs:comment        "Specifies the bend radius of the tube.\n"@en;
        rdfs:domain         vec:TubeSpecification;
        rdfs:label          "bendRadius"@en;
        rdfs:range          vec:NumericalValue;
        rdfs:subPropertyOf  vec:contains .

vec:IECUnitName  rdf:type    owl:Class;
        rdfs:comment         "Enumeration for the definition of IEC unit names.\n"@en;
        rdfs:label           "IECUnitName"@en;
        rdfs:subClassOf      vec:ClosedEnumeration;
        owl:equivalentClass  [ rdf:type   owl:Class;
                               owl:oneOf  ( vec:IECUnitName_Bit vec:IECUnitName_Byte )
                             ] .

vec:LanguageCode_Kn  rdf:type  vec:LanguageCode , owl:NamedIndividiual;
        vec:enumLiteral  "Kn" .

vec:harnessGeometrySpecification3DType
        rdf:type            owl:ObjectProperty;
        rdfs:comment        "Specifies the type of the harness geometry.\n"@en;
        rdfs:domain         vec:HarnessGeometrySpecification3D;
        rdfs:label          "type"@en;
        rdfs:range          vec:GeometryType;
        rdfs:subPropertyOf  vec:contains .

vec:terminalPairingContactResistance
        rdf:type            owl:ObjectProperty;
        rdfs:comment        "Specifies the resistance of the terminal pairing."@en;
        rdfs:domain         vec:TerminalPairing;
        rdfs:label          "contactResistance"@en;
        rdfs:range          vec:NumericalValue;
        rdfs:subPropertyOf  vec:contains .

vec:wireGroupingConnectionGroup
        rdf:type      owl:ObjectProperty;
        rdfs:comment  "References the ConnectionGroup that is realized by this WireGrouping.\n"@en;
        rdfs:domain   vec:WireGrouping;
        rdfs:label    "connectionGroup"@en;
        rdfs:range    vec:ConnectionGroup .

vec:LanguageCode_Sm  rdf:type  vec:LanguageCode , owl:NamedIndividiual;
        vec:enumLiteral  "Sm" .

vec:LabelingSpecification
        rdf:type         owl:Class;
        rdfs:comment     "A component (of any type) can labeled in many ways either during the manufacturing process, for example a label that is imprinted on the component during the general manufacturing process┬á(e.g. the part number), or in its concrete use (e.g. with wire number or a usage node id). The LabelingSpecification defines general labeling properties of the component. Labeling properties in its concrete use are defined with the correspoding role."@en;
        rdfs:label       "LabelingSpecification"@en;
        rdfs:subClassOf  vec:PartOrUsageRelatedSpecification .

vec:cavityAddOnType  rdf:type  owl:ObjectProperty;
        rdfs:comment        "Defines the type of the add-on (see CavityAddOn ).\n"@en;
        rdfs:domain         vec:CavityAddOn;
        rdfs:label          "type"@en;
        rdfs:range          vec:WireAddOnType;
        rdfs:subPropertyOf  vec:contains .

vec:pinOpticalInformationAttenuation
        rdf:type            owl:ObjectProperty;
        rdfs:comment        "The attenuation of the optical pin at the defined frequency.\n"@en;
        rdfs:domain         vec:PinOpticalInformation;
        rdfs:label          "attenuation"@en;
        rdfs:range          vec:NumericalValue;
        rdfs:subPropertyOf  vec:contains .

vec:AssignmentGroup  rdf:type  owl:Class;
        rdfs:comment     "An AssignmentGroup is a concept that allows the clustering of arbitrary elements in ways that are orthogonal to hierarchical and semantic structure of the VEC.\n"@en;
        rdfs:label       "AssignmentGroup"@en;
        rdfs:subClassOf  vec:ExtendableElement .

vec:requirementsConformanceStatementDescription
        rdf:type            owl:ObjectProperty;
        rdfs:comment        "A free text description / additional information /┬ácomment for the RequirementsConformanceStatement.\n"@en;
        rdfs:domain         vec:RequirementsConformanceStatement;
        rdfs:label          "description"@en;
        rdfs:range          vec:LocalizedString;
        rdfs:subPropertyOf  vec:contains .

vec:ImperialUnitName_HundredWeight
        rdf:type         vec:ImperialUnitName , owl:NamedIndividiual;
        vec:enumLiteral  "HundredWeight" .

vec:terminalPairingReferencedCoreSpecification
        rdf:type      owl:ObjectProperty;
        rdfs:comment  "References the CoreSpecification that is used on both sides of the ContactSystem.\n"@en;
        rdfs:domain   vec:TerminalPairing;
        rdfs:label    "referencedCoreSpecification"@en;
        rdfs:range    vec:ConductorSpecification .

vec:internalComponentConnectionIdentification
        rdf:type      owl:DatatypeProperty;
        rdfs:comment  "Identification of the InternalComponentConnection , which must be distinct for all InternalComponentConnection of an EEComponent .\n"@en;
        rdfs:domain   vec:InternalComponentConnection;
        rdfs:label    "identification"@en;
        rdfs:range    xs:string .

vec:PartStructureContentType_Variant
        rdf:type         vec:PartStructureContentType , owl:NamedIndividiual;
        rdfs:comment     "A concrete variant of a harness (100%)."@en;
        vec:enumLiteral  "Variant" .

vec:wireTupleSpecificationFixationAccessory
        rdf:type            owl:ObjectProperty;
        rdfs:comment        "Specifies PartRelations that can / have to be used for the fixation."@en;
        rdfs:domain         vec:WireTupleSpecification;
        rdfs:label          "fixationAccessory"@en;
        rdfs:range          vec:PartRelation;
        rdfs:subPropertyOf  vec:contains .

vec:LanguageCode_Mo  rdf:type  vec:LanguageCode , owl:NamedIndividiual;
        vec:enumLiteral  "Mo" .

vec:cavitySpecificationCavityDimension
        rdf:type            owl:ObjectProperty;
        rdfs:comment        "Specifies the dimension of the cavity in the sealing area of the cavity (crimp end), not in the contacting area (box end).\nThe Height of a cavity is defined as the dimension of cavity in the direction of the primary locking. The Width is the dimension orthogonal to the Height.\nFor cavities with Geometry = Circular the Size.Width shall be equal to Size.Height.\n"@en;
        rdfs:domain         vec:CavitySpecification;
        rdfs:label          "cavityDimension"@en;
        rdfs:range          vec:Size;
        rdfs:subPropertyOf  vec:contains .

vec:NetworkPortViewItemSide_Bottom
        rdf:type         vec:NetworkPortViewItemSide , owl:NamedIndividiual;
        vec:enumLiteral  "Bottom" .

vec:stripeSpecificationThickness
        rdf:type            owl:ObjectProperty;
        rdfs:comment        "Specifies the thickness of the stripe (adhesive + backing).\n"@en;
        rdfs:domain         vec:StripeSpecification;
        rdfs:label          "thickness"@en;
        rdfs:range          vec:NumericalValue;
        rdfs:subPropertyOf  vec:contains .

vec:DocumentType_NetworkSymbol
        rdf:type         vec:DocumentType , owl:NamedIndividiual;
        rdfs:comment     "Documents of this type represent a graphical symbol (2D), which is normally an external file (e.g. an SVG, PNG). The use case for this document type are symbols that are used in network /┬áarchitecture diagrams.\n"@en;
        vec:enumLiteral  "NetworkSymbol" .

vec:ModuleListSpecification
        rdf:type         owl:Class;
        rdfs:comment     "Specification for the description of module lists (see ModuleList).\n"@en;
        rdfs:label       "ModuleListSpecification"@en;
        rdfs:subClassOf  vec:Specification .

vec:cavityCavityNumber
        rdf:type      owl:DatatypeProperty;
        rdfs:comment  "Provides an identifier for the cavity. The cavity number needs to be unique within a Slot .\n"@en;
        rdfs:domain   vec:Cavity;
        rdfs:label    "cavityNumber"@en;
        rdfs:range    xs:string .

vec:signalSignalTransmissionMediumType
        rdf:type            owl:ObjectProperty;
        rdfs:comment        "Specifies the type of the transmission medium for the signal.\n"@en;
        rdfs:domain         vec:Signal;
        rdfs:label          "signalTransmissionMediumType"@en;
        rdfs:range          vec:SignalTransmissionMediumType;
        rdfs:subPropertyOf  vec:contains .

vec:connectorHousingCapRoleConnectorHousingCapSpecification
        rdf:type      owl:ObjectProperty;
        rdfs:comment  "References the ConnectorHousingCapSpecification that is instanced by this ConnectorHousingCapRole.\n"@en;
        rdfs:domain   vec:ConnectorHousingCapRole;
        rdfs:label    "connectorHousingCapSpecification"@en;
        rdfs:range    vec:ConnectorHousingCapSpecification .

vec:fixingSpecificationNominalSize
        rdf:type            owl:ObjectProperty;
        rdfs:domain         vec:FixingSpecification;
        rdfs:label          "nominalSize"@en;
        rdfs:range          vec:NumericalValue;
        rdfs:subPropertyOf  vec:contains .

vec:materialReferenceSystem
        rdf:type      owl:DatatypeProperty;
        rdfs:comment  "The identification of the material reference system, which is defining possible values and the semantic of material keys.\n"@en;
        rdfs:domain   vec:Material;
        rdfs:label    "referenceSystem"@en;
        rdfs:range    xs:string .

vec:projectCarClassificationLevel2
        rdf:type      owl:DatatypeProperty;
        rdfs:comment  "Provides a classification according to \"CC8 Recommended Practices Specification and Configuration, Product Structures\". Car classification is the identification of a set of similar cars to be offered to the market. Level 2 stands for \"Technical information / platform\" and reflects the level of a product class in a BoM system which represents a main technical product base (e.g. project, platform, engineering series etc.). In some cases, this level carries a complete BoM (\"Maximum BoM\") for a project, platform, engineering series etc. This level is in some cases called technical documentation.\n"@en;
        rdfs:domain   vec:Project;
        rdfs:label    "carClassificationLevel2"@en;
        rdfs:range    xs:string .

vec:SignalType_Information
        rdf:type         vec:SignalType , owl:NamedIndividiual;
        vec:enumLiteral  "information" .

vec:LanguageCode_As  rdf:type  vec:LanguageCode , owl:NamedIndividiual;
        vec:enumLiteral  "As" .

vec:LanguageCode_Wo  rdf:type  vec:LanguageCode , owl:NamedIndividiual;
        vec:enumLiteral  "Wo" .

vec:Coding  rdf:type     owl:Class;
        rdfs:comment     "Specifies the coding of a slot or a connector housing.\n"@en;
        rdfs:label       "Coding"@en;
        rdfs:subClassOf  vec:ExtendableElement .

vec:slotSpecificationEmvProtectionRequired
        rdf:type      owl:DatatypeProperty;
        rdfs:comment  "Specifies whether the slot needs EMV protection.\n"@en;
        rdfs:domain   vec:SlotSpecification;
        rdfs:label    "emvProtectionRequired"@en;
        rdfs:range    xs:boolean .

vec:boltTerminalSpecificationTorsionProtection
        rdf:type      owl:DatatypeProperty;
        rdfs:comment  "Specifies if the bolt provides torsion protected or not.\n"@en;
        rdfs:domain   vec:BoltTerminalSpecification;
        rdfs:label    "torsionProtection"@en;
        rdfs:range    xs:boolean .

vec:SiUnitName_Siemens
        rdf:type         vec:SiUnitName , owl:NamedIndividiual;
        vec:enumLiteral  "Siemens" .

vec:CableLeadThroughType
        rdf:type         owl:Class;
        rdfs:comment     "Defines valid types for CableLeadThroughs.\n"@en;
        rdfs:label       "CableLeadThroughType"@en;
        rdfs:subClassOf  vec:OpenEnumeration .

vec:FixingSpecification
        rdf:type         owl:Class;
        rdfs:comment     "Specification for the definition of fixings. A fixing is used to fix the harness in a certain position (e.g. at the car body, a seat, an ECU etc.). The FixingSpecification describes how the fixing is attached to the \"non-harness\" element. The attachment to harness is described by a PlaceableElementSpecification.\n"@en;
        rdfs:label       "FixingSpecification"@en;
        rdfs:subClassOf  vec:PartOrUsageRelatedSpecification .

vec:ComponentNodeType_Relay
        rdf:type         vec:ComponentNodeType , owl:NamedIndividiual;
        rdfs:comment     " Deprecated since VEC V1.2. Use instead ComponentSubType Relay.┬á\n"@en;
        vec:enumLiteral  "Relay" .

vec:TubeSlitStyle_SelfClosing
        rdf:type         vec:TubeSlitStyle , owl:NamedIndividiual;
        rdfs:comment     "The slit of the tube is self-closing.\n"@en;
        vec:enumLiteral  "SelfClosing" .

vec:PrimaryPartType_Terminal
        rdf:type         vec:PrimaryPartType , owl:NamedIndividiual;
        vec:enumLiteral  "Terminal" .

vec:ComponentNodeType_OpenLink
        rdf:type         vec:ComponentNodeType , owl:NamedIndividiual;
        rdfs:comment     "Defines that this ComponentNode is an OpenLink. In the description of partial systems, it can be necessary to reference a ComponentNode that is not defined in the scope of the partial system (e.g. vehicle infrastructure like power, ground, bus systems). OpenLinks must be resolved and replaced by a determined ComponentNode when a partial system is integrated into a vehicle system.\n"@en;
        vec:enumLiteral  "OpenLink" .

vec:PinVoltageType_OverrunVoltage
        rdf:type         vec:PinVoltageType , owl:NamedIndividiual;
        vec:enumLiteral  "overrunVoltage" .

vec:CouplingPoint  rdf:type  owl:Class;
        rdfs:comment     "A CouplingPoint defines a single coupling. If a coupling takes place, all sub elements are connected. If the coupling is disconnected, all subelements are disconnected.\nIf a coupling occurs between two connectors, and not just between two terminals, the CouplingPoint references the respective ConnectorHousingRoles .\n"@en;
        rdfs:label       "CouplingPoint"@en;
        rdfs:subClassOf  vec:ConfigurableElement .

vec:itemEquivalenceCompanyName
        rdf:type      owl:DatatypeProperty;
        rdfs:comment  "Specifies the company which states the ItemEquivalence.\n"@en;
        rdfs:domain   vec:ItemEquivalence;
        rdfs:label    "companyName"@en;
        rdfs:range    xs:string .

vec:DocumentType_NetworkArchitecture
        rdf:type         vec:DocumentType , owl:NamedIndividiual;
        rdfs:comment     ""@en;
        vec:enumLiteral  "NetworkArchitecture" .

vec:usageConstraintProjectPhase
        rdf:type      owl:DatatypeProperty;
        rdfs:comment  "Specifies the project phases to which the usage constraint applies.\n"@en;
        rdfs:domain   vec:UsageConstraint;
        rdfs:label    "projectPhase"@en;
        rdfs:range    xs:string .

vec:BooleanValueProperty
        rdf:type         owl:Class;
        rdfs:comment     "A custom property with a boolean value.\n"@en;
        rdfs:label       "BooleanValueProperty"@en;
        rdfs:subClassOf  vec:CustomProperty .

vec:LanguageCode_Ks  rdf:type  vec:LanguageCode , owl:NamedIndividiual;
        vec:enumLiteral  "Ks" .

vec:housingComponentDescription
        rdf:type            owl:ObjectProperty;
        rdfs:comment        "Specifies additional, human readable information about the HousingComponent .\n"@en;
        rdfs:domain         vec:HousingComponent;
        rdfs:label          "description"@en;
        rdfs:range          vec:AbstractLocalizedString;
        rdfs:subPropertyOf  vec:contains .

vec:matingPointSecondTerminalRole
        rdf:type      owl:ObjectProperty;
        rdfs:comment  "References the second terminal that is mated.\n"@en;
        rdfs:domain   vec:MatingPoint;
        rdfs:label    "secondTerminalRole"@en;
        rdfs:range    vec:TerminalRole .

vec:componentPortViewItemComponentPort
        rdf:type      owl:ObjectProperty;
        rdfs:comment  "References the ComponentPort that is represented by this ComponentPortViewItem . "@en;
        rdfs:domain   vec:ComponentPortViewItem;
        rdfs:label    "componentPort"@en;
        rdfs:range    vec:ComponentPort .

vec:cavityPositionDetailInsertionVector
        rdf:type            owl:ObjectProperty;
        rdfs:comment        "The direction in which a terminal is inserted from the InsertionPosition into the connector. The amount of the vector defines the length auf the cavity┬á(The distance the terminal must travel from the InsertionPostion to its final position."@en;
        rdfs:domain         vec:CavityPositionDetail;
        rdfs:label          "insertionVector"@en;
        rdfs:range          vec:CartesianVector3D;
        rdfs:subPropertyOf  vec:contains .

vec:LanguageCode_Sr  rdf:type  vec:LanguageCode , owl:NamedIndividiual;
        vec:enumLiteral  "Sr" .

vec:topologyNodeNodeType
        rdf:type            owl:ObjectProperty;
        rdfs:comment        "Specifies the type of the TopologyNode. A Node can either be an EndNode, a Junction or an Inliner.\n"@en;
        rdfs:domain         vec:TopologyNode;
        rdfs:label          "nodeType"@en;
        rdfs:range          vec:NodeType;
        rdfs:subPropertyOf  vec:contains .

vec:ConductorType  rdf:type  owl:Class;
        rdfs:comment     "Specifies the type of the conductor, e.g. if it is rigid or stranded.\n"@en;
        rdfs:label       "ConductorType"@en;
        rdfs:subClassOf  vec:OpenEnumeration .

vec:applicationConstraintType
        rdf:type            owl:ObjectProperty;
        rdfs:comment        "Defines if the application constraint is positive (allowance) or negative (denial). If the ApplicationConstraint has a baseInclusion that baseInclusion shall define the same type.\n"@en;
        rdfs:domain         vec:ApplicationConstraint;
        rdfs:label          "type"@en;
        rdfs:range          vec:ApplicationConstraintType;
        rdfs:subPropertyOf  vec:contains .

vec:itemVersionCreation
        rdf:type            owl:ObjectProperty;
        rdfs:comment        "Specifies the information about the creation of the ItemVersion. \n"@en;
        rdfs:domain         vec:ItemVersion;
        rdfs:label          "creation"@en;
        rdfs:range          vec:Creation;
        rdfs:subPropertyOf  vec:contains .

vec:LanguageCode_Eu  rdf:type  vec:LanguageCode , owl:NamedIndividiual;
        vec:enumLiteral  "Eu" .

vec:CableDuctOutlet  rdf:type  owl:Class;
        rdfs:comment     "Specifies one outlet of the cable duct.\n"@en;
        rdfs:label       "CableDuctOutlet"@en;
        rdfs:subClassOf  vec:ExtendableElement .

vec:HousingComponent  rdf:type  owl:Class;
        rdfs:comment     "A HousingComponent describes the interface of an EEComponent with which it can be connected to another EEComponent or a harness. The characteristics of the interface can be described with a referenced ConnectorHousingSpecification. (see KBLFRM-300)\n"@en;
        rdfs:label       "HousingComponent"@en;
        rdfs:subClassOf  vec:ConfigurableElement .

vec:networkNodeIdentification
        rdf:type      owl:DatatypeProperty;
        rdfs:comment  "Specifies a unique identification of the NetworkNode. The identification is guaranteed to be unique within the NetSpecification.\n"@en;
        rdfs:domain   vec:NetworkNode;
        rdfs:label    "identification"@en;
        rdfs:range    xs:string .

vec:SignalTransmissionMediumType_Hydraulic
        rdf:type         vec:SignalTransmissionMediumType , owl:NamedIndividiual;
        vec:enumLiteral  "hydraulic" .

vec:SiPrefix_Yocto  rdf:type  vec:SiPrefix , owl:NamedIndividiual;
        vec:enumLiteral  "Yocto" .

vec:LanguageCode_Mt  rdf:type  vec:LanguageCode , owl:NamedIndividiual;
        vec:enumLiteral  "Mt" .

vec:connectorHousingSpecificationOutletDirection
        rdf:type            owl:ObjectProperty;
        rdfs:comment        "Defines the OutletDirection for wires.\nThis attribute is defined as an OpenEnumeration .\n"@en;
        rdfs:domain         vec:ConnectorHousingSpecification;
        rdfs:label          "outletDirection"@en;
        rdfs:range          vec:ConnectorOutletDirection;
        rdfs:subPropertyOf  vec:contains .

vec:terminalReceptionGender
        rdf:type      owl:DatatypeProperty;
        rdfs:comment  "Specifies the gender of the TerminalReception. The gender is included in the TerminalReception class in order to be able to refer the same TerminalReceptionSpecification gender independent.\n"@en;
        rdfs:domain   vec:TerminalReception;
        rdfs:label    "gender"@en;
        rdfs:range    xs:string .

vec:wireElementSpecificationMinBendRadiusDynamic
        rdf:type            owl:ObjectProperty;
        rdfs:comment        "Specifies the minimum bend radius for wire element, if it is used in a dynamic environment, where it is bended repeatedly (e.g. in grommet of the back door). (see KLBFRM-311)\n"@en;
        rdfs:domain         vec:WireElementSpecification;
        rdfs:label          "minBendRadiusDynamic"@en;
        rdfs:range          vec:NumericalValue;
        rdfs:subPropertyOf  vec:contains .

vec:connectionGroupSubGroup
        rdf:type            owl:ObjectProperty;
        rdfs:comment        "Specifies the ConnectionGroups that are a subgroup of this ConnectionGroup.\n"@en;
        rdfs:domain         vec:ConnectionGroup;
        rdfs:label          "subGroup"@en;
        rdfs:range          vec:ConnectionGroup;
        rdfs:subPropertyOf  vec:contains .

vec:grommetSpecificationPlateThickness
        rdf:type            owl:ObjectProperty;
        rdfs:comment        "Specifies valid the plate thickness at the hole into which the grommet fits.\n"@en;
        rdfs:domain         vec:GrommetSpecification;
        rdfs:label          "plateThickness"@en;
        rdfs:range          vec:ValueRange;
        rdfs:subPropertyOf  vec:contains .

vec:PartWithSubComponentsRole
        rdf:type         owl:Class;
        rdfs:comment     "A PartWithSubComponentsRole defines the instance specific properties and relationships of a part with subcomponents. A PartWithSubComponents is a composite part like an Assembly, a Module, Harness.\n"@en;
        rdfs:label       "PartWithSubComponentsRole"@en;
        rdfs:subClassOf  vec:Role .

vec:VariantConfiguration
        rdf:type         owl:Class;
        rdfs:comment     "A variant configuration defines a condition with which it is possible to express the inclusion or exclusion of ConfigurableElements in different variants of a product.\nA VariantConfiguration can reference another VariantConfiguration as baseInclusion . In this case, a VariantConfiguration can only be satisfied if its baseInclusion is also satisfied.\n"@en;
        rdfs:label       "VariantConfiguration"@en;
        rdfs:subClassOf  vec:ExtendableElement .

vec:SignalForm  rdf:type  owl:Class;
        rdfs:label       "SignalForm"@en;
        rdfs:subClassOf  vec:OpenEnumeration .

vec:holeMountedFixingSpecificationHoleDiameter
        rdf:type            owl:ObjectProperty;
        rdfs:comment        "Specifies the diameter of the hole in which the fixing is mounted.\n"@en;
        rdfs:domain         vec:HoleMountedFixingSpecification;
        rdfs:label          "holeDiameter"@en;
        rdfs:range          vec:NumericalValue;
        rdfs:subPropertyOf  vec:contains .

vec:VecVersion  rdf:type     owl:Class;
        rdfs:label           "VecVersion"@en;
        rdfs:subClassOf      vec:ClosedEnumeration;
        owl:equivalentClass  [ rdf:type   owl:Class;
                               owl:oneOf  ( vec:VecVersion_1.1.1 vec:VecVersion_1.1.2 vec:VecVersion_1.1.3 vec:VecVersion_1.2.0 vec:VecVersion_1.2.1 vec:VecVersion_1.2.2 vec:VecVersion_2.0.0 )
                             ] .

vec:wireGroupSpecificationLengthOfTwist
        rdf:type            owl:ObjectProperty;
        rdfs:comment        "Specifies the length of twist if the wire group is representing a twisted pair.\n"@en;
        rdfs:domain         vec:WireGroupSpecification;
        rdfs:label          "lengthOfTwist"@en;
        rdfs:range          vec:NumericalValue;
        rdfs:subPropertyOf  vec:contains .

vec:TypeOfPermission_Released
        rdf:type         vec:TypeOfPermission , owl:NamedIndividiual;
        vec:enumLiteral  "Released" .

vec:terminalPairingMatingForce
        rdf:type            owl:ObjectProperty;
        rdfs:comment        "Specifies the joining force of the two terminals.\n"@en;
        rdfs:domain         vec:TerminalPairing;
        rdfs:label          "matingForce"@en;
        rdfs:range          vec:NumericalValue;
        rdfs:subPropertyOf  vec:contains .

vec:networkPortViewItemSide
        rdf:type            owl:ObjectProperty;
        rdfs:comment        "Specifies the side of the NetworkNodeViewItem on which the port should be displayed."@en;
        rdfs:domain         vec:NetworkPortViewItem;
        rdfs:label          "side"@en;
        rdfs:range          vec:NetworkPortViewItemSide;
        rdfs:subPropertyOf  vec:contains .

vec:toleranceUpperBoundary
        rdf:type      owl:DatatypeProperty;
        rdfs:comment  "Specifies the upper boundary for the tolerance.\n"@en;
        rdfs:domain   vec:Tolerance;
        rdfs:label    "upperBoundary"@en;
        rdfs:range    xs:double .

vec:SegmentConnectionPoint
        rdf:type         owl:Class;
        rdfs:comment     "Specifies a point where the connector can be attached to the topology (sometimes called bundle position point or insertion point).\n"@en;
        rdfs:label       "SegmentConnectionPoint"@en;
        rdfs:subClassOf  vec:ExtendableElement .

vec:RelaisType_Bistable
        rdf:type         vec:RelaisType , owl:NamedIndividiual;
        rdfs:comment     "Defines a relais that is bistable .\n"@en;
        vec:enumLiteral  "bistable" .

vec:UsageConstraintSpecification
        rdf:type         owl:Class;
        rdfs:comment     "Specification for the definition of usage constraints. The associated UsageConstraints are restricting the possible usages of the associated PartVersions and PartUsages.\n"@en;
        rdfs:label       "UsageConstraintSpecification"@en;
        rdfs:subClassOf  vec:Specification .

vec:ImperialUnitName_Gill
        rdf:type         vec:ImperialUnitName , owl:NamedIndividiual;
        vec:enumLiteral  "Gill" .

vec:zoneAssignmentAssignedSegment
        rdf:type      owl:ObjectProperty;
        rdfs:comment  "The TopologySegment that is assigned to TopologyZone with this ZoneAssignment.\n"@en;
        rdfs:domain   vec:ZoneAssignment;
        rdfs:label    "assignedSegment"@en;
        rdfs:range    vec:TopologySegment .

vec:NetGroup  rdf:type   owl:Class;
        rdfs:comment     "Defines a logical grouping of specific Nets . For example, it can be used to identify all Nets of specific CAN domain, a function, a requirement level (e.g. Safety┬á&┬áSecurity).\n"@en;
        rdfs:label       "NetGroup"@en;
        rdfs:subClassOf  vec:ConfigurableElement .

vec:UsageNodeType_Grommet
        rdf:type         vec:UsageNodeType , owl:NamedIndividiual;
        vec:enumLiteral  "Grommet" .

vec:terminalTypeNominalSize
        rdf:type      owl:DatatypeProperty;
        rdfs:comment  "Specifies the nominal size of terminals that fit into the cavity. (e.g. 2x4).\n"@en;
        rdfs:domain   vec:TerminalType;
        rdfs:label    "nominalSize"@en;
        rdfs:range    xs:string .

vec:LanguageCode_Iw  rdf:type  vec:LanguageCode , owl:NamedIndividiual;
        vec:enumLiteral  "Iw" .

vec:componentNodeAbbreviation
        rdf:type            owl:ObjectProperty;
        rdfs:comment        "Room for a short name of the ComponentNode.\n"@en;
        rdfs:domain         vec:ComponentNode;
        rdfs:label          "abbreviation"@en;
        rdfs:range          vec:LocalizedString;
        rdfs:subPropertyOf  vec:contains .

vec:PinVoltageType_BlockVoltage
        rdf:type         vec:PinVoltageType , owl:NamedIndividiual;
        vec:enumLiteral  "blockVoltage" .

vec:InsulationState_Insulated
        rdf:type         vec:InsulationState , owl:NamedIndividiual;
        rdfs:comment     "The splice is electrically insulated.\n"@en;
        vec:enumLiteral  "Insulated" .

vec:abstractLocalizedStringLanguageCode
        rdf:type            owl:ObjectProperty;
        rdfs:comment        "References the corresponding languageCode of the value.\n"@en;
        rdfs:domain         vec:AbstractLocalizedString;
        rdfs:label          "languageCode"@en;
        rdfs:range          vec:LanguageCode;
        rdfs:subPropertyOf  vec:contains .

vec:sheetOrChapterSheetNumber
        rdf:type      owl:DatatypeProperty;
        rdfs:comment  "The sheetNumber is the major identifier of a SheetOrChapter. The format is user defined and respectively company specific. This field has to be used if a SheetOrChapter has its own \"DocumentNumber\".\n"@en;
        rdfs:domain   vec:SheetOrChapter;
        rdfs:label    "sheetNumber"@en;
        rdfs:range    xs:string .

vec:LanguageCode_Cy  rdf:type  vec:LanguageCode , owl:NamedIndividiual;
        vec:enumLiteral  "Cy" .

vec:dimensionIdentification
        rdf:type      owl:DatatypeProperty;
        rdfs:comment  "Specifies a unique identification of the Dimension. The identification is guaranteed to be unique within the containing PlacementSpecification.\n"@en;
        rdfs:domain   vec:Dimension;
        rdfs:label    "identification"@en;
        rdfs:range    xs:string .

vec:TerminalCurrentInformation
        rdf:type      owl:Class;
        rdfs:comment  "Allows the definition of valid current ranges for a terminal. A current range is always defined for a coreCrossSectionArea and a nominal voltage. Attributes of the type CurrentRangeInformation normally have the multiplicity [0..*]. This means that such an attribute can have CurrentRangeInformation entries for different coreCrossSectionAreas and nominalVoltages. It must not have multiple entries for the same coreCrossSectionAreas and nominalVoltages.\n"@en;
        rdfs:label    "TerminalCurrentInformation"@en .

vec:HistoryEntryType_Derivation
        rdf:type         vec:HistoryEntryType , owl:NamedIndividiual;
        vec:enumLiteral  "Derivation" .

vec:ClosedEnumeration
        rdf:type         owl:Class;
        rdfs:comment     "Classes in the model that can be enumerated and where all values are known (closed)."@en;
        rdfs:label       "ClosedEnumeration"@en;
        rdfs:subClassOf  vec:Enumeration .

vec:ConnectionSpecification
        rdf:type         owl:Class;
        rdfs:comment     "A ConnectionSpecification is used to define electrological connectivity.\n"@en;
        rdfs:label       "ConnectionSpecification"@en;
        rdfs:subClassOf  vec:Specification .

vec:buildingBlockSpecification3DPlacedElementViewItem3D
        rdf:type            owl:ObjectProperty;
        rdfs:comment        "Specifies the view items for OccurrenceOrUsages in a BuildingBlockSpecification3D. \n"@en;
        rdfs:domain         vec:BuildingBlockSpecification3D;
        rdfs:label          "placedElementViewItem3D"@en;
        rdfs:range          vec:OccurrenceOrUsageViewItem3D;
        rdfs:subPropertyOf  vec:contains .

vec:AnchorType_FromStartNode
        rdf:type         vec:AnchorType , owl:NamedIndividiual;
        rdfs:comment     "The offset of the location is measured from the startNode of the TopologySegment.\n"@en;
        vec:enumLiteral  "FromStartNode" .

vec:LanguageCode_Sw  rdf:type  vec:LanguageCode , owl:NamedIndividiual;
        vec:enumLiteral  "Sw" .

vec:PinComponentType_Switch
        rdf:type         vec:PinComponentType , owl:NamedIndividiual;
        vec:enumLiteral  "Switch" .

vec:LocalizedTypedStringType
        rdf:type         owl:Class;
        rdfs:label       "LocalizedTypedStringType"@en;
        rdfs:subClassOf  vec:OpenEnumeration .

vec:partSubstitutionSpecificationAlternativePartVersions
        rdf:type     owl:ObjectProperty;
        rdfs:domain  vec:PartSubstitutionSpecification;
        rdfs:label   "alternativePartVersions"@en;
        rdfs:range   vec:PartVersion .

vec:ConnectorOutletDirection
        rdf:type         owl:Class;
        rdfs:comment     "Defines the OutletDirection of a connector for wires.\n"@en;
        rdfs:label       "ConnectorOutletDirection"@en;
        rdfs:subClassOf  vec:OpenEnumeration .

vec:TubeShape_Circular
        rdf:type         vec:TubeShape , owl:NamedIndividiual;
        rdfs:comment     "The tube has circular cross section.\n"@en;
        vec:enumLiteral  "Circular" .

vec:moduleListCompletionComponents
        rdf:type      owl:ObjectProperty;
        rdfs:comment  "References the components that are used as completion, if any of the Modules in the ModuleList appears in a configuration. \n"@en;
        rdfs:domain   vec:ModuleList;
        rdfs:label    "completionComponents"@en;
        rdfs:range    vec:OccurrenceOrUsage .

vec:LanguageCode_My  rdf:type  vec:LanguageCode , owl:NamedIndividiual;
        vec:enumLiteral  "My" .

vec:transformation2DA12
        rdf:type     owl:DatatypeProperty;
        rdfs:domain  vec:Transformation2D;
        rdfs:label   "a12"@en;
        rdfs:range   xs:double .

vec:buildingBlockSpecification3DBaseUnit
        rdf:type      owl:ObjectProperty;
        rdfs:comment  ""@en;
        rdfs:domain   vec:BuildingBlockSpecification3D;
        rdfs:label    "baseUnit"@en;
        rdfs:range    vec:Unit .

vec:VariantStructureNode
        rdf:type         owl:Class;
        rdfs:comment     " VariantStructureNodes can be used to define a hierarchical structure on VariantGroups . Every VariantStructureNodes can reference VariantGroups and VariantStructureNodes as children.\n"@en;
        rdfs:label       "VariantStructureNode"@en;
        rdfs:subClassOf  vec:ExtendableElement .

vec:applicationConstraintToSerialNumber
        rdf:type      owl:DatatypeProperty;
        rdfs:comment  "Specifies the upper bound of a serial number range to which the application constraint applies.\n"@en;
        rdfs:domain   vec:ApplicationConstraint;
        rdfs:label    "toSerialNumber"@en;
        rdfs:range    xs:string .

vec:wireReceptionPlacementPoint
        rdf:type      owl:ObjectProperty;
        rdfs:comment  "Specifies the PlacementPoint that represents this WireReception in a PlaceableElementSpecification.\n"@en;
        rdfs:domain   vec:WireReception;
        rdfs:label    "placementPoint"@en;
        rdfs:range    vec:PlacementPoint .

vec:TerminalReceptionSpecification
        rdf:type         owl:Class;
        rdfs:comment     "Specification for the definition of terminal receptions. A TerminalReception is the area of a terminal where the contacting with another terminal (e.g. between a connector housing and a control unit) takes place. Normally the terminal reception is placed in a cavity of a connector housing.\n"@en;
        rdfs:label       "TerminalReceptionSpecification"@en;
        rdfs:subClassOf  vec:Specification .

vec:GrommetMountingType_Moulded
        rdf:type         vec:GrommetMountingType , owl:NamedIndividiual;
        rdfs:comment     "The grommet created in place around the harness with some kind of moulding or foaming manufacturing process."@en;
        vec:enumLiteral  "Moulded" .

vec:conductorSpecificationMassInformation
        rdf:type            owl:ObjectProperty;
        rdfs:comment        "Specifies the mass information of the conductor. In most cases this mass information is known as copper weight and is normally specified as mass per length (e.g. gram per meter).\n"@en;
        rdfs:domain         vec:ConductorSpecification;
        rdfs:label          "massInformation"@en;
        rdfs:range          vec:MassInformation;
        rdfs:subPropertyOf  vec:contains .

vec:wireReceptionSpecificationRearBellMouthLength
        rdf:type            owl:ObjectProperty;
        rdfs:comment        "Specifies the length of the rear bell mouth of the conductor crimp (wire reception, see diagram \"Terminal Dimensions\").\n"@en;
        rdfs:domain         vec:WireReceptionSpecification;
        rdfs:label          "rearBellMouthLength"@en;
        rdfs:range          vec:NumericalValue;
        rdfs:subPropertyOf  vec:contains .

vec:usageNodeAbbreviation
        rdf:type            owl:ObjectProperty;
        rdfs:comment        "Specifies an abbreviation of the UsageNode . Normally this a human readable short name.\n"@en;
        rdfs:domain         vec:UsageNode;
        rdfs:label          "abbreviation"@en;
        rdfs:range          vec:LocalizedString;
        rdfs:subPropertyOf  vec:contains .

vec:ImperialUnitName_Ton
        rdf:type         vec:ImperialUnitName , owl:NamedIndividiual;
        vec:enumLiteral  "Ton" .

vec:nURBSCurveKnots  rdf:type  owl:DatatypeProperty;
        rdfs:comment  "Defines the knot-vector of the NURBS(for details see the class description of NURBSCurve).\n"@en;
        rdfs:domain   vec:NURBSCurve;
        rdfs:label    "knots"@en;
        rdfs:range    xs:double .

vec:ConductorStructure
        rdf:type         owl:Class;
        rdfs:comment     "Specifies the structure of the conductor according to ISO 6722-1 for ConductorSpecifications with Type = Stranded.\n"@en;
        rdfs:label       "ConductorStructure"@en;
        rdfs:subClassOf  vec:OpenEnumeration .

vec:partOccurrenceAlternativeOccurrence
        rdf:type      owl:ObjectProperty;
        rdfs:comment  "References the PartOccurrences that are an alternative for this PartOccurrence.\n"@en;
        rdfs:domain   vec:PartOccurrence;
        rdfs:label    "alternativeOccurrence"@en;
        rdfs:range    vec:PartOccurrence .

vec:FileBasedInstruction
        rdf:type         owl:Class;
        rdfs:comment     "A FileBasedInstruction is an Instruction that references a file packaged (VEC-Package) together with a VEC-file. Such a file can be for example an image.\n"@en;
        rdfs:label       "FileBasedInstruction"@en;
        rdfs:subClassOf  vec:Instruction .

vec:RelaisType_Switch
        rdf:type         vec:RelaisType , owl:NamedIndividiual;
        rdfs:comment     "Defines a relais that is a switch.\n"@en;
        vec:enumLiteral  "switch" .

vec:wireReceptionReferenceIdentification
        rdf:type      owl:DatatypeProperty;
        rdfs:comment  "Specifies a unique identification of the WireReceptionReference . The identification is guaranteed to be unique within the TerminalRole (this might be for example a reception number).\n"@en;
        rdfs:domain   vec:WireReceptionReference;
        rdfs:label    "identification"@en;
        rdfs:range    xs:string .

vec:FerriteSpecification
        rdf:type         owl:Class;
        rdfs:comment     "Specification for the definition of ferrites.\n"@en;
        rdfs:label       "FerriteSpecification"@en;
        rdfs:subClassOf  vec:PartOrUsageRelatedSpecification .

vec:slotCouplingFirstSlot
        rdf:type     owl:ObjectProperty;
        rdfs:domain  vec:SlotCoupling;
        rdfs:label   "firstSlot"@en;
        rdfs:range   vec:AbstractSlotReference .

vec:buildingBlockPositioning3DReferenced3DBuildingBlock
        rdf:type      owl:ObjectProperty;
        rdfs:comment  "References the building block that is positioned.\n"@en;
        rdfs:domain   vec:BuildingBlockPositioning3D;
        rdfs:label    "referenced3DBuildingBlock"@en;
        rdfs:range    vec:BuildingBlockSpecification3D .

vec:SlotLayoutType_USBMicroA
        rdf:type         vec:SlotLayoutType , owl:NamedIndividiual;
        vec:enumLiteral  "USBMicroA" .

vec:documentVersionDigitalRepresentationIndex
        rdf:type      owl:DatatypeProperty;
        rdfs:comment  "An arbitrary change index that indicates if the digital representation (the content in VEC) of this DocumentVersion has been changed /┬áregenerated. This can be for example an index, a timestamp or a checksum. This allows the detection of changes in the content, even when the DocumentNumber &┬áDocumentVersion is the same.\nFor a more detailed explanation in the context see \"Parts┬á&┬áDocuments\". KBLFRM-837.\n"@en;
        rdfs:domain   vec:DocumentVersion;
        rdfs:label    "digitalRepresentationIndex"@en;
        rdfs:range    xs:string .

vec:geometryNode3DCartesianPoint
        rdf:type      owl:ObjectProperty;
        rdfs:comment  "References the CartesianPoint3D where the GeometryNode3D is located. \n"@en;
        rdfs:domain   vec:GeometryNode3D;
        rdfs:label    "cartesianPoint"@en;
        rdfs:range    vec:CartesianPoint3D .

vec:WireElement  rdf:type  owl:Class;
        rdfs:comment     "A WireElement specifies a WireElementSpecification in the context of a WireSpecification . This is necessary to define a unique identification of a WireElementSpecification in the context of a WireSpecification. Additionally, the WireElement serves as anchor for the instancing of a wire ( WireElementReference ) as the WireElementSpecifications are not uniquely related to a WireSpecification for reasons of reusability.\n"@en;
        rdfs:label       "WireElement"@en;
        rdfs:subClassOf  vec:ExtendableElement .

vec:wireProtectionSpecificationSoundDampingClass
        rdf:type            owl:ObjectProperty;
        rdfs:comment        "Specifies the class of sound damping. According to the VDA this is a value between A & E. KBLFRM-311\n"@en;
        rdfs:domain         vec:WireProtectionSpecification;
        rdfs:label          "soundDampingClass"@en;
        rdfs:range          vec:SoundDampingClass;
        rdfs:subPropertyOf  vec:contains .

vec:SiUnitName_Lumen  rdf:type  vec:SiUnitName , owl:NamedIndividiual;
        vec:enumLiteral  "Lumen" .

vec:USUnitName_Rood  rdf:type  vec:USUnitName , owl:NamedIndividiual;
        vec:enumLiteral  "Rood" .

vec:ComponentNodeType_Lamp
        rdf:type         vec:ComponentNodeType , owl:NamedIndividiual;
        rdfs:comment     " Deprecated since VEC V1.2. Use ComponentNodeType \"Actuator\" instead and ComponentSubType Lamp .\n"@en;
        vec:enumLiteral  "Lamp" .

<http://www.prostep.org/ontologies/ecad/2024/03/vec#RelaisType_Normally%20closed>
        rdf:type         vec:RelaisType , owl:NamedIndividiual;
        rdfs:comment     "Defines a relais that is closed in its normal state.\n"@en;
        vec:enumLiteral  "normally closed" .

vec:CableLeadThroughReference
        rdf:type      owl:Class;
        rdfs:comment  "A CableLeadThroughReference is the instance of a CableLeadThrough. It can define a set of plugs or seals that are used together with it. Plugs are used if no wire is present, seals are used together with a wire.\n"@en;
        rdfs:label    "CableLeadThroughReference"@en .

vec:ImperialUnitName_Perch
        rdf:type         vec:ImperialUnitName , owl:NamedIndividiual;
        vec:enumLiteral  "Perch" .

vec:IECPrefix_Tebi  rdf:type  vec:IECPrefix , owl:NamedIndividiual;
        vec:enumLiteral  "Tebi" .

vec:SimpleValueProperty
        rdf:type         owl:Class;
        rdfs:comment     "A custom property with a simple value (string).\n"@en;
        rdfs:label       "SimpleValueProperty"@en;
        rdfs:subClassOf  vec:CustomProperty .

vec:PartRelationType  rdf:type  owl:Class;
        rdfs:comment         "Defines how the set of acessoryParts referenced by a PartRelation should be interpreted.\n"@en;
        rdfs:label           "PartRelationType"@en;
        rdfs:subClassOf      vec:ClosedEnumeration;
        owl:equivalentClass  [ rdf:type   owl:Class;
                               owl:oneOf  ( vec:PartRelationType_Mandatory vec:PartRelationType_Optional vec:PartRelationType_OneOfAll vec:PartRelationType_Custom )
                             ] .

vec:ComplexProperty  rdf:type  owl:Class;
        rdfs:comment     "A custom property that represents a tuple of values.\n"@en;
        rdfs:label       "ComplexProperty"@en;
        rdfs:subClassOf  vec:CustomProperty .

vec:WindingFirmness_Limp
        rdf:type         vec:WindingFirmness , owl:NamedIndividiual;
        rdfs:comment     "┬áThe taping is applied limp (loose taping).\n"@en;
        vec:enumLiteral  "Limp" .

vec:OtherUnitName_Pi  rdf:type  vec:OtherUnitName , owl:NamedIndividiual;
        vec:enumLiteral  "Pi" .

vec:BoundingBox  rdf:type  owl:Class;
        rdfs:comment  "The bounding box is used to define a cuboid┬á(box) that can contain a described part completely. Therefore, it is a simplified representation of the bounding volume and represents a definition of the maximum volume occupied by the part.\nIt is valid to use the BoundingBox to describe the dimensions of a component, even if not all dimensions are known (e.g. only length and width). However, it must be possible to transform such a partial bounding box into a complete bounding box by adding the missing dimensions.\n"@en;
        rdfs:label    "BoundingBox"@en .

vec:LanguageCode_Ha  rdf:type  vec:LanguageCode , owl:NamedIndividiual;
        vec:enumLiteral  "Ha" .

vec:geometryNodeReferenceNode
        rdf:type      owl:ObjectProperty;
        rdfs:comment  "References the TopologyNode that is represented by the GeometryNode.\n"@en;
        rdfs:domain   vec:GeometryNode;
        rdfs:label    "referenceNode"@en;
        rdfs:range    vec:TopologyNode .

vec:buildingBlockSpecification2DPlacedElementViewItem
        rdf:type            owl:ObjectProperty;
        rdfs:comment        "Specifies the view items for OccurrenceOrUsages on a BuildingBlockSpecification2D. \n"@en;
        rdfs:domain         vec:BuildingBlockSpecification2D;
        rdfs:label          "placedElementViewItem"@en;
        rdfs:range          vec:OccurrenceOrUsageViewItem2D;
        rdfs:subPropertyOf  vec:contains .

vec:netGroupNet  rdf:type  owl:ObjectProperty;
        rdfs:comment  "References the Nets that are grouped by the NetGroup. \n"@en;
        rdfs:domain   vec:NetGroup;
        rdfs:label    "net"@en;
        rdfs:range    vec:Net .

vec:signalSignalCurve
        rdf:type            owl:ObjectProperty;
        rdfs:comment        "Specifies the curve of the signal.\n"@en;
        rdfs:domain         vec:Signal;
        rdfs:label          "signalCurve"@en;
        rdfs:range          vec:SignalCurve;
        rdfs:subPropertyOf  vec:contains .

vec:PinComponentType_Ground
        rdf:type         vec:PinComponentType , owl:NamedIndividiual;
        vec:enumLiteral  "Ground" .

vec:slotMappingCavityMapping
        rdf:type            owl:ObjectProperty;
        rdfs:comment        ""@en;
        rdfs:domain         vec:SlotMapping;
        rdfs:label          "cavityMapping"@en;
        rdfs:range          vec:CavityMapping;
        rdfs:subPropertyOf  vec:contains .

vec:LevelOfApproval_Develop
        rdf:type         vec:LevelOfApproval , owl:NamedIndividiual;
        rdfs:comment     "An approval during the development process. There might process specific different approvals out of this category. See Approval.additionalLevelInformation for more information about the details.\n"@en;
        vec:enumLiteral  "Develop" .

vec:moduleListModuleInList
        rdf:type      owl:ObjectProperty;
        rdfs:comment  "References the Modules that belong to the ModuleList. If any of the referenced Modules participates in a configuration the completion components participate, too.\n"@en;
        rdfs:domain   vec:ModuleList;
        rdfs:label    "moduleInList"@en;
        rdfs:range    vec:PartWithSubComponentsRole .

vec:TerminalBoltNominalSize_M16
        rdf:type         vec:TerminalBoltNominalSize , owl:NamedIndividiual;
        vec:enumLiteral  "M16" .

vec:NetworkNode  rdf:type  owl:Class;
        rdfs:comment     "A NetworkNode is a representative for an actor in the electric system, e.g. an actuator, a sensor, an ECU\n"@en;
        rdfs:label       "NetworkNode"@en;
        rdfs:subClassOf  vec:ConfigurableElement .

vec:PinCurrentType_TypicalCurrent
        rdf:type         vec:PinCurrentType , owl:NamedIndividiual;
        vec:enumLiteral  "typicalCurrent" .

vec:TerminalBoltNominalSize_1
        rdf:type         vec:TerminalBoltNominalSize , owl:NamedIndividiual;
        vec:enumLiteral  "1" .

vec:CableLeadThroughGeometry_Square
        rdf:type         vec:CableLeadThroughGeometry , owl:NamedIndividiual;
        vec:enumLiteral  "Square" .

vec:batterySpecificationCapacity
        rdf:type            owl:ObjectProperty;
        rdfs:comment        "Specifies the power capacity of the battery.\n"@en;
        rdfs:domain         vec:BatterySpecification;
        rdfs:label          "capacity"@en;
        rdfs:range          vec:NumericalValue;
        rdfs:subPropertyOf  vec:contains .

vec:dimensionPath  rdf:type  owl:ObjectProperty;
        rdfs:comment        "Specifies a path in the topology along which the dimension is defined. \n"@en;
        rdfs:domain         vec:Dimension;
        rdfs:label          "path"@en;
        rdfs:range          vec:Path;
        rdfs:subPropertyOf  vec:contains .

vec:connectorHousingCapSpecificationOutletDirection
        rdf:type            owl:ObjectProperty;
        rdfs:comment        "Defines the OutletDirection for wires.\nThis attribute is defined as an OpenEnumeration .\n"@en;
        rdfs:domain         vec:ConnectorHousingCapSpecification;
        rdfs:label          "outletDirection"@en;
        rdfs:range          vec:ConnectorOutletDirection;
        rdfs:subPropertyOf  vec:contains .

vec:connectionGroupConnection
        rdf:type      owl:ObjectProperty;
        rdfs:comment  "References the Connections that are grouped by the ConnectionGroup. \n"@en;
        rdfs:domain   vec:ConnectionGroup;
        rdfs:label    "connection"@en;
        rdfs:range    vec:Connection .

vec:itemVersionCopyrightInformation
        rdf:type      owl:ObjectProperty;
        rdfs:comment  "References the CopyrightInformation that is in effect for this ItemVersion. If no CopyrightInformation is referenced by the ItemVersion , the CopyrightInformation that is referenced by the VecContent (if defined) shall be considered as in effect for this ItemVersion.\n"@en;
        rdfs:domain   vec:ItemVersion;
        rdfs:label    "copyrightInformation"@en;
        rdfs:range    vec:CopyrightInformation .

vec:integerValuePropertyValue
        rdf:type      owl:DatatypeProperty;
        rdfs:comment  "Defines the value of the CustomProperty.\n"@en;
        rdfs:domain   vec:IntegerValueProperty;
        rdfs:label    "value"@en;
        rdfs:range    xs:integer .

vec:ItemVersion  rdf:type  owl:Class;
        rdfs:comment     "Abstract super-class for physical objects (e.g. a Terminal), virtual objects (e.g. a 150% Harness) as well as documents (e.g. a wiring diagram). In difference to AP 212 the VEC makes it only possible to describe/exchange information about Versions since Master-Objects cannot exist without one or more Versions.\n"@en;
        rdfs:label       "ItemVersion"@en;
        rdfs:subClassOf  vec:ExtendableElement .

vec:ConfigurationConstraint
        rdf:type         owl:Class;
        rdfs:comment     "Represents a ConfigurationContraint (\"When does this element exist?\") for a specific application ( ApplicationConstraint) and a \"configuration universe\"┬á( VariantConfiguration.configurationType )\n"@en;
        rdfs:label       "ConfigurationConstraint"@en;
        rdfs:subClassOf  vec:ExtendableElement .

vec:holeMountedFixingSpecificationPlateThickness
        rdf:type            owl:ObjectProperty;
        rdfs:comment        "Specifies the thickness of the plate in which the hole is positioned.\n"@en;
        rdfs:domain         vec:HoleMountedFixingSpecification;
        rdfs:label          "plateThickness"@en;
        rdfs:range          vec:ValueRange;
        rdfs:subPropertyOf  vec:contains .

vec:transformation3DA21
        rdf:type     owl:DatatypeProperty;
        rdfs:domain  vec:Transformation3D;
        rdfs:label   "a21"@en;
        rdfs:range   xs:double .

vec:FuseSpecification
        rdf:type         owl:Class;
        rdfs:comment     "Specification of the electrological aspects of a fuse.\n"@en;
        rdfs:label       "FuseSpecification"@en;
        rdfs:subClassOf  vec:EEComponentSpecification .

vec:cableLeadThroughSpecificationMinSegmentOutsideDiameter
        rdf:type            owl:ObjectProperty;
        rdfs:comment        "Specifies the minimum diameter a segment can have to fit through the cable lead through. This definition is necessary, since segments that are too small might cause movements and unacceptable torsion forces or they are not sealable.\n"@en;
        rdfs:domain         vec:CableLeadThroughSpecification;
        rdfs:label          "minSegmentOutsideDiameter"@en;
        rdfs:range          vec:NumericalValue;
        rdfs:subPropertyOf  vec:contains .

vec:itemVersionAbbreviation
        rdf:type            owl:ObjectProperty;
        rdfs:comment        "Room for a short name of the Item. In case of a document the attribute is wanted to contain its title.\n"@en;
        rdfs:domain         vec:ItemVersion;
        rdfs:label          "abbreviation"@en;
        rdfs:range          vec:LocalizedString;
        rdfs:subPropertyOf  vec:contains .

vec:WireAddOnType_Production
        rdf:type         vec:WireAddOnType , owl:NamedIndividiual;
        rdfs:comment     "The add-on length for the use in production environments.\n"@en;
        vec:enumLiteral  "Production" .

vec:ImperialUnitName_Furlong
        rdf:type         vec:ImperialUnitName , owl:NamedIndividiual;
        vec:enumLiteral  "Furlong" .

vec:holeMountedFixingSpecificationHoleType
        rdf:type            owl:ObjectProperty;
        rdfs:comment        "Specifies the type of how the fixing is fixated in the hole.┬áIn other words, it defines what features the hole has to provide to allow a fixation of the fixing.\n"@en;
        rdfs:domain         vec:HoleMountedFixingSpecification;
        rdfs:label          "holeType"@en;
        rdfs:range          vec:HoleMountedFixingHoleType;
        rdfs:subPropertyOf  vec:contains .

vec:ComponentPort  rdf:type  owl:Class;
        rdfs:comment     "Defines a port of ComponentNode. A ComponentPort is usually the realization of a NetworkPort. Electrological connections are defined between two or more ComponentPorts.\n"@en;
        rdfs:label       "ComponentPort"@en;
        rdfs:subClassOf  vec:ConfigurableElement .

vec:ImperialUnitName_Acre
        rdf:type         vec:ImperialUnitName , owl:NamedIndividiual;
        vec:enumLiteral  "Acre" .

vec:PartRelationType_Optional
        rdf:type         vec:PartRelationType , owl:NamedIndividiual;
        rdfs:comment     " Optional means that in a usage of a component some referenced acessoryParts can be used by choice.\n"@en;
        vec:enumLiteral  "Optional" .

vec:complexPropertyCustomProperty
        rdf:type            owl:ObjectProperty;
        rdfs:comment        "The customProperties that represent the individual values of the complex property.\n"@en;
        rdfs:domain         vec:ComplexProperty;
        rdfs:label          "customProperty"@en;
        rdfs:range          vec:CustomProperty;
        rdfs:subPropertyOf  vec:contains .

vec:SignalType_Ground
        rdf:type         vec:SignalType , owl:NamedIndividiual;
        vec:enumLiteral  "ground" .

vec:contactPointCavityMounting
        rdf:type            owl:ObjectProperty;
        rdfs:comment        "Defines the mounting to a cavity of the terminal associated with the ContactPoint. \nThe cardinality is 0..* in order to allow a variant dependant cavity mounting. In such a scenario a cavity mounting is valid in a configuration if all addressed cavities and therefore the associated connector housing is available. \n"@en;
        rdfs:domain         vec:ContactPoint;
        rdfs:label          "cavityMounting"@en;
        rdfs:range          vec:CavityMounting;
        rdfs:subPropertyOf  vec:contains .

vec:vecContentProject
        rdf:type            owl:ObjectProperty;
        rdfs:comment        "Specifies the Projects used in the VEC-file. \n"@en;
        rdfs:domain         vec:VecContent;
        rdfs:label          "project"@en;
        rdfs:range          vec:Project;
        rdfs:subPropertyOf  vec:contains .

vec:LabelPosition_Continuous
        rdf:type         vec:LabelPosition , owl:NamedIndividiual;
        vec:enumLiteral  "Continuous" .

vec:PartSubstitutionSpecification
        rdf:type         owl:Class;
        rdfs:comment     "A PartSubstitutionSpecification defines a set of PartVersions that can be used alternatively, due to an incomplete specification for the 150% product description. For a concrete wiring harness only on valid PartVersion remains. The selection logic for valid PartVersions is not included in the VEC.\nA PartSubstitutionSpecification can be used for example tubes or ring terminals, where a part of the specification is known at design time, but not yet the complete specification. For tubes for example the tube diameter is not known at design time, since it depends on the bundle diameter of a specific configuration.\n"@en;
        rdfs:label       "PartSubstitutionSpecification"@en;
        rdfs:subClassOf  vec:Specification .

vec:InsulationState_Uninsulated
        rdf:type         vec:InsulationState , owl:NamedIndividiual;
        rdfs:comment     "The splice is not electrically insulated.\n"@en;
        vec:enumLiteral  "Uninsulated" .

vec:wireTypeReferenceSystem
        rdf:type      owl:DatatypeProperty;
        rdfs:comment  "Specifies the reference system for the wire type.\n"@en;
        rdfs:domain   vec:WireType;
        rdfs:label    "referenceSystem"@en;
        rdfs:range    xs:string .

vec:documentRelatedAssignmentGroupRelatedSheetOrChapter
        rdf:type      owl:ObjectProperty;
        rdfs:comment  "Allows a more specific relationship to a SheetOrChapter within the relatedDocumentVersion. ┬á\n"@en;
        rdfs:domain   vec:DocumentRelatedAssignmentGroup;
        rdfs:label    "relatedSheetOrChapter"@en;
        rdfs:range    vec:SheetOrChapter .

[ rdf:type     owl:AllDisjointClasses;
  owl:members  ( vec:MeasurementPointReference vec:Location )
] .

vec:terminalCurrentInformationCurrentRange
        rdf:type            owl:ObjectProperty;
        rdfs:comment        "Specifies the valid current range for the terminal. It is defined as a value range, because there are terminals where minimum current is needed to avoid corrosion.\n"@en;
        rdfs:domain         vec:TerminalCurrentInformation;
        rdfs:label          "currentRange"@en;
        rdfs:range          vec:ValueRange;
        rdfs:subPropertyOf  vec:contains .

vec:VariantGroupType  rdf:type  owl:Class;
        rdfs:comment     "Defines valid values for the type of VariantGroups.\n"@en;
        rdfs:label       "VariantGroupType"@en;
        rdfs:subClassOf  vec:OpenEnumeration .

vec:TubeSpecification
        rdf:type         owl:Class;
        rdfs:comment     "Specifies tubes.\n"@en;
        rdfs:label       "TubeSpecification"@en;
        rdfs:subClassOf  vec:WireProtectionSpecification .

vec:WireMountingDetail
        rdf:type         owl:Class;
        rdfs:comment     "With a WireMountingDetail it is possible to describe a detailed wire mounting.\nThis is needed if the information which wire end is mounted onto which wire reception is important (e.g. coax contacts).\n"@en;
        rdfs:label       "WireMountingDetail"@en;
        rdfs:subClassOf  vec:ExtendableElement .

vec:SignalTransmissionMediumType_RadioTransmission
        rdf:type         vec:SignalTransmissionMediumType , owl:NamedIndividiual;
        rdfs:comment     "Signal transmission via electromagnetic waves (e.g. Wi-Fi, 4G, 5G)\n"@en;
        vec:enumLiteral  "radioTransmission" .

vec:LanguageCode_Bh  rdf:type  vec:LanguageCode , owl:NamedIndividiual;
        vec:enumLiteral  "Bh" .

[ rdf:type     owl:AllDisjointClasses;
  owl:members  ( vec:CavityPlugSpecification vec:CavitySealSpecification vec:CavityAccessorySpecification )
] .

vec:housingComponentIdentification
        rdf:type      owl:DatatypeProperty;
        rdfs:comment  "Identification of the HousingComponent, which must be distinct for all HousingComponents of an EEComponent.\n"@en;
        rdfs:domain   vec:HousingComponent;
        rdfs:label    "identification"@en;
        rdfs:range    xs:string .

vec:componentNodeRealizedUsageNode
        rdf:type      owl:ObjectProperty;
        rdfs:comment  "References the UsageNode that is realized by this ComponentNode .\n"@en;
        rdfs:domain   vec:ComponentNode;
        rdfs:label    "realizedUsageNode"@en;
        rdfs:range    vec:UsageNode .

vec:requirementsConformanceStatementSatisfies
        rdf:type      owl:DatatypeProperty;
        rdfs:comment  "Defines if the describedParts satisfy (satisfy =┬átrue) or explicitly fail (satisfy = false) to conform with the requirementsSpecification .\n"@en;
        rdfs:domain   vec:RequirementsConformanceStatement;
        rdfs:label    "satisfies"@en;
        rdfs:range    xs:boolean .

vec:mappingSlotMapping
        rdf:type            owl:ObjectProperty;
        rdfs:comment        ""@en;
        rdfs:domain         vec:Mapping;
        rdfs:label          "slotMapping"@en;
        rdfs:range          vec:SlotMapping;
        rdfs:subPropertyOf  vec:contains .

vec:ComponentNodeType_ECU
        rdf:type         vec:ComponentNodeType , owl:NamedIndividiual;
        rdfs:comment     "Electronic Control Unit. An electronic control unit (ECU) is any embedded system in automotive electronics that controls one or more of the electrical systems or subsystems in a vehicle.\n"@en;
        vec:enumLiteral  "ECU" .

vec:SignalSubType_RGB
        rdf:type         vec:SignalSubType , owl:NamedIndividiual;
        vec:enumLiteral  "RGB" .

vec:VariantStructureSpecification
        rdf:type         owl:Class;
        rdfs:comment     "Specification to define any hierarchical structure on variant groups (e.g. by the means of a functional organization).┬áThe hierarchy starts with a single root node.\n"@en;
        rdfs:label       "VariantStructureSpecification"@en;
        rdfs:subClassOf  vec:Specification .

vec:pinComponentIdentification
        rdf:type      owl:DatatypeProperty;
        rdfs:comment  "Identification of the PinComponent, which must be distinct for all PinComponent of a HousingComponents.\n"@en;
        rdfs:domain   vec:PinComponent;
        rdfs:label    "identification"@en;
        rdfs:range    xs:string .

vec:DocumentRelationType
        rdf:type         owl:Class;
        rdfs:label       "DocumentRelationType"@en;
        rdfs:subClassOf  vec:OpenEnumeration .

vec:pathSegmentCurveRadius
        rdf:type            owl:ObjectProperty;
        rdfs:comment        "The radius of the curve which describes the appearance of the path segment.\n"@en;
        rdfs:domain         vec:PathSegment;
        rdfs:label          "curveRadius"@en;
        rdfs:range          vec:NumericalValue;
        rdfs:subPropertyOf  vec:contains .

<http://www.prostep.org/ontologies/ecad/2024/03/vec#TerminalBoltNominalSize_3%2F4>
        rdf:type         vec:TerminalBoltNominalSize , owl:NamedIndividiual;
        vec:enumLiteral  "3/4" .

vec:Transformation3D  rdf:type  owl:Class;
        rdfs:comment     "A Transformation is a geometric transformation and specifies a transformation matrix.\n"@en;
        rdfs:label       "Transformation3D"@en;
        rdfs:subClassOf  vec:ExtendableElement .

vec:SpecificRole  rdf:type  owl:Class;
        rdfs:comment     "A SpecificRole is the possibility to define instance specific properties with custom properties (see ExtendableElement). This is necessary, if the part is described by custom properties of a PartOrUsageRelatedSpecification.\n"@en;
        rdfs:label       "SpecificRole"@en;
        rdfs:subClassOf  vec:Role .

vec:WireAddOnType  rdf:type  owl:Class;
        rdfs:comment     "Specifies possible values for the t ype of wire add-ons (e.g. CavityAddOn ).┬á\n"@en;
        rdfs:label       "WireAddOnType"@en;
        rdfs:subClassOf  vec:OpenEnumeration .

vec:USUnitName_Chain  rdf:type  vec:USUnitName , owl:NamedIndividiual;
        vec:enumLiteral  "Chain" .

vec:personEmailAddress
        rdf:type      owl:DatatypeProperty;
        rdfs:comment  "Specifies the person's email address.\n"@en;
        rdfs:domain   vec:Person;
        rdfs:label    "emailAddress"@en;
        rdfs:range    xs:string .

vec:LanguageCode_Tg  rdf:type  vec:LanguageCode , owl:NamedIndividiual;
        vec:enumLiteral  "Tg" .

vec:LabelingRole  rdf:type  owl:Class;
        rdfs:comment     "If a component is labeled in its concrete usage, label informations are defined with the LabelingRole. "@en;
        rdfs:label       "LabelingRole"@en;
        rdfs:subClassOf  vec:Role .

vec:BoltTerminalSpecification
        rdf:type         owl:Class;
        rdfs:comment     "Specification for the definition of bolt terminals. These are the counterparts to ring terminals.\n"@en;
        rdfs:label       "BoltTerminalSpecification"@en;
        rdfs:subClassOf  vec:TerminalSpecification .

vec:PartStructureContentType_Module
        rdf:type         vec:PartStructureContentType , owl:NamedIndividiual;
        rdfs:comment     "A module /┬áoption in a customer specific or configurable harness (KSK┬á/┬áStufenleitungssatz). The content of a module is normally free of variance, but does not represent a functional subset on its own. (10%)\n"@en;
        vec:enumLiteral  "Module" .

vec:LanguageCode_Fj  rdf:type  vec:LanguageCode , owl:NamedIndividiual;
        vec:enumLiteral  "Fj" .

vec:permissionPermitter
        rdf:type            owl:ObjectProperty;
        rdfs:comment        "Specifies the person who was involved in the approval process giving a certain Permission.\n"@en;
        rdfs:domain         vec:Permission;
        rdfs:label          "permitter"@en;
        rdfs:range          vec:Person;
        rdfs:subPropertyOf  vec:contains .

vec:GrommetMountingType_Threading
        rdf:type         vec:GrommetMountingType , owl:NamedIndividiual;
        rdfs:comment     "The wires must threaded through the grommet."@en;
        vec:enumLiteral  "Threading" .

vec:SignalSubType  rdf:type  owl:Class;
        rdfs:label       "SignalSubType"@en;
        rdfs:subClassOf  vec:OpenEnumeration .

vec:WireReceptionType_UltraSonicWelding
        rdf:type         vec:WireReceptionType , owl:NamedIndividiual;
        vec:enumLiteral  "UltraSonicWelding" .

[ rdf:type     owl:AllDisjointClasses;
  owl:members  ( vec:CorrugatedPipeSpecification vec:ShrinkableTubeSpecification )
] .

vec:SiUnitName_Ampere
        rdf:type         vec:SiUnitName , owl:NamedIndividiual;
        vec:enumLiteral  "Ampere" .

vec:SignalCurve  rdf:type  owl:Class;
        rdfs:label       "SignalCurve"@en;
        rdfs:subClassOf  vec:OpenEnumeration .

vec:LocalizedStringProperty
        rdf:type         owl:Class;
        rdfs:label       "LocalizedStringProperty"@en;
        rdfs:subClassOf  vec:CustomProperty .

<http://www.prostep.org/ontologies/ecad/2024/03/vec#RobustnessClassReferenceSystem_LV%20312>
        rdf:type         vec:RobustnessClassReferenceSystem , owl:NamedIndividiual;
        rdfs:comment     "Protective systems for wiring harnesses in motor vehicles Hoses\n"@en;
        vec:enumLiteral  "LV 312" .

vec:cavityReferenceIdentification
        rdf:type      owl:DatatypeProperty;
        rdfs:comment  "Specifies a unique identification of the CavityReference. The identification is guaranteed to be unique within the ConnectorHousingRole. The cavity & slot number is defined by the associated cavity and slot.\n"@en;
        rdfs:domain   vec:CavityReference;
        rdfs:label    "identification"@en;
        rdfs:range    xs:string .

vec:TubeSlitStyle  rdf:type  owl:Class;
        rdfs:comment     "Defines valid types / styles of a slitted tube.\n"@en;
        rdfs:label       "TubeSlitStyle"@en;
        rdfs:subClassOf  vec:OpenEnumeration .

vec:SiUnitName_Hertz  rdf:type  vec:SiUnitName , owl:NamedIndividiual;
        vec:enumLiteral  "Hertz" .

vec:ImperialUnitName_Gallon
        rdf:type         vec:ImperialUnitName , owl:NamedIndividiual;
        vec:enumLiteral  "Gallon" .

vec:tapeRoleWindingType
        rdf:type            owl:ObjectProperty;
        rdfs:comment        "Defines the type of the tape's winding (see WindingType ).\n"@en;
        rdfs:domain         vec:TapeRole;
        rdfs:label          "windingType"@en;
        rdfs:range          vec:WindingType;
        rdfs:subPropertyOf  vec:contains .

vec:slotLayoutGridX  rdf:type  owl:ObjectProperty;
        rdfs:comment        "The horizontal distance between the center points of two cavities.\n"@en;
        rdfs:domain         vec:SlotLayout;
        rdfs:label          "gridX"@en;
        rdfs:range          vec:NumericalValue;
        rdfs:subPropertyOf  vec:contains .

vec:tapeSpecificationBacking
        rdf:type            owl:ObjectProperty;
        rdfs:comment        "Specifies the material of carrier of the tape, on which the adhesive material is applied.\n"@en;
        rdfs:domain         vec:TapeSpecification;
        rdfs:label          "backing"@en;
        rdfs:range          vec:Material;
        rdfs:subPropertyOf  vec:contains .

vec:SignalInformationType_Analog
        rdf:type         vec:SignalInformationType , owl:NamedIndividiual;
        vec:enumLiteral  "analog" .

vec:tubeSpecificationOuterDiameter
        rdf:type            owl:ObjectProperty;
        rdfs:comment        "Specifies the outer diameter of the tube. The outer diameter of a tube shall only be used for circular tubes (shape = Circular). For other shapes, height and width shall be used.\n"@en;
        rdfs:domain         vec:TubeSpecification;
        rdfs:label          "outerDiameter"@en;
        rdfs:range          vec:NumericalValue;
        rdfs:subPropertyOf  vec:contains .

vec:cavityHasIntegratedTerminal
        rdf:type      owl:DatatypeProperty;
        rdfs:comment  "Defines whether the cavity has an integrated terminal (for example an IDC cavity)┬áor if an additional terminal is required.\nIf this attribute is \"true\", the cavity can reference a TerminalSpecification as integratedTerminalSpecification in order to specify the integrated terminal.\n"@en;
        rdfs:domain   vec:Cavity;
        rdfs:label    "hasIntegratedTerminal"@en;
        rdfs:range    xs:boolean .

vec:HoleMountedFixingHoleShape_Circular
        rdf:type         vec:HoleMountedFixingHoleShape , owl:NamedIndividiual;
        vec:enumLiteral  "Circular" .

vec:PrimaryPartType_MultiCavityPlug
        rdf:type         vec:PrimaryPartType , owl:NamedIndividiual;
        vec:enumLiteral  "MultiCavityPlug" .

vec:cableDuctOutletIdentification
        rdf:type      owl:DatatypeProperty;
        rdfs:comment  "Specifies the identification of the Outlet. This must be unique within a CableDuctSpecification.\n"@en;
        rdfs:domain   vec:CableDuctOutlet;
        rdfs:label    "identification"@en;
        rdfs:range    xs:string .

vec:couplingPointIdentification
        rdf:type     owl:DatatypeProperty;
        rdfs:domain  vec:CouplingPoint;
        rdfs:label   "identification"@en;
        rdfs:range   xs:string .

vec:abstractSlotSlotNumber
        rdf:type      owl:DatatypeProperty;
        rdfs:comment  "Specifies the number of the slot. This must be unique within a ConnectorHousingSpecification.\n"@en;
        rdfs:domain   vec:AbstractSlot;
        rdfs:label    "slotNumber"@en;
        rdfs:range    xs:string .

vec:DefaultDimension  rdf:type  owl:Class;
        rdfs:comment  "A DefaultDimension defines a tolerance value that shall be applied to a part, if no explicit tolerance value has been defined.\n"@en;
        rdfs:label    "DefaultDimension"@en .

vec:cavityCouplingFirstCavity
        rdf:type     owl:ObjectProperty;
        rdfs:domain  vec:CavityCoupling;
        rdfs:label   "firstCavity"@en;
        rdfs:range   vec:CavityReference .

vec:VecVersion_1.1.2  rdf:type  vec:VecVersion , owl:NamedIndividiual;
        vec:enumLiteral  "1.1.2" .

vec:conductorSpecificationStrandDiameter
        rdf:type            owl:ObjectProperty;
        rdfs:comment        "Specifies the diameter of a single strand in the conductor.\n"@en;
        rdfs:domain         vec:ConductorSpecification;
        rdfs:label          "strandDiameter"@en;
        rdfs:range          vec:NumericalValue;
        rdfs:subPropertyOf  vec:contains .

vec:toleranceLowerBoundary
        rdf:type      owl:DatatypeProperty;
        rdfs:comment  "Specifies the lower boundary for the tolerance.\n"@en;
        rdfs:domain   vec:Tolerance;
        rdfs:label    "lowerBoundary"@en;
        rdfs:range    xs:double .

vec:SIUnit  rdf:type     owl:Class;
        rdfs:comment     "The SIUnit class can define quantities in the terms of the SI-Unit-System by specifying the corresponding SI prefix (optional) and a SI unit name. The usage of SI units must be the preferred way of expressing units, since these units can be easily translated into other SI units.\n"@en;
        rdfs:label       "SIUnit"@en;
        rdfs:subClassOf  vec:Unit .

vec:LabelingTechnology_PreCoded
        rdf:type         vec:LabelingTechnology , owl:NamedIndividiual;
        rdfs:comment     "In case precoded labels (e.g. RFID)."@en;
        vec:enumLiteral  "PreCoded" .

vec:configurableElementApplicationConstraint
        rdf:type        owl:ObjectProperty;
        rdfs:comment    ""@en , " Deprecated since VEC┬áV2.0.0. Use ConfigurationConstraints instead.\nReferences the application constraints that apply to the ConfigurableElement.\n"@en;
        rdfs:domain     vec:ConfigurableElement;
        rdfs:label      "applicationConstraint"@en;
        rdfs:range      vec:ApplicationConstraint;
        owl:deprecated  true .

vec:documentVersionCreatingSystem
        rdf:type      owl:DatatypeProperty;
        rdfs:comment  "The creatingSystem specifies the computer application or the machine which is used to create the document.\n"@en;
        rdfs:domain   vec:DocumentVersion;
        rdfs:label    "creatingSystem"@en;
        rdfs:range    xs:string .

vec:VecVersion_2.0.0  rdf:type  vec:VecVersion , owl:NamedIndividiual;
        vec:enumLiteral  "2.0.0" .

vec:LanguageCode_Tl  rdf:type  vec:LanguageCode , owl:NamedIndividiual;
        vec:enumLiteral  "Tl" .

vec:UsageNodeType_EnergyStorage
        rdf:type         vec:UsageNodeType , owl:NamedIndividiual;
        vec:enumLiteral  "EnergyStorage" .

vec:LanguageCode_Fo  rdf:type  vec:LanguageCode , owl:NamedIndividiual;
        vec:enumLiteral  "Fo" .

vec:modularSlotOptional
        rdf:type      owl:DatatypeProperty;
        rdfs:comment  "Specifies whether the allocation of the ModularSlot is optional or not (can a usage of the connector housing leave this ModularSlot empty.\n"@en;
        rdfs:domain   vec:ModularSlot;
        rdfs:label    "optional"@en;
        rdfs:range    xs:boolean .

[ rdf:type     owl:AllDisjointClasses;
  owl:members  ( vec:PlacementPointPosition vec:MeasurePointPosition )
] .

vec:    rdf:type        owl:Ontology;
        rdfs:comment    "\nThis file is provided under the terms of the MIT license reproduced here.\nCopyright ┬® 2021 prostep ivip association\n\nPermission is hereby granted, free of charge, to any person obtaining a copy of this software and associated documentation files (the \"Software\"), to deal in the Software without restriction, including without limitation the rights to use, copy, modify, merge, publish, distribute, sublicense, and/or sell copies of the Software, and to permit persons to whom the Software is furnished to do so, subject to the following conditions:\nThe above copyright notice and this permission notice shall be included in all copies or substantial portions of the Software.\nTHE SOFTWARE IS PROVIDED \"AS IS\", WITHOUT WARRANTY OF ANY KIND, EXPRESS OR IMPLIED, INCLUDING BUT NOT LIMITED TO THE WARRANTIES OF MERCHANTABILITY, FITNESS FOR A PARTICULAR PURPOSE AND NONINFRINGEMENT. IN NO EVENT SHALL THE AUTHORS OR COPYRIGHT HOLDERS BE LIABLE FOR ANY CLAIM, DAMAGES OR OTHER LIABILITY, WHETHER IN AN ACTION OF CONTRACT, TORT OR OTHERWISE, ARISING FROM, OUT OF OR IN CONNECTION WITH THE SOFTWARE OR THE USE OR OTHER DEALINGS IN THE SOFTWARE.\t\t\n\n---------------------------------------------------------------------------------------------------\n\nGenerated Ontology from VEC model. Changelog can be found at https://track.prostep.com/browse/KBLFRM.\nAttention: If this is a SNAPSHOT version, then this schema is produced by a nightly or preview build, \nis NO OFFICIAL RELEASE and can change at any time.\n\nVersion:   2.0.0\nRevision:  not-set\nTimestamp: not-set\n---------------------------------------------------------------------------------------------------                    \n                "@en;
        rdfs:label      "Vehicle Electric Container Ontology"@en;
        owl:versionIRI  <http://www.prostep.org/ontologies/ecad/2024/03/vec/2.0.0#> .

vec:tapeRoleWindingFirmness
        rdf:type            owl:ObjectProperty;
        rdfs:comment        "Defines the firmness of the tape's winding (see WindingFirmness).\n"@en;
        rdfs:domain         vec:TapeRole;
        rdfs:label          "windingFirmness"@en;
        rdfs:range          vec:WindingFirmness;
        rdfs:subPropertyOf  vec:contains .

vec:DiodeSpecification
        rdf:type         owl:Class;
        rdfs:comment     "Specification of the electrological aspects of a diode.\n"@en;
        rdfs:label       "DiodeSpecification"@en;
        rdfs:subClassOf  vec:EEComponentSpecification .

<http://www.prostep.org/ontologies/ecad/2024/03/vec#TerminalBoltNominalSize_%232>
        rdf:type         vec:TerminalBoltNominalSize , owl:NamedIndividiual;
        vec:enumLiteral  "#2" .

vec:NetViewSpecification
        rdf:type         owl:Class;
        rdfs:comment     "The NetViewSpecification supports the exchange of a basic layout for a NetSpecification .\n"@en;
        rdfs:label       "NetViewSpecification"@en;
        rdfs:subClassOf  vec:Specification .

vec:wireTupleSpecificationMaximumUntwistDualSided
        rdf:type            owl:ObjectProperty;
        rdfs:comment        "Specifies the maximum untwist for both sides together (A+B)."@en;
        rdfs:domain         vec:WireTupleSpecification;
        rdfs:label          "maximumUntwistDualSided"@en;
        rdfs:range          vec:NumericalValue;
        rdfs:subPropertyOf  vec:contains .

vec:WireLengthType  rdf:type  owl:Class;
        rdfs:comment     "Specifies possible values for the lengthType of WireLength .\n"@en;
        rdfs:label       "WireLengthType"@en;
        rdfs:subClassOf  vec:OpenEnumeration .

vec:buildingBlockSpecification2DGeometrySegment
        rdf:type            owl:ObjectProperty;
        rdfs:comment        "Specifies the GeometrySegment2Ds defined by the BuildingBlockSpecification2D.\n"@en;
        rdfs:domain         vec:BuildingBlockSpecification2D;
        rdfs:label          "geometrySegment"@en;
        rdfs:range          vec:GeometrySegment2D;
        rdfs:subPropertyOf  vec:contains .

vec:variantConfigurationLogisticControlString
        rdf:type      owl:DatatypeProperty;
        rdfs:comment  "Specifies a logisticControlString which can be used if the variant management is not done by boolean logic.\n"@en;
        rdfs:domain   vec:VariantConfiguration;
        rdfs:label    "logisticControlString"@en;
        rdfs:range    xs:string .

vec:SiPrefix_Micro  rdf:type  vec:SiPrefix , owl:NamedIndividiual;
        vec:enumLiteral  "Micro" .

vec:SignalSubType_NFC
        rdf:type         vec:SignalSubType , owl:NamedIndividiual;
        rdfs:comment     "Near Field Communication\n"@en;
        vec:enumLiteral  "NFC" .

vec:LanguageCode_Br  rdf:type  vec:LanguageCode , owl:NamedIndividiual;
        vec:enumLiteral  "Br" .

vec:boltMountedFixingSpecificationBoltShape
        rdf:type            owl:ObjectProperty;
        rdfs:comment        "Specifies the shape of the bolt on which the fixing can be mounted.\n"@en;
        rdfs:domain         vec:BoltMountedFixingSpecification;
        rdfs:label          "boltShape"@en;
        rdfs:range          vec:BoltMountedFixingBoltShape;
        rdfs:subPropertyOf  vec:contains .

vec:buildingBlockPositioning2DIdentification
        rdf:type      owl:DatatypeProperty;
        rdfs:comment  "Specifies a unique (optional) identification of the BuildingBlockPositioning2D. The identification is guaranteed to be unique within the HarnessDrawingSpecification2D.\n"@en;
        rdfs:domain   vec:BuildingBlockPositioning2D;
        rdfs:label    "identification"@en;
        rdfs:range    xs:string .

vec:dimensionDimensionAnchor
        rdf:type      owl:ObjectProperty;
        rdfs:comment  "References the location that is used as dimension point for the dimensioning (e.g. the entry point of a bundle into a connector housing).\nSee KBLFRM-329 and KBLFRM-391.\n"@en;
        rdfs:domain   vec:Dimension;
        rdfs:label    "dimensionAnchor"@en;
        rdfs:range    vec:DimensionAnchor .

vec:GeometrySegment2D
        rdf:type         owl:Class;
        rdfs:comment     "A GeometrySegment2D is the geometric representation of a TopologySegment in 2D-space.\n"@en;
        rdfs:label       "GeometrySegment2D"@en;
        rdfs:subClassOf  vec:GeometrySegment .

vec:defaultDimensionSpecificationDefaultDimension
        rdf:type            owl:ObjectProperty;
        rdfs:domain         vec:DefaultDimensionSpecification;
        rdfs:label          "defaultDimension"@en;
        rdfs:range          vec:DefaultDimension;
        rdfs:subPropertyOf  vec:contains .

vec:wireRoleWireSpecification
        rdf:type      owl:ObjectProperty;
        rdfs:comment  "References the WireSpecification that is instanced by this WireRole.\n"@en;
        rdfs:domain   vec:WireRole;
        rdfs:label    "wireSpecification"@en;
        rdfs:range    vec:WireSpecification .

vec:connectionIdentification
        rdf:type      owl:DatatypeProperty;
        rdfs:comment  "Specifies a unique identification of the Connection. The identification is guaranteed to be unique within the ConnectionSpecification.\n"@en;
        rdfs:domain   vec:Connection;
        rdfs:label    "identification"@en;
        rdfs:range    xs:string .

vec:BaselineState_Frozen
        rdf:type         vec:BaselineState , owl:NamedIndividiual;
        rdfs:comment     "Frozen means that the baseline is finalized and new ItemVersions must not be added without creating a new version of the baseline itself.\n"@en;
        vec:enumLiteral  "Frozen" .

vec:wireReceptionSpecificationSealable
        rdf:type      owl:DatatypeProperty;
        rdfs:comment  "Specifies if the wire reception can be sealed. (see KBLFRM-311)\n"@en;
        rdfs:domain   vec:WireReceptionSpecification;
        rdfs:label    "sealable"@en;
        rdfs:range    xs:boolean .

vec:moduleFamilyIdentification
        rdf:type      owl:DatatypeProperty;
        rdfs:comment  "Specifies a unique identification of the ModuleFamily. The identification is guaranteed to be unique within the ModuleFamilySpecification. For all VEC-documents a ModuleFamily-instance can be trusted to be the same if the ModuleFamilySpecification-instance is the same and the identification of the ModuleFamily is the same.\n"@en;
        rdfs:domain   vec:ModuleFamily;
        rdfs:label    "identification"@en;
        rdfs:range    xs:string .

vec:occurrenceOrUsageReferenceElement
        rdf:type      owl:ObjectProperty;
        rdfs:comment  "References the OccurrenceOrUsage for which this OccurrenceOrUsage is an accessory /┬ásupplementary component. If an OccurrenceOrUsage defines more than one referenceElement , the semantic is that it is related to the combination all \"reference elements\" and not to each individually. In other words, in a variable product definition the OccurrenceOrUsage only exists if all referenceElements exist.\n"@en;
        rdfs:domain   vec:OccurrenceOrUsage;
        rdfs:label    "referenceElement"@en;
        rdfs:range    vec:OccurrenceOrUsage .

[ rdf:type     owl:AllDisjointClasses;
  owl:members  ( vec:ContactPoint vec:RoutableElement vec:HousingComponent vec:PinComponent vec:PinComponentBehavior vec:InternalComponentConnection vec:SwitchingState vec:ExtensionSlot vec:BuildingBlockPositioning2D vec:BuildingBlockPositioning3D vec:OccurrenceOrUsage vec:HousingComponentReference vec:PinComponentReference vec:ExtensionSlotReference vec:MatingPoint vec:CouplingPoint vec:SlotCoupling vec:CavityCoupling vec:Net vec:NetGroup vec:NetworkNode vec:NetworkPort vec:Dimension vec:Placement vec:Routing vec:ComponentNode vec:ComponentPort vec:ConnectionEnd vec:ConnectionGroup vec:ComponentConnector vec:GeometryNode vec:GeometrySegment vec:TopologyNode vec:TopologySegment vec:TopologyZone vec:UsageNode )
] .

vec:TerminalBoltNominalSize_M3
        rdf:type         vec:TerminalBoltNominalSize , owl:NamedIndividiual;
        vec:enumLiteral  "M3" .

vec:potentialDistributorSpecificationBoltDiameter
        rdf:type            owl:ObjectProperty;
        rdfs:comment        "Specifies the diameter of the bolt for which the potential distributor is designed for.\n"@en;
        rdfs:domain         vec:PotentialDistributorSpecification;
        rdfs:label          "boltDiameter"@en;
        rdfs:range          vec:NumericalValue;
        rdfs:subPropertyOf  vec:contains .

vec:cableLeadThroughSpecificationSealingDimension
        rdf:type            owl:ObjectProperty;
        rdfs:comment        "Specifies the dimension of the cable lead through in the sealing area.\n"@en;
        rdfs:domain         vec:CableLeadThroughSpecification;
        rdfs:label          "sealingDimension"@en;
        rdfs:range          vec:Size;
        rdfs:subPropertyOf  vec:contains .

vec:ConnectorHousingSpecification
        rdf:type         owl:Class;
        rdfs:comment     "Specification for the definition of connector housings. A connector housing consists of a one or more slots. In the means of the VEC, a connector housing can be a conventional connector housing, a contact module or a connector shell.\n"@en;
        rdfs:label       "ConnectorHousingSpecification"@en;
        rdfs:subClassOf  vec:PartOrUsageRelatedSpecification .

vec:networkNodeViewItemOrientation
        rdf:type            owl:ObjectProperty;
        rdfs:comment        "Specifies the position /┬áplacement of the NetworkNodeViewItem within the layout."@en;
        rdfs:domain         vec:NetworkNodeViewItem;
        rdfs:label          "orientation"@en;
        rdfs:range          vec:Transformation2D;
        rdfs:subPropertyOf  vec:contains .

vec:TopologyGroupSpecification
        rdf:type         owl:Class;
        rdfs:comment     "A TopologyGroupSpecification defines a new Topology based on the grouped Topologies. (see KBLFRM-240)\n"@en;
        rdfs:label       "TopologyGroupSpecification"@en;
        rdfs:subClassOf  vec:TopologySpecification .

vec:VariantConfigurationType_Logistic
        rdf:type         vec:VariantConfigurationType , owl:NamedIndividiual;
        rdfs:comment     "The VariantConfiguration is a concrete logistic key (e.g. within a vehicle project) that used for example in order /┬ádelivery systems."@en;
        vec:enumLiteral  "Logistic" .

vec:LanguageCode_Hu  rdf:type  vec:LanguageCode , owl:NamedIndividiual;
        vec:enumLiteral  "Hu" .

vec:slotSpecificationLayoutType
        rdf:type            owl:ObjectProperty;
        rdfs:comment        "Specifies the layout of the slot from a mechanical /┬ágeometrical point of view.\n"@en;
        rdfs:domain         vec:SlotSpecification;
        rdfs:label          "layoutType"@en;
        rdfs:range          vec:SlotLayoutType;
        rdfs:subPropertyOf  vec:contains .

vec:CavityGeometry  rdf:type  owl:Class;
        rdfs:comment     "Defines valid values of the geometry of cavities in the sealing area (crimp end).\n"@en;
        rdfs:label       "CavityGeometry"@en;
        rdfs:subClassOf  vec:OpenEnumeration .

[ rdf:type     owl:AllDisjointClasses;
  owl:members  ( vec:TopologyGroupSpecification )
] .

<http://www.prostep.org/ontologies/ecad/2024/03/vec#RelaisType_Normally%20open>
        rdf:type         vec:RelaisType , owl:NamedIndividiual;
        rdfs:comment     ""@en;
        vec:enumLiteral  "normally open" .

vec:networkNodeViewItemIdentification
        rdf:type      owl:DatatypeProperty;
        rdfs:comment  "Specifies a unique identification of the NetworkNodeViewItem . The identification is guaranteed to be unique within the NetViewSpecification .\n"@en;
        rdfs:domain   vec:NetworkNodeViewItem;
        rdfs:label    "identification"@en;
        rdfs:range    xs:string .

vec:LanguageCode_Pt  rdf:type  vec:LanguageCode , owl:NamedIndividiual;
        vec:enumLiteral  "Pt" .

vec:creationCreator  rdf:type  owl:ObjectProperty;
        rdfs:comment        "Specifies the person who has created the Item.\n"@en;
        rdfs:domain         vec:Creation;
        rdfs:label          "creator"@en;
        rdfs:range          vec:Person;
        rdfs:subPropertyOf  vec:contains .

vec:WireLengthType_DMU
        rdf:type         vec:WireLengthType , owl:NamedIndividiual;
        rdfs:comment     "The length of the wire is calculated from the sum of the lengths of the neutral axes of the corresponding segments in the DMU model.\n"@en;
        vec:enumLiteral  "DMU" .

vec:placementIdentification
        rdf:type      owl:DatatypeProperty;
        rdfs:comment  "Specifies a unique identification of the Location. The identification is guaranteed to be unique within the PlacementSpecification.\n"@en;
        rdfs:domain   vec:Placement;
        rdfs:label    "identification"@en;
        rdfs:range    xs:string .

vec:DefaultDimensionSpecification
        rdf:type         owl:Class;
        rdfs:comment     "A DefaultDimensionSpecification defines tolerances that shall be applied to a part, if no explicit tolerance value has been defined.\n"@en;
        rdfs:label       "DefaultDimensionSpecification"@en;
        rdfs:subClassOf  vec:Specification .

vec:variantCodeDescription
        rdf:type            owl:ObjectProperty;
        rdfs:comment        "On optional human readable description of the variant code.\n"@en;
        rdfs:domain         vec:VariantCode;
        rdfs:label          "description"@en;
        rdfs:range          vec:AbstractLocalizedString;
        rdfs:subPropertyOf  vec:contains .

vec:TerminalBoltType_MetricThread
        rdf:type         vec:TerminalBoltType , owl:NamedIndividiual;
        rdfs:comment     "A bolt with a metric scale thread.\n"@en;
        vec:enumLiteral  "MetricThread" .

vec:SignalSubType_PowerGround
        rdf:type         vec:SignalSubType , owl:NamedIndividiual;
        vec:enumLiteral  "PowerGround" .

vec:ApplicationConstraintType_Allow
        rdf:type         vec:ApplicationConstraintType , owl:NamedIndividiual;
        vec:enumLiteral  "Allow" .

vec:ImperialUnitName_Thou
        rdf:type         vec:ImperialUnitName , owl:NamedIndividiual;
        vec:enumLiteral  "Thou" .

vec:soundDampingClassClassKey
        rdf:type      owl:DatatypeProperty;
        rdfs:comment  "Specifies a key for the level defined in the sound damping class (e.g. A, B, C).\n"@en;
        rdfs:domain   vec:SoundDampingClass;
        rdfs:label    "classKey"@en;
        rdfs:range    xs:string .

vec:NominalVoltage_12V
        rdf:type         vec:NominalVoltage , owl:NamedIndividiual;
        vec:enumLiteral  "12V" .

vec:FuseType_MITOX  rdf:type  vec:FuseType , owl:NamedIndividiual;
        vec:enumLiteral  "MITOX" .

vec:variantStructureNodeDescription
        rdf:type            owl:ObjectProperty;
        rdfs:comment        "On optional human readable description of the VariantStructureNode .\n"@en;
        rdfs:domain         vec:VariantStructureNode;
        rdfs:label          "description"@en;
        rdfs:range          vec:AbstractLocalizedString;
        rdfs:subPropertyOf  vec:contains .

vec:LanguageCode_Ru  rdf:type  vec:LanguageCode , owl:NamedIndividiual;
        vec:enumLiteral  "Ru" .

vec:ModularSlotAddOn  rdf:type  owl:Class;
        rdfs:comment  "Specifies the wire addon needed to reach a ModularSlot from a specific SegmentConnectionPoint . The addon needed to reach the cavities of the insert(s) from this point is defined by the ConnectorHousingSpecification of the insert.\n"@en;
        rdfs:label    "ModularSlotAddOn"@en .

vec:externalMappingSpecificationMappings
        rdf:type            owl:ObjectProperty;
        rdfs:comment        "Specifies the mappings of individual element.\n"@en;
        rdfs:domain         vec:ExternalMappingSpecification;
        rdfs:label          "mappings"@en;
        rdfs:range          vec:ExternalMapping;
        rdfs:subPropertyOf  vec:contains .

vec:localGeometrySpecificationPositions
        rdf:type            owl:ObjectProperty;
        rdfs:comment        "All position defined by this LocalGeometrySpecification.\n"@en;
        rdfs:domain         vec:LocalGeometrySpecification;
        rdfs:label          "positions"@en;
        rdfs:range          vec:LocalPosition;
        rdfs:subPropertyOf  vec:contains .

vec:generalTechnicalPartSpecificationPartRelation
        rdf:type            owl:ObjectProperty;
        rdfs:comment        "Specifies possible relations (accessories) of the specified part with other PartVersion (e.g. caps, clips). "@en;
        rdfs:domain         vec:GeneralTechnicalPartSpecification;
        rdfs:label          "partRelation"@en;
        rdfs:range          vec:PartRelation;
        rdfs:subPropertyOf  vec:contains .

vec:matingDetailConnection
        rdf:type      owl:ObjectProperty;
        rdfs:comment  "References the Connection that is realized by this MatingPointDetail . For example, when a connection is realized by directly plugging or screwing two E/E components together.\nThe definition at level of the MatingDetail might be required if the TerminalRole of the MatingPoint carries multiple different potentials (e.g. Coax).\n"@en;
        rdfs:domain   vec:MatingDetail;
        rdfs:label    "connection"@en;
        rdfs:range    vec:Connection .

vec:LabelType_QRCode  rdf:type  vec:LabelType , owl:NamedIndividiual;
        vec:enumLiteral  "QRCode" .

vec:wireMountingReferencedWireEnd
        rdf:type      owl:ObjectProperty;
        rdfs:comment  "References the wire ends that are used for the wire mounting. The minimum cardinality is one, because a wire mounting without wire end makes no sense.\nThe maximum cardinality is * in order to support multi crimps.\n"@en;
        rdfs:domain   vec:WireMounting;
        rdfs:label    "referencedWireEnd"@en;
        rdfs:range    vec:WireEnd .

vec:pinWireMappingPointPinComponentReference
        rdf:type     owl:ObjectProperty;
        rdfs:domain  vec:PinWireMappingPoint;
        rdfs:label   "pinComponentReference"@en;
        rdfs:range   vec:PinComponentReference .

vec:SlotLayoutType_Type_SF30
        rdf:type         vec:SlotLayoutType , owl:NamedIndividiual;
        rdfs:comment     "Fuse type according to ISO8820, also known as: midi\n"@en;
        vec:enumLiteral  "Type_SF30" .

vec:variantGroupIdentification
        rdf:type      owl:DatatypeProperty;
        rdfs:comment  "Specifies a unique identification of the variant code.\n"@en;
        rdfs:domain   vec:VariantGroup;
        rdfs:label    "identification"@en;
        rdfs:range    xs:string .

vec:VariantConfigurationSpecification
        rdf:type         owl:Class;
        rdfs:comment     "Specification for the definition of variant configurations.\n"@en;
        rdfs:label       "VariantConfigurationSpecification"@en;
        rdfs:subClassOf  vec:Specification .

vec:partVersionPreferredUseCase
        rdf:type            owl:ObjectProperty;
        rdfs:comment        "Contains a part description from the point of view of the preferred use case. Defines the function for which the part was initially designed. (e.g. \"Grommet for Hatch\", \"...passenger compartment\"). This can be an important information for searching and selecting parts.\n"@en;
        rdfs:domain         vec:PartVersion;
        rdfs:label          "preferredUseCase"@en;
        rdfs:range          vec:LocalizedString;
        rdfs:subPropertyOf  vec:contains .

vec:ConnectorOutletDirection_Angled
        rdf:type         vec:ConnectorOutletDirection , owl:NamedIndividiual;
        vec:enumLiteral  "Angled" .

vec:LanguageCode_Fy  rdf:type  vec:LanguageCode , owl:NamedIndividiual;
        vec:enumLiteral  "Fy" .

vec:SiUnitName_Gray  rdf:type  vec:SiUnitName , owl:NamedIndividiual;
        vec:enumLiteral  "Gray" .

vec:wireTupleTerminationFixationOffset
        rdf:type            owl:ObjectProperty;
        rdfs:comment        "Specifies the offset of the fixation."@en;
        rdfs:domain         vec:WireTupleTermination;
        rdfs:label          "fixationOffset"@en;
        rdfs:range          vec:NumericalValue;
        rdfs:subPropertyOf  vec:contains .

vec:CableLeadThroughType_Foamed
        rdf:type         vec:CableLeadThroughType , owl:NamedIndividiual;
        vec:enumLiteral  "Foamed" .

vec:TerminalBoltNominalSize_M8
        rdf:type         vec:TerminalBoltNominalSize , owl:NamedIndividiual;
        vec:enumLiteral  "M8" .

vec:BoltMountedFixingBoltType_ImperialThread
        rdf:type         vec:BoltMountedFixingBoltType , owl:NamedIndividiual;
        rdfs:comment     "A bolt with a imperial scale thread.\n"@en;
        vec:enumLiteral  "ImperialThread" .

vec:transformation2DA21
        rdf:type     owl:DatatypeProperty;
        rdfs:domain  vec:Transformation2D;
        rdfs:label   "a21"@en;
        rdfs:range   xs:double .

vec:ConductorType_Rigid
        rdf:type         vec:ConductorType , owl:NamedIndividiual;
        rdfs:comment     "Used for conductors that are made of solid material.\n"@en;
        vec:enumLiteral  "Rigid" .

vec:wireRoleWireElementReference
        rdf:type            owl:ObjectProperty;
        rdfs:comment        "Specifies the WireElementReferences used in the WireRole. For multi core wires more than one WireElementReference is needed. \n"@en;
        rdfs:domain         vec:WireRole;
        rdfs:label          "wireElementReference"@en;
        rdfs:range          vec:WireElementReference;
        rdfs:subPropertyOf  vec:contains .

vec:SlotLayoutType_Type_SF51
        rdf:type         vec:SlotLayoutType , owl:NamedIndividiual;
        rdfs:comment     "Fuse type according to ISO8820, also known as: mega\n"@en;
        vec:enumLiteral  "Type_SF51" .

vec:batterySpecificationU
        rdf:type            owl:ObjectProperty;
        rdfs:comment        "Specifies the nominal voltage of the battery.\n"@en;
        rdfs:domain         vec:BatterySpecification;
        rdfs:label          "u"@en;
        rdfs:range          vec:NumericalValue;
        rdfs:subPropertyOf  vec:contains .

vec:customPropertyPropertyType
        rdf:type     owl:DatatypeProperty;
        rdfs:domain  vec:CustomProperty;
        rdfs:label   "propertyType"@en;
        rdfs:range   xs:string .

vec:RelaisApplianceType_Soldered
        rdf:type         vec:RelaisApplianceType , owl:NamedIndividiual;
        vec:enumLiteral  "soldered" .

vec:cavityPartSpecificationCompatibleTerminalType
        rdf:type            owl:ObjectProperty;
        rdfs:comment        "Defines a list of terminal types that are compatible to this CavitySealSpecification. This defines as well the compatible cavities, since a plug is normally used when no terminals are present.\n"@en;
        rdfs:domain         vec:CavityPartSpecification;
        rdfs:label          "compatibleTerminalType"@en;
        rdfs:range          vec:TerminalType;
        rdfs:subPropertyOf  vec:contains .

vec:SignalSubType_FBAS
        rdf:type         vec:SignalSubType , owl:NamedIndividiual;
        vec:enumLiteral  "FBAS" .

vec:specificationDescription
        rdf:type            owl:ObjectProperty;
        rdfs:comment        "Specifies additional, human readable information about the specification.\n"@en;
        rdfs:domain         vec:Specification;
        rdfs:label          "description"@en;
        rdfs:range          vec:AbstractLocalizedString;
        rdfs:subPropertyOf  vec:contains .

vec:cavitySpecificationGeometry
        rdf:type            owl:ObjectProperty;
        rdfs:comment        "Defines the geometry of a cavity in the sealing area (crimp end).\n"@en;
        rdfs:domain         vec:CavitySpecification;
        rdfs:label          "geometry"@en;
        rdfs:range          vec:CavityGeometry;
        rdfs:subPropertyOf  vec:contains .

vec:tubeSpecificationIsSlit
        rdf:type      owl:DatatypeProperty;
        rdfs:comment  "Specifies whether the tube is slit or not. The style of the slitting can be defined with the slitStyle. If a slitStyle is defined, it implies that isSlit=true .\n"@en;
        rdfs:domain   vec:TubeSpecification;
        rdfs:label    "isSlit"@en;
        rdfs:range    xs:boolean .

vec:cableDuctSpecificationOutlet
        rdf:type            owl:ObjectProperty;
        rdfs:comment        ""@en;
        rdfs:domain         vec:CableDuctSpecification;
        rdfs:label          "outlet"@en;
        rdfs:range          vec:CableDuctOutlet;
        rdfs:subPropertyOf  vec:contains .

vec:USUnitName_Inch  rdf:type  vec:USUnitName , owl:NamedIndividiual;
        vec:enumLiteral  "Inch" .

vec:fittingOutletIdentification
        rdf:type      owl:DatatypeProperty;
        rdfs:comment  "Specifies the identification of the Outlet. This must be unique within a FittingSpecification.\n"@en;
        rdfs:domain   vec:FittingOutlet;
        rdfs:label    "identification"@en;
        rdfs:range    xs:string .

vec:eEComponentSpecificationConnections
        rdf:type            owl:ObjectProperty;
        rdfs:domain         vec:EEComponentSpecification;
        rdfs:label          "connections"@en;
        rdfs:range          vec:InternalComponentConnection;
        rdfs:subPropertyOf  vec:contains .

vec:PlaceableElementRole
        rdf:type         owl:Class;
        rdfs:comment     "A PlaceableElementRole defines the instance specific properties and relationships of a PlaceableElement.\n"@en;
        rdfs:label       "PlaceableElementRole"@en;
        rdfs:subClassOf  vec:Role .

vec:boltTerminalSpecificationBoltNominalSize
        rdf:type            owl:ObjectProperty;
        rdfs:comment        "Defines the size (diameter) of the bolt in a nominal way (e.g. \"M8\").\n"@en;
        rdfs:domain         vec:BoltTerminalSpecification;
        rdfs:label          "boltNominalSize"@en;
        rdfs:range          vec:TerminalBoltNominalSize;
        rdfs:subPropertyOf  vec:contains .

vec:RelaisApplianceType
        rdf:type         owl:Class;
        rdfs:comment     "Specifies the appliance type of a relais.\n"@en;
        rdfs:label       "RelaisApplianceType"@en;
        rdfs:subClassOf  vec:OpenEnumeration .

vec:WireElementShape_Circular
        rdf:type         vec:WireElementShape , owl:NamedIndividiual;
        vec:enumLiteral  "Circular" .

vec:PrimaryPartType_Fitting
        rdf:type         vec:PrimaryPartType , owl:NamedIndividiual;
        vec:enumLiteral  "Fitting" .

vec:TerminalBoltNominalSize_M20
        rdf:type         vec:TerminalBoltNominalSize , owl:NamedIndividiual;
        vec:enumLiteral  "M20" .

vec:WireLengthType_Drawing
        rdf:type         vec:WireLengthType , owl:NamedIndividiual;
        rdfs:comment     "The length is rounded length from the DMU model (shown on the drawing), without any add-ons\n"@en;
        vec:enumLiteral  "Drawing" .

vec:terminalReceptionSpecificationPlatingMaterial
        rdf:type            owl:ObjectProperty;
        rdfs:comment        "Specifies the plating material of the terminal reception.\n"@en;
        rdfs:domain         vec:TerminalReceptionSpecification;
        rdfs:label          "platingMaterial"@en;
        rdfs:range          vec:Material;
        rdfs:subPropertyOf  vec:contains .

vec:signalDataRate  rdf:type  owl:ObjectProperty;
        rdfs:comment        "Defines the data rate of the signal. This applies only to signals with signalType = 'information ' and signalInformationType = 'digital' . For the numerical value, an appropriate IECUnit combination shall be used (e.g. GBit┬á/┬áSecond).\n"@en;
        rdfs:domain         vec:Signal;
        rdfs:label          "dataRate"@en;
        rdfs:range          vec:NumericalValue;
        rdfs:subPropertyOf  vec:contains .

vec:FuseType  rdf:type   owl:Class;
        rdfs:comment     "Defines the values for the type a fuse. This is the geometrical type.\n"@en;
        rdfs:label       "FuseType"@en;
        rdfs:subClassOf  vec:OpenEnumeration .

vec:PrimaryPartType_Diode
        rdf:type         vec:PrimaryPartType , owl:NamedIndividiual;
        vec:enumLiteral  "Diode" .

vec:terminalRoleTerminalSpecification
        rdf:type      owl:ObjectProperty;
        rdfs:comment  "┬áReferences the TerminalSpecification that is instanced by this TerminalRole.\n"@en;
        rdfs:domain   vec:TerminalRole;
        rdfs:label    "terminalSpecification"@en;
        rdfs:range    vec:TerminalSpecification .

vec:wireReceptionSpecificationPlatingMaterial
        rdf:type            owl:ObjectProperty;
        rdfs:comment        "Specifies the plating material of the wire reception.\n"@en;
        rdfs:domain         vec:WireReceptionSpecification;
        rdfs:label          "platingMaterial"@en;
        rdfs:range          vec:Material;
        rdfs:subPropertyOf  vec:contains .

vec:sheetOrChapterIdentification
        rdf:type      owl:DatatypeProperty;
        rdfs:comment  "The identification of the sheet or chapter within the document. This value must be distinct within the context of a document.\n"@en;
        rdfs:domain   vec:SheetOrChapter;
        rdfs:label    "identification"@en;
        rdfs:range    xs:string .

vec:variantConfigurationDescription
        rdf:type            owl:ObjectProperty;
        rdfs:comment        "On optional human readable description of the variant configuration.\n"@en;
        rdfs:domain         vec:VariantConfiguration;
        rdfs:label          "description"@en;
        rdfs:range          vec:AbstractLocalizedString;
        rdfs:subPropertyOf  vec:contains .

vec:tapeRoleTapeOverlap
        rdf:type            owl:ObjectProperty;
        rdfs:comment        "Specifies the amount of overlap two rounds of taping around a segment have, as an absolute value. A negative value means, that there is a gap between two rounds.\n"@en;
        rdfs:domain         vec:TapeRole;
        rdfs:label          "tapeOverlap"@en;
        rdfs:range          vec:NumericalValue;
        rdfs:subPropertyOf  vec:contains .

vec:cableTieSpecificationWidth
        rdf:type            owl:ObjectProperty;
        rdfs:domain         vec:CableTieSpecification;
        rdfs:label          "width"@en;
        rdfs:range          vec:NumericalValue;
        rdfs:subPropertyOf  vec:contains .

vec:locationPlacedPlacementPoints
        rdf:type      owl:ObjectProperty;
        rdfs:comment  "References the PlacementPointReference that is placed by this location.\n"@en;
        rdfs:domain   vec:Location;
        rdfs:label    "placedPlacementPoints"@en;
        rdfs:range    vec:PlacementPointReference .

vec:SealedCavitiesAssignment
        rdf:type      owl:Class;
        rdfs:comment  "A SealedCavitiesAssignment groups the cavities of ONE connector that are sealed by a MultiCavityPlug. If a MultiCavityPlug fits into more than one connector, than there are as many SealedCavitiesAssignments .\n"@en;
        rdfs:label    "SealedCavitiesAssignment"@en .

vec:variantGroupSpecificationVariantGroup
        rdf:type            owl:ObjectProperty;
        rdfs:comment        "Specifies the individual VariantGroups defined in the VariantGroupSpecification.\n"@en;
        rdfs:domain         vec:VariantGroupSpecification;
        rdfs:label          "variantGroup"@en;
        rdfs:range          vec:VariantGroup;
        rdfs:subPropertyOf  vec:contains .

vec:cartesianPoint3DZ
        rdf:type      owl:DatatypeProperty;
        rdfs:comment  "Specifies the value of z-coordinate of the Cartesian point. The unit of this value is the baseUnit of containing BuildingBlockSpecification3D.\n"@en;
        rdfs:domain   vec:CartesianPoint3D;
        rdfs:label    "z"@en;
        rdfs:range    xs:double .

vec:wireReceptionSpecificationCoreCrossSectionArea
        rdf:type            owl:ObjectProperty;
        rdfs:comment        "Specifies a value range for cross-section areas of cores that are compatible with the wire reception.\nFor wire receptions where a single core is attached to, this value defines the ValueRange of the crossSectionArea of the core. For wire receptions where more than one core is attached to (e.g. ring terminals, splices), this attribute defines the valid value range for the sum of the cross-section areas of all attached cores.\n"@en;
        rdfs:domain         vec:WireReceptionSpecification;
        rdfs:label          "coreCrossSectionArea"@en;
        rdfs:range          vec:ValueRange;
        rdfs:subPropertyOf  vec:contains .

vec:wireElementReferenceConnectionGroup
        rdf:type      owl:ObjectProperty;
        rdfs:comment  "References the ConnectionGroup that is realized by this WireElementReference. This applies normally to WireElementReference that have subWireElements .\n"@en;
        rdfs:domain   vec:WireElementReference;
        rdfs:label    "connectionGroup"@en;
        rdfs:range    vec:ConnectionGroup .

vec:ModularSlot  rdf:type  owl:Class;
        rdfs:comment     "A ModularSlot is a place in a connector housing where different other connector housings can be placed during the assembly (e.g. by clicking them into the connector housing).\n"@en;
        rdfs:label       "ModularSlot"@en;
        rdfs:subClassOf  vec:AbstractSlot .

vec:USUnitName_Pint  rdf:type  vec:USUnitName , owl:NamedIndividiual;
        vec:enumLiteral  "Pint" .

vec:applicationConstraintProjectPhase
        rdf:type      owl:DatatypeProperty;
        rdfs:comment  "Specifies the project phases to which the application constraint applies.\n"@en;
        rdfs:domain   vec:ApplicationConstraint;
        rdfs:label    "projectPhase"@en;
        rdfs:range    xs:string .

vec:MappingSpecification
        rdf:type         owl:Class;
        rdfs:comment     "Specification for the description of a PinMapping. A PinMapping allows the mapping between the Cavities of two independent ConnectorHousingSpecifications. This is for example needed to determine the Mating for an Inliner or for the Mating between an EE-Component and a ConnectorHousing. The PinMapping is a part master data.\n"@en;
        rdfs:label       "MappingSpecification"@en;
        rdfs:subClassOf  vec:Specification .

vec:signalSignalForm  rdf:type  owl:ObjectProperty;
        rdfs:comment        "Specifies the form of the signal.\n"@en;
        rdfs:domain         vec:Signal;
        rdfs:label          "signalForm"@en;
        rdfs:range          vec:SignalForm;
        rdfs:subPropertyOf  vec:contains .

vec:imperialUnitImperialUnitName
        rdf:type            owl:ObjectProperty;
        rdfs:comment        "Specifies the name of the imperial unit.\n"@en;
        rdfs:domain         vec:ImperialUnit;
        rdfs:label          "imperialUnitName"@en;
        rdfs:range          vec:ImperialUnitName;
        rdfs:subPropertyOf  vec:contains .

vec:LanguageCode_Aa  rdf:type  vec:LanguageCode , owl:NamedIndividiual;
        rdfs:comment     "Afar\n"@en;
        vec:enumLiteral  "Aa" .

vec:SiPrefix  rdf:type       owl:Class;
        rdfs:comment         "Enumeration for the definition of SI unit prefixes.\n"@en;
        rdfs:label           "SiPrefix"@en;
        rdfs:subClassOf      vec:ClosedEnumeration;
        owl:equivalentClass  [ rdf:type   owl:Class;
                               owl:oneOf  ( vec:SiPrefix_Yotta vec:SiPrefix_Zetta vec:SiPrefix_Exa vec:SiPrefix_Peta vec:SiPrefix_Tera vec:SiPrefix_Giga vec:SiPrefix_Mega vec:SiPrefix_Kilo vec:SiPrefix_Hecto vec:SiPrefix_Deca vec:SiPrefix_Deci vec:SiPrefix_Centi vec:SiPrefix_Milli vec:SiPrefix_Micro vec:SiPrefix_Nano vec:SiPrefix_Pico vec:SiPrefix_Femto vec:SiPrefix_Atto vec:SiPrefix_Zepto vec:SiPrefix_Yocto )
                             ] .

vec:IECPrefix_Mebi  rdf:type  vec:IECPrefix , owl:NamedIndividiual;
        vec:enumLiteral  "Mebi" .

vec:partOrUsageRelatedSpecificationDescribedPart
        rdf:type      owl:ObjectProperty;
        rdfs:comment  "References the PartVersion(s) to which the information defined in this specification applies.\nExample: If the PartOrUsageRelatedSpecification is a GeneralTechnicalPartSpecifcation and it defines that the color is \"green\" then all PartVersion referenced by this association are \"green\".\n"@en;
        rdfs:domain   vec:PartOrUsageRelatedSpecification;
        rdfs:label    "describedPart"@en;
        rdfs:range    vec:PartVersion .

vec:ColorReferenceSystem_RGB
        rdf:type         vec:ColorReferenceSystem , owl:NamedIndividiual;
        vec:enumLiteral  "RGB" .

vec:wireElementReferenceReferencedWireElement
        rdf:type      owl:ObjectProperty;
        rdfs:comment  "References the WireElement that is represented by the WireElementReference.\n"@en;
        rdfs:domain   vec:WireElementReference;
        rdfs:label    "referencedWireElement"@en;
        rdfs:range    vec:WireElement .

vec:TerminalBoltType  rdf:type  owl:Class;
        rdfs:comment     "Open Enumeration to define different types of bolts for bolt /┬áring terminals."@en;
        rdfs:label       "TerminalBoltType"@en;
        rdfs:subClassOf  vec:OpenEnumeration .

vec:NominalVoltage_HV2
        rdf:type         vec:NominalVoltage , owl:NamedIndividiual;
        rdfs:comment     "HV Class 2 (300V┬áDC)\n"@en;
        vec:enumLiteral  "HV2" .

vec:spliceTerminalRoleInsulationState
        rdf:type            owl:ObjectProperty;
        rdfs:comment        "Specifies the insulation state of the splice, in other words is electrically insulated or not.\n"@en;
        rdfs:domain         vec:SpliceTerminalRole;
        rdfs:label          "insulationState"@en;
        rdfs:range          vec:InsulationState;
        rdfs:subPropertyOf  vec:contains .

vec:slotCouplingSecondSlot
        rdf:type     owl:ObjectProperty;
        rdfs:domain  vec:SlotCoupling;
        rdfs:label   "secondSlot"@en;
        rdfs:range   vec:AbstractSlotReference .

vec:geometrySegment2DPathSegment
        rdf:type            owl:ObjectProperty;
        rdfs:comment        "Specifies an ordered list of PathSegments that describe the appearance of the GeometrySegment2D. The appearance is described by the concatenation of the PathSegments beginning at the startNode of the GeometrySegment2D.\n"@en;
        rdfs:domain         vec:GeometrySegment2D;
        rdfs:label          "pathSegment"@en;
        rdfs:range          vec:PathSegment , vec:Ordered;
        rdfs:subPropertyOf  vec:contains .

vec:GrommetType_ConnectorCover
        rdf:type         vec:GrommetType , owl:NamedIndividiual;
        vec:enumLiteral  "ConnectorCover" .

vec:LanguageCode_Ka  rdf:type  vec:LanguageCode , owl:NamedIndividiual;
        vec:enumLiteral  "Ka" .

vec:labelingRoleLabelingSpecification
        rdf:type     owl:ObjectProperty;
        rdfs:domain  vec:LabelingRole;
        rdfs:label   "labelingSpecification"@en;
        rdfs:range   vec:LabelingSpecification .

vec:pinComponentReferenceTerminalRole
        rdf:type            owl:ObjectProperty;
        rdfs:comment        "References the TerminalRole of PinComponentReference. This is required to specify a Mating for EEComponents with other EEComponents or a Harness. \n(KBLFRM-401)\n"@en;
        rdfs:domain         vec:PinComponentReference;
        rdfs:label          "terminalRole"@en;
        rdfs:range          vec:TerminalRole;
        rdfs:subPropertyOf  vec:contains .

vec:generalTechnicalPartSpecificationRobustnessProperties
        rdf:type            owl:ObjectProperty;
        rdfs:comment        "Specifies the robustness of a part.\n"@en;
        rdfs:domain         vec:GeneralTechnicalPartSpecification;
        rdfs:label          "robustnessProperties"@en;
        rdfs:range          vec:RobustnessProperties;
        rdfs:subPropertyOf  vec:contains .

vec:slotSpecificationSecondaryLocking
        rdf:type      owl:DatatypeProperty;
        rdfs:comment  "Specifies whether the slot supports secondary locking.\n"@en;
        rdfs:domain   vec:SlotSpecification;
        rdfs:label    "secondaryLocking"@en;
        rdfs:range    xs:boolean .

vec:cartesianVector2DY
        rdf:type      owl:DatatypeProperty;
        rdfs:comment  "Specifies the y-coordinate in 2D space.\n"@en;
        rdfs:domain   vec:CartesianVector2D;
        rdfs:label    "y"@en;
        rdfs:range    xs:double .

vec:segmentLengthLength
        rdf:type            owl:ObjectProperty;
        rdfs:comment        "Specifies the length of the TopologySegment.\n"@en;
        rdfs:domain         vec:SegmentLength;
        rdfs:label          "length"@en;
        rdfs:range          vec:NumericalValue;
        rdfs:subPropertyOf  vec:contains .

vec:SlotSealingType  rdf:type  owl:Class;
        rdfs:comment     "Defines the possible sealing types for a slot, if the slot shall be sealed in its usage.\n"@en;
        rdfs:label       "SlotSealingType"@en;
        rdfs:subClassOf  vec:OpenEnumeration .

vec:contractCompanyName
        rdf:type      owl:DatatypeProperty;
        rdfs:comment  "Specifies the company which acts in the specified Role in the Contract Relationship.\n"@en;
        rdfs:domain   vec:Contract;
        rdfs:label    "companyName"@en;
        rdfs:range    xs:string .

vec:networkNodeViewItemDisplayedPort
        rdf:type            owl:ObjectProperty;
        rdfs:comment        "Specifies all NetworkPortViewItems that are displayed on this NetworkNodeViewItem. The order of this association defines the clockwise arrangement of the ports on the node. As each NetworkPortViewItem can also define the side on which it is placed, side definitions take precedence over order. ┬á Caution: This association is ordered ! ┬á\n"@en;
        rdfs:domain         vec:NetworkNodeViewItem;
        rdfs:label          "displayedPort"@en;
        rdfs:range          vec:NetworkPortViewItem , vec:Ordered;
        rdfs:subPropertyOf  vec:contains .

vec:occurrenceOrUsageRole
        rdf:type            owl:ObjectProperty;
        rdfs:comment        "Specifies the different roles of the OccurrenceOrUsage.\n"@en;
        rdfs:domain         vec:OccurrenceOrUsage;
        rdfs:label          "role"@en;
        rdfs:range          vec:Role;
        rdfs:subPropertyOf  vec:contains .

vec:internalTerminalConnectionWireReception
        rdf:type      owl:ObjectProperty;
        rdfs:comment  "References the WireReceptions that participate in the InternalTerminalConnection.\n"@en;
        rdfs:domain   vec:InternalTerminalConnection;
        rdfs:label    "wireReception"@en;
        rdfs:range    vec:WireReception .

vec:BoltMountedFixingBoltType_Plain
        rdf:type         vec:BoltMountedFixingBoltType , owl:NamedIndividiual;
        rdfs:comment     "A plain bolt without an special features.\n"@en;
        vec:enumLiteral  "Plain" .

vec:SiUnitName_Becquerel
        rdf:type         vec:SiUnitName , owl:NamedIndividiual;
        vec:enumLiteral  "Becquerel" .

vec:FunctionalRequirementType_Crash
        rdf:type         vec:FunctionalRequirementType , owl:NamedIndividiual;
        rdfs:comment     "Crash requirements e.g. post-crash functionality.\n┬á\n"@en;
        vec:enumLiteral  "Crash" .

vec:wireMountingWireMountingDetail
        rdf:type            owl:ObjectProperty;
        rdfs:comment        "Specifies the WireMoutingDetails, if a detailed description of the relationships between WireEnds and WireReceptions is needed.\n"@en;
        rdfs:domain         vec:WireMounting;
        rdfs:label          "wireMountingDetail"@en;
        rdfs:range          vec:WireMountingDetail;
        rdfs:subPropertyOf  vec:contains .

vec:connectionNodeViewItemOrientation
        rdf:type            owl:ObjectProperty;
        rdfs:comment        "Specifies the position /┬áplacement of the ConnectionNodeViewItem within the layout."@en;
        rdfs:domain         vec:ConnectionNodeViewItem;
        rdfs:label          "orientation"@en;
        rdfs:range          vec:Transformation2D;
        rdfs:subPropertyOf  vec:contains .

vec:partVersionPartNumber
        rdf:type      owl:DatatypeProperty;
        rdfs:comment  "The partNumber is the major identifier of a PartVersion. The format is user defined and respectively company specific. For all VEC-documents a PartVersion-instance can be trusted to be identical if the combination of partNumber, partVersion and companyName is identical.\n"@en;
        rdfs:domain   vec:PartVersion;
        rdfs:label    "partNumber"@en;
        rdfs:range    xs:string .

vec:pathSegment  rdf:type   owl:ObjectProperty;
        rdfs:comment        "This association is defined as unique='false' and ordered='true'. This can not be represented efficiently directly in RDF/OWL. Therefore, this association references Wrappers as proxies to the actual elements, instead of the actual elements itself (like a regular association)." , "Specifies an ordered list of TopologySegments the routing goes through. \n"@en;
        rdfs:domain         vec:Path;
        rdfs:label          "segment"@en;
        rdfs:range          vec:TopologySegmentWrapper , vec:Ordered;
        rdfs:subPropertyOf  vec:contains .

vec:LanguageCode_Gd  rdf:type  vec:LanguageCode , owl:NamedIndividiual;
        vec:enumLiteral  "Gd" .

vec:signalRecommendedConductorSpecification
        rdf:type      owl:ObjectProperty;
        rdfs:comment  "Defines a recommended Specification for the cores that implement this signal.\n"@en;
        rdfs:domain   vec:Signal;
        rdfs:label    "recommendedConductorSpecification"@en;
        rdfs:range    vec:ConductorSpecification .

vec:ZoneAssignment  rdf:type  owl:Class;
        rdfs:comment  "A ZoneAssignment defines that a specific TopologySegment is affected by the TopologyZone. If a coverage is defined, only the parts of the Segment that have a coverage are affected. If no coverage is defined, the whole segment is affected.\n"@en;
        rdfs:label    "ZoneAssignment"@en .

vec:ComponentNodeType_PowerDistribution
        rdf:type         vec:ComponentNodeType , owl:NamedIndividiual;
        rdfs:comment     "A device that distributes power to other devices (e.g. a fuse box).\n"@en;
        vec:enumLiteral  "PowerDistribution" .

vec:SignalInformationType_Digital
        rdf:type         vec:SignalInformationType , owl:NamedIndividiual;
        vec:enumLiteral  "digital" .

vec:fuseSpecificationFuseType
        rdf:type            owl:ObjectProperty;
        rdfs:comment        "The geometric type of a fuse.\n"@en;
        rdfs:domain         vec:FuseSpecification;
        rdfs:label          "fuseType"@en;
        rdfs:range          vec:FuseType;
        rdfs:subPropertyOf  vec:contains .

vec:LanguageCode_Oc  rdf:type  vec:LanguageCode , owl:NamedIndividiual;
        vec:enumLiteral  "Oc" .

vec:USUnitName_Quarter
        rdf:type         vec:USUnitName , owl:NamedIndividiual;
        vec:enumLiteral  "Quarter" .

vec:massInformationValueSource
        rdf:type            owl:ObjectProperty;
        rdfs:comment        "The valueSource defines in an OpenEnumeration the source from which the MassInformation has been retrieved. This information, in combination with the ValueDetermination gives a hint about the reliability of the MassInformation\n"@en;
        rdfs:domain         vec:MassInformation;
        rdfs:label          "valueSource"@en;
        rdfs:range          vec:MassInformationSource;
        rdfs:subPropertyOf  vec:contains .

vec:BuildingBlockPositioning3D
        rdf:type         owl:Class;
        rdfs:comment     "Defines the position of a BuildingBlock3D in the HarnessGeometry.\n"@en;
        rdfs:label       "BuildingBlockPositioning3D"@en;
        rdfs:subClassOf  vec:ConfigurableElement .

vec:LanguageCode_Af  rdf:type  vec:LanguageCode , owl:NamedIndividiual;
        vec:enumLiteral  "Af" .

vec:NumericalValueProperty
        rdf:type         owl:Class;
        rdfs:comment     "A custom property with a numerical value. (see KBLFRM-319)\n"@en;
        rdfs:label       "NumericalValueProperty"@en;
        rdfs:subClassOf  vec:CustomProperty .

vec:OnPointPlacement  rdf:type  owl:Class;
        rdfs:comment     "An OnPointPlacement is a placement of an OccurrenceOrUsage that places it onto discrete points, in most cases one point. In some cases, it is necessary to place a component (with more than one reference point) onto multiple points (e.g. a cable duct).\n"@en;
        rdfs:label       "OnPointPlacement"@en;
        rdfs:subClassOf  vec:Placement .

vec:LanguageCode_Ie  rdf:type  vec:LanguageCode , owl:NamedIndividiual;
        vec:enumLiteral  "Ie" .

vec:PowerConsumptionType_Typical
        rdf:type         vec:PowerConsumptionType , owl:NamedIndividiual;
        vec:enumLiteral  "Typical" .

vec:segmentCrossSectionAreaValueDetermination
        rdf:type            owl:ObjectProperty;
        rdfs:comment        "Specifies the method for determination of the value.\n"@en;
        rdfs:domain         vec:SegmentCrossSectionArea;
        rdfs:label          "valueDetermination"@en;
        rdfs:range          vec:ValueDetermination;
        rdfs:subPropertyOf  vec:contains .

vec:ConnectionGroupType
        rdf:type         owl:Class;
        rdfs:comment     "Defines the type of physical realization that is expressed by a ConnectionGroup.\n"@en;
        rdfs:label       "ConnectionGroupType"@en;
        rdfs:subClassOf  vec:OpenEnumeration .

vec:ImperialUnit  rdf:type  owl:Class;
        rdfs:comment     "The ImperialUnit class can define quantities in the terms of the Imperial-Unit-System by specifying the corresponding Imperial unit name.\n"@en;
        rdfs:label       "ImperialUnit"@en;
        rdfs:subClassOf  vec:Unit .

vec:wireElementSpecificationInsulationSpecification
        rdf:type      owl:ObjectProperty;
        rdfs:comment  "If the WireElement has an insulation then the specification of the insulation is referenced here.\n"@en;
        rdfs:domain   vec:WireElementSpecification;
        rdfs:label    "insulationSpecification"@en;
        rdfs:range    vec:InsulationSpecification .

vec:boltMountedFixingSpecificationBoltType
        rdf:type            owl:ObjectProperty;
        rdfs:comment        "Specifies the type of the bolt on which the fixing can be mounted.\n"@en;
        rdfs:domain         vec:BoltMountedFixingSpecification;
        rdfs:label          "boltType"@en;
        rdfs:range          vec:BoltMountedFixingBoltType;
        rdfs:subPropertyOf  vec:contains .

vec:RelaisType  rdf:type  owl:Class;
        rdfs:comment     "Defines the type of a relais (switching behaviour).\n"@en;
        rdfs:label       "RelaisType"@en;
        rdfs:subClassOf  vec:OpenEnumeration .

vec:pinComponentPinComponentType
        rdf:type            owl:ObjectProperty;
        rdfs:comment        "Specifies the type of a PinComponent .\n"@en;
        rdfs:domain         vec:PinComponent;
        rdfs:label          "pinComponentType"@en;
        rdfs:range          vec:PinComponentType;
        rdfs:subPropertyOf  vec:contains .

vec:vecContentVecVersion
        rdf:type            owl:ObjectProperty;
        rdfs:comment        "Specifies the version of the VEC used for the file.\n"@en;
        rdfs:domain         vec:VecContent;
        rdfs:label          "vecVersion"@en;
        rdfs:range          vec:VecVersion;
        rdfs:subPropertyOf  vec:contains .

vec:CartesianPoint2D  rdf:type  owl:Class;
        rdfs:comment     "A CartesianPoint2D is a point that is defined by its coordinates in a rectangular two-dimensional Cartesian coordinate system.\n"@en;
        rdfs:label       "CartesianPoint2D"@en;
        rdfs:subClassOf  vec:ExtendableElement .

vec:SlotLayoutType_Type_E
        rdf:type         vec:SlotLayoutType , owl:NamedIndividiual;
        rdfs:comment     "Fuse type according to ISO8820, also known as: maxi\n"@en;
        vec:enumLiteral  "Type_E" .

[ rdf:type     owl:AllDisjointClasses;
  owl:members  ( vec:ModularSlotReference vec:SlotReference )
] .

vec:cableLeadThroughSpecificationType
        rdf:type            owl:ObjectProperty;
        rdfs:comment        "Defines the type of a cable lead through. Standardized values are defined in an OpenEnumeration .\n"@en;
        rdfs:domain         vec:CableLeadThroughSpecification;
        rdfs:label          "type"@en;
        rdfs:range          vec:CableLeadThroughType;
        rdfs:subPropertyOf  vec:contains .

vec:PrimaryPartType_Fuse
        rdf:type         vec:PrimaryPartType , owl:NamedIndividiual;
        vec:enumLiteral  "Fuse" .

vec:componentNodeComponentConnector
        rdf:type            owl:ObjectProperty;
        rdfs:comment        "Specifies the ComponentConnectors of a ComponentNode."@en;
        rdfs:domain         vec:ComponentNode;
        rdfs:label          "componentConnector"@en;
        rdfs:range          vec:ComponentConnector;
        rdfs:subPropertyOf  vec:contains .

vec:placementPointPositionPlacementPoint
        rdf:type     owl:ObjectProperty;
        rdfs:domain  vec:PlacementPointPosition;
        rdfs:label   "placementPoint"@en;
        rdfs:range   vec:PlacementPoint .

vec:variantConfigurationIdentification
        rdf:type      owl:DatatypeProperty;
        rdfs:comment  "Specifies a unique identification of the variant configuration. The identification is guaranteed to be unique within the specification and does not change over the time.\n"@en;
        rdfs:domain   vec:VariantConfiguration;
        rdfs:label    "identification"@en;
        rdfs:range    xs:string .

vec:NetworkNodeSubType
        rdf:type         owl:Class;
        rdfs:comment     "Defines agreed values for NetworkNodeSubTypes . Not all combinations of NetworkNodeSubTypes and NetworkNodeTypes are semantically correct (e.g.┬áLamp, Microphone, Speaker, Motor are all Actuators).\n"@en;
        rdfs:label       "NetworkNodeSubType"@en;
        rdfs:subClassOf  vec:OpenEnumeration .

vec:PowerConsumptionType_DeepSleep
        rdf:type         vec:PowerConsumptionType , owl:NamedIndividiual;
        vec:enumLiteral  "DeepSleep" .

vec:Location  rdf:type   owl:Class;
        rdfs:comment     "A Location specifies a distinct position on a topology. Locations can be used for the placement of components or for the definition of Dimensions.\n"@en;
        rdfs:label       "Location"@en;
        rdfs:subClassOf  vec:DimensionAnchor .

vec:LanguageCode_Mg  rdf:type  vec:LanguageCode , owl:NamedIndividiual;
        vec:enumLiteral  "Mg" .

<http://www.prostep.org/ontologies/ecad/2024/03/vec#RobustnessClassReferenceSystem_LV%20215>
        rdf:type         vec:RobustnessClassReferenceSystem , owl:NamedIndividiual;
        rdfs:comment     "OEM┬áSpecification for High Voltage contacting.\n"@en;
        vec:enumLiteral  "LV 215" .

vec:SignalTransmissionMediumType_Optical
        rdf:type         vec:SignalTransmissionMediumType , owl:NamedIndividiual;
        vec:enumLiteral  "optical" .

vec:colorKey  rdf:type  owl:DatatypeProperty;
        rdfs:comment  "The key of the color in the corresponding color reference system.\n"@en;
        rdfs:domain   vec:Color;
        rdfs:label    "key"@en;
        rdfs:range    xs:string .

vec:PotentialDistributorSpecification
        rdf:type         owl:Class;
        rdfs:comment     "Specifies the properties of a potential distributor (e.g. a joint connector).\n"@en;
        rdfs:label       "PotentialDistributorSpecification"@en;
        rdfs:subClassOf  vec:EEComponentSpecification .

<http://www.prostep.org/ontologies/ecad/2024/03/vec#TerminalBoltNominalSize_%2312>
        rdf:type         vec:TerminalBoltNominalSize , owl:NamedIndividiual;
        vec:enumLiteral  "#12" .

vec:NodeType_Junction
        rdf:type         vec:NodeType , owl:NamedIndividiual;
        rdfs:comment     "A Junction is a TopologyNode where no electrical component is placed.\n"@en;
        vec:enumLiteral  "Junction" .

vec:multiFuseSpecificationFuseType
        rdf:type            owl:ObjectProperty;
        rdfs:comment        "Defines the manufacturing types of a Multi-fuse.\n"@en;
        rdfs:domain         vec:MultiFuseSpecification;
        rdfs:label          "fuseType"@en;
        rdfs:range          vec:MultiFuseType;
        rdfs:subPropertyOf  vec:contains .

vec:PowerConsumptionType_Standby
        rdf:type         vec:PowerConsumptionType , owl:NamedIndividiual;
        vec:enumLiteral  "Standby" .

vec:eEComponentRoleHousingComponentRef
        rdf:type            owl:ObjectProperty;
        rdfs:comment        "Specifies the HousingComponentReferences used in the EEComponentRole. \n(KBLFRM-401)\n"@en;
        rdfs:domain         vec:EEComponentRole;
        rdfs:label          "housingComponentRef"@en;
        rdfs:range          vec:HousingComponentReference;
        rdfs:subPropertyOf  vec:contains .

vec:functionalStructureNodeDescription
        rdf:type            owl:ObjectProperty;
        rdfs:comment        "On optional human readable description of the FunctionalStructureNode .\n"@en;
        rdfs:domain         vec:FunctionalStructureNode;
        rdfs:label          "description"@en;
        rdfs:range          vec:AbstractLocalizedString;
        rdfs:subPropertyOf  vec:contains .

vec:vecContentDateOfCreation
        rdf:type      owl:DatatypeProperty;
        rdfs:comment  "Specifies the date of creation of the VEC-file.\n"@en;
        rdfs:domain   vec:VecContent;
        rdfs:label    "dateOfCreation"@en;
        rdfs:range    xs:dateTime .

vec:PinCurrentType_StandbyCurrent
        rdf:type         vec:PinCurrentType , owl:NamedIndividiual;
        vec:enumLiteral  "standbyCurrent" .

vec:componentNodeComponentNodeType
        rdf:type            owl:ObjectProperty;
        rdfs:comment        "Specifies the type of the ComponentNode.\n"@en;
        rdfs:domain         vec:ComponentNode;
        rdfs:label          "componentNodeType"@en;
        rdfs:range          vec:ComponentNodeType;
        rdfs:subPropertyOf  vec:contains .

vec:terminalSpecificationOverallLength
        rdf:type            owl:ObjectProperty;
        rdfs:comment        "Specifies the overall length the terminal (see diagram \"Terminal Dimensions\").\n"@en;
        rdfs:domain         vec:TerminalSpecification;
        rdfs:label          "overallLength"@en;
        rdfs:range          vec:NumericalValue;
        rdfs:subPropertyOf  vec:contains .

vec:changeDescriptionDescription
        rdf:type            owl:ObjectProperty;
        rdfs:comment        "Specifies additional, human readable, information about the ChangeDescription.\n"@en;
        rdfs:domain         vec:ChangeDescription;
        rdfs:label          "description"@en;
        rdfs:range          vec:AbstractLocalizedString;
        rdfs:subPropertyOf  vec:contains .

vec:OtherUnitName_Piece
        rdf:type         vec:OtherUnitName , owl:NamedIndividiual;
        vec:enumLiteral  "Piece" .

vec:BoltMountedFixingBoltShape_Oval
        rdf:type         vec:BoltMountedFixingBoltShape , owl:NamedIndividiual;
        vec:enumLiteral  "Oval" .

vec:wireTupleTerminationPermittedUntwist
        rdf:type            owl:ObjectProperty;
        rdfs:comment        "Specifies the allowed length of untwist for the WireElementReferences on the sides of associated WireEnds."@en;
        rdfs:domain         vec:WireTupleTermination;
        rdfs:label          "permittedUntwist"@en;
        rdfs:range          vec:NumericalValue;
        rdfs:subPropertyOf  vec:contains .

vec:SignalSubType_SignalGround
        rdf:type         vec:SignalSubType , owl:NamedIndividiual;
        vec:enumLiteral  "SignalGround" .

vec:geometrySegment3DEndVector
        rdf:type            owl:ObjectProperty;
        rdfs:comment        "Specifies the end vector of the geometry segment. The end vector is a tangent to the segment at the end position.\n"@en;
        rdfs:domain         vec:GeometrySegment3D;
        rdfs:label          "endVector"@en;
        rdfs:range          vec:CartesianVector3D;
        rdfs:subPropertyOf  vec:contains .

vec:creationCreationDate
        rdf:type      owl:DatatypeProperty;
        rdfs:comment  "Specifies the date when the associated ItemVersion was created. (see KBLFRM-241)\n"@en;
        rdfs:domain   vec:Creation;
        rdfs:label    "creationDate"@en;
        rdfs:range    xs:dateTime .

vec:wireElementSpecificationTransmissionMediumType
        rdf:type            owl:ObjectProperty;
        rdfs:comment        "Defines the transmission medium in this wire element."@en;
        rdfs:domain         vec:WireElementSpecification;
        rdfs:label          "transmissionMediumType"@en;
        rdfs:range          vec:TransmissionMediumType;
        rdfs:subPropertyOf  vec:contains .

vec:WireType  rdf:type  owl:Class;
        rdfs:comment  "Specifies a wire type. A wire type is always defined by a key value. What wire type is meant by this key value is defined by a standard reference system.\n"@en;
        rdfs:label    "WireType"@en .

vec:tapeSpecificationAdhesive
        rdf:type            owl:ObjectProperty;
        rdfs:comment        "Specifies the adhesive material of the tape.\n"@en;
        rdfs:domain         vec:TapeSpecification;
        rdfs:label          "adhesive"@en;
        rdfs:range          vec:Material;
        rdfs:subPropertyOf  vec:contains .

vec:changeDescriptionApprover
        rdf:type            owl:ObjectProperty;
        rdfs:comment        "Specifies the person who has approved the change.\n"@en;
        rdfs:domain         vec:ChangeDescription;
        rdfs:label          "approver"@en;
        rdfs:range          vec:Person;
        rdfs:subPropertyOf  vec:contains .

vec:doubleValuePropertyValue
        rdf:type      owl:DatatypeProperty;
        rdfs:comment  "Defines the value of the CustomProperty.\n"@en;
        rdfs:domain   vec:DoubleValueProperty;
        rdfs:label    "value"@en;
        rdfs:range    xs:double .

vec:LanguageCode_Kk  rdf:type  vec:LanguageCode , owl:NamedIndividiual;
        vec:enumLiteral  "Kk" .

vec:conductorMaterialMaterial
        rdf:type            owl:ObjectProperty;
        rdfs:comment        "Specifies the material.\n"@en;
        rdfs:domain         vec:ConductorMaterial;
        rdfs:label          "material"@en;
        rdfs:range          vec:Material;
        rdfs:subPropertyOf  vec:contains .

vec:robustnessPropertiesClassKey
        rdf:type      owl:DatatypeProperty;
        rdfs:comment  "Specifies a key for the robustness level defined in the specified robustness class (e.g. A, B, C).\n"@en;
        rdfs:domain   vec:RobustnessProperties;
        rdfs:label    "classKey"@en;
        rdfs:range    xs:string .

vec:cavitySpecificationMinWireElementOutsideDiameter
        rdf:type            owl:ObjectProperty;
        rdfs:comment        "Specifies the minimum diameter a wire is allowed to have to fit into the cavity. This definition is necessary, since wires that are too small might cause movements and in acceptable torsion forces on terminals.\n"@en;
        rdfs:domain         vec:CavitySpecification;
        rdfs:label          "minWireElementOutsideDiameter"@en;
        rdfs:range          vec:NumericalValue;
        rdfs:subPropertyOf  vec:contains .

vec:sizeHeight  rdf:type    owl:ObjectProperty;
        rdfs:comment        "The height of the element.\n"@en;
        rdfs:domain         vec:Size;
        rdfs:label          "height"@en;
        rdfs:range          vec:NumericalValue;
        rdfs:subPropertyOf  vec:contains .

vec:PinComponentType_PowerSupply
        rdf:type         vec:PinComponentType , owl:NamedIndividiual;
        rdfs:comment     " PowerSupply defines a PinComponent that is used to supply the component itself with power (in contrast to PowerDistribution ). PinComponentBehaviours of PinComponents with this type always have the SignalDirection \"In \".\n"@en;
        vec:enumLiteral  "PowerSupply" .

vec:wireElementSpecificationOutsideDiameter
        rdf:type            owl:ObjectProperty;
        rdfs:comment        "Specifies the outside diameter of the WireElement.\n"@en;
        rdfs:domain         vec:WireElementSpecification;
        rdfs:label          "outsideDiameter"@en;
        rdfs:range          vec:NumericalValue;
        rdfs:subPropertyOf  vec:contains .

vec:InternalTerminalConnection
        rdf:type         owl:Class;
        rdfs:comment     "An InternalTerminalConnection represents an electrical connection within a terminal. For standard terminals all receptions (wire- and terminal-receptions) have an electrical connection. For non-standard terminals (e.g. coax) only some receptions have an electrical connection. The InternalTerminalConnection is modelled as a separate class and not as relationship between wire- and terminal-reception, since it is possible that a terminal has only one kind of reception (e.g. a parallel connector, a cavity bridge). (see KBLFRM-302)\n"@en;
        rdfs:label       "InternalTerminalConnection"@en;
        rdfs:subClassOf  vec:ExtendableElement .

vec:RobustnessClass_AmbientTemperature
        rdf:type         vec:RobustnessClass , owl:NamedIndividiual;
        vec:enumLiteral  "AmbientTemperature" .

vec:cavitySpecificationPrimaryLockingType
        rdf:type            owl:ObjectProperty;
        rdfs:comment        "Specifies if the cavity has a primary locking and of what type it is.\n"@en;
        rdfs:domain         vec:CavitySpecification;
        rdfs:label          "primaryLockingType"@en;
        rdfs:range          vec:PrimaryLockingType;
        rdfs:subPropertyOf  vec:contains .

vec:LanguageCode_Ml  rdf:type  vec:LanguageCode , owl:NamedIndividiual;
        vec:enumLiteral  "Ml" .

vec:wireElementSubWireElement
        rdf:type            owl:ObjectProperty;
        rdfs:comment        "Defines the subWireElements of this WireElement . The subWireElements shall be consistent with the subWireElementSpecifications of the WireElementSpecification referenced by this WireElement and shall resemble that hierarchy.\n"@en;
        rdfs:domain         vec:WireElement;
        rdfs:label          "subWireElement"@en;
        rdfs:range          vec:WireElement;
        rdfs:subPropertyOf  vec:contains .

vec:LanguageCode_Uk  rdf:type  vec:LanguageCode , owl:NamedIndividiual;
        vec:enumLiteral  "Uk" .

vec:placementPointReferenceUsedSupplementaryParts
        rdf:type     owl:ObjectProperty;
        rdfs:domain  vec:PlacementPointReference;
        rdfs:label   "usedSupplementaryParts"@en;
        rdfs:range   vec:OccurrenceOrUsage .

vec:DocumentType_PartMaster
        rdf:type         vec:DocumentType , owl:NamedIndividiual;
        rdfs:comment     "Documents of this type describe the master data of a part / component (e.g. a ConnectorHousing , a┬á Terminal , a Wire ).\n"@en;
        vec:enumLiteral  "PartMaster" .

vec:LanguageCode_Gn  rdf:type  vec:LanguageCode , owl:NamedIndividiual;
        vec:enumLiteral  "Gn" .

vec:signalWireTupleRequirements
        rdf:type      owl:ObjectProperty;
        rdfs:comment  "Defines a requirement for wire tuples.\n"@en;
        rdfs:domain   vec:Signal;
        rdfs:label    "wireTupleRequirements"@en;
        rdfs:range    vec:WireTupleSpecification .

vec:networkNodePort  rdf:type  owl:ObjectProperty;
        rdfs:comment        "Specifies the NetworkPorts of a NetworkNode. \n"@en;
        rdfs:domain         vec:NetworkNode;
        rdfs:label          "port"@en;
        rdfs:range          vec:NetworkPort;
        rdfs:subPropertyOf  vec:contains .

vec:partRelationAccessoryPart
        rdf:type            owl:ObjectProperty;
        rdfs:comment        "This association is defined as unique='false' and ordered='false'. This can not be represented efficiently directly in RDF/OWL. Therefore, this association references Wrappers as proxies to the actual elements, instead of the actual elements itself (like a regular association)." , "References the PartVersions that are related by the PartRelation. \n"@en;
        rdfs:domain         vec:PartRelation;
        rdfs:label          "accessoryPart"@en;
        rdfs:range          vec:PartVersionWrapper;
        rdfs:subPropertyOf  vec:contains .

vec:LabelingTechnology_Moulded
        rdf:type         vec:LabelingTechnology , owl:NamedIndividiual;
        vec:enumLiteral  "Moulded" .

vec:cavityAccessoryRoleCavityAccessorySpecification
        rdf:type     owl:ObjectProperty;
        rdfs:domain  vec:CavityAccessoryRole;
        rdfs:label   "cavityAccessorySpecification"@en;
        rdfs:range   vec:CavityAccessorySpecification .

vec:dimensionValueComponent
        rdf:type      owl:DatatypeProperty;
        rdfs:comment  "Defines the value of the dimension. This value can be null, if it shall be calculated and only a tolerance shall be defined.\n"@en;
        rdfs:domain   vec:Dimension;
        rdfs:label    "valueComponent"@en;
        rdfs:range    xs:double .

vec:NodeType_EndNode  rdf:type  vec:NodeType , owl:NamedIndividiual;
        rdfs:comment     "Electrical components are normally placed on an EndNode.\n"@en;
        vec:enumLiteral  "EndNode" .

vec:LanguageCode_Om  rdf:type  vec:LanguageCode , owl:NamedIndividiual;
        vec:enumLiteral  "Om" .

vec:signalNominalVoltage
        rdf:type            owl:ObjectProperty;
        rdfs:domain         vec:Signal;
        rdfs:label          "nominalVoltage"@en;
        rdfs:range          vec:NominalVoltage;
        rdfs:subPropertyOf  vec:contains .

vec:USUnitName_Drachm
        rdf:type         vec:USUnitName , owl:NamedIndividiual;
        vec:enumLiteral  "Drachm" .

vec:USUnitName_Ounce  rdf:type  vec:USUnitName , owl:NamedIndividiual;
        vec:enumLiteral  "Ounce" .

vec:cableLeadThroughSpecificationGeometry
        rdf:type            owl:ObjectProperty;
        rdfs:comment        "Defines the geometry of a cable lead through in the sealing area. Standardized values are defined in an OpenEnumeration .\n"@en;
        rdfs:domain         vec:CableLeadThroughSpecification;
        rdfs:label          "geometry"@en;
        rdfs:range          vec:CableLeadThroughGeometry;
        rdfs:subPropertyOf  vec:contains .

vec:fuseComponentIdentification
        rdf:type      owl:DatatypeProperty;
        rdfs:comment  "Identification of the FuseComponent, which must be distinct for all FuseComponents of an MultiFuseSpecification.\n"@en;
        rdfs:domain   vec:FuseComponent;
        rdfs:label    "identification"@en;
        rdfs:range    xs:string .

vec:grommetSpecificationMountingType
        rdf:type            owl:ObjectProperty;
        rdfs:comment        "Defines how the grommet is mounted onto the harness (not the vehicle body)."@en;
        rdfs:domain         vec:GrommetSpecification;
        rdfs:label          "mountingType"@en;
        rdfs:range          vec:GrommetMountingType;
        rdfs:subPropertyOf  vec:contains .

vec:labelingRoleLabelValue
        rdf:type      owl:DatatypeProperty;
        rdfs:comment  "Specifies the value of a label printed on the component.\n"@en;
        rdfs:domain   vec:LabelingRole;
        rdfs:label    "labelValue"@en;
        rdfs:range    xs:string .

vec:StatusOfApproval_Approved
        rdf:type         vec:StatusOfApproval , owl:NamedIndividiual;
        vec:enumLiteral  "Approved" .

vec:segmentCrossSectionAreaArea
        rdf:type            owl:ObjectProperty;
        rdfs:comment        "Specifies the value of the cross-section area of the segment.\n"@en;
        rdfs:domain         vec:SegmentCrossSectionArea;
        rdfs:label          "area"@en;
        rdfs:range          vec:NumericalValue;
        rdfs:subPropertyOf  vec:contains .

vec:LanguageCode_So  rdf:type  vec:LanguageCode , owl:NamedIndividiual;
        vec:enumLiteral  "So" .

vec:TemperatureType  rdf:type  owl:Class;
        rdfs:comment     "Defines the type (scenario)┬áfor which a TemperatureInformation applies."@en;
        rdfs:label       "TemperatureType"@en;
        rdfs:subClassOf  vec:OpenEnumeration .

vec:terminalTypeName  rdf:type  owl:DatatypeProperty;
        rdfs:comment  "Specifies the type of the cavity (e.g. MQS, DFK, ...).\n"@en;
        rdfs:domain   vec:TerminalType;
        rdfs:label    "name"@en;
        rdfs:range    xs:string .

vec:VecVersion_1.2.1  rdf:type  vec:VecVersion , owl:NamedIndividiual;
        vec:enumLiteral  "1.2.1" .

vec:segmentConnectionPointReachableCavities
        rdf:type      owl:ObjectProperty;
        rdfs:comment  "Specifies the Cavities that are reachable with wires through this SegmentConnectionPoint.\n"@en;
        rdfs:domain   vec:SegmentConnectionPoint;
        rdfs:label    "reachableCavities"@en;
        rdfs:range    vec:Cavity .

vec:PartUsageSpecification
        rdf:type         owl:Class;
        rdfs:comment     "Specification for the definition of PartUsages.\n"@en;
        rdfs:label       "PartUsageSpecification"@en;
        rdfs:subClassOf  vec:Specification .

vec:relaySpecificationLowNoise
        rdf:type      owl:DatatypeProperty;
        rdfs:comment  "Defines if the relais switch with low noise /┬ásilently or not.\n"@en;
        rdfs:domain   vec:RelaySpecification;
        rdfs:label    "lowNoise"@en;
        rdfs:range    xs:boolean .

vec:SiUnitName_Henry  rdf:type  vec:SiUnitName , owl:NamedIndividiual;
        vec:enumLiteral  "Henry" .

vec:TerminalBoltNominalSize
        rdf:type         owl:Class;
        rdfs:comment     "Defines the nominal sizes for threaded bolts as \"ISO metric screw thread\" or as \"Unified Thread Standard\" (Imperial).\nSee also TerminalBoltType.MetricThread /┬áImperialThread. ┬á\nFor the definition of the values see https://en.wikipedia.org/wiki/ISO_metric_screw_thread and https://de.wikipedia.org/wiki/Unified_Thread_Standard .\n"@en;
        rdfs:label       "TerminalBoltNominalSize"@en;
        rdfs:subClassOf  vec:OpenEnumeration .

vec:WireAddOnType_Contract
        rdf:type         vec:WireAddOnType , owl:NamedIndividiual;
        rdfs:comment     "The agreed add-on for any negotiations and calculations.\n"@en;
        vec:enumLiteral  "Contract" .

vec:FillerSpecification
        rdf:type         owl:Class;
        rdfs:comment     "Specification for the definition of filler elements in the wire.\n"@en;
        rdfs:label       "FillerSpecification"@en;
        rdfs:subClassOf  vec:Specification .

vec:grommetSpecificationHoleDiameter
        rdf:type            owl:ObjectProperty;
        rdfs:comment        "Specifies the valid diameter of a hole into which the grommet fits.\n"@en;
        rdfs:domain         vec:GrommetSpecification;
        rdfs:label          "holeDiameter"@en;
        rdfs:range          vec:NumericalValue;
        rdfs:subPropertyOf  vec:contains .

vec:couplingPointFirstConnector
        rdf:type     owl:ObjectProperty;
        rdfs:domain  vec:CouplingPoint;
        rdfs:label   "firstConnector"@en;
        rdfs:range   vec:ConnectorHousingRole .

vec:segmentConnectionPointPlacementPoint
        rdf:type      owl:ObjectProperty;
        rdfs:comment  "Specifies the PlacementPoint that represents this SegmentConnectionPoint in a PlaceableElementSpecification.\n"@en;
        rdfs:domain   vec:SegmentConnectionPoint;
        rdfs:label    "placementPoint"@en;
        rdfs:range    vec:PlacementPoint .

vec:SlotMapping  rdf:type  owl:Class;
        rdfs:comment  "Defines the mapping of two slots contained PartVersion A & B of the containing Mapping-object.\n"@en;
        rdfs:label    "SlotMapping"@en .

vec:PluggableTerminalType_PiggyBack
        rdf:type         vec:PluggableTerminalType , owl:NamedIndividiual;
        vec:enumLiteral  "PiggyBack" .

vec:SegmentMapping  rdf:type  owl:Class;
        rdfs:comment  "Defines the relationship of an inner segment to its outer topology. The relationship to the outer topology is expressed with a Path. ┬á\n"@en;
        rdfs:label    "SegmentMapping"@en .

vec:SignalSubType_USB2
        rdf:type         vec:SignalSubType , owl:NamedIndividiual;
        rdfs:comment     "Universal Serial┬áBus Version 2.0\n"@en;
        vec:enumLiteral  "USB2" .

vec:segmentConnectionPointHCPlacementPoint
        rdf:type      owl:ObjectProperty;
        rdfs:comment  "Specifies the PlacementPoint that represents this SegmentConnectionPoint in a PlaceableElementSpecification.\n"@en;
        rdfs:domain   vec:SegmentConnectionPointHC;
        rdfs:label    "placementPoint"@en;
        rdfs:range    vec:PlacementPoint .

vec:LanguageCode_Or  rdf:type  vec:LanguageCode , owl:NamedIndividiual;
        vec:enumLiteral  "Or" .

vec:TopologyNode  rdf:type  owl:Class;
        rdfs:comment     "A TopologyNode is a point in the Topology where TopologySegments are starting and ending.\n"@en;
        rdfs:label       "TopologyNode"@en;
        rdfs:subClassOf  vec:ConfigurableElement .

vec:FunctionalRequirement
        rdf:type      owl:Class;
        rdfs:comment  "Allows the definition of functional requirements in an enumerable way (e.g. conformance to a certain ASIL┬álevel). Attributes of this type have the multiplicity of [0..*].┬áThe following restrictions apply: For a combination of type &┬áreferenceSystem only a single value is allowed. For single type For a specific type and different references systems, multiple values are allowed.┬áHowever, they must express the same semantic value. For different types multiple values are allowed. ┬á\n"@en;
        rdfs:label    "FunctionalRequirement"@en .

vec:eEComponentSpecificationPowerConsumption
        rdf:type            owl:ObjectProperty;
        rdfs:comment        "Specifies the PowerConsumptions of this EEComponentSpecification. This refers to the internal power consumption of this E/E-component, not the power-consumption that might occur indirectly over other E/E-components that are supplied through this component.\n"@en;
        rdfs:domain         vec:EEComponentSpecification;
        rdfs:label          "powerConsumption"@en;
        rdfs:range          vec:PowerConsumption;
        rdfs:subPropertyOf  vec:contains .

vec:nodeMappingMappedPosition
        rdf:type            owl:ObjectProperty;
        rdfs:domain         vec:NodeMapping;
        rdfs:label          "mappedPosition"@en;
        rdfs:range          vec:Location;
        rdfs:subPropertyOf  vec:contains .

vec:ProtectionMaterialLength
        rdf:type      owl:Class;
        rdfs:comment  "Defines the material length of a WireProtectionRole . A WireProtectionRole can have multiple lengths of different types but must not have more than one length of the same type.\n"@en;
        rdfs:label    "ProtectionMaterialLength"@en .

vec:IECUnitName_Bit  rdf:type  vec:IECUnitName , owl:NamedIndividiual;
        vec:enumLiteral  "Bit" .

vec:couplingPointSecondConnector
        rdf:type     owl:ObjectProperty;
        rdfs:domain  vec:CouplingPoint;
        rdfs:label   "secondConnector"@en;
        rdfs:range   vec:ConnectorHousingRole .

vec:projectCarClassificationLevel4
        rdf:type      owl:DatatypeProperty;
        rdfs:comment  "Provides a classification according to \"CC8 Recommended Practices Specification and Configuration, Product Structures\". Car classification is the identification of a set of similar cars to be offered to the market. Level 4 stands for \"Furthest pre-configured abstract product class\" and represents the furthest configured class of a product, which is not yet a real product. E.g. this could be a complete vehicle, engine, gearbox etc. which has not been evaluated against customer special choices or an abstract vehicle, engine, gear-box etc. which could become a real one after the associated BoM is evaluated. The purpose of this level of a product class instance is in any case to reflect that level of product class of a BoM system which leads to the individual BoM for a single product.\n"@en;
        rdfs:domain   vec:Project;
        rdfs:label    "carClassificationLevel4"@en;
        rdfs:range    xs:string .

vec:connectionNet  rdf:type  owl:ObjectProperty;
        rdfs:comment  "References the Net that is realized by the Connection.\n"@en;
        rdfs:domain   vec:Connection;
        rdfs:label    "net"@en;
        rdfs:range    vec:Net .

vec:roleIdentification
        rdf:type      owl:DatatypeProperty;
        rdfs:comment  "Specifies a unique identification of the Role. The identification is guaranteed to be unique within the OccurrenceOrUsage.\n"@en;
        rdfs:domain   vec:Role;
        rdfs:label    "identification"@en;
        rdfs:range    xs:string .

vec:unitExponent  rdf:type  owl:DatatypeProperty;
        rdfs:comment  "Defines the exponent with which this unit instance should be used. In order to define square meters for example, the SIUnit \"metre\" with an exponent of 2 will be used. If no exponent is defined it is equivalent to the value 1.\n"@en;
        rdfs:domain   vec:Unit;
        rdfs:label    "exponent"@en;
        rdfs:range    xs:integer .

vec:conductorCurrentInformationVoltage
        rdf:type            owl:ObjectProperty;
        rdfs:comment        "The voltage for which this maximum current value is applicable.\n"@en;
        rdfs:domain         vec:ConductorCurrentInformation;
        rdfs:label          "voltage"@en;
        rdfs:range          vec:NumericalValue;
        rdfs:subPropertyOf  vec:contains .

vec:boundingBoxX  rdf:type  owl:ObjectProperty;
        rdfs:comment        "Defines the extent of the bounding box in the direction of x (length).\n"@en;
        rdfs:domain         vec:BoundingBox;
        rdfs:label          "x"@en;
        rdfs:range          vec:NumericalValue;
        rdfs:subPropertyOf  vec:contains .

vec:cavitySpecificationSealable
        rdf:type      owl:DatatypeProperty;
        rdfs:comment  "Specifies if the cavity is sealable.\n"@en;
        rdfs:domain   vec:CavitySpecification;
        rdfs:label    "sealable"@en;
        rdfs:range    xs:boolean .

vec:wireEndPositionOnWire
        rdf:type      owl:DatatypeProperty;
        rdfs:comment  "Specifies the position of the WireEnd on the wire. This must be a value between 0 and 1.\n"@en;
        rdfs:domain   vec:WireEnd;
        rdfs:label    "positionOnWire"@en;
        rdfs:range    xs:double .

vec:SlotSealingType_Moulded
        rdf:type         vec:SlotSealingType , owl:NamedIndividiual;
        rdfs:comment     "The Slot is sealed by moulding it with some sort of sealing compound.\n"@en;
        vec:enumLiteral  "Moulded" .

vec:fileBasedInstructionLastModified
        rdf:type      owl:DatatypeProperty;
        rdfs:comment  "The last modified timestamp of the file.\n"@en;
        rdfs:domain   vec:FileBasedInstruction;
        rdfs:label    "lastModified"@en;
        rdfs:range    xs:dateTime .

vec:WireTupleTerminationSpecification
        rdf:type         owl:Class;
        rdfs:comment     "A WireTupleTerminationSpecification is the container specification for WireTupleTerminations .\n"@en;
        rdfs:label       "WireTupleTerminationSpecification"@en;
        rdfs:subClassOf  vec:Specification .

vec:LanguageCode_It  rdf:type  vec:LanguageCode , owl:NamedIndividiual;
        vec:enumLiteral  "It" .

vec:vecContentGeneratingSystemVersion
        rdf:type      owl:DatatypeProperty;
        rdfs:comment  "Specifies the version of the system that has generated the VEC-file.\n"@en;
        rdfs:domain   vec:VecContent;
        rdfs:label    "generatingSystemVersion"@en;
        rdfs:range    xs:string .

vec:cavityPositionDetailInsertionPosition
        rdf:type            owl:ObjectProperty;
        rdfs:comment        "The position of the center of the cavity in the entrance surface of the connector during the insertion process.\n"@en;
        rdfs:domain         vec:CavityPositionDetail;
        rdfs:label          "insertionPosition"@en;
        rdfs:range          vec:CartesianPoint3D;
        rdfs:subPropertyOf  vec:contains .

vec:wireElementWireElementSpecification
        rdf:type      owl:ObjectProperty;
        rdfs:comment  "Reference the WireElementSpecification that is represented by the WireElement.\n"@en;
        rdfs:domain   vec:WireElement;
        rdfs:label    "wireElementSpecification"@en;
        rdfs:range    vec:WireElementSpecification .

vec:PrimaryPartType_Fixing
        rdf:type         vec:PrimaryPartType , owl:NamedIndividiual;
        vec:enumLiteral  "Fixing" .

vec:ExtendableElement
        rdf:type      owl:Class;
        rdfs:comment  "Abstract base class for extendable elements. Extendable elements have the possibility to define non-standard custom properties.\n"@en;
        rdfs:label    "ExtendableElement"@en .

vec:dimensionUnitComponent
        rdf:type     owl:ObjectProperty;
        rdfs:domain  vec:Dimension;
        rdfs:label   "unitComponent"@en;
        rdfs:range   vec:Unit .

vec:stripeSpecificationLength
        rdf:type            owl:ObjectProperty;
        rdfs:comment        "Specifies the length of the stripe.\n"@en;
        rdfs:domain         vec:StripeSpecification;
        rdfs:label          "length"@en;
        rdfs:range          vec:NumericalValue;
        rdfs:subPropertyOf  vec:contains .

vec:pinComponentBehaviour
        rdf:type            owl:ObjectProperty;
        rdfs:comment        "Specifies the configuration dependent electrical behavior of the PinComponent.\n"@en;
        rdfs:domain         vec:PinComponent;
        rdfs:label          "behaviour"@en;
        rdfs:range          vec:PinComponentBehavior;
        rdfs:subPropertyOf  vec:contains .

vec:WireElementShape_Flat
        rdf:type         vec:WireElementShape , owl:NamedIndividiual;
        vec:enumLiteral  "Flat" .

vec:slotCavity  rdf:type    owl:ObjectProperty;
        rdfs:comment        "Specifies the Cavities forming the Slot.\n"@en;
        rdfs:domain         vec:Slot;
        rdfs:label          "cavity"@en;
        rdfs:range          vec:Cavity;
        rdfs:subPropertyOf  vec:contains .

vec:cartesianPoint2DX
        rdf:type      owl:DatatypeProperty;
        rdfs:comment  "Specifies the value of x-coordinate of the Cartesian point. The unit of this value is the baseUnit of containing BuildingBlockSpecification2D.\n"@en;
        rdfs:domain   vec:CartesianPoint2D;
        rdfs:label    "x"@en;
        rdfs:range    xs:double .

vec:LanguageCode_Ku  rdf:type  vec:LanguageCode , owl:NamedIndividiual;
        vec:enumLiteral  "Ku" .

vec:wireElementSpecificationValidWireReceptionTypes
        rdf:type            owl:ObjectProperty;
        rdfs:comment        "Defines the WireReceptionTypes that are allowed for joining with the specified WireElement.\n"@en;
        rdfs:domain         vec:WireElementSpecification;
        rdfs:label          "validWireReceptionTypes"@en;
        rdfs:range          vec:WireReceptionType;
        rdfs:subPropertyOf  vec:contains .

vec:VariantCode  rdf:type  owl:Class;
        rdfs:comment     "VariantCodes are defining the literals on which VariantConfiguration are stated. Possible VariantCodes might be different for steering types, optional equipment, engine-power class.\n"@en;
        rdfs:label       "VariantCode"@en;
        rdfs:subClassOf  vec:ExtendableElement .

vec:routingSpecialRoutedComment
        rdf:type            owl:ObjectProperty;
        rdfs:comment        "Allows the specification of an explanation why this routing has been routed in a special way.\n"@en;
        rdfs:domain         vec:Routing;
        rdfs:label          "specialRoutedComment"@en;
        rdfs:range          vec:LocalizedString;
        rdfs:subPropertyOf  vec:contains .

vec:CurrentType_DC  rdf:type  vec:CurrentType , owl:NamedIndividiual;
        vec:enumLiteral  "DC" .

vec:usageConstraintToEffectivityControlKey
        rdf:type      owl:DatatypeProperty;
        rdfs:comment  "See FromEffectivityControlKey.\n"@en;
        rdfs:domain   vec:UsageConstraint;
        rdfs:label    "toEffectivityControlKey"@en;
        rdfs:range    xs:string .

vec:CartesianVector2D
        rdf:type         owl:Class;
        rdfs:comment     "A Cartesian vector in the two-dimensional space.\n"@en;
        rdfs:label       "CartesianVector2D"@en;
        rdfs:subClassOf  vec:CartesianVector .

vec:LanguageCode_St  rdf:type  vec:LanguageCode , owl:NamedIndividiual;
        vec:enumLiteral  "St" .

vec:segmentConnectionPointHCWireAddOn
        rdf:type            owl:ObjectProperty;
        rdfs:comment        "Defines the wire add-on that is required the reach the referenced SegmentConnectionPoint from this SegmentConnectionPointHC with which the individual cavity add-ons are defined."@en;
        rdfs:domain         vec:SegmentConnectionPointHC;
        rdfs:label          "wireAddOn"@en;
        rdfs:range          vec:NumericalValue;
        rdfs:subPropertyOf  vec:contains .

vec:NetworkNodeType_ECU
        rdf:type         vec:NetworkNodeType , owl:NamedIndividiual;
        rdfs:comment     "Electronic Control Unit. An electronic control unit (ECU) is any embedded system in automotive electronics that controls one or more of the electrical systems or subsystems in a vehicle.\n"@en;
        vec:enumLiteral  "ECU" .

vec:PrimaryPartType_Wire
        rdf:type         vec:PrimaryPartType , owl:NamedIndividiual;
        vec:enumLiteral  "Wire" .

vec:terminalRoleSealState
        rdf:type            owl:ObjectProperty;
        rdfs:comment        "Specifies if this instance of a terminal should be sealed (waterproof). This applies for example to SpliceTerminals.\n"@en;
        rdfs:domain         vec:TerminalRole;
        rdfs:label          "sealState"@en;
        rdfs:range          vec:SealState;
        rdfs:subPropertyOf  vec:contains .

vec:topologySegmentForm
        rdf:type            owl:ObjectProperty;
        rdfs:comment        "Specifies the form of the TopologySegment. A TopologySegment can either be circular or noncircular.\n"@en;
        rdfs:domain         vec:TopologySegment;
        rdfs:label          "form"@en;
        rdfs:range          vec:SegmentForm;
        rdfs:subPropertyOf  vec:contains .

vec:LengthClassification
        rdf:type         owl:Class;
        rdfs:comment     "Enumeration for the definition of a LengthClassification.\n"@en;
        rdfs:label       "LengthClassification"@en;
        rdfs:subClassOf  vec:OpenEnumeration .

vec:DocumentType_GraphicsSymbol
        rdf:type         vec:DocumentType , owl:NamedIndividiual;
        rdfs:comment     "Documents of this type represent a graphical symbol (2D), which is normally an external file (e.g. an SVG, PNG). The use case for this document type are symbols that are used in 2D┬áharness and form board drawings.\n"@en;
        vec:enumLiteral  "GraphicsSymbol" .

vec:requirementsConformanceStatementDocumentVersion
        rdf:type      owl:ObjectProperty;
        rdfs:comment  "References the DocumentVersion that contains the requirements to which a conformance statement shall be expressed.\n"@en;
        rdfs:domain   vec:RequirementsConformanceStatement;
        rdfs:label    "documentVersion"@en;
        rdfs:range    vec:DocumentVersion .

vec:generalTechnicalPartSpecificationColorInformation
        rdf:type            owl:ObjectProperty;
        rdfs:comment        "Specifies the color of the part.\n"@en;
        rdfs:domain         vec:GeneralTechnicalPartSpecification;
        rdfs:label          "colorInformation"@en;
        rdfs:range          vec:Color;
        rdfs:subPropertyOf  vec:contains .

vec:SignalCurve_DiscreteSignal
        rdf:type         vec:SignalCurve , owl:NamedIndividiual;
        vec:enumLiteral  "discreteSignal" .

vec:SealingGeometry_Oval
        rdf:type         vec:SealingGeometry , owl:NamedIndividiual;
        vec:enumLiteral  "Oval" .

vec:cavityReferenceReferencedCavity
        rdf:type      owl:ObjectProperty;
        rdfs:comment  "Points to the cavity referenced by the cavity reference. \n"@en;
        rdfs:domain   vec:CavityReference;
        rdfs:label    "referencedCavity"@en;
        rdfs:range    vec:Cavity .

vec:sIUnitSiPrefix  rdf:type  owl:ObjectProperty;
        rdfs:comment        "Specifies the prefix of the SI unit (e.g. milli, centi, mirco,...)\n"@en;
        rdfs:domain         vec:SIUnit;
        rdfs:label          "siPrefix"@en;
        rdfs:range          vec:SiPrefix;
        rdfs:subPropertyOf  vec:contains .

vec:applicationConstraintFromDate
        rdf:type      owl:DatatypeProperty;
        rdfs:comment  "Specifies the lower bound of the time period to which the application constraint applies.\n"@en;
        rdfs:domain   vec:ApplicationConstraint;
        rdfs:label    "fromDate"@en;
        rdfs:range    xs:dateTime .

vec:RobustnessClass_AbrasionResistance
        rdf:type         vec:RobustnessClass , owl:NamedIndividiual;
        vec:enumLiteral  "AbrasionResistance" .

vec:topologySegmentInstantiatedSegment
        rdf:type      owl:ObjectProperty;
        rdfs:comment  "If this TopologySegment is an instance of another To pologySegment that is defined elsewhere (e.g. the topology of an assembly), then the instantiated may be referenced here.\n"@en;
        rdfs:domain   vec:TopologySegment;
        rdfs:label    "instantiatedSegment"@en;
        rdfs:range    vec:TopologySegment .

vec:topologyZoneAssignment
        rdf:type            owl:ObjectProperty;
        rdfs:comment        "The assignments of specific topology elements to this zone.\n"@en;
        rdfs:domain         vec:TopologyZone;
        rdfs:label          "assignment"@en;
        rdfs:range          vec:ZoneAssignment;
        rdfs:subPropertyOf  vec:contains .

vec:EEComponentSpecification
        rdf:type         owl:Class;
        rdfs:comment     "Base-class for the specification of electrological components, which are connected to the harness. Usually electrological components are not part of the harness e.g. a fuse, a switch or a control device. All EEComponents can have one or more HousingComponents which are possible interfaces for the connection to a harness.\n"@en;
        rdfs:label       "EEComponentSpecification"@en;
        rdfs:subClassOf  vec:PartOrUsageRelatedSpecification .

vec:cavityMappingIdentificationB
        rdf:type      owl:DatatypeProperty;
        rdfs:comment  "The identification of the Cavity on side B\n"@en;
        rdfs:domain   vec:CavityMapping;
        rdfs:label    "identificationB"@en;
        rdfs:range    xs:string .

vec:WindingType  rdf:type  owl:Class;
        rdfs:comment     "┬áDefines the type of taping.\n"@en;
        rdfs:label       "WindingType"@en;
        rdfs:subClassOf  vec:OpenEnumeration .

vec:LanguageCode_Az  rdf:type  vec:LanguageCode , owl:NamedIndividiual;
        vec:enumLiteral  "Az" .

vec:GeometryType_Dmu  rdf:type  vec:GeometryType , owl:NamedIndividiual;
        rdfs:comment     "The Geometry is a DMU model of the vehicle.\n"@en;
        vec:enumLiteral  "Dmu" .

vec:SlotLayoutType_USBMiniB
        rdf:type         vec:SlotLayoutType , owl:NamedIndividiual;
        vec:enumLiteral  "USBMiniB" .

vec:cavityReferenceIntegratedTerminalRole
        rdf:type            owl:ObjectProperty;
        rdfs:comment        "Contains the terminal role if the cavity has an integrated terminal (e.g. an IDC).\n"@en;
        rdfs:domain         vec:CavityReference;
        rdfs:label          "integratedTerminalRole"@en;
        rdfs:range          vec:TerminalRole;
        rdfs:subPropertyOf  vec:contains .

vec:simpleValuePropertyValue
        rdf:type      owl:DatatypeProperty;
        rdfs:comment  "Defines the value of the CustomProperty.\n"@en;
        rdfs:domain   vec:SimpleValueProperty;
        rdfs:label    "value"@en;
        rdfs:range    xs:string .

vec:PrimaryPartType_SpliceTerminal
        rdf:type         vec:PrimaryPartType , owl:NamedIndividiual;
        vec:enumLiteral  "SpliceTerminal" .

vec:SignalSubType_LVDS
        rdf:type         vec:SignalSubType , owl:NamedIndividiual;
        rdfs:comment     "low-voltage differential signalling\n"@en;
        vec:enumLiteral  "LVDS" .

vec:cavitySealSpecificationWireElementOutsideDiameter
        rdf:type            owl:ObjectProperty;
        rdfs:comment        "Specifies a range of valid wire diameters to which the cavity seal fits.\n"@en;
        rdfs:domain         vec:CavitySealSpecification;
        rdfs:label          "wireElementOutsideDiameter"@en;
        rdfs:range          vec:ValueRange;
        rdfs:subPropertyOf  vec:contains .

vec:matingPointFirstTerminalRole
        rdf:type      owl:ObjectProperty;
        rdfs:comment  "References the first terminal that is mated.\n"@en;
        rdfs:domain   vec:MatingPoint;
        rdfs:label    "firstTerminalRole"@en;
        rdfs:range    vec:TerminalRole .

vec:DocumentType_SystemSchematic
        rdf:type         vec:DocumentType , owl:NamedIndividiual;
        rdfs:comment     ""@en;
        vec:enumLiteral  "SystemSchematic" .

vec:TopologyZone  rdf:type  owl:Class;
        rdfs:comment     "A TopologyZone divides a topology in different sections / design spaces. A TopologyZone may be subdivided in further TopologyZone . There can be multiple reasons for creating an orthogonal sectioning on a Topology . Therefore, TopologyZones can be overlapping.\n"@en;
        rdfs:label       "TopologyZone"@en;
        rdfs:subClassOf  vec:ConfigurableElement .

vec:robustnessPropertiesClass
        rdf:type            owl:ObjectProperty;
        rdfs:comment        "Specifies the identifier of a robustness class defined by the robustness class reference system. Robustness classes are for example: oil, petrol, UV, water. Specific known and used classes are defined in an open enumeration.\n"@en;
        rdfs:domain         vec:RobustnessProperties;
        rdfs:label          "class"@en;
        rdfs:range          vec:RobustnessClass;
        rdfs:subPropertyOf  vec:contains .

vec:potentialDistributorSpecificationScrewable
        rdf:type      owl:DatatypeProperty;
        rdfs:comment  "Defines if the PotentialDistributor can be screwed by itself to be fixed. This fixation is a non-electrical connection. If the PotentialDistributor can be fixated electrical (like a ring terminal) it shall have one PinComponent with a RingTerminalSpecification .\n"@en;
        rdfs:domain   vec:PotentialDistributorSpecification;
        rdfs:label    "screwable"@en;
        rdfs:range    xs:boolean .

vec:labelingSpecificationLabelingTechnology
        rdf:type            owl:ObjectProperty;
        rdfs:comment        "Specifies the used labeling technology if the label is already defined in this specification."@en;
        rdfs:domain         vec:LabelingSpecification;
        rdfs:label          "labelingTechnology"@en;
        rdfs:range          vec:LabelingTechnology;
        rdfs:subPropertyOf  vec:contains .

vec:robustnessPropertiesDescription
        rdf:type            owl:ObjectProperty;
        rdfs:comment        "On optional human readable description of the robustness (e.g. the name).\n"@en;
        rdfs:domain         vec:RobustnessProperties;
        rdfs:label          "description"@en;
        rdfs:range          vec:LocalizedString;
        rdfs:subPropertyOf  vec:contains .

vec:pinTimingTime  rdf:type  owl:ObjectProperty;
        rdfs:comment        "Specifies the time value of the timing.\n"@en;
        rdfs:domain         vec:PinTiming;
        rdfs:label          "time"@en;
        rdfs:range          vec:NumericalValue;
        rdfs:subPropertyOf  vec:contains .

vec:personDepartment  rdf:type  owl:DatatypeProperty;
        rdfs:comment  "Specifies the department the person belongs to.\n"@en;
        rdfs:domain   vec:Person;
        rdfs:label    "department"@en;
        rdfs:range    xs:string .

vec:ConnectionEndGender_Male
        rdf:type         vec:ConnectionEndGender , owl:NamedIndividiual;
        vec:enumLiteral  "Male" .

vec:transformation2DOrigin
        rdf:type      owl:ObjectProperty;
        rdfs:comment  "References the CartesianPoint2D that is the origin of the Transformation2D. \n"@en;
        rdfs:domain   vec:Transformation2D;
        rdfs:label    "origin"@en;
        rdfs:range    vec:CartesianPoint2D .

vec:customUnitIdentification
        rdf:type      owl:DatatypeProperty;
        rdfs:comment  "A unique identification of the custom unit.\n"@en;
        rdfs:domain   vec:CustomUnit;
        rdfs:label    "identification"@en;
        rdfs:range    xs:string .

vec:BuildingBlockSpecification3D
        rdf:type         owl:Class;
        rdfs:comment     "Specification for the description of a three-dimensional building block. A building block is a reusable section of a geometry.\n"@en;
        rdfs:label       "BuildingBlockSpecification3D"@en;
        rdfs:subClassOf  vec:Specification .

vec:PrimaryPartType_Ferrite
        rdf:type         vec:PrimaryPartType , owl:NamedIndividiual;
        vec:enumLiteral  "Ferrite" .

vec:cavitySpecificationCavitySealingLength
        rdf:type            owl:ObjectProperty;
        rdfs:comment        "Defines the length of the sealing area in the cavity."@en;
        rdfs:domain         vec:CavitySpecification;
        rdfs:label          "cavitySealingLength"@en;
        rdfs:range          vec:NumericalValue;
        rdfs:subPropertyOf  vec:contains .

vec:CoreSpecification
        rdf:type         owl:Class;
        rdfs:comment     "Defines the properties of a circular conductor (core) which are specific for them.\n"@en;
        rdfs:label       "CoreSpecification"@en;
        rdfs:subClassOf  vec:ConductorSpecification .

vec:cableLeadThroughReferenceUsedSeals
        rdf:type      owl:ObjectProperty;
        rdfs:comment  ""@en;
        rdfs:domain   vec:CableLeadThroughReference;
        rdfs:label    "usedSeals"@en;
        rdfs:range    vec:CavitySealRole .

vec:occurrenceOrUsageViewItem3DIdentification
        rdf:type      owl:DatatypeProperty;
        rdfs:comment  "Specifies a unique identification of the OccurrenceOrUsageViewItem. The identification is guaranteed to be unique within the BuildingBlockSpecification3D.\n"@en;
        rdfs:domain   vec:OccurrenceOrUsageViewItem3D;
        rdfs:label    "identification"@en;
        rdfs:range    xs:string .

vec:cableDuctRoleCableDuctSpecification
        rdf:type      owl:ObjectProperty;
        rdfs:comment  "References the CableDuctSpecification that is instanced by this CableDuctRole.\n"@en;
        rdfs:domain   vec:CableDuctRole;
        rdfs:label    "cableDuctSpecification"@en;
        rdfs:range    vec:CableDuctSpecification .

vec:SiPrefix_Kilo  rdf:type  vec:SiPrefix , owl:NamedIndividiual;
        vec:enumLiteral  "Kilo" .

vec:cableTieSpecificationTensioningStrength
        rdf:type            owl:ObjectProperty;
        rdfs:domain         vec:CableTieSpecification;
        rdfs:label          "tensioningStrength"@en;
        rdfs:range          vec:NumericalValue;
        rdfs:subPropertyOf  vec:contains .

vec:CopyrightInformation
        rdf:type         owl:Class;
        rdfs:comment     "A CopyrightInformation-instance specifies copyright information for one or more Items.\n"@en;
        rdfs:label       "CopyrightInformation"@en;
        rdfs:subClassOf  vec:ExtendableElement .

vec:LanguageCode_Uz  rdf:type  vec:LanguageCode , owl:NamedIndividiual;
        vec:enumLiteral  "Uz" .

vec:StatusOfApproval_NotYetApproved
        rdf:type         vec:StatusOfApproval , owl:NamedIndividiual;
        vec:enumLiteral  "NotYetApproved" .

[ rdf:type     owl:AllDisjointClasses;
  owl:members  ( vec:PluggableTerminalRole vec:RingTerminalRole vec:SpliceTerminalRole vec:BoltTerminalRole vec:OpenWireEndTerminalRole vec:BridgeTerminalRole )
] .

vec:wireElementReferenceLabelValue
        rdf:type      owl:DatatypeProperty;
        rdfs:comment  "Specifies the value of label, if this WireElementReference is labled."@en;
        rdfs:domain   vec:WireElementReference;
        rdfs:label    "labelValue"@en;
        rdfs:range    xs:string .

vec:ringTerminalSpecificationThickness
        rdf:type            owl:ObjectProperty;
        rdfs:comment        "Specifies the thickness of the contact surface of the ring terminal.\n"@en;
        rdfs:domain         vec:RingTerminalSpecification;
        rdfs:label          "thickness"@en;
        rdfs:range          vec:NumericalValue;
        rdfs:subPropertyOf  vec:contains .

vec:SiPrefix_Zetta  rdf:type  vec:SiPrefix , owl:NamedIndividiual;
        vec:enumLiteral  "Zetta" .

vec:NominalVoltage_24V
        rdf:type         vec:NominalVoltage , owl:NamedIndividiual;
        vec:enumLiteral  "24V" .

vec:SiUnitName_Tesla  rdf:type  vec:SiUnitName , owl:NamedIndividiual;
        vec:enumLiteral  "Tesla" .

vec:SiUnitName_Mole  rdf:type  vec:SiUnitName , owl:NamedIndividiual;
        vec:enumLiteral  "Mole" .

vec:partUsageSpecificationPartUsage
        rdf:type            owl:ObjectProperty;
        rdfs:comment        "Specifies the PartUsages defined by the PartUsageSpecification.\n"@en;
        rdfs:domain         vec:PartUsageSpecification;
        rdfs:label          "partUsage"@en;
        rdfs:range          vec:PartUsage;
        rdfs:subPropertyOf  vec:contains .

vec:BoltMountedFixingBoltShape_Square
        rdf:type         vec:BoltMountedFixingBoltShape , owl:NamedIndividiual;
        vec:enumLiteral  "Square" .

vec:CavityReference  rdf:type  owl:Class;
        rdfs:comment     "A CavityReference represents the usage of a Cavity in the context of PartUsage or PartOccurrence.\n"@en;
        rdfs:label       "CavityReference"@en;
        rdfs:subClassOf  vec:ExtendableElement .

vec:PartVersion  rdf:type  owl:Class;
        rdfs:comment     "The PartVersion is one of the two anchors for PDM information in the VEC. All technical information about a PartVersion is contained in one or more documents. These describing elements are normally referencing to the PartVersion.\n"@en;
        rdfs:label       "PartVersion"@en;
        rdfs:subClassOf  vec:ItemVersion .

vec:placementPointReferenceIdentification
        rdf:type      owl:DatatypeProperty;
        rdfs:comment  "Specifies a unique identification of the PlacementPointReference. The identification is guaranteed to be unique within the containing PlaceableElementRole.\n"@en;
        rdfs:domain   vec:PlacementPointReference;
        rdfs:label    "identification"@en;
        rdfs:range    xs:string .

vec:PartStructureContentType_Assembly
        rdf:type         vec:PartStructureContentType , owl:NamedIndividiual;
        rdfs:comment     "Definition of part / component without variance, that has a bill of material (100%)."@en;
        vec:enumLiteral  "Assembly" .

vec:CartesianDimension
        rdf:type         owl:Class;
        rdfs:comment     "The CartesianDimension specifies the size of an object in 2D-space. "@en;
        rdfs:label       "CartesianDimension"@en;
        rdfs:subClassOf  vec:ExtendableElement .

vec:SignalDirection  rdf:type  owl:Class;
        rdfs:comment         "Enumeration for the definition of SignalDirections.\n"@en;
        rdfs:label           "SignalDirection"@en;
        rdfs:subClassOf      vec:ClosedEnumeration;
        owl:equivalentClass  [ rdf:type   owl:Class;
                               owl:oneOf  ( vec:SignalDirection_In vec:SignalDirection_Out vec:SignalDirection_InOut )
                             ] .

vec:WireSpecification
        rdf:type         owl:Class;
        rdfs:comment     "Specification for the definition of a wire. This can either be a complex multicore wire or a normal single core. In the VEC a wire is defined by one WireElement, which may be composed from other WireElements.\n"@en;
        rdfs:label       "WireSpecification"@en;
        rdfs:subClassOf  vec:PartOrUsageRelatedSpecification .

vec:componentNodeDescription
        rdf:type            owl:ObjectProperty;
        rdfs:comment        "Room for additional, human readable information about the ComponentNode.\n"@en;
        rdfs:domain         vec:ComponentNode;
        rdfs:label          "description"@en;
        rdfs:range          vec:AbstractLocalizedString;
        rdfs:subPropertyOf  vec:contains .

vec:topologyMappingSpecificationInnerTopolgy
        rdf:type     owl:ObjectProperty;
        rdfs:domain  vec:TopologyMappingSpecification;
        rdfs:label   "innerTopolgy"@en;
        rdfs:range   vec:TopologySpecification .

vec:SignalTransmissionMediumType_Acoustic
        rdf:type         vec:SignalTransmissionMediumType , owl:NamedIndividiual;
        vec:enumLiteral  "acoustic" .

vec:pinComponentBehaviorCurrentInformation
        rdf:type            owl:ObjectProperty;
        rdfs:comment        "Specifies the current information of the PinComponent in this PinComponentBehavior . Since the current values of a pin can be defined for different types and times it is possible to define multiple PinCurrentInformations for a PinComponentBehavior .\n"@en;
        rdfs:domain         vec:PinComponentBehavior;
        rdfs:label          "currentInformation"@en;
        rdfs:range          vec:PinCurrentInformation;
        rdfs:subPropertyOf  vec:contains .

vec:documentVersionSpecification
        rdf:type            owl:ObjectProperty;
        rdfs:comment        "Specifies the Specifications contained in the DocumentVersion. All structured, technical information in the VEC is described by such Specifications. \n"@en;
        rdfs:domain         vec:DocumentVersion;
        rdfs:label          "specification"@en;
        rdfs:range          vec:Specification;
        rdfs:subPropertyOf  vec:contains .

vec:eEComponentSpecificationHousingComponent
        rdf:type            owl:ObjectProperty;
        rdfs:comment        "Specifies the available connector interfaces of the EEComponent. \n"@en;
        rdfs:domain         vec:EEComponentSpecification;
        rdfs:label          "housingComponent"@en;
        rdfs:range          vec:HousingComponent;
        rdfs:subPropertyOf  vec:contains .

vec:wireGroupingIdentification
        rdf:type      owl:DatatypeProperty;
        rdfs:comment  "Specifies a unique identification of the WireGrouping. The identification is guaranteed to be unique within the WireGroupingSpecification.\n"@en;
        rdfs:domain   vec:WireGrouping;
        rdfs:label    "identification"@en;
        rdfs:range    xs:string .

vec:potentialDistributorSpecificationBoltType
        rdf:type            owl:ObjectProperty;
        rdfs:comment        "Specifies the type of the bolt to which the potential distributor is compatible.\n┬á\n"@en;
        rdfs:domain         vec:PotentialDistributorSpecification;
        rdfs:label          "boltType"@en;
        rdfs:range          vec:TerminalBoltType;
        rdfs:subPropertyOf  vec:contains .

vec:LanguageCode_Da  rdf:type  vec:LanguageCode , owl:NamedIndividiual;
        vec:enumLiteral  "Da" .

vec:PartRelationType_OneOfAll
        rdf:type         vec:PartRelationType , owl:NamedIndividiual;
        rdfs:comment     " OneOfAll means that in a usage of a component exactly one of the referenced acessoryParts must be selected.\n"@en;
        vec:enumLiteral  "OneOfAll" .

vec:partOccurrencePart
        rdf:type      owl:ObjectProperty;
        rdfs:comment  "References the PartVersion that is instantiated by this PartOccurrence.\n"@en;
        rdfs:domain   vec:PartOccurrence;
        rdfs:label    "part"@en;
        rdfs:range    vec:PartVersion .

vec:slotPermittedTerminalSupplierCompanyNames
        rdf:type      owl:DatatypeProperty;
        rdfs:comment  "If this attribute is defined, it is only permitted to use terminals of one of the listed terminal suppliers.\nThe used company name shall be same as the one used as PartVersion.companyName for part numbers of this supplier.\n"@en;
        rdfs:domain   vec:Slot;
        rdfs:label    "permittedTerminalSupplierCompanyNames"@en;
        rdfs:range    xs:string .

vec:TerminalBoltNominalSize_M1.2
        rdf:type         vec:TerminalBoltNominalSize , owl:NamedIndividiual;
        vec:enumLiteral  "M1.2" .

vec:geometrySegmentIdentification
        rdf:type      owl:DatatypeProperty;
        rdfs:comment  "Specifies a unique identification of the GeometrySegment. The identification is guaranteed to be unique within the corresponding BuildingBlockSpecification. For all VEC-documents a GeometrySegment-instance can be trusted to be the same if the BuildingBlockSpecification-instance is the same (see BuildingBlockSpecification) and the identification of the GeometrySegment is the same.\n"@en;
        rdfs:domain   vec:GeometrySegment;
        rdfs:label    "identification"@en;
        rdfs:range    xs:string .

vec:NetSpecification  rdf:type  owl:Class;
        rdfs:comment     "Specification for the description of electrological nets.\n"@en;
        rdfs:label       "NetSpecification"@en;
        rdfs:subClassOf  vec:Specification .

vec:TopologyMappingSpecification
        rdf:type         owl:Class;
        rdfs:comment     "A┬á TopologyMappingSpecification allows the definition of hierarchical topologies. It relates an outer topology with an enclosed inner topology.\n"@en;
        rdfs:label       "TopologyMappingSpecification"@en;
        rdfs:subClassOf  vec:Specification .

vec:wireReceptionSpecificationCrimpConnectionLength
        rdf:type            owl:ObjectProperty;
        rdfs:comment        "Specifies the length of the crimp area, conductor + insulation crimp (wire reception, see diagram \"Terminal Dimensions\").\n"@en;
        rdfs:domain         vec:WireReceptionSpecification;
        rdfs:label          "crimpConnectionLength"@en;
        rdfs:range          vec:NumericalValue;
        rdfs:subPropertyOf  vec:contains .

vec:SegmentLength  rdf:type  owl:Class;
        rdfs:comment     "Specifies the length of a TopologySegment . The length of a TopologySegment is defined as the length of the centerline of the segment.\nAttributes of the type SegmentLength normally have the multiplicity [0..*]. This means that such an attribute can have SegmentLength-entries for different classifications. It must not have multiple entries with the same classification.\n"@en;
        rdfs:label       "SegmentLength"@en;
        rdfs:subClassOf  vec:ExtendableElement .

vec:documentRelatedAssignmentGroupRelatedIdentification
        rdf:type      owl:DatatypeProperty;
        rdfs:comment  "If this group relates to a specific element in the relatedDocumentVersion the identifier of the element is defined in this attribute (e.g. a requirements number).\n"@en;
        rdfs:domain   vec:DocumentRelatedAssignmentGroup;
        rdfs:label    "relatedIdentification"@en;
        rdfs:range    xs:string .

vec:mappingA  rdf:type  owl:ObjectProperty;
        rdfs:comment  ""@en;
        rdfs:domain   vec:Mapping;
        rdfs:label    "A"@en;
        rdfs:range    vec:PartVersion .

vec:placementPointSupplementaryParts
        rdf:type      owl:ObjectProperty;
        rdfs:comment  "References the PartRelations that specify supplementary parts for this PlacementPoint , e.g. cable ties for attaching the component on the harness.\n"@en;
        rdfs:domain   vec:PlacementPoint;
        rdfs:label    "supplementaryParts"@en;
        rdfs:range    vec:PartRelation .

vec:wireGroupingContainedWireGroupings
        rdf:type            owl:ObjectProperty;
        rdfs:comment        "References the WireGroupings that are contained in this WireGrouping .\n"@en;
        rdfs:domain         vec:WireGrouping;
        rdfs:label          "containedWireGroupings"@en;
        rdfs:range          vec:WireGrouping;
        rdfs:subPropertyOf  vec:contains .

vec:sIUnitSiUnitName  rdf:type  owl:ObjectProperty;
        rdfs:comment        "Specifies the name of SI unit (e.g. metre, second,...)\n"@en;
        rdfs:domain         vec:SIUnit;
        rdfs:label          "siUnitName"@en;
        rdfs:range          vec:SiUnitName;
        rdfs:subPropertyOf  vec:contains .

vec:LevelOfApproval_Restricted
        rdf:type         vec:LevelOfApproval , owl:NamedIndividiual;
        rdfs:comment     "The Usage of the ItemVersion is restricted in some way. See additionalLevelInformation for more details.\n"@en;
        vec:enumLiteral  "Restricted" .

vec:PrimaryPartType_Capacitor
        rdf:type         vec:PrimaryPartType , owl:NamedIndividiual;
        vec:enumLiteral  "Capacitor" .

vec:TypeOfPermission_Checked
        rdf:type         vec:TypeOfPermission , owl:NamedIndividiual;
        vec:enumLiteral  "Checked" .

vec:PrimaryPartType_PotentialDistributor
        rdf:type         vec:PrimaryPartType , owl:NamedIndividiual;
        vec:enumLiteral  "PotentialDistributor" .

vec:LanguageCode_Na  rdf:type  vec:LanguageCode , owl:NamedIndividiual;
        vec:enumLiteral  "Na" .

vec:GeometryNode  rdf:type  owl:Class;
        rdfs:comment     "A GeometryNode is the geometric representation of a TopologyNode. A TopologyNode may be represented by more than one GeometryNodes, but only within different BuildingBlockSpecification2D/3D. That means, in a single BuildingBlockSpecification a TopologyNode shall only be represent once┬á(or not).\nA GeometryNode is either a GeometryNode2D or a GeometryNode3D.\n"@en;
        rdfs:label       "GeometryNode"@en;
        rdfs:subClassOf  vec:ConfigurableElement .

vec:variantCodeAliasId
        rdf:type            owl:ObjectProperty;
        rdfs:comment        "Room to specify additional identifiers for the VariantCode.\n"@en;
        rdfs:domain         vec:VariantCode;
        rdfs:label          "aliasId"@en;
        rdfs:range          vec:AliasIdentification;
        rdfs:subPropertyOf  vec:contains .

vec:matingDetailIdentification
        rdf:type     owl:DatatypeProperty;
        rdfs:domain  vec:MatingDetail;
        rdfs:label   "identification"@en;
        rdfs:range   xs:string .

vec:NetworkNodeSubType_Speaker
        rdf:type         vec:NetworkNodeSubType , owl:NamedIndividiual;
        vec:enumLiteral  "Speaker" .

vec:PrimaryPartType_Antenna
        rdf:type         vec:PrimaryPartType , owl:NamedIndividiual;
        vec:enumLiteral  "Antenna" .

vec:PrimaryPartType_Tape
        rdf:type         vec:PrimaryPartType , owl:NamedIndividiual;
        vec:enumLiteral  "Tape" .

vec:topologyZoneDescription
        rdf:type            owl:ObjectProperty;
        rdfs:comment        "Specifies additional, human readable information about the zone.\n"@en;
        rdfs:domain         vec:TopologyZone;
        rdfs:label          "description"@en;
        rdfs:range          vec:AbstractLocalizedString;
        rdfs:subPropertyOf  vec:contains .

vec:StripeSpecification
        rdf:type         owl:Class;
        rdfs:comment     "Specifies a stripe which has fixed length and width. A stripe is a textile, foam or similar piece with fixed length &┬áwidth that is wrapped around the harness.\n"@en;
        rdfs:label       "StripeSpecification"@en;
        rdfs:subClassOf  vec:WireProtectionSpecification .

vec:itemHistoryEntryPredecessorVersion
        rdf:type      owl:ObjectProperty;
        rdfs:comment  "References the ItemVersion that is the predecessor in the ItemHistoryEntry. \n"@en;
        rdfs:domain   vec:ItemHistoryEntry;
        rdfs:label    "predecessorVersion"@en;
        rdfs:range    vec:ItemVersion .

vec:wireElementSpecificationSuitedForDynamicUse
        rdf:type      owl:DatatypeProperty;
        rdfs:comment  "Specifies if it is allowed to use the WireElement in a dynamic environment. (see KBLFRM-311)\n"@en;
        rdfs:domain   vec:WireElementSpecification;
        rdfs:label    "suitedForDynamicUse"@en;
        rdfs:range    xs:boolean .

vec:LanguageCode_Be  rdf:type  vec:LanguageCode , owl:NamedIndividiual;
        vec:enumLiteral  "Be" .

vec:TerminalBoltType_Snappable
        rdf:type         vec:TerminalBoltType , owl:NamedIndividiual;
        rdfs:comment     "A bolt with a groove or similiar that allows the counter part to snap on."@en;
        vec:enumLiteral  "Snappable" .

vec:CableLeadThroughType_WithSealingComponent
        rdf:type         vec:CableLeadThroughType , owl:NamedIndividiual;
        rdfs:comment     "Literal used when the CableLeadThrough is sealed with an additional sealing component (a \"cavity seal\").\n"@en;
        vec:enumLiteral  "WithSealingComponent" .

vec:VariantGroupType_LogicalGroup
        rdf:type         vec:VariantGroupType , owl:NamedIndividiual;
        rdfs:comment     "Defines a logical grouping on variant codes. However, no semantic constraint is implied."@en;
        vec:enumLiteral  "LogicalGroup" .

vec:pinComponentReferencedCavity
        rdf:type      owl:ObjectProperty;
        rdfs:comment  "Defines the cavity in the corresponding ConnectorHousingSpecification of the HousingComponent where the PinComponent is located. \n(see KBLFRM-300)\n"@en;
        rdfs:domain   vec:PinComponent;
        rdfs:label    "referencedCavity"@en;
        rdfs:range    vec:Cavity .

vec:HousingComponentType_Relay
        rdf:type         vec:HousingComponentType , owl:NamedIndividiual;
        vec:enumLiteral  "Relay" .

vec:TemperatureType_OperatingTemperature
        rdf:type         vec:TemperatureType , owl:NamedIndividiual;
        vec:enumLiteral  "OperatingTemperature" .

vec:TerminalBoltNominalSize_M18
        rdf:type         vec:TerminalBoltNominalSize , owl:NamedIndividiual;
        vec:enumLiteral  "M18" .

vec:eEComponentSpecificationStates
        rdf:type            owl:ObjectProperty;
        rdfs:comment        "Specifies the available SwitchingStates of the EEComponent.\n"@en;
        rdfs:domain         vec:EEComponentSpecification;
        rdfs:label          "states"@en;
        rdfs:range          vec:SwitchingState;
        rdfs:subPropertyOf  vec:contains .

vec:ContractRole_Oem  rdf:type  vec:ContractRole , owl:NamedIndividiual;
        vec:enumLiteral  "Oem" .

vec:documentVersionDocumentVersion
        rdf:type      owl:DatatypeProperty;
        rdfs:comment  "The documentVersion specifies the version index of a document (see also documentNumber).\n"@en;
        rdfs:domain   vec:DocumentVersion;
        rdfs:label    "documentVersion"@en;
        rdfs:range    xs:string .

vec:SiPrefix_Exa  rdf:type  vec:SiPrefix , owl:NamedIndividiual;
        vec:enumLiteral  "Exa" .

vec:aliasIdentificationIdentificationValue
        rdf:type      owl:DatatypeProperty;
        rdfs:comment  "Specifies the identification value.\n"@en;
        rdfs:domain   vec:AliasIdentification;
        rdfs:label    "identificationValue"@en;
        rdfs:range    xs:string .

vec:sealedCavitiesAssignmentSealedCavities
        rdf:type      owl:ObjectProperty;
        rdfs:comment  "Specifies the Cavities that are sealed.\n"@en;
        rdfs:domain   vec:SealedCavitiesAssignment;
        rdfs:label    "sealedCavities"@en;
        rdfs:range    vec:Cavity .

vec:transformation3DA23
        rdf:type     owl:DatatypeProperty;
        rdfs:domain  vec:Transformation3D;
        rdfs:label   "a23"@en;
        rdfs:range   xs:double .

[ rdf:type     owl:AllDisjointClasses;
  owl:members  ( vec:GeometrySegment2D vec:GeometrySegment3D )
] .

vec:PrimaryPartType_CavitySeal
        rdf:type         vec:PrimaryPartType , owl:NamedIndividiual;
        vec:enumLiteral  "CavitySeal" .

vec:WindingType_DoubleOverlap
        rdf:type         vec:WindingType , owl:NamedIndividiual;
        rdfs:comment     " DoubleOverlap describes a taping where each round overlaps the preceeding round and the taping is done twice (forward and backwards).\n"@en;
        vec:enumLiteral  "DoubleOverlap" .

vec:usageNodeUsageNodeType
        rdf:type            owl:ObjectProperty;
        rdfs:comment        "Defines the type of the UsageNode. The type determines how the UsageNode is handled in the latter processes.\n"@en;
        rdfs:domain         vec:UsageNode;
        rdfs:label          "usageNodeType"@en;
        rdfs:range          vec:UsageNodeType;
        rdfs:subPropertyOf  vec:contains .

vec:TerminalBoltNominalSize_M39
        rdf:type         vec:TerminalBoltNominalSize , owl:NamedIndividiual;
        vec:enumLiteral  "M39" .

vec:cavitySpecificationMaxWireElementOutsideDiameter
        rdf:type            owl:ObjectProperty;
        rdfs:comment        "Specifies the maximum diameter a wire is allowed to have to fit into the cavity.\n"@en;
        rdfs:domain         vec:CavitySpecification;
        rdfs:label          "maxWireElementOutsideDiameter"@en;
        rdfs:range          vec:NumericalValue;
        rdfs:subPropertyOf  vec:contains .

vec:housingComponentCompatibleTypes
        rdf:type            owl:ObjectProperty;
        rdfs:comment        "The values of this attribute define the HousingComponentTypes that are valid to be associated with this HousingComponent. In other word, if this HousingComponent can be associated with a relay, a fuse, a connector housing of a harness. The values are matching the PrimaryPartType of the PartVersion of the component that should be associated (plugged) into this housing component.\n"@en;
        rdfs:domain         vec:HousingComponent;
        rdfs:label          "compatibleTypes"@en;
        rdfs:range          vec:HousingComponentType;
        rdfs:subPropertyOf  vec:contains .

vec:WireGroupingSpecification
        rdf:type         owl:Class;
        rdfs:comment     "Specification for the description of WireGroupings.\n"@en;
        rdfs:label       "WireGroupingSpecification"@en;
        rdfs:subClassOf  vec:Specification .

vec:generalTechnicalPartSpecificationUnspecifiedAccessoryPermitted
        rdf:type      owl:DatatypeProperty;
        rdfs:comment  "Defines whether accessories which are not explicitly defined by a PartRelation may be used with instances of this part. If this attribute is not specified the default value is true.\n"@en;
        rdfs:domain   vec:GeneralTechnicalPartSpecification;
        rdfs:label    "unspecifiedAccessoryPermitted"@en;
        rdfs:range    xs:boolean .

vec:assignmentGroupIdentification
        rdf:type      owl:DatatypeProperty;
        rdfs:comment  "Specifies a unique identification of the AssignmentGroup. The identification is guaranteed to be unique within the specification.\n"@en;
        rdfs:domain   vec:AssignmentGroup;
        rdfs:label    "identification"@en;
        rdfs:range    xs:string .

vec:cavityPositionDetailBaseUnit
        rdf:type      owl:ObjectProperty;
        rdfs:comment  "The Unit in which all coordinates (e.g. cartesian points) of this CavityPositionDetail┬á are defined. Shall be a unit of length┬á(e.g. millimetre).\n"@en;
        rdfs:domain   vec:CavityPositionDetail;
        rdfs:label    "baseUnit"@en;
        rdfs:range    vec:Unit .

vec:ComponentNodeSubType_Speaker
        rdf:type         vec:ComponentNodeSubType , owl:NamedIndividiual;
        vec:enumLiteral  "Speaker" .

vec:MatingDetail  rdf:type  owl:Class;
        rdfs:comment     "If the mating of the two terminals is not unambiguously, a MatingDetail can specify the TerminalReceptions that are mated.\n"@en;
        rdfs:label       "MatingDetail"@en;
        rdfs:subClassOf  vec:ExtendableElement .

vec:wireGroupingWireGroupSpecification
        rdf:type      owl:ObjectProperty;
        rdfs:comment  "References the WireGroupSpecification that applies to the WireGrouping .\n"@en;
        rdfs:domain   vec:WireGrouping;
        rdfs:label    "wireGroupSpecification"@en;
        rdfs:range    vec:WireGroupSpecification .

vec:cartesianVector3DX
        rdf:type      owl:DatatypeProperty;
        rdfs:comment  "Specifies the x-coordinate in 3D space.\n"@en;
        rdfs:domain   vec:CartesianVector3D;
        rdfs:label    "x"@en;
        rdfs:range    xs:double .

vec:LabelType_AlphaNumerical
        rdf:type         vec:LabelType , owl:NamedIndividiual;
        vec:enumLiteral  "AlphaNumerical" .

vec:wireElementReferenceSignal
        rdf:type      owl:ObjectProperty;
        rdfs:comment  "References the signal that is transmitted by the WireElementReference.\n"@en;
        rdfs:domain   vec:WireElementReference;
        rdfs:label    "signal"@en;
        rdfs:range    vec:Signal .

vec:ModuleFamilySpecification
        rdf:type         owl:Class;
        rdfs:comment     "Specification for the description of module families (see ModuleFamily).\n"@en;
        rdfs:label       "ModuleFamilySpecification"@en;
        rdfs:subClassOf  vec:Specification .

vec:HousingComponentType_Terminal
        rdf:type         vec:HousingComponentType , owl:NamedIndividiual;
        vec:enumLiteral  "Terminal" .

vec:SiPrefix_Atto  rdf:type  vec:SiPrefix , owl:NamedIndividiual;
        vec:enumLiteral  "Atto" .

vec:connectionSpecificationConnection
        rdf:type            owl:ObjectProperty;
        rdfs:comment        "Specifies the Connection defined by the ConnectionSpecification.\n"@en;
        rdfs:domain         vec:ConnectionSpecification;
        rdfs:label          "connection"@en;
        rdfs:range          vec:Connection;
        rdfs:subPropertyOf  vec:contains .

vec:ConductorCurrentInformation
        rdf:type      owl:Class;
        rdfs:comment  "The ConductorCurrentInformation specifies the maximum current for which a conductor is approved. As the maximum current is dependent from the voltage and the environment temperature it is modelled as a class and not only as an attribute.\n"@en;
        rdfs:label    "ConductorCurrentInformation"@en .

vec:CavityPlugSpecification
        rdf:type         owl:Class;
        rdfs:comment     "Specification for the definition of cavity seals. A cavity plug is a watertight non-electrical object to fill an empty cavity.\n"@en;
        rdfs:label       "CavityPlugSpecification"@en;
        rdfs:subClassOf  vec:CavityPartSpecification .

vec:configurationConstraintApplicationConstraint
        rdf:type      owl:ObjectProperty;
        rdfs:comment  "References the application constraint that applies to the ConfigurationConstraint.\n"@en;
        rdfs:domain   vec:ConfigurationConstraint;
        rdfs:label    "applicationConstraint"@en;
        rdfs:range    vec:ApplicationConstraint .

vec:PartStructureSpecification
        rdf:type         owl:Class;
        rdfs:comment     "Specification for the description of a part structure. This specification defines the PartOccurrences that are in the bill of material of the described PartOrUsage. This is necessary, because it is possible, that for a definite description a Part more PartOccurrences are needed than the ones that are in the bill of material (see CompositionSpecification).\n"@en;
        rdfs:label       "PartStructureSpecification"@en;
        rdfs:subClassOf  vec:PartOrUsageRelatedSpecification .

vec:SignalSubType_APIX3
        rdf:type         vec:SignalSubType , owl:NamedIndividiual;
        vec:enumLiteral  "APIX3" .

vec:permissionPermission
        rdf:type            owl:ObjectProperty;
        rdfs:comment        "Specifies the type of permission. Predefined values are: Seen, Checked, Released.\n"@en;
        rdfs:domain         vec:Permission;
        rdfs:label          "permission"@en;
        rdfs:range          vec:TypeOfPermission;
        rdfs:subPropertyOf  vec:contains .

[ rdf:type     owl:AllDisjointClasses;
  owl:members  ( vec:CartesianVector2D vec:CartesianVector3D )
] .

vec:conductorSpecificationType
        rdf:type            owl:ObjectProperty;
        rdfs:comment        "Specifies the type of the conductor, e.g. if it is rigid or stranded.\n"@en;
        rdfs:domain         vec:ConductorSpecification;
        rdfs:label          "type"@en;
        rdfs:range          vec:ConductorType;
        rdfs:subPropertyOf  vec:contains .

vec:ComponentPortViewItemSide_Right
        rdf:type         vec:ComponentPortViewItemSide , owl:NamedIndividiual;
        vec:enumLiteral  "Right" .

vec:CavityPartSpecification
        rdf:type         owl:Class;
        rdfs:comment     "The CavityPartSpecification is an abstract class for common properties of non-electrical parts that are used in Cavities .\n"@en;
        rdfs:label       "CavityPartSpecification"@en;
        rdfs:subClassOf  vec:PartOrUsageRelatedSpecification .

vec:SealingGeometry_Square
        rdf:type         vec:SealingGeometry , owl:NamedIndividiual;
        vec:enumLiteral  "Square" .

vec:assignmentGroupDescription
        rdf:type            owl:ObjectProperty;
        rdfs:comment        "Specifies additional, human readable information about the AssignmentGroup .\n"@en;
        rdfs:domain         vec:AssignmentGroup;
        rdfs:label          "description"@en;
        rdfs:range          vec:AbstractLocalizedString;
        rdfs:subPropertyOf  vec:contains .

vec:massInformationDeterminationType
        rdf:type            owl:ObjectProperty;
        rdfs:comment        "Specifies the determination type of the mass information.\n"@en;
        rdfs:domain         vec:MassInformation;
        rdfs:label          "determinationType"@en;
        rdfs:range          vec:ValueDetermination;
        rdfs:subPropertyOf  vec:contains .

vec:ComponentConnector
        rdf:type         owl:Class;
        rdfs:comment     "A ComponentConnector is a grouping of ComponentPorts and represents a logical abstraction of a connector of an EEComponent . When the ComponentNode is realized by an EEComponentRole the ComponentConnector will result in a HousingComponent.\nIt is permitted that a ComponentConnector is a 150% definition of connector.\n"@en;
        rdfs:label       "ComponentConnector"@en;
        rdfs:subClassOf  vec:ConfigurableElement .

vec:PrimaryPartType_PluggableTerminal
        rdf:type         vec:PrimaryPartType , owl:NamedIndividiual;
        vec:enumLiteral  "PluggableTerminal" .

vec:fittingOutletNominalSize
        rdf:type      owl:DatatypeProperty;
        rdfs:comment  "Defines the nominal size of a tube. The nominal size is a name for the size of the tube that is somehow related to the inner diameter of the tube. However, it is not the inner diameter (e.g. \"10.5\").\n"@en;
        rdfs:domain   vec:FittingOutlet;
        rdfs:label    "nominalSize"@en;
        rdfs:range    xs:string .

vec:LanguageCode_Ji  rdf:type  vec:LanguageCode , owl:NamedIndividiual;
        vec:enumLiteral  "Ji" .

vec:transformation3DOrigin
        rdf:type      owl:ObjectProperty;
        rdfs:comment  "Specifies the coordinates of the translation.\n"@en;
        rdfs:domain   vec:Transformation3D;
        rdfs:label    "origin"@en;
        rdfs:range    vec:CartesianPoint3D .

vec:onPointPlacementLocation
        rdf:type            owl:ObjectProperty;
        rdfs:comment        "References the Locations where Placement places the reference points of the placed element. \n"@en;
        rdfs:domain         vec:OnPointPlacement;
        rdfs:label          "location"@en;
        rdfs:range          vec:Location;
        rdfs:subPropertyOf  vec:contains .

vec:slotMappingIdentificationA
        rdf:type      owl:DatatypeProperty;
        rdfs:comment  "The identification of the Slot on side A\n"@en;
        rdfs:domain   vec:SlotMapping;
        rdfs:label    "identificationA"@en;
        rdfs:range    xs:string .

vec:SlotGender  rdf:type  owl:Class;
        rdfs:comment     "Defines the gender of a slot.\n"@en;
        rdfs:label       "SlotGender"@en;
        rdfs:subClassOf  vec:OpenEnumeration .

vec:iECUnitIecPrefix  rdf:type  owl:ObjectProperty;
        rdfs:comment        "Specifies the prefix of the IEC unit.\n"@en;
        rdfs:domain         vec:IECUnit;
        rdfs:label          "iecPrefix"@en;
        rdfs:range          vec:IECPrefix;
        rdfs:subPropertyOf  vec:contains .

vec:Dimension  rdf:type  owl:Class;
        rdfs:comment     "A Dimension defines a measurement for the distance between two Locations. An acceptable tolerance can be specified additionally. If the Locations are not located on adjacent topology-elements it is possible to specify a Path for the dimension along which the measurement must be taken.\nThe value for the Dimension is not specified as NumericalValue (which can define a Tolerance as well). This is because the \"valueComponent\" of the NumericalValue is mandatory. For Dimensions it shall be optional since there are scenarios where the dimension only specifies a Tolerance for a distance defined by the topology (segment length + placement information).\n"@en;
        rdfs:label       "Dimension"@en;
        rdfs:subClassOf  vec:ConfigurableElement .

vec:ConnectorHousingCapRole
        rdf:type         owl:Class;
        rdfs:comment     "A┬á ConnectorHousingCapRole defines the instance-specific properties of a cap for a connector (backshells).\n"@en;
        rdfs:label       "ConnectorHousingCapRole"@en;
        rdfs:subClassOf  vec:Role .

vec:PinType  rdf:type    owl:Class;
        rdfs:comment     "Defines the type of a pin.\n"@en;
        rdfs:label       "PinType"@en;
        rdfs:subClassOf  vec:OpenEnumeration .

vec:fittingSpecificationOutlet
        rdf:type            owl:ObjectProperty;
        rdfs:comment        ""@en;
        rdfs:domain         vec:FittingSpecification;
        rdfs:label          "outlet"@en;
        rdfs:range          vec:FittingOutlet;
        rdfs:subPropertyOf  vec:contains .

vec:insulationSpecificationLabelIdentificationType
        rdf:type            owl:ObjectProperty;
        rdfs:comment        "Specifies the type of a label printed, stamped or integrated on or in the insulation of the wire (e.g. alpha numerical, bar code).\n"@en;
        rdfs:domain         vec:InsulationSpecification;
        rdfs:label          "labelIdentificationType"@en;
        rdfs:range          vec:LabelType;
        rdfs:subPropertyOf  vec:contains .

vec:USUnitName_League
        rdf:type         vec:USUnitName , owl:NamedIndividiual;
        vec:enumLiteral  "League" .

vec:SiPrefix_Hecto  rdf:type  vec:SiPrefix , owl:NamedIndividiual;
        vec:enumLiteral  "Hecto" .

vec:ComponentNodeSubType_Fuse
        rdf:type         vec:ComponentNodeSubType , owl:NamedIndividiual;
        vec:enumLiteral  "Fuse" .

vec:pinComponentBehaviorSignal
        rdf:type      owl:ObjectProperty;
        rdfs:comment  "Specifies the Signal associated with the pin in this behavior.\n"@en;
        rdfs:domain   vec:PinComponentBehavior;
        rdfs:label    "signal"@en;
        rdfs:range    vec:Signal .

vec:HarnessGeometrySpecification3D
        rdf:type         owl:Class;
        rdfs:comment     "The HarnessGeometrieSpecification3D specifies a three-dimensional model of a harness. A harness model is composed of one or more BuildingBlockSpecifaction3D which are placed in the model.\n"@en;
        rdfs:label       "HarnessGeometrySpecification3D"@en;
        rdfs:subClassOf  vec:Specification .

[ rdf:type     owl:AllDisjointClasses;
  owl:members  ( vec:DocumentVersion vec:PartVersion )
] .

vec:protectionMaterialLengthLengthValue
        rdf:type            owl:ObjectProperty;
        rdfs:domain         vec:ProtectionMaterialLength;
        rdfs:label          "lengthValue"@en;
        rdfs:range          vec:NumericalValue;
        rdfs:subPropertyOf  vec:contains .

vec:signalAliasId  rdf:type  owl:ObjectProperty;
        rdfs:comment        "Specifies additional identifiers for the Signal .\n"@en;
        rdfs:domain         vec:Signal;
        rdfs:label          "aliasId"@en;
        rdfs:range          vec:AliasIdentification;
        rdfs:subPropertyOf  vec:contains .

vec:potentialDistributorSpecificationBoltNominalSize
        rdf:type            owl:ObjectProperty;
        rdfs:comment        "Defines the size (diameter) of the bolt for which the potential distributor is designed for in a nominal way (e.g. \"M8\").\n"@en;
        rdfs:domain         vec:PotentialDistributorSpecification;
        rdfs:label          "boltNominalSize"@en;
        rdfs:range          vec:TerminalBoltNominalSize;
        rdfs:subPropertyOf  vec:contains .

vec:TerminalSealingType
        rdf:type         owl:Class;
        rdfs:comment     "Defines the possible sealing types for a terminal, if the terminal shall be sealed in its usage.\n"@en;
        rdfs:label       "TerminalSealingType"@en;
        rdfs:subClassOf  vec:OpenEnumeration .

vec:NetworkNodeType_Sensor
        rdf:type         vec:NetworkNodeType , owl:NamedIndividiual;
        rdfs:comment     "A sensor is a device that detects changes to the environment and sends them as information to other devices (e.g. an ECU).\n"@en;
        vec:enumLiteral  "Sensor" .

vec:wireTupleTerminationFixation
        rdf:type      owl:DatatypeProperty;
        rdfs:comment  "Specifies if a fixation of the WireEnds is required."@en;
        rdfs:domain   vec:WireTupleTermination;
        rdfs:label    "fixation"@en;
        rdfs:range    xs:boolean .

vec:AbstractSlot  rdf:type  owl:Class;
        rdfs:comment     "An AbstractSlot is a geometrical place in a connector housing, which can contain / group cavities. This can be either direct, if it is Slot and indirect if it is a ModularSlot .\nIf it is a Slot , then it is an inseparable part of the connector housing, which means it is created during the manufacturing process of the connector housing.\nIf it is a ModularSlot it is a place where one or more other connector housing can be place during the assembly.\n"@en;
        rdfs:label       "AbstractSlot"@en;
        rdfs:subClassOf  vec:ExtendableElement .

vec:RobustnessClass_LiquidIngressProtection
        rdf:type         vec:RobustnessClass , owl:NamedIndividiual;
        vec:enumLiteral  "LiquidIngressProtection" .

vec:ConductorSpecification
        rdf:type         owl:Class;
        rdfs:comment     "Specification for the definition of conducting properties of a WireElement.\n"@en;
        rdfs:label       "ConductorSpecification"@en;
        rdfs:subClassOf  vec:Specification .

vec:SiPrefix_Pico  rdf:type  vec:SiPrefix , owl:NamedIndividiual;
        vec:enumLiteral  "Pico" .

vec:BatterySpecification
        rdf:type         owl:Class;
        rdfs:comment     "Specification of the electrological aspects of a battery.\n"@en;
        rdfs:label       "BatterySpecification"@en;
        rdfs:subClassOf  vec:EEComponentSpecification .

vec:netSpecificationNetType
        rdf:type            owl:ObjectProperty;
        rdfs:domain         vec:NetSpecification;
        rdfs:label          "netType"@en;
        rdfs:range          vec:NetType;
        rdfs:subPropertyOf  vec:contains .

vec:GrommetType  rdf:type  owl:Class;
        rdfs:comment     ""@en;
        rdfs:label       "GrommetType"@en;
        rdfs:subClassOf  vec:OpenEnumeration .

vec:LanguageCode_Pl  rdf:type  vec:LanguageCode , owl:NamedIndividiual;
        vec:enumLiteral  "Pl" .

vec:connectionEndGender
        rdf:type            owl:ObjectProperty;
        rdfs:comment        "Specifies if the ConnectionEnd is male or female. This may be e.g. important in case of an inliner.\n"@en;
        rdfs:domain         vec:ConnectionEnd;
        rdfs:label          "gender"@en;
        rdfs:range          vec:ConnectionEndGender;
        rdfs:subPropertyOf  vec:contains .

vec:VariantConfigurationType_Technical
        rdf:type         vec:VariantConfigurationType , owl:NamedIndividiual;
        rdfs:comment     "The VariantConfiguration is a technical (feature or function oriented) key normally used in a building block set. In a concrete vehicle project those keys are mapped to specific logistic keys within the project."@en;
        vec:enumLiteral  "Technical" .

vec:LanguageCode_Bo  rdf:type  vec:LanguageCode , owl:NamedIndividiual;
        vec:enumLiteral  "Bo" .

vec:applicationConstraintToDate
        rdf:type      owl:DatatypeProperty;
        rdfs:comment  "Specifies the upper bound of the time period to which the application constraint applies.\n"@en;
        rdfs:domain   vec:ApplicationConstraint;
        rdfs:label    "toDate"@en;
        rdfs:range    xs:dateTime .

vec:partOccurrenceInstanciatedOccurrence
        rdf:type      owl:ObjectProperty;
        rdfs:comment  "References the PartOccurrence which is instantiated by the PartOccurrence. This reference is for example needed in the case of usage of assemblies.\n"@en;
        rdfs:domain   vec:PartOccurrence;
        rdfs:label    "instanciatedOccurrence"@en;
        rdfs:range    vec:PartOccurrence .

vec:VariantCodeType_Prototype
        rdf:type         vec:VariantCodeType , owl:NamedIndividiual;
        rdfs:comment     ""@en;
        vec:enumLiteral  "Prototype" .

vec:connectionDescription
        rdf:type            owl:ObjectProperty;
        rdfs:comment        "Specifies additional, human readable information about the Connection.\n"@en;
        rdfs:domain         vec:Connection;
        rdfs:label          "description"@en;
        rdfs:range          vec:AbstractLocalizedString;
        rdfs:subPropertyOf  vec:contains .

vec:CavityAccessorySpecification
        rdf:type         owl:Class;
        rdfs:comment     "A CavityAccessory is a non-electrical part used in a cavity with no sealing properties (e.g. a wire fixation).\n"@en;
        rdfs:label       "CavityAccessorySpecification"@en;
        rdfs:subClassOf  vec:CavityPartSpecification .

vec:componentPortDescription
        rdf:type            owl:ObjectProperty;
        rdfs:comment        "Room for additional, human readable information about the ComponentPort.\n"@en;
        rdfs:domain         vec:ComponentPort;
        rdfs:label          "description"@en;
        rdfs:range          vec:AbstractLocalizedString;
        rdfs:subPropertyOf  vec:contains .

vec:ImperialUnitName_Yard
        rdf:type         vec:ImperialUnitName , owl:NamedIndividiual;
        vec:enumLiteral  "Yard" .

vec:LanguageCode_Rm  rdf:type  vec:LanguageCode , owl:NamedIndividiual;
        vec:enumLiteral  "Rm" .

vec:TemperatureType_ProcessingTemperature
        rdf:type         vec:TemperatureType , owl:NamedIndividiual;
        vec:enumLiteral  "ProcessingTemperature" .

vec:Instruction  rdf:type  owl:Class;
        rdfs:comment     "Abstract super class to specify different types of instructions. Possible instructions are text, file or document based.\n"@en;
        rdfs:label       "Instruction"@en;
        rdfs:subClassOf  vec:ExtendableElement .

vec:usageNodeDescription
        rdf:type            owl:ObjectProperty;
        rdfs:comment        "Specifies additional, human readable information about the UsageNode .\n"@en;
        rdfs:domain         vec:UsageNode;
        rdfs:label          "description"@en;
        rdfs:range          vec:AbstractLocalizedString;
        rdfs:subPropertyOf  vec:contains .

vec:connectorHousingSpecificationCoding
        rdf:type            owl:ObjectProperty;
        rdfs:comment        "Defines coding of the connector housing that is satisfied by the connector housing. \n"@en;
        rdfs:domain         vec:ConnectorHousingSpecification;
        rdfs:label          "coding"@en;
        rdfs:range          vec:Coding;
        rdfs:subPropertyOf  vec:contains .

vec:SwitchingState  rdf:type  owl:Class;
        rdfs:comment     "A SwitchingState defines a certain static state of an EEComponent . Under which conditions or when such a state applies, should be described in an external description model.\nA SwitchingState references a collection of InternalComponentConnections , with the semantic that these connections exist (and only these connections) when the switching state is active.\n"@en;
        rdfs:label       "SwitchingState"@en;
        rdfs:subClassOf  vec:ConfigurableElement .

vec:LanguageCode_Lo  rdf:type  vec:LanguageCode , owl:NamedIndividiual;
        vec:enumLiteral  "Lo" .

[ rdf:type     owl:AllDisjointClasses;
  owl:members  ( vec:FittingSpecification vec:StripeSpecification vec:TapeSpecification vec:TubeSpecification )
] .

vec:placeableElementRolePlacementPointReference
        rdf:type            owl:ObjectProperty;
        rdfs:comment        ""@en;
        rdfs:domain         vec:PlaceableElementRole;
        rdfs:label          "placementPointReference"@en;
        rdfs:range          vec:PlacementPointReference;
        rdfs:subPropertyOf  vec:contains .

vec:tapeSpecificationCoilCoreDiameter
        rdf:type            owl:ObjectProperty;
        rdfs:comment        "Specifies the inner diameter of the coil on which the tape is delivered.\n"@en;
        rdfs:domain         vec:TapeSpecification;
        rdfs:label          "coilCoreDiameter"@en;
        rdfs:range          vec:NumericalValue;
        rdfs:subPropertyOf  vec:contains .

vec:FixingRole  rdf:type  owl:Class;
        rdfs:comment     "A FixingRole defines the instance specific properties and relationships of a fixing.\n"@en;
        rdfs:label       "FixingRole"@en;
        rdfs:subClassOf  vec:Role .

vec:LanguageCode_Tn  rdf:type  vec:LanguageCode , owl:NamedIndividiual;
        vec:enumLiteral  "Tn" .

vec:GrommetMountingType_MultiPiece
        rdf:type         vec:GrommetMountingType , owl:NamedIndividiual;
        rdfs:comment     "The grommet consists of multiple parts that are assembled arround the harness to create the final appearance."@en;
        vec:enumLiteral  "MultiPiece" .

vec:cavityMountingDetailEquippedCavityRef
        rdf:type      owl:ObjectProperty;
        rdfs:comment  "References the cavity that is used for the detailed description of the cavity mounting. \n"@en;
        rdfs:domain   vec:CavityMountingDetail;
        rdfs:label    "equippedCavityRef"@en;
        rdfs:range    vec:CavityReference .

vec:routingSpecialRouted
        rdf:type      owl:DatatypeProperty;
        rdfs:comment  "Specifies that routing has been created in a special way. This means it has not been calculated in the standard way, because for some reason the result of the standard calculation has been inconvenient.\n"@en;
        rdfs:domain   vec:Routing;
        rdfs:label    "specialRouted"@en;
        rdfs:range    xs:boolean .

vec:DocumentType  rdf:type  owl:Class;
        rdfs:comment     "Defines the predefined DocumentTypes of a PartVersion. A certain DocumentType has normally a typical set of information that is defined within its scope. E.g. a part master document contains Specifications that are used for the description of a defined PartVersion. The content and the degree of information a DocumentType may vary in the different processes.\n"@en;
        rdfs:label       "DocumentType"@en;
        rdfs:subClassOf  vec:OpenEnumeration .

vec:SlotSealingType_None
        rdf:type         vec:SlotSealingType , owl:NamedIndividiual;
        rdfs:comment     "The Slot cannot be sealed at all.\n"@en;
        vec:enumLiteral  "None" .

vec:boltTerminalSpecificationBoltHeight
        rdf:type            owl:ObjectProperty;
        rdfs:comment        "┬áSpecifies the height of the bolt (the height of the part to which ring terminals can be attached).\n"@en;
        rdfs:domain         vec:BoltTerminalSpecification;
        rdfs:label          "boltHeight"@en;
        rdfs:range          vec:NumericalValue;
        rdfs:subPropertyOf  vec:contains .

vec:RobustnessClass_SolidParticleProtection
        rdf:type         vec:RobustnessClass , owl:NamedIndividiual;
        vec:enumLiteral  "SolidParticleProtection" .

vec:geometrySegment3DEndNode
        rdf:type      owl:ObjectProperty;
        rdfs:comment  "References the GeometryNode3D where the GeometrySegment3D ends. \n"@en;
        rdfs:domain   vec:GeometrySegment3D;
        rdfs:label    "endNode"@en;
        rdfs:range    vec:GeometryNode3D .

vec:FittingSpecification
        rdf:type         owl:Class;
        rdfs:comment     "Specification for the definition of fittings. A fitting is a part that is used to connect pipes or tube. A fitting has a specific form (e.g. Y,T)\n"@en;
        rdfs:label       "FittingSpecification"@en;
        rdfs:subClassOf  vec:WireProtectionSpecification .

vec:LanguageCode_Vo  rdf:type  vec:LanguageCode , owl:NamedIndividiual;
        vec:enumLiteral  "Vo" .

vec:StatusOfApproval_Withdrawn
        rdf:type         vec:StatusOfApproval , owl:NamedIndividiual;
        vec:enumLiteral  "Withdrawn" .

<http://www.prostep.org/ontologies/ecad/2024/03/vec#TerminalBoltNominalSize_%234>
        rdf:type         vec:TerminalBoltNominalSize , owl:NamedIndividiual;
        vec:enumLiteral  "#4" .

vec:LanguageCode_Hr  rdf:type  vec:LanguageCode , owl:NamedIndividiual;
        vec:enumLiteral  "Hr" .

vec:wireReceptionReferenceWireReception
        rdf:type      owl:ObjectProperty;
        rdfs:comment  "References the WireReception that is instanced by this WireReceptionReference.\n"@en;
        rdfs:domain   vec:WireReceptionReference;
        rdfs:label    "wireReception"@en;
        rdfs:range    vec:WireReception .

vec:conductorCurrentInformationEnvironmentTemperature
        rdf:type            owl:ObjectProperty;
        rdfs:comment        "The environment temperature for which this maximum current value is applicable.\n"@en;
        rdfs:domain         vec:ConductorCurrentInformation;
        rdfs:label          "environmentTemperature"@en;
        rdfs:range          vec:NumericalValue;
        rdfs:subPropertyOf  vec:contains .

vec:TopologyZoneType_EnvironmentZone
        rdf:type         vec:TopologyZoneType , owl:NamedIndividiual;
        vec:enumLiteral  "EnvironmentZone" .

vec:projectIdentification
        rdf:type      owl:DatatypeProperty;
        rdfs:comment  "Specifies the development order number (car or engine project)\n"@en;
        rdfs:domain   vec:Project;
        rdfs:label    "identification"@en;
        rdfs:range    xs:string .

vec:PrimaryPartType_EdgeMountedFixing
        rdf:type         vec:PrimaryPartType , owl:NamedIndividiual;
        vec:enumLiteral  "EdgeMountedFixing" .

vec:SlotGender_Male  rdf:type  vec:SlotGender , owl:NamedIndividiual;
        vec:enumLiteral  "Male" .

vec:tubeSpecificationNominalSize
        rdf:type      owl:DatatypeProperty;
        rdfs:comment  "Defines the nominal size of a tube. The nominal size is a name for the size of the tube that is somehow related to the inner diameter of the tube. However, it is not the inner diameter (e.g. \"10.5\").\n"@en;
        rdfs:domain   vec:TubeSpecification;
        rdfs:label    "nominalSize"@en;
        rdfs:range    xs:string .

vec:USUnitName  rdf:type     owl:Class;
        rdfs:comment         "Enumeration for the definition of US unit names.\n"@en;
        rdfs:label           "USUnitName"@en;
        rdfs:subClassOf      vec:ClosedEnumeration;
        owl:equivalentClass  [ rdf:type   owl:Class;
                               owl:oneOf  ( vec:USUnitName_Thou vec:USUnitName_Inch vec:USUnitName_Foot vec:USUnitName_Yard vec:USUnitName_Chain vec:USUnitName_Furlong vec:USUnitName_Mile vec:USUnitName_League vec:USUnitName_FluidOunce vec:USUnitName_Gill vec:USUnitName_Pint vec:USUnitName_Quart vec:USUnitName_Gallon vec:USUnitName_Grain vec:USUnitName_Drachm vec:USUnitName_Ounce vec:USUnitName_Pound vec:USUnitName_Stone vec:USUnitName_Quarter vec:USUnitName_HundredWeight vec:USUnitName_Ton vec:USUnitName_Perch vec:USUnitName_Rood vec:USUnitName_Acre vec:USUnitName_AWG )
                             ] .

vec:DocumentType_HarnessDescription
        rdf:type         vec:DocumentType , owl:NamedIndividiual;
        rdfs:comment     "Documents of this type contain the description of a Harness┬á (which is for example the scope of the KBL).\n"@en;
        vec:enumLiteral  "HarnessDescription" .

vec:ComponentNodeType_OpenEnd
        rdf:type         vec:ComponentNodeType , owl:NamedIndividiual;
        rdfs:comment     "Defines that this ComponentNode is the end point for some unconnected connections that require wires and routings in the resulting harness (e.g. an antenna). A component node of this type is used whenever connections shall not be connected (on one side), regardless if it is an individual wire or a core of a multi core wire.\n"@en;
        vec:enumLiteral  "OpenEnd" .

vec:ValueDetermination_Calculated
        rdf:type         vec:ValueDetermination , owl:NamedIndividiual;
        rdfs:comment     "The value is determined by a calculation algorithm.\n"@en;
        vec:enumLiteral  "Calculated" .

vec:VariantCodeType_Serial
        rdf:type         vec:VariantCodeType , owl:NamedIndividiual;
        rdfs:comment     ""@en;
        vec:enumLiteral  "Serial" .

vec:wireTupleSpecificationMaximumUntwistSingleSided
        rdf:type            owl:ObjectProperty;
        rdfs:comment        "Specifies the maximum untwist for one side."@en;
        rdfs:domain         vec:WireTupleSpecification;
        rdfs:label          "maximumUntwistSingleSided"@en;
        rdfs:range          vec:NumericalValue;
        rdfs:subPropertyOf  vec:contains .

vec:SiUnitName_Watt  rdf:type  vec:SiUnitName , owl:NamedIndividiual;
        vec:enumLiteral  "Watt" .

vec:HousingComponentType_MultiFuse
        rdf:type         vec:HousingComponentType , owl:NamedIndividiual;
        vec:enumLiteral  "MultiFuse" .

vec:terminalReceptionSpecificationPullOutForce
        rdf:type            owl:ObjectProperty;
        rdfs:comment        "The force until the terminal is pulled out of the housing (normally a not intended case). KBLFRM-366\n"@en;
        rdfs:domain         vec:TerminalReceptionSpecification;
        rdfs:label          "pullOutForce"@en;
        rdfs:range          vec:NumericalValue;
        rdfs:subPropertyOf  vec:contains .

vec:InsulationState  rdf:type  owl:Class;
        rdfs:comment     "Enumeration for the definition of the insulation state of the splice.\n"@en;
        rdfs:label       "InsulationState"@en;
        rdfs:subClassOf  vec:OpenEnumeration .

vec:topologySegmentWrapperItem
        rdf:type      owl:ObjectProperty;
        rdfs:comment  "References the actual item for a Wrapper.";
        rdfs:domain   vec:TopologySegmentWrapper;
        rdfs:range    vec:TopologySegment .

vec:ZoneCoverage  rdf:type  owl:Class;
        rdfs:comment  "A ZoneCoverage defines an area on a TopologySegment that lies within a TopologyZone. The area is defined with two Locations . Locations are the same mechanism that is used to define placements for components. The area that is in the TopologyZone is the area between the two locations. There is no semantic in the direction of the definition, so the assignment of first &┬ásecond Location is completely arbitrary.\nHowever, there are some restrictions for the definition of the locations. All locations have to be in relation to the┬á TopologySegment that is referenced by the containing ZoneAssignment . This means the Locations have to be either a SegmentLocation on the respective TopologySegment or a NodeLocation on the start or end node of this particular T opologySegment. A ZoneCoverage from start to end node of a TopologySegment is equivalent to the complete omission of ZoneCoverages for a particular ZoneAssignment .\n┬á\n"@en;
        rdfs:label    "ZoneCoverage"@en .

vec:Contract  rdf:type   owl:Class;
        rdfs:comment     "A Contract-instance describes the relationship between an ItemVersion-instance and a Company-instance additionally defining the role the company takes in reference to the ItemVersion.\n"@en;
        rdfs:label       "Contract"@en;
        rdfs:subClassOf  vec:ExtendableElement .

vec:variantStructureSpecificationRootNode
        rdf:type            owl:ObjectProperty;
        rdfs:comment        ""@en;
        rdfs:domain         vec:VariantStructureSpecification;
        rdfs:label          "rootNode"@en;
        rdfs:range          vec:VariantStructureNode;
        rdfs:subPropertyOf  vec:contains .

vec:SiUnitName_Radian
        rdf:type         vec:SiUnitName , owl:NamedIndividiual;
        vec:enumLiteral  "Radian" .

vec:networkNodeAbbreviation
        rdf:type            owl:ObjectProperty;
        rdfs:comment        "Room for a short name of the NetworkNode.\n"@en;
        rdfs:domain         vec:NetworkNode;
        rdfs:label          "abbreviation"@en;
        rdfs:range          vec:LocalizedString;
        rdfs:subPropertyOf  vec:contains .

vec:wireReceptionSpecificationInsulationCrimpLength
        rdf:type            owl:ObjectProperty;
        rdfs:comment        "Specifies the length of the insulation crimp (wire reception, see diagram \"Terminal Dimensions\").\n"@en;
        rdfs:domain         vec:WireReceptionSpecification;
        rdfs:label          "insulationCrimpLength"@en;
        rdfs:range          vec:NumericalValue;
        rdfs:subPropertyOf  vec:contains .

vec:extendableElementReferencedExternalDocuments
        rdf:type      owl:ObjectProperty;
        rdfs:comment  "This association allows all ExtendableElements in the VEC┬áto reference DocumentVersions as \"external reference\".\nThis association shall be used for the extension of elements in the VEC┬áwith information that cannot be represented in the VEC┬áin an appropriate way but can be expressed in some external format (e.g. a specific symbol for a ComponentNode ).\nD ocumentVersions referenced by this association shall not contain any Specifications.\nThis association is no replacement for associations with a more precise semantic like the DocumentBasedInstruction or the associations between PartVersion and DocumentVersion.\n┬á\n"@en;
        rdfs:domain   vec:ExtendableElement;
        rdfs:label    "referencedExternalDocuments"@en;
        rdfs:range    vec:DocumentVersion .

vec:extensionSlotIdentification
        rdf:type      owl:DatatypeProperty;
        rdfs:comment  "Identification of the ExtensionSlot, which must be distinct for all ExtensionSlots of an EEComponent.\n"@en;
        rdfs:domain   vec:ExtensionSlot;
        rdfs:label    "identification"@en;
        rdfs:range    xs:string .

vec:wireReceptionIdentification
        rdf:type      owl:DatatypeProperty;
        rdfs:comment  "Specifies a unique identification of the WireReception. The identification is guaranteed to be unique within the TerminalSpecification (this might be for example a reception number).\n"@en;
        rdfs:domain   vec:WireReception;
        rdfs:label    "identification"@en;
        rdfs:range    xs:string .

vec:LanguageCode_Lt  rdf:type  vec:LanguageCode , owl:NamedIndividiual;
        vec:enumLiteral  "Lt" .

vec:ComponentNodeSubType_Microphone
        rdf:type         vec:ComponentNodeSubType , owl:NamedIndividiual;
        vec:enumLiteral  "Microphone" .

vec:connectorHousingRoleSlotReference
        rdf:type            owl:ObjectProperty;
        rdfs:comment        "Specifies the SlotReferences used in the ConnectorHousingRole. \n"@en;
        rdfs:domain         vec:ConnectorHousingRole;
        rdfs:label          "slotReference"@en;
        rdfs:range          vec:AbstractSlotReference;
        rdfs:subPropertyOf  vec:contains .

vec:CableLeadThroughOutlet
        rdf:type      owl:Class;
        rdfs:comment  "Specifies one outlet the a CableLeadThrough . For most CableLeadThroughs , there will be two."@en;
        rdfs:label    "CableLeadThroughOutlet"@en .

vec:connectionGroupInstallationInstruction
        rdf:type            owl:ObjectProperty;
        rdfs:comment        "Specifies additional InstallationInstructions for the ConnectionGroup.\n"@en;
        rdfs:domain         vec:ConnectionGroup;
        rdfs:label          "installationInstruction"@en;
        rdfs:range          vec:Instruction;
        rdfs:subPropertyOf  vec:contains .

vec:WireReceptionType_PlasmaSoldering
        rdf:type         vec:WireReceptionType , owl:NamedIndividiual;
        vec:enumLiteral  "PlasmaSoldering" .

vec:LanguageCode_Ts  rdf:type  vec:LanguageCode , owl:NamedIndividiual;
        vec:enumLiteral  "Ts" .

vec:documentVersionDocumentNumber
        rdf:type      owl:DatatypeProperty;
        rdfs:comment  "The documentNumber is the major identifier of a DocumentVersion. The format is user defined and respectively company specific.\n"@en;
        rdfs:domain   vec:DocumentVersion;
        rdfs:label    "documentNumber"@en;
        rdfs:range    xs:string .

[ rdf:type     owl:AllDisjointClasses;
  owl:members  ( vec:TerminalPairingSpecification vec:ContactingSpecification vec:PartOrUsageRelatedSpecification vec:PartSubstitutionSpecification vec:BaselineSpecification vec:CavitySpecification vec:ConductorSpecification vec:FillerSpecification vec:InsulationSpecification vec:SlotSpecification vec:TerminalReceptionSpecification vec:WireElementSpecification vec:WireGroupSpecification vec:WireReceptionSpecification vec:WireTupleSpecification vec:ExternalMappingSpecification vec:BuildingBlockSpecification2D vec:HarnessDrawingSpecification2D vec:BuildingBlockSpecification3D vec:HarnessGeometrySpecification3D vec:WireGroupingSpecification vec:WireTupleTerminationSpecification vec:MappingSpecification vec:CouplingSpecification vec:ModuleFamilySpecification vec:ModuleListSpecification vec:NetSpecification vec:NetViewSpecification vec:CableLeadThroughSpecification vec:CompositionSpecification vec:PartUsageSpecification vec:PlacementSpecification vec:DefaultDimensionSpecification vec:RoutingSpecification vec:ConnectionSpecification vec:ConnectionViewSpecification vec:SignalSpecification vec:TopologySpecification vec:TopologyZoneSpecification vec:TopologyMappingSpecification vec:TopologyBendingRestrictionSpecification vec:UsageConstraintSpecification vec:UsageNodeSpecification vec:VariantCodeSpecification vec:VariantConfigurationSpecification vec:VariantGroupSpecification vec:ApplicationConstraintSpecification vec:VariantStructureSpecification vec:PinWireMappingSpecification vec:AssignmentGroupSpecification vec:FunctionalStructureSpecification )
] .

vec:configurableElementConfigurationConstraint
        rdf:type            owl:ObjectProperty;
        rdfs:comment        "Contains or more ConfigurationContraints that apply to this ConfigurableElement. This is explained in more details in the recommendation chapter / model diagram \"Variants\".\n"@en;
        rdfs:domain         vec:ConfigurableElement;
        rdfs:label          "configurationConstraint"@en;
        rdfs:range          vec:ConfigurationConstraint;
        rdfs:subPropertyOf  vec:contains .

vec:routingMandatorySegment
        rdf:type      owl:ObjectProperty;
        rdfs:comment  "Specifies some constraints for the routing. If the path of the routing is recalculated the referenced segments must be visited. \n"@en;
        rdfs:domain   vec:Routing;
        rdfs:label    "mandatorySegment"@en;
        rdfs:range    vec:TopologySegment .

vec:PartNature_Productive
        rdf:type         vec:PartNature , owl:NamedIndividiual;
        rdfs:comment     " Productive PartVersions represent regular part numbers that are used in serial production.\n"@en;
        vec:enumLiteral  "Productive" .

vec:TerminalBoltNominalSize_M5
        rdf:type         vec:TerminalBoltNominalSize , owl:NamedIndividiual;
        vec:enumLiteral  "M5" .

vec:dimensionDefinedLocations
        rdf:type            owl:ObjectProperty;
        rdfs:comment        ""@en;
        rdfs:domain         vec:Dimension;
        rdfs:label          "definedLocations"@en;
        rdfs:range          vec:Location;
        rdfs:subPropertyOf  vec:contains .

vec:pinComponentBehaviorIdentification
        rdf:type      owl:DatatypeProperty;
        rdfs:comment  "Identification of the PinComponentBehavior which identifies it from a user perspective, and which must be distinct for all PinComponentBehaviors of a PinComponent.\n"@en;
        rdfs:domain   vec:PinComponentBehavior;
        rdfs:label    "identification"@en;
        rdfs:range    xs:string .

vec:approvalIdentification
        rdf:type      owl:DatatypeProperty;
        rdfs:comment  "Specifies a unique identification of the approval. The identification is guaranteed to be unique over all VEC-documents. Normally this would reference to a company specific approval number or something similar. KBLFRM-349\n"@en;
        rdfs:domain   vec:Approval;
        rdfs:label    "identification"@en;
        rdfs:range    xs:string .

vec:cavitySealRoleCavitySealSpecification
        rdf:type      owl:ObjectProperty;
        rdfs:comment  "References the CavitySealSpecification that is instanced by this CavitySealRole.\n"@en;
        rdfs:domain   vec:CavitySealRole;
        rdfs:label    "cavitySealSpecification"@en;
        rdfs:range    vec:CavitySealSpecification .

vec:occurrenceOrUsageViewItem3DOrientation
        rdf:type            owl:ObjectProperty;
        rdfs:comment        "Specifies the orientation of the view item.\n"@en;
        rdfs:domain         vec:OccurrenceOrUsageViewItem3D;
        rdfs:label          "orientation"@en;
        rdfs:range          vec:Transformation3D;
        rdfs:subPropertyOf  vec:contains .

vec:extensionSlotReferenceExtensionSlot
        rdf:type     owl:ObjectProperty;
        rdfs:domain  vec:ExtensionSlotReference;
        rdfs:label   "extensionSlot"@en;
        rdfs:range   vec:ExtensionSlot .

vec:PluggableTerminalType
        rdf:type         owl:Class;
        rdfs:comment     "Defines valid values for the type of PluggableTerminals. The type defines constraints about the numbers of wire and┬áterminal receptions and their relations.\n"@en;
        rdfs:label       "PluggableTerminalType"@en;
        rdfs:subClassOf  vec:OpenEnumeration .

vec:PinWireMappingPoint
        rdf:type      owl:Class;
        rdfs:comment  "The PinWireMappingPoint creates a single variance free mapping between a ContactPoint and a PinComponentReference within a PinWireMappingSpecification (more details there) .\n"@en;
        rdfs:label    "PinWireMappingPoint"@en .

vec:vecContentUnit  rdf:type  owl:ObjectProperty;
        rdfs:comment        "Specifies the Units used in the VEC-file. \n"@en;
        rdfs:domain         vec:VecContent;
        rdfs:label          "unit"@en;
        rdfs:range          vec:Unit;
        rdfs:subPropertyOf  vec:contains .

vec:bridgeTerminalRoleConnection
        rdf:type      owl:ObjectProperty;
        rdfs:comment  "References the Connection that is realized by this BridgeTerminalRole.\n"@en;
        rdfs:domain   vec:BridgeTerminalRole;
        rdfs:label    "connection"@en;
        rdfs:range    vec:Connection .

vec:usageConstraintType
        rdf:type            owl:ObjectProperty;
        rdfs:comment        "Defines if the usage constraint is positive (allowance) or negative (denial).\n"@en;
        rdfs:domain         vec:UsageConstraint;
        rdfs:label          "type"@en;
        rdfs:range          vec:UsageConstraintType;
        rdfs:subPropertyOf  vec:contains .

vec:NodeMapping  rdf:type  owl:Class;
        rdfs:comment  "Defines the relationship of an inner node to its outer topology. The relationship to the outer topology is expressed with a Location .\n"@en;
        rdfs:label    "NodeMapping"@en .

vec:ContactingSpecification
        rdf:type         owl:Class;
        rdfs:comment     "Specification for the description of the contacting. A contacting defines the relationships between Terminals, Seals, Plugs, Cavities and Wires. "@en;
        rdfs:label       "ContactingSpecification"@en;
        rdfs:subClassOf  vec:Specification .

vec:SignalSubType_Ethernet
        rdf:type         vec:SignalSubType , owl:NamedIndividiual;
        vec:enumLiteral  "Ethernet" .

vec:FunctionalStructureNode
        rdf:type      owl:Class;
        rdfs:comment  " FunctionalStructureNodes can be used to define a hierarchical structure on FunctionalAssignmentGroups . Every FunctionalStructureNode can reference FunctionalAssignmentGroups and FunctionalStructureNodes as children.\n"@en;
        rdfs:label    "FunctionalStructureNode"@en .

vec:documentVersionNumberOfSheets
        rdf:type      owl:DatatypeProperty;
        rdfs:comment  "The number of sheets contained in the document.\n"@en;
        rdfs:domain   vec:DocumentVersion;
        rdfs:label    "numberOfSheets"@en;
        rdfs:range    xs:integer .

vec:extensionSlotReferenceIdentification
        rdf:type     owl:DatatypeProperty;
        rdfs:domain  vec:ExtensionSlotReference;
        rdfs:label   "identification"@en;
        rdfs:range   xs:string .

vec:AnchorType  rdf:type     owl:Class;
        rdfs:comment         "Enumeration for the definition of AnchorType of the SegmentLocation.\n"@en;
        rdfs:label           "AnchorType"@en;
        rdfs:subClassOf      vec:ClosedEnumeration;
        owl:equivalentClass  [ rdf:type   owl:Class;
                               owl:oneOf  ( vec:AnchorType_FromStartNode vec:AnchorType_FromEndNode )
                             ] .

vec:couplingSpecificationCouplingPoint
        rdf:type            owl:ObjectProperty;
        rdfs:domain         vec:CouplingSpecification;
        rdfs:label          "couplingPoint"@en;
        rdfs:range          vec:CouplingPoint;
        rdfs:subPropertyOf  vec:contains .

vec:HousingComponentType_EEComponent
        rdf:type         vec:HousingComponentType , owl:NamedIndividiual;
        vec:enumLiteral  "EEComponent" .

vec:PrimaryPartType_ConnectorHousingCap
        rdf:type         vec:PrimaryPartType , owl:NamedIndividiual;
        vec:enumLiteral  "ConnectorHousingCap" .

vec:CurrentType_ACThreePhase
        rdf:type         vec:CurrentType , owl:NamedIndividiual;
        vec:enumLiteral  "ACThreePhase" .

vec:occurrenceOrUsageViewItem2DOrientation
        rdf:type            owl:ObjectProperty;
        rdfs:comment        "Specifies the orientation of the view item.\n"@en;
        rdfs:domain         vec:OccurrenceOrUsageViewItem2D;
        rdfs:label          "orientation"@en;
        rdfs:range          vec:Transformation2D;
        rdfs:subPropertyOf  vec:contains .

vec:buildingBlockPositioning3DPositioning
        rdf:type            owl:ObjectProperty;
        rdfs:comment        "Specifies the positioning of the building block in the harness geometry.\n"@en;
        rdfs:domain         vec:BuildingBlockPositioning3D;
        rdfs:label          "positioning"@en;
        rdfs:range          vec:Transformation3D;
        rdfs:subPropertyOf  vec:contains .

vec:ItemEquivalence  rdf:type  owl:Class;
        rdfs:comment     "Defines two or more ItemVersions to be equivalent out of the view of a certain company. The ItemEquivalence class will most likely be used by a company to express which PartNumber a certain PartVersion has in the context of other companies (same applies to DocumentVersions ). However, for every other company separate ItemEquivalences are needed as the statement of equivalence can be very subjective.\n"@en;
        rdfs:label       "ItemEquivalence"@en;
        rdfs:subClassOf  vec:ExtendableElement .

[ rdf:type     owl:AllDisjointClasses;
  owl:members  ( vec:MultiCavityPlugSpecification )
] .

vec:LanguageCode_Rw  rdf:type  vec:LanguageCode , owl:NamedIndividiual;
        vec:enumLiteral  "Rw" .

vec:variantGroupVariantCode
        rdf:type      owl:ObjectProperty;
        rdfs:comment  "References the VariantCodes that are member of the VariantGroup. \n"@en;
        rdfs:domain   vec:VariantGroup;
        rdfs:label    "variantCode"@en;
        rdfs:range    vec:VariantCode .

vec:wireElementReferenceUnconnected
        rdf:type      owl:DatatypeProperty;
        rdfs:comment  "If this attribute is true , the WireElementReference is not connected (unused) on purpose. This can be the case for example if a multi core is used, but not all cores are necessary in a specific situation.\nHowever, for all WireElements defined in the WireSpecification a corresponding WireElementReference shall exist. This attribute can be used to mark these unused cores explicitly.\n"@en;
        rdfs:domain   vec:WireElementReference;
        rdfs:label    "unconnected"@en;
        rdfs:range    xs:boolean .

vec:LanguageCode_Dz  rdf:type  vec:LanguageCode , owl:NamedIndividiual;
        vec:enumLiteral  "Dz" .

vec:GrommetSpecification
        rdf:type         owl:Class;
        rdfs:comment     "Specification for the definition of grommets.\n"@en;
        rdfs:label       "GrommetSpecification"@en;
        rdfs:subClassOf  vec:PartOrUsageRelatedSpecification .

vec:WindingFirmness  rdf:type  owl:Class;
        rdfs:comment     "Defines the firmness with which a tape is applied to a segment.\n"@en;
        rdfs:label       "WindingFirmness"@en;
        rdfs:subClassOf  vec:OpenEnumeration .

vec:DocumentType_ManufacturingDescription
        rdf:type         vec:DocumentType , owl:NamedIndividiual;
        rdfs:comment     ""@en;
        vec:enumLiteral  "ManufacturingDescription" .

vec:FunctionalRequirementType
        rdf:type         owl:Class;
        rdfs:label       "FunctionalRequirementType"@en;
        rdfs:subClassOf  vec:OpenEnumeration .

vec:ComponentNodeType_PotentialDistributor
        rdf:type         vec:ComponentNodeType , owl:NamedIndividiual;
        rdfs:comment     "A passive device that distributes one or more potentials. Splits a network into different Connections with the same Signal.\n"@en;
        vec:enumLiteral  "PotentialDistributor" .

vec:segmentMappingMappedPosition
        rdf:type            owl:ObjectProperty;
        rdfs:domain         vec:SegmentMapping;
        rdfs:label          "mappedPosition"@en;
        rdfs:range          vec:Path;
        rdfs:subPropertyOf  vec:contains .

vec:connectionNodeViewItemComponentNode
        rdf:type      owl:ObjectProperty;
        rdfs:comment  "References the ComponentNode that is represented by this ComponentNodeViewItem . "@en;
        rdfs:domain   vec:ConnectionNodeViewItem;
        rdfs:label    "componentNode"@en;
        rdfs:range    vec:ComponentNode .

vec:SignalSubType_CAN
        rdf:type         vec:SignalSubType , owl:NamedIndividiual;
        rdfs:comment     "┬áController Area Network\n"@en;
        vec:enumLiteral  "CAN" .

vec:contactPointWireMounting
        rdf:type            owl:ObjectProperty;
        rdfs:comment        "Specifies the WireMouting defined by ContactPoint. More than one WireMounting is allowed in order to support variance. In concrete configuration the WireMounting with all referenced elements present is used.\n"@en;
        rdfs:domain         vec:ContactPoint;
        rdfs:label          "wireMounting"@en;
        rdfs:range          vec:WireMounting;
        rdfs:subPropertyOf  vec:contains .

vec:UsageNodeType_Actuator
        rdf:type         vec:UsageNodeType , owl:NamedIndividiual;
        vec:enumLiteral  "Actuator" .

vec:fileBasedInstructionFileName
        rdf:type      owl:DatatypeProperty;
        rdfs:comment  "The name of the file as it appears in the package, including the folder structure (fully qualified name).\n"@en;
        rdfs:domain   vec:FileBasedInstruction;
        rdfs:label    "fileName"@en;
        rdfs:range    xs:string .

vec:connectionGroupConnectionGroupType
        rdf:type            owl:ObjectProperty;
        rdfs:comment        "Specifies the type of the connectionGroup, valid literals are defined in the open enumeration ConnectionGroupType .\n"@en;
        rdfs:domain         vec:ConnectionGroup;
        rdfs:label          "connectionGroupType"@en;
        rdfs:range          vec:ConnectionGroupType;
        rdfs:subPropertyOf  vec:contains .

vec:externalMappingExternalReference
        rdf:type      owl:DatatypeProperty;
        rdfs:comment  "Defines the unique key of the external element. How this key shall be interpreted is dependent from the format of the external data source.\n"@en;
        rdfs:domain   vec:ExternalMapping;
        rdfs:label    "externalReference"@en;
        rdfs:range    xs:string .

vec:permissionPermissionDate
        rdf:type      owl:DatatypeProperty;
        rdfs:comment  "Specifies the date when the permission was stated.\n"@en;
        rdfs:domain   vec:Permission;
        rdfs:label    "permissionDate"@en;
        rdfs:range    xs:dateTime .

vec:segmentConnectionPointHCConnectorSegmentConnectionPoint
        rdf:type      owl:ObjectProperty;
        rdfs:comment  "References the SegementConnectionPoint of the ConnectorHousingSpecification that is used to \"enter\" the connector housing."@en;
        rdfs:domain   vec:SegmentConnectionPointHC;
        rdfs:label    "connectorSegmentConnectionPoint"@en;
        rdfs:range    vec:SegmentConnectionPoint .

vec:DocumentType_ChangeDescription
        rdf:type         vec:DocumentType , owl:NamedIndividiual;
        rdfs:comment     ""@en;
        vec:enumLiteral  "ChangeDescription" .

vec:CavityMountingDetail
        rdf:type         owl:Class;
        rdfs:comment     "With a CavityMountingDetail it is possible to describe a detailed cavity mounting.\nThis is needed if the information which terminal reception is mounted into which cavity is important. There are cases where this information can be relevant (e.g. bridge contacts with an asymmetric wire mounting).\n"@en;
        rdfs:label       "CavityMountingDetail"@en;
        rdfs:subClassOf  vec:ExtendableElement .

vec:geometryNodeAliasId
        rdf:type            owl:ObjectProperty;
        rdfs:comment        "Specifies additional identifiers for the GeometryNode.\n"@en;
        rdfs:domain         vec:GeometryNode;
        rdfs:label          "aliasId"@en;
        rdfs:range          vec:AliasIdentification;
        rdfs:subPropertyOf  vec:contains .

vec:DocumentType_HarnessCoupling
        rdf:type         vec:DocumentType , owl:NamedIndividiual;
        rdfs:comment     " DocumentVersions of this type define the coupling information of wiring harnesses in a vehicle network. The DocumentVersion contains the necessary CouplingSpecifications and the PartUsages for the coupling devices.\n"@en;
        vec:enumLiteral  "HarnessCoupling" .

vec:ConnectionEnd  rdf:type  owl:Class;
        rdfs:comment     "A connection end is the end of a Connection at a ComponentPort.\n"@en;
        rdfs:label       "ConnectionEnd"@en;
        rdfs:subClassOf  vec:ConfigurableElement .

vec:tubeSpecificationHeight
        rdf:type            owl:ObjectProperty;
        rdfs:comment        "Specifies the height of the tube. If the height is defined, a width shall be defined, too. The height and width of a tube shall only be used for tubes that are not circular (shape != Circular). For circular shapes, the outside diameter shall be used.\n"@en;
        rdfs:domain         vec:TubeSpecification;
        rdfs:label          "height"@en;
        rdfs:range          vec:NumericalValue;
        rdfs:subPropertyOf  vec:contains .

vec:segmentLocationReferencedSegment
        rdf:type      owl:ObjectProperty;
        rdfs:comment  "References the TopologySegment on which the Location is located.\n"@en;
        rdfs:domain   vec:SegmentLocation;
        rdfs:label    "referencedSegment"@en;
        rdfs:range    vec:TopologySegment .

vec:placementPointSegmentDiameter
        rdf:type            owl:ObjectProperty;
        rdfs:comment        "Specifies the valid segment diameter range for which this PlacementPoint is suitable.\n"@en;
        rdfs:domain         vec:PlacementPoint;
        rdfs:label          "segmentDiameter"@en;
        rdfs:range          vec:ValueRange;
        rdfs:subPropertyOf  vec:contains .

vec:wireTupleTerminationAssociatedWireEnds
        rdf:type     owl:ObjectProperty;
        rdfs:domain  vec:WireTupleTermination;
        rdfs:label   "associatedWireEnds"@en;
        rdfs:range   vec:WireEnd .

vec:topologyBendingRestrictionRestrictedPath
        rdf:type            owl:ObjectProperty;
        rdfs:comment        "The path that defines the restricted way in the topology.\n"@en;
        rdfs:domain         vec:TopologyBendingRestriction;
        rdfs:label          "restrictedPath"@en;
        rdfs:range          vec:Path;
        rdfs:subPropertyOf  vec:contains .

vec:documentVersionLocation
        rdf:type      owl:DatatypeProperty;
        rdfs:comment  "The location is a possibility to provide a reference to the source location of the DocumentVersion (e.g. a document management system or an archive system) where the original document can be found . The location shall be provided either as an URN┬áor URL.\n┬á\n"@en;
        rdfs:domain   vec:DocumentVersion;
        rdfs:label    "location"@en;
        rdfs:range    xs:string .

vec:TerminalBoltNominalSize_M22
        rdf:type         vec:TerminalBoltNominalSize , owl:NamedIndividiual;
        vec:enumLiteral  "M22" .

vec:segmentLocationOffset
        rdf:type            owl:ObjectProperty;
        rdfs:comment        "Specifies the offset / distance of the Location to the anchor of the location.\n"@en;
        rdfs:domain         vec:SegmentLocation;
        rdfs:label          "offset"@en;
        rdfs:range          vec:NumericalValue;
        rdfs:subPropertyOf  vec:contains .

vec:TerminalReceptionReference
        rdf:type      owl:Class;
        rdfs:comment  "A TerminalReceptionReference is an instance of a TerminalReception .\n"@en;
        rdfs:label    "TerminalReceptionReference"@en .

vec:signalNetType  rdf:type  owl:ObjectProperty;
        rdfs:domain  vec:Signal;
        rdfs:label   "netType"@en;
        rdfs:range   vec:NetType .

vec:antennaSpecificationFMin
        rdf:type            owl:ObjectProperty;
        rdfs:comment        "Specifies the minimum operating frequency of the antenna.\n"@en;
        rdfs:domain         vec:AntennaSpecification;
        rdfs:label          "fMin"@en;
        rdfs:range          vec:NumericalValue;
        rdfs:subPropertyOf  vec:contains .

vec:connectionEndInstallationInstruction
        rdf:type            owl:ObjectProperty;
        rdfs:comment        "Specifies installation instruction for the ConnectionEnd .\n"@en;
        rdfs:domain         vec:ConnectionEnd;
        rdfs:label          "installationInstruction"@en;
        rdfs:range          vec:Instruction;
        rdfs:subPropertyOf  vec:contains .

vec:SegmentCrossSectionAreaType
        rdf:type         owl:Class;
        rdfs:comment     "Defines valid values the type of the cross-section area of a TopologySegment , since a TopologySegment can have different cross section areas with different meanings in the process.\n"@en;
        rdfs:label       "SegmentCrossSectionAreaType"@en;
        rdfs:subClassOf  vec:OpenEnumeration .

vec:IECPrefix_Yobi  rdf:type  vec:IECPrefix , owl:NamedIndividiual;
        vec:enumLiteral  "Yobi" .

vec:PinComponentType_Coil
        rdf:type         vec:PinComponentType , owl:NamedIndividiual;
        vec:enumLiteral  "Coil" .

<http://www.prostep.org/ontologies/ecad/2024/03/vec#TerminalBoltNominalSize_5%2F8>
        rdf:type         vec:TerminalBoltNominalSize , owl:NamedIndividiual;
        vec:enumLiteral  "5/8" .

vec:UsageNodeType_PowerDistribution
        rdf:type         vec:UsageNodeType , owl:NamedIndividiual;
        vec:enumLiteral  "PowerDistribution" .

vec:WireReceptionType_UltraSonicCompactation
        rdf:type         vec:WireReceptionType , owl:NamedIndividiual;
        rdfs:comment     "┬áUltraSonicCompactation, typically used for aluminium wires.\n"@en;
        vec:enumLiteral  "UltraSonicCompactation" .

vec:LanguageCode_Ga  rdf:type  vec:LanguageCode , owl:NamedIndividiual;
        vec:enumLiteral  "Ga" .

vec:NetworkNodeViewItem
        rdf:type      owl:Class;
        rdfs:comment  "A NetworkNodeViewItem represents a NetworkNode within a NetViewSpecification and defines its position within the layout."@en;
        rdfs:label    "NetworkNodeViewItem"@en .

vec:ImperialUnitName_Rood
        rdf:type         vec:ImperialUnitName , owl:NamedIndividiual;
        vec:enumLiteral  "Rood" .

vec:TerminalBoltNominalSize_M64
        rdf:type         vec:TerminalBoltNominalSize , owl:NamedIndividiual;
        vec:enumLiteral  "M64" .

vec:SlotLayoutType_USBTypeA
        rdf:type         vec:SlotLayoutType , owl:NamedIndividiual;
        vec:enumLiteral  "USBTypeA" .

vec:pinComponentBehaviorDescription
        rdf:type            owl:ObjectProperty;
        rdfs:comment        "Specifies additional, human readable information about the PinComponentBehaviour .\n"@en;
        rdfs:domain         vec:PinComponentBehavior;
        rdfs:label          "description"@en;
        rdfs:range          vec:AbstractLocalizedString;
        rdfs:subPropertyOf  vec:contains .

vec:SignalSubType_RTPGE
        rdf:type         vec:SignalSubType , owl:NamedIndividiual;
        vec:enumLiteral  "RTPGE" .

[ rdf:type     owl:AllDisjointClasses;
  owl:members  ( vec:DocumentBasedInstruction vec:FileBasedInstruction vec:TextBasedInstruction )
] .

vec:buildingBlockSpecification2DCartesianPoint
        rdf:type            owl:ObjectProperty;
        rdfs:comment        "Specifies the CartesianPoint2Ds that are used in the BuildingBlockSpecification2D.\n"@en;
        rdfs:domain         vec:BuildingBlockSpecification2D;
        rdfs:label          "cartesianPoint"@en;
        rdfs:range          vec:CartesianPoint2D;
        rdfs:subPropertyOf  vec:contains .

vec:ComponentNodeType_Fuse
        rdf:type         vec:ComponentNodeType , owl:NamedIndividiual;
        rdfs:comment     " Deprecated since VEC V1.2. Use instead ComponentSubType Fuse.┬á\n"@en;
        vec:enumLiteral  "Fuse" .

vec:networkPortNetType
        rdf:type     owl:ObjectProperty;
        rdfs:domain  vec:NetworkPort;
        rdfs:label   "netType"@en;
        rdfs:range   vec:NetType .

vec:LocalizedTypedStringType_Title
        rdf:type         vec:LocalizedTypedStringType , owl:NamedIndividiual;
        rdfs:comment     "The LocalizedTypedString represents a Title in accordance to ISO 7200.\n"@en;
        vec:enumLiteral  "Title" .

vec:NominalVoltage_HV4
        rdf:type         vec:NominalVoltage , owl:NamedIndividiual;
        rdfs:comment     "HV Class 4 (900V┬áDC)\n"@en;
        vec:enumLiteral  "HV4" .

vec:topologyGroupSpecificationTopologySpecification
        rdf:type      owl:ObjectProperty;
        rdfs:comment  ""@en;
        rdfs:domain   vec:TopologyGroupSpecification;
        rdfs:label    "topologySpecification"@en;
        rdfs:range    vec:TopologySpecification .

vec:insulationSpecificationLabelIdentificationValue
        rdf:type      owl:DatatypeProperty;
        rdfs:comment  "Specifies the value of a label printed on the insulation of the wire. This value applies to all wire elements that satisfy this specification, so all instances share the same label value (e.g. a wire type or a core number in a multi core wire).\nIf instances of a wire require individual labeling it has to be defined on the WireElementReference .\n"@en;
        rdfs:domain   vec:InsulationSpecification;
        rdfs:label    "labelIdentificationValue"@en;
        rdfs:range    xs:string .

vec:eEComponentSpecificationExtensionSlots
        rdf:type            owl:ObjectProperty;
        rdfs:comment        "Specifies the available ExtensionSlots of the EEComponent. "@en;
        rdfs:domain         vec:EEComponentSpecification;
        rdfs:label          "extensionSlots"@en;
        rdfs:range          vec:ExtensionSlot;
        rdfs:subPropertyOf  vec:contains .

vec:connectionSignal  rdf:type  owl:ObjectProperty;
        rdfs:comment  "References the signal that is transmitted by the connection.\n"@en;
        rdfs:domain   vec:Connection;
        rdfs:label    "signal"@en;
        rdfs:range    vec:Signal .

vec:pinVoltageInformationVoltage
        rdf:type            owl:ObjectProperty;
        rdfs:comment        "The voltage of the pin.\n"@en;
        rdfs:domain         vec:PinVoltageInformation;
        rdfs:label          "voltage"@en;
        rdfs:range          vec:NumericalValue;
        rdfs:subPropertyOf  vec:contains .

vec:connectionGroupIdentification
        rdf:type      owl:DatatypeProperty;
        rdfs:comment  "Specifies a unique identification of the ConnectionGroup. The identification is guaranteed to be unique within the ConnectionSpecification.\n"@en;
        rdfs:domain   vec:ConnectionGroup;
        rdfs:label    "identification"@en;
        rdfs:range    xs:string .

vec:ConductorType_Foil
        rdf:type         vec:ConductorType , owl:NamedIndividiual;
        rdfs:comment     "Used for conductors that are a foil (e.g. some shields).\n"@en;
        vec:enumLiteral  "Foil" .

vec:networkPortIdentification
        rdf:type      owl:DatatypeProperty;
        rdfs:comment  "Specifies a unique identification of the NetworkPort. The identification is guaranteed to be unique within the NetSpecification.\n"@en;
        rdfs:domain   vec:NetworkPort;
        rdfs:label    "identification"@en;
        rdfs:range    xs:string .

vec:topologyNodeInstantiatedNode
        rdf:type      owl:ObjectProperty;
        rdfs:comment  "If this TopologyNode is an instance of another To pologyNode that is defined elsewhere (e.g. the topology of an assembly), then the instantiated may be referenced here.\n"@en;
        rdfs:domain   vec:TopologyNode;
        rdfs:label    "instantiatedNode"@en;
        rdfs:range    vec:TopologyNode .

vec:MeasurementPointReference
        rdf:type         owl:Class;
        rdfs:comment     "A MeasurementPointReference is the instance of a MeasurementPoint in the context of an OccurrenceOrUsage .\n"@en;
        rdfs:label       "MeasurementPointReference"@en;
        rdfs:subClassOf  vec:DimensionAnchor .

vec:PinComponent  rdf:type  owl:Class;
        rdfs:comment     "A PinComponent describes a pin of an EEComponent. A PinComponent is part of a HousingComponent and is defined by tree aspects. Its geometric position in the HousingComponent , which is defined by the referencedCavity. Its physical electrical properties, which are defined by the referenced TerminalSpecification. Its electrical behaviour, which is defined configuration dependent by its PinComponentBehaviour. "@en;
        rdfs:label       "PinComponent"@en;
        rdfs:subClassOf  vec:ConfigurableElement .

vec:transformation3DA11
        rdf:type     owl:DatatypeProperty;
        rdfs:domain  vec:Transformation3D;
        rdfs:label   "a11"@en;
        rdfs:range   xs:double .

vec:cavityAddOnWireAddOn
        rdf:type            owl:ObjectProperty;
        rdfs:comment        "Specifies the wire length add on needed for the cavity.\n"@en;
        rdfs:domain         vec:CavityAddOn;
        rdfs:label          "wireAddOn"@en;
        rdfs:range          vec:NumericalValue;
        rdfs:subPropertyOf  vec:contains .

vec:ConductorType_Stranded
        rdf:type         vec:ConductorType , owl:NamedIndividiual;
        rdfs:comment     "Used for conductors that are made of multiple individual strands (used for most automotive cores).\n"@en;
        vec:enumLiteral  "Stranded" .

vec:tubeSpecificationLength
        rdf:type            owl:ObjectProperty;
        rdfs:comment        "Specifies the length of the tube if it is a predefined value.\n"@en;
        rdfs:domain         vec:TubeSpecification;
        rdfs:label          "length"@en;
        rdfs:range          vec:NumericalValue;
        rdfs:subPropertyOf  vec:contains .

vec:TerminalBoltNominalSize_M27
        rdf:type         vec:TerminalBoltNominalSize , owl:NamedIndividiual;
        vec:enumLiteral  "M27" .

vec:functionalStructureNodeContainedGroups
        rdf:type     owl:ObjectProperty;
        rdfs:domain  vec:FunctionalStructureNode;
        rdfs:label   "containedGroups"@en;
        rdfs:range   vec:FunctionalAssignmentGroup .

vec:CableLeadThroughType_ShrinkingTube
        rdf:type         vec:CableLeadThroughType , owl:NamedIndividiual;
        rdfs:comment     ""@en;
        vec:enumLiteral  "ShrinkingTube" .

vec:ExternalMappingSpecification
        rdf:type         owl:Class;
        rdfs:comment     "An ExternalMappingSpecification is used to define a mapping between an external data source (represented by the referenced mappedDocument ) and the content of a VEC file.\n"@en;
        rdfs:label       "ExternalMappingSpecification"@en;
        rdfs:subClassOf  vec:Specification .

vec:WireReceptionType_SpotResistentWelding
        rdf:type         vec:WireReceptionType , owl:NamedIndividiual;
        vec:enumLiteral  "SpotResistentWelding" .

vec:massInformationValue
        rdf:type            owl:ObjectProperty;
        rdfs:comment        "Specifies the mass as numerical value.\n"@en;
        rdfs:domain         vec:MassInformation;
        rdfs:label          "value"@en;
        rdfs:range          vec:NumericalValue;
        rdfs:subPropertyOf  vec:contains .

vec:USUnit  rdf:type     owl:Class;
        rdfs:comment     "The USUnit class can define quantities in the terms of the US-Unit-System by specifying the corresponding US unit name. The US Unit System is quite similar to the imperial unit system; however, some units are defined slightly different.\n"@en;
        rdfs:label       "USUnit"@en;
        rdfs:subClassOf  vec:Unit .

vec:transformation3DA32
        rdf:type     owl:DatatypeProperty;
        rdfs:domain  vec:Transformation3D;
        rdfs:label   "a32"@en;
        rdfs:range   xs:double .

vec:WireGroupSpecification
        rdf:type         owl:Class;
        rdfs:comment     "Specification for the definition of WireGroups. Wire groups are for example used for the representation of twisted pairs.\n"@en;
        rdfs:label       "WireGroupSpecification"@en;
        rdfs:subClassOf  vec:Specification .

vec:topologyBendingRestrictionMinBendRadiusDynamic
        rdf:type            owl:ObjectProperty;
        rdfs:comment        "Specifies the minimum bend radius for the restricted path, if it is used in a dynamic environment, where it is bended repeatedly (e.g. in the grommet of the back door).\n"@en;
        rdfs:domain         vec:TopologyBendingRestriction;
        rdfs:label          "minBendRadiusDynamic"@en;
        rdfs:range          vec:NumericalValue;
        rdfs:subPropertyOf  vec:contains .

vec:networkNodeViewItemNetworkNode
        rdf:type      owl:ObjectProperty;
        rdfs:comment  "References the NetworkNode that is represented by this NetworkNodeViewItem. "@en;
        rdfs:domain   vec:NetworkNodeViewItem;
        rdfs:label    "networkNode"@en;
        rdfs:range    vec:NetworkNode .

vec:TerminalBoltNominalSize_M48
        rdf:type         vec:TerminalBoltNominalSize , owl:NamedIndividiual;
        vec:enumLiteral  "M48" .

vec:ItemHistoryEntry  rdf:type  owl:Class;
        rdfs:comment     "An ItemHistroyEntry defines the direct relationship between ItemVersions in the terms of predecessor and successor. There are two possible types of relationships between ItemVersions, derivation and sequence. Derivation means for example for parts, that the successor version is a new part developed on the base of the predecessor version. Sequence means the successor version is an improvement of the predecessor version. By the combination of more than one ItemHistoryEntry a linear sequence of ItemVersions can be represented.\n"@en;
        rdfs:label       "ItemHistoryEntry"@en;
        rdfs:subClassOf  vec:ExtendableElement .

vec:numericalValueValueComponent
        rdf:type      owl:DatatypeProperty;
        rdfs:comment  "Specifies the value of the numerical value.\n"@en;
        rdfs:domain   vec:NumericalValue;
        rdfs:label    "valueComponent"@en;
        rdfs:range    xs:double .

vec:HistoryEntryType  rdf:type  owl:Class;
        rdfs:comment         "Enumeration for the definition of the type of relationship represented by an ItemHistoryEntry. (see KBLFRM-271)\n"@en;
        rdfs:label           "HistoryEntryType"@en;
        rdfs:subClassOf      vec:ClosedEnumeration;
        owl:equivalentClass  [ rdf:type   owl:Class;
                               owl:oneOf  ( vec:HistoryEntryType_Derivation vec:HistoryEntryType_Sequence )
                             ] .

vec:pinComponentBehaviorSignalDirection
        rdf:type            owl:ObjectProperty;
        rdfs:comment        "The direction of the signal on this pin.\n"@en;
        rdfs:domain         vec:PinComponentBehavior;
        rdfs:label          "signalDirection"@en;
        rdfs:range          vec:SignalDirection;
        rdfs:subPropertyOf  vec:contains .

vec:PinCurrentType_MinCurrent
        rdf:type         vec:PinCurrentType , owl:NamedIndividiual;
        vec:enumLiteral  "minCurrent" .

vec:vecContentDocumentVersion
        rdf:type            owl:ObjectProperty;
        rdfs:comment        "Specifies the DocumentVersions contained in the VEC-file. \n"@en;
        rdfs:domain         vec:VecContent;
        rdfs:label          "documentVersion"@en;
        rdfs:range          vec:DocumentVersion;
        rdfs:subPropertyOf  vec:contains .

vec:placeableElementSpecificationPlacementPoint
        rdf:type            owl:ObjectProperty;
        rdfs:comment        "Specifies the PlacementPoints of a PlaceableElementSpecification .\n"@en;
        rdfs:domain         vec:PlaceableElementSpecification;
        rdfs:label          "placementPoint"@en;
        rdfs:range          vec:PlacementPoint;
        rdfs:subPropertyOf  vec:contains .

vec:PrimaryPartType_Battery
        rdf:type         vec:PrimaryPartType , owl:NamedIndividiual;
        vec:enumLiteral  "Battery" .

vec:changeDescriptionIdentification
        rdf:type      owl:DatatypeProperty;
        rdfs:comment  "Specifies an identifier for the ChangeDescription. This can be the ID of a change order or an ID which indicates model upgrading. (see KBLFRM-249)\n"@en;
        rdfs:domain   vec:ChangeDescription;
        rdfs:label    "identification"@en;
        rdfs:range    xs:string .

vec:netGroupDescription
        rdf:type            owl:ObjectProperty;
        rdfs:comment        "Room for additional, human readable information about the NetGroup.\n"@en;
        rdfs:domain         vec:NetGroup;
        rdfs:label          "description"@en;
        rdfs:range          vec:AbstractLocalizedString;
        rdfs:subPropertyOf  vec:contains .

vec:boltMountedFixingSpecificationBoltHeight
        rdf:type            owl:ObjectProperty;
        rdfs:comment        "Specifies the height of the bolt on which the fixing can be mounted.\n"@en;
        rdfs:domain         vec:BoltMountedFixingSpecification;
        rdfs:label          "boltHeight"@en;
        rdfs:range          vec:NumericalValue;
        rdfs:subPropertyOf  vec:contains .

vec:wireElementSpecificationGridSpacing
        rdf:type            owl:ObjectProperty;
        rdfs:comment        "Defines the grid spacing. The grid spacing is the distance between the centres of two adjacent sub wire elements.\nThis attribute is only valid for WireElementSpecifications that have SubWireElementSpecifications.\n"@en;
        rdfs:domain         vec:WireElementSpecification;
        rdfs:label          "gridSpacing"@en;
        rdfs:range          vec:NumericalValue;
        rdfs:subPropertyOf  vec:contains .

vec:geometrySegmentReferenceSegment
        rdf:type      owl:ObjectProperty;
        rdfs:comment  "References the TopologySegment that is represented by the GeometrySegment. \n"@en;
        rdfs:domain   vec:GeometrySegment;
        rdfs:label    "referenceSegment"@en;
        rdfs:range    vec:TopologySegment .

vec:wireElementSpecificationImpedance
        rdf:type            owl:ObjectProperty;
        rdfs:comment        "Defines the impedance of this wireElement. Typically used for WireElements that have subWireElements e.g. twisted pair or coax wires.\n"@en;
        rdfs:domain         vec:WireElementSpecification;
        rdfs:label          "impedance"@en;
        rdfs:range          vec:NumericalValue;
        rdfs:subPropertyOf  vec:contains .

vec:functionalStructureNodeIdentification
        rdf:type      owl:DatatypeProperty;
        rdfs:comment  "Specifies a unique identification of the FunctionalStructureNode.\n"@en;
        rdfs:domain   vec:FunctionalStructureNode;
        rdfs:label    "identification"@en;
        rdfs:range    xs:string .

vec:connectorHousingSpecificationVoltageRange
        rdf:type            owl:ObjectProperty;
        rdfs:comment        "Specifies the allowed voltage range for the connector housing.\n"@en;
        rdfs:domain         vec:ConnectorHousingSpecification;
        rdfs:label          "voltageRange"@en;
        rdfs:range          vec:ValueRange;
        rdfs:subPropertyOf  vec:contains .

vec:vecContentCopyrightInformation
        rdf:type            owl:ObjectProperty;
        rdfs:comment        "Specifies the CopyrightInformation used in the VEC-file. \n"@en;
        rdfs:domain         vec:VecContent;
        rdfs:label          "copyrightInformation"@en;
        rdfs:range          vec:CopyrightInformation;
        rdfs:subPropertyOf  vec:contains .

vec:TerminalSpecification
        rdf:type         owl:Class;
        rdfs:comment     "Specification for the definition of terminals. A terminal can own multiple WireReceptions & TerminalReceptions.\n"@en;
        rdfs:label       "TerminalSpecification"@en;
        rdfs:subClassOf  vec:PartOrUsageRelatedSpecification .

vec:SiUnitName_Steradian
        rdf:type         vec:SiUnitName , owl:NamedIndividiual;
        vec:enumLiteral  "Steradian" .

vec:slotSpecificationNumberOfCavities
        rdf:type      owl:DatatypeProperty;
        rdfs:comment  "The possible number of cavities in the layout defined by the SlotSpecification. This includes all cavities in the layout. The actual Slot can define specific cavities in the layout as \"not available\".\n"@en;
        rdfs:domain   vec:SlotSpecification;
        rdfs:label    "numberOfCavities"@en;
        rdfs:range    xs:integer .

vec:Person  rdf:type  owl:Class;
        rdfs:comment  "Specifies all relevant data of a person.\n"@en;
        rdfs:label    "Person"@en .

vec:MatingPoint  rdf:type  owl:Class;
        rdfs:comment     "A MatingPoint defines the Mating of two terminals. This normally occurs when two inliners are connected. Then terminals of one side (female) are mated with terminals of the other side (male).\n"@en;
        rdfs:label       "MatingPoint"@en;
        rdfs:subClassOf  vec:ConfigurableElement .

vec:OtherUnitName  rdf:type  owl:Class;
        rdfs:comment         "Enumeration for the definition of other unit names.\n"@en;
        rdfs:label           "OtherUnitName"@en;
        rdfs:subClassOf      vec:ClosedEnumeration;
        owl:equivalentClass  [ rdf:type   owl:Class;
                               owl:oneOf  ( vec:OtherUnitName_Pi vec:OtherUnitName_Piece )
                             ] .

vec:configurationConstraintConfigInfo
        rdf:type      owl:ObjectProperty;
        rdfs:comment  "References the configuration information that applies to the ConfigurationConstraint.\n"@en;
        rdfs:domain   vec:ConfigurationConstraint;
        rdfs:label    "configInfo"@en;
        rdfs:range    vec:VariantConfiguration .

vec:Transformation2D  rdf:type  owl:Class;
        rdfs:comment     "A Transformation is a geometric transformation and specifies a transformation matrix.\n"@en;
        rdfs:label       "Transformation2D"@en;
        rdfs:subClassOf  vec:ExtendableElement .

vec:ValueWithUnit  rdf:type  owl:Class;
        rdfs:comment  "Abstract class either for a single numerical measure or a range of numerical measures with upper, lower, or upper and lower bounds.\n"@en;
        rdfs:label    "ValueWithUnit"@en .

vec:TubeSlitStyle_TwoParts
        rdf:type         vec:TubeSlitStyle , owl:NamedIndividiual;
        rdfs:comment     "Two-parted tubes consist of inner tube and an outer tube (normally defined as one PartNumber) . Both tubes are slit and are combined into each other during assembly, thus creating one closed tube.\n"@en;
        vec:enumLiteral  "TwoParts" .

vec:partVersionNature
        rdf:type            owl:ObjectProperty;
        rdfs:comment        "The nature specifies how the PartVersion can be used in the different processes or the significance of the PartVersion in the process.\nThe nature of a PartVersion is normally inherent and does not change. If the nature the underlying part changes a new (other) partNumber is assigned to the part and respectively a new PartVersion is created.\nIt used to differentiate for example normal (productive) part numbers from preliminary (prototypic) part numbers.\n"@en;
        rdfs:domain         vec:PartVersion;
        rdfs:label          "nature"@en;
        rdfs:range          vec:PartNature;
        rdfs:subPropertyOf  vec:contains .

[ rdf:type     owl:AllDisjointClasses;
  owl:members  ( vec:PartOccurrence vec:PartUsage )
] .

vec:LanguageCode_Sg  rdf:type  vec:LanguageCode , owl:NamedIndividiual;
        vec:enumLiteral  "Sg" .

vec:baselineSpecificationContent
        rdf:type            owl:ObjectProperty;
        rdfs:comment        "Defines the state of the content of the baseline in regard of its defined scope.\n┬á\n"@en;
        rdfs:domain         vec:BaselineSpecification;
        rdfs:label          "content"@en;
        rdfs:range          vec:BaselineContent;
        rdfs:subPropertyOf  vec:contains .

vec:PinType_Optical  rdf:type  vec:PinType , owl:NamedIndividiual;
        vec:enumLiteral  "optical" .

vec:ShrinkableTubeSpecification
        rdf:type         owl:Class;
        rdfs:comment     "Specification of tubes that are shrinkable.\n"@en;
        rdfs:label       "ShrinkableTubeSpecification"@en;
        rdfs:subClassOf  vec:TubeSpecification .

vec:PinVoltageType_StandbyVoltage
        rdf:type         vec:PinVoltageType , owl:NamedIndividiual;
        vec:enumLiteral  "standbyVoltage" .

vec:componentConnectorComponentPort
        rdf:type            owl:ObjectProperty;
        rdfs:comment        "Specifies the ComponentPorts of the ComponentConnector.\n"@en;
        rdfs:domain         vec:ComponentConnector;
        rdfs:label          "componentPort"@en;
        rdfs:range          vec:ComponentPort;
        rdfs:subPropertyOf  vec:contains .

vec:networkPortDescription
        rdf:type            owl:ObjectProperty;
        rdfs:comment        "Room for additional, human readable information about the NetworkPort.\n"@en;
        rdfs:domain         vec:NetworkPort;
        rdfs:label          "description"@en;
        rdfs:range          vec:AbstractLocalizedString;
        rdfs:subPropertyOf  vec:contains .

vec:Placement  rdf:type  owl:Class;
        rdfs:comment     "A placement defines the placement of a PlaceableElementRole onto a Topology. For the definition of the place on the Topology, Locations are used. A Placement can either be a placement on discrete points (OnPointPlacement) or on an area of the topology (OnWayPlacement).\n"@en;
        rdfs:label       "Placement"@en;
        rdfs:subClassOf  vec:ConfigurableElement .

vec:SiUnitName_Pascal
        rdf:type         vec:SiUnitName , owl:NamedIndividiual;
        vec:enumLiteral  "Pascal" .

[ rdf:type     owl:AllDisjointClasses;
  owl:members  ( vec:PartWithSubComponentsRole vec:SpecificRole vec:CavityPlugRole vec:CavitySealRole vec:ConnectorHousingRole vec:EEComponentRole vec:TerminalRole vec:WireRole vec:ConnectorHousingCapRole vec:WireEndAccessoryRole vec:CavityAccessoryRole vec:LabelingRole vec:FixingRole vec:GrommetRole vec:WireProtectionRole vec:CableDuctRole vec:CableTieRole vec:FerriteRole vec:PlaceableElementRole )
] .

vec:LanguageCode_Mi  rdf:type  vec:LanguageCode , owl:NamedIndividiual;
        vec:enumLiteral  "Mi" .

vec:HoleMountedFixingHoleShape
        rdf:type         owl:Class;
        rdfs:comment     "Open Enumeration of standard hole shapes (see HoleMountedFixingSpecification.holeShape)."@en;
        rdfs:label       "HoleMountedFixingHoleShape"@en;
        rdfs:subClassOf  vec:OpenEnumeration .

vec:edgeMountedFixingSpecificationEdgeThickness
        rdf:type            owl:ObjectProperty;
        rdfs:comment        "Defines a range of valid thicknesses, onto which the fixing can be mounted.\n"@en;
        rdfs:domain         vec:EdgeMountedFixingSpecification;
        rdfs:label          "edgeThickness"@en;
        rdfs:range          vec:ValueRange;
        rdfs:subPropertyOf  vec:contains .

vec:pinComponentReferencePinComponent
        rdf:type      owl:ObjectProperty;
        rdfs:comment  "Points to the PinComponent referenced by the PinComponent reference. \n(KBLFRM-401)\n"@en;
        rdfs:domain   vec:PinComponentReference;
        rdfs:label    "pinComponent"@en;
        rdfs:range    vec:PinComponent .

vec:localGeometrySpecificationBaseUnit
        rdf:type      owl:ObjectProperty;
        rdfs:comment  "The Unit in which all coordinates (e.g. cartesian points)┬áare defined. Shall be a unit of length┬á(e.g. millimetre).\n"@en;
        rdfs:domain   vec:LocalGeometrySpecification;
        rdfs:label    "baseUnit"@en;
        rdfs:range    vec:Unit .

vec:wireReceptionSpecificationMultiContact
        rdf:type      owl:DatatypeProperty;
        rdfs:comment  "Specifies if it is possible to contact more than one core at the wire reception. If this attribute is set to true, the wire reception is allowed for more than one wire, but one wire is possible as well. If set to false, only one wire is allowed.\n"@en;
        rdfs:domain   vec:WireReceptionSpecification;
        rdfs:label    "multiContact"@en;
        rdfs:range    xs:boolean .

vec:NetworkNodeType_EnergyStorage
        rdf:type         vec:NetworkNodeType , owl:NamedIndividiual;
        rdfs:comment     "A┬ádevice that stores energy in some kind of way (e.g. a battery).\n"@en;
        vec:enumLiteral  "EnergyStorage" .

vec:placementSpecificationPlacement
        rdf:type            owl:ObjectProperty;
        rdfs:comment        "Specifies the Placements defined by the PlacementSpecification.\n"@en;
        rdfs:domain         vec:PlacementSpecification;
        rdfs:label          "placement"@en;
        rdfs:range          vec:Placement;
        rdfs:subPropertyOf  vec:contains .

vec:functionalStructureNodeAliasId
        rdf:type            owl:ObjectProperty;
        rdfs:comment        "Room to specify additional identifiers for the FunctionalStructureNode .\n"@en;
        rdfs:domain         vec:FunctionalStructureNode;
        rdfs:label          "aliasId"@en;
        rdfs:range          vec:AliasIdentification;
        rdfs:subPropertyOf  vec:contains .

vec:cavitySealSpecificationWireReceptionType
        rdf:type            owl:ObjectProperty;
        rdfs:comment        "Specifies the wireReceptionType to which the cavity seal fits.\n"@en;
        rdfs:domain         vec:CavitySealSpecification;
        rdfs:label          "wireReceptionType"@en;
        rdfs:range          vec:WireReceptionType;
        rdfs:subPropertyOf  vec:contains .

vec:LanguageCode_Am  rdf:type  vec:LanguageCode , owl:NamedIndividiual;
        vec:enumLiteral  "Am" .

vec:harnessGeometrySpecification3DBuildingBlockPositionings
        rdf:type            owl:ObjectProperty;
        rdfs:comment        "Specifies the BuildingBlockPositioning3Ds that are forming the HarnessGeometrySpecification3D.\n"@en;
        rdfs:domain         vec:HarnessGeometrySpecification3D;
        rdfs:label          "buildingBlockPositionings"@en;
        rdfs:range          vec:BuildingBlockPositioning3D;
        rdfs:subPropertyOf  vec:contains .

vec:USUnitName_Gallon
        rdf:type         vec:USUnitName , owl:NamedIndividiual;
        vec:enumLiteral  "Gallon" .

vec:PrimaryPartType_PartStructure
        rdf:type         vec:PrimaryPartType , owl:NamedIndividiual;
        vec:enumLiteral  "PartStructure" .

vec:netTypeSignalTransmissionMediumType
        rdf:type            owl:ObjectProperty;
        rdfs:comment        "Specifies the type of the transmission medium for signals of this type.\n"@en;
        rdfs:domain         vec:NetType;
        rdfs:label          "signalTransmissionMediumType"@en;
        rdfs:range          vec:SignalTransmissionMediumType;
        rdfs:subPropertyOf  vec:contains .

vec:WireGroupType_Twisted
        rdf:type         vec:WireGroupType , owl:NamedIndividiual;
        vec:enumLiteral  "Twisted" .

vec:diodeSpecificationCathode
        rdf:type     owl:ObjectProperty;
        rdfs:domain  vec:DiodeSpecification;
        rdfs:label   "cathode"@en;
        rdfs:range   vec:PinComponent .

vec:connectionEndIdentification
        rdf:type      owl:DatatypeProperty;
        rdfs:comment  "Specifies a unique identification of the ConnectionEnd. The identification is guaranteed to be unique within the ConnectionSpecification.\n"@en;
        rdfs:domain   vec:ConnectionEnd;
        rdfs:label    "identification"@en;
        rdfs:range    xs:string .

vec:LanguageCode_Km  rdf:type  vec:LanguageCode , owl:NamedIndividiual;
        vec:enumLiteral  "Km" .

vec:FittingForm_Cap  rdf:type  vec:FittingForm , owl:NamedIndividiual;
        rdfs:comment     "Cap for the closure of tubes and pipes.\n"@en;
        vec:enumLiteral  "Cap" .

vec:cableTieSpecificationLength
        rdf:type            owl:ObjectProperty;
        rdfs:comment        ""@en;
        rdfs:domain         vec:CableTieSpecification;
        rdfs:label          "length"@en;
        rdfs:range          vec:NumericalValue;
        rdfs:subPropertyOf  vec:contains .

vec:LanguageCode_Sl  rdf:type  vec:LanguageCode , owl:NamedIndividiual;
        vec:enumLiteral  "Sl" .

vec:cartesianDimensionHeight
        rdf:type      owl:DatatypeProperty;
        rdfs:comment  "Specifies the height of the object. The unit of this value is the baseUnit of containing BuildingBlockSpecification2D.\n"@en;
        rdfs:domain   vec:CartesianDimension;
        rdfs:label    "height"@en;
        rdfs:range    xs:double .

vec:IECPrefix_Gibi  rdf:type  vec:IECPrefix , owl:NamedIndividiual;
        vec:enumLiteral  "Gibi" .

vec:SlotGender_Unspecified
        rdf:type         vec:SlotGender , owl:NamedIndividiual;
        vec:enumLiteral  "Unspecified" .

vec:LanguageCode_Eo  rdf:type  vec:LanguageCode , owl:NamedIndividiual;
        vec:enumLiteral  "Eo" .

vec:PinCurrentInformation
        rdf:type      owl:Class;
        rdfs:comment  "Allows the definition of currents for a pin of an EEComponent. A current can be further specified by a duration. Attributes of the type PinCurrentInformation normally have the multiplicity [0..*]. This means that such an attribute can have PinCurrentInformation entries for different types and durations. It must not have multiple entries for the same type and duration.\n"@en;
        rdfs:label    "PinCurrentInformation"@en .

vec:functionalRequirementReferenceSystem
        rdf:type      owl:DatatypeProperty;
        rdfs:comment  "The reference system identifies the system in which the values are defined (e.g. ISO26262)\n"@en;
        rdfs:domain   vec:FunctionalRequirement;
        rdfs:label    "referenceSystem"@en;
        rdfs:range    xs:string .

vec:LanguageCode_Mn  rdf:type  vec:LanguageCode , owl:NamedIndividiual;
        vec:enumLiteral  "Mn" .

vec:sheetOrChapterSheetFormat
        rdf:type      owl:DatatypeProperty;
        rdfs:comment  "Defines the format┬áof the SheetOrChapter. This is an alias for a specific sheet /┬ápaper size (e.g. DINA4). If both attributes are defined the SheetSize takes precedence.\n"@en;
        rdfs:domain   vec:SheetOrChapter;
        rdfs:label    "sheetFormat"@en;
        rdfs:range    xs:string .

vec:occurrenceOrUsageViewItem3DAliasId
        rdf:type            owl:ObjectProperty;
        rdfs:comment        "Specifies additional identifiers for the OccurrenceOrUsageViewItem3D.\n"@en;
        rdfs:domain         vec:OccurrenceOrUsageViewItem3D;
        rdfs:label          "aliasId"@en;
        rdfs:range          vec:AliasIdentification;
        rdfs:subPropertyOf  vec:contains .

vec:NetworkNodeType_Switch
        rdf:type         vec:NetworkNodeType , owl:NamedIndividiual;
        rdfs:comment     "A \"Switch\" is a device that can change its internal connectivity in reaction to some external action (e.g. connect /┬ádisconnect┬ásome pins). A switch has no \"active\" logic (in contrast to an ECU).\n"@en;
        vec:enumLiteral  "Switch" .
