@prefix :     <http://www.prostep.org/ontologies/ecad/2024/03/vec#> .
@prefix owl:  <http://www.w3.org/2002/07/owl#> .
@prefix rdf:  <http://www.w3.org/1999/02/22-rdf-syntax-ns#> .
@prefix rdfs: <http://www.w3.org/2000/01/rdf-schema#> .
@prefix vec:  <http://www.prostep.org/ontologies/ecad/2024/03/vec#> .
@prefix xs:   <http://www.w3.org/2001/XMLSchema#> .

vec:ImperialUnitName_Quarter
        rdf:type         vec:ImperialUnitName , owl:NamedIndividiual;
        vec:enumLiteral  "Quarter" .

vec:specificationDescription
        rdf:type            owl:ObjectProperty;
        rdfs:comment        "Specifies additional, human readable information about the specification.\n"@en;
        rdfs:domain         vec:Specification;
        rdfs:label          "description"@en;
        rdfs:range          vec:AbstractLocalizedString;
        rdfs:subPropertyOf  vec:contains .

vec:ImperialUnitName_Furlong
        rdf:type         vec:ImperialUnitName , owl:NamedIndividiual;
        vec:enumLiteral  "Furlong" .

vec:sheetOrChapterIdentification
        rdf:type      owl:DatatypeProperty;
        rdfs:comment  "The identification of the sheet or chapter within the document. This value must be distinct within the context of a document.\n"@en;
        rdfs:domain   vec:SheetOrChapter;
        rdfs:label    "identification"@en;
        rdfs:range    xs:string .

vec:LanguageCode_Pa  rdf:type  vec:LanguageCode , owl:NamedIndividiual;
        vec:enumLiteral  "Pa" .

vec:relaySpecificationSwitchContact
        rdf:type      owl:ObjectProperty;
        rdfs:comment  "References the PinComponents that are the SwitchContacts of the Relay. \n"@en;
        rdfs:domain   vec:RelaySpecification;
        rdfs:label    "switchContact"@en;
        rdfs:range    vec:PinComponent .

vec:connectionEndConnectedComponentPort
        rdf:type      owl:ObjectProperty;
        rdfs:comment  "References the ComponentPort that is connected by the ConnectionEnd. \n"@en;
        rdfs:domain   vec:ConnectionEnd;
        rdfs:label    "connectedComponentPort"@en;
        rdfs:range    vec:ComponentPort .

vec:locationIdentification
        rdf:type      owl:DatatypeProperty;
        rdfs:comment  "Specifies a unique identification of the Location. The identification is guaranteed to be unique within the PlacementSpecification.\n"@en;
        rdfs:domain   vec:Location;
        rdfs:label    "identification"@en;
        rdfs:range    xs:string .

vec:CompatibilitySpecification
        rdf:type         owl:Class;
        rdfs:comment     "A CompatibilitySpecification specifies a set of CompatibilityStatements.\n"@en;
        rdfs:label       "CompatibilitySpecification"@en;
        rdfs:subClassOf  vec:Specification .

vec:GeometryNode  rdf:type  owl:Class;
        rdfs:comment     "A GeometryNode is the geometric representation of a TopologyNode. A TopologyNode may be represented by more than one GeometryNodes. A GeometryNode is either a GeometryNode2D or a GeometryNode3D.\n"@en;
        rdfs:label       "GeometryNode"@en;
        rdfs:subClassOf  vec:ConfigurableElement .

vec:PinVoltageType_StandbyVoltage
        rdf:type         vec:PinVoltageType , owl:NamedIndividiual;
        vec:enumLiteral  "standbyVoltage" .

vec:cableDuctSpecificationOutlet
        rdf:type            owl:ObjectProperty;
        rdfs:comment        ""@en;
        rdfs:domain         vec:CableDuctSpecification;
        rdfs:label          "outlet"@en;
        rdfs:range          vec:CableDuctOutlet;
        rdfs:subPropertyOf  vec:contains .

vec:occurrenceOrUsageDescription
        rdf:type            owl:ObjectProperty;
        rdfs:comment        "Specifies additional, human readable information about the OccurrenceOrUsage.\n"@en;
        rdfs:domain         vec:OccurrenceOrUsage;
        rdfs:label          "description"@en;
        rdfs:range          vec:AbstractLocalizedString;
        rdfs:subPropertyOf  vec:contains .

vec:SiPrefix_Hecto  rdf:type  vec:SiPrefix , owl:NamedIndividiual;
        vec:enumLiteral  "Hecto" .

vec:ImperialUnitName_Perch
        rdf:type         vec:ImperialUnitName , owl:NamedIndividiual;
        vec:enumLiteral  "Perch" .

vec:SegmentLength  rdf:type  owl:Class;
        rdfs:comment     "Specifies the length of a segment. Attributes of the type SegmentLength normally have the multiplicity [0..*]. This means that such an attribute can have SegmentLength-entries for different classifications. It must not have multiple entries with the same classification.\n"@en;
        rdfs:label       "SegmentLength"@en;
        rdfs:subClassOf  vec:ExtendableElement .

vec:WireEnd  rdf:type    owl:Class;
        rdfs:comment     "A WireEnd is the end of a wire. This class mainly needed for the definition of a contacting. As a wire can be contacted on more than two ends (e.g. IDC) the WireEnd has a position on the wire.\n"@en;
        rdfs:label       "WireEnd"@en;
        rdfs:subClassOf  vec:ExtendableElement .

vec:itemVersionContract
        rdf:type      owl:ObjectProperty;
        rdfs:comment  "References the contracts that apply to an ItemVersion.\n"@en;
        rdfs:domain   vec:ItemVersion;
        rdfs:label    "contract"@en;
        rdfs:range    vec:Contract .

vec:ExternalMappingSpecification
        rdf:type         owl:Class;
        rdfs:comment     "An ExternalMappingSpecification is used to define a mapping between an external data source (represented by the referenced mappedDocument ) and the content of a VEC file.\n"@en;
        rdfs:label       "ExternalMappingSpecification"@en;
        rdfs:subClassOf  vec:Specification .

[ rdf:type     owl:AllDisjointClasses;
  owl:members  ( vec:PluggableTerminalSpecification vec:RingTerminalSpecification vec:SpliceTerminalSpecification )
] .

vec:OccurrenceOrUsage
        rdf:type         owl:Class;
        rdfs:comment     "An OccurrenceOrUsage is an abstract appearance of a part in the harness. This can either be a concrete part (with a part number a.s.o) or the description (specification / requirements) of a part that should be used at that position. In the first case it would be a PartOccurrence in the second case a PartUsage.\n"@en;
        rdfs:label       "OccurrenceOrUsage"@en;
        rdfs:subClassOf  vec:ConfigurableElement .

vec:abrasionResistanceClassClassKey
        rdf:type      owl:DatatypeProperty;
        rdfs:comment  "Specifies a key for the level defined in the abrasion resistance class (e.g. A, B, C).\n"@en;
        rdfs:domain   vec:AbrasionResistanceClass;
        rdfs:label    "classKey"@en;
        rdfs:range    xs:string .

vec:soundDampingClassClassKey
        rdf:type      owl:DatatypeProperty;
        rdfs:comment  "Specifies a key for the level defined in the sound damping class (e.g. A, B, C).\n"@en;
        rdfs:domain   vec:SoundDampingClass;
        rdfs:label    "classKey"@en;
        rdfs:range    xs:string .

vec:LanguageCode_Cy  rdf:type  vec:LanguageCode , owl:NamedIndividiual;
        vec:enumLiteral  "Cy" .

vec:LanguageCode_Tr  rdf:type  vec:LanguageCode , owl:NamedIndividiual;
        vec:enumLiteral  "Tr" .

vec:cavitySealSpecificationWireElementOutsideDiameter
        rdf:type            owl:ObjectProperty;
        rdfs:comment        "Specifies a range of valid wire diameters to which the cavity seal fits.\n"@en;
        rdfs:domain         vec:CavitySealSpecification;
        rdfs:label          "wireElementOutsideDiameter"@en;
        rdfs:range          vec:ValueRange;
        rdfs:subPropertyOf  vec:contains .

vec:cavityPlugRoleCavityPlugSpecification
        rdf:type      owl:ObjectProperty;
        rdfs:comment  "References the CavityPlugSpecification that is instanced by this CavityPlugRole.\n"@en;
        rdfs:domain   vec:CavityPlugRole;
        rdfs:label    "cavityPlugSpecification"@en;
        rdfs:range    vec:CavityPlugSpecification .

vec:relaySpecificationIMax
        rdf:type            owl:ObjectProperty;
        rdfs:comment        "Specifies the maximum current allowed for the relais.\n"@en;
        rdfs:domain         vec:RelaySpecification;
        rdfs:label          "iMax"@en;
        rdfs:range          vec:NumericalValue;
        rdfs:subPropertyOf  vec:contains .

vec:netNetworkPort  rdf:type  owl:ObjectProperty;
        rdfs:comment  "References the NetworkPorts that are connected by the Net. \n"@en;
        rdfs:domain   vec:Net;
        rdfs:label    "networkPort"@en;
        rdfs:range    vec:NetworkPort .

vec:CavityPlugSpecification
        rdf:type         owl:Class;
        rdfs:comment     "Specification for the definition of cavity seals. A cavity plug is a water tight non-electrical object to fill an empty cavity.\n"@en;
        rdfs:label       "CavityPlugSpecification"@en;
        rdfs:subClassOf  vec:PartOrUsageRelatedSpecification .

vec:contactPointWireMounting
        rdf:type            owl:ObjectProperty;
        rdfs:comment        "Specifies the WireMouting defined by ContactPoint. More than one WireMounting is allowed in order to support variance. In concrete configuration the WireMounting with all referenced elements present is used.\n"@en;
        rdfs:domain         vec:ContactPoint;
        rdfs:label          "wireMounting"@en;
        rdfs:range          vec:WireMounting;
        rdfs:subPropertyOf  vec:contains .

vec:LanguageCode_So  rdf:type  vec:LanguageCode , owl:NamedIndividiual;
        vec:enumLiteral  "So" .

vec:temperatureInformationTemperatureType
        rdf:type      owl:DatatypeProperty;
        rdfs:comment  "The type of a TemperatureInformation. This should be an enumeration of values defined in a conformance class. Possible values are: EnvironmentTemperature, OperationTemperature, StorageTemperature, ProcessingTemperature. (see KBLFRM-311)\n"@en;
        rdfs:domain   vec:TemperatureInformation;
        rdfs:label    "temperatureType"@en;
        rdfs:range    xs:string .

vec:LanguageCode_As  rdf:type  vec:LanguageCode , owl:NamedIndividiual;
        vec:enumLiteral  "As" .

vec:compatibilityStatementHasCompatibility
        rdf:type      owl:DatatypeProperty;
        rdfs:comment  "If true the CompatibilityStatement states compatibility, otherwise incompatibility.\n"@en;
        rdfs:domain   vec:CompatibilityStatement;
        rdfs:label    "hasCompatibility"@en;
        rdfs:range    xs:boolean .

vec:LanguageCode_In  rdf:type  vec:LanguageCode , owl:NamedIndividiual;
        vec:enumLiteral  "In" .

vec:PlacementType_OnWay
        rdf:type         vec:PlacementType , owl:NamedIndividiual;
        rdfs:comment     " OnWay refers to an OnWayPlacement .\n"@en;
        vec:enumLiteral  "OnWay" .

vec:SiUnitName_Metre  rdf:type  vec:SiUnitName , owl:NamedIndividiual;
        vec:enumLiteral  "Metre" .

vec:documentVersionSpecification
        rdf:type            owl:ObjectProperty;
        rdfs:comment        "Specifies the Specifications contained in the DocumentVersion. All structured, technical information in the VEC is described by such Specifications. \n"@en;
        rdfs:domain         vec:DocumentVersion;
        rdfs:label          "specification"@en;
        rdfs:range          vec:Specification;
        rdfs:subPropertyOf  vec:contains .

vec:conductorCurrentInformationVoltage
        rdf:type            owl:ObjectProperty;
        rdfs:comment        "The voltage for which this maximum current value is applicable.\n"@en;
        rdfs:domain         vec:ConductorCurrentInformation;
        rdfs:label          "voltage"@en;
        rdfs:range          vec:NumericalValue;
        rdfs:subPropertyOf  vec:contains .

vec:imperialUnitImperialUnitName
        rdf:type            owl:ObjectProperty;
        rdfs:comment        "Specifies the name of the imperial unit.\n"@en;
        rdfs:domain         vec:ImperialUnit;
        rdfs:label          "imperialUnitName"@en;
        rdfs:range          vec:ImperialUnitName;
        rdfs:subPropertyOf  vec:contains .

vec:eEComponentSpecificationHousingComponent
        rdf:type            owl:ObjectProperty;
        rdfs:comment        "Specifies the available connector interfaces of the EEComponent. \n"@en;
        rdfs:domain         vec:EEComponentSpecification;
        rdfs:label          "housingComponent"@en;
        rdfs:range          vec:HousingComponent;
        rdfs:subPropertyOf  vec:contains .

vec:compatibilityStatementTerminalSpecification
        rdf:type      owl:ObjectProperty;
        rdfs:comment  "References the TerminalSpecifications for which the compatibility statement is stated.\n"@en;
        rdfs:domain   vec:CompatibilityStatement;
        rdfs:label    "terminalSpecification"@en;
        rdfs:range    vec:TerminalSpecification .

vec:wireMountingMountedCavitySeal
        rdf:type      owl:ObjectProperty;
        rdfs:comment  "References the cavity seal that is used for the wire mounting.\n"@en;
        rdfs:domain   vec:WireMounting;
        rdfs:label    "mountedCavitySeal"@en;
        rdfs:range    vec:CavitySealRole .

vec:SIUnit  rdf:type     owl:Class;
        rdfs:comment     "The SIUnit class can define quantities in the terms of the SI-Unit-System by specifying the corresponding SI prefix (optional) and a SI unit name. The usage of SI units must be the preferred way of expressing units, since these units can be easily translated into other SI units.\n"@en;
        rdfs:label       "SIUnit"@en;
        rdfs:subClassOf  vec:Unit .

vec:cartesianPoint3DWrapperItem
        rdf:type      owl:ObjectProperty;
        rdfs:comment  "References the actual item for a Wrapper.";
        rdfs:domain   vec:CartesianPoint3DWrapper;
        rdfs:range    vec:CartesianPoint3D .

vec:USUnitName_Acre  rdf:type  vec:USUnitName , owl:NamedIndividiual;
        vec:enumLiteral  "Acre" .

vec:itemEquivalenceItem
        rdf:type      owl:ObjectProperty;
        rdfs:comment  "References all ItemVersion that are considered to be equivalent by the ItemEquivalence. \n"@en;
        rdfs:domain   vec:ItemEquivalence;
        rdfs:label    "item"@en;
        rdfs:range    vec:ItemVersion .

vec:LanguageCode_Oc  rdf:type  vec:LanguageCode , owl:NamedIndividiual;
        vec:enumLiteral  "Oc" .

vec:pinComponentIdentification
        rdf:type      owl:DatatypeProperty;
        rdfs:comment  "Identification of the PinComponent, which must be distinct for all PinComponent of a HousingComponents.\n"@en;
        rdfs:domain   vec:PinComponent;
        rdfs:label    "identification"@en;
        rdfs:range    xs:string .

vec:cartesianPoint2DWrapperItem
        rdf:type      owl:ObjectProperty;
        rdfs:comment  "References the actual item for a Wrapper.";
        rdfs:domain   vec:CartesianPoint2DWrapper;
        rdfs:range    vec:CartesianPoint2D .

vec:tubeSpecificationOuterDiameter
        rdf:type            owl:ObjectProperty;
        rdfs:comment        "Specifies the outer diameter of the tube.\n"@en;
        rdfs:domain         vec:TubeSpecification;
        rdfs:label          "outerDiameter"@en;
        rdfs:range          vec:NumericalValue;
        rdfs:subPropertyOf  vec:contains .

vec:wireReceptionSpecificationWireElementOutsideDiameter
        rdf:type            owl:ObjectProperty;
        rdfs:comment        "Specifies a value range for valid diameters a WireElement must have to fit to the wire reception.\n"@en;
        rdfs:domain         vec:WireReceptionSpecification;
        rdfs:label          "wireElementOutsideDiameter"@en;
        rdfs:range          vec:ValueRange;
        rdfs:subPropertyOf  vec:contains .

vec:NodeType_Inliner  rdf:type  vec:NodeType , owl:NamedIndividiual;
        rdfs:comment     "An Inliner is a TopologyNode where one section of the electrical system is connected to another section.\n"@en;
        vec:enumLiteral  "Inliner" .

vec:ImperialUnitName_Chain
        rdf:type         vec:ImperialUnitName , owl:NamedIndividiual;
        vec:enumLiteral  "Chain" .

vec:TerminalRole  rdf:type  owl:Class;
        rdfs:comment     "A TerminalRole defines the instance specific properties and relationships of a terminal.\n"@en;
        rdfs:label       "TerminalRole"@en;
        rdfs:subClassOf  vec:Role .

vec:contactSystemContactResistance
        rdf:type            owl:ObjectProperty;
        rdfs:comment        "Specifies the resistance of the contact system."@en;
        rdfs:domain         vec:ContactSystem;
        rdfs:label          "contactResistance"@en;
        rdfs:range          vec:NumericalValue;
        rdfs:subPropertyOf  vec:contains .

vec:wireGroupSpecificationGroupType
        rdf:type      owl:DatatypeProperty;
        rdfs:comment  "Specifies the type of the group. This should be an enumeration of values defined in a conformance class (e.g. twisted pair, ...).\n"@en;
        rdfs:domain   vec:WireGroupSpecification;
        rdfs:label    "groupType"@en;
        rdfs:range    xs:string .

vec:LanguageCode_Uz  rdf:type  vec:LanguageCode , owl:NamedIndividiual;
        vec:enumLiteral  "Uz" .

vec:colorKey  rdf:type  owl:DatatypeProperty;
        rdfs:comment  "The key of the color in the corresponding color reference system.\n"@en;
        rdfs:domain   vec:Color;
        rdfs:label    "key"@en;
        rdfs:range    xs:string .

vec:SiPrefix_Yotta  rdf:type  vec:SiPrefix , owl:NamedIndividiual;
        vec:enumLiteral  "Yotta" .

vec:fixingSpecificationOffset
        rdf:type            owl:ObjectProperty;
        rdfs:domain         vec:FixingSpecification;
        rdfs:label          "offset"@en;
        rdfs:range          vec:NumericalValue;
        rdfs:subPropertyOf  vec:contains .

vec:PrimaryPartType_MultiCavitySeal
        rdf:type         vec:PrimaryPartType , owl:NamedIndividiual;
        vec:enumLiteral  "MultiCavitySeal" .

vec:pinComponentBehaviorSignalDirection
        rdf:type            owl:ObjectProperty;
        rdfs:comment        "The direction of the signal on this pin.\n"@en;
        rdfs:domain         vec:PinComponentBehavior;
        rdfs:label          "signalDirection"@en;
        rdfs:range          vec:SignalDirection;
        rdfs:subPropertyOf  vec:contains .

vec:VariantCode  rdf:type  owl:Class;
        rdfs:comment     "VariantCodes are defining the literals on which VariantConfiguration are stated. Possible VariantCodes might be different for steering types, optional equipment, engine-power class.\n"@en;
        rdfs:label       "VariantCode"@en;
        rdfs:subClassOf  vec:ExtendableElement .

vec:LanguageCode_Tw  rdf:type  vec:LanguageCode , owl:NamedIndividiual;
        vec:enumLiteral  "Tw" .

vec:WireElementSpecification
        rdf:type         owl:Class;
        rdfs:comment     "A WireElementSpecification is the basic element to describe a wire in the VEC. A WireElementSpecification can be atomic or composed recursively out of other WireElementSpecifications. A WireElementSpecification can reference an InsulationSpecification, if it has an insulation, a CoreSpecification, if it has a core or a WireGroupSpecification if it is a grouping of other WireElementSpecifications in the Wire (e.g. a multi-core wire with twisted pairs).\n"@en;
        rdfs:label       "WireElementSpecification"@en;
        rdfs:subClassOf  vec:Specification .

vec:usageNodeUsageNodeType
        rdf:type            owl:ObjectProperty;
        rdfs:comment        "Defines the type of the UsageNode. The type determines how the UsageNode is handled in the latter processes.\n"@en;
        rdfs:domain         vec:UsageNode;
        rdfs:label          "usageNodeType"@en;
        rdfs:range          vec:UsageNodeType;
        rdfs:subPropertyOf  vec:contains .

vec:LanguageCode_Ky  rdf:type  vec:LanguageCode , owl:NamedIndividiual;
        vec:enumLiteral  "Ky" .

vec:SiPrefix_Kilo  rdf:type  vec:SiPrefix , owl:NamedIndividiual;
        vec:enumLiteral  "Kilo" .

vec:SiUnitName_Pascal
        rdf:type         vec:SiUnitName , owl:NamedIndividiual;
        vec:enumLiteral  "Pascal" .

vec:UsageConstraintType_Allow
        rdf:type         vec:UsageConstraintType , owl:NamedIndividiual;
        vec:enumLiteral  "Allow" .

vec:wireElementSpecificationOutsideDiameter
        rdf:type            owl:ObjectProperty;
        rdfs:comment        "Specifies the outside diameter of the WireElement.\n"@en;
        rdfs:domain         vec:WireElementSpecification;
        rdfs:label          "outsideDiameter"@en;
        rdfs:range          vec:NumericalValue;
        rdfs:subPropertyOf  vec:contains .

vec:LanguageCode_St  rdf:type  vec:LanguageCode , owl:NamedIndividiual;
        vec:enumLiteral  "St" .

vec:Routing  rdf:type    owl:Class;
        rdfs:comment     "A Routing is the assignment of a RoutableElement (Connection or WireElementReference) to a path in the topology.\n"@en;
        rdfs:label       "Routing"@en;
        rdfs:subClassOf  vec:ConfigurableElement .

[ rdf:type     owl:AllDisjointClasses;
  owl:members  ( vec:CompositeUnit vec:CustomUnit vec:IECUnit vec:ImperialUnit vec:OtherUnit vec:SIUnit vec:USUnit )
] .

vec:SiPrefix_Pico  rdf:type  vec:SiPrefix , owl:NamedIndividiual;
        vec:enumLiteral  "Pico" .

vec:UsageNode  rdf:type  owl:Class;
        rdfs:comment     "A UsageNode represents a position in an abstract vehicle. For example the \"Head Light Left\". UsageNodes belong to the master data and they are defined on some companywide level. They can be used to enforce consistent naming over different projects and different development streams (e.g. between Geometry and Electrologic).\nA UsageNode can be realized by different elements in the VEC (e.g. NetworkNode, OccurrenceOrUsage, TopologyNode, ComponentNode ).\n"@en;
        rdfs:label       "UsageNode"@en;
        rdfs:subClassOf  vec:ConfigurableElement .

vec:grommetSpecificationSealingClass
        rdf:type            owl:ObjectProperty;
        rdfs:comment        "Specifies the sealing class of the grommet.\n"@en;
        rdfs:domain         vec:GrommetSpecification;
        rdfs:label          "sealingClass"@en;
        rdfs:range          vec:SealingClass;
        rdfs:subPropertyOf  vec:contains .

vec:contactPointCavityMounting
        rdf:type            owl:ObjectProperty;
        rdfs:comment        "Defines the mounting to a cavity of the terminal associated with the ContactPoint. \nThe cardinality is 0..* in order to allow a variant dependant cavity mounting. In such a scenario a cavity mounting is valid in a configuration if all addressed cavities and therefore the associated connector housing is available. \n"@en;
        rdfs:domain         vec:ContactPoint;
        rdfs:label          "cavityMounting"@en;
        rdfs:range          vec:CavityMounting;
        rdfs:subPropertyOf  vec:contains .

vec:LanguageCode_Is  rdf:type  vec:LanguageCode , owl:NamedIndividiual;
        vec:enumLiteral  "Is" .

[ rdf:type     owl:AllDisjointClasses;
  owl:members  ( vec:CartesianVector2D vec:CartesianVector3D )
] .

vec:SiUnitName_Lumen  rdf:type  vec:SiUnitName , owl:NamedIndividiual;
        vec:enumLiteral  "Lumen" .

vec:LanguageCode_Yi  rdf:type  vec:LanguageCode , owl:NamedIndividiual;
        vec:enumLiteral  "Yi" .

vec:transformation2DA21
        rdf:type     owl:DatatypeProperty;
        rdfs:domain  vec:Transformation2D;
        rdfs:label   "a21"@en;
        rdfs:range   xs:double .

vec:WireProtectionRole
        rdf:type         owl:Class;
        rdfs:comment     "A WireProtectionRole defines the instance specific properties and relationships of a wire protection.\n"@en;
        rdfs:label       "WireProtectionRole"@en;
        rdfs:subClassOf  vec:Role .

vec:toleranceUpperBoundary
        rdf:type      owl:DatatypeProperty;
        rdfs:comment  "Specifies the upper boundary for the tolerance.\n"@en;
        rdfs:domain   vec:Tolerance;
        rdfs:label    "upperBoundary"@en;
        rdfs:range    xs:double .

vec:ComponentNode  rdf:type  owl:Class;
        rdfs:comment     "A ComponentNode is a node where an electrological component is located. It is a representative for an element in the electric system, e.g. an actuator, a sensor, an ECU. In this way it is quite similar to a NetworkNode and may even reference the corresponding NetworkNode in this case. However, a ComponentNode is more likely to be used as a representative of an inliner or a splice. Moreover, a ComponentNode can define childNodes in order to describe its internal structure.\n"@en;
        rdfs:label       "ComponentNode"@en;
        rdfs:subClassOf  vec:ConfigurableElement .

vec:WireType  rdf:type  owl:Class;
        rdfs:comment  "Specifies a wire type. A wire type is always defined by a key value. What wire type is meant by this key value is defined by a standard reference system.\n"@en;
        rdfs:label    "WireType"@en .

vec:networkPortIdentification
        rdf:type      owl:DatatypeProperty;
        rdfs:comment  "Specifies a unique identification of the NetworkPort. The identification is guaranteed to be unique within the NetSpecification.\n"@en;
        rdfs:domain   vec:NetworkPort;
        rdfs:label    "identification"@en;
        rdfs:range    xs:string .

vec:occurrenceOrUsageViewItem3DOccurrenceOrUsage
        rdf:type      owl:ObjectProperty;
        rdfs:comment  "Specifies the OccurrenceOrUsage which is represented by the view item.\n"@en;
        rdfs:domain   vec:OccurrenceOrUsageViewItem3D;
        rdfs:label    "occurrenceOrUsage"@en;
        rdfs:range    vec:OccurrenceOrUsage .

vec:signalRecommendedConductorSpecification
        rdf:type      owl:ObjectProperty;
        rdfs:comment  "Defines a recommended Specification for the cores that implement this signal.\n"@en;
        rdfs:domain   vec:Signal;
        rdfs:label    "recommendedConductorSpecification"@en;
        rdfs:range    vec:ConductorSpecification .

vec:Specification  rdf:type  owl:Class;
        rdfs:comment     "Abstract super-class for all specifications. Every technical information exchanged with the VEC is contained in the different specializations of a specification.\n"@en;
        rdfs:label       "Specification"@en;
        rdfs:subClassOf  vec:ExtendableElement .

vec:documentVersionFileName
        rdf:type      owl:DatatypeProperty;
        rdfs:comment  "If this DocumentVersion is a link to an external document (e.g. a ComponentSymbol), then the fileName attribute points to the file containing the original document. To use this attribute is only valid, if the original document is distributed along with the VEC-file e.g. in a ZIP-archive. It must not point to any file location which is not part of the bundle provided together with the VEC-file (e.g. a File on a central server file share).\n"@en;
        rdfs:domain   vec:DocumentVersion;
        rdfs:label    "fileName"@en;
        rdfs:range    xs:string .

vec:conductorSpecificationType
        rdf:type      owl:DatatypeProperty;
        rdfs:comment  "Specifies the type of the conductor. This should be an enumeration of values defined in a conformance class (e.g. solid, meshwork).\n"@en;
        rdfs:domain   vec:ConductorSpecification;
        rdfs:label    "type"@en;
        rdfs:range    xs:string .

vec:occurrenceOrUsageAliasId
        rdf:type            owl:ObjectProperty;
        rdfs:comment        "Room to specify additional identifiers for the OccurrenceOrUsage.\n"@en;
        rdfs:domain         vec:OccurrenceOrUsage;
        rdfs:label          "aliasId"@en;
        rdfs:range          vec:AliasIdentification;
        rdfs:subPropertyOf  vec:contains .

vec:partVersionPreferredUseCase
        rdf:type      owl:DatatypeProperty;
        rdfs:comment  "Defines the function for which the part was initially designed. (e.g. \"Grommet for Hatch\", \"...passenger compartment\",...) This is an important information for searching and selecting parts in the context of KOMP.\n"@en;
        rdfs:domain   vec:PartVersion;
        rdfs:label    "preferredUseCase"@en;
        rdfs:range    xs:string .

vec:LanguageCode_Fj  rdf:type  vec:LanguageCode , owl:NamedIndividiual;
        vec:enumLiteral  "Fj" .

vec:corrugatedPipeSpecificationCorrugationHeight
        rdf:type            owl:ObjectProperty;
        rdfs:comment        "Specifies the height of a corrugation of the pipe.\n"@en;
        rdfs:domain         vec:CorrugatedPipeSpecification;
        rdfs:label          "corrugationHeight"@en;
        rdfs:range          vec:NumericalValue;
        rdfs:subPropertyOf  vec:contains .

vec:DocumentVersion  rdf:type  owl:Class;
        rdfs:comment     "The DocumentVersion is one of the two anchors for PDM information in the VEC. All technical information about a PartVersion is contained in one or more documents. The documents are containing the actual content of the VEC since all Specifications are an element of a document.\n"@en;
        rdfs:label       "DocumentVersion"@en;
        rdfs:subClassOf  vec:ItemVersion .

vec:LanguageCode_Ne  rdf:type  vec:LanguageCode , owl:NamedIndividiual;
        vec:enumLiteral  "Ne" .

vec:insulationSpecificationFirstIdentificationColor
        rdf:type            owl:ObjectProperty;
        rdfs:comment        "Specifies the first identification color of the insulation.\n"@en;
        rdfs:domain         vec:InsulationSpecification;
        rdfs:label          "firstIdentificationColor"@en;
        rdfs:range          vec:Color;
        rdfs:subPropertyOf  vec:contains .

vec:grommetRoleGrommetSpecification
        rdf:type      owl:ObjectProperty;
        rdfs:comment  "References the GrommetSpecification that is instanced by this GrommetRole.\n"@en;
        rdfs:domain   vec:GrommetRole;
        rdfs:label    "grommetSpecification"@en;
        rdfs:range    vec:GrommetSpecification .

vec:ConnectionSpecification
        rdf:type         owl:Class;
        rdfs:comment     "A ConnectionSpecification is used to define electrological connectivity.\n"@en;
        rdfs:label       "ConnectionSpecification"@en;
        rdfs:subClassOf  vec:Specification .

vec:cavityPlugSpecificationHardness
        rdf:type            owl:ObjectProperty;
        rdfs:comment        "Specifies the hardness of the cavity plug.\n"@en;
        rdfs:domain         vec:CavityPlugSpecification;
        rdfs:label          "hardness"@en;
        rdfs:range          vec:NumericalValue;
        rdfs:subPropertyOf  vec:contains .

vec:CartesianVector3D
        rdf:type         owl:Class;
        rdfs:comment     "A Cartesian vector in three dimensional space.\n"@en;
        rdfs:label       "CartesianVector3D"@en;
        rdfs:subClassOf  vec:CartesianVector .

vec:UsageConstraintSpecification
        rdf:type         owl:Class;
        rdfs:comment     "Specification for the definition of usage constraints. The associated UsageContraints are restricting the possible usages of the associated PartVersions and PartUsages.\n"@en;
        rdfs:label       "UsageConstraintSpecification"@en;
        rdfs:subClassOf  vec:Specification .

vec:eEComponentRoleMountingSlot
        rdf:type      owl:ObjectProperty;
        rdfs:comment  "Specifies the slots to which into which the EE-component is mounted. \n"@en;
        rdfs:domain   vec:EEComponentRole;
        rdfs:label    "mountingSlot"@en;
        rdfs:range    vec:AbstractSlotReference .

vec:AntennaSpecification
        rdf:type         owl:Class;
        rdfs:comment     "Specification of the electrological aspects of an antenna.\n"@en;
        rdfs:label       "AntennaSpecification"@en;
        rdfs:subClassOf  vec:EEComponentSpecification .

vec:AbrasionResistanceClass
        rdf:type      owl:Class;
        rdfs:comment  "Allows the definition of an abrasion resistance class. The abrasion resistance class of a component is specified as a level of resistance against abrasion. The level is specified by the ClassKey. Valid keys are specified by the reference system.\nAttributes of the type AbrasionResistanceClass normally have the multiplicity [0..*]. This means that such an attribute can have AbrasionResistanceClass entries for different ReferenceSystems. It must not have multiple entries for the same reference system.\n"@en;
        rdfs:label    "AbrasionResistanceClass"@en .

vec:wireProtectionRoleGradient
        rdf:type            owl:ObjectProperty;
        rdfs:comment        "Specifies the gradient of the taping.\n"@en;
        rdfs:domain         vec:WireProtectionRole;
        rdfs:label          "gradient"@en;
        rdfs:range          vec:ValueWithUnit;
        rdfs:subPropertyOf  vec:contains .

vec:LanguageCode_Ca  rdf:type  vec:LanguageCode , owl:NamedIndividiual;
        vec:enumLiteral  "Ca" .

vec:EEComponentRole  rdf:type  owl:Class;
        rdfs:comment     "An EEComponentRole defines the instance specific properties and relationships of an EE-component.\n"@en;
        rdfs:label       "EEComponentRole"@en;
        rdfs:subClassOf  vec:Role .

vec:uSUnitUsUnitName  rdf:type  owl:ObjectProperty;
        rdfs:comment        "Specifies the name of the USUnit .\n"@en;
        rdfs:domain         vec:USUnit;
        rdfs:label          "usUnitName"@en;
        rdfs:range          vec:USUnitName;
        rdfs:subPropertyOf  vec:contains .

vec:PlacementType_OnPoint
        rdf:type         vec:PlacementType , owl:NamedIndividiual;
        rdfs:comment     " OnPoint refers to an OnPointPlacement .\n"@en;
        vec:enumLiteral  "OnPoint" .

[ rdf:type     owl:AllDisjointClasses;
  owl:members  ( vec:NumericalValueProperty vec:SimpleValueProperty vec:ValueRangeProperty vec:LocalizedStringProperty )
] .

vec:approvalStatus  rdf:type  owl:ObjectProperty;
        rdfs:comment        "The approval level concerning approval status. Predefined are the values: NotYetApproved, Approved and Withdrawn. KBLFRM-349\n"@en;
        rdfs:domain         vec:Approval;
        rdfs:label          "status"@en;
        rdfs:range          vec:StatusOfApproval;
        rdfs:subPropertyOf  vec:contains .

vec:WireReception  rdf:type  owl:Class;
        rdfs:comment     "A WireReception is the area of a terminal where the contacting with a (e.g. by crimping) takes place. This class represents such an area on the terminal. Its description is done with a WireReceptionSpecification, which is independent from the TerminalSpecification. This allows the reuse of the specification of similar WireReception on different terminals.\n"@en;
        rdfs:label       "WireReception"@en;
        rdfs:subClassOf  vec:ExtendableElement .

vec:UsageNodeType_Inliner
        rdf:type         vec:UsageNodeType , owl:NamedIndividiual;
        vec:enumLiteral  "Inliner" .

vec:generalTechnicalPartSpecificationTemperatureInformation
        rdf:type            owl:ObjectProperty;
        rdfs:comment        "Specifies valid temperatures for a part.\n"@en;
        rdfs:domain         vec:GeneralTechnicalPartSpecification;
        rdfs:label          "temperatureInformation"@en;
        rdfs:range          vec:TemperatureInformation;
        rdfs:subPropertyOf  vec:contains .

vec:robustnessPropertiesClass
        rdf:type      owl:DatatypeProperty;
        rdfs:comment  "Specifies the identifier of a robustness class defined by the robustness class reference system. Robustness classes are for example: oil, petrol, UV, water.\n"@en;
        rdfs:domain   vec:RobustnessProperties;
        rdfs:label    "class"@en;
        rdfs:range    xs:string .

vec:componentNodeComponentNodeType
        rdf:type      owl:DatatypeProperty;
        rdfs:comment  "Specifies the type of the ComponentNode.\n"@en;
        rdfs:domain   vec:ComponentNode;
        rdfs:label    "componentNodeType"@en;
        rdfs:range    xs:string .

vec:valueRangeMaximum
        rdf:type      owl:DatatypeProperty;
        rdfs:comment  "Upper bound of the value range.\n"@en;
        rdfs:domain   vec:ValueRange;
        rdfs:label    "maximum"@en;
        rdfs:range    xs:double .

vec:documentVersionLocation
        rdf:type      owl:DatatypeProperty;
        rdfs:comment  "The location specifies where a document can be found in a digital or physical data storage system.\n"@en;
        rdfs:domain   vec:DocumentVersion;
        rdfs:label    "location"@en;
        rdfs:range    xs:string .

vec:LanguageCode_Hu  rdf:type  vec:LanguageCode , owl:NamedIndividiual;
        vec:enumLiteral  "Hu" .

vec:creationResponsibleDesigner
        rdf:type            owl:ObjectProperty;
        rdfs:comment        "Specifies the person, which is the responsible designer for the ItemVersion at the point of creation.\n"@en;
        rdfs:domain         vec:Creation;
        rdfs:label          "responsibleDesigner"@en;
        rdfs:range          vec:Person;
        rdfs:subPropertyOf  vec:contains .

vec:wireElementSpecificationFillerSpecification
        rdf:type      owl:ObjectProperty;
        rdfs:comment  "If the WireElement is a filler then the specification of the filler is referenced here.\n"@en;
        rdfs:domain   vec:WireElementSpecification;
        rdfs:label    "fillerSpecification"@en;
        rdfs:range    vec:FillerSpecification .

vec:wireEndPositionOnWire
        rdf:type      owl:DatatypeProperty;
        rdfs:comment  "Specifies the position of the WireEnd on the wire. This must be a value between 0 and 1.\n"@en;
        rdfs:domain   vec:WireEnd;
        rdfs:label    "positionOnWire"@en;
        rdfs:range    xs:double .

vec:topologySpecificationTopologySegment
        rdf:type            owl:ObjectProperty;
        rdfs:comment        "Specifies the TopologySegments defined by the TopologySpecification.\n"@en;
        rdfs:domain         vec:TopologySpecification;
        rdfs:label          "topologySegment"@en;
        rdfs:range          vec:TopologySegment;
        rdfs:subPropertyOf  vec:contains .

vec:zoneDescription  rdf:type  owl:ObjectProperty;
        rdfs:comment        "Specifies additional, human readable information about the zone.\n"@en;
        rdfs:domain         vec:Zone;
        rdfs:label          "description"@en;
        rdfs:range          vec:AbstractLocalizedString;
        rdfs:subPropertyOf  vec:contains .

vec:segmentLengthLength
        rdf:type            owl:ObjectProperty;
        rdfs:comment        "Specifies the length of the TopologySegment.\n"@en;
        rdfs:domain         vec:SegmentLength;
        rdfs:label          "length"@en;
        rdfs:range          vec:NumericalValue;
        rdfs:subPropertyOf  vec:contains .

vec:transformation3DA32
        rdf:type     owl:DatatypeProperty;
        rdfs:domain  vec:Transformation3D;
        rdfs:label   "a32"@en;
        rdfs:range   xs:double .

vec:LanguageCode_Om  rdf:type  vec:LanguageCode , owl:NamedIndividiual;
        vec:enumLiteral  "Om" .

vec:LanguageCode_Fo  rdf:type  vec:LanguageCode , owl:NamedIndividiual;
        vec:enumLiteral  "Fo" .

vec:SiPrefix_Nano  rdf:type  vec:SiPrefix , owl:NamedIndividiual;
        vec:enumLiteral  "Nano" .

vec:fittingOutletNominalSize
        rdf:type      owl:DatatypeProperty;
        rdfs:comment  "Defines the nominal size of a tube. The nominal size is a name for the size of the tube that is somehow related to the inner diameter of the tube. However it is not the inner diameter (e.g. \"10.5\").\n"@en;
        rdfs:domain   vec:FittingOutlet;
        rdfs:label    "nominalSize"@en;
        rdfs:range    xs:string .

vec:itemVersionDescription
        rdf:type            owl:ObjectProperty;
        rdfs:comment        "Room for additional, human readable information about the ItemVersion. e.g. Buchsengeh├ñuse 26-polig\n"@en;
        rdfs:domain         vec:ItemVersion;
        rdfs:label          "description"@en;
        rdfs:range          vec:AbstractLocalizedString;
        rdfs:subPropertyOf  vec:contains .

vec:SlotGender_Unspecified
        rdf:type         vec:SlotGender , owl:NamedIndividiual;
        vec:enumLiteral  "Unspecified" .

vec:wireSpecificationWireElementSpecification
        rdf:type      owl:ObjectProperty;
        rdfs:comment  "References the WireElementSpecification that defines the properties of the top-most WireElement.\n"@en;
        rdfs:domain   vec:WireSpecification;
        rdfs:label    "wireElementSpecification"@en;
        rdfs:range    vec:WireElementSpecification .

vec:connectorHousingSpecificationSealingClass
        rdf:type            owl:ObjectProperty;
        rdfs:comment        "Specifies the sealing class of the slot.\n"@en;
        rdfs:domain         vec:ConnectorHousingSpecification;
        rdfs:label          "sealingClass"@en;
        rdfs:range          vec:SealingClass;
        rdfs:subPropertyOf  vec:contains .

vec:modularSlotReferenceUsedInserts
        rdf:type      owl:ObjectProperty;
        rdfs:comment  "References the inserts that are used in this ModularSlotReference. More than one insert is valid in the case variant dependent equipment of the slot.\n"@en;
        rdfs:domain   vec:ModularSlotReference;
        rdfs:label    "usedInserts"@en;
        rdfs:range    vec:ConnectorHousingRole .

vec:LanguageCode_El  rdf:type  vec:LanguageCode , owl:NamedIndividiual;
        vec:enumLiteral  "El" .

vec:LengthClassification_Adapted
        rdf:type         vec:LengthClassification , owl:NamedIndividiual;
        rdfs:comment     "An adapted length means that the value is not the exact value taken from the design tool, but is adapted in some way. Adapted values are normally created for example by rounding the designed values.\n"@en;
        vec:enumLiteral  "Adapted" .

vec:partRelationRelationType
        rdf:type            owl:ObjectProperty;
        rdfs:comment        "Specifies the type of the relation.\n"@en;
        rdfs:domain         vec:PartRelation;
        rdfs:label          "relationType"@en;
        rdfs:range          vec:PartRelationType;
        rdfs:subPropertyOf  vec:contains .

vec:LanguageCode_Mg  rdf:type  vec:LanguageCode , owl:NamedIndividiual;
        vec:enumLiteral  "Mg" .

vec:housingComponentPinComponent
        rdf:type            owl:ObjectProperty;
        rdfs:comment        "Specifies the PinComponents of HousingComponent. \n\n(see KBLFRM-300)\n"@en;
        rdfs:domain         vec:HousingComponent;
        rdfs:label          "pinComponent"@en;
        rdfs:range          vec:PinComponent;
        rdfs:subPropertyOf  vec:contains .

vec:wireElementIdentification
        rdf:type      owl:DatatypeProperty;
        rdfs:comment  "The identification of the WireElement. The identification is guaranteed to be unique within a wire and immutable. The identification is guaranteed to be the same for the same WireElement over different VEC documents.\n"@en;
        rdfs:domain   vec:WireElement;
        rdfs:label    "identification"@en;
        rdfs:range    xs:string .

vec:contactSystemSecondTerminal
        rdf:type      owl:ObjectProperty;
        rdfs:comment  "References the second terminal of the ContactSystem.\n"@en;
        rdfs:domain   vec:ContactSystem;
        rdfs:label    "secondTerminal"@en;
        rdfs:range    vec:PartVersion .

vec:topologyNodeMatchingPointId
        rdf:type      owl:DatatypeProperty;
        rdfs:comment  "Specifies an identification of a TopologyNode which be used for matching nodes that belong to different TopologySpecifications and that are actually representing the same node. Example: There are two TopologySpecifications, each specifying the topology of a certain zone of the car. If the zones are adjacent, it is possible that there are TopologyNodes where the two topologies are connected. These \"connection-nodes\" would carry the same matchingPointId.\n"@en;
        rdfs:domain   vec:TopologyNode;
        rdfs:label    "matchingPointId"@en;
        rdfs:range    xs:string .

vec:geometrySegment2DEndVector
        rdf:type            owl:ObjectProperty;
        rdfs:comment        "Specifies the end vector of the geometry segment. The end vector is a tangent to the segment at the end position.\n"@en;
        rdfs:domain         vec:GeometrySegment2D;
        rdfs:label          "endVector"@en;
        rdfs:range          vec:CartesianVector2D;
        rdfs:subPropertyOf  vec:contains .

vec:topologySegmentCrossSectionAreaInformation
        rdf:type            owl:ObjectProperty;
        rdfs:comment        "Specifies the different SegmentCrossSectionAreas of the TopologySegment. \n"@en;
        rdfs:domain         vec:TopologySegment;
        rdfs:label          "crossSectionAreaInformation"@en;
        rdfs:range          vec:SegmentCrossSectionArea;
        rdfs:subPropertyOf  vec:contains .

vec:fuseSpecificationIMax
        rdf:type            owl:ObjectProperty;
        rdfs:comment        "Specifies the maximum electric current tolerated by the fuse.\n"@en;
        rdfs:domain         vec:FuseSpecification;
        rdfs:label          "iMax"@en;
        rdfs:range          vec:NumericalValue;
        rdfs:subPropertyOf  vec:contains .

vec:WireElement  rdf:type  owl:Class;
        rdfs:comment     "A WireElement specifies a WireElementSpecification in the context of a WireSpecification . This is necessary to define a unique identification of a WireElementSpecification in the context of a WireSpecification. Additionally the WireElement serves as anchor for the instancing of a wire ( WireElementReference ).\n"@en;
        rdfs:label       "WireElement"@en;
        rdfs:subClassOf  vec:ExtendableElement .

vec:slotSealingType  rdf:type  owl:DatatypeProperty;
        rdfs:comment  "Specifies the type of the sealing of the slot. This should be an enumeration of values defined in a conformance class.\n"@en;
        rdfs:domain   vec:Slot;
        rdfs:label    "sealingType"@en;
        rdfs:range    xs:string .

vec:fileBasedInstructionDataFormat
        rdf:type      owl:DatatypeProperty;
        rdfs:comment  "The dataFormat specifies the format of the FileReference. This could be for example the mime-type of the external file.\n"@en;
        rdfs:domain   vec:FileBasedInstruction;
        rdfs:label    "dataFormat"@en;
        rdfs:range    xs:string .

vec:zoneIdentification
        rdf:type      owl:DatatypeProperty;
        rdfs:comment  "Specifies a unique identification of the Zone (normally the name). The identification is guaranteed to be unique within the TopologySpecification. Over all VEC-documents a Zone-instance can be trusted to be the same if the TopologySpecification-instance is the same (see TopologySpecification) and the identification of the Zone is the same.\n"@en;
        rdfs:domain   vec:Zone;
        rdfs:label    "identification"@en;
        rdfs:range    xs:string .

vec:documentVersionReferencedPart
        rdf:type      owl:ObjectProperty;
        rdfs:comment  "The association is an informative link which PartVersions are described by the DocumentVersion. \n"@en;
        rdfs:domain   vec:DocumentVersion;
        rdfs:label    "referencedPart"@en;
        rdfs:range    vec:PartVersion .

vec:geometryNode3DCartesianPoint
        rdf:type      owl:ObjectProperty;
        rdfs:comment  "References the CartesianPoint3D where the GeometryNode3D is located. \n"@en;
        rdfs:domain   vec:GeometryNode3D;
        rdfs:label    "cartesianPoint"@en;
        rdfs:range    vec:CartesianPoint3D .

vec:LanguageCode_Ka  rdf:type  vec:LanguageCode , owl:NamedIndividiual;
        vec:enumLiteral  "Ka" .

vec:slotReferenceCavityReference
        rdf:type            owl:ObjectProperty;
        rdfs:comment        "Specifies the CavityReferences used in the SlotReference.\n"@en;
        rdfs:domain         vec:SlotReference;
        rdfs:label          "cavityReference"@en;
        rdfs:range          vec:CavityReference;
        rdfs:subPropertyOf  vec:contains .

vec:housingComponentHousingSpecification
        rdf:type      owl:ObjectProperty;
        rdfs:comment  "References the ConnectorHousingSpecification that is describing the connector interface of the HousingComponent (e.g. Slots, Cavities, Design, Coding).\n"@en;
        rdfs:domain   vec:HousingComponent;
        rdfs:label    "housingSpecification"@en;
        rdfs:range    vec:ConnectorHousingSpecification .

vec:VariantGroupSpecification
        rdf:type         owl:Class;
        rdfs:comment     "Specification for the definition of variant groups.\n"@en;
        rdfs:label       "VariantGroupSpecification"@en;
        rdfs:subClassOf  vec:Specification .

vec:SealState  rdf:type  owl:Class;
        rdfs:comment     "Enumeration for the definition of the sealing state of the splice.\n"@en;
        rdfs:label       "SealState"@en;
        rdfs:subClassOf  vec:OpenEnumeration .

vec:CavitySealSpecification
        rdf:type         owl:Class;
        rdfs:comment     "Specification for the definition of cavity seals. A Cavity_seal is a water tight non-electrical object to fill a populated Cavity.\n"@en;
        rdfs:label       "CavitySealSpecification"@en;
        rdfs:subClassOf  vec:PartOrUsageRelatedSpecification .

vec:HistoryEntryType  rdf:type  owl:Class;
        rdfs:comment         "Enumeration for the definition of the type of relationship represented by an ItemHistoryEntry. (see KBLFRM-271)\n"@en;
        rdfs:label           "HistoryEntryType"@en;
        rdfs:subClassOf      vec:ClosedEnumeration;
        owl:equivalentClass  [ rdf:type   owl:Class;
                               owl:oneOf  ( vec:HistoryEntryType_Derivation vec:HistoryEntryType_Sequence )
                             ] .

vec:signalRecommendedInsulationSpecification
        rdf:type      owl:ObjectProperty;
        rdfs:comment  "Defines a recommended Specification for the insulation (e.g. the color) that implements this signal.\n"@en;
        rdfs:domain   vec:Signal;
        rdfs:label    "recommendedInsulationSpecification"@en;
        rdfs:range    vec:InsulationSpecification .

vec:terminalSpecificationWireReception
        rdf:type            owl:ObjectProperty;
        rdfs:comment        "Specifies the WireReceptions of the terminal described by the TerminalSpecification.\n"@en;
        rdfs:domain         vec:TerminalSpecification;
        rdfs:label          "wireReception"@en;
        rdfs:range          vec:WireReception;
        rdfs:subPropertyOf  vec:contains .

vec:StatusOfApproval_NotYetApproved
        rdf:type         vec:StatusOfApproval , owl:NamedIndividiual;
        vec:enumLiteral  "NotYetApproved" .

vec:occurrenceOrUsageViewItem3DOrientation
        rdf:type            owl:ObjectProperty;
        rdfs:comment        "Specifies the orientation of the view item.\n"@en;
        rdfs:domain         vec:OccurrenceOrUsageViewItem3D;
        rdfs:label          "orientation"@en;
        rdfs:range          vec:Transformation3D;
        rdfs:subPropertyOf  vec:contains .

[ rdf:type     owl:AllDisjointClasses;
  owl:members  ( vec:MultiCavityPlugSpecification )
] .

vec:LanguageCode_Or  rdf:type  vec:LanguageCode , owl:NamedIndividiual;
        vec:enumLiteral  "Or" .

vec:bSplineCurveDegree
        rdf:type      owl:DatatypeProperty;
        rdfs:comment  "The algebraic degree of the basis functions.\n"@en;
        rdfs:domain   vec:BSplineCurve;
        rdfs:label    "degree"@en;
        rdfs:range    xs:integer .

vec:NumericalValue  rdf:type  owl:Class;
        rdfs:comment     "A quantity expressed with a numerical value and a unit.\n"@en;
        rdfs:label       "NumericalValue"@en;
        rdfs:subClassOf  vec:ValueWithUnit .

vec:topologyNodeIdentification
        rdf:type      owl:DatatypeProperty;
        rdfs:comment  "Specifies a unique identification of the TopologyNode. The identification is guaranteed to be unique within the TopologySpecification. Over all VEC-documents a TopologyNode-instance can be trusted to be the same if the TopologySpecification-instance is the same (see TopologySpecification) and the identification of the TopologyNode is the same.\n"@en;
        rdfs:domain   vec:TopologyNode;
        rdfs:label    "identification"@en;
        rdfs:range    xs:string .

vec:SiPrefix_Zepto  rdf:type  vec:SiPrefix , owl:NamedIndividiual;
        vec:enumLiteral  "Zepto" .

vec:occurrenceOrUsageViewItem2DOrientation
        rdf:type            owl:ObjectProperty;
        rdfs:comment        "Specifies the orientation of the view item.\n"@en;
        rdfs:domain         vec:OccurrenceOrUsageViewItem2D;
        rdfs:label          "orientation"@en;
        rdfs:range          vec:Transformation2D;
        rdfs:subPropertyOf  vec:contains .

vec:wireTypeType  rdf:type  owl:DatatypeProperty;
        rdfs:comment  "Specifies the type of the wire (e.g. FLRY, NYFAZw). Valid values are defined by the wireTypeReferenceSystem.\n"@en;
        rdfs:domain   vec:WireType;
        rdfs:label    "type"@en;
        rdfs:range    xs:string .

vec:segmentConnectionPointPlacementPoint
        rdf:type      owl:ObjectProperty;
        rdfs:comment  "Specifies the PlacementPoint that represents this SegmentConnectionPoint in a PlaceableElementSpecification.\n"@en;
        rdfs:domain   vec:SegmentConnectionPoint;
        rdfs:label    "placementPoint"@en;
        rdfs:range    vec:PlacementPoint .

vec:LanguageCode_No  rdf:type  vec:LanguageCode , owl:NamedIndividiual;
        vec:enumLiteral  "No" .

vec:EdgeMountedFixingSpecification
        rdf:type         owl:Class;
        rdfs:comment     "Specification for fixings that are mounted onto an edge.\n"@en;
        rdfs:label       "EdgeMountedFixingSpecification"@en;
        rdfs:subClassOf  vec:FixingSpecification .

vec:connectionEndGender
        rdf:type      owl:DatatypeProperty;
        rdfs:comment  "Specifies if the ConnectionEnd is male or female. This may be e.g. important in case of an inliner.\n"@en;
        rdfs:domain   vec:ConnectionEnd;
        rdfs:label    "gender"@en;
        rdfs:range    xs:string .

vec:HousingComponent  rdf:type  owl:Class;
        rdfs:comment     "A HousingComponent describes the interface of an EEComponent with which it can be connected to another EEComponent or a harness. The characteristics of the interface can be described with a referenced ConnectorHousingSpecification. (see KBLFRM-300)\n"@en;
        rdfs:label       "HousingComponent"@en;
        rdfs:subClassOf  vec:ExtendableElement .

vec:PinCurrentType_BlockCurrent
        rdf:type         vec:PinCurrentType , owl:NamedIndividiual;
        vec:enumLiteral  "blockCurrent" .

vec:cavityMappingIdentificationB
        rdf:type      owl:DatatypeProperty;
        rdfs:comment  "The identification of the Cavity on side B\n"@en;
        rdfs:domain   vec:CavityMapping;
        rdfs:label    "identificationB"@en;
        rdfs:range    xs:string .

vec:usageNodeSubUsageNodes
        rdf:type            owl:ObjectProperty;
        rdfs:comment        ""@en;
        rdfs:domain         vec:UsageNode;
        rdfs:label          "subUsageNodes"@en;
        rdfs:range          vec:UsageNode;
        rdfs:subPropertyOf  vec:contains .

vec:tubeSpecificationInnerDiameter
        rdf:type            owl:ObjectProperty;
        rdfs:comment        "Defines the inner diameter of a tube. In the case of a shrinkable tube, it is the diameter of the tube in the unshrinked state.\n"@en;
        rdfs:domain         vec:TubeSpecification;
        rdfs:label          "innerDiameter"@en;
        rdfs:range          vec:NumericalValue;
        rdfs:subPropertyOf  vec:contains .

vec:IECPrefix_Pebi  rdf:type  vec:IECPrefix , owl:NamedIndividiual;
        vec:enumLiteral  "Pebi" .

vec:transformation3DA11
        rdf:type     owl:DatatypeProperty;
        rdfs:domain  vec:Transformation3D;
        rdfs:label   "a11"@en;
        rdfs:range   xs:double .

vec:ItemHistoryEntry  rdf:type  owl:Class;
        rdfs:comment     "An ItemHistroyEntry defines the direct relationship between ItemVersions in the terms of predecessor and successor. There are two possible types of relationships between ItemVersions, derivation and sequence. Derivation means for example for parts, that the successor version is a new part developed on the base of the predecessor version. Sequence means the successor version is an improvement of the predecessor version. By the combination of more than one ItemHistoryEntry a linear sequence of ItemVersions can be represented.\n"@en;
        rdfs:label       "ItemHistoryEntry"@en;
        rdfs:subClassOf  vec:ExtendableElement .

vec:LanguageCode_Ml  rdf:type  vec:LanguageCode , owl:NamedIndividiual;
        vec:enumLiteral  "Ml" .

vec:SiUnitName_Sievert
        rdf:type         vec:SiUnitName , owl:NamedIndividiual;
        vec:enumLiteral  "Sievert" .

vec:terminalReceptionIdentification
        rdf:type      owl:DatatypeProperty;
        rdfs:comment  "Specifies a unique identification of the TerminalReception. The identification is guaranteed to be unique within the TerminalSpecification (this might be for example a reception number).\n"@en;
        rdfs:domain   vec:TerminalReception;
        rdfs:label    "identification"@en;
        rdfs:range    xs:string .

vec:VariantConfiguration
        rdf:type         owl:Class;
        rdfs:comment     "A variant configuration defines a condition with which it is possible to express the inclusion or exclusion of ConfigurableElements in different variants of a product.\n"@en;
        rdfs:label       "VariantConfiguration"@en;
        rdfs:subClassOf  vec:ExtendableElement .

vec:LanguageCode_Ug  rdf:type  vec:LanguageCode , owl:NamedIndividiual;
        vec:enumLiteral  "Ug" .

vec:GeometrySegment3D
        rdf:type         owl:Class;
        rdfs:comment     "A GeometrySegment3D is the geometric representation of a TopologySegment in 3D-space.\n"@en;
        rdfs:label       "GeometrySegment3D"@en;
        rdfs:subClassOf  vec:GeometrySegment .

vec:materialDescription
        rdf:type            owl:ObjectProperty;
        rdfs:comment        "On optional human readable description of the material (e.g. the name).\n"@en;
        rdfs:domain         vec:Material;
        rdfs:label          "description"@en;
        rdfs:range          vec:LocalizedString;
        rdfs:subPropertyOf  vec:contains .

vec:itemVersionProcessingInstruction
        rdf:type            owl:ObjectProperty;
        rdfs:comment        "Processing instructions for the application of the part or the document.\n"@en;
        rdfs:domain         vec:ItemVersion;
        rdfs:label          "processingInstruction"@en;
        rdfs:range          vec:Instruction;
        rdfs:subPropertyOf  vec:contains .

vec:SiUnitName_Watt  rdf:type  vec:SiUnitName , owl:NamedIndividiual;
        vec:enumLiteral  "Watt" .

vec:conductorCurrentInformationEnvironmentTemperature
        rdf:type            owl:ObjectProperty;
        rdfs:comment        "The environment temperature for which this maximum current value is applicable.\n"@en;
        rdfs:domain         vec:ConductorCurrentInformation;
        rdfs:label          "environmentTemperature"@en;
        rdfs:range          vec:NumericalValue;
        rdfs:subPropertyOf  vec:contains .

vec:robustnessPropertiesClassKey
        rdf:type      owl:DatatypeProperty;
        rdfs:comment  "Specifies a key for the robustness level defined in the specified robustness class (e.g. A, B, C).\n"@en;
        rdfs:domain   vec:RobustnessProperties;
        rdfs:label    "classKey"@en;
        rdfs:range    xs:string .

[ rdf:type     owl:AllDisjointClasses;
  owl:members  ( vec:PartOccurrence vec:PartUsage )
] .

vec:CompositeUnit  rdf:type  owl:Class;
        rdfs:comment     "Defines a unit as a composition of other units. The composition is done by multiplying the different other units. By this way combined units like kg/m can be formed.\n"@en;
        rdfs:label       "CompositeUnit"@en;
        rdfs:subClassOf  vec:Unit .

vec:simpleValuePropertyValue
        rdf:type      owl:DatatypeProperty;
        rdfs:comment  "Defines the value of the CustomProperty.\n"@en;
        rdfs:domain   vec:SimpleValueProperty;
        rdfs:label    "value"@en;
        rdfs:range    xs:string .

vec:LanguageCode_Bh  rdf:type  vec:LanguageCode , owl:NamedIndividiual;
        vec:enumLiteral  "Bh" .

vec:LanguageCode_Sa  rdf:type  vec:LanguageCode , owl:NamedIndividiual;
        vec:enumLiteral  "Sa" .

vec:SiPrefix_Milli  rdf:type  vec:SiPrefix , owl:NamedIndividiual;
        vec:enumLiteral  "Milli" .

vec:USUnitName_League
        rdf:type         vec:USUnitName , owl:NamedIndividiual;
        vec:enumLiteral  "League" .

vec:ExternalMapping  rdf:type  owl:Class;
        rdfs:comment     "An ExternalMapping is used to relate an ExtendableElement in the VEC with an element located in an external data source. The element in the VEC┬áis referenced by the mappedElement , the external element is identified by the attribute externalReference.\n"@en;
        rdfs:label       "ExternalMapping"@en;
        rdfs:subClassOf  vec:ExtendableElement .

vec:buildingBlockSpecification2DGeometrySegment
        rdf:type            owl:ObjectProperty;
        rdfs:comment        "Specifies the GeometrySegment2Ds defined by the BuildingBlockSpecification2D.\n"@en;
        rdfs:domain         vec:BuildingBlockSpecification2D;
        rdfs:label          "geometrySegment"@en;
        rdfs:range          vec:GeometrySegment2D;
        rdfs:subPropertyOf  vec:contains .

vec:variantConfigurationConfigurationType
        rdf:type      owl:DatatypeProperty;
        rdfs:comment  "Allows the classification of a VariantConfiguration.\n(see KBLFRM-250, KBLFRM-314, KBLFRM-290)\n"@en;
        rdfs:domain   vec:VariantConfiguration;
        rdfs:label    "configurationType"@en;
        rdfs:range    xs:string .

vec:codingCoding  rdf:type  owl:DatatypeProperty;
        rdfs:comment  "Specifies the name of the coding.\n"@en;
        rdfs:domain   vec:Coding;
        rdfs:label    "coding"@en;
        rdfs:range    xs:string .

vec:PinCurrentType_InitCurrent
        rdf:type         vec:PinCurrentType , owl:NamedIndividiual;
        vec:enumLiteral  "initCurrent" .

vec:wireElementSpecificationImpedance
        rdf:type            owl:ObjectProperty;
        rdfs:comment        "Defines the impedance of this wireElement. Typically used for WireElements that have subWireElements e.g. twisted pair or coax wires.\n"@en;
        rdfs:domain         vec:WireElementSpecification;
        rdfs:label          "impedance"@en;
        rdfs:range          vec:NumericalValue;
        rdfs:subPropertyOf  vec:contains .

vec:CartesianPoint2D  rdf:type  owl:Class;
        rdfs:comment     "A CartesianPoint2D is a point that is defined by its coordinates in a rectangular two-dimensional Cartesian coordinate system.\n"@en;
        rdfs:label       "CartesianPoint2D"@en;
        rdfs:subClassOf  vec:ExtendableElement .

vec:Permission  rdf:type  owl:Class;
        rdfs:comment     "Describes an act of acceptance together with information about the responsible person, department and company who directly provoked the approval level and status as described in the referenced Approval-instance. (see KBLFRM-229)\n"@en;
        rdfs:label       "Permission"@en;
        rdfs:subClassOf  vec:ExtendableElement .

vec:wireReceptionSpecificationCoreCrossSectionArea
        rdf:type            owl:ObjectProperty;
        rdfs:comment        "Specifies a value range for valid cross section areas a core must have to fit to the wire reception.\n"@en;
        rdfs:domain         vec:WireReceptionSpecification;
        rdfs:label          "coreCrossSectionArea"@en;
        rdfs:range          vec:ValueRange;
        rdfs:subPropertyOf  vec:contains .

vec:ModuleFamily  rdf:type  owl:Class;
        rdfs:comment     "A ModuleFamily is a mechanism to group mutually exclusive modules. This could be for example something like \"audio equipment\", \"diesel engine\".\nIn other words, a module family groups different variants of the same basic feature. In a real car configuration only one member of the family can participate. For the example module family \"audio equipment\" the members may be named: \"Basic Audio Equipment\", \"Standard Audio Equipment\", \"Premium / High End Audio Equipment\".\n"@en;
        rdfs:label       "ModuleFamily"@en;
        rdfs:subClassOf  vec:ExtendableElement .

vec:LanguageCode_Fy  rdf:type  vec:LanguageCode , owl:NamedIndividiual;
        vec:enumLiteral  "Fy" .

vec:PartRelationType_Mandatory
        rdf:type         vec:PartRelationType , owl:NamedIndividiual;
        rdfs:comment     " Mandatory means that in a usage of a component all referenced acessoryParts must be used.\n"@en;
        vec:enumLiteral  "Mandatory" .

vec:TubeSpecification
        rdf:type         owl:Class;
        rdfs:comment     "Specifies tubes.\n"@en;
        rdfs:label       "TubeSpecification"@en;
        rdfs:subClassOf  vec:WireProtectionSpecification .

vec:vecContentCopyrightInformation
        rdf:type            owl:ObjectProperty;
        rdfs:comment        "Specifies the CopyrightInformation used in the VEC-file. \n"@en;
        rdfs:domain         vec:VecContent;
        rdfs:label          "copyrightInformation"@en;
        rdfs:range          vec:CopyrightInformation;
        rdfs:subPropertyOf  vec:contains .

vec:geometrySegment3DEndVector
        rdf:type            owl:ObjectProperty;
        rdfs:comment        "Specifies the end vector of the geometry segment. The end vector is a tangent to the segment at the end position.\n"@en;
        rdfs:domain         vec:GeometrySegment3D;
        rdfs:label          "endVector"@en;
        rdfs:range          vec:CartesianVector3D;
        rdfs:subPropertyOf  vec:contains .

vec:LanguageCode_Vo  rdf:type  vec:LanguageCode , owl:NamedIndividiual;
        vec:enumLiteral  "Vo" .

vec:dimensionDimensionAnchor
        rdf:type      owl:ObjectProperty;
        rdfs:comment  "References the location that is used as dimension point for the dimensioning (e.g. the entry point of a bundle into a connector housing).\nSee KBLFRM-329 and KBLFRM-391.\n"@en;
        rdfs:domain   vec:Dimension;
        rdfs:label    "dimensionAnchor"@en;
        rdfs:range    vec:DimensionAnchor .

vec:insulationSpecificationLabelIdentificationType
        rdf:type      owl:DatatypeProperty;
        rdfs:comment  "Specifies the type of a label printed on the insulation of the wire (e.g. alpha numerical, bar code).\n"@en;
        rdfs:domain   vec:InsulationSpecification;
        rdfs:label    "labelIdentificationType"@en;
        rdfs:range    xs:string .

vec:LanguageCode_Ln  rdf:type  vec:LanguageCode , owl:NamedIndividiual;
        vec:enumLiteral  "Ln" .

vec:MappingSpecification
        rdf:type         owl:Class;
        rdfs:comment     "Specification for the description of a PinMapping. A PinMapping allows the mapping between the Cavities of two independent ConnectorHousingSpecifications. This is for example needed to determine the Mating for an Inliner or for the Mating between an EE-Component and a ConnectorHousing. The PinMapping is a part master data.\n"@en;
        rdfs:label       "MappingSpecification"@en;
        rdfs:subClassOf  vec:Specification .

vec:cavitySealSpecificationWireReceptionType
        rdf:type      owl:DatatypeProperty;
        rdfs:comment  "Specifies the wireReceptionType to which the cavity seal fits. This should be an enumeration of values defined in a conformance class.\n"@en;
        rdfs:domain   vec:CavitySealSpecification;
        rdfs:label    "wireReceptionType"@en;
        rdfs:range    xs:string .

vec:cartesianDimensionWidth
        rdf:type      owl:DatatypeProperty;
        rdfs:comment  "Specifies the width of the object. The unit of this value is the baseUnit of containing BuildingBlockSpecification2D.\n"@en;
        rdfs:domain   vec:CartesianDimension;
        rdfs:label    "width"@en;
        rdfs:range    xs:double .

vec:USUnitName_Gill  rdf:type  vec:USUnitName , owl:NamedIndividiual;
        vec:enumLiteral  "Gill" .

vec:SiPrefix_Centi  rdf:type  vec:SiPrefix , owl:NamedIndividiual;
        vec:enumLiteral  "Centi" .

vec:LanguageCode_Kk  rdf:type  vec:LanguageCode , owl:NamedIndividiual;
        vec:enumLiteral  "Kk" .

vec:moduleListIdentification
        rdf:type      owl:DatatypeProperty;
        rdfs:comment  "Specifies a unique identification of the ModuleList. The identification is guaranteed to be unique within the ModuleListSpecification. Over all VEC-documents a ModuleList-instance can be trusted to be the same if the ModuleListSpecification-instance is the same and the identification of the ModuleList is the same.\n"@en;
        rdfs:domain   vec:ModuleList;
        rdfs:label    "identification"@en;
        rdfs:range    xs:string .

vec:SlotSpecification
        rdf:type         owl:Class;
        rdfs:comment     "Specification for the definition of slots.\n"@en;
        rdfs:label       "SlotSpecification"@en;
        rdfs:subClassOf  vec:Specification .

vec:TerminalType  rdf:type  owl:Class;
        rdfs:comment     "Defines the type of a terminal. The type is specified by a combination of a name for and an optional nominalSize.\n"@en;
        rdfs:label       "TerminalType"@en;
        rdfs:subClassOf  vec:ExtendableElement .

vec:USUnitName_Ounce  rdf:type  vec:USUnitName , owl:NamedIndividiual;
        vec:enumLiteral  "Ounce" .

vec:cavityCavitySpecification
        rdf:type      owl:ObjectProperty;
        rdfs:comment  "References the CavitySpecification that is satisfied by the cavity.\n"@en;
        rdfs:domain   vec:Cavity;
        rdfs:label    "cavitySpecification"@en;
        rdfs:range    vec:CavitySpecification .

vec:SiUnitName_Mole  rdf:type  vec:SiUnitName , owl:NamedIndividiual;
        vec:enumLiteral  "Mole" .

vec:buildingBlockSpecification2DPlacedElementViewItem
        rdf:type            owl:ObjectProperty;
        rdfs:comment        "Specifies the view items for OccurrenceOrUsages on a BuildingBlockSpecification2D. \n"@en;
        rdfs:domain         vec:BuildingBlockSpecification2D;
        rdfs:label          "placedElementViewItem"@en;
        rdfs:range          vec:OccurrenceOrUsageViewItem2D;
        rdfs:subPropertyOf  vec:contains .

vec:TopologySegmentWrapper
        rdf:type      owl:Class;
        rdfs:comment  "Container class for TopologySegment to participate in non-unique and/or ordered associations." .

vec:terminalSpecificationTerminalReception
        rdf:type            owl:ObjectProperty;
        rdfs:comment        "Specifies the TerminalReceptions of the terminal described by the TerminalSpecification.\n"@en;
        rdfs:domain         vec:TerminalSpecification;
        rdfs:label          "terminalReception"@en;
        rdfs:range          vec:TerminalReception;
        rdfs:subPropertyOf  vec:contains .

vec:BuildingBlockPositioning2D
        rdf:type         owl:Class;
        rdfs:comment     "Defines the position of a BuildingBlock2D on a HarnessDrawing.\n"@en;
        rdfs:label       "BuildingBlockPositioning2D"@en;
        rdfs:subClassOf  vec:ConfigurableElement .

vec:LanguageCode_Ie  rdf:type  vec:LanguageCode , owl:NamedIndividiual;
        vec:enumLiteral  "Ie" .

vec:USUnitName_Drachm
        rdf:type         vec:USUnitName , owl:NamedIndividiual;
        vec:enumLiteral  "Drachm" .

vec:GeometryNode3D  rdf:type  owl:Class;
        rdfs:comment     "A GeometryNode3D is the geometric representation of a TopologyNode in 3D-space.\n"@en;
        rdfs:label       "GeometryNode3D"@en;
        rdfs:subClassOf  vec:GeometryNode .

vec:slotSpecificationSecondaryLocking
        rdf:type      owl:DatatypeProperty;
        rdfs:comment  "Specifies whether the slot supports secondary locking.\n"@en;
        rdfs:domain   vec:SlotSpecification;
        rdfs:label    "secondaryLocking"@en;
        rdfs:range    xs:boolean .

vec:PartOrUsageRelatedSpecification
        rdf:type         owl:Class;
        rdfs:comment     "Base class for all specifications which are describing a PartVersion or a PartUsage . A PartOrUsageRelatedSpecification specifies a certain aspect of the described part or usage (e.g. general technical part information, connector housing aspects or wire aspects).\n"@en;
        rdfs:label       "PartOrUsageRelatedSpecification"@en;
        rdfs:subClassOf  vec:Specification .

vec:conformanceClassIdentification
        rdf:type      owl:DatatypeProperty;
        rdfs:comment  "Specifies the name of the conformance class.\n"@en;
        rdfs:domain   vec:ConformanceClass;
        rdfs:label    "identification"@en;
        rdfs:range    xs:string .

vec:dimensionDimensionValue
        rdf:type            owl:ObjectProperty;
        rdfs:comment        "Specifies the length of the dimension.\n"@en;
        rdfs:domain         vec:Dimension;
        rdfs:label          "dimensionValue"@en;
        rdfs:range          vec:NumericalValue;
        rdfs:subPropertyOf  vec:contains .

vec:ImperialUnitName_Yard
        rdf:type         vec:ImperialUnitName , owl:NamedIndividiual;
        vec:enumLiteral  "Yard" .

vec:creationCreator  rdf:type  owl:ObjectProperty;
        rdfs:comment        "Specifies the person who has created the Item.\n"@en;
        rdfs:domain         vec:Creation;
        rdfs:label          "creator"@en;
        rdfs:range          vec:Person;
        rdfs:subPropertyOf  vec:contains .

vec:segmentLocationOffset
        rdf:type            owl:ObjectProperty;
        rdfs:comment        "Specifies the offset / distance of the Location to the anchor of the location.\n"@en;
        rdfs:domain         vec:SegmentLocation;
        rdfs:label          "offset"@en;
        rdfs:range          vec:NumericalValue;
        rdfs:subPropertyOf  vec:contains .

vec:spliceTerminalRoleInsulationState
        rdf:type            owl:ObjectProperty;
        rdfs:comment        "Specifies the insulation state of the splice, in other words is electrically insulated or not.\n"@en;
        rdfs:domain         vec:SpliceTerminalRole;
        rdfs:label          "insulationState"@en;
        rdfs:range          vec:InsulationState;
        rdfs:subPropertyOf  vec:contains .

vec:cavityMountingReplacedPlug
        rdf:type      owl:ObjectProperty;
        rdfs:comment  "References the cavity plugs that are obsolete if the cavity mounting is realized. \n"@en;
        rdfs:domain   vec:CavityMounting;
        rdfs:label    "replacedPlug"@en;
        rdfs:range    vec:CavityPlugRole .

vec:CustomUnit  rdf:type  owl:Class;
        rdfs:comment     "A CustomUnit can be used to define \"FreeText\"-Units. Custom units must not be used for units that can be expressed by any of the other subclasses of Unit. Custom units are only allowed if a unit is needed that cannot be handled by any of the other classes.\n"@en;
        rdfs:label       "CustomUnit"@en;
        rdfs:subClassOf  vec:Unit .

vec:partUsagePartOrUsageRelatedSpecification
        rdf:type      owl:ObjectProperty;
        rdfs:comment  "References the PartOrUsageRelatedSpecification(s) that describe the PartOrUsageRelatedSpecification. \nKBLFRM-399\n"@en;
        rdfs:domain   vec:PartUsage;
        rdfs:label    "partOrUsageRelatedSpecification"@en;
        rdfs:range    vec:PartOrUsageRelatedSpecification .

vec:connectionNet  rdf:type  owl:ObjectProperty;
        rdfs:comment  "References the Net that is realized by the Connection.\n"@en;
        rdfs:domain   vec:Connection;
        rdfs:label    "net"@en;
        rdfs:range    vec:Net .

vec:PinCurrentType_StartStopCurrent
        rdf:type         vec:PinCurrentType , owl:NamedIndividiual;
        vec:enumLiteral  "startStopCurrent" .

vec:itemVersionAbbreviation
        rdf:type            owl:ObjectProperty;
        rdfs:comment        "Room for a short name of the Item. In case of a document the attribute is wanted to contain its title.\n"@en;
        rdfs:domain         vec:ItemVersion;
        rdfs:label          "abbreviation"@en;
        rdfs:range          vec:LocalizedString;
        rdfs:subPropertyOf  vec:contains .

vec:Dimension  rdf:type  owl:Class;
        rdfs:comment     "A Dimension defines a measurement for the distance between two Locations. An acceptable tolerance can be specified additionally. If the Locations are not located on adjacent topology-elements it is possible to specify a Path for the dimension along which the measurement must be taken.\n"@en;
        rdfs:label       "Dimension"@en;
        rdfs:subClassOf  vec:ConfigurableElement .

vec:temperatureInformationTemperatureRange
        rdf:type            owl:ObjectProperty;
        rdfs:comment        "Specifies the allowed temperature range for this type of temperature.\n"@en;
        rdfs:domain         vec:TemperatureInformation;
        rdfs:label          "temperatureRange"@en;
        rdfs:range          vec:ValueRange;
        rdfs:subPropertyOf  vec:contains .

vec:itemVersionApproval
        rdf:type            owl:ObjectProperty;
        rdfs:comment        "Specifies the approval information of the ItemVersion. \n"@en;
        rdfs:domain         vec:ItemVersion;
        rdfs:label          "approval"@en;
        rdfs:range          vec:Approval;
        rdfs:subPropertyOf  vec:contains .

vec:LanguageCode_Tn  rdf:type  vec:LanguageCode , owl:NamedIndividiual;
        vec:enumLiteral  "Tn" .

[ rdf:type     owl:AllDisjointClasses;
  owl:members  ( vec:MultiCavitySealSpecification )
] .

vec:moduleListModuleInList
        rdf:type      owl:ObjectProperty;
        rdfs:comment  "References the Modules that belong to the ModuleList. If any of the referenced Modules participates in a configuration the completition components participate, too.\n"@en;
        rdfs:domain   vec:ModuleList;
        rdfs:label    "moduleInList"@en;
        rdfs:range    vec:PartWithSubComponentsRole .

vec:wireProtectionRoleProtectionLength
        rdf:type            owl:ObjectProperty;
        rdfs:comment        "Specifies the length of the protection.\n"@en;
        rdfs:domain         vec:WireProtectionRole;
        rdfs:label          "protectionLength"@en;
        rdfs:range          vec:NumericalValue;
        rdfs:subPropertyOf  vec:contains .

vec:SheetOrChapter  rdf:type  owl:Class;
        rdfs:comment     "Documents can be structured into sheets or chapters. Since it is possible, that one document describes a couple of parts it is necessary to be able to specify which sheet or chapter contains the description of which part. (see KBLFRM-308)\n"@en;
        rdfs:label       "SheetOrChapter"@en;
        rdfs:subClassOf  vec:ExtendableElement .

vec:terminalReceptionReferenceIdentification
        rdf:type      owl:DatatypeProperty;
        rdfs:comment  "Specifies a unique identification of the TerminalReceptionReference . The identification is guaranteed to be unique within the TerminalRole (this might be for example a reception number).\n"@en;
        rdfs:domain   vec:TerminalReceptionReference;
        rdfs:label    "identification"@en;
        rdfs:range    xs:string .

vec:moduleFamilyModuleInFamily
        rdf:type      owl:ObjectProperty;
        rdfs:comment  "References the Modules that belong to the ModuleFamily. \n"@en;
        rdfs:domain   vec:ModuleFamily;
        rdfs:label    "moduleInFamily"@en;
        rdfs:range    vec:PartWithSubComponentsRole .

vec:LanguageCode_Br  rdf:type  vec:LanguageCode , owl:NamedIndividiual;
        vec:enumLiteral  "Br" .

vec:LanguageCode_Sk  rdf:type  vec:LanguageCode , owl:NamedIndividiual;
        vec:enumLiteral  "Sk" .

vec:usageNodeDescription
        rdf:type            owl:ObjectProperty;
        rdfs:comment        "Specifies additional, human readable information about the UsageNode .\n"@en;
        rdfs:domain         vec:UsageNode;
        rdfs:label          "description"@en;
        rdfs:range          vec:AbstractLocalizedString;
        rdfs:subPropertyOf  vec:contains .

vec:ConnectionGroup  rdf:type  owl:Class;
        rdfs:comment     "A ConnectionGroup references two or more Connections expressing that the physical realization of the referenced Connection shall be somehow grouped e.g. twisted. For complex structures a ConnectionGroup can specify subgroups.\n"@en;
        rdfs:label       "ConnectionGroup"@en;
        rdfs:subClassOf  vec:ConfigurableElement .

vec:pinComponentBehaviorCurrentInformation
        rdf:type            owl:ObjectProperty;
        rdfs:comment        "Specifies the current information of the PinComponent in this PinComponentBehavior . Since the current values of a pin can be defined for different types and times it is possible to define multiple PinCurrentInformations for a PinComponentBehavior .\n"@en;
        rdfs:domain         vec:PinComponentBehavior;
        rdfs:label          "currentInformation"@en;
        rdfs:range          vec:PinCurrentInformation;
        rdfs:subPropertyOf  vec:contains .

vec:conductorCurrentInformationMaxCurrent
        rdf:type            owl:ObjectProperty;
        rdfs:comment        "The maximum current value.\n"@en;
        rdfs:domain         vec:ConductorCurrentInformation;
        rdfs:label          "maxCurrent"@en;
        rdfs:range          vec:NumericalValue;
        rdfs:subPropertyOf  vec:contains .

vec:signalSignalTransmissionMediumType
        rdf:type            owl:ObjectProperty;
        rdfs:comment        "Specifies the type of the transmission medium for the signal.\n"@en;
        rdfs:domain         vec:Signal;
        rdfs:label          "signalTransmissionMediumType"@en;
        rdfs:range          vec:SignalTransmissionMediumType;
        rdfs:subPropertyOf  vec:contains .

vec:slotLayoutGridX  rdf:type  owl:ObjectProperty;
        rdfs:comment        "The horizontal distance between the center points of two cavities.\n"@en;
        rdfs:domain         vec:SlotLayout;
        rdfs:label          "gridX"@en;
        rdfs:range          vec:NumericalValue;
        rdfs:subPropertyOf  vec:contains .

vec:compatibilityStatementCavityPlugSpecification
        rdf:type      owl:ObjectProperty;
        rdfs:comment  "References the CavityPlugSpecifications for which the compatibility statement is stated.\n"@en;
        rdfs:domain   vec:CompatibilityStatement;
        rdfs:label    "cavityPlugSpecification"@en;
        rdfs:range    vec:CavityPlugSpecification .

vec:SiPrefix_Tera  rdf:type  vec:SiPrefix , owl:NamedIndividiual;
        vec:enumLiteral  "Tera" .

vec:PinApplianceType_ShortTerm
        rdf:type         vec:PinApplianceType , owl:NamedIndividiual;
        vec:enumLiteral  "shortTerm" .

vec:cableLeadThroughPlacementPoint
        rdf:type      owl:ObjectProperty;
        rdfs:comment  "Specifies the PlacementPoint that represents this CableLeadThrough in a PlaceableElementSpecification.\n"@en;
        rdfs:domain   vec:CableLeadThrough;
        rdfs:label    "placementPoint"@en;
        rdfs:range    vec:PlacementPoint .

vec:itemHistoryEntryPredecessorVersion
        rdf:type      owl:ObjectProperty;
        rdfs:comment  "References the ItemVersion that is the predecessor in the ItemHistoryEntry. \n"@en;
        rdfs:domain   vec:ItemHistoryEntry;
        rdfs:label    "predecessorVersion"@en;
        rdfs:range    vec:ItemVersion .

vec:NodeType_EndNode  rdf:type  vec:NodeType , owl:NamedIndividiual;
        rdfs:comment     "Electrical components are normally placed on an EndNode.\n"@en;
        vec:enumLiteral  "EndNode" .

vec:PinTimingType_StartStopTime
        rdf:type         vec:PinTimingType , owl:NamedIndividiual;
        vec:enumLiteral  "startStopTime" .

vec:LanguageCode_Gd  rdf:type  vec:LanguageCode , owl:NamedIndividiual;
        vec:enumLiteral  "Gd" .

vec:LocalizedStringProperty
        rdf:type         owl:Class;
        rdfs:label       "LocalizedStringProperty"@en;
        rdfs:subClassOf  vec:CustomProperty .

vec:abstractSlotReferenceIdentification
        rdf:type      owl:DatatypeProperty;
        rdfs:comment  "Specifies a unique identification of the SlotReference. The identification is guaranteed to be unique within the ConnectorHousingRole. The cavity & slot number is defined by the associated cavity and slot.\n"@en;
        rdfs:domain   vec:AbstractSlotReference;
        rdfs:label    "identification"@en;
        rdfs:range    xs:string .

vec:harnessGeometrySpecification3DType
        rdf:type            owl:ObjectProperty;
        rdfs:comment        "Specifies the type of the harness geometry.\n"@en;
        rdfs:domain         vec:HarnessGeometrySpecification3D;
        rdfs:label          "type"@en;
        rdfs:range          vec:GeometryType;
        rdfs:subPropertyOf  vec:contains .

vec:CompositionSpecification
        rdf:type         owl:Class;
        rdfs:comment     "The CompositionSpecificiation is used to define a set of occurrences required to describe unambiguously the design of a composite part. This does not have to be necessarily the same occurrences which are building the bill of material. Example: A company might want to regard an antenna cable as one part out of a bill of material perspective. However, at the same time it may be useful for the company to be able to describe the contacting of the antenna cable within the VEC. (see also PartStructureSpecification)\n"@en;
        rdfs:label       "CompositionSpecification"@en;
        rdfs:subClassOf  vec:Specification .

vec:OpenEnumeration  rdf:type  owl:Class;
        rdfs:comment     "Classes in the model where some value can be enumerated, but not all values are known (Open)."@en;
        rdfs:label       "OpenEnumeration"@en;
        rdfs:subClassOf  vec:Enumeration .

vec:LanguageCode_Fa  rdf:type  vec:LanguageCode , owl:NamedIndividiual;
        vec:enumLiteral  "Fa" .

vec:stripeSpecificationWidth
        rdf:type            owl:ObjectProperty;
        rdfs:comment        "Specifies the width of the stripe.\n"@en;
        rdfs:domain         vec:StripeSpecification;
        rdfs:label          "width"@en;
        rdfs:range          vec:NumericalValue;
        rdfs:subPropertyOf  vec:contains .

vec:pinComponentBehaviorPinType
        rdf:type            owl:ObjectProperty;
        rdfs:comment        "Specifies the PinType of the PinComponent .\n"@en;
        rdfs:domain         vec:PinComponentBehavior;
        rdfs:label          "pinType"@en;
        rdfs:range          vec:PinType;
        rdfs:subPropertyOf  vec:contains .

vec:variantGroupGroupType
        rdf:type      owl:DatatypeProperty;
        rdfs:comment  "Allows the classification of a VariantGroups into different types. For example: - composition (e.g. winter package) - choice (e.g. right hand / left hand driving)\n"@en;
        rdfs:domain   vec:VariantGroup;
        rdfs:label    "groupType"@en;
        rdfs:range    xs:string .

vec:HousingComponentReference
        rdf:type      owl:Class;
        rdfs:comment  "A HousingComponentReference represents the usage of a HousingComponent in the context of a PartUsage or PartOccurrence. (KBLFRM-401)\n"@en;
        rdfs:label    "HousingComponentReference"@en .

vec:PrimaryPartType_RingTerminal
        rdf:type         vec:PrimaryPartType , owl:NamedIndividiual;
        vec:enumLiteral  "RingTerminal" .

vec:UsageConstraintType
        rdf:type             owl:Class;
        rdfs:comment         "Enumeration for the definition of the type of a UsageContstraint. Valid values are: allow, deny.\n"@en;
        rdfs:label           "UsageConstraintType"@en;
        rdfs:subClassOf      vec:ClosedEnumeration;
        owl:equivalentClass  [ rdf:type   owl:Class;
                               owl:oneOf  ( vec:UsageConstraintType_Allow vec:UsageConstraintType_Deny )
                             ] .

vec:cableDuctOutletPlacementPoint
        rdf:type      owl:ObjectProperty;
        rdfs:comment  "Specifies the PlacementPoint that represents this CableDuctOutlet in a PlaceableElementSpecification.\n"@en;
        rdfs:domain   vec:CableDuctOutlet;
        rdfs:label    "placementPoint"@en;
        rdfs:range    vec:PlacementPoint .

[ rdf:type     owl:AllDisjointClasses;
  owl:members  ( vec:GeometrySegment2D vec:GeometrySegment3D )
] .

vec:pinComponentBehaviorDescription
        rdf:type            owl:ObjectProperty;
        rdfs:comment        "Specifies additional, human readable information about the PinComponentBehaviour .\n"@en;
        rdfs:domain         vec:PinComponentBehavior;
        rdfs:label          "description"@en;
        rdfs:range          vec:AbstractLocalizedString;
        rdfs:subPropertyOf  vec:contains .

vec:locationMatchingId
        rdf:type      owl:DatatypeProperty;
        rdfs:comment  "Specifies an identification for matching the location with a reference point of component (e.g. a cable channel).\n"@en;
        rdfs:domain   vec:Location;
        rdfs:label    "matchingId"@en;
        rdfs:range    xs:string .

vec:AnchorType_FromStartNode
        rdf:type         vec:AnchorType , owl:NamedIndividiual;
        rdfs:comment     "The offset of the location is measured from the startNode of the TopologySegment.\n"@en;
        vec:enumLiteral  "FromStartNode" .

vec:ImperialUnit  rdf:type  owl:Class;
        rdfs:comment     "The ImperialUnit class can define quantities in the terms of the Imperial-Unit-System by specifying the corresponding Imperial unit name.\n"@en;
        rdfs:label       "ImperialUnit"@en;
        rdfs:subClassOf  vec:Unit .

vec:housingComponentIdentification
        rdf:type      owl:DatatypeProperty;
        rdfs:comment  "Identification of the HousingComponent, which must be distinct for all HousingComponents of an EEComponent.\n"@en;
        rdfs:domain   vec:HousingComponent;
        rdfs:label    "identification"@en;
        rdfs:range    xs:string .

vec:SiPrefix_Zetta  rdf:type  vec:SiPrefix , owl:NamedIndividiual;
        vec:enumLiteral  "Zetta" .

vec:LanguageCode_Ts  rdf:type  vec:LanguageCode , owl:NamedIndividiual;
        vec:enumLiteral  "Ts" .

vec:orderedIndex  rdf:type  owl:DataProperty;
        rdfs:comment  "Defines the order of Ordered elements. Lower indices are further forward in a list. 0 is the lowest index, i.e. the first element."@en;
        rdfs:domain   vec:Ordered;
        rdfs:range    xs:nonNegativeInteger .

vec:abstractSlotCoding
        rdf:type            owl:ObjectProperty;
        rdfs:comment        "Defines coding of the slot that is satisfied by the Slot.\n"@en;
        rdfs:domain         vec:AbstractSlot;
        rdfs:label          "coding"@en;
        rdfs:range          vec:Coding;
        rdfs:subPropertyOf  vec:contains .

vec:SiUnitName_Siemens
        rdf:type         vec:SiUnitName , owl:NamedIndividiual;
        vec:enumLiteral  "Siemens" .

vec:signalSignalInformationType
        rdf:type            owl:ObjectProperty;
        rdfs:comment        "Specifies the information type of the signal.\n"@en;
        rdfs:domain         vec:Signal;
        rdfs:label          "signalInformationType"@en;
        rdfs:range          vec:SignalInformationType;
        rdfs:subPropertyOf  vec:contains .

vec:LanguageCode_Ku  rdf:type  vec:LanguageCode , owl:NamedIndividiual;
        vec:enumLiteral  "Ku" .

vec:customUnitIdentification
        rdf:type      owl:DatatypeProperty;
        rdfs:comment  "A unique identification of the custom unit.\n"@en;
        rdfs:domain   vec:CustomUnit;
        rdfs:label    "identification"@en;
        rdfs:range    xs:string .

vec:FixingRole  rdf:type  owl:Class;
        rdfs:comment     "A FixingRole defines the instance specific properties and relationships of a fixing.\n"@en;
        rdfs:label       "FixingRole"@en;
        rdfs:subClassOf  vec:Role .

vec:connectionGroupIdentification
        rdf:type      owl:DatatypeProperty;
        rdfs:comment  "Specifies a unique identification of the ConnectionGroup. The identification is guaranteed to be unique within the ConnectionSpecification.\n"@en;
        rdfs:domain   vec:ConnectionGroup;
        rdfs:label    "identification"@en;
        rdfs:range    xs:string .

vec:PinVoltageType_InitVoltage
        rdf:type         vec:PinVoltageType , owl:NamedIndividiual;
        vec:enumLiteral  "initVoltage" .

vec:PinType_Optical  rdf:type  vec:PinType , owl:NamedIndividiual;
        vec:enumLiteral  "optical" .

vec:occurrenceOrUsageRealizedUsageNode
        rdf:type      owl:ObjectProperty;
        rdfs:comment  "References the UsageNode that is realized by this OccurrenceOrUsage .\n"@en;
        rdfs:domain   vec:OccurrenceOrUsage;
        rdfs:label    "realizedUsageNode"@en;
        rdfs:range    vec:UsageNode .

vec:colorDescription  rdf:type  owl:ObjectProperty;
        rdfs:comment        "On optional human readable description of the color (e.g. the name).\n"@en;
        rdfs:domain         vec:Color;
        rdfs:label          "description"@en;
        rdfs:range          vec:LocalizedString;
        rdfs:subPropertyOf  vec:contains .

vec:placeableElementRoleMeasurementPointReference
        rdf:type            owl:ObjectProperty;
        rdfs:comment        ""@en;
        rdfs:domain         vec:PlaceableElementRole;
        rdfs:label          "measurementPointReference"@en;
        rdfs:range          vec:MeasurementPointReference;
        rdfs:subPropertyOf  vec:contains .

vec:wireMountingDetailReferencedWireEnd
        rdf:type      owl:ObjectProperty;
        rdfs:comment  "References the WireEnds that are mounted to referenced WireReception. A cardinality of more than one is allowed in order support parallel connectors, where multiple wire ends are placed on one side of the connector (one wire reception) and the other wire ends are placed on the other side of the connector (the other wire reception).\n"@en;
        rdfs:domain   vec:WireMountingDetail;
        rdfs:label    "referencedWireEnd"@en;
        rdfs:range    vec:WireEnd .

vec:multiCavitySealSpecificationAssignment
        rdf:type            owl:ObjectProperty;
        rdfs:comment        "References the OpenCavitiesAssignments that are valid for this MultiCavitySeal . One individual OpenCavitiesAssignment is used for each connector housing that matches witch this MultiCavitySeal.\n"@en;
        rdfs:domain         vec:MultiCavitySealSpecification;
        rdfs:label          "assignment"@en;
        rdfs:range          vec:OpenCavitiesAssignment;
        rdfs:subPropertyOf  vec:contains .

vec:LanguageCode_Rm  rdf:type  vec:LanguageCode , owl:NamedIndividiual;
        vec:enumLiteral  "Rm" .

vec:TypeOfPermission_Seen
        rdf:type         vec:TypeOfPermission , owl:NamedIndividiual;
        vec:enumLiteral  "Seen" .

vec:ringTerminalSpecificationThickness
        rdf:type            owl:ObjectProperty;
        rdfs:comment        "Specifies the thickness of the contact surface of the ring terminal.\n"@en;
        rdfs:domain         vec:RingTerminalSpecification;
        rdfs:label          "thickness"@en;
        rdfs:range          vec:NumericalValue;
        rdfs:subPropertyOf  vec:contains .

vec:cavityAvailable  rdf:type  owl:DatatypeProperty;
        rdfs:comment  "Defines whether the cavity is available for contacting. If the cavity is not available, it means that it is completely closed.\n"@en;
        rdfs:domain   vec:Cavity;
        rdfs:label    "available"@en;
        rdfs:range    xs:boolean .

vec:LanguageCode_Zh  rdf:type  vec:LanguageCode , owl:NamedIndividiual;
        rdfs:comment     "Chinese\n"@en;
        vec:enumLiteral  "Zh" .

vec:fillerSpecificationMaterial
        rdf:type            owl:ObjectProperty;
        rdfs:comment        "Specifies the material of the filler.\n"@en;
        rdfs:domain         vec:FillerSpecification;
        rdfs:label          "material"@en;
        rdfs:range          vec:Material;
        rdfs:subPropertyOf  vec:contains .

vec:wireReceptionSpecificationWireReceptionType
        rdf:type      owl:DatatypeProperty;
        rdfs:comment  "Specifies the type of the wire reception. This should be an enumeration of values defined in a conformance class.\n"@en;
        rdfs:domain   vec:WireReceptionSpecification;
        rdfs:label    "wireReceptionType"@en;
        rdfs:range    xs:string .

vec:wireElementReferenceReferencedWireElement
        rdf:type      owl:ObjectProperty;
        rdfs:comment  "References the WireElement that is represented by the WireElementReference.\n"@en;
        rdfs:domain   vec:WireElementReference;
        rdfs:label    "referencedWireElement"@en;
        rdfs:range    vec:WireElement .

vec:SlotLayout  rdf:type  owl:Class;
        rdfs:comment  "For regularly laid out slots the slot layout describes the positions of the cavities\n"@en;
        rdfs:label    "SlotLayout"@en .

vec:ImperialUnitName_Inch
        rdf:type         vec:ImperialUnitName , owl:NamedIndividiual;
        vec:enumLiteral  "Inch" .

vec:topologySegmentForm
        rdf:type            owl:ObjectProperty;
        rdfs:comment        "Specifies the form of the TopologySegment. A TopologySegment can either be circular or noncircular.\n"@en;
        rdfs:domain         vec:TopologySegment;
        rdfs:label          "form"@en;
        rdfs:range          vec:SegmentForm;
        rdfs:subPropertyOf  vec:contains .

vec:netDescription  rdf:type  owl:ObjectProperty;
        rdfs:comment        "Room for additional, human readable information about the Net.\n"@en;
        rdfs:domain         vec:Net;
        rdfs:label          "description"@en;
        rdfs:range          vec:AbstractLocalizedString;
        rdfs:subPropertyOf  vec:contains .

vec:Signal  rdf:type     owl:Class;
        rdfs:comment     "Specifies a signal.\n"@en;
        rdfs:label       "Signal"@en;
        rdfs:subClassOf  vec:ExtendableElement .

vec:cartesianVector3DX
        rdf:type      owl:DatatypeProperty;
        rdfs:comment  "Specifies the x-coordinate in 3D space.\n"@en;
        rdfs:domain   vec:CartesianVector3D;
        rdfs:label    "x"@en;
        rdfs:range    xs:double .

[ rdf:type     owl:AllDisjointClasses;
  owl:members  ( vec:LocalizedString vec:LocalizedTypedString )
] .

vec:variantCodeCodeType
        rdf:type      owl:DatatypeProperty;
        rdfs:comment  "Allows the classification of a VariantCodes (e.g. Base-Option, Extra-Option, ...).\n"@en;
        rdfs:domain   vec:VariantCode;
        rdfs:label    "codeType"@en;
        rdfs:range    xs:string .

vec:NetworkPort  rdf:type  owl:Class;
        rdfs:comment     "NetworkPort is the source or the receiver of a signal transmitted by a Net.\n"@en;
        rdfs:label       "NetworkPort"@en;
        rdfs:subClassOf  vec:ConfigurableElement .

vec:SiUnitName_Katal  rdf:type  vec:SiUnitName , owl:NamedIndividiual;
        vec:enumLiteral  "Katal" .

vec:colorReferenceSystem
        rdf:type      owl:DatatypeProperty;
        rdfs:comment  "The identification of the color reference system, which is defining possible values and the semantic of color keys. (see KBLFRM-315)\n"@en;
        rdfs:domain   vec:Color;
        rdfs:label    "referenceSystem"@en;
        rdfs:range    xs:string .

vec:measurementPointReferenceMeasurementPoint
        rdf:type      owl:ObjectProperty;
        rdfs:comment  "References the MeasurementPoint that is instanced by this MeasurementPointReference.\n"@en;
        rdfs:domain   vec:MeasurementPointReference;
        rdfs:label    "measurementPoint"@en;
        rdfs:range    vec:MeasurementPoint .

vec:wireReceptionReferenceWireReception
        rdf:type      owl:ObjectProperty;
        rdfs:comment  "References the WireReception that is instanced by this WireReceptionReference.\n"@en;
        rdfs:domain   vec:WireReceptionReference;
        rdfs:label    "wireReception"@en;
        rdfs:range    vec:WireReception .

vec:EEComponentSpecification
        rdf:type         owl:Class;
        rdfs:comment     "Base-class for the specification of electrological components, which are connected to the harness. Usually electrological components are not part of the harness e.g. a fuses, a switch or a control device. All EEComponents can have one or more HousingComponents which are possible interfaces for the connection to a harness.\n"@en;
        rdfs:label       "EEComponentSpecification"@en;
        rdfs:subClassOf  vec:PartOrUsageRelatedSpecification .

vec:wireGroupingWireGroupSpecification
        rdf:type      owl:ObjectProperty;
        rdfs:comment  "References the WireGroupSpecification that applies to the WireGrouping. \n"@en;
        rdfs:domain   vec:WireGrouping;
        rdfs:label    "wireGroupSpecification"@en;
        rdfs:range    vec:WireGroupSpecification .

vec:sealingClassClass
        rdf:type      owl:DatatypeProperty;
        rdfs:comment  "Specifies the identifier of a sealing class defined by the sealing class reference system.\n"@en;
        rdfs:domain   vec:SealingClass;
        rdfs:label    "class"@en;
        rdfs:range    xs:string .

vec:CableDuctSpecification
        rdf:type         owl:Class;
        rdfs:comment     "Specification for cable ducts. A cable duct can have one or more outlets.\n"@en;
        rdfs:label       "CableDuctSpecification"@en;
        rdfs:subClassOf  vec:PartOrUsageRelatedSpecification .

vec:LanguageCode_Na  rdf:type  vec:LanguageCode , owl:NamedIndividiual;
        vec:enumLiteral  "Na" .

vec:ImperialUnitName_Ton
        rdf:type         vec:ImperialUnitName , owl:NamedIndividiual;
        vec:enumLiteral  "Ton" .

vec:wireGroupSpecificationLengthOfTwist
        rdf:type            owl:ObjectProperty;
        rdfs:comment        "Specifies the length of twist if the wire group is representing a twisted pair.\n"@en;
        rdfs:domain         vec:WireGroupSpecification;
        rdfs:label          "lengthOfTwist"@en;
        rdfs:range          vec:NumericalValue;
        rdfs:subPropertyOf  vec:contains .

vec:PinVoltageType_BlockVoltage
        rdf:type         vec:PinVoltageType , owl:NamedIndividiual;
        vec:enumLiteral  "blockVoltage" .

vec:Cavity  rdf:type     owl:Class;
        rdfs:comment     "A cavity is a defined space in a connector housing for location of an electrical terminal or cavity plug or seal. A cavity may also be empty.\n"@en;
        rdfs:label       "Cavity"@en;
        rdfs:subClassOf  vec:ExtendableElement .

vec:documentBasedInstructionReferencedSheetOrChapter
        rdf:type      owl:ObjectProperty;
        rdfs:comment  "References the SheetOrChapter that is used as an Instruction.\n"@en;
        rdfs:domain   vec:DocumentBasedInstruction;
        rdfs:label    "referencedSheetOrChapter"@en;
        rdfs:range    vec:SheetOrChapter .

vec:PinVoltageType_MaxVoltage
        rdf:type         vec:PinVoltageType , owl:NamedIndividiual;
        vec:enumLiteral  "maxVoltage" .

vec:cavitySealSpecificationSealingClass
        rdf:type            owl:ObjectProperty;
        rdfs:comment        "Specifies the sealing class of the cavity seal.\n"@en;
        rdfs:domain         vec:CavitySealSpecification;
        rdfs:label          "sealingClass"@en;
        rdfs:range          vec:SealingClass;
        rdfs:subPropertyOf  vec:contains .

vec:externalMappingSpecificationMappings
        rdf:type            owl:ObjectProperty;
        rdfs:comment        "Specifies the mappings of individual element.\n"@en;
        rdfs:domain         vec:ExternalMappingSpecification;
        rdfs:label          "mappings"@en;
        rdfs:range          vec:ExternalMapping;
        rdfs:subPropertyOf  vec:contains .

vec:networkNodeDescription
        rdf:type            owl:ObjectProperty;
        rdfs:comment        "Room for additional, human readable information about the NetworkNode.\n"@en;
        rdfs:domain         vec:NetworkNode;
        rdfs:label          "description"@en;
        rdfs:range          vec:AbstractLocalizedString;
        rdfs:subPropertyOf  vec:contains .

vec:terminalTypeNominalSize
        rdf:type      owl:DatatypeProperty;
        rdfs:comment  "Specifies the nominal size of terminals that fit into the cavity. (e.g. 2x4).\n"@en;
        rdfs:domain   vec:TerminalType;
        rdfs:label    "nominalSize"@en;
        rdfs:range    xs:string .

vec:pinComponentBehaviorApplianceType
        rdf:type            owl:ObjectProperty;
        rdfs:comment        "Specifies the PinApplianceType of the PinComponent .\n"@en;
        rdfs:domain         vec:PinComponentBehavior;
        rdfs:label          "applianceType"@en;
        rdfs:range          vec:PinApplianceType;
        rdfs:subPropertyOf  vec:contains .

vec:PartRelation  rdf:type  owl:Class;
        rdfs:comment  "A PartRelation can define Accessories to a specific Part. For example a fixing can need an additional cable tie. Accessories can either be mandatory, optional or one out of a group. (see KBLFRM-311)\n"@en;
        rdfs:label    "PartRelation"@en .

vec:LanguageCode_Su  rdf:type  vec:LanguageCode , owl:NamedIndividiual;
        vec:enumLiteral  "Su" .

vec:TapingDirection_Right
        rdf:type         vec:TapingDirection , owl:NamedIndividiual;
        vec:enumLiteral  "Right" .

vec:SiUnitName_Hertz  rdf:type  vec:SiUnitName , owl:NamedIndividiual;
        vec:enumLiteral  "Hertz" .

vec:ValueRange  rdf:type  owl:Class;
        rdfs:comment     "A pair of numerical values representing a value range.\n"@en;
        rdfs:label       "ValueRange"@en;
        rdfs:subClassOf  vec:ValueWithUnit .

vec:LanguageCode_Jw  rdf:type  vec:LanguageCode , owl:NamedIndividiual;
        vec:enumLiteral  "Jw" .

vec:projectCarClassificationLevel2
        rdf:type      owl:DatatypeProperty;
        rdfs:comment  "Provides a classification according to \"CC8 Recommended Practices Specification and Configuration, Product Structures\". Car classification is the identification of a set of similar cars to be offered to the market. Level 2 stands for \"Technical information / platform\" and reflects the level of a product class in a BoM system which represents a main technical product base (e.g. project, platform, engineering series etc.). In some cases this level carries a complete BoM (\"Maximum BoM\") for a project, platform, engineering series etc. This level is in some cases called technical documentation.\n"@en;
        rdfs:domain   vec:Project;
        rdfs:label    "carClassificationLevel2"@en;
        rdfs:range    xs:string .

vec:AliasIdentification
        rdf:type      owl:Class;
        rdfs:comment  "Class for the definition of alias identifications. Alias identifications are additional identifications for VEC-elements, which are valid in a certain scope (e.g. PPS-ID's).\n"@en;
        rdfs:label    "AliasIdentification"@en .

vec:placementPointReferenceIdentification
        rdf:type      owl:DatatypeProperty;
        rdfs:comment  "Specifies a unique identification of the PlacementPointReference. The identification is guaranteed to be unique within the containing PlaceableElementRole.\n"@en;
        rdfs:domain   vec:PlacementPointReference;
        rdfs:label    "identification"@en;
        rdfs:range    xs:string .

vec:LanguageCode_Ay  rdf:type  vec:LanguageCode , owl:NamedIndividiual;
        vec:enumLiteral  "Ay" .

[ rdf:type     owl:AllDisjointClasses;
  owl:members  ( vec:WireElementReference vec:Connection )
] .

vec:netGroupNetGroupType
        rdf:type      owl:DatatypeProperty;
        rdfs:comment  "Specifies the type of the group.\n"@en;
        rdfs:domain   vec:NetGroup;
        rdfs:label    "netGroupType"@en;
        rdfs:range    xs:string .

vec:housingComponentReferenceHousingComponent
        rdf:type      owl:ObjectProperty;
        rdfs:comment  "Points to the HousingComponent referenced by the HousingComponent reference. \n(KBLFRM-401)\n"@en;
        rdfs:domain   vec:HousingComponentReference;
        rdfs:label    "housingComponent"@en;
        rdfs:range    vec:HousingComponent .

vec:LanguageCode_It  rdf:type  vec:LanguageCode , owl:NamedIndividiual;
        vec:enumLiteral  "It" .

vec:internalTerminalConnectionWireReception
        rdf:type      owl:ObjectProperty;
        rdfs:comment  "References the WireReceptions that participate in the InternalTerminalConnection.\n"@en;
        rdfs:domain   vec:InternalTerminalConnection;
        rdfs:label    "wireReception"@en;
        rdfs:range    vec:WireReception .

vec:PrimaryPartType_WireProtection
        rdf:type         vec:PrimaryPartType , owl:NamedIndividiual;
        vec:enumLiteral  "WireProtection" .

vec:PrimaryPartType_CableDuct
        rdf:type         vec:PrimaryPartType , owl:NamedIndividiual;
        vec:enumLiteral  "CableDuct" .

vec:matingSpecificationMatingPoint
        rdf:type            owl:ObjectProperty;
        rdfs:comment        "Specifies the MatingPoints defined by the MatingSpecification.\n"@en;
        rdfs:domain         vec:MatingSpecification;
        rdfs:label          "matingPoint"@en;
        rdfs:range          vec:MatingPoint;
        rdfs:subPropertyOf  vec:contains .

vec:permissionPermitter
        rdf:type            owl:ObjectProperty;
        rdfs:comment        "Specifies the person who was involved in the approval process giving a certain Permission.\n"@en;
        rdfs:domain         vec:Permission;
        rdfs:label          "permitter"@en;
        rdfs:range          vec:Person;
        rdfs:subPropertyOf  vec:contains .

vec:FittingSpecification
        rdf:type         owl:Class;
        rdfs:comment     "Specification for the definition of fittings. A fitting is a part that is used to connect pipes or tube. A fitting has a specific form (e.g. Y,T)\n"@en;
        rdfs:label       "FittingSpecification"@en;
        rdfs:subClassOf  vec:WireProtectionSpecification .

vec:wireReceptionIdentification
        rdf:type      owl:DatatypeProperty;
        rdfs:comment  "Specifies a unique identification of the WireReception. The identification is guaranteed to be unique within the TerminalSpecification (this might be for example a reception number).\n"@en;
        rdfs:domain   vec:WireReception;
        rdfs:label    "identification"@en;
        rdfs:range    xs:string .

vec:topologySpecificationTopologyNode
        rdf:type            owl:ObjectProperty;
        rdfs:comment        "Specifies the TopologyNodes defined by the TopologySpecification.\n"@en;
        rdfs:domain         vec:TopologySpecification;
        rdfs:label          "topologyNode"@en;
        rdfs:range          vec:TopologyNode;
        rdfs:subPropertyOf  vec:contains .

vec:netSpecificationNetworkNode
        rdf:type            owl:ObjectProperty;
        rdfs:comment        "Specifies the NetWorkNodes defined in the NetSpecification.\n"@en;
        rdfs:domain         vec:NetSpecification;
        rdfs:label          "networkNode"@en;
        rdfs:range          vec:NetworkNode;
        rdfs:subPropertyOf  vec:contains .

vec:transformation2DA22
        rdf:type     owl:DatatypeProperty;
        rdfs:domain  vec:Transformation2D;
        rdfs:label   "a22"@en;
        rdfs:range   xs:double .

vec:SiPrefix_Yocto  rdf:type  vec:SiPrefix , owl:NamedIndividiual;
        vec:enumLiteral  "Yocto" .

vec:SignalTransmissionMediumType_Pneumatic
        rdf:type         vec:SignalTransmissionMediumType , owl:NamedIndividiual;
        vec:enumLiteral  "pneumatic" .

vec:StatusOfApproval  rdf:type  owl:Class;
        rdfs:comment     "Enumeration for the definition of the state of an approval.\n"@en;
        rdfs:label       "StatusOfApproval"@en;
        rdfs:subClassOf  vec:OpenEnumeration .

vec:LanguageCode_Pl  rdf:type  vec:LanguageCode , owl:NamedIndividiual;
        vec:enumLiteral  "Pl" .

vec:wireElementSpecificationWireGroupSpecification
        rdf:type      owl:ObjectProperty;
        rdfs:comment  "If the WireElement is a member of a wire group then the specification of the wire group is referenced here.\n"@en;
        rdfs:domain   vec:WireElementSpecification;
        rdfs:label    "wireGroupSpecification"@en;
        rdfs:range    vec:WireGroupSpecification .

vec:LanguageCode_Gn  rdf:type  vec:LanguageCode , owl:NamedIndividiual;
        vec:enumLiteral  "Gn" .

vec:shieldSpecificationWindingType
        rdf:type      owl:DatatypeProperty;
        rdfs:comment  "Defines the type of winding of the shield. E.g. if the shield is a sheet, it can be folded around the inner elements and along them like a cigarette paper or it can be winded around them like the taping of a harness. Both types result in different manufacturing and EMC properties.\n"@en;
        rdfs:domain   vec:ShieldSpecification;
        rdfs:label    "windingType"@en;
        rdfs:range    xs:string .

vec:robustnessPropertiesClassReferenceSystem
        rdf:type      owl:DatatypeProperty;
        rdfs:comment  "The identification of the robustness class reference system, which is defining possible values and the semantic of robustness classes and robustness class keys.\n"@en;
        rdfs:domain   vec:RobustnessProperties;
        rdfs:label    "classReferenceSystem"@en;
        rdfs:range    xs:string .

vec:mappingSlotMapping
        rdf:type            owl:ObjectProperty;
        rdfs:comment        ""@en;
        rdfs:domain         vec:Mapping;
        rdfs:label          "slotMapping"@en;
        rdfs:range          vec:SlotMapping;
        rdfs:subPropertyOf  vec:contains .

vec:SiUnitName  rdf:type     owl:Class;
        rdfs:comment         "Enumeration for the definition of SI unit names. In difference to the SI-System gram is used as literal for the measurement of mass, instead of kilogram. Since a unit is formed with prefix and unit name gram would have to be defined as milli kilogram otherwise.\n"@en;
        rdfs:label           "SiUnitName"@en;
        rdfs:subClassOf      vec:ClosedEnumeration;
        owl:equivalentClass  [ rdf:type   owl:Class;
                               owl:oneOf  ( vec:SiUnitName_Metre vec:SiUnitName_Gram vec:SiUnitName_Second vec:SiUnitName_Ampere vec:SiUnitName_Kelvin vec:SiUnitName_Mole vec:SiUnitName_Candela vec:SiUnitName_Radian vec:SiUnitName_Steradian vec:SiUnitName_Hertz vec:SiUnitName_Newton vec:SiUnitName_Pascal vec:SiUnitName_Joule vec:SiUnitName_Watt vec:SiUnitName_Coulomb vec:SiUnitName_Volt vec:SiUnitName_Farad vec:SiUnitName_Ohm vec:SiUnitName_Siemens vec:SiUnitName_Weber vec:SiUnitName_Tesla vec:SiUnitName_Henry vec:SiUnitName_DegreeCelsius vec:SiUnitName_Lumen vec:SiUnitName_Lux vec:SiUnitName_Becquerel vec:SiUnitName_Gray vec:SiUnitName_Sievert vec:SiUnitName_Katal )
                             ] .

vec:terminalRoleSealState
        rdf:type            owl:ObjectProperty;
        rdfs:comment        "Specifies if this instance of a terminal should be sealed (waterproof). This applies for example to SpliceTerminals.\n"@en;
        rdfs:domain         vec:TerminalRole;
        rdfs:label          "sealState"@en;
        rdfs:range          vec:SealState;
        rdfs:subPropertyOf  vec:contains .

vec:CartesianPoint3DWrapper
        rdf:type      owl:Class;
        rdfs:comment  "Container class for CartesianPoint3D to participate in non-unique and/or ordered associations." .

vec:FillerSpecification
        rdf:type         owl:Class;
        rdfs:comment     "Specification for the definition of filler elements in the wire.\n"@en;
        rdfs:label       "FillerSpecification"@en;
        rdfs:subClassOf  vec:Specification .

vec:signalAliasId  rdf:type  owl:ObjectProperty;
        rdfs:comment        "Specifies additional identifiers for the Signal .\n"@en;
        rdfs:domain         vec:Signal;
        rdfs:label          "aliasId"@en;
        rdfs:range          vec:AliasIdentification;
        rdfs:subPropertyOf  vec:contains .

vec:SegmentForm  rdf:type  owl:Class;
        rdfs:comment     "Enumeration for the definition of the SegmentForm.\n"@en;
        rdfs:label       "SegmentForm"@en;
        rdfs:subClassOf  vec:OpenEnumeration .

vec:placementIdentification
        rdf:type      owl:DatatypeProperty;
        rdfs:comment  "Specifies a unique identification of the Location. The identification is guaranteed to be unique within the PlacementSpecification.\n"@en;
        rdfs:domain   vec:Placement;
        rdfs:label    "identification"@en;
        rdfs:range    xs:string .

vec:wireReceptionWireReceptionSpecification
        rdf:type      owl:ObjectProperty;
        rdfs:comment  "References the WireReceptionSpecification that specifies the WireReception. \n"@en;
        rdfs:domain   vec:WireReception;
        rdfs:label    "wireReceptionSpecification"@en;
        rdfs:range    vec:WireReceptionSpecification .

vec:iECUnitIecUnitName
        rdf:type            owl:ObjectProperty;
        rdfs:comment        "Specifies the name of the IEC unit.\n"@en;
        rdfs:domain         vec:IECUnit;
        rdfs:label          "iecUnitName"@en;
        rdfs:range          vec:IECUnitName;
        rdfs:subPropertyOf  vec:contains .

vec:PartVersion  rdf:type  owl:Class;
        rdfs:comment     "The PartVersion is one of the two anchors for PDM information in the VEC. All technical information about a PartVersion is contained in one or more documents. These describing elements are normally referencing to the PartVersion.\n"@en;
        rdfs:label       "PartVersion"@en;
        rdfs:subClassOf  vec:ItemVersion .

vec:cavitySealSpecificationCavityDiameter
        rdf:type            owl:ObjectProperty;
        rdfs:comment        "Specifies a range of valid cavity diameters to which the cavity seal fits.\n"@en;
        rdfs:domain         vec:CavitySealSpecification;
        rdfs:label          "cavityDiameter"@en;
        rdfs:range          vec:ValueRange;
        rdfs:subPropertyOf  vec:contains .

vec:holeMountedFixingSpecificationHoleType
        rdf:type     owl:DatatypeProperty;
        rdfs:domain  vec:HoleMountedFixingSpecification;
        rdfs:label   "holeType"@en;
        rdfs:range   xs:string .

vec:wireProtectionRoleWireProtectionSpecification
        rdf:type      owl:ObjectProperty;
        rdfs:comment  "References the WireProtectionSpecification that is instanced by this WireProtectionRole.\n"@en;
        rdfs:domain   vec:WireProtectionRole;
        rdfs:label    "wireProtectionSpecification"@en;
        rdfs:range    vec:WireProtectionSpecification .

vec:wireSpecificationWireElement
        rdf:type            owl:ObjectProperty;
        rdfs:comment        "Specifies the WireElements that are available in the WireSpecification .\n"@en;
        rdfs:domain         vec:WireSpecification;
        rdfs:label          "wireElement"@en;
        rdfs:range          vec:WireElement;
        rdfs:subPropertyOf  vec:contains .

vec:WireGroupSpecification
        rdf:type         owl:Class;
        rdfs:comment     "Specification for the definition of WireGroups. Wire groups are for example used for the representation of twisted pairs.\n"@en;
        rdfs:label       "WireGroupSpecification"@en;
        rdfs:subClassOf  vec:Specification .

vec:PrimaryPartType_Fixing
        rdf:type         vec:PrimaryPartType , owl:NamedIndividiual;
        vec:enumLiteral  "Fixing" .

vec:personCompanyName
        rdf:type      owl:DatatypeProperty;
        rdfs:comment  "Specifies the name of the company the person belongs to.\n"@en;
        rdfs:domain   vec:Person;
        rdfs:label    "companyName"@en;
        rdfs:range    xs:string .

vec:SignalInformationType_Digital
        rdf:type         vec:SignalInformationType , owl:NamedIndividiual;
        vec:enumLiteral  "digital" .

vec:compatibilityStatementConnectorHousingSpecification
        rdf:type      owl:ObjectProperty;
        rdfs:comment  "References the ConnectorHousingSpecifications for which the compatibility statement is stated.\n"@en;
        rdfs:domain   vec:CompatibilityStatement;
        rdfs:label    "connectorHousingSpecification"@en;
        rdfs:range    vec:ConnectorHousingSpecification .

vec:partOrUsageRelatedSpecificationSpecialPartType
        rdf:type      owl:DatatypeProperty;
        rdfs:comment  "The specialPartType allows the specification of subclassifications for a PartOrUsageRelatedSpecification (e.g. different types of connector housings).\n"@en;
        rdfs:domain   vec:PartOrUsageRelatedSpecification;
        rdfs:label    "specialPartType"@en;
        rdfs:range    xs:string .

vec:connectionGroupSubGroup
        rdf:type            owl:ObjectProperty;
        rdfs:comment        "Specifies the ConnectionGroups that are a subgroup of this ConnectionGroup.\n"@en;
        rdfs:domain         vec:ConnectionGroup;
        rdfs:label          "subGroup"@en;
        rdfs:range          vec:ConnectionGroup;
        rdfs:subPropertyOf  vec:contains .

vec:boltMountedFixingSpecificationBoltDiameter
        rdf:type            owl:ObjectProperty;
        rdfs:comment        "Specifies the diameter of the bolt of the fixing.\n"@en;
        rdfs:domain         vec:BoltMountedFixingSpecification;
        rdfs:label          "boltDiameter"@en;
        rdfs:range          vec:NumericalValue;
        rdfs:subPropertyOf  vec:contains .

vec:LanguageCode_De  rdf:type  vec:LanguageCode , owl:NamedIndividiual;
        vec:enumLiteral  "De" .

vec:PinType  rdf:type    owl:Class;
        rdfs:comment     "Defines the type of a pin.\n"@en;
        rdfs:label       "PinType"@en;
        rdfs:subClassOf  vec:OpenEnumeration .

vec:valueWithUnitUnitComponent
        rdf:type      owl:ObjectProperty;
        rdfs:comment  "References the unit of the value. \n"@en;
        rdfs:domain   vec:ValueWithUnit;
        rdfs:label    "unitComponent"@en;
        rdfs:range    vec:Unit .

vec:SignalForm_SinusWave
        rdf:type         vec:SignalForm , owl:NamedIndividiual;
        vec:enumLiteral  "sinusWave" .

vec:cavityReferenceComponentPort
        rdf:type      owl:ObjectProperty;
        rdfs:comment  "References the ComponentPort that is implemented by this CavityReference .\n"@en;
        rdfs:domain   vec:CavityReference;
        rdfs:label    "componentPort"@en;
        rdfs:range    vec:ComponentPort .

vec:cartesianPoint3DX
        rdf:type      owl:DatatypeProperty;
        rdfs:comment  "Specifies the value of x-coordinate of the Cartesian point. The unit of this value is the baseUnit of containing BuildingBlockSpecification3D.\n"@en;
        rdfs:domain   vec:CartesianPoint3D;
        rdfs:label    "x"@en;
        rdfs:range    xs:double .

vec:LanguageCode_Rw  rdf:type  vec:LanguageCode , owl:NamedIndividiual;
        vec:enumLiteral  "Rw" .

vec:usageConstraintType
        rdf:type            owl:ObjectProperty;
        rdfs:comment        "Defines if the usage constraint is positive (allowance) or negative (denial).\n"@en;
        rdfs:domain         vec:UsageConstraint;
        rdfs:label          "type"@en;
        rdfs:range          vec:UsageConstraintType;
        rdfs:subPropertyOf  vec:contains .

vec:SignalInformationType
        rdf:type         owl:Class;
        rdfs:label       "SignalInformationType"@en;
        rdfs:subClassOf  vec:OpenEnumeration .

vec:WireProtectionSpecification
        rdf:type         owl:Class;
        rdfs:comment     "Specification for the description of wire protections.\n"@en;
        rdfs:label       "WireProtectionSpecification"@en;
        rdfs:subClassOf  vec:PartOrUsageRelatedSpecification .

vec:LanguageCode_Yo  rdf:type  vec:LanguageCode , owl:NamedIndividiual;
        vec:enumLiteral  "Yo" .

vec:CorrugatedPipeSpecification
        rdf:type         owl:Class;
        rdfs:comment     "Specification for the definition of corrugated pipes.\n"@en;
        rdfs:label       "CorrugatedPipeSpecification"@en;
        rdfs:subClassOf  vec:TubeSpecification .

vec:SignalTransmissionMediumType_Electrical
        rdf:type         vec:SignalTransmissionMediumType , owl:NamedIndividiual;
        vec:enumLiteral  "electrical" .

vec:PrimaryPartType_Grommet
        rdf:type         vec:PrimaryPartType , owl:NamedIndividiual;
        vec:enumLiteral  "Grommet" .

vec:FileBasedInstruction
        rdf:type         owl:Class;
        rdfs:comment     "A FileBasedInstruction is an Instruction that references a file packaged together with a VEC-document. Such a file can be for example an image.\n"@en;
        rdfs:label       "FileBasedInstruction"@en;
        rdfs:subClassOf  vec:Instruction .

vec:transformation3DA33
        rdf:type     owl:DatatypeProperty;
        rdfs:domain  vec:Transformation3D;
        rdfs:label   "a33"@en;
        rdfs:range   xs:double .

vec:materialKey  rdf:type  owl:DatatypeProperty;
        rdfs:comment  "The key of the material in the corresponding material reference system.\n"@en;
        rdfs:domain   vec:Material;
        rdfs:label    "key"@en;
        rdfs:range    xs:string .

vec:Size  rdf:type    owl:Class;
        rdfs:comment  "Defines the size of an element by width & height.\n"@en;
        rdfs:label    "Size"@en .

vec:compatibilityStatementCavitySealSpecification
        rdf:type      owl:ObjectProperty;
        rdfs:comment  "References the CavitySealSpecifications for which the compatibility statement is stated.\n"@en;
        rdfs:domain   vec:CompatibilityStatement;
        rdfs:label    "cavitySealSpecification"@en;
        rdfs:range    vec:CavitySealSpecification .

vec:tapeSpecificationBacking
        rdf:type            owl:ObjectProperty;
        rdfs:comment        "Specifies the material of carrier of the tape, on which the adhesive material is applied.\n"@en;
        rdfs:domain         vec:TapeSpecification;
        rdfs:label          "backing"@en;
        rdfs:range          vec:Material;
        rdfs:subPropertyOf  vec:contains .

vec:placementPointIdentification
        rdf:type      owl:DatatypeProperty;
        rdfs:comment  "Specifies a unique identification of the PlacementPoint. The identification is guaranteed to be unique within a component.\n"@en;
        rdfs:domain   vec:PlacementPoint;
        rdfs:label    "identification"@en;
        rdfs:range    xs:string .

vec:SiUnitName_Farad  rdf:type  vec:SiUnitName , owl:NamedIndividiual;
        vec:enumLiteral  "Farad" .

vec:terminalReceptionSpecificationPrimaryLockingType
        rdf:type      owl:DatatypeProperty;
        rdfs:comment  "Specifies if the terminal reception has a primary locking and of what type it is.\n"@en;
        rdfs:domain   vec:TerminalReceptionSpecification;
        rdfs:label    "primaryLockingType"@en;
        rdfs:range    xs:string .

vec:connectionGroupNetGroup
        rdf:type      owl:ObjectProperty;
        rdfs:comment  "References the NetworkGroup that is realized by the ComponentGroup.\n"@en;
        rdfs:domain   vec:ConnectionGroup;
        rdfs:label    "netGroup"@en;
        rdfs:range    vec:NetGroup .

vec:PrimaryPartType_Battery
        rdf:type         vec:PrimaryPartType , owl:NamedIndividiual;
        vec:enumLiteral  "Battery" .

vec:placementPointSegmentDiameter
        rdf:type            owl:ObjectProperty;
        rdfs:comment        "Specifies the valid segment diameter range for which this PlacementPoint is suitable.\n"@en;
        rdfs:domain         vec:PlacementPoint;
        rdfs:label          "segmentDiameter"@en;
        rdfs:range          vec:ValueRange;
        rdfs:subPropertyOf  vec:contains .

vec:PrimaryPartType_Other
        rdf:type         vec:PrimaryPartType , owl:NamedIndividiual;
        vec:enumLiteral  "Other" .

vec:signalSpecificationSignal
        rdf:type            owl:ObjectProperty;
        rdfs:comment        "Specifies the signals.\n"@en;
        rdfs:domain         vec:SignalSpecification;
        rdfs:label          "signal"@en;
        rdfs:range          vec:Signal;
        rdfs:subPropertyOf  vec:contains .

vec:PrimaryPartType_Antenna
        rdf:type         vec:PrimaryPartType , owl:NamedIndividiual;
        vec:enumLiteral  "Antenna" .

vec:slotLayoutRowCount
        rdf:type      owl:DatatypeProperty;
        rdfs:comment  "The number of cavity rows of the slot.\n"@en;
        rdfs:domain   vec:SlotLayout;
        rdfs:label    "rowCount"@en;
        rdfs:range    xs:integer .

vec:cavitySpecificationCompatibleTerminalType
        rdf:type            owl:ObjectProperty;
        rdfs:comment        "Defines a list of terminal types that are compatible to this CavitySpecification.\n"@en;
        rdfs:domain         vec:CavitySpecification;
        rdfs:label          "compatibleTerminalType"@en;
        rdfs:range          vec:TerminalType;
        rdfs:subPropertyOf  vec:contains .

vec:variantGroupDescription
        rdf:type            owl:ObjectProperty;
        rdfs:comment        "On optional human readable description of the variant group.\n"@en;
        rdfs:domain         vec:VariantGroup;
        rdfs:label          "description"@en;
        rdfs:range          vec:AbstractLocalizedString;
        rdfs:subPropertyOf  vec:contains .

vec:projectIdentification
        rdf:type      owl:DatatypeProperty;
        rdfs:comment  "Specifies the development order number (car or engine project)\n"@en;
        rdfs:domain   vec:Project;
        rdfs:label    "identification"@en;
        rdfs:range    xs:string .

vec:geometryNodeReferenceNode
        rdf:type      owl:ObjectProperty;
        rdfs:comment  "References the TopologyNode that is represented by the GeometryNode.\n"@en;
        rdfs:domain   vec:GeometryNode;
        rdfs:label    "referenceNode"@en;
        rdfs:range    vec:TopologyNode .

vec:edgeMountedFixingSpecificationEdgeThickness
        rdf:type            owl:ObjectProperty;
        rdfs:comment        "Defines a range of valid thicknesses, onto which the fixing can be mounted.\n"@en;
        rdfs:domain         vec:EdgeMountedFixingSpecification;
        rdfs:label          "edgeThickness"@en;
        rdfs:range          vec:ValueRange;
        rdfs:subPropertyOf  vec:contains .

vec:routingMandatorySegment
        rdf:type      owl:ObjectProperty;
        rdfs:comment  "Specifies some constraints for the routing. If the path of the routing is recalculated the referenced segments must be visited. \n"@en;
        rdfs:domain   vec:Routing;
        rdfs:label    "mandatorySegment"@en;
        rdfs:range    vec:TopologySegment .

vec:MeasurementPointReference
        rdf:type         owl:Class;
        rdfs:comment     "A MeasurementPointReference is the instance of a MeasurementPoint in the context of an OccurrenceOrUsage .\n"@en;
        rdfs:label       "MeasurementPointReference"@en;
        rdfs:subClassOf  vec:DimensionAnchor .

vec:SiUnitName_Henry  rdf:type  vec:SiUnitName , owl:NamedIndividiual;
        vec:enumLiteral  "Henry" .

vec:vecContentDocumentVersion
        rdf:type            owl:ObjectProperty;
        rdfs:comment        "Specifies the DocumentVersions contained in the VEC-file. \n"@en;
        rdfs:domain         vec:VecContent;
        rdfs:label          "documentVersion"@en;
        rdfs:range          vec:DocumentVersion;
        rdfs:subPropertyOf  vec:contains .

vec:wireElementSpecificationSuitedForDynamicUse
        rdf:type      owl:DatatypeProperty;
        rdfs:comment  "Specifies if it is allowed to use the WireElement in a dynamic environment. (see KBLFRM-311)\n"@en;
        rdfs:domain   vec:WireElementSpecification;
        rdfs:label    "suitedForDynamicUse"@en;
        rdfs:range    xs:boolean .

vec:compatibilityStatementWireSpecification
        rdf:type      owl:ObjectProperty;
        rdfs:comment  "References the WireSpecifications for which the compatibility statement is stated.\n"@en;
        rdfs:domain   vec:CompatibilityStatement;
        rdfs:label    "wireSpecification"@en;
        rdfs:range    vec:WireSpecification .

vec:conductorSpecificationVoltageRange
        rdf:type            owl:ObjectProperty;
        rdfs:comment        "Specifies the voltageRange for which the conductor is approved.\n"@en;
        rdfs:domain         vec:ConductorSpecification;
        rdfs:label          "voltageRange"@en;
        rdfs:range          vec:NumericalValue;
        rdfs:subPropertyOf  vec:contains .

vec:cavityPlugSpecificationSealingClass
        rdf:type            owl:ObjectProperty;
        rdfs:comment        "Specifies the sealing class of the cavity plug.\n"@en;
        rdfs:domain         vec:CavityPlugSpecification;
        rdfs:label          "sealingClass"@en;
        rdfs:range          vec:SealingClass;
        rdfs:subPropertyOf  vec:contains .

vec:ClosedEnumeration
        rdf:type         owl:Class;
        rdfs:comment     "Classes in the model that can be enumerated and where all values are known (closed)."@en;
        rdfs:label       "ClosedEnumeration"@en;
        rdfs:subClassOf  vec:Enumeration .

vec:connectionSignal  rdf:type  owl:ObjectProperty;
        rdfs:comment  "References the signal that is transmitted by the connection.\n"@en;
        rdfs:domain   vec:Connection;
        rdfs:label    "signal"@en;
        rdfs:range    vec:Signal .

vec:LanguageCode_Aa  rdf:type  vec:LanguageCode , owl:NamedIndividiual;
        rdfs:comment     "Afar\n"@en;
        vec:enumLiteral  "Aa" .

vec:occurrenceOrUsageAbbreviation
        rdf:type            owl:ObjectProperty;
        rdfs:comment        "Specifies an abbreviation of the OccurrenceOrUsage . Normally this a human readable short name.\n"@en;
        rdfs:domain         vec:OccurrenceOrUsage;
        rdfs:label          "abbreviation"@en;
        rdfs:range          vec:LocalizedString;
        rdfs:subPropertyOf  vec:contains .

vec:variantConfigurationLogisticControlString
        rdf:type      owl:DatatypeProperty;
        rdfs:comment  "Specifies a logisticControlString which can be used if the variant management is not done by boolean logic.\n"@en;
        rdfs:domain   vec:VariantConfiguration;
        rdfs:label    "logisticControlString"@en;
        rdfs:range    xs:string .

vec:fittingSpecificationForm
        rdf:type      owl:DatatypeProperty;
        rdfs:comment  "Specifies the form of the fitting (e.g. Y, T).\n"@en;
        rdfs:domain   vec:FittingSpecification;
        rdfs:label    "form"@en;
        rdfs:range    xs:string .

vec:zoneAmbientTemperature
        rdf:type            owl:ObjectProperty;
        rdfs:comment        "Defines the ambient temperature that can occur in this zone. This can result in specific requirements for the used components.\n"@en;
        rdfs:domain         vec:Zone;
        rdfs:label          "ambientTemperature"@en;
        rdfs:range          vec:TemperatureInformation;
        rdfs:subPropertyOf  vec:contains .

vec:conformanceClassUrl
        rdf:type      owl:DatatypeProperty;
        rdfs:comment  "Specifies the URL of the conformance class where conformance class file is available.\n"@en;
        rdfs:domain   vec:ConformanceClass;
        rdfs:label    "url"@en;
        rdfs:range    xs:string .

vec:wireGroupingRelatedWireRole
        rdf:type      owl:ObjectProperty;
        rdfs:comment  "References the concrete wire elements (WireElementReference) that are grouped by the WireGrouping. \n"@en;
        rdfs:domain   vec:WireGrouping;
        rdfs:label    "relatedWireRole"@en;
        rdfs:range    vec:WireElementReference .

vec:variantConfigurationSpecificationVariantConfiguration
        rdf:type            owl:ObjectProperty;
        rdfs:comment        "Specifies the individual VariantConfigurations defined in the VariantConfigurationSpecification.\n"@en;
        rdfs:domain         vec:VariantConfigurationSpecification;
        rdfs:label          "variantConfiguration"@en;
        rdfs:range          vec:VariantConfiguration;
        rdfs:subPropertyOf  vec:contains .

vec:wireReceptionSpecificationPlatingMaterial
        rdf:type            owl:ObjectProperty;
        rdfs:comment        "Specifies the plating material of the wire reception.\n"@en;
        rdfs:domain         vec:WireReceptionSpecification;
        rdfs:label          "platingMaterial"@en;
        rdfs:range          vec:Material;
        rdfs:subPropertyOf  vec:contains .

vec:transformation2DOrigin
        rdf:type      owl:ObjectProperty;
        rdfs:comment  "References the CartesianPoint2D that is the origin of the Transformation2D. \n"@en;
        rdfs:domain   vec:Transformation2D;
        rdfs:label    "origin"@en;
        rdfs:range    vec:CartesianPoint2D .

vec:cartesianPoint2DSheet
        rdf:type      owl:ObjectProperty;
        rdfs:comment  "A two dimensional building block can contain one or more sheets. The CartesianPoint can reference the sheet on which it is placed. \n"@en;
        rdfs:domain   vec:CartesianPoint2D;
        rdfs:label    "sheet"@en;
        rdfs:range    vec:SheetOrChapter .

vec:fileBasedInstructionLastModified
        rdf:type      owl:DatatypeProperty;
        rdfs:comment  "The last modified timestamp of the file.\n"@en;
        rdfs:domain   vec:FileBasedInstruction;
        rdfs:label    "lastModified"@en;
        rdfs:range    xs:dateTime .

vec:geometrySegmentIdentification
        rdf:type      owl:DatatypeProperty;
        rdfs:comment  "Specifies a unique identification of the GeometrySegment. The identification is guaranteed to be unique within the corresponding BuildingBlockSpecification. Over all VEC-documents a GeometrySegment-instance can be trusted to be the same if the BuildingBlockSpecification-instance is the same (see BuildingBlockSpecification) and the identification of the GeometrySegment is the same.\n"@en;
        rdfs:domain   vec:GeometrySegment;
        rdfs:label    "identification"@en;
        rdfs:range    xs:string .

vec:RelaySpecification
        rdf:type         owl:Class;
        rdfs:comment     "Specification of the electrological aspects of a relay.\n"@en;
        rdfs:label       "RelaySpecification"@en;
        rdfs:subClassOf  vec:EEComponentSpecification .

vec:cavityReferenceIdentification
        rdf:type      owl:DatatypeProperty;
        rdfs:comment  "Specifies a unique identification of the CavityReference. The identification is guaranteed to be unique within the ConnectorHousingRole. The cavity & slot number is defined by the associated cavity and slot.\n"@en;
        rdfs:domain   vec:CavityReference;
        rdfs:label    "identification"@en;
        rdfs:range    xs:string .

vec:USUnitName_Foot  rdf:type  vec:USUnitName , owl:NamedIndividiual;
        vec:enumLiteral  "Foot" .

vec:geometryNode2DCartesianPoint
        rdf:type      owl:ObjectProperty;
        rdfs:comment  "References the CartesianPoint2D where the GeometryNode2D is located. \n"@en;
        rdfs:domain   vec:GeometryNode2D;
        rdfs:label    "cartesianPoint"@en;
        rdfs:range    vec:CartesianPoint2D .

vec:InsulationSpecification
        rdf:type         owl:Class;
        rdfs:comment     "Specification for the definition of insulation properties of a WireElement.\n"@en;
        rdfs:label       "InsulationSpecification"@en;
        rdfs:subClassOf  vec:Specification .

vec:buildingBlockPositioning2DReferenced2DBuildingBlock
        rdf:type      owl:ObjectProperty;
        rdfs:comment  "References the building block which is placed on the harness drawing. \n"@en;
        rdfs:domain   vec:BuildingBlockPositioning2D;
        rdfs:label    "referenced2DBuildingBlock"@en;
        rdfs:range    vec:BuildingBlockSpecification2D .

vec:transformation3DA12
        rdf:type     owl:DatatypeProperty;
        rdfs:domain  vec:Transformation3D;
        rdfs:label   "a12"@en;
        rdfs:range   xs:double .

vec:aliasIdentificationDescription
        rdf:type            owl:ObjectProperty;
        rdfs:comment        "On optional human readable description of the AliasIdentification.\n"@en;
        rdfs:domain         vec:AliasIdentification;
        rdfs:label          "description"@en;
        rdfs:range          vec:AbstractLocalizedString;
        rdfs:subPropertyOf  vec:contains .

vec:matingPointFirstTerminalRole
        rdf:type      owl:ObjectProperty;
        rdfs:comment  "References the first terminal that is mated.\n"@en;
        rdfs:domain   vec:MatingPoint;
        rdfs:label    "firstTerminalRole"@en;
        rdfs:range    vec:TerminalRole .

vec:LanguageCode_Te  rdf:type  vec:LanguageCode , owl:NamedIndividiual;
        vec:enumLiteral  "Te" .

vec:ImperialUnitName_Thou
        rdf:type         vec:ImperialUnitName , owl:NamedIndividiual;
        vec:enumLiteral  "Thou" .

vec:moduleListSpecificationModuleListConfiguration
        rdf:type            owl:ObjectProperty;
        rdfs:comment        "Specifies the ModuleLists defined in the ModuleListSpecification.\n"@en;
        rdfs:domain         vec:ModuleListSpecification;
        rdfs:label          "moduleListConfiguration"@en;
        rdfs:range          vec:ModuleList;
        rdfs:subPropertyOf  vec:contains .

vec:itemHistoryEntryType
        rdf:type            owl:ObjectProperty;
        rdfs:comment        "Specifies the type of relationship between the ItemVersions.\n"@en;
        rdfs:domain         vec:ItemHistoryEntry;
        rdfs:label          "type"@en;
        rdfs:range          vec:HistoryEntryType;
        rdfs:subPropertyOf  vec:contains .

vec:variantCodeIdentification
        rdf:type      owl:DatatypeProperty;
        rdfs:comment  "Specifies a unique identification of the variant code. This is also the literal value for the VariantCode, which shall be used in the logisticControlExrpessions of VariantConfigurations.\n"@en;
        rdfs:domain   vec:VariantCode;
        rdfs:label    "identification"@en;
        rdfs:range    xs:string .

vec:ringTerminalSpecificationBoltDiameter
        rdf:type            owl:ObjectProperty;
        rdfs:comment        "Specifies the diameter of the bolt for which the ring terminal is designed for.\n"@en;
        rdfs:domain         vec:RingTerminalSpecification;
        rdfs:label          "boltDiameter"@en;
        rdfs:range          vec:NumericalValue;
        rdfs:subPropertyOf  vec:contains .

vec:placementSpecificationPlacement
        rdf:type            owl:ObjectProperty;
        rdfs:comment        "Specifies the Placements defined by the PlacementSpecification.\n"@en;
        rdfs:domain         vec:PlacementSpecification;
        rdfs:label          "placement"@en;
        rdfs:range          vec:Placement;
        rdfs:subPropertyOf  vec:contains .

vec:corrugatedPipeSpecificationCorrugationWidth
        rdf:type            owl:ObjectProperty;
        rdfs:comment        "Specifies the width of a corrugation of the pipe.\n"@en;
        rdfs:domain         vec:CorrugatedPipeSpecification;
        rdfs:label          "corrugationWidth"@en;
        rdfs:range          vec:NumericalValue;
        rdfs:subPropertyOf  vec:contains .

vec:moduleFamilyDescription
        rdf:type            owl:ObjectProperty;
        rdfs:comment        "Room for additional, human readable information about the ModuleFamily.\n"@en;
        rdfs:domain         vec:ModuleFamily;
        rdfs:label          "description"@en;
        rdfs:range          vec:AbstractLocalizedString;
        rdfs:subPropertyOf  vec:contains .

vec:LanguageCode_Bi  rdf:type  vec:LanguageCode , owl:NamedIndividiual;
        vec:enumLiteral  "Bi" .

vec:dimensionDefinedLocations
        rdf:type            owl:ObjectProperty;
        rdfs:comment        ""@en;
        rdfs:domain         vec:Dimension;
        rdfs:label          "definedLocations"@en;
        rdfs:range          vec:Location;
        rdfs:subPropertyOf  vec:contains .

vec:terminalReceptionSpecificationCavityDesign
        rdf:type      owl:DatatypeProperty;
        rdfs:comment  "Specifies the structural shape of the cavity, e.g. round, flat, box that the terminal fits in.\n"@en;
        rdfs:domain   vec:TerminalReceptionSpecification;
        rdfs:label    "cavityDesign"@en;
        rdfs:range    xs:string .

vec:CavitySealRole  rdf:type  owl:Class;
        rdfs:comment     "A CavitySealRole defines the instance specific properties and relationships of a cavity seal.\n"@en;
        rdfs:label       "CavitySealRole"@en;
        rdfs:subClassOf  vec:Role .

vec:PathSegment  rdf:type  owl:Class;
        rdfs:comment     "A PathSegment is a part of the 2D presentation of a GeometrySegment2D. The complete presentation of a GeometrySegment2D is built from an ordered list of PathSegments. Each PathSegment has an ordered list of control points through which the path goes. If no curveRadius is specified the control points are connected by a direct straight lines. If a curveRadius is specified, the PathSegment can be drawn by a segment of a circle which touches all control points and has the radius specified.\n"@en;
        rdfs:label       "PathSegment"@en;
        rdfs:subClassOf  vec:ExtendableElement .

vec:PrimaryPartType_Wire
        rdf:type         vec:PrimaryPartType , owl:NamedIndividiual;
        vec:enumLiteral  "Wire" .

vec:LanguageCode_Af  rdf:type  vec:LanguageCode , owl:NamedIndividiual;
        vec:enumLiteral  "Af" .

vec:sealingClassClassReferenceSystem
        rdf:type      owl:DatatypeProperty;
        rdfs:comment  "The identification of the sealing class reference system, which is defining possible values and the semantic of sealing classes and sealing class keys.\n"@en;
        rdfs:domain   vec:SealingClass;
        rdfs:label    "classReferenceSystem"@en;
        rdfs:range    xs:string .

vec:occurrenceOrUsageInstallationInstruction
        rdf:type            owl:ObjectProperty;
        rdfs:comment        "Room to specify InstallationInstruction(s) for the OccurrenceOrUsage. \n"@en;
        rdfs:domain         vec:OccurrenceOrUsage;
        rdfs:label          "installationInstruction"@en;
        rdfs:range          vec:Instruction;
        rdfs:subPropertyOf  vec:contains .

vec:slotSpecificationEmvProtectionRequired
        rdf:type      owl:DatatypeProperty;
        rdfs:comment  "Specifies whether the slot needs EMV protection.\n"@en;
        rdfs:domain   vec:SlotSpecification;
        rdfs:label    "emvProtectionRequired"@en;
        rdfs:range    xs:boolean .

vec:documentVersionCreatingSystem
        rdf:type      owl:DatatypeProperty;
        rdfs:comment  "The creatingSystem specifies the computer application or the machine which is used to create the document.\n"@en;
        rdfs:domain   vec:DocumentVersion;
        rdfs:label    "creatingSystem"@en;
        rdfs:range    xs:string .

vec:abstractLocalizedStringLanguageCode
        rdf:type            owl:ObjectProperty;
        rdfs:comment        "References the corresponding languageCode of the value.\n"@en;
        rdfs:domain         vec:AbstractLocalizedString;
        rdfs:label          "languageCode"@en;
        rdfs:range          vec:LanguageCode;
        rdfs:subPropertyOf  vec:contains .

vec:AbstractLocalizedString
        rdf:type      owl:Class;
        rdfs:comment  "Abstract super-class for Localized text values. "@en;
        rdfs:label    "AbstractLocalizedString"@en .

vec:terminalCurrentInformationCoreCrossSectionArea
        rdf:type            owl:ObjectProperty;
        rdfs:comment        "Specifies the coreCrossSectionArea for which the CurrentRangeInformation is valid. The coreCrossSectionArea is a relevant information, because the thermal absorption of the core depends on the cross section area and thus is a influence factor for the valid current range.\n"@en;
        rdfs:domain         vec:TerminalCurrentInformation;
        rdfs:label          "coreCrossSectionArea"@en;
        rdfs:range          vec:NumericalValue;
        rdfs:subPropertyOf  vec:contains .

vec:VariantGroup  rdf:type  owl:Class;
        rdfs:comment     "With a VariantGroup it is possible to group VariantCodes. The semantic of this grouping should be defined with the groupType (e.g. composition, choice, etc.).\n"@en;
        rdfs:label       "VariantGroup"@en;
        rdfs:subClassOf  vec:ExtendableElement .

vec:LanguageCode_Ia  rdf:type  vec:LanguageCode , owl:NamedIndividiual;
        vec:enumLiteral  "Ia" .

vec:batterySpecificationCapacity
        rdf:type            owl:ObjectProperty;
        rdfs:comment        "Specifies the power capacity of the battery.\n"@en;
        rdfs:domain         vec:BatterySpecification;
        rdfs:label          "capacity"@en;
        rdfs:range          vec:NumericalValue;
        rdfs:subPropertyOf  vec:contains .

vec:ConductorCurrentInformation
        rdf:type      owl:Class;
        rdfs:comment  "The ConductorCurrentInformation specifies the maximum current for which a conductor is approved. As the maximum current is dependent from the voltage and the environment temperature it is modeled as a class and not only as an attribute.\n"@en;
        rdfs:label    "ConductorCurrentInformation"@en .

vec:MultiCavitySealSpecification
        rdf:type         owl:Class;
        rdfs:comment     "Specification for cavity seals that apply to more than one cavity. A CavitySeal is a water tight non-electrical object to fill a populated Cavity. MultiCavitySeals are formed to fit into one connector / slot and to seal more than one cavity at once.\nThere are existing two types of MultiCavitySeals: In first type the MultiCavitySeal has an opening for all cavities of the connector. Each opening can be filled either with a wire (without an individual seal) or with a CavityPlug (e.g. a synthetic pin) or a MultiCavityPlug. In the second type, the MultiCavitySeal has a specific configuration of openings for some cavities of the connector. These MultiCavitySeals are sealing all cavities with an opening and a wire in it and all cavities where no opening in the MultiCavitySeal exists. For each opening that has no wire it an additional CavityPlug is needed.┬á The cavities that are left open by a MultiCavitySeal are defined with a SealedCavitiesAssignment.\n"@en;
        rdfs:label       "MultiCavitySealSpecification"@en;
        rdfs:subClassOf  vec:CavitySealSpecification .

vec:usageConstraintSpecificationPartUsageConstraint
        rdf:type            owl:ObjectProperty;
        rdfs:comment        "Specifies the UsageConstraints that apply to the PartVersion or PartUsages described by the UsageConstraintSpecification. \n"@en;
        rdfs:domain         vec:UsageConstraintSpecification;
        rdfs:label          "partUsageConstraint"@en;
        rdfs:range          vec:UsageConstraint , vec:Ordered;
        rdfs:subPropertyOf  vec:contains .

vec:AnchorType  rdf:type     owl:Class;
        rdfs:comment         "Enumeration for the definition of AnchorType of the SegmentLocation.\n"@en;
        rdfs:label           "AnchorType"@en;
        rdfs:subClassOf      vec:ClosedEnumeration;
        owl:equivalentClass  [ rdf:type   owl:Class;
                               owl:oneOf  ( vec:AnchorType_FromStartNode vec:AnchorType_FromEndNode )
                             ] .

vec:componentPortDescription
        rdf:type            owl:ObjectProperty;
        rdfs:comment        "Room for additional, human readable information about the ComponentPort.\n"@en;
        rdfs:domain         vec:ComponentPort;
        rdfs:label          "description"@en;
        rdfs:range          vec:AbstractLocalizedString;
        rdfs:subPropertyOf  vec:contains .

vec:onWayPlacementEndLocation
        rdf:type            owl:ObjectProperty;
        rdfs:comment        "References the Location where OnWayPlacement ends. \n"@en;
        rdfs:domain         vec:OnWayPlacement;
        rdfs:label          "endLocation"@en;
        rdfs:range          vec:Location;
        rdfs:subPropertyOf  vec:contains .

[ rdf:type     owl:AllDisjointClasses;
  owl:members  ( vec:DocumentBasedInstruction vec:FileBasedInstruction vec:TextBasedInstruction )
] .

vec:pinVoltageInformationVoltage
        rdf:type            owl:ObjectProperty;
        rdfs:comment        "The voltage of the pin.\n"@en;
        rdfs:domain         vec:PinVoltageInformation;
        rdfs:label          "voltage"@en;
        rdfs:range          vec:NumericalValue;
        rdfs:subPropertyOf  vec:contains .

vec:abstractSlotSlotSpecification
        rdf:type      owl:ObjectProperty;
        rdfs:comment  "References the SlotSpecification that is satisfied by the slot.\n"@en;
        rdfs:domain   vec:AbstractSlot;
        rdfs:label    "slotSpecification"@en;
        rdfs:range    vec:SlotSpecification .

vec:antennaSpecificationImpedance
        rdf:type            owl:ObjectProperty;
        rdfs:comment        "Specifies the impedance of the antenna.\n"@en;
        rdfs:domain         vec:AntennaSpecification;
        rdfs:label          "impedance"@en;
        rdfs:range          vec:NumericalValue;
        rdfs:subPropertyOf  vec:contains .

vec:topologySegmentStartNode
        rdf:type      owl:ObjectProperty;
        rdfs:comment  "References the TopologyNode where the TopologySegment starts. \n"@en;
        rdfs:domain   vec:TopologySegment;
        rdfs:label    "startNode"@en;
        rdfs:range    vec:TopologyNode .

vec:IECPrefix_Gibi  rdf:type  vec:IECPrefix , owl:NamedIndividiual;
        vec:enumLiteral  "Gibi" .

[ rdf:type     owl:AllDisjointClasses;
  owl:members  ( vec:ModularSlotReference vec:SlotReference )
] .

vec:BuildingBlockSpecification3D
        rdf:type         owl:Class;
        rdfs:comment     "Specification for the description of a three dimensional building block. A building block is a reusable section of a geometry.\n"@en;
        rdfs:label       "BuildingBlockSpecification3D"@en;
        rdfs:subClassOf  vec:Specification .

vec:terminalSpecificationVoltageRange
        rdf:type            owl:ObjectProperty;
        rdfs:comment        "Specifies the allowed voltage range for the connector housing.\n"@en;
        rdfs:domain         vec:TerminalSpecification;
        rdfs:label          "voltageRange"@en;
        rdfs:range          vec:ValueRange;
        rdfs:subPropertyOf  vec:contains .

vec:LanguageCode_Mr  rdf:type  vec:LanguageCode , owl:NamedIndividiual;
        vec:enumLiteral  "Mr" .

vec:coreSpecificationOutsideDiameter
        rdf:type            owl:ObjectProperty;
        rdfs:comment        "Specifies the outside diameter of the core.\n"@en;
        rdfs:domain         vec:CoreSpecification;
        rdfs:label          "outsideDiameter"@en;
        rdfs:range          vec:NumericalValue;
        rdfs:subPropertyOf  vec:contains .

vec:MatingDetail  rdf:type  owl:Class;
        rdfs:comment     "If the mating of the two terminals is not unambiguously, a MatingDetail can specify the TerminalReceptions that are mated.\n"@en;
        rdfs:label       "MatingDetail"@en;
        rdfs:subClassOf  vec:ExtendableElement .

vec:IECPrefix_Exbi  rdf:type  vec:IECPrefix , owl:NamedIndividiual;
        vec:enumLiteral  "Exbi" .

vec:InsulationState_Insulated
        rdf:type         vec:InsulationState , owl:NamedIndividiual;
        rdfs:comment     "The splice is electrically insulated.\n"@en;
        vec:enumLiteral  "Insulated" .

vec:LanguageCode_Lo  rdf:type  vec:LanguageCode , owl:NamedIndividiual;
        vec:enumLiteral  "Lo" .

vec:bSplineCurveControlPoint
        rdf:type            owl:ObjectProperty;
        rdfs:comment        "This association is defined as unique='false' and ordered='true'. This can not be represented efficiently directly in RDF/OWL. Therefore, this association references Wrappers as proxies to the actual elements, instead of the actual elements itself (like a regular association)." , "The list of control points for the curve. The list shall contain at least 2 elements. \n"@en;
        rdfs:domain         vec:BSplineCurve;
        rdfs:label          "controlPoint"@en;
        rdfs:range          vec:CartesianPoint3DWrapper , vec:Ordered;
        rdfs:subPropertyOf  vec:contains .

vec:onWayPlacementStartLocation
        rdf:type            owl:ObjectProperty;
        rdfs:comment        "References the Location where OnWayPlacement starts. \n"@en;
        rdfs:domain         vec:OnWayPlacement;
        rdfs:label          "startLocation"@en;
        rdfs:range          vec:Location;
        rdfs:subPropertyOf  vec:contains .

[ rdf:type     owl:AllDisjointClasses;
  owl:members  ( vec:DocumentVersion vec:PartVersion )
] .

vec:ConductorSpecification
        rdf:type         owl:Class;
        rdfs:comment     "Specification for the definition of conducting properties of a WireElement.\n"@en;
        rdfs:label       "ConductorSpecification"@en;
        rdfs:subClassOf  vec:Specification .

vec:toleranceLowerBoundary
        rdf:type      owl:DatatypeProperty;
        rdfs:comment  "Specifies the lower boundary for the tolerance.\n"@en;
        rdfs:domain   vec:Tolerance;
        rdfs:label    "lowerBoundary"@en;
        rdfs:range    xs:double .

vec:usageConstraintUsageNode
        rdf:type      owl:ObjectProperty;
        rdfs:comment  "References the UsageNode to which the UsageConstraint applies. This means the described PartVersion is allowed / denied in the referenced UsageConstraint."@en;
        rdfs:domain   vec:UsageConstraint;
        rdfs:label    "usageNode"@en;
        rdfs:range    vec:UsageNode .

vec:componentPortIdentification
        rdf:type      owl:DatatypeProperty;
        rdfs:comment  "Specifies a unique identification of the ComponentPort. The identification is guaranteed to be unique within the ConnectionSpecification.\n"@en;
        rdfs:domain   vec:ComponentPort;
        rdfs:label    "identification"@en;
        rdfs:range    xs:string .

vec:Transformation2D  rdf:type  owl:Class;
        rdfs:comment     "A Transformation is a geometric transformation and specifies a transformation matrix.\n"@en;
        rdfs:label       "Transformation2D"@en;
        rdfs:subClassOf  vec:ExtendableElement .

vec:geometrySegment3DStartNode
        rdf:type      owl:ObjectProperty;
        rdfs:comment  "References the GeometryNode3D where the GeometrySegment3D starts. \n"@en;
        rdfs:domain   vec:GeometrySegment3D;
        rdfs:label    "startNode"@en;
        rdfs:range    vec:GeometryNode3D .

vec:LanguageCode_Kl  rdf:type  vec:LanguageCode , owl:NamedIndividiual;
        vec:enumLiteral  "Kl" .

vec:terminalRoleTerminalSpecification
        rdf:type      owl:ObjectProperty;
        rdfs:comment  "┬áReferences the TerminalSpecification that is instanced by this TerminalRole.\n"@en;
        rdfs:domain   vec:TerminalRole;
        rdfs:label    "terminalSpecification"@en;
        rdfs:range    vec:TerminalSpecification .

vec:ItemEquivalence  rdf:type  owl:Class;
        rdfs:comment     "Defines two or more ItemVersions to be equivalent out of the view of a certain company. The ItemEquivalence class will most likely be used by a company to express which PartNumber a certain PartVersion has in the context of other companies. However, for every other company separate ItemVersion-instances are needed as the statement of equivalence can be very subjective.\n"@en;
        rdfs:label       "ItemEquivalence"@en;
        rdfs:subClassOf  vec:ExtendableElement .

vec:ValueRangeProperty
        rdf:type         owl:Class;
        rdfs:comment     "A custom property with a value range. (see KBLFRM-319)\n"@en;
        rdfs:label       "ValueRangeProperty"@en;
        rdfs:subClassOf  vec:CustomProperty .

vec:LanguageCode_Bn  rdf:type  vec:LanguageCode , owl:NamedIndividiual;
        vec:enumLiteral  "Bn" .

vec:connectorHousingRoleConnectorHousingSpecification
        rdf:type      owl:ObjectProperty;
        rdfs:comment  "References the ConnectorHousingSpecification that is instanced by this ConnectorHousingRole.\n"@en;
        rdfs:domain   vec:ConnectorHousingRole;
        rdfs:label    "connectorHousingSpecification"@en;
        rdfs:range    vec:ConnectorHousingSpecification .

vec:LanguageCode_Sg  rdf:type  vec:LanguageCode , owl:NamedIndividiual;
        vec:enumLiteral  "Sg" .

vec:LanguageCode_Ji  rdf:type  vec:LanguageCode , owl:NamedIndividiual;
        vec:enumLiteral  "Ji" .

vec:usageNodeSpecificationUsageNodes
        rdf:type            owl:ObjectProperty;
        rdfs:comment        "Specifies the UsageNodes defined by this UsageNodeSpecification.\n"@en;
        rdfs:domain         vec:UsageNodeSpecification;
        rdfs:label          "usageNodes"@en;
        rdfs:range          vec:UsageNode;
        rdfs:subPropertyOf  vec:contains .

vec:routingSpecificationRouting
        rdf:type            owl:ObjectProperty;
        rdfs:comment        "Specifies the Routings described by the RoutingSpecification.\n"@en;
        rdfs:domain         vec:RoutingSpecification;
        rdfs:label          "routing"@en;
        rdfs:range          vec:Routing;
        rdfs:subPropertyOf  vec:contains .

vec:Mapping  rdf:type    owl:Class;
        rdfs:comment     "The Mapping defines the concrete mapping two parts aliased as A & B. For performance reasons the roles PartSideA and PartSideB are abbreviated to A & B.\n"@en;
        rdfs:label       "Mapping"@en;
        rdfs:subClassOf  vec:ExtendableElement .

vec:wireReceptionSpecificationSealable
        rdf:type      owl:DatatypeProperty;
        rdfs:comment  "Specifies if the wire reception can be sealed. (see KBLFRM-311)\n"@en;
        rdfs:domain   vec:WireReceptionSpecification;
        rdfs:label    "sealable"@en;
        rdfs:range    xs:boolean .

vec:wireElementReferenceSignal
        rdf:type      owl:ObjectProperty;
        rdfs:comment  "References the signal that is transmitted by the WireElementReference.\n"@en;
        rdfs:domain   vec:WireElementReference;
        rdfs:label    "signal"@en;
        rdfs:range    vec:Signal .

vec:Role  rdf:type       owl:Class;
        rdfs:comment     "A Role is the corresponding mechanism for OccurrenceOrUsages to the PartOrUsageRelatedSpecifcations for PartVersions or PartUsages. The PartOrUsageRelatedSpecifcations are describing a certain aspect of the master data of a part. A Role describes the corresponding properties and relationships for instances of a part (e.g. the usage specific properties of a wire occurrence like the length or the contacting).\n"@en;
        rdfs:label       "Role"@en;
        rdfs:subClassOf  vec:ExtendableElement .

vec:pinCurrentInformationCurrent
        rdf:type            owl:ObjectProperty;
        rdfs:comment        "The current of the pin.\n"@en;
        rdfs:domain         vec:PinCurrentInformation;
        rdfs:label          "current"@en;
        rdfs:range          vec:NumericalValue;
        rdfs:subPropertyOf  vec:contains .

vec:PinTimingType_InitTime
        rdf:type         vec:PinTimingType , owl:NamedIndividiual;
        vec:enumLiteral  "initTime" .

vec:PrimaryPartType_HoleMountedFixing
        rdf:type         vec:PrimaryPartType , owl:NamedIndividiual;
        vec:enumLiteral  "HoleMountedFixing" .

vec:localizedStringPropertyValue
        rdf:type            owl:ObjectProperty;
        rdfs:comment        "Defines the value of the CustomProperty.\n"@en;
        rdfs:domain         vec:LocalizedStringProperty;
        rdfs:label          "value"@en;
        rdfs:range          vec:LocalizedString;
        rdfs:subPropertyOf  vec:contains .

vec:geometrySegment3DEndNode
        rdf:type      owl:ObjectProperty;
        rdfs:comment  "References the GeometryNode3D where the GeometrySegment3D ends. \n"@en;
        rdfs:domain   vec:GeometrySegment3D;
        rdfs:label    "endNode"@en;
        rdfs:range    vec:GeometryNode3D .

vec:SignalCurve_ContinuousSignal
        rdf:type         vec:SignalCurve , owl:NamedIndividiual;
        vec:enumLiteral  "continuousSignal" .

vec:PrimaryPartType  rdf:type  owl:Class;
        rdfs:comment         "The primary type of the part defines the type of the part (e.g. ConnectorHousing, Fixing, etc.) Since the VEC supports dual use parts (e.g. Fixing & WireProtection) the primary part type is necessary to define which specification associated to part is the primary character of the part. Therefore all primary part types correspond to a PartOrUsageRelatedSpecification (e.g. ConnectorHousing --> ConnectorHousingSpecification).\nThe primary part type 'Other' is used if the PartVersion is not further specified by the VEC, which means it has no PartOrUsageRelatedSpecification, only a GeneralTechnicalPartSpecification or a direct instance of PartOrUsageRelatedSpecification.\n"@en;
        rdfs:label           "PrimaryPartType"@en;
        rdfs:subClassOf      vec:ClosedEnumeration;
        owl:equivalentClass  [ rdf:type   owl:Class;
                               owl:oneOf  ( vec:PrimaryPartType_Antenna vec:PrimaryPartType_Battery vec:PrimaryPartType_BoltMountedFixing vec:PrimaryPartType_CableDuct vec:PrimaryPartType_CavityPlug vec:PrimaryPartType_CavitySeal vec:PrimaryPartType_ConnectorHousing vec:PrimaryPartType_CorrugatedPipe vec:PrimaryPartType_EEComponent vec:PrimaryPartType_Fitting vec:PrimaryPartType_Fixing vec:PrimaryPartType_Fuse vec:PrimaryPartType_Grommet vec:PrimaryPartType_HoleMountedFixing vec:PrimaryPartType_MultiCavityPlug vec:PrimaryPartType_MultiCavitySeal vec:PrimaryPartType_Other vec:PrimaryPartType_PartStructure vec:PrimaryPartType_PluggableTerminal vec:PrimaryPartType_Relay vec:PrimaryPartType_RingTerminal vec:PrimaryPartType_ShrinkableTube vec:PrimaryPartType_SpliceTerminal vec:PrimaryPartType_Stripe vec:PrimaryPartType_Tape vec:PrimaryPartType_Terminal vec:PrimaryPartType_Tube vec:PrimaryPartType_Wire vec:PrimaryPartType_WireProtection )
                             ] .

vec:ContractRole_Manufacturer
        rdf:type         vec:ContractRole , owl:NamedIndividiual;
        vec:enumLiteral  "Manufacturer" .

vec:pinOpticalInformationAttenuation
        rdf:type            owl:ObjectProperty;
        rdfs:comment        "The attenuation of the optical pin at the defined frequency.\n"@en;
        rdfs:domain         vec:PinOpticalInformation;
        rdfs:label          "attenuation"@en;
        rdfs:range          vec:NumericalValue;
        rdfs:subPropertyOf  vec:contains .

vec:pinComponentDescription
        rdf:type            owl:ObjectProperty;
        rdfs:comment        "Specifies additional, human readable information about the PinComponent .\n"@en;
        rdfs:domain         vec:PinComponent;
        rdfs:label          "description"@en;
        rdfs:range          vec:AbstractLocalizedString;
        rdfs:subPropertyOf  vec:contains .

vec:FixingSpecification
        rdf:type         owl:Class;
        rdfs:comment     "Specification for the definition of fixings. A fixing is used to fix the harness in a certain position (e.g. at the car body, a seat, an ECU etc.). The FixingSpecification describes how the fixing is attached to the \"non-harness\" element. The attachment to harness is described by a PlaceableElementSpecification.\n"@en;
        rdfs:label       "FixingSpecification"@en;
        rdfs:subClassOf  vec:PartOrUsageRelatedSpecification .

vec:connectionEndIsExternalEnd
        rdf:type      owl:DatatypeProperty;
        rdfs:comment  "Specifies if the ConnectionEnd is connected to the internal or the external side of the ComponentPort.\n"@en;
        rdfs:domain   vec:ConnectionEnd;
        rdfs:label    "isExternalEnd"@en;
        rdfs:range    xs:boolean .

vec:PrimaryPartType_Tape
        rdf:type         vec:PrimaryPartType , owl:NamedIndividiual;
        vec:enumLiteral  "Tape" .

vec:USUnitName_Furlong
        rdf:type         vec:USUnitName , owl:NamedIndividiual;
        vec:enumLiteral  "Furlong" .

vec:SiUnitName_Gram  rdf:type  vec:SiUnitName , owl:NamedIndividiual;
        vec:enumLiteral  "Gram" .

vec:PrimaryPartType_CavityPlug
        rdf:type         vec:PrimaryPartType , owl:NamedIndividiual;
        vec:enumLiteral  "CavityPlug" .

vec:placementPointReferencePlacementPoint
        rdf:type      owl:ObjectProperty;
        rdfs:comment  "References the PlacementPoint that is instanced by this PlacementPointReference.\n"@en;
        rdfs:domain   vec:PlacementPointReference;
        rdfs:label    "placementPoint"@en;
        rdfs:range    vec:PlacementPoint .

vec:topologyNodeRealizedUsageNode
        rdf:type      owl:ObjectProperty;
        rdfs:comment  "References the UsageNode that is realized by this TopologyNode .\n"@en;
        rdfs:domain   vec:TopologyNode;
        rdfs:label    "realizedUsageNode"@en;
        rdfs:range    vec:UsageNode .

vec:partOccurrencePart
        rdf:type      owl:ObjectProperty;
        rdfs:comment  "References the PartVersion that is instantiated by this PartOccurrence.\n"@en;
        rdfs:domain   vec:PartOccurrence;
        rdfs:label    "part"@en;
        rdfs:range    vec:PartVersion .

vec:PinVoltageInformation
        rdf:type      owl:Class;
        rdfs:comment  "Allows the definition of voltages for a pin of an EEComponent . A current can be further specified by a duration. Attributes of the type PinVoltageInformation normally have the multiplicity [0..*]. This means that such an attribute can have PinVoltageInformation entries for different types and durations. It must not have multiple entries for the same type and duration.\n"@en;
        rdfs:label    "PinVoltageInformation"@en .

vec:Placement  rdf:type  owl:Class;
        rdfs:comment     "A placement defines the placement of a PlaceableElementRole onto a Topology. For the definition of the place on the Topology, Locations are used. A Placement can either be a placement on discrete points (OnPointPlacement) or on an area of the topology (OnWayPlacement).\n"@en;
        rdfs:label       "Placement"@en;
        rdfs:subClassOf  vec:ConfigurableElement .

vec:abrasionResistanceClassReferenceSystem
        rdf:type      owl:DatatypeProperty;
        rdfs:comment  "The identification of the abrasion resistance class reference system, which is defining possible values and the semantic of abrasion resistance keys.\n"@en;
        rdfs:domain   vec:AbrasionResistanceClass;
        rdfs:label    "referenceSystem"@en;
        rdfs:range    xs:string .

vec:CavityReference  rdf:type  owl:Class;
        rdfs:comment     "A CavityReference represents the usage of a Cavity in the context of PartUsage or PartOccurrence.\n"@en;
        rdfs:label       "CavityReference"@en;
        rdfs:subClassOf  vec:ExtendableElement .

vec:terminalReceptionReferenceTerminalReception
        rdf:type      owl:ObjectProperty;
        rdfs:comment  "References the TerminalReception that is instanced by this TerminalReceptionReference.\n"@en;
        rdfs:domain   vec:TerminalReceptionReference;
        rdfs:label    "terminalReception"@en;
        rdfs:range    vec:TerminalReception .

vec:LanguageCode_Ur  rdf:type  vec:LanguageCode , owl:NamedIndividiual;
        vec:enumLiteral  "Ur" .

vec:PrimaryPartType_BoltMountedFixing
        rdf:type         vec:PrimaryPartType , owl:NamedIndividiual;
        vec:enumLiteral  "BoltMountedFixing" .

vec:segmentCrossSectionAreaCrossSectionAreaType
        rdf:type      owl:DatatypeProperty;
        rdfs:comment  "Specifies the type of the cross section area of the segment. Different types are for example needed to differentiate between the designed space of a segment and the actually needed space (e.g. calculated from the wires going through the segment). (see KBLFRM-303)\n"@en;
        rdfs:domain   vec:SegmentCrossSectionArea;
        rdfs:label    "crossSectionAreaType"@en;
        rdfs:range    xs:string .

vec:partVersionIsPreferredPart
        rdf:type      owl:DatatypeProperty;
        rdfs:comment  "Flags a part as \"preferred\" by the means of being a preferred part out of a group of parts with identical technical properties. The preferred part should be used, if the other properties of a couple of parts do not allow a distinct decision. (see KBLFRM-311)\n"@en;
        rdfs:domain   vec:PartVersion;
        rdfs:label    "isPreferredPart"@en;
        rdfs:range    xs:string .

vec:LanguageCode_Lt  rdf:type  vec:LanguageCode , owl:NamedIndividiual;
        vec:enumLiteral  "Lt" .

vec:segmentCrossSectionAreaValueDetermination
        rdf:type            owl:ObjectProperty;
        rdfs:comment        "Specifies the method for determination of the value.\n"@en;
        rdfs:domain         vec:SegmentCrossSectionArea;
        rdfs:label          "valueDetermination"@en;
        rdfs:range          vec:ValueDetermination;
        rdfs:subPropertyOf  vec:contains .

vec:wireReceptionPlacementPoint
        rdf:type      owl:ObjectProperty;
        rdfs:comment  "Specifies the PlacementPoint that represents this WireReception in a PlaceableElementSpecification.\n"@en;
        rdfs:domain   vec:WireReception;
        rdfs:label    "placementPoint"@en;
        rdfs:range    vec:PlacementPoint .

vec:BoltMountedFixingSpecification
        rdf:type         owl:Class;
        rdfs:comment     "Specification for fixings that are mounted with a bolt. This means, the fixing itself has got a bolt, which is mounted into a hole.\n"@en;
        rdfs:label       "BoltMountedFixingSpecification"@en;
        rdfs:subClassOf  vec:FixingSpecification .

vec:AnchorType_FromEndNode
        rdf:type         vec:AnchorType , owl:NamedIndividiual;
        rdfs:comment     "The offset of the location is measured from the endNode of the TopologySegment.\n"@en;
        vec:enumLiteral  "FromEndNode" .

vec:IECPrefix_Zebi  rdf:type  vec:IECPrefix , owl:NamedIndividiual;
        vec:enumLiteral  "Zebi" .

vec:LanguageCode_To  rdf:type  vec:LanguageCode , owl:NamedIndividiual;
        vec:enumLiteral  "To" .

vec:specificRoleSpecificRoleType
        rdf:type      owl:DatatypeProperty;
        rdfs:comment  "Specifies the type for role.\n"@en;
        rdfs:domain   vec:SpecificRole;
        rdfs:label    "specificRoleType"@en;
        rdfs:range    xs:string .

vec:ValueDetermination_Measured
        rdf:type         vec:ValueDetermination , owl:NamedIndividiual;
        rdfs:comment     "The value is determined by an exact measurement.\n"@en;
        vec:enumLiteral  "Measured" .

vec:componentNodeComponentPort
        rdf:type            owl:ObjectProperty;
        rdfs:comment        "Specifies the ComponentPorts of the ComponentNode.\n"@en;
        rdfs:domain         vec:ComponentNode;
        rdfs:label          "componentPort"@en;
        rdfs:range          vec:ComponentPort;
        rdfs:subPropertyOf  vec:contains .

vec:insulationSpecificationBaseColor
        rdf:type            owl:ObjectProperty;
        rdfs:comment        "Specifies the base color of the insulation.\n"@en;
        rdfs:domain         vec:InsulationSpecification;
        rdfs:label          "baseColor"@en;
        rdfs:range          vec:Color;
        rdfs:subPropertyOf  vec:contains .

vec:cableDuctRoleCableDuctSpecification
        rdf:type      owl:ObjectProperty;
        rdfs:comment  "References the CableDuctSpecification that is instanced by this CableDuctRole.\n"@en;
        rdfs:domain   vec:CableDuctRole;
        rdfs:label    "cableDuctSpecification"@en;
        rdfs:range    vec:CableDuctSpecification .

vec:LanguageCode_Sl  rdf:type  vec:LanguageCode , owl:NamedIndividiual;
        vec:enumLiteral  "Sl" .

vec:SiPrefix_Deci  rdf:type  vec:SiPrefix , owl:NamedIndividiual;
        vec:enumLiteral  "Deci" .

vec:extendableElementCustomProperty
        rdf:type            owl:ObjectProperty;
        rdfs:comment        "Specifies the CustomProperties of the ExtendableElement. \n"@en;
        rdfs:domain         vec:ExtendableElement;
        rdfs:label          "customProperty"@en;
        rdfs:range          vec:CustomProperty;
        rdfs:subPropertyOf  vec:contains .

vec:spliceTerminalRoleSpliceType
        rdf:type            owl:ObjectProperty;
        rdfs:comment        "Specifies the type of splice (inline, end).\n"@en;
        rdfs:domain         vec:SpliceTerminalRole;
        rdfs:label          "spliceType"@en;
        rdfs:range          vec:SpliceType;
        rdfs:subPropertyOf  vec:contains .

vec:partVersionPrimaryPartType
        rdf:type            owl:ObjectProperty;
        rdfs:comment        "The primary type of the part defines the type of the part (e.g. ConnectorHousing, Fixing, etc.) Since the VEC supports dual use parts (e.g. Fixing & WireProtection) the primary part type is necessary to define which specification associated to part is the primary character of the part. Therefore all primary part types correspond to a PartOrUsageRelatedSpecification (e.g. ConnectorHousing --> ConnectorHousingSpecification).\n"@en;
        rdfs:domain         vec:PartVersion;
        rdfs:label          "primaryPartType"@en;
        rdfs:range          vec:PrimaryPartType;
        rdfs:subPropertyOf  vec:contains .

vec:LanguageCode_Ik  rdf:type  vec:LanguageCode , owl:NamedIndividiual;
        vec:enumLiteral  "Ik" .

vec:buildingBlockSpecification3DBaseUnit
        rdf:type      owl:ObjectProperty;
        rdfs:comment  ""@en;
        rdfs:domain   vec:BuildingBlockSpecification3D;
        rdfs:label    "baseUnit"@en;
        rdfs:range    vec:Unit .

vec:SignalInformationType_Analog
        rdf:type         vec:SignalInformationType , owl:NamedIndividiual;
        vec:enumLiteral  "analog" .

vec:slotLayoutGridY  rdf:type  owl:ObjectProperty;
        rdfs:comment        "The vertical distance between the center points of two cavities.\n"@en;
        rdfs:domain         vec:SlotLayout;
        rdfs:label          "gridY"@en;
        rdfs:range          vec:NumericalValue;
        rdfs:subPropertyOf  vec:contains .

vec:batterySpecificationI
        rdf:type            owl:ObjectProperty;
        rdfs:comment        "Specifies the current the battery provides.\n"@en;
        rdfs:domain         vec:BatterySpecification;
        rdfs:label          "i"@en;
        rdfs:range          vec:NumericalValue;
        rdfs:subPropertyOf  vec:contains .

vec:ConnectionEnd  rdf:type  owl:Class;
        rdfs:comment     "A connection end is the end of a Connection at a ComponentPort.\n"@en;
        rdfs:label       "ConnectionEnd"@en;
        rdfs:subClassOf  vec:ConfigurableElement .

vec:wireReceptionSpecificationInsulationDisplacementLength
        rdf:type            owl:ObjectProperty;
        rdfs:comment        "Specifies the length of the insulation which must be stripped off to fit to this wire reception.\n"@en;
        rdfs:domain         vec:WireReceptionSpecification;
        rdfs:label          "insulationDisplacementLength"@en;
        rdfs:range          vec:NumericalValue;
        rdfs:subPropertyOf  vec:contains .

vec:compatibilityStatementCavity
        rdf:type      owl:ObjectProperty;
        rdfs:comment  "References explicit cavities for which the compatibility statement is stated.\n"@en;
        rdfs:domain   vec:CompatibilityStatement;
        rdfs:label    "cavity"@en;
        rdfs:range    vec:Cavity .

vec:OccurrenceOrUsageViewItem2D
        rdf:type         owl:Class;
        rdfs:comment     "An OccurrenceOrUsageViewItem2D specifies the representation of a OcurrenceOrUsage in a 2DDrawing.\n"@en;
        rdfs:label       "OccurrenceOrUsageViewItem2D"@en;
        rdfs:subClassOf  vec:ExtendableElement .

[ rdf:type     owl:AllDisjointClasses;
  owl:members  ( vec:PartWithSubComponentsRole vec:SpecificRole vec:CavityPlugRole vec:CavitySealRole vec:ConnectorHousingRole vec:EEComponentRole vec:TerminalRole vec:WireRole vec:FixingRole vec:GrommetRole vec:WireProtectionRole vec:CableDuctRole vec:PlaceableElementRole )
] .

vec:customPropertyPropertyType
        rdf:type     owl:DatatypeProperty;
        rdfs:domain  vec:CustomProperty;
        rdfs:label   "propertyType"@en;
        rdfs:range   xs:string .

vec:CavityPlugRole  rdf:type  owl:Class;
        rdfs:comment     "A CavityPlugRole defines the instance specific properties and relationships of a cavity plug.\n"@en;
        rdfs:label       "CavityPlugRole"@en;
        rdfs:subClassOf  vec:Role .

vec:changeDescriptionRelatedChangeRequest
        rdf:type      owl:DatatypeProperty;
        rdfs:comment  "Specifies the identification of a corresponding changeRequest. (see KBLFRM-249)\n"@en;
        rdfs:domain   vec:ChangeDescription;
        rdfs:label    "relatedChangeRequest"@en;
        rdfs:range    xs:string .

vec:changeDescriptionApprover
        rdf:type            owl:ObjectProperty;
        rdfs:comment        "Specifies the person who has approved the change.\n"@en;
        rdfs:domain         vec:ChangeDescription;
        rdfs:label          "approver"@en;
        rdfs:range          vec:Person;
        rdfs:subPropertyOf  vec:contains .

vec:PartRelationType_Optional
        rdf:type         vec:PartRelationType , owl:NamedIndividiual;
        rdfs:comment     " Optional means that in a usage of a component some referenced acessoryParts can be used by choice.\n"@en;
        vec:enumLiteral  "Optional" .

vec:PartOccurrence  rdf:type  owl:Class;
        rdfs:comment     "A PartOccurrence is an instance of a component with a specified part number (PartVersion).\n"@en;
        rdfs:label       "PartOccurrence"@en;
        rdfs:subClassOf  vec:OccurrenceOrUsage .

vec:wireGroupingIdentification
        rdf:type      owl:DatatypeProperty;
        rdfs:comment  "Specifies a unique identification of the WireGrouping. The identification is guaranteed to be unique within the WireGroupingSpecification.\n"@en;
        rdfs:domain   vec:WireGrouping;
        rdfs:label    "identification"@en;
        rdfs:range    xs:string .

vec:tubeSpecificationWallThickness
        rdf:type            owl:ObjectProperty;
        rdfs:comment        "Specifies the thickness of the wall of the tube.\n"@en;
        rdfs:domain         vec:TubeSpecification;
        rdfs:label          "wallThickness"@en;
        rdfs:range          vec:NumericalValue;
        rdfs:subPropertyOf  vec:contains .

vec:PinApplianceType  rdf:type  owl:Class;
        rdfs:comment     "Defines the appliance type of a pin.\n"@en;
        rdfs:label       "PinApplianceType"@en;
        rdfs:subClassOf  vec:OpenEnumeration .

vec:specificRoleSpecification
        rdf:type      owl:ObjectProperty;
        rdfs:comment  "References the PartOrUsageRelatedSpecification that is instantiated by this SpecificRole.\n"@en;
        rdfs:domain   vec:SpecificRole;
        rdfs:label    "specification"@en;
        rdfs:range    vec:PartOrUsageRelatedSpecification .

vec:wireProtectionSpecificationAbrasionResistanceClass
        rdf:type            owl:ObjectProperty;
        rdfs:comment        "Specifies the abrasion resistance class of the wire protection. According to the VDA this is a value between A & G.\nKBLFRM-311\n"@en;
        rdfs:domain         vec:WireProtectionSpecification;
        rdfs:label          "abrasionResistanceClass"@en;
        rdfs:range          vec:AbrasionResistanceClass;
        rdfs:subPropertyOf  vec:contains .

vec:Net  rdf:type        owl:Class;
        rdfs:comment     "A Net is an undirected connection between a number of NetworkPorts.\n"@en;
        rdfs:label       "Net"@en;
        rdfs:subClassOf  vec:ConfigurableElement .

vec:copyrightInformationCopyrightNote
        rdf:type            owl:ObjectProperty;
        rdfs:comment        "An informal text which specifies copyright information.\n"@en;
        rdfs:domain         vec:CopyrightInformation;
        rdfs:label          "copyrightNote"@en;
        rdfs:range          vec:LocalizedString;
        rdfs:subPropertyOf  vec:contains .

vec:USUnitName_AWG  rdf:type  vec:USUnitName , owl:NamedIndividiual;
        rdfs:comment     "American wire gauge (AWG), also known as the Brown & Sharpe wire gauge, is a standardized wire gauge system used in the United States and Canada.\n"@en;
        vec:enumLiteral  "AWG" .

vec:wireElementReferenceConnection
        rdf:type      owl:ObjectProperty;
        rdfs:comment  "References the Connection that is realized by the referenced WireElement (WireElementReference).\nKBLFRM-341\n"@en;
        rdfs:domain   vec:WireElementReference;
        rdfs:label    "connection"@en;
        rdfs:range    vec:Connection .

vec:vecContentPartVersion
        rdf:type            owl:ObjectProperty;
        rdfs:comment        "Specifies the PartVersions contained in the VEC-file. \n"@en;
        rdfs:domain         vec:VecContent;
        rdfs:label          "partVersion"@en;
        rdfs:range          vec:PartVersion;
        rdfs:subPropertyOf  vec:contains .

vec:creationCreationDate
        rdf:type      owl:DatatypeProperty;
        rdfs:comment  "Specifies the date when the associated ItemVersion was created. (see KBLFRM-241)\n"@en;
        rdfs:domain   vec:Creation;
        rdfs:label    "creationDate"@en;
        rdfs:range    xs:dateTime .

vec:slotSpecificationNumberOfCavities
        rdf:type      owl:DatatypeProperty;
        rdfs:comment  "The possible number of cavities in the layout defined by the SlotSpecification. This includes all cavities in the layout. The actual Slot can define specific cavities in the layout as \"not available\".\n"@en;
        rdfs:domain   vec:SlotSpecification;
        rdfs:label    "numberOfCavities"@en;
        rdfs:range    xs:integer .

vec:LanguageCode_Tt  rdf:type  vec:LanguageCode , owl:NamedIndividiual;
        vec:enumLiteral  "Tt" .

vec:SegmentForm_NonCircular
        rdf:type         vec:SegmentForm , owl:NamedIndividiual;
        vec:enumLiteral  "NonCircular" .

vec:ContractRole_Oem  rdf:type  vec:ContractRole , owl:NamedIndividiual;
        vec:enumLiteral  "Oem" .

vec:variantGroupIdentification
        rdf:type      owl:DatatypeProperty;
        rdfs:comment  "Specifies a unique identification of the variant code.\n"@en;
        rdfs:domain   vec:VariantGroup;
        rdfs:label    "identification"@en;
        rdfs:range    xs:string .

vec:occurrenceOrUsageViewItem3DAliasId
        rdf:type            owl:ObjectProperty;
        rdfs:comment        "Specifies additional identifiers for the OccurrenceOrUsageViewItem3D.\n"@en;
        rdfs:domain         vec:OccurrenceOrUsageViewItem3D;
        rdfs:label          "aliasId"@en;
        rdfs:range          vec:AliasIdentification;
        rdfs:subPropertyOf  vec:contains .

vec:wireMountingWireMountingDetail
        rdf:type            owl:ObjectProperty;
        rdfs:comment        "Specifies the WireMoutingDetails, if a detailed description of the relationships between WireEnds and WireReceptions is needed.\n"@en;
        rdfs:domain         vec:WireMounting;
        rdfs:label          "wireMountingDetail"@en;
        rdfs:range          vec:WireMountingDetail;
        rdfs:subPropertyOf  vec:contains .

vec:documentVersionDocumentNumber
        rdf:type      owl:DatatypeProperty;
        rdfs:comment  "The documentNumber is the major identifier of a DocumentVersion. The format is user defined and respectively company specific. Over all VEC-documents a DocumentVersion-instance can be trusted to be identical if the combination of documentNumber, documentVersion and companyName is identical.\n"@en;
        rdfs:domain   vec:DocumentVersion;
        rdfs:label    "documentNumber"@en;
        rdfs:range    xs:string .

vec:sealedCavitiesAssignmentSealedCavities
        rdf:type      owl:ObjectProperty;
        rdfs:comment  "Specifies the Cavities that are sealed.\n"@en;
        rdfs:domain   vec:SealedCavitiesAssignment;
        rdfs:label    "sealedCavities"@en;
        rdfs:range    vec:Cavity .

vec:LanguageCode_Sq  rdf:type  vec:LanguageCode , owl:NamedIndividiual;
        vec:enumLiteral  "Sq" .

vec:cavitySpecificationPrimaryLockingType
        rdf:type      owl:DatatypeProperty;
        rdfs:comment  "Specifies if the cavity has a primary locking and of what type it is.\n"@en;
        rdfs:domain   vec:CavitySpecification;
        rdfs:label    "primaryLockingType"@en;
        rdfs:range    xs:string .

vec:partOccurrenceRealizedPartUsage
        rdf:type      owl:ObjectProperty;
        rdfs:comment  "References the PartUsage that is realized by the PartOccurrence. \n"@en;
        rdfs:domain   vec:PartOccurrence;
        rdfs:label    "realizedPartUsage"@en;
        rdfs:range    vec:PartUsage .

vec:netGroupDescription
        rdf:type            owl:ObjectProperty;
        rdfs:comment        "Room for additional, human readable information about the NetGroup.\n"@en;
        rdfs:domain         vec:NetGroup;
        rdfs:label          "description"@en;
        rdfs:range          vec:AbstractLocalizedString;
        rdfs:subPropertyOf  vec:contains .

vec:moduleFamilyIdentification
        rdf:type      owl:DatatypeProperty;
        rdfs:comment  "Specifies a unique identification of the ModuleFamily. The identification is guaranteed to be unique within the ModuleFamilySpecification. Over all VEC-documents a ModuleFamily-instance can be trusted to be the same if the ModuleFamilySpecification-instance is the same and the identification of the ModuleFamily is the same.\n"@en;
        rdfs:domain   vec:ModuleFamily;
        rdfs:label    "identification"@en;
        rdfs:range    xs:string .

vec:grommetSpecificationPlateThickness
        rdf:type            owl:ObjectProperty;
        rdfs:comment        "Specifies valid the plate thickness at the hole into which the grommet fits.\n"@en;
        rdfs:domain         vec:GrommetSpecification;
        rdfs:label          "plateThickness"@en;
        rdfs:range          vec:ValueRange;
        rdfs:subPropertyOf  vec:contains .

vec:LanguageCode_Rn  rdf:type  vec:LanguageCode , owl:NamedIndividiual;
        vec:enumLiteral  "Rn" .

vec:CavityMapping  rdf:type  owl:Class;
        rdfs:comment  "Defines the mapping of two cavities contained Slot A & B of the containing SlotMapping-object.\n"@en;
        rdfs:label    "CavityMapping"@en .

vec:LanguageCode_Zi  rdf:type  vec:LanguageCode , owl:NamedIndividiual;
        vec:enumLiteral  "Zi" .

vec:SiUnitName_DegreeCelsius
        rdf:type         vec:SiUnitName , owl:NamedIndividiual;
        vec:enumLiteral  "DegreeCelsius" .

vec:stripeSpecificationLength
        rdf:type            owl:ObjectProperty;
        rdfs:comment        "Specifies the length of the stripe.\n"@en;
        rdfs:domain         vec:StripeSpecification;
        rdfs:label          "length"@en;
        rdfs:range          vec:NumericalValue;
        rdfs:subPropertyOf  vec:contains .

vec:Path  rdf:type       owl:Class;
        rdfs:comment     "Describes a path in the topology. A Path is a continuous way through a topology without interruptions, defined by an ordered list of TopologySegments .\n"@en;
        rdfs:label       "Path"@en;
        rdfs:subClassOf  vec:ConfigurableElement .

vec:networkNodeRealizedUsageNode
        rdf:type      owl:ObjectProperty;
        rdfs:comment  "References the UsageNode that is realized by this NetworkNode .\n"@en;
        rdfs:domain   vec:NetworkNode;
        rdfs:label    "realizedUsageNode"@en;
        rdfs:range    vec:UsageNode .

vec:topologySegmentLengthInformation
        rdf:type            owl:ObjectProperty;
        rdfs:comment        "Specifies the different SegmentLengths of the TopologySegment. \n"@en;
        rdfs:domain         vec:TopologySegment;
        rdfs:label          "lengthInformation"@en;
        rdfs:range          vec:SegmentLength;
        rdfs:subPropertyOf  vec:contains .

vec:vecContentGeneratingSystemName
        rdf:type      owl:DatatypeProperty;
        rdfs:comment  "Specifies the name of the system that has generated the VEC-file.\n"@en;
        rdfs:domain   vec:VecContent;
        rdfs:label    "generatingSystemName"@en;
        rdfs:range    xs:string .

vec:usageConstraintToSerialNumber
        rdf:type      owl:DatatypeProperty;
        rdfs:comment  "Specifies the upper bound of a serial number range to which the usage constraint applies.\n"@en;
        rdfs:domain   vec:UsageConstraint;
        rdfs:label    "toSerialNumber"@en;
        rdfs:range    xs:string .

vec:documentVersionDataFormat
        rdf:type      owl:DatatypeProperty;
        rdfs:comment  "The dataFormat specifies the convention that was used to structure the information in the document. This is useful if the DocumentVersion is actually a pointer to an external document, which is not contained in the VEC or if the content of this DocumentVersion was automatically generated by the extraction of the information out of the original document.\n"@en;
        rdfs:domain   vec:DocumentVersion;
        rdfs:label    "dataFormat"@en;
        rdfs:range    xs:string .

vec:netSignal  rdf:type  owl:ObjectProperty;
        rdfs:comment  "References the Signal that is transmitted by the Net .\n"@en;
        rdfs:domain   vec:Net;
        rdfs:label    "signal"@en;
        rdfs:range    vec:Signal .

vec:cartesianVector3DY
        rdf:type      owl:DatatypeProperty;
        rdfs:comment  "Specifies the y-coordinate in 3D space.\n"@en;
        rdfs:domain   vec:CartesianVector3D;
        rdfs:label    "y"@en;
        rdfs:range    xs:double .

vec:CableLeadThrough  rdf:type  owl:Class;
        rdfs:comment     "A CableLeadThrough specifies a hole in the grommet through which wires can pass through the grommet.\n"@en;
        rdfs:label       "CableLeadThrough"@en;
        rdfs:subClassOf  vec:ExtendableElement .

vec:componentNodeRealizedUsageNode
        rdf:type      owl:ObjectProperty;
        rdfs:comment  "References the UsageNode that is realized by this ComponentNode .\n"@en;
        rdfs:domain   vec:ComponentNode;
        rdfs:label    "realizedUsageNode"@en;
        rdfs:range    vec:UsageNode .

vec:SiUnitName_Tesla  rdf:type  vec:SiUnitName , owl:NamedIndividiual;
        vec:enumLiteral  "Tesla" .

vec:compatibilityStatementCavitySpecification
        rdf:type      owl:ObjectProperty;
        rdfs:comment  "References the CavitySpecifications for which the compatibility statement is stated.\n"@en;
        rdfs:domain   vec:CompatibilityStatement;
        rdfs:label    "cavitySpecification"@en;
        rdfs:range    vec:CavitySpecification .

vec:SiUnitName_Volt  rdf:type  vec:SiUnitName , owl:NamedIndividiual;
        vec:enumLiteral  "Volt" .

vec:approvalCompanyInScope
        rdf:type      owl:DatatypeProperty;
        rdfs:comment  "Room to specify for which companies the Approval is valid. It might be e.g. that an approved Item may only be delivered by some specific company.\n"@en;
        rdfs:domain   vec:Approval;
        rdfs:label    "companyInScope"@en;
        rdfs:range    xs:string .

vec:partStructureSpecificationInBillOfMaterial
        rdf:type      owl:ObjectProperty;
        rdfs:comment  "References the PartOccurrences that are building the bill of material of a composite part.\n"@en;
        rdfs:domain   vec:PartStructureSpecification;
        rdfs:label    "inBillOfMaterial"@en;
        rdfs:range    vec:PartOccurrence .

vec:antennaSpecificationFMin
        rdf:type            owl:ObjectProperty;
        rdfs:comment        "Specifies the minimum operating frequency of the antenna.\n"@en;
        rdfs:domain         vec:AntennaSpecification;
        rdfs:label          "fMin"@en;
        rdfs:range          vec:NumericalValue;
        rdfs:subPropertyOf  vec:contains .

vec:partRelationAccessoryPart
        rdf:type            owl:ObjectProperty;
        rdfs:comment        "This association is defined as unique='false' and ordered='false'. This can not be represented efficiently directly in RDF/OWL. Therefore, this association references Wrappers as proxies to the actual elements, instead of the actual elements itself (like a regular association)." , "References the PartVersions that are related by the PartRelation. \n"@en;
        rdfs:domain         vec:PartRelation;
        rdfs:label          "accessoryPart"@en;
        rdfs:range          vec:PartVersionWrapper;
        rdfs:subPropertyOf  vec:contains .

vec:cavityPlugSpecificationCavityDiameter
        rdf:type            owl:ObjectProperty;
        rdfs:comment        "Specifies a range of valid cavity diameters to which the cavity plug fits.\n"@en;
        rdfs:domain         vec:CavityPlugSpecification;
        rdfs:label          "cavityDiameter"@en;
        rdfs:range          vec:ValueRange;
        rdfs:subPropertyOf  vec:contains .

vec:USUnitName_Perch  rdf:type  vec:USUnitName , owl:NamedIndividiual;
        vec:enumLiteral  "Perch" .

vec:cavitySpecificationCavityDiameter
        rdf:type            owl:ObjectProperty;
        rdfs:comment        "Specifies the diameter of the cavity.\n"@en;
        rdfs:domain         vec:CavitySpecification;
        rdfs:label          "cavityDiameter"@en;
        rdfs:range          vec:NumericalValue;
        rdfs:subPropertyOf  vec:contains .

vec:ImperialUnitName_Acre
        rdf:type         vec:ImperialUnitName , owl:NamedIndividiual;
        vec:enumLiteral  "Acre" .

vec:Instruction  rdf:type  owl:Class;
        rdfs:comment     "Abstract super class to specify different types of instructions. Possible instructions are text, file or document based.\n"@en;
        rdfs:label       "Instruction"@en;
        rdfs:subClassOf  vec:ExtendableElement .

vec:PinCurrentType_OverrunCurrent
        rdf:type         vec:PinCurrentType , owl:NamedIndividiual;
        vec:enumLiteral  "overrunCurrent" .

vec:buildingBlockSpecification2DBoundingBox
        rdf:type            owl:ObjectProperty;
        rdfs:comment        "Specifies the size of the area described by the BuildingBlockSpecification2D in Cartesian dimensions. \n"@en;
        rdfs:domain         vec:BuildingBlockSpecification2D;
        rdfs:label          "boundingBox"@en;
        rdfs:range          vec:CartesianDimension;
        rdfs:subPropertyOf  vec:contains .

vec:personAliasId  rdf:type  owl:ObjectProperty;
        rdfs:comment        "Specifies identifiers for the Person in different contexts.\n"@en;
        rdfs:domain         vec:Person;
        rdfs:label          "aliasId"@en;
        rdfs:range          vec:AliasIdentification;
        rdfs:subPropertyOf  vec:contains .

vec:Slot  rdf:type       owl:Class;
        rdfs:comment     "A slot is a group of cavities in a connector housing with own properties. The design of a slot is described in a SlotSpecification.\n"@en;
        rdfs:label       "Slot"@en;
        rdfs:subClassOf  vec:AbstractSlot .

vec:WireReceptionSpecification
        rdf:type         owl:Class;
        rdfs:comment     "Specification for the definition of wire receptions. A WireReception is the area of a terminal where the contacting with a (e.g. by crimping) takes place.\n"@en;
        rdfs:label       "WireReceptionSpecification"@en;
        rdfs:subClassOf  vec:Specification .

vec:conformanceClassVersion
        rdf:type      owl:DatatypeProperty;
        rdfs:comment  "Specifies the version of the conformance class.\n"@en;
        rdfs:domain   vec:ConformanceClass;
        rdfs:label    "version"@en;
        rdfs:range    xs:string .

vec:ringTerminalSpecificationTorsionProtection
        rdf:type      owl:DatatypeProperty;
        rdfs:comment  "Specifies if the ring terminal is torsion protected or not. (see KBLFRM-311)\n"@en;
        rdfs:domain   vec:RingTerminalSpecification;
        rdfs:label    "torsionProtection"@en;
        rdfs:range    xs:boolean .

vec:buildingBlockSpecification2DGeometryNode
        rdf:type            owl:ObjectProperty;
        rdfs:comment        "Specifies the GeometryNode2Ds defined by the BuildingBlockSpecification2D.\n"@en;
        rdfs:domain         vec:BuildingBlockSpecification2D;
        rdfs:label          "geometryNode"@en;
        rdfs:range          vec:GeometryNode2D;
        rdfs:subPropertyOf  vec:contains .

vec:shrinkableTubeSpecificationResin
        rdf:type            owl:ObjectProperty;
        rdfs:comment        "Defines the material of the resin usable for this shrinkable tube.\n"@en;
        rdfs:domain         vec:ShrinkableTubeSpecification;
        rdfs:label          "resin"@en;
        rdfs:range          vec:Material;
        rdfs:subPropertyOf  vec:contains .

vec:LanguageCode_Da  rdf:type  vec:LanguageCode , owl:NamedIndividiual;
        vec:enumLiteral  "Da" .

vec:wireElementSpecificationMinBendRadiusDynamic
        rdf:type            owl:ObjectProperty;
        rdfs:comment        "Specifies the minimum bend radius for wire element, if it is used in a dynamic environment, where it is bended repeatedly (e.g in grommet of the back door). (see KLBFRM-311)\n"@en;
        rdfs:domain         vec:WireElementSpecification;
        rdfs:label          "minBendRadiusDynamic"@en;
        rdfs:range          vec:NumericalValue;
        rdfs:subPropertyOf  vec:contains .

vec:SiPrefix_Mega  rdf:type  vec:SiPrefix , owl:NamedIndividiual;
        vec:enumLiteral  "Mega" .

vec:PartStructureSpecification
        rdf:type         owl:Class;
        rdfs:comment     "Specification for the description of a part structure. This specification defines what PartOccurrences are actually in the bill of material of the described PartOrUsage. This is necessary, because it possible, that for a definite description a Part more PartOccurrences are needed than the ones that are in the bill of material (see CompositionSpecification).\n"@en;
        rdfs:label       "PartStructureSpecification"@en;
        rdfs:subClassOf  vec:PartOrUsageRelatedSpecification .

vec:PinVoltageType  rdf:type  owl:Class;
        rdfs:comment     "Defines the different available voltage types of a pin.\n"@en;
        rdfs:label       "PinVoltageType"@en;
        rdfs:subClassOf  vec:OpenEnumeration .

vec:IECPrefix_Tebi  rdf:type  vec:IECPrefix , owl:NamedIndividiual;
        vec:enumLiteral  "Tebi" .

vec:GeometryType_Dmu  rdf:type  vec:GeometryType , owl:NamedIndividiual;
        rdfs:comment     "The Geometry is a DMU model of the vehicle.\n"@en;
        vec:enumLiteral  "Dmu" .

vec:LanguageCode_Sv  rdf:type  vec:LanguageCode , owl:NamedIndividiual;
        vec:enumLiteral  "Sv" .

vec:networkNodeNetworkNodeType
        rdf:type      owl:DatatypeProperty;
        rdfs:comment  "Specifies the type of a NetworkNode. Appropriate values should be defined in a conformance class.\n"@en;
        rdfs:domain   vec:NetworkNode;
        rdfs:label    "networkNodeType"@en;
        rdfs:range    xs:string .

vec:PinVoltageType_MinVoltage
        rdf:type         vec:PinVoltageType , owl:NamedIndividiual;
        vec:enumLiteral  "minVoltage" .

vec:WireLength  rdf:type  owl:Class;
        rdfs:comment     "Defines the length of a WireElementReference. A WireElementReference can have multiple lengths of different types, but must not have more than one length of the same type.\n"@en;
        rdfs:label       "WireLength"@en;
        rdfs:subClassOf  vec:ExtendableElement .

vec:permissionPermissionDate
        rdf:type      owl:DatatypeProperty;
        rdfs:comment  "Specifies the date when the permission was stated.\n"@en;
        rdfs:domain   vec:Permission;
        rdfs:label    "permissionDate"@en;
        rdfs:range    xs:dateTime .

vec:projectCarClassificationLevel3
        rdf:type      owl:DatatypeProperty;
        rdfs:comment  "Provides a classification according to \"CC8 Recommended Practices Specification and Configuration, Product Structures\". Car classification is the identification of a set of similar cars to be offered to the market. Level 3 stands for \"Configuration information / product family\" where all variant control mechanism are attached.\n"@en;
        rdfs:domain   vec:Project;
        rdfs:label    "carClassificationLevel3"@en;
        rdfs:range    xs:string .

vec:SiUnitName_Lux  rdf:type  vec:SiUnitName , owl:NamedIndividiual;
        vec:enumLiteral  "Lux" .

vec:LanguageCode_Az  rdf:type  vec:LanguageCode , owl:NamedIndividiual;
        vec:enumLiteral  "Az" .

vec:PrimaryPartType_PartStructure
        rdf:type         vec:PrimaryPartType , owl:NamedIndividiual;
        vec:enumLiteral  "PartStructure" .

vec:eEComponentSpecificationPowerConsumption
        rdf:type            owl:ObjectProperty;
        rdfs:comment        "Specifies the PowerConsumptions of this EEComponentSpecification.\n"@en;
        rdfs:domain         vec:EEComponentSpecification;
        rdfs:label          "powerConsumption"@en;
        rdfs:range          vec:PowerConsumption;
        rdfs:subPropertyOf  vec:contains .

vec:SiUnitName_Steradian
        rdf:type         vec:SiUnitName , owl:NamedIndividiual;
        vec:enumLiteral  "Steradian" .

vec:LanguageCode_Iu  rdf:type  vec:LanguageCode , owl:NamedIndividiual;
        vec:enumLiteral  "Iu" .

vec:shrinkableTubeSpecificationShrinkingFactor
        rdf:type      owl:DatatypeProperty;
        rdfs:comment  "Defines the factor of shrinking for the tube.\n"@en;
        rdfs:domain   vec:ShrinkableTubeSpecification;
        rdfs:label    "shrinkingFactor"@en;
        rdfs:range    xs:double .

vec:fileBasedInstructionFileName
        rdf:type      owl:DatatypeProperty;
        rdfs:comment  "The name of the file.\n"@en;
        rdfs:domain   vec:FileBasedInstruction;
        rdfs:label    "fileName"@en;
        rdfs:range    xs:string .

vec:PrimaryPartType_Stripe
        rdf:type         vec:PrimaryPartType , owl:NamedIndividiual;
        vec:enumLiteral  "Stripe" .

vec:placeableElementSpecificationMeasurementPoint
        rdf:type            owl:ObjectProperty;
        rdfs:comment        "Specifies the MeasurementPoints of an PlaceableElement .\n"@en;
        rdfs:domain         vec:PlaceableElementSpecification;
        rdfs:label          "measurementPoint"@en;
        rdfs:range          vec:MeasurementPoint;
        rdfs:subPropertyOf  vec:contains .

vec:slotMappingCavityMapping
        rdf:type            owl:ObjectProperty;
        rdfs:comment        ""@en;
        rdfs:domain         vec:SlotMapping;
        rdfs:label          "cavityMapping"@en;
        rdfs:range          vec:CavityMapping;
        rdfs:subPropertyOf  vec:contains .

vec:segmentLengthClassification
        rdf:type            owl:ObjectProperty;
        rdfs:comment        "Specifies the classification of the segment length.\n"@en;
        rdfs:domain         vec:SegmentLength;
        rdfs:label          "classification"@en;
        rdfs:range          vec:LengthClassification;
        rdfs:subPropertyOf  vec:contains .

vec:zoneSubZone  rdf:type   owl:ObjectProperty;
        rdfs:comment        "Specifies the sub Zones that are part the Zone. \n"@en;
        rdfs:domain         vec:Zone;
        rdfs:label          "subZone"@en;
        rdfs:range          vec:Zone;
        rdfs:subPropertyOf  vec:contains .

vec:partWithSubComponentsRoleSubComponent
        rdf:type      owl:ObjectProperty;
        rdfs:comment  "References the subcomponents that belong to this instance of a PartWithSubComponents.\n"@en;
        rdfs:domain   vec:PartWithSubComponentsRole;
        rdfs:label    "subComponent"@en;
        rdfs:range    vec:OccurrenceOrUsage .

vec:LanguageCode_Hr  rdf:type  vec:LanguageCode , owl:NamedIndividiual;
        vec:enumLiteral  "Hr" .

vec:ModularSlotReference
        rdf:type         owl:Class;
        rdfs:comment     "A ModularSlotReference represents the usage of a ModularSlot in the context of PartUsage or PartOccurrence.\n"@en;
        rdfs:label       "ModularSlotReference"@en;
        rdfs:subClassOf  vec:AbstractSlotReference .

vec:connectionGroupDescription
        rdf:type            owl:ObjectProperty;
        rdfs:comment        "Room for additional, human readable information about the ConnectionGroup.\n"@en;
        rdfs:domain         vec:ConnectionGroup;
        rdfs:label          "description"@en;
        rdfs:range          vec:AbstractLocalizedString;
        rdfs:subPropertyOf  vec:contains .

vec:geometryNodeIdentification
        rdf:type      owl:DatatypeProperty;
        rdfs:comment  "Specifies a unique identification of the GeometryNode. The identification is guaranteed to be unique within the corresponding BuildingBlockSpecification. Over all VEC-documents a GeometryNode-instance can be trusted to be the same if the BuildingBlockSpecification-instance is the same (see BuildingBlockSpecification) and the identification of the GeometryNode is the same.\n"@en;
        rdfs:domain   vec:GeometryNode;
        rdfs:label    "identification"@en;
        rdfs:range    xs:string .

vec:LanguageCode_Xh  rdf:type  vec:LanguageCode , owl:NamedIndividiual;
        vec:enumLiteral  "Xh" .

vec:antennaSpecificationFMax
        rdf:type            owl:ObjectProperty;
        rdfs:comment        "Specifies the maximum operating frequency of the antenna.\n"@en;
        rdfs:domain         vec:AntennaSpecification;
        rdfs:label          "fMax"@en;
        rdfs:range          vec:NumericalValue;
        rdfs:subPropertyOf  vec:contains .

vec:SiPrefix  rdf:type       owl:Class;
        rdfs:comment         "Enumeration for the definition of SI unit prefixes.\n"@en;
        rdfs:label           "SiPrefix"@en;
        rdfs:subClassOf      vec:ClosedEnumeration;
        owl:equivalentClass  [ rdf:type   owl:Class;
                               owl:oneOf  ( vec:SiPrefix_Yotta vec:SiPrefix_Zetta vec:SiPrefix_Exa vec:SiPrefix_Peta vec:SiPrefix_Tera vec:SiPrefix_Giga vec:SiPrefix_Mega vec:SiPrefix_Kilo vec:SiPrefix_Hecto vec:SiPrefix_Deca vec:SiPrefix_Deci vec:SiPrefix_Centi vec:SiPrefix_Milli vec:SiPrefix_Micro vec:SiPrefix_Nano vec:SiPrefix_Pico vec:SiPrefix_Femto vec:SiPrefix_Atto vec:SiPrefix_Zepto vec:SiPrefix_Yocto )
                             ] .

vec:componentNodeDescription
        rdf:type            owl:ObjectProperty;
        rdfs:comment        "Room for additional, human readable information about the ComponentNode.\n"@en;
        rdfs:domain         vec:ComponentNode;
        rdfs:label          "description"@en;
        rdfs:range          vec:AbstractLocalizedString;
        rdfs:subPropertyOf  vec:contains .

vec:USUnitName_Chain  rdf:type  vec:USUnitName , owl:NamedIndividiual;
        vec:enumLiteral  "Chain" .

vec:USUnitName_Rood  rdf:type  vec:USUnitName , owl:NamedIndividiual;
        vec:enumLiteral  "Rood" .

vec:wireReceptionSpecificationMultiContact
        rdf:type      owl:DatatypeProperty;
        rdfs:comment  "Specifies if it is possible to contact more than core at the wire reception.\n"@en;
        rdfs:domain   vec:WireReceptionSpecification;
        rdfs:label    "multiContact"@en;
        rdfs:range    xs:boolean .

vec:cavitySpecificationAngle
        rdf:type            owl:ObjectProperty;
        rdfs:comment        "Specifies the angle against two planes of the connector housing a terminal used in this cavity can be buckled.\n"@en;
        rdfs:domain         vec:CavitySpecification;
        rdfs:label          "angle"@en;
        rdfs:range          vec:NumericalValue , vec:Ordered;
        rdfs:subPropertyOf  vec:contains .

vec:pathSegmentCurveRadius
        rdf:type            owl:ObjectProperty;
        rdfs:comment        "The radius of the curve which describes the appearance of the path segment.\n"@en;
        rdfs:domain         vec:PathSegment;
        rdfs:label          "curveRadius"@en;
        rdfs:range          vec:NumericalValue;
        rdfs:subPropertyOf  vec:contains .

vec:Creation  rdf:type   owl:Class;
        rdfs:comment     "A Creation-instance provides additional information to the owning ItemVersion stating personal information on the creator and the creation date.\n"@en;
        rdfs:label       "Creation"@en;
        rdfs:subClassOf  vec:ExtendableElement .

vec:openCavitiesAssignmentOpenCavities
        rdf:type      owl:ObjectProperty;
        rdfs:comment  "Specifies the cavities that are open.\n"@en;
        rdfs:domain   vec:OpenCavitiesAssignment;
        rdfs:label    "openCavities"@en;
        rdfs:range    vec:Cavity .

vec:parent  rdf:type   owl:ObjectProperty;
        rdfs:comment   "The inverse of 'contains'."@en;
        rdfs:label     "parent"@en;
        owl:inverseOf  vec:contains .

vec:SiUnitName_Becquerel
        rdf:type         vec:SiUnitName , owl:NamedIndividiual;
        vec:enumLiteral  "Becquerel" .

vec:generalTechnicalPartSpecificationMaterialInformation
        rdf:type            owl:ObjectProperty;
        rdfs:comment        "Specifies the material of a part.\n"@en;
        rdfs:domain         vec:GeneralTechnicalPartSpecification;
        rdfs:label          "materialInformation"@en;
        rdfs:range          vec:Material;
        rdfs:subPropertyOf  vec:contains .

vec:modularSlotOptional
        rdf:type      owl:DatatypeProperty;
        rdfs:comment  "Specifies whether the allocation of the ModularSlot is optional or not (can a usage of the connector housing leave this ModularSlot empty.\n"@en;
        rdfs:domain   vec:ModularSlot;
        rdfs:label    "optional"@en;
        rdfs:range    xs:boolean .

vec:matingDetailSecondTerminalReception
        rdf:type      owl:ObjectProperty;
        rdfs:comment  "References the second terminal reception that is mated.\n"@en;
        rdfs:domain   vec:MatingDetail;
        rdfs:label    "secondTerminalReception"@en;
        rdfs:range    vec:TerminalReceptionReference .

vec:PlacementSpecification
        rdf:type         owl:Class;
        rdfs:comment     "Specification for the description of placements. Placements are used to connect OccurrenceOrUsages with a topology.\n"@en;
        rdfs:label       "PlacementSpecification"@en;
        rdfs:subClassOf  vec:Specification .

vec:WireMountingDetail
        rdf:type         owl:Class;
        rdfs:comment     "With a WireMountingDetail it is possible to describe a detailed wire mounting.\nThis is needed if the information which wire end is mounted onto which wire reception is important (e.g. coax contacts).\n"@en;
        rdfs:label       "WireMountingDetail"@en;
        rdfs:subClassOf  vec:ExtendableElement .

[ rdf:type     owl:AllDisjointClasses;
  owl:members  ( vec:ModularSlot vec:Slot )
] .

vec:Ordered  rdf:type  owl:Class;
        rdfs:comment  "Class of elements that are ordered within their containment."@en;
        rdfs:label    "Ordered"@en .

vec:slotSpecificationSlotLayout
        rdf:type            owl:ObjectProperty;
        rdfs:comment        "References the layout associated with this slot.\n"@en;
        rdfs:domain         vec:SlotSpecification;
        rdfs:label          "slotLayout"@en;
        rdfs:range          vec:SlotLayout;
        rdfs:subPropertyOf  vec:contains .

vec:LanguageCode_La  rdf:type  vec:LanguageCode , owl:NamedIndividiual;
        vec:enumLiteral  "La" .

vec:wireElementSpecificationSubWireElementSpecification
        rdf:type      owl:ObjectProperty;
        rdfs:comment  "Specifies the contained subWireElements if the WireElement has sub elements. \n"@en;
        rdfs:domain   vec:WireElementSpecification;
        rdfs:label    "subWireElementSpecification"@en;
        rdfs:range    vec:WireElementSpecification .

vec:sheetOrChapterReferencedPart
        rdf:type      owl:ObjectProperty;
        rdfs:comment  "The association is an informative link which PartVersions are described by the SheetOrChapter. \n"@en;
        rdfs:domain   vec:SheetOrChapter;
        rdfs:label    "referencedPart"@en;
        rdfs:range    vec:PartVersion .

vec:cartesianPoint3DY
        rdf:type      owl:DatatypeProperty;
        rdfs:comment  "Specifies the value of y-coordinate of the Cartesian point. The unit of this value is the baseUnit of containing BuildingBlockSpecification3D.\n"@en;
        rdfs:domain   vec:CartesianPoint3D;
        rdfs:label    "y"@en;
        rdfs:range    xs:double .

vec:conductorSpecificationStructure
        rdf:type      owl:DatatypeProperty;
        rdfs:comment  "Specifies the structure of the conductor (e.g. symmetrical, asymmetrical).\n"@en;
        rdfs:domain   vec:ConductorSpecification;
        rdfs:label    "structure"@en;
        rdfs:range    xs:string .

vec:terminalCurrentInformationCurrentRange
        rdf:type            owl:ObjectProperty;
        rdfs:comment        "Specifies the valid current range for the terminal. It is defined as a value range, because there are terminals where minimum current is needed to avoid corrosion.\n"@en;
        rdfs:domain         vec:TerminalCurrentInformation;
        rdfs:label          "currentRange"@en;
        rdfs:range          vec:ValueRange;
        rdfs:subPropertyOf  vec:contains .

vec:fileBasedInstructionLocation
        rdf:type      owl:DatatypeProperty;
        rdfs:comment  "Specifies where (at which location) the file could be found.\n"@en;
        rdfs:domain   vec:FileBasedInstruction;
        rdfs:label    "location"@en;
        rdfs:range    xs:string .

vec:IECUnitName_Byte  rdf:type  vec:IECUnitName , owl:NamedIndividiual;
        vec:enumLiteral  "Byte" .

vec:topologySegmentAliasId
        rdf:type            owl:ObjectProperty;
        rdfs:comment        "Specifies additional identifiers for the TopologySegment.\nExample: TopologySegment Ids may vary from one CAD system export to another. Therefore the CAD system Id is improper for identification attribute. The identification shall have a value which is unique within the Topology. AliasId may be used for the CAD system Id.\n"@en;
        rdfs:domain         vec:TopologySegment;
        rdfs:label          "aliasId"@en;
        rdfs:range          vec:AliasIdentification;
        rdfs:subPropertyOf  vec:contains .

vec:CavityMountingDetail
        rdf:type         owl:Class;
        rdfs:comment     "With a CavityMountingDetail it is possible to describe a detailed cavity mounting.\nThis is needed if the information which terminal reception is mounted into which cavity is important. There are cases where this information can be relevant (e.g. bridge contacts with an asymmetric wire mounting).\n"@en;
        rdfs:label       "CavityMountingDetail"@en;
        rdfs:subClassOf  vec:ExtendableElement .

vec:cartesianVector2DX
        rdf:type      owl:DatatypeProperty;
        rdfs:comment  "Specifies the x-coordinate in 2D space.\n"@en;
        rdfs:domain   vec:CartesianVector2D;
        rdfs:label    "x"@en;
        rdfs:range    xs:double .

vec:cavitySealRoleCavitySealSpecification
        rdf:type      owl:ObjectProperty;
        rdfs:comment  "References the CavitySealSpecification that is instanced by this CavitySealRole.\n"@en;
        rdfs:domain   vec:CavitySealRole;
        rdfs:label    "cavitySealSpecification"@en;
        rdfs:range    vec:CavitySealSpecification .

vec:GeometryType  rdf:type  owl:Class;
        rdfs:comment     "Enumeration for the definition of the GeometryType.\n"@en;
        rdfs:label       "GeometryType"@en;
        rdfs:subClassOf  vec:OpenEnumeration .

vec:LanguageCode_Qu  rdf:type  vec:LanguageCode , owl:NamedIndividiual;
        vec:enumLiteral  "Qu" .

vec:SpliceTerminalSpecification
        rdf:type         owl:Class;
        rdfs:comment     "Specification for the definition of splice terminals.\n"@en;
        rdfs:label       "SpliceTerminalSpecification"@en;
        rdfs:subClassOf  vec:TerminalSpecification .

vec:holeMountedFixingSpecificationHoleShape
        rdf:type     owl:DatatypeProperty;
        rdfs:domain  vec:HoleMountedFixingSpecification;
        rdfs:label   "holeShape"@en;
        rdfs:range   xs:string .

vec:SiPrefix_Giga  rdf:type  vec:SiPrefix , owl:NamedIndividiual;
        vec:enumLiteral  "Giga" .

vec:NodeLocation  rdf:type  owl:Class;
        rdfs:comment     "Specifies a TopologyNode as a Location.\n"@en;
        rdfs:label       "NodeLocation"@en;
        rdfs:subClassOf  vec:Location .

vec:numericalValueValueComponent
        rdf:type      owl:DatatypeProperty;
        rdfs:comment  "Specifies the value of the numerical value.\n"@en;
        rdfs:domain   vec:NumericalValue;
        rdfs:label    "valueComponent"@en;
        rdfs:range    xs:double .

vec:SlotReference  rdf:type  owl:Class;
        rdfs:comment     "A SlotReference represents the usage of a Slot in the context of PartUsage or PartOccurrence.\n"@en;
        rdfs:label       "SlotReference"@en;
        rdfs:subClassOf  vec:AbstractSlotReference .

vec:wireReceptionReferenceIdentification
        rdf:type      owl:DatatypeProperty;
        rdfs:comment  "Specifies a unique identification of the WireReceptionReference . The identification is guaranteed to be unique within the TerminalRole (this might be for example a reception number).\n"@en;
        rdfs:domain   vec:WireReceptionReference;
        rdfs:label    "identification"@en;
        rdfs:range    xs:string .

vec:approvalDescription
        rdf:type            owl:ObjectProperty;
        rdfs:comment        "Room for additional information about the item.\n"@en;
        rdfs:domain         vec:Approval;
        rdfs:label          "description"@en;
        rdfs:range          vec:AbstractLocalizedString;
        rdfs:subPropertyOf  vec:contains .

vec:harnessGeometrySpecification3DGeometryType
        rdf:type      owl:ObjectProperty;
        rdfs:comment  "Specifies the type of geometry. Valid values are Dmu, Formboard.\n"@en;
        rdfs:domain   vec:HarnessGeometrySpecification3D;
        rdfs:label    "geometryType"@en;
        rdfs:range    vec:GeometryType .

vec:conductorSpecificationCurrentInformation
        rdf:type            owl:ObjectProperty;
        rdfs:comment        "Specifies the current information of the conductor. These are the maximum currents for which the conductor is approved.\n"@en;
        rdfs:domain         vec:ConductorSpecification;
        rdfs:label          "currentInformation"@en;
        rdfs:range          vec:ConductorCurrentInformation;
        rdfs:subPropertyOf  vec:contains .

vec:locationPlacedPlacementPoints
        rdf:type      owl:ObjectProperty;
        rdfs:comment  "References the PlacementPointReference that is placed by this location.\n"@en;
        rdfs:domain   vec:Location;
        rdfs:label    "placedPlacementPoints"@en;
        rdfs:range    vec:PlacementPointReference .

vec:SiUnitName_Ohm  rdf:type  vec:SiUnitName , owl:NamedIndividiual;
        vec:enumLiteral  "Ohm" .

vec:transformation3DA21
        rdf:type     owl:DatatypeProperty;
        rdfs:domain  vec:Transformation3D;
        rdfs:label   "a21"@en;
        rdfs:range   xs:double .

vec:LanguageCode_Nl  rdf:type  vec:LanguageCode , owl:NamedIndividiual;
        vec:enumLiteral  "Nl" .

vec:variantConfigurationIdentification
        rdf:type      owl:DatatypeProperty;
        rdfs:comment  "Specifies a unique identification of the variant configuration. The identification is guaranteed to be unique within the specification and does not change over the time.\n"@en;
        rdfs:domain   vec:VariantConfiguration;
        rdfs:label    "identification"@en;
        rdfs:range    xs:string .

vec:occurrenceOrUsageViewItem2DGridSquare
        rdf:type      owl:DatatypeProperty;
        rdfs:comment  "Specifies the grid square in which the OccurrenceOrUsageViewItem2D is placed (e.g. E/40).\n"@en;
        rdfs:domain   vec:OccurrenceOrUsageViewItem2D;
        rdfs:label    "gridSquare"@en;
        rdfs:range    xs:string .

vec:slotSpecificationLayoutType
        rdf:type      owl:DatatypeProperty;
        rdfs:comment  "Specifies the slot's layout type. This should be an enumeration of values defined in a conformance class.\n"@en;
        rdfs:domain   vec:SlotSpecification;
        rdfs:label    "layoutType"@en;
        rdfs:range    xs:string .

vec:LanguageCode_En  rdf:type  vec:LanguageCode , owl:NamedIndividiual;
        vec:enumLiteral  "En" .

vec:pinComponentBehaviorOpticalInformation
        rdf:type            owl:ObjectProperty;
        rdfs:comment        "Specifies the optical information of the pin, if it has the type optical.\n"@en;
        rdfs:domain         vec:PinComponentBehavior;
        rdfs:label          "opticalInformation"@en;
        rdfs:range          vec:PinOpticalInformation;
        rdfs:subPropertyOf  vec:contains .

vec:PinOpticalInformation
        rdf:type      owl:Class;
        rdfs:comment  "Allows the specification of optical information in a PinComponentBehavior.\n"@en;
        rdfs:label    "PinOpticalInformation"@en .

vec:LanguageCode_Mi  rdf:type  vec:LanguageCode , owl:NamedIndividiual;
        vec:enumLiteral  "Mi" .

vec:PinComponentReference
        rdf:type      owl:Class;
        rdfs:comment  "A PinComponentReference represents the usage of a PinComponent in the context of a PartUsage or PartOccurrence. (KBLFRM-401)\n"@en;
        rdfs:label    "PinComponentReference"@en .

vec:contains  rdf:type  owl:ObjectProperty;
        rdfs:comment  "This is the representation of the containment modeled in the UML. All associations that are a \"containment\" in the UML model are subproperties of this property."@en;
        rdfs:label    "contains"@en .

vec:compositeUnitFactors
        rdf:type      owl:ObjectProperty;
        rdfs:comment  "References the Units that are used as factors to create the CompositeUnit.\n"@en;
        rdfs:domain   vec:CompositeUnit;
        rdfs:label    "factors"@en;
        rdfs:range    vec:Unit .

vec:otherUnitOtherUnitName
        rdf:type            owl:ObjectProperty;
        rdfs:comment        "Specifies the name of the unit.\n"@en;
        rdfs:domain         vec:OtherUnit;
        rdfs:label          "otherUnitName"@en;
        rdfs:range          vec:OtherUnitName;
        rdfs:subPropertyOf  vec:contains .

vec:PinApplianceType_LongTerm
        rdf:type         vec:PinApplianceType , owl:NamedIndividiual;
        vec:enumLiteral  "longTerm" .

vec:ImperialUnitName_League
        rdf:type         vec:ImperialUnitName , owl:NamedIndividiual;
        vec:enumLiteral  "League" .

vec:RingTerminalSpecification
        rdf:type         owl:Class;
        rdfs:comment     "Specification for the definition of ring terminals.\n"@en;
        rdfs:label       "RingTerminalSpecification"@en;
        rdfs:subClassOf  vec:TerminalSpecification .

vec:terminalReceptionSpecificationTerminalType
        rdf:type            owl:ObjectProperty;
        rdfs:comment        "Specifies the terminal type that is associated with the terminal reception.\n"@en;
        rdfs:domain         vec:TerminalReceptionSpecification;
        rdfs:label          "terminalType"@en;
        rdfs:range          vec:TerminalType;
        rdfs:subPropertyOf  vec:contains .

vec:routingSpecialRouted
        rdf:type      owl:DatatypeProperty;
        rdfs:comment  "Specifies that routing has been created in a special way. This means it has not been calculated in the standard way, because for some reason the result of the standard calculation has been inconvenient.\n"@en;
        rdfs:domain   vec:Routing;
        rdfs:label    "specialRouted"@en;
        rdfs:range    xs:boolean .

vec:LanguageCode_Ta  rdf:type  vec:LanguageCode , owl:NamedIndividiual;
        vec:enumLiteral  "Ta" .

vec:ImperialUnitName_FluidOunce
        rdf:type         vec:ImperialUnitName , owl:NamedIndividiual;
        vec:enumLiteral  "FluidOunce" .

vec:zoneRequiredRobustnessProperties
        rdf:type            owl:ObjectProperty;
        rdfs:comment        "Defines the robustness properties that are required in this zone. This can result in specific requirements for the used components (e.g. the ability for sealing).\n"@en;
        rdfs:domain         vec:Zone;
        rdfs:label          "requiredRobustnessProperties"@en;
        rdfs:range          vec:RobustnessProperties;
        rdfs:subPropertyOf  vec:contains .

vec:segmentLocationReferencedSegment
        rdf:type      owl:ObjectProperty;
        rdfs:comment  "References the TopologieSegment on which the Location is located. \n"@en;
        rdfs:domain   vec:SegmentLocation;
        rdfs:label    "referencedSegment"@en;
        rdfs:range    vec:TopologySegment .

vec:LanguageCode_Be  rdf:type  vec:LanguageCode , owl:NamedIndividiual;
        vec:enumLiteral  "Be" .

vec:itemEquivalenceCompanyName
        rdf:type      owl:DatatypeProperty;
        rdfs:comment  "Specifies the company which states the ItemEquivalence.\n"@en;
        rdfs:domain   vec:ItemEquivalence;
        rdfs:label    "companyName"@en;
        rdfs:range    xs:string .

vec:conductorSpecificationNumberOfStrands
        rdf:type            owl:ObjectProperty;
        rdfs:comment        "Specifies the number of strands in one conductor. If the conductor is solid than the number of strands would be one.\n"@en;
        rdfs:domain         vec:ConductorSpecification;
        rdfs:label          "numberOfStrands"@en;
        rdfs:range          vec:NumericalValue;
        rdfs:subPropertyOf  vec:contains .

vec:LanguageCode_Ab  rdf:type  vec:LanguageCode , owl:NamedIndividiual;
        rdfs:comment     "Abkhazian\n"@en;
        vec:enumLiteral  "Ab" .

[ rdf:type     owl:AllDisjointClasses;
  owl:members  ( vec:CoreSpecification vec:ShieldSpecification )
] .

vec:connectorHousingRoleComponentNode
        rdf:type      owl:ObjectProperty;
        rdfs:comment  "References the ComponentNode that is realized by the referenced ConnectorHousing (OccurrenceOrUsage with ConnectorHousingRole). This can especially be relevant for inliners. KBLFRM-341.\n"@en;
        rdfs:domain   vec:ConnectorHousingRole;
        rdfs:label    "componentNode"@en;
        rdfs:range    vec:ComponentNode .

vec:fittingOutletOuterDiameter
        rdf:type            owl:ObjectProperty;
        rdfs:comment        "Specifies the outer diameter of the outlet.\n"@en;
        rdfs:domain         vec:FittingOutlet;
        rdfs:label          "outerDiameter"@en;
        rdfs:range          vec:NumericalValue;
        rdfs:subPropertyOf  vec:contains .

vec:slotSpecificationGender
        rdf:type            owl:ObjectProperty;
        rdfs:comment        "Specifies the gender of the slot. This should be an enumeration of values defined in a conformance class.\n"@en;
        rdfs:domain         vec:SlotSpecification;
        rdfs:label          "gender"@en;
        rdfs:range          vec:SlotGender;
        rdfs:subPropertyOf  vec:contains .

vec:fittingOutletIdentification
        rdf:type      owl:DatatypeProperty;
        rdfs:comment  "Specifies the identification of the Outlet. This must be unique within a FittingSpecification.\n"@en;
        rdfs:domain   vec:FittingOutlet;
        rdfs:label    "identification"@en;
        rdfs:range    xs:string .

vec:partOccurrenceAlternativeOccurrence
        rdf:type      owl:ObjectProperty;
        rdfs:comment  "References the PartOcurrences that are an alternative for this PartOccurrence.\n"@en;
        rdfs:domain   vec:PartOccurrence;
        rdfs:label    "alternativeOccurrence"@en;
        rdfs:range    vec:PartOccurrence .

vec:networkNodeIdentification
        rdf:type      owl:DatatypeProperty;
        rdfs:comment  "Specifies a unique identification of the NetworkNode. The identification is guaranteed to be unique within the NetSpecification.\n"@en;
        rdfs:domain   vec:NetworkNode;
        rdfs:label    "identification"@en;
        rdfs:range    xs:string .

vec:cavitySealSpecificationHardness
        rdf:type            owl:ObjectProperty;
        rdfs:comment        "Specifies the hardness of the cavity seal.\n"@en;
        rdfs:domain         vec:CavitySealSpecification;
        rdfs:label          "hardness"@en;
        rdfs:range          vec:NumericalValue;
        rdfs:subPropertyOf  vec:contains .

vec:CartesianPoint3D  rdf:type  owl:Class;
        rdfs:comment     "A CartesianPoint3D is a point that is defined by its coordinates in a rectangular three-dimensional Cartesian coordinate system.\n"@en;
        rdfs:label       "CartesianPoint3D"@en;
        rdfs:subClassOf  vec:ExtendableElement .

vec:netGroupIdentification
        rdf:type      owl:DatatypeProperty;
        rdfs:comment  "Specifies a unique identification of the NetGroup. The identification is guaranteed to be unique within the NetSpecification.\n"@en;
        rdfs:domain   vec:NetGroup;
        rdfs:label    "identification"@en;
        rdfs:range    xs:string .

vec:CartesianVector  rdf:type  owl:Class;
        rdfs:comment  "Abstract super class for vectors, either 2D or 3D.\n"@en;
        rdfs:label    "CartesianVector"@en .

vec:PlacementPoint  rdf:type  owl:Class;
        rdfs:comment     "Defines a point on the component which can be placed explicitly in the topology (e.g. opening in a grommet, the entry point of a connector housing). If a PlacementPoint requires further specification for a certain component type (e.g. the entry point of a connector housing), this is done by an element specific for the component type, which related to the placement point.\n"@en;
        rdfs:label       "PlacementPoint"@en;
        rdfs:subClassOf  vec:ExtendableElement .

vec:netGroupNet  rdf:type  owl:ObjectProperty;
        rdfs:comment  "References the Nets that are grouped by the NetGroup. \n"@en;
        rdfs:domain   vec:NetGroup;
        rdfs:label    "net"@en;
        rdfs:range    vec:Net .

[ rdf:type     owl:AllDisjointClasses;
  owl:members  ( vec:GeometryNode2D vec:GeometryNode3D )
] .

vec:LanguageCode_Wo  rdf:type  vec:LanguageCode , owl:NamedIndividiual;
        vec:enumLiteral  "Wo" .

vec:TerminalReceptionSpecification
        rdf:type         owl:Class;
        rdfs:comment     "Specification for the definition of terminal receptions. A TerminalReception is the area of a terminal where the contacting with another terminal (e.g. between a connector housing and a control unit) takes place. Normally the terminal reception is placed in a cavity of a connector housing.\n"@en;
        rdfs:label       "TerminalReceptionSpecification"@en;
        rdfs:subClassOf  vec:Specification .

vec:partOccurrenceInstanciatedOccurrence
        rdf:type      owl:ObjectProperty;
        rdfs:comment  "References the PartOccurrence which is instantiated by the PartOccurrence. This reference is for example needed in the case of usage of assemblies.\n"@en;
        rdfs:domain   vec:PartOccurrence;
        rdfs:label    "instanciatedOccurrence"@en;
        rdfs:range    vec:PartOccurrence .

vec:networkNodeAbbreviation
        rdf:type            owl:ObjectProperty;
        rdfs:comment        "Room for a short name of the NetworkNode.\n"@en;
        rdfs:domain         vec:NetworkNode;
        rdfs:label          "abbreviation"@en;
        rdfs:range          vec:LocalizedString;
        rdfs:subPropertyOf  vec:contains .

vec:ImperialUnitName  rdf:type  owl:Class;
        rdfs:comment         "Enumeration for the definition of imperial unit names.\n"@en;
        rdfs:label           "ImperialUnitName"@en;
        rdfs:subClassOf      vec:ClosedEnumeration;
        owl:equivalentClass  [ rdf:type   owl:Class;
                               owl:oneOf  ( vec:ImperialUnitName_Thou vec:ImperialUnitName_Inch vec:ImperialUnitName_Foot vec:ImperialUnitName_Yard vec:ImperialUnitName_Chain vec:ImperialUnitName_Furlong vec:ImperialUnitName_Mile vec:ImperialUnitName_League vec:ImperialUnitName_FluidOunce vec:ImperialUnitName_Gill vec:ImperialUnitName_Pint vec:ImperialUnitName_Quart vec:ImperialUnitName_Gallon vec:ImperialUnitName_Grain vec:ImperialUnitName_Drachm vec:ImperialUnitName_Ounce vec:ImperialUnitName_Pound vec:ImperialUnitName_Stone vec:ImperialUnitName_Quarter vec:ImperialUnitName_HundredWeight vec:ImperialUnitName_Ton vec:ImperialUnitName_Perch vec:ImperialUnitName_Rood vec:ImperialUnitName_Acre )
                             ] .

vec:cartesianPoint2DX
        rdf:type      owl:DatatypeProperty;
        rdfs:comment  "Specifies the value of x-coordinate of the Cartesian point. The unit of this value is the baseUnit of containing BuildingBlockSpecification2D.\n"@en;
        rdfs:domain   vec:CartesianPoint2D;
        rdfs:label    "x"@en;
        rdfs:range    xs:double .

vec:LanguageCode_Es  rdf:type  vec:LanguageCode , owl:NamedIndividiual;
        vec:enumLiteral  "Es" .

vec:SiUnitName_Weber  rdf:type  vec:SiUnitName , owl:NamedIndividiual;
        vec:enumLiteral  "Weber" .

vec:measurementPointReferenceIdentification
        rdf:type      owl:DatatypeProperty;
        rdfs:comment  "Specifies a unique identification of the MeasurementPointReference. The identification is guaranteed to be unique within the containing PlaceableElementRole.\n"@en;
        rdfs:domain   vec:MeasurementPointReference;
        rdfs:label    "identification"@en;
        rdfs:range    xs:string .

vec:transformation3DA13
        rdf:type     owl:DatatypeProperty;
        rdfs:domain  vec:Transformation3D;
        rdfs:label   "a13"@en;
        rdfs:range   xs:double .

vec:Project  rdf:type    owl:Class;
        rdfs:comment     "Specifies a certain development project. Instances of this class are assumed to be constant. Thus this is located directly under VEC-root element.\n"@en;
        rdfs:label       "Project"@en;
        rdfs:subClassOf  vec:ExtendableElement .

vec:LanguageCode_Mn  rdf:type  vec:LanguageCode , owl:NamedIndividiual;
        vec:enumLiteral  "Mn" .

vec:StatusOfApproval_Withdrawn
        rdf:type         vec:StatusOfApproval , owl:NamedIndividiual;
        vec:enumLiteral  "Withdrawn" .

vec:usageConstraintProject
        rdf:type      owl:ObjectProperty;
        rdfs:comment  "References the Projects to which the UsageConstraint applies. This means the described PartVersion is allowed / denied in the referenced UsageConstraint.\n"@en;
        rdfs:domain   vec:UsageConstraint;
        rdfs:label    "project"@en;
        rdfs:range    vec:Project .

vec:cavityPlugRolePluggedCavityRef
        rdf:type      owl:ObjectProperty;
        rdfs:comment  "Defines which cavity / cavities in a connector instance is sealed by the plug. \n"@en;
        rdfs:domain   vec:CavityPlugRole;
        rdfs:label    "pluggedCavityRef"@en;
        rdfs:range    vec:CavityReference .

vec:wireProtectionRoleTapeOverlap
        rdf:type      owl:DatatypeProperty;
        rdfs:comment  "Specifies the amount of overlap two rounds of taping around a segment have.\n"@en;
        rdfs:domain   vec:WireProtectionRole;
        rdfs:label    "tapeOverlap"@en;
        rdfs:range    xs:string .

vec:SimpleValueProperty
        rdf:type         owl:Class;
        rdfs:comment     "A custom property with a simple value (string).\n"@en;
        rdfs:label       "SimpleValueProperty"@en;
        rdfs:subClassOf  vec:CustomProperty .

vec:connectionIdentification
        rdf:type      owl:DatatypeProperty;
        rdfs:comment  "Specifies a unique identification of the Connection. The identification is guaranteed to be unique within the ConnectionSpecification.\n"@en;
        rdfs:domain   vec:Connection;
        rdfs:label    "identification"@en;
        rdfs:range    xs:string .

vec:roleIdentification
        rdf:type      owl:DatatypeProperty;
        rdfs:comment  "Specifies a unique identification of the Role. The identification is guaranteed to be unqiue within the OccurrenceOrUsage.\n"@en;
        rdfs:domain   vec:Role;
        rdfs:label    "identification"@en;
        rdfs:range    xs:string .

vec:eEComponentRoleComponentNode
        rdf:type      owl:ObjectProperty;
        rdfs:comment  "References the ComponentNode that is realized by the referenced EEComponent (OccurrenceOrUsage with EEComponentRole).\nKBLFRM-341\n"@en;
        rdfs:domain   vec:EEComponentRole;
        rdfs:label    "componentNode"@en;
        rdfs:range    vec:ComponentNode .

vec:buildingBlockSpecification3DCartesianPoint
        rdf:type            owl:ObjectProperty;
        rdfs:comment        "Specifies the CartesianPoint3Ds that are used in the BuildingBlockSpecification3D.\n"@en;
        rdfs:domain         vec:BuildingBlockSpecification3D;
        rdfs:label          "cartesianPoint"@en;
        rdfs:range          vec:CartesianPoint3D;
        rdfs:subPropertyOf  vec:contains .

vec:ImperialUnitName_Drachm
        rdf:type         vec:ImperialUnitName , owl:NamedIndividiual;
        vec:enumLiteral  "Drachm" .

vec:PluggableTerminalSpecification
        rdf:type         owl:Class;
        rdfs:comment     "Specification for the definition of pluggable terminals.\n"@en;
        rdfs:label       "PluggableTerminalSpecification"@en;
        rdfs:subClassOf  vec:TerminalSpecification .

vec:segmentConnectionPointIdentification
        rdf:type      owl:DatatypeProperty;
        rdfs:comment  "Specifies a unique identification of the SegmentConnectionPoint. The identification is guaranteed to be unique within the ConnectorHousingSpecification.\n"@en;
        rdfs:domain   vec:SegmentConnectionPoint;
        rdfs:label    "identification"@en;
        rdfs:range    xs:string .

vec:RoutableElement  rdf:type  owl:Class;
        rdfs:comment     "A RoutableElement is an element that can be routed, which mean it is possible to assign it to a Path in the Topology.\n"@en;
        rdfs:label       "RoutableElement"@en;
        rdfs:subClassOf  vec:ConfigurableElement .

vec:SlotGender_Female
        rdf:type         vec:SlotGender , owl:NamedIndividiual;
        vec:enumLiteral  "Female" .

vec:massInformationValue
        rdf:type            owl:ObjectProperty;
        rdfs:comment        "Specifies the mass as numerical value.\n"@en;
        rdfs:domain         vec:MassInformation;
        rdfs:label          "value"@en;
        rdfs:range          vec:NumericalValue;
        rdfs:subPropertyOf  vec:contains .

vec:BuildingBlockPositioning3D
        rdf:type         owl:Class;
        rdfs:comment     "Defines the position of a BuildingBlock3D in the HarnessGeometry.\n"@en;
        rdfs:label       "BuildingBlockPositioning3D"@en;
        rdfs:subClassOf  vec:ConfigurableElement .

vec:partVersionPartVersion
        rdf:type      owl:DatatypeProperty;
        rdfs:comment  "The partVersion specifies the version index of a part (see also partNumber).\n"@en;
        rdfs:domain   vec:PartVersion;
        rdfs:label    "partVersion"@en;
        rdfs:range    xs:string .

vec:SignalCurve  rdf:type  owl:Class;
        rdfs:label       "SignalCurve"@en;
        rdfs:subClassOf  vec:OpenEnumeration .

vec:wireProtectionRoleTapingDirection
        rdf:type            owl:ObjectProperty;
        rdfs:comment        "Specifies the direction of the taping.\n"@en;
        rdfs:domain         vec:WireProtectionRole;
        rdfs:label          "tapingDirection"@en;
        rdfs:range          vec:TapingDirection;
        rdfs:subPropertyOf  vec:contains .

vec:wireGroupingSpecificationWireGrouping
        rdf:type            owl:ObjectProperty;
        rdfs:comment        "Specifies the WireGroupings described by the WireGroupingSpecification.\n"@en;
        rdfs:domain         vec:WireGroupingSpecification;
        rdfs:label          "wireGrouping"@en;
        rdfs:range          vec:WireGrouping;
        rdfs:subPropertyOf  vec:contains .

vec:OtherUnit  rdf:type  owl:Class;
        rdfs:comment     "The OtherUnit class can be used to define a unit, which is necessary in the context of data exchange but not contained in the standard systems (e.g. Piece).\n"@en;
        rdfs:label       "OtherUnit"@en;
        rdfs:subClassOf  vec:Unit .

vec:cavityMountingDetailTerminalReceptionReference
        rdf:type      owl:ObjectProperty;
        rdfs:comment  "References the TerminalReception that is used for the detailed description of the cavity mounting. \n"@en;
        rdfs:domain   vec:CavityMountingDetail;
        rdfs:label    "terminalReceptionReference"@en;
        rdfs:range    vec:TerminalReceptionReference .

vec:LengthClassification_Designed
        rdf:type         vec:LengthClassification , owl:NamedIndividiual;
        rdfs:comment     "A designed length means that the value is taken directly from a design tool.\n"@en;
        vec:enumLiteral  "Designed" .

vec:PlaceableElementRole
        rdf:type         owl:Class;
        rdfs:comment     "A PlaceableElementRole defines the instance specific properties and relationships of a PlaceableElement.\n"@en;
        rdfs:label       "PlaceableElementRole"@en;
        rdfs:subClassOf  vec:Role .

vec:PrimaryPartType_MultiCavityPlug
        rdf:type         vec:PrimaryPartType , owl:NamedIndividiual;
        vec:enumLiteral  "MultiCavityPlug" .

vec:MatingSpecification
        rdf:type         owl:Class;
        rdfs:comment     "Specification for the description of a Mating. A mating allows the mapping between independent harness sections of the electrical system. This is done by the mapping of TerminalRoles of one side to the other.\n"@en;
        rdfs:label       "MatingSpecification"@en;
        rdfs:subClassOf  vec:Specification .

vec:eEComponentRoleMountingHousing
        rdf:type      owl:ObjectProperty;
        rdfs:comment  "Specifies the connector housing to which into which the EE-component is mounted. \n"@en;
        rdfs:domain   vec:EEComponentRole;
        rdfs:label    "mountingHousing"@en;
        rdfs:range    vec:ConnectorHousingRole .

vec:LocalizedTypedString
        rdf:type         owl:Class;
        rdfs:comment     "Allows the internationalization of text contents in a typed way. Attributes of the type LocalizedTypedString normally have the multiplicity [0..*]. This means that such an attribute can have multiple values for different locales and types. It must not have multiple values for the same locale and type."@en;
        rdfs:label       "LocalizedTypedString"@en;
        rdfs:subClassOf  vec:AbstractLocalizedString .

vec:wireElementSpecificationInsulationSpecification
        rdf:type      owl:ObjectProperty;
        rdfs:comment  "If the WireElement has an insulation then the specification of the insulation is referenced here.\n"@en;
        rdfs:domain   vec:WireElementSpecification;
        rdfs:label    "insulationSpecification"@en;
        rdfs:range    vec:InsulationSpecification .

vec:USUnitName_HundredWeight
        rdf:type         vec:USUnitName , owl:NamedIndividiual;
        vec:enumLiteral  "HundredWeight" .

vec:TypeOfPermission_Checked
        rdf:type         vec:TypeOfPermission , owl:NamedIndividiual;
        vec:enumLiteral  "Checked" .

vec:SiPrefix_Femto  rdf:type  vec:SiPrefix , owl:NamedIndividiual;
        vec:enumLiteral  "Femto" .

vec:PowerConsumption  rdf:type  owl:Class;
        rdfs:comment  "Defines the power consumption of an EEComponent . An EEComponent can have multiple different PowerConsumptions e.g. standby, maximum. An EEComponent can have multiple PowerConsumptions , but must not have more than one PowerConsumptions of the same type .\n"@en;
        rdfs:label    "PowerConsumption"@en .

vec:contactingSpecificationContactPoint
        rdf:type            owl:ObjectProperty;
        rdfs:comment        "Specifies the ContactPoints defined by the ContactingSpecification.\n"@en;
        rdfs:domain         vec:ContactingSpecification;
        rdfs:label          "contactPoint"@en;
        rdfs:range          vec:ContactPoint;
        rdfs:subPropertyOf  vec:contains .

vec:partStructureSpecificationContent
        rdf:type      owl:DatatypeProperty;
        rdfs:comment  "Specifies the type of content of the bill of material (e.g. module, harness complete set)\n"@en;
        rdfs:domain   vec:PartStructureSpecification;
        rdfs:label    "content"@en;
        rdfs:range    xs:string .

vec:WireReceptionReference
        rdf:type      owl:Class;
        rdfs:comment  "A WireReceptionReference is an instance of a WireReception .\n"@en;
        rdfs:label    "WireReceptionReference"@en .

vec:textBasedInstructionInstallationInstruction
        rdf:type            owl:ObjectProperty;
        rdfs:comment        "Specifies the instruction in a human readable form. Different languages are possible.\n"@en;
        rdfs:domain         vec:TextBasedInstruction;
        rdfs:label          "installationInstruction"@en;
        rdfs:range          vec:LocalizedString;
        rdfs:subPropertyOf  vec:contains .

vec:vecContentCompliantConformanceClass
        rdf:type            owl:ObjectProperty;
        rdfs:comment        "Specifies references to the conformance classes that apply to the VEC-file. \n"@en;
        rdfs:domain         vec:VecContent;
        rdfs:label          "compliantConformanceClass"@en;
        rdfs:range          vec:ConformanceClass;
        rdfs:subPropertyOf  vec:contains .

vec:nodeLocationReferencedNode
        rdf:type      owl:ObjectProperty;
        rdfs:comment  "References the TopologieNode on which the Location is located. \n"@en;
        rdfs:domain   vec:NodeLocation;
        rdfs:label    "referencedNode"@en;
        rdfs:range    vec:TopologyNode .

vec:sizeWidth  rdf:type     owl:ObjectProperty;
        rdfs:comment        "The width of the element.\n"@en;
        rdfs:domain         vec:Size;
        rdfs:label          "width"@en;
        rdfs:range          vec:NumericalValue;
        rdfs:subPropertyOf  vec:contains .

vec:OnPointPlacement  rdf:type  owl:Class;
        rdfs:comment     "An OnPointPlacement is a placement of an OccurrenceOrUsage that places it onto discrete points, in most cases one point. In some cases it is necessary to place a component (with more than one reference point) onto multiple points (e.g. a cable channel).\n"@en;
        rdfs:label       "OnPointPlacement"@en;
        rdfs:subClassOf  vec:Placement .

[ rdf:type     owl:AllDisjointClasses;
  owl:members  ( vec:TopologyGroupSpecification )
] .

vec:grommetSpecificationCableLeadThrough
        rdf:type            owl:ObjectProperty;
        rdfs:comment        "Specifies the CableLeadThroughs of the Grommet. \n"@en;
        rdfs:domain         vec:GrommetSpecification;
        rdfs:label          "cableLeadThrough"@en;
        rdfs:range          vec:CableLeadThrough;
        rdfs:subPropertyOf  vec:contains .

vec:numericalValuePropertyValue
        rdf:type            owl:ObjectProperty;
        rdfs:comment        "Defines the value of the CustomProperty.\n"@en;
        rdfs:domain         vec:NumericalValueProperty;
        rdfs:label          "value"@en;
        rdfs:range          vec:NumericalValue;
        rdfs:subPropertyOf  vec:contains .

vec:connectionGroupInstallationInstruction
        rdf:type            owl:ObjectProperty;
        rdfs:comment        "Specifies additional InstallationInstructions for the ConnectionGroup.\n"@en;
        rdfs:domain         vec:ConnectionGroup;
        rdfs:label          "installationInstruction"@en;
        rdfs:range          vec:Instruction;
        rdfs:subPropertyOf  vec:contains .

vec:sIUnitSiPrefix  rdf:type  owl:ObjectProperty;
        rdfs:comment        "Specifies the prefix of the SI unit (e.g. milli, centi, mirco,...)\n"@en;
        rdfs:domain         vec:SIUnit;
        rdfs:label          "siPrefix"@en;
        rdfs:range          vec:SiPrefix;
        rdfs:subPropertyOf  vec:contains .

vec:LanguageCode_Ms  rdf:type  vec:LanguageCode , owl:NamedIndividiual;
        vec:enumLiteral  "Ms" .

vec:SignalForm_SquareWave
        rdf:type         vec:SignalForm , owl:NamedIndividiual;
        vec:enumLiteral  "squareWave" .

vec:configurableElementConfigInfo
        rdf:type      owl:ObjectProperty;
        rdfs:comment  "References the configuration information that applies to the ConfigurableElement.\n"@en;
        rdfs:domain   vec:ConfigurableElement;
        rdfs:label    "configInfo"@en;
        rdfs:range    vec:VariantConfiguration .

vec:CartesianDimension
        rdf:type         owl:Class;
        rdfs:comment     "The CartesianDimension specifies the size of an object in 2D-space. "@en;
        rdfs:label       "CartesianDimension"@en;
        rdfs:subClassOf  vec:ExtendableElement .

vec:PinType_Resistive
        rdf:type         vec:PinType , owl:NamedIndividiual;
        vec:enumLiteral  "resistive" .

vec:connectionGroupConnection
        rdf:type      owl:ObjectProperty;
        rdfs:comment  "References the Connections that are grouped by the ConnectionGroup. \n"@en;
        rdfs:domain   vec:ConnectionGroup;
        rdfs:label    "connection"@en;
        rdfs:range    vec:Connection .

vec:geometrySegment2DPathSegment
        rdf:type            owl:ObjectProperty;
        rdfs:comment        "Specifies an ordered list of PathSegments that describe the appearance of the GeometrySegment2D. The appearance is described by the concatenation of the PathSegments beginning at the startNode of the GeometrySegment2D.\n"@en;
        rdfs:domain         vec:GeometrySegment2D;
        rdfs:label          "pathSegment"@en;
        rdfs:range          vec:PathSegment , vec:Ordered;
        rdfs:subPropertyOf  vec:contains .

vec:tapeSpecificationAdhesive
        rdf:type            owl:ObjectProperty;
        rdfs:comment        "Specifies the adhesive material of the tape.\n"@en;
        rdfs:domain         vec:TapeSpecification;
        rdfs:label          "adhesive"@en;
        rdfs:range          vec:Material;
        rdfs:subPropertyOf  vec:contains .

vec:networkPortDescription
        rdf:type            owl:ObjectProperty;
        rdfs:comment        "Room for additional, human readable information about the NetworkPort.\n"@en;
        rdfs:domain         vec:NetworkPort;
        rdfs:label          "description"@en;
        rdfs:range          vec:AbstractLocalizedString;
        rdfs:subPropertyOf  vec:contains .

vec:occurrenceOrUsageViewItem2DOccurrenceOrUsage
        rdf:type      owl:ObjectProperty;
        rdfs:comment  "Specifies the OccurrenceOrUsage which is represented by the view item.\n"@en;
        rdfs:domain   vec:OccurrenceOrUsageViewItem2D;
        rdfs:label    "occurrenceOrUsage"@en;
        rdfs:range    vec:OccurrenceOrUsage .

vec:LanguageCode_Tk  rdf:type  vec:LanguageCode , owl:NamedIndividiual;
        vec:enumLiteral  "Tk" .

vec:pinComponentReferencedCavity
        rdf:type      owl:ObjectProperty;
        rdfs:comment  "Defines the cavity in the corresponding ConnectorHousingSpecification of the HousingComponent where the PinComponent is located. \n(see KBLFRM-300)\n"@en;
        rdfs:domain   vec:PinComponent;
        rdfs:label    "referencedCavity"@en;
        rdfs:range    vec:Cavity .

vec:occurrenceOrUsageRole
        rdf:type            owl:ObjectProperty;
        rdfs:comment        "Specifies the different roles of the OccurrenceOrUsage.\n"@en;
        rdfs:domain         vec:OccurrenceOrUsage;
        rdfs:label          "role"@en;
        rdfs:range          vec:Role;
        rdfs:subPropertyOf  vec:contains .

vec:LanguageCode_Km  rdf:type  vec:LanguageCode , owl:NamedIndividiual;
        vec:enumLiteral  "Km" .

[ rdf:type     owl:AllDisjointClasses;
  owl:members  ( vec:NodeLocation vec:SegmentLocation )
] .

vec:connectionGroupConnectionGroupType
        rdf:type      owl:DatatypeProperty;
        rdfs:comment  "Specifies the type of the connectionGroup (e.g. twisted).\n"@en;
        rdfs:domain   vec:ConnectionGroup;
        rdfs:label    "connectionGroupType"@en;
        rdfs:range    xs:string .

vec:SiUnitName_Kelvin
        rdf:type         vec:SiUnitName , owl:NamedIndividiual;
        vec:enumLiteral  "Kelvin" .

vec:vecContentVecVersion
        rdf:type            owl:ObjectProperty;
        rdfs:comment        "Specifies the version of the VEC used for the file.\n"@en;
        rdfs:domain         vec:VecContent;
        rdfs:label          "vecVersion"@en;
        rdfs:range          vec:VecVersion;
        rdfs:subPropertyOf  vec:contains .

vec:LanguageCode_Bo  rdf:type  vec:LanguageCode , owl:NamedIndividiual;
        vec:enumLiteral  "Bo" .

vec:LanguageCode_Sh  rdf:type  vec:LanguageCode , owl:NamedIndividiual;
        vec:enumLiteral  "Sh" .

vec:abstractLocalizedStringValue
        rdf:type      owl:DatatypeProperty;
        rdfs:comment  "The value of the LocalizedString in language defined by the languageCode.\n"@en;
        rdfs:domain   vec:AbstractLocalizedString;
        rdfs:label    "value"@en;
        rdfs:range    xs:string .

vec:ImperialUnitName_Gill
        rdf:type         vec:ImperialUnitName , owl:NamedIndividiual;
        vec:enumLiteral  "Gill" .

vec:UsageNodeType_Protection
        rdf:type         vec:UsageNodeType , owl:NamedIndividiual;
        vec:enumLiteral  "Protection" .

[ rdf:type     owl:AllDisjointClasses;
  owl:members  ( vec:CorrugatedPipeSpecification vec:ShrinkableTubeSpecification )
] .

vec:SignalDirection  rdf:type  owl:Class;
        rdfs:comment         "Enumeration for the definition of SignalDirections.\n"@en;
        rdfs:label           "SignalDirection"@en;
        rdfs:subClassOf      vec:ClosedEnumeration;
        owl:equivalentClass  [ rdf:type   owl:Class;
                               owl:oneOf  ( vec:SignalDirection_In vec:SignalDirection_Out vec:SignalDirection_InOut )
                             ] .

vec:unitExponent  rdf:type  owl:DatatypeProperty;
        rdfs:comment  "Defines the exponent with which this unit instance should be used. In order to define square meters for example, the SIUnit \"metre\" with an exponent of 2 will be used. If no exponent is defined it is equivalent to the value 1.\n"@en;
        rdfs:domain   vec:Unit;
        rdfs:label    "exponent"@en;
        rdfs:range    xs:integer .

vec:NetGroup  rdf:type   owl:Class;
        rdfs:comment     "A NetGroup allows the grouping of the Nets.\n"@en;
        rdfs:label       "NetGroup"@en;
        rdfs:subClassOf  vec:ConfigurableElement .

vec:signalDescription
        rdf:type            owl:ObjectProperty;
        rdfs:comment        "A human readable description of the signal.\n"@en;
        rdfs:domain         vec:Signal;
        rdfs:label          "description"@en;
        rdfs:range          vec:AbstractLocalizedString;
        rdfs:subPropertyOf  vec:contains .

vec:conductorSpecificationCrossSectionArea
        rdf:type            owl:ObjectProperty;
        rdfs:comment        "Specifies the cross section area of the conductor (e.g. 0,5 mm┬▓). The cross section area is a nominal value, which refers to the conducting properties of the conductor normalized to the properties of a full material core.\n"@en;
        rdfs:domain         vec:ConductorSpecification;
        rdfs:label          "crossSectionArea"@en;
        rdfs:range          vec:NumericalValue;
        rdfs:subPropertyOf  vec:contains .

vec:TapeSpecification
        rdf:type         owl:Class;
        rdfs:comment     "Specification for the description of tapes.\n"@en;
        rdfs:label       "TapeSpecification"@en;
        rdfs:subClassOf  vec:WireProtectionSpecification .

[ rdf:type     owl:AllDisjointClasses;
  owl:members  ( vec:ContactPoint vec:RoutableElement vec:PinComponentBehavior vec:BuildingBlockPositioning2D vec:BuildingBlockPositioning3D vec:OccurrenceOrUsage vec:MatingPoint vec:Net vec:NetGroup vec:NetworkNode vec:NetworkPort vec:Dimension vec:Path vec:Placement vec:Routing vec:ComponentNode vec:ComponentPort vec:ConnectionEnd vec:ConnectionGroup vec:GeometryNode vec:GeometrySegment vec:TopologyNode vec:TopologySegment vec:Zone vec:UsageNode )
] .

vec:buildingBlockPositioning2DCenterPoint
        rdf:type            owl:ObjectProperty;
        rdfs:comment        "Specifies the center point of the BuildingBlock in the coordinate system of the harness drawing. \n"@en;
        rdfs:domain         vec:BuildingBlockPositioning2D;
        rdfs:label          "centerPoint"@en;
        rdfs:range          vec:CartesianPoint2D;
        rdfs:subPropertyOf  vec:contains .

vec:componentPortNetworkPort
        rdf:type      owl:ObjectProperty;
        rdfs:comment  "References the NetworkPort that is realized by the ComponentPort.\n"@en;
        rdfs:domain   vec:ComponentPort;
        rdfs:label    "networkPort"@en;
        rdfs:range    vec:NetworkPort .

vec:cavitySpecificationCavityDesign
        rdf:type      owl:DatatypeProperty;
        rdfs:comment  "Specifies the structural shape of the cavity, e.g. round, flat, box.\n"@en;
        rdfs:domain   vec:CavitySpecification;
        rdfs:label    "cavityDesign"@en;
        rdfs:range    xs:string .

vec:PinCurrentType_StandbyCurrent
        rdf:type         vec:PinCurrentType , owl:NamedIndividiual;
        vec:enumLiteral  "standbyCurrent" .

vec:PartWithSubComponentsRole
        rdf:type         owl:Class;
        rdfs:comment     "A PartWithSubComponentsRole defines the instance specific properties and relationships of a part with subcomponents. A PartWithSubComponents is a composite part like an Assembly, a Module, Harness.\n"@en;
        rdfs:label       "PartWithSubComponentsRole"@en;
        rdfs:subClassOf  vec:Role .

vec:CompatibilityStatement
        rdf:type         owl:Class;
        rdfs:comment     "A CompatibilityStatement is used to express compatibility between parts. This can be either compatibility for contacting (terminals, wires, seals, a.s.o.) or for plugging (connector housings, slots, a.s.o.).\nA CompatibilityStatement can be used to explicitly express compatibility (hasCompatibility = true) or to express incompatibility / negation (hasCompatibility = false).\nThe CompatibilityStatement is stated by referencing the corresponding specifications. In the concrete implementation this mechanisms allows three different variants to express compatibility.\nIn the first variant the CompatibilityStatement references specifications that are not directly related to a concrete PartVersion (association in the super-class PartOrUsageRelatedSpecification). In this case the attributes of the specification represent a search pattern for searching compatible parts in a component library.\nIn the second variant the CompatibilityStatement references the same specifications that are used to specify the component attributes of a PartVersion. This would be equivalent to an explicit mapping compatible PartVersions.\nIn the third variant the CompatibilityStatement references specifications that do not have any attributes at all. These specifications are normally defined in the same document that defines the CompatibilitySpecification. Such a specification can group multiple PartVersion by referencing them. This is possible, because the VEC makes no restriction on the number of specifications that can be defined for single PartVersion.\n"@en;
        rdfs:label       "CompatibilityStatement"@en;
        rdfs:subClassOf  vec:ExtendableElement .

vec:buildingBlockPositioning3DReferenced3DBuildingBlock
        rdf:type      owl:ObjectProperty;
        rdfs:comment  "References the building block that is positioned.\n"@en;
        rdfs:domain   vec:BuildingBlockPositioning3D;
        rdfs:label    "referenced3DBuildingBlock"@en;
        rdfs:range    vec:BuildingBlockSpecification3D .

vec:SegmentLocation  rdf:type  owl:Class;
        rdfs:comment     "Specifies a point on a TopologySegment as a Location.\n"@en;
        rdfs:label       "SegmentLocation"@en;
        rdfs:subClassOf  vec:Location .

vec:SealState_Sealed  rdf:type  vec:SealState , owl:NamedIndividiual;
        rdfs:comment     "The splice is waterproof.\n"@en;
        vec:enumLiteral  "Sealed" .

vec:powerConsumptionValue
        rdf:type            owl:ObjectProperty;
        rdfs:comment        "Specifies the power consumption for this type of PowerConsumption .\n"@en;
        rdfs:domain         vec:PowerConsumption;
        rdfs:label          "value"@en;
        rdfs:range          vec:NumericalValue;
        rdfs:subPropertyOf  vec:contains .

vec:partVersionAliasId
        rdf:type            owl:ObjectProperty;
        rdfs:comment        "Room to specify additional identifiers for the PartVersion. This field must not be used for alternative PartNumbers. It is intended for identifiers others than PartNumbers, such as human readable identifiers printed on the part e.g. a number of fuse or a relay. Therefore it does not have to be strictly unique.\n"@en;
        rdfs:domain         vec:PartVersion;
        rdfs:label          "aliasId"@en;
        rdfs:range          vec:AliasIdentification;
        rdfs:subPropertyOf  vec:contains .

vec:terminalReceptionGender
        rdf:type      owl:DatatypeProperty;
        rdfs:comment  "Specifies the gender of the TerminalReception. This should be an enumeration of values defined in a conformance class (e.g. male, female). The gender is included in the TerminalReception class in order to be able to refer the same TerminalReceptionSpecification gender-independent. KBLFRM-360\n"@en;
        rdfs:domain   vec:TerminalReception;
        rdfs:label    "gender"@en;
        rdfs:range    xs:string .

vec:transformation3DOrigin
        rdf:type      owl:ObjectProperty;
        rdfs:comment  "Specifies the coordinates of the translation.\n"@en;
        rdfs:domain   vec:Transformation3D;
        rdfs:label    "origin"@en;
        rdfs:range    vec:CartesianPoint3D .

vec:wireElementReferenceIdentification
        rdf:type      owl:DatatypeProperty;
        rdfs:comment  "Specifies a unique identification of the WireElementReference. The identification is guaranteed to be unique within the WireRole.\n"@en;
        rdfs:domain   vec:WireElementReference;
        rdfs:label    "identification"@en;
        rdfs:range    xs:string .

vec:internalTerminalConnectionIdentification
        rdf:type      owl:DatatypeProperty;
        rdfs:comment  "Specifies a unique identification of the InternalTerminalConnection. The identification is guaranteed to be unique within the TerminalSpecification (this might be for example an internal connection number).\n"@en;
        rdfs:domain   vec:InternalTerminalConnection;
        rdfs:label    "identification"@en;
        rdfs:range    xs:string .

vec:housingComponentReferencePinComponentRef
        rdf:type            owl:ObjectProperty;
        rdfs:comment        "Specifies the PinComponentReferences used in the HousingComponentReference. \n(KBLFRM-401)\n"@en;
        rdfs:domain         vec:HousingComponentReference;
        rdfs:label          "pinComponentRef"@en;
        rdfs:range          vec:PinComponentReference;
        rdfs:subPropertyOf  vec:contains .

vec:cavitySealSpecificationCompatibleTerminalType
        rdf:type            owl:ObjectProperty;
        rdfs:comment        "Defines a list of terminal types that are compatible to this CavitySealSpecification.\n"@en;
        rdfs:domain         vec:CavitySealSpecification;
        rdfs:label          "compatibleTerminalType"@en;
        rdfs:range          vec:TerminalType;
        rdfs:subPropertyOf  vec:contains .

vec:LanguageCode_Ga  rdf:type  vec:LanguageCode , owl:NamedIndividiual;
        vec:enumLiteral  "Ga" .

vec:housingComponentReferenceIdentification
        rdf:type      owl:DatatypeProperty;
        rdfs:comment  "Specifies a unique identification of the HousingComponentReference. The identification is guaranteed to be unique within the EEComponentRole.\n"@en;
        rdfs:domain   vec:HousingComponentReference;
        rdfs:label    "identification"@en;
        rdfs:range    xs:string .

vec:usageConstraintFromSerialNumber
        rdf:type      owl:DatatypeProperty;
        rdfs:comment  "Specifies the lower bound of a serial number range to which the usage constraint applies.\n"@en;
        rdfs:domain   vec:UsageConstraint;
        rdfs:label    "fromSerialNumber"@en;
        rdfs:range    xs:string .

vec:IECPrefix  rdf:type      owl:Class;
        rdfs:comment         "Enumeration for the definition of IEC unit prefixes.\n"@en;
        rdfs:label           "IECPrefix"@en;
        rdfs:subClassOf      vec:ClosedEnumeration;
        owl:equivalentClass  [ rdf:type   owl:Class;
                               owl:oneOf  ( vec:IECPrefix_Yobi vec:IECPrefix_Zebi vec:IECPrefix_Exbi vec:IECPrefix_Pebi vec:IECPrefix_Tebi vec:IECPrefix_Gibi vec:IECPrefix_Mebi vec:IECPrefix_Kibi )
                             ] .

vec:FittingOutlet  rdf:type  owl:Class;
        rdfs:comment     "Specifies one outlet of the fitting.\n"@en;
        rdfs:label       "FittingOutlet"@en;
        rdfs:subClassOf  vec:ExtendableElement .

vec:SoundDampingClass
        rdf:type      owl:Class;
        rdfs:comment  "Allows the definition of a sound damping class. The sound damping class of a component is specified as a level of sound damping. The level is specified by the classKey . Valid keys are specified by the referenceSystem . Attributes of the type SoundDampingClass normally have the multiplicity [0..*]. This means that such an attribute can have SoundDampingClass entries for different referenceSystems . It must not have multiple entries for the same referenceSystem .\n"@en;
        rdfs:label    "SoundDampingClass"@en .

vec:itemVersionChangeDescription
        rdf:type            owl:ObjectProperty;
        rdfs:comment        "Specifies the change history of the ItemVersion. \n"@en;
        rdfs:domain         vec:ItemVersion;
        rdfs:label          "changeDescription"@en;
        rdfs:range          vec:ChangeDescription;
        rdfs:subPropertyOf  vec:contains .

vec:pathSegmentControlPoint
        rdf:type            owl:ObjectProperty;
        rdfs:comment        "This association is defined as unique='false' and ordered='true'. This can not be represented efficiently directly in RDF/OWL. Therefore, this association references Wrappers as proxies to the actual elements, instead of the actual elements itself (like a regular association)." , "The ordered list of control points through which the PathSegment goes. \n"@en;
        rdfs:domain         vec:PathSegment;
        rdfs:label          "controlPoint"@en;
        rdfs:range          vec:CartesianPoint2DWrapper , vec:Ordered;
        rdfs:subPropertyOf  vec:contains .

vec:LanguageCode_Dz  rdf:type  vec:LanguageCode , owl:NamedIndividiual;
        vec:enumLiteral  "Dz" .

vec:documentVersionDocumentType
        rdf:type      owl:DatatypeProperty;
        rdfs:comment  "The type of the document. This should be an enumeration of values defined in a conformance class. Typical values would be example: WiringDiagram, HarnessDrawing, etc.\n"@en;
        rdfs:domain   vec:DocumentVersion;
        rdfs:label    "documentType"@en;
        rdfs:range    xs:string .

vec:PinComponent  rdf:type  owl:Class;
        rdfs:comment     "A PinComponent describes a pin of an EEComponent. A PinComponent is part of a HousingComponent and is defined by tree aspects. Its geometric position in the HousingComponent , which is defined by the referencedCavity. Its physical electrical properties, which are defined by the referenced TerminalSpecification. Its electrical behaviour, which is defined configuration dependent by its PinComponentBehaviour. "@en;
        rdfs:label       "PinComponent"@en;
        rdfs:subClassOf  vec:ExtendableElement .

vec:PinCurrentType_MaxCurrent
        rdf:type         vec:PinCurrentType , owl:NamedIndividiual;
        vec:enumLiteral  "maxCurrent" .

vec:dimensionPath  rdf:type  owl:ObjectProperty;
        rdfs:comment        "Specifies a path in the topology along which the dimension is defined. \n"@en;
        rdfs:domain         vec:Dimension;
        rdfs:label          "path"@en;
        rdfs:range          vec:Path;
        rdfs:subPropertyOf  vec:contains .

vec:TapingDirection_Left
        rdf:type         vec:TapingDirection , owl:NamedIndividiual;
        vec:enumLiteral  "Left" .

vec:cavityMountingCavityMountingDetail
        rdf:type            owl:ObjectProperty;
        rdfs:comment        "Specifies the CavityMoutingDetails, if a detailed description of the relationships between Cavities and TerminalReceptions is needed.\n"@en;
        rdfs:domain         vec:CavityMounting;
        rdfs:label          "cavityMountingDetail"@en;
        rdfs:range          vec:CavityMountingDetail;
        rdfs:subPropertyOf  vec:contains .

vec:USUnitName_Gallon
        rdf:type         vec:USUnitName , owl:NamedIndividiual;
        vec:enumLiteral  "Gallon" .

vec:boltMountedFixingSpecificationBoltType
        rdf:type            owl:ObjectProperty;
        rdfs:comment        "Specifies the type of the bolt of the fixing. Appropriate values should be defined in a conformance class.\n"@en;
        rdfs:domain         vec:BoltMountedFixingSpecification;
        rdfs:label          "boltType"@en;
        rdfs:range          vec:BoltMountedFixingSpecification;
        rdfs:subPropertyOf  vec:contains .

vec:LanguageCode_Sm  rdf:type  vec:LanguageCode , owl:NamedIndividiual;
        vec:enumLiteral  "Sm" .

vec:fuseSpecificationFuseType
        rdf:type      owl:DatatypeProperty;
        rdfs:comment  "The type of a fuse. This should be an enumeration of values defined in a conformance class.\n"@en;
        rdfs:domain   vec:FuseSpecification;
        rdfs:label    "fuseType"@en;
        rdfs:range    xs:string .

vec:partUsageSpecificationPartUsage
        rdf:type            owl:ObjectProperty;
        rdfs:comment        "Specifies the PartUsages defined by the PartUsageSpecification.\n"@en;
        rdfs:domain         vec:PartUsageSpecification;
        rdfs:label          "partUsage"@en;
        rdfs:range          vec:PartUsage;
        rdfs:subPropertyOf  vec:contains .

vec:PluggableTerminalRole
        rdf:type         owl:Class;
        rdfs:comment     "A PluggableTerminalRole defines the instance specific properties and relationships of a pluggable terminal.\n"@en;
        rdfs:label       "PluggableTerminalRole"@en;
        rdfs:subClassOf  vec:TerminalRole .

vec:contactPointMountedTerminal
        rdf:type      owl:ObjectProperty;
        rdfs:comment  "References the terminal that is used for contacting defined by the ContactPoint. \n"@en;
        rdfs:domain   vec:ContactPoint;
        rdfs:label    "mountedTerminal"@en;
        rdfs:range    vec:TerminalRole .

vec:SpliceType_EndSplice
        rdf:type         vec:SpliceType , owl:NamedIndividiual;
        rdfs:comment     "An endSplice is a splice where wires only from one side are connected.\n"@en;
        vec:enumLiteral  "EndSplice" .

vec:ContactPoint  rdf:type  owl:Class;
        rdfs:comment     "A contact point defines the relationship between Terminals, Seals, Plugs, Cavities and Wires. A ContactPoint is expected to have only one electrical potential.\nIf a contacting of a terminal has more than one potential (e.g. a coax-contact) one contact point for each potential is needed.\n"@en;
        rdfs:label       "ContactPoint"@en;
        rdfs:subClassOf  vec:ConfigurableElement .

vec:CoreSpecification
        rdf:type         owl:Class;
        rdfs:comment     "Defines the properties of a conductor which are specific for cores.\n"@en;
        rdfs:label       "CoreSpecification"@en;
        rdfs:subClassOf  vec:ConductorSpecification .

vec:ComponentPort  rdf:type  owl:Class;
        rdfs:comment     "Defines a port of ComponentNode. A ComponentPort is usually the realization of a NetworkPort. Electrological connections are defined between two or more ComponentPorts.\n"@en;
        rdfs:label       "ComponentPort"@en;
        rdfs:subClassOf  vec:ConfigurableElement .

vec:partOrUsageRelatedSpecificationDescribedPart
        rdf:type      owl:ObjectProperty;
        rdfs:comment  "References the PartVersion(s) to which the information defined in this specification applies.\nExample: If the PartOrUsageRelatedSpecification is a GeneralTechnicalPartSpecifcation and it defines that the color is \"green\" then all PartVersion referenced by this association are \"green\".\n"@en;
        rdfs:domain   vec:PartOrUsageRelatedSpecification;
        rdfs:label    "describedPart"@en;
        rdfs:range    vec:PartVersion .

vec:NodeType  rdf:type   owl:Class;
        rdfs:comment     "Enumeration for the definition of the type of a TopologyNode.\n"@en;
        rdfs:label       "NodeType"@en;
        rdfs:subClassOf  vec:OpenEnumeration .

vec:buildingBlockSpecification3DGeometrySegment
        rdf:type            owl:ObjectProperty;
        rdfs:comment        "Specifies the GeometrySegment3Ds defined by the BuildingBlockSpecification3D.\n"@en;
        rdfs:domain         vec:BuildingBlockSpecification3D;
        rdfs:label          "geometrySegment"@en;
        rdfs:range          vec:GeometrySegment3D;
        rdfs:subPropertyOf  vec:contains .

vec:TerminalReception
        rdf:type         owl:Class;
        rdfs:comment     "A TerminalReception is the area of a terminal where the contacting with another terminal (e.g. between a connector housing and a control unit) takes place. Normally the terminal reception is placed in a cavity of a connector housing.\nThis class represents such an area on the terminal.\n"@en;
        rdfs:label       "TerminalReception"@en;
        rdfs:subClassOf  vec:ExtendableElement .

vec:LanguageCode_Hi  rdf:type  vec:LanguageCode , owl:NamedIndividiual;
        vec:enumLiteral  "Hi" .

vec:fittingOutletInnerDiameter
        rdf:type            owl:ObjectProperty;
        rdfs:comment        "Specifies the inner diameter of the outlet.\n"@en;
        rdfs:domain         vec:FittingOutlet;
        rdfs:label          "innerDiameter"@en;
        rdfs:range          vec:NumericalValue;
        rdfs:subPropertyOf  vec:contains .

vec:generalTechnicalPartSpecificationMassInformation
        rdf:type            owl:ObjectProperty;
        rdfs:comment        "Specifies the mass of the part.\n"@en;
        rdfs:domain         vec:GeneralTechnicalPartSpecification;
        rdfs:label          "massInformation"@en;
        rdfs:range          vec:MassInformation;
        rdfs:subPropertyOf  vec:contains .

vec:compatibilityStatementSlot
        rdf:type      owl:ObjectProperty;
        rdfs:comment  "References explicit Slots for which the compatibility statement is stated.\n"@en;
        rdfs:domain   vec:CompatibilityStatement;
        rdfs:label    "slot"@en;
        rdfs:range    vec:AbstractSlot .

vec:contactSystemFirstTerminal
        rdf:type      owl:ObjectProperty;
        rdfs:comment  "References the first terminal of the ContactSystem.\n"@en;
        rdfs:domain   vec:ContactSystem;
        rdfs:label    "firstTerminal"@en;
        rdfs:range    vec:PartVersion .

vec:PrimaryPartType_ShrinkableTube
        rdf:type         vec:PrimaryPartType , owl:NamedIndividiual;
        vec:enumLiteral  "ShrinkableTube" .

vec:IECUnitName_Bit  rdf:type  vec:IECUnitName , owl:NamedIndividiual;
        vec:enumLiteral  "Bit" .

vec:SlotMapping  rdf:type  owl:Class;
        rdfs:comment  "Defines the mapping of two slots contained PartVersion A & B of the containing Mapping-object.\n"@en;
        rdfs:label    "SlotMapping"@en .

vec:SealingClass  rdf:type  owl:Class;
        rdfs:comment  "Allows the definition of a sealing class. The sealing class of a component is specified as a level of sealing against a specific influence. The influence is specified by the sealingClass and the level is specified by the sealingClassKey. Valid sealing classes and keys are specified by the reference system. Attributes of the type SealingClass normally have the multiplicity [0..*]. This means that such an attribute can have SealingClass entries for different sealingClassReferenceSystems and sealingClasses. It must not have multiple entries for the same sealing class and reference system.\n"@en;
        rdfs:label    "SealingClass"@en .

vec:HistoryEntryType_Sequence
        rdf:type         vec:HistoryEntryType , owl:NamedIndividiual;
        vec:enumLiteral  "Sequence" .

vec:conductorSpecificationStrandDiameter
        rdf:type            owl:ObjectProperty;
        rdfs:comment        "Specifies the diameter of a single strand in the conductor.\n"@en;
        rdfs:domain         vec:ConductorSpecification;
        rdfs:label          "strandDiameter"@en;
        rdfs:range          vec:NumericalValue;
        rdfs:subPropertyOf  vec:contains .

vec:GrommetRole  rdf:type  owl:Class;
        rdfs:comment     "A GrommetRole defines the instance specific properties and relationships of a grommet.\n"@en;
        rdfs:label       "GrommetRole"@en;
        rdfs:subClassOf  vec:Role .

vec:TextBasedInstruction
        rdf:type         owl:Class;
        rdfs:comment     "A TextBasedInstruction is used to specify human readable instructions in text.\n"@en;
        rdfs:label       "TextBasedInstruction"@en;
        rdfs:subClassOf  vec:Instruction .

vec:occurrenceOrUsageIdentification
        rdf:type      owl:DatatypeProperty;
        rdfs:comment  "Specifies a unique identification of the OccurrenceOrUsage. The identification is guaranteed to be unique within the context. Over all VEC-documents an OccurrenceOrUsage-instance can be trusted to be the same if the context-instance is the same and the identification of the OccurrenceOrUsage is the same.\n"@en;
        rdfs:domain   vec:OccurrenceOrUsage;
        rdfs:label    "identification"@en;
        rdfs:range    xs:string .

vec:cableLeadThroughIdentification
        rdf:type      owl:DatatypeProperty;
        rdfs:comment  "Specifies the identification of the CableLeadThrough. This must be unique within a GrommetSpecification.\n"@en;
        rdfs:domain   vec:CableLeadThrough;
        rdfs:label    "identification"@en;
        rdfs:range    xs:string .

vec:SiPrefix_Peta  rdf:type  vec:SiPrefix , owl:NamedIndividiual;
        vec:enumLiteral  "Peta" .

vec:contactSystemJoiningForce
        rdf:type            owl:ObjectProperty;
        rdfs:comment        "Specifies the joining force of the two terminals.\n"@en;
        rdfs:domain         vec:ContactSystem;
        rdfs:label          "joiningForce"@en;
        rdfs:range          vec:NumericalValue;
        rdfs:subPropertyOf  vec:contains .

vec:ImperialUnitName_Mile
        rdf:type         vec:ImperialUnitName , owl:NamedIndividiual;
        vec:enumLiteral  "Mile" .

vec:LanguageCode  rdf:type   owl:Class;
        rdfs:comment         "Enumeration for the definition of ISO language codes. (see KBLFRM-317)\n"@en;
        rdfs:label           "LanguageCode"@en;
        rdfs:subClassOf      vec:ClosedEnumeration;
        owl:equivalentClass  [ rdf:type   owl:Class;
                               owl:oneOf  ( vec:LanguageCode_Aa vec:LanguageCode_Ab vec:LanguageCode_Af vec:LanguageCode_Am vec:LanguageCode_Ar vec:LanguageCode_As vec:LanguageCode_Ay vec:LanguageCode_Az vec:LanguageCode_Ba vec:LanguageCode_Be vec:LanguageCode_Bg vec:LanguageCode_Bh vec:LanguageCode_Bi vec:LanguageCode_Bn vec:LanguageCode_Bo vec:LanguageCode_Br vec:LanguageCode_Ca vec:LanguageCode_Co vec:LanguageCode_Cs vec:LanguageCode_Cy vec:LanguageCode_Da vec:LanguageCode_De vec:LanguageCode_Dz vec:LanguageCode_El vec:LanguageCode_En vec:LanguageCode_Eo vec:LanguageCode_Es vec:LanguageCode_Et vec:LanguageCode_Eu vec:LanguageCode_Fa vec:LanguageCode_Fi vec:LanguageCode_Fj vec:LanguageCode_Fo vec:LanguageCode_Fr vec:LanguageCode_Fy vec:LanguageCode_Ga vec:LanguageCode_Gd vec:LanguageCode_Gl vec:LanguageCode_Gn vec:LanguageCode_Gu vec:LanguageCode_Ha vec:LanguageCode_Hi vec:LanguageCode_He vec:LanguageCode_Hr vec:LanguageCode_Hu vec:LanguageCode_Hy vec:LanguageCode_Ia vec:LanguageCode_Id vec:LanguageCode_Ie vec:LanguageCode_Ik vec:LanguageCode_In vec:LanguageCode_Is vec:LanguageCode_It vec:LanguageCode_Iu vec:LanguageCode_Iw vec:LanguageCode_Ja vec:LanguageCode_Ji vec:LanguageCode_Jw vec:LanguageCode_Ka vec:LanguageCode_Kk vec:LanguageCode_Kl vec:LanguageCode_Km vec:LanguageCode_Kn vec:LanguageCode_Ko vec:LanguageCode_Ks vec:LanguageCode_Ku vec:LanguageCode_Ky vec:LanguageCode_La vec:LanguageCode_Ln vec:LanguageCode_Lo vec:LanguageCode_Lt vec:LanguageCode_Lv vec:LanguageCode_Mg vec:LanguageCode_Mi vec:LanguageCode_Mk vec:LanguageCode_Ml vec:LanguageCode_Mn vec:LanguageCode_Mo vec:LanguageCode_Mr vec:LanguageCode_Ms vec:LanguageCode_Mt vec:LanguageCode_My vec:LanguageCode_Na vec:LanguageCode_Ne vec:LanguageCode_Nl vec:LanguageCode_No vec:LanguageCode_Oc vec:LanguageCode_Om vec:LanguageCode_Or vec:LanguageCode_Pa vec:LanguageCode_Pl vec:LanguageCode_Ps vec:LanguageCode_Pt vec:LanguageCode_Qu vec:LanguageCode_Rm vec:LanguageCode_Rn vec:LanguageCode_Ro vec:LanguageCode_Ru vec:LanguageCode_Rw vec:LanguageCode_Sa vec:LanguageCode_Sd vec:LanguageCode_Sg vec:LanguageCode_Sh vec:LanguageCode_Si vec:LanguageCode_Sk vec:LanguageCode_Sl vec:LanguageCode_Sm vec:LanguageCode_Sn vec:LanguageCode_So vec:LanguageCode_Sq vec:LanguageCode_Sr vec:LanguageCode_Ss vec:LanguageCode_St vec:LanguageCode_Su vec:LanguageCode_Sv vec:LanguageCode_Sw vec:LanguageCode_Ta vec:LanguageCode_Te vec:LanguageCode_Tg vec:LanguageCode_Th vec:LanguageCode_Zi vec:LanguageCode_Tk vec:LanguageCode_Tl vec:LanguageCode_Tn vec:LanguageCode_To vec:LanguageCode_Tr vec:LanguageCode_Ts vec:LanguageCode_Tt vec:LanguageCode_Tw vec:LanguageCode_Ug vec:LanguageCode_Uk vec:LanguageCode_Ur vec:LanguageCode_Uz vec:LanguageCode_Vi vec:LanguageCode_Vo vec:LanguageCode_Wo vec:LanguageCode_Xh vec:LanguageCode_Yi vec:LanguageCode_Yo vec:LanguageCode_Za vec:LanguageCode_Zh vec:LanguageCode_Zu )
                             ] .

vec:SignalDirection_In
        rdf:type         vec:SignalDirection , owl:NamedIndividiual;
        vec:enumLiteral  "In" .

vec:PartUsageSpecification
        rdf:type         owl:Class;
        rdfs:comment     "Specification for the definition of PartUsages.\n"@en;
        rdfs:label       "PartUsageSpecification"@en;
        rdfs:subClassOf  vec:Specification .

vec:LanguageCode_Sr  rdf:type  vec:LanguageCode , owl:NamedIndividiual;
        vec:enumLiteral  "Sr" .

vec:MassInformation  rdf:type  owl:Class;
        rdfs:comment  "Allows the definition of mass information. Attributes of the type MassInformation normally have the multiplicity [0..*]. This means that such an attribute can have mass values for different determinationTypes. It must not have multiple values for the same determinationType.\n"@en;
        rdfs:label    "MassInformation"@en .

vec:soundDampingClassReferenceSystem
        rdf:type      owl:DatatypeProperty;
        rdfs:comment  "The identification of the sound damping class reference system, which is defining possible values and the semantic of sound damping keys.\n"@en;
        rdfs:domain   vec:SoundDampingClass;
        rdfs:label    "referenceSystem"@en;
        rdfs:range    xs:string .

vec:vecContentDateOfCreation
        rdf:type      owl:DatatypeProperty;
        rdfs:comment  "Specifies the date of creation of the VEC-file.\n"@en;
        rdfs:domain   vec:VecContent;
        rdfs:label    "dateOfCreation"@en;
        rdfs:range    xs:dateTime .

vec:conductorSpecificationMaterial
        rdf:type            owl:ObjectProperty;
        rdfs:comment        "Specifies the material of the conductor.\n"@en;
        rdfs:domain         vec:ConductorSpecification;
        rdfs:label          "material"@en;
        rdfs:range          vec:Material;
        rdfs:subPropertyOf  vec:contains .

vec:numericalValueTolerance
        rdf:type            owl:ObjectProperty;
        rdfs:comment        "Specifies the tolerance for the dimension. \n"@en;
        rdfs:domain         vec:NumericalValue;
        rdfs:label          "tolerance"@en;
        rdfs:range          vec:Tolerance;
        rdfs:subPropertyOf  vec:contains .

vec:placementPlacedElement
        rdf:type      owl:ObjectProperty;
        rdfs:comment  "References the PlaceableElementRoles placed by the Placement. \n"@en;
        rdfs:domain   vec:Placement;
        rdfs:label    "placedElement"@en;
        rdfs:range    vec:PlaceableElementRole .

vec:LanguageCode_Ro  rdf:type  vec:LanguageCode , owl:NamedIndividiual;
        vec:enumLiteral  "Ro" .

vec:USUnit  rdf:type     owl:Class;
        rdfs:comment     "The USUnit class can define quantities in the terms of the US-Unit-System by specifying the corresponding US unit name. The US Unit System is quite similar to the imperial unit system, however some units are defined slightly different.\n"@en;
        rdfs:label       "USUnit"@en;
        rdfs:subClassOf  vec:Unit .

vec:cableDuctOutletIdentification
        rdf:type      owl:DatatypeProperty;
        rdfs:comment  "Specifies the identification of the Outlet. This must be unique within a CableDuctSpecification.\n"@en;
        rdfs:domain   vec:CableDuctOutlet;
        rdfs:label    "identification"@en;
        rdfs:range    xs:string .

vec:permissionPermission
        rdf:type            owl:ObjectProperty;
        rdfs:comment        "Specifies the type of permission. Predefined values are: Seen, Checked, Released.\n"@en;
        rdfs:domain         vec:Permission;
        rdfs:label          "permission"@en;
        rdfs:range          vec:TypeOfPermission;
        rdfs:subPropertyOf  vec:contains .

vec:contractCompanyName
        rdf:type      owl:DatatypeProperty;
        rdfs:comment  "Specifies the company which acts in the specified Role in the Contract Relationship.\n"@en;
        rdfs:domain   vec:Contract;
        rdfs:label    "companyName"@en;
        rdfs:range    xs:string .

vec:VecVersion  rdf:type     owl:Class;
        rdfs:label           "VecVersion"@en;
        rdfs:subClassOf      vec:ClosedEnumeration;
        owl:equivalentClass  [ rdf:type   owl:Class;
                               owl:oneOf  ( vec:VecVersion_1.1.1 )
                             ] .

vec:changeDescriptionChangeDate
        rdf:type      owl:DatatypeProperty;
        rdfs:comment  "Specifies the date when the change was performed.\n"@en;
        rdfs:domain   vec:ChangeDescription;
        rdfs:label    "changeDate"@en;
        rdfs:range    xs:dateTime .

vec:buildingBlockSpecification3DPlacedElementViewItem3D
        rdf:type            owl:ObjectProperty;
        rdfs:comment        "Specifies the view items for OccurrenceOrUsages in a BuildingBlockSpecification3D. \n"@en;
        rdfs:domain         vec:BuildingBlockSpecification3D;
        rdfs:label          "placedElementViewItem3D"@en;
        rdfs:range          vec:OccurrenceOrUsageViewItem3D;
        rdfs:subPropertyOf  vec:contains .

vec:connectionConnectionEnd
        rdf:type            owl:ObjectProperty;
        rdfs:comment        "Specifies the ConnectionEnds of the Connection. The ConnectionEnds are required to be an ordered list, because it is possible to define Connections with more than two ConnectionEnds (bus systems). In these cases it is relevant which ConnectionEnds are in the end of connection and which ConnectionEnds are in between. KBLFRM-378\n"@en;
        rdfs:domain         vec:Connection;
        rdfs:label          "connectionEnd"@en;
        rdfs:range          vec:ConnectionEnd , vec:Ordered;
        rdfs:subPropertyOf  vec:contains .

vec:DimensionAnchor  rdf:type  owl:Class;
        rdfs:comment     "A DimensionAnchor represents an abstract anchor onto which a Dimension can be specified.\n"@en;
        rdfs:label       "DimensionAnchor"@en;
        rdfs:subClassOf  vec:ExtendableElement .

vec:ModuleList  rdf:type  owl:Class;
        rdfs:comment     "A ModuleList is a mechanism to control additional / completition PartOccurrences. This means for a car configuration, if at least one of the modules in the list participates in the configuration, the \"completitionComponent\" participates, too.\n"@en;
        rdfs:label       "ModuleList"@en;
        rdfs:subClassOf  vec:ExtendableElement .

vec:connectorHousingSpecificationAverageWireLengthAddOn
        rdf:type            owl:ObjectProperty;
        rdfs:comment        "Specifies the average wire length add on for this connector.\n"@en;
        rdfs:domain         vec:ConnectorHousingSpecification;
        rdfs:label          "averageWireLengthAddOn"@en;
        rdfs:range          vec:NumericalValue;
        rdfs:subPropertyOf  vec:contains .

vec:cartesianVector3DZ
        rdf:type      owl:DatatypeProperty;
        rdfs:comment  "Specifies the z-coordinate in 3D space.\n"@en;
        rdfs:domain   vec:CartesianVector3D;
        rdfs:label    "z"@en;
        rdfs:range    xs:double .

vec:HarnessGeometrySpecification3D
        rdf:type         owl:Class;
        rdfs:comment     "The HarnessGeometrieSpecification3D specifies a three dimensional model of a harness. A harness model is composed of one or more BuildingBlockSpecifaction3D which are placed in the model.\n"@en;
        rdfs:label       "HarnessGeometrySpecification3D"@en;
        rdfs:subClassOf  vec:Specification .

vec:relaySpecificationCoilContact
        rdf:type      owl:ObjectProperty;
        rdfs:comment  "References the PinComponents that are the CoilContacts of the Relay. \n(see KBLFRM-300)\n"@en;
        rdfs:domain   vec:RelaySpecification;
        rdfs:label    "coilContact"@en;
        rdfs:range    vec:PinComponent .

vec:contactPointIdentification
        rdf:type      owl:DatatypeProperty;
        rdfs:comment  "Specifies a unique identification of the ContactPoint. The identification is guaranteed to be unique within the ContactingSpecification.\n"@en;
        rdfs:domain   vec:ContactPoint;
        rdfs:label    "identification"@en;
        rdfs:range    xs:string .

vec:terminalRoleComponentPort
        rdf:type      owl:ObjectProperty;
        rdfs:comment  "References the ComponentPort that is realized by the referenced Terminal (OccurrenceOrUsage with TerminalRole).\nKBLFRM-341\n"@en;
        rdfs:domain   vec:TerminalRole;
        rdfs:label    "componentPort"@en;
        rdfs:range    vec:ComponentPort .

vec:personLastName  rdf:type  owl:DatatypeProperty;
        rdfs:comment  "Specifies the person's last name.\n"@en;
        rdfs:domain   vec:Person;
        rdfs:label    "lastName"@en;
        rdfs:range    xs:string .

vec:partVersionPartNumber
        rdf:type      owl:DatatypeProperty;
        rdfs:comment  "The partNumber is the major identifier of a PartVersion. The format is user defined and respectively company specific. Over all VEC-documents a PartVersion-instance can be trusted to be identical if the combination of partNumber, partVersion and companyName is identical.\n"@en;
        rdfs:domain   vec:PartVersion;
        rdfs:label    "partNumber"@en;
        rdfs:range    xs:string .

vec:connectorHousingSpecificationVoltageRange
        rdf:type            owl:ObjectProperty;
        rdfs:comment        "Specifies the allowed voltage range for the connector housing.\n"@en;
        rdfs:domain         vec:ConnectorHousingSpecification;
        rdfs:label          "voltageRange"@en;
        rdfs:range          vec:ValueRange;
        rdfs:subPropertyOf  vec:contains .

vec:buildingBlockSpecification3DGeometryNode
        rdf:type            owl:ObjectProperty;
        rdfs:comment        "Specifies the GeometryNode3Ds defined by the BuildingBlockSpecification3D.\n"@en;
        rdfs:domain         vec:BuildingBlockSpecification3D;
        rdfs:label          "geometryNode"@en;
        rdfs:range          vec:GeometryNode3D;
        rdfs:subPropertyOf  vec:contains .

vec:segmentConnectionPointReachableCavities
        rdf:type      owl:ObjectProperty;
        rdfs:comment  "Specifies the Cavities that are reachable with wires through this SegmentConnectionPoint.\n"@en;
        rdfs:domain   vec:SegmentConnectionPoint;
        rdfs:label    "reachableCavities"@en;
        rdfs:range    vec:Cavity .

vec:ContactSystem  rdf:type  owl:Class;
        rdfs:comment     "A contact system is a standard reference setup of two terminals and defined length of a core contacted to both terminals. "@en;
        rdfs:label       "ContactSystem"@en;
        rdfs:subClassOf  vec:ExtendableElement .

vec:aliasIdentificationIdentificationValue
        rdf:type      owl:DatatypeProperty;
        rdfs:comment  "Specifies the identification value.\n"@en;
        rdfs:domain   vec:AliasIdentification;
        rdfs:label    "IdentificationValue"@en;
        rdfs:range    xs:string .

vec:TerminalCurrentInformation
        rdf:type      owl:Class;
        rdfs:comment  "Allows the definition of valid current ranges for a terminal. A current range is always defined for a coreCrossSectionArea and a nominal voltage. Attributes of the type CurrentRangeInformation normally have the multiplicity [0..*]. This means that such an attribute can have CurrentRangeInformation entries for different coreCrossSectionAreas and nominalVoltages. It must not have multiple entries for the same coreCrossSectionAreas and nominalVoltages.\n"@en;
        rdfs:label    "TerminalCurrentInformation"@en .

vec:SignalCurve_DiscreteSignal
        rdf:type         vec:SignalCurve , owl:NamedIndividiual;
        vec:enumLiteral  "discreteSignal" .

vec:USUnitName_Grain  rdf:type  vec:USUnitName , owl:NamedIndividiual;
        vec:enumLiteral  "Grain" .

vec:modularSlotAllowedInserts
        rdf:type      owl:ObjectProperty;
        rdfs:comment  "References the ConnectorHousingSpecifications that are valid inserts for this ModularSlot.\n"@en;
        rdfs:domain   vec:ModularSlot;
        rdfs:label    "allowedInserts"@en;
        rdfs:range    vec:ConnectorHousingSpecification .

vec:partWithSubComponentsRolePartStructureSpecification
        rdf:type      owl:ObjectProperty;
        rdfs:comment  "References the PartStructureSpecification that is instantiated by this PartWithSubComponentsRole .\n"@en;
        rdfs:domain   vec:PartWithSubComponentsRole;
        rdfs:label    "partStructureSpecification"@en;
        rdfs:range    vec:PartStructureSpecification .

vec:SiUnitName_Newton
        rdf:type         vec:SiUnitName , owl:NamedIndividiual;
        vec:enumLiteral  "Newton" .

vec:fittingOutletPlacementPoint
        rdf:type      owl:ObjectProperty;
        rdfs:comment  "Specifies the PlacementPoint that represents this FittingOutlet in a PlaceableElementSpecification.\n"@en;
        rdfs:domain   vec:FittingOutlet;
        rdfs:label    "placementPoint"@en;
        rdfs:range    vec:PlacementPoint .

vec:ImperialUnitName_HundredWeight
        rdf:type         vec:ImperialUnitName , owl:NamedIndividiual;
        vec:enumLiteral  "HundredWeight" .

vec:USUnitName_Mile  rdf:type  vec:USUnitName , owl:NamedIndividiual;
        vec:enumLiteral  "Mile" .

vec:LocalizedString  rdf:type  owl:Class;
        rdfs:comment     "Allows the internationalization of text contents. Attributes of the type LocalizedString normally have the multiplicity [0..*]. This means that such an attribute can have multiple values for different locales. It must not have multiple values for the same locale.\n"@en;
        rdfs:label       "LocalizedString"@en;
        rdfs:subClassOf  vec:AbstractLocalizedString .

vec:ImperialUnitName_Grain
        rdf:type         vec:ImperialUnitName , owl:NamedIndividiual;
        vec:enumLiteral  "Grain" .

vec:placeableElementSpecificationPlacementPoint
        rdf:type            owl:ObjectProperty;
        rdfs:comment        "Specifies the PlacementPoints of an PlaceableElementSpecification .\n"@en;
        rdfs:domain         vec:PlaceableElementSpecification;
        rdfs:label          "placementPoint"@en;
        rdfs:range          vec:PlacementPoint;
        rdfs:subPropertyOf  vec:contains .

vec:LanguageCode_Sw  rdf:type  vec:LanguageCode , owl:NamedIndividiual;
        vec:enumLiteral  "Sw" .

[ rdf:type     owl:AllDisjointClasses;
  owl:members  ( vec:AntennaSpecification vec:BatterySpecification vec:FuseSpecification vec:RelaySpecification )
] .

vec:geometrySegment3DStartVector
        rdf:type            owl:ObjectProperty;
        rdfs:comment        "Specifies the start vector of the geometry segment. The start vector is a tangent to the segment at the start position.\n"@en;
        rdfs:domain         vec:GeometrySegment3D;
        rdfs:label          "startVector"@en;
        rdfs:range          vec:CartesianVector3D;
        rdfs:subPropertyOf  vec:contains .

vec:projectCarClassificationLevel4
        rdf:type      owl:DatatypeProperty;
        rdfs:comment  "Provides a classification according to \"CC8 Recommended Practices Specification and Configuration, Product Structures\". Car classification is the identification of a set of similar cars to be offered to the market. Level 4 stands for \"Furthest pre-configured abstract product class\" and represents the furthest configured class of a product, which is not yet a real product. E.g. this could be a complete vehicle, engine, gear-box etc. which has not been evaluated against customer special choices or an abstract vehicle, engine, gear-box etc. which could become a real one after the associated BoM is evaluated. The purpose of this level of a product class instance is in any case to reflect that level of product class of a BoM system which leads to the individual BoM for a single product.\n"@en;
        rdfs:domain   vec:Project;
        rdfs:label    "carClassificationLevel4"@en;
        rdfs:range    xs:string .

vec:personFirstName  rdf:type  owl:DatatypeProperty;
        rdfs:comment  "Specifies the person's first name.\n"@en;
        rdfs:domain   vec:Person;
        rdfs:label    "firstName"@en;
        rdfs:range    xs:string .

vec:OtherUnitName  rdf:type  owl:Class;
        rdfs:comment         "Enumeration for the definition of other unit names.\n"@en;
        rdfs:label           "OtherUnitName"@en;
        rdfs:subClassOf      vec:ClosedEnumeration;
        owl:equivalentClass  [ rdf:type   owl:Class;
                               owl:oneOf  ( vec:OtherUnitName_Pi vec:OtherUnitName_Piece )
                             ] .

vec:documentVersionDocumentVersion
        rdf:type      owl:DatatypeProperty;
        rdfs:comment  "The documentVersion specifies the version index of a document (see also documentNumber).\n"@en;
        rdfs:domain   vec:DocumentVersion;
        rdfs:label    "documentVersion"@en;
        rdfs:range    xs:string .

vec:PinVoltageType_TypicalVoltage
        rdf:type         vec:PinVoltageType , owl:NamedIndividiual;
        vec:enumLiteral  "typicalVoltage" .

[ rdf:type     owl:AllDisjointClasses;
  owl:members  ( vec:OnPointPlacement vec:OnWayPlacement )
] .

vec:geometrySegment2DStartVector
        rdf:type            owl:ObjectProperty;
        rdfs:comment        "Specifies the start vector of the geometry segment. The start vector is a tangent to the segment at the start position.\n"@en;
        rdfs:domain         vec:GeometrySegment2D;
        rdfs:label          "startVector"@en;
        rdfs:range          vec:CartesianVector2D;
        rdfs:subPropertyOf  vec:contains .

vec:placementIsOnTopOf
        rdf:type      owl:ObjectProperty;
        rdfs:comment  "Specifies constraints on ordering of Placements. All referenced Placements have to be below (nearer to the center of the Segment) this Placement. \n(see KBLFRM-171)\n"@en;
        rdfs:domain   vec:Placement;
        rdfs:label    "isOnTopOf"@en;
        rdfs:range    vec:Placement .

vec:conductorSpecificationResistance
        rdf:type            owl:ObjectProperty;
        rdfs:comment        "Specifies the electrical resistance of the conductor. In most cases this is specified as resistance per length (e.g. Ohm per meter).\n"@en;
        rdfs:domain         vec:ConductorSpecification;
        rdfs:label          "resistance"@en;
        rdfs:range          vec:NumericalValue;
        rdfs:subPropertyOf  vec:contains .

vec:usageConstraintSpecificationConstrainedParts
        rdf:type      owl:ObjectProperty;
        rdfs:comment  "References the PartVersions to which this UsageConstraintSpecification applies.\n"@en;
        rdfs:domain   vec:UsageConstraintSpecification;
        rdfs:label    "constrainedParts"@en;
        rdfs:range    vec:PartVersion .

vec:itemHistoryEntrySuccessorVersion
        rdf:type      owl:ObjectProperty;
        rdfs:comment  "References the ItemVersion that is the successor in the ItemHistoryEntry. \n"@en;
        rdfs:domain   vec:ItemHistoryEntry;
        rdfs:label    "successorVersion"@en;
        rdfs:range    vec:ItemVersion .

vec:HarnessDrawingSpecification2D
        rdf:type         owl:Class;
        rdfs:comment     "The HarnessDrawingSpecification2D specifies a two dimensional drawing of a harness. A harness drawing is composed of one or more BuildingBlockSpecifaction2D which are placed on the drawing.\n"@en;
        rdfs:label       "HarnessDrawingSpecification2D"@en;
        rdfs:subClassOf  vec:Specification .

vec:routingSpecialRoutedComment
        rdf:type            owl:ObjectProperty;
        rdfs:comment        "Allows the specification of an explanation why this routing has been routed in a special way.\n"@en;
        rdfs:domain         vec:Routing;
        rdfs:label          "specialRoutedComment"@en;
        rdfs:range          vec:LocalizedString;
        rdfs:subPropertyOf  vec:contains .

vec:connectionSpecificationComponentNode
        rdf:type            owl:ObjectProperty;
        rdfs:comment        "Specifies the ComponentNodes defined by the ConnectionSpecification.\n"@en;
        rdfs:domain         vec:ConnectionSpecification;
        rdfs:label          "componentNode"@en;
        rdfs:range          vec:ComponentNode;
        rdfs:subPropertyOf  vec:contains .

vec:documentBasedInstructionReferencedDocument
        rdf:type      owl:ObjectProperty;
        rdfs:comment  "References the DocumentVersion that is used as an Instruction.\n"@en;
        rdfs:domain   vec:DocumentBasedInstruction;
        rdfs:label    "referencedDocument"@en;
        rdfs:range    vec:DocumentVersion .

vec:signalSignalCurve
        rdf:type            owl:ObjectProperty;
        rdfs:comment        "Specifies the curve of the signal.\n"@en;
        rdfs:domain         vec:Signal;
        rdfs:label          "signalCurve"@en;
        rdfs:range          vec:SignalCurve;
        rdfs:subPropertyOf  vec:contains .

vec:transformation2DA11
        rdf:type     owl:DatatypeProperty;
        rdfs:domain  vec:Transformation2D;
        rdfs:label   "a11"@en;
        rdfs:range   xs:double .

vec:wireElementReferenceWireEnd
        rdf:type            owl:ObjectProperty;
        rdfs:comment        "Specifies the ends of the WireElementReference for contacting purposes. \n"@en;
        rdfs:domain         vec:WireElementReference;
        rdfs:label          "wireEnd"@en;
        rdfs:range          vec:WireEnd;
        rdfs:subPropertyOf  vec:contains .

vec:vecContentContract
        rdf:type            owl:ObjectProperty;
        rdfs:comment        "Specifies the contracts used in the VEC-file. \n"@en;
        rdfs:domain         vec:VecContent;
        rdfs:label          "contract"@en;
        rdfs:range          vec:Contract;
        rdfs:subPropertyOf  vec:contains .

vec:ValueWithUnit  rdf:type  owl:Class;
        rdfs:comment  "Abstract class either for a single numerical measure or a range of numerical measures with upper, lower, or upper and lower bounds.\n"@en;
        rdfs:label    "ValueWithUnit"@en .

vec:geometryNodeAliasId
        rdf:type            owl:ObjectProperty;
        rdfs:comment        "Specifies additional identifiers for the GeometryNode.\n"@en;
        rdfs:domain         vec:GeometryNode;
        rdfs:label          "aliasId"@en;
        rdfs:range          vec:AliasIdentification;
        rdfs:subPropertyOf  vec:contains .

vec:grommetSpecificationGrommetType
        rdf:type      owl:DatatypeProperty;
        rdfs:comment  "Specifies the type of the grommet. Appropriate values should be defined in a conformance class.\n"@en;
        rdfs:domain   vec:GrommetSpecification;
        rdfs:label    "grommetType"@en;
        rdfs:range    xs:string .

vec:NetworkNode  rdf:type  owl:Class;
        rdfs:comment     "A NetworkNode is a representative for an actor in the electric system, e.g. an actuator, a sensor, an ECU\n"@en;
        rdfs:label       "NetworkNode"@en;
        rdfs:subClassOf  vec:ConfigurableElement .

vec:Contract  rdf:type   owl:Class;
        rdfs:comment     "A Contract-instance describes the relationship between an ItemVersion-instance and a Company-instance additionally defining the role the company takes in reference to the ItemVersion.\n"@en;
        rdfs:label       "Contract"@en;
        rdfs:subClassOf  vec:ExtendableElement .

vec:corrugatedPipeSpecificationCorrugationGradient
        rdf:type            owl:ObjectProperty;
        rdfs:comment        "Specifies the gradient of a corrugation of the pipe.\n"@en;
        rdfs:domain         vec:CorrugatedPipeSpecification;
        rdfs:label          "corrugationGradient"@en;
        rdfs:range          vec:NumericalValue;
        rdfs:subPropertyOf  vec:contains .

vec:partVersionProject
        rdf:type      owl:ObjectProperty;
        rdfs:comment  "References the project that develops the PartVersion. \n"@en;
        rdfs:domain   vec:PartVersion;
        rdfs:label    "project"@en;
        rdfs:range    vec:Project .

vec:connectionEndInstallationInstruction
        rdf:type            owl:ObjectProperty;
        rdfs:comment        "Specifies installation instruction for the ConnectionEnd ."@en;
        rdfs:domain         vec:ConnectionEnd;
        rdfs:label          "installationInstruction"@en;
        rdfs:range          vec:Instruction;
        rdfs:subPropertyOf  vec:contains .

vec:PinCurrentType_TypicalCurrent
        rdf:type         vec:PinCurrentType , owl:NamedIndividiual;
        vec:enumLiteral  "typicalCurrent" .

vec:SiUnitName_Radian
        rdf:type         vec:SiUnitName , owl:NamedIndividiual;
        vec:enumLiteral  "Radian" .

vec:terminalSpecificationInternalTerminalConnection
        rdf:type            owl:ObjectProperty;
        rdfs:comment        "Specifies the InternalTerminalConnections of the terminal. \n"@en;
        rdfs:domain         vec:TerminalSpecification;
        rdfs:label          "internalTerminalConnection"@en;
        rdfs:range          vec:InternalTerminalConnection;
        rdfs:subPropertyOf  vec:contains .

vec:USUnitName_Ton  rdf:type  vec:USUnitName , owl:NamedIndividiual;
        vec:enumLiteral  "Ton" .

vec:sizeHeight  rdf:type    owl:ObjectProperty;
        rdfs:comment        "The height of the element.\n"@en;
        rdfs:domain         vec:Size;
        rdfs:label          "height"@en;
        rdfs:range          vec:NumericalValue;
        rdfs:subPropertyOf  vec:contains .

vec:IECPrefix_Kibi  rdf:type  vec:IECPrefix , owl:NamedIndividiual;
        vec:enumLiteral  "Kibi" .

[ rdf:type     owl:AllDisjointClasses;
  owl:members  ( vec:Location vec:MeasurementPointReference )
] .

vec:mappingA  rdf:type  owl:ObjectProperty;
        rdfs:comment  ""@en;
        rdfs:domain   vec:Mapping;
        rdfs:label    "A"@en;
        rdfs:range    vec:PartVersion .

vec:cartesianPoint3DZ
        rdf:type      owl:DatatypeProperty;
        rdfs:comment  "Specifies the value of z-coordinate of the Cartesian point. The unit of this value is the baseUnit of containing BuildingBlockSpecification3D.\n"@en;
        rdfs:domain   vec:CartesianPoint3D;
        rdfs:label    "z"@en;
        rdfs:range    xs:double .

vec:CartesianVector2D
        rdf:type         owl:Class;
        rdfs:comment     "A Cartesian vector in the two dimensional space.\n"@en;
        rdfs:label       "CartesianVector2D"@en;
        rdfs:subClassOf  vec:CartesianVector .

vec:LanguageCode_Ba  rdf:type  vec:LanguageCode , owl:NamedIndividiual;
        vec:enumLiteral  "Ba" .

vec:cartesianVector2DY
        rdf:type      owl:DatatypeProperty;
        rdfs:comment  "Specifies the y-coordinate in 2D space.\n"@en;
        rdfs:domain   vec:CartesianVector2D;
        rdfs:label    "y"@en;
        rdfs:range    xs:double .

vec:PinTimingType  rdf:type  owl:Class;
        rdfs:comment     "Defines the different available timing types of a pin.\n"@en;
        rdfs:label       "PinTimingType"@en;
        rdfs:subClassOf  vec:OpenEnumeration .

vec:pinCurrentInformationTime
        rdf:type            owl:ObjectProperty;
        rdfs:comment        "Specifies the timing of the PinCurrentInformation.\n"@en;
        rdfs:domain         vec:PinCurrentInformation;
        rdfs:label          "time"@en;
        rdfs:range          vec:PinTiming;
        rdfs:subPropertyOf  vec:contains .

vec:MultiCavityPlugSpecification
        rdf:type         owl:Class;
        rdfs:comment     "Specification for the definition of cavity plugs that apply to more than one cavity. A cavity plug is a water tight non-electrical object to fill an empty cavity. MultiCavityPlugs are formed to fit into one connector / slot and to seal more than one cavity at once. Normally there are different variants of these MultiCavityPlugs that can seal a connector in different pinning scenarios. The cavities that are plugged by a MultiCavityPlug are defined with a SealedCavitiesAssignment.\n"@en;
        rdfs:label       "MultiCavityPlugSpecification"@en;
        rdfs:subClassOf  vec:CavityPlugSpecification .

vec:valueRangeMinimum
        rdf:type      owl:DatatypeProperty;
        rdfs:comment  "Lower bound of the value range.\n"@en;
        rdfs:domain   vec:ValueRange;
        rdfs:label    "minimum"@en;
        rdfs:range    xs:double .

vec:ValueDetermination
        rdf:type             owl:Class;
        rdfs:comment         "Enumeration for the definition of a value determination. (see KBLFRM-316)\n"@en;
        rdfs:label           "ValueDetermination"@en;
        rdfs:subClassOf      vec:ClosedEnumeration;
        owl:equivalentClass  [ rdf:type   owl:Class;
                               owl:oneOf  ( vec:ValueDetermination_Calculated vec:ValueDetermination_Measured vec:ValueDetermination_Estimated )
                             ] .

vec:tapeSpecificationWidth
        rdf:type            owl:ObjectProperty;
        rdfs:comment        "Specifies the width of the tape.\n"@en;
        rdfs:domain         vec:TapeSpecification;
        rdfs:label          "width"@en;
        rdfs:range          vec:NumericalValue;
        rdfs:subPropertyOf  vec:contains .

vec:ItemVersion  rdf:type  owl:Class;
        rdfs:comment     "Abstract super-class for physical objects (e.g. a Terminal), virtual objects (e.g a 150% Harness) as well as documents (e.g a wiring diagram). In difference to AP 212 the VEC makes it only possible to describe/exchange information about Versions for the reason that Master-Objects cannot exist without one or more Versions.\n"@en;
        rdfs:label       "ItemVersion"@en;
        rdfs:subClassOf  vec:ExtendableElement .

vec:placementSpecificationDimension
        rdf:type            owl:ObjectProperty;
        rdfs:comment        "Specifies the Dimensions defined by the PlacementSpecification.\n"@en;
        rdfs:domain         vec:PlacementSpecification;
        rdfs:label          "dimension"@en;
        rdfs:range          vec:Dimension;
        rdfs:subPropertyOf  vec:contains .

vec:componentNodeNetworkNode
        rdf:type      owl:ObjectProperty;
        rdfs:comment  "References the NetworkNode that is realized by the ComponentNode.\n"@en;
        rdfs:domain   vec:ComponentNode;
        rdfs:label    "networkNode"@en;
        rdfs:range    vec:NetworkNode .

vec:terminalSpecificationCurrentInformation
        rdf:type            owl:ObjectProperty;
        rdfs:comment        "Specifies the TerminalCurrentInformation that is applicable for the terminal.\n"@en;
        rdfs:domain         vec:TerminalSpecification;
        rdfs:label          "currentInformation"@en;
        rdfs:range          vec:TerminalCurrentInformation;
        rdfs:subPropertyOf  vec:contains .

vec:LanguageCode_Ps  rdf:type  vec:LanguageCode , owl:NamedIndividiual;
        vec:enumLiteral  "Ps" .

vec:conductorSpecificationPlatingMaterial
        rdf:type            owl:ObjectProperty;
        rdfs:comment        "Specifies the plating material of the conductor.\n"@en;
        rdfs:domain         vec:ConductorSpecification;
        rdfs:label          "platingMaterial"@en;
        rdfs:range          vec:Material;
        rdfs:subPropertyOf  vec:contains .

vec:ConfigurableElement
        rdf:type         owl:Class;
        rdfs:comment     "Abstract base class for all elements which can be configured with a VariantConfiguration.\n"@en;
        rdfs:label       "ConfigurableElement"@en;
        rdfs:subClassOf  vec:ExtendableElement .

vec:zoneRequiredSealingClass
        rdf:type            owl:ObjectProperty;
        rdfs:comment        "Defines the SealingClass that is required in this Zone.\n"@en;
        rdfs:domain         vec:Zone;
        rdfs:label          "requiredSealingClass"@en;
        rdfs:range          vec:SealingClass;
        rdfs:subPropertyOf  vec:contains .

vec:SignalDirection_InOut
        rdf:type         vec:SignalDirection , owl:NamedIndividiual;
        vec:enumLiteral  "InOut" .

vec:cavityReferenceReferencedCavity
        rdf:type      owl:ObjectProperty;
        rdfs:comment  "Points to the cavity referenced by the cavity reference. \n"@en;
        rdfs:domain   vec:CavityReference;
        rdfs:label    "referencedCavity"@en;
        rdfs:range    vec:Cavity .

vec:LanguageCode_Gu  rdf:type  vec:LanguageCode , owl:NamedIndividiual;
        vec:enumLiteral  "Gu" .

vec:powerConsumptionType
        rdf:type      owl:DatatypeProperty;
        rdfs:comment  "The type of a PowerConsumption . This should be an enumeration of values defined in a conformance class.\n"@en;
        rdfs:domain   vec:PowerConsumption;
        rdfs:label    "type"@en;
        rdfs:range    xs:string .

vec:UsageNodeType_Splice
        rdf:type         vec:UsageNodeType , owl:NamedIndividiual;
        vec:enumLiteral  "Splice" .

vec:pinComponentPinSpecification
        rdf:type      owl:ObjectProperty;
        rdfs:comment  "References the TerminalSpecification describing the electrical connectivity aspect of the PinComponent. \n(see KBLFRM-300)\n"@en;
        rdfs:domain   vec:PinComponent;
        rdfs:label    "pinSpecification"@en;
        rdfs:range    vec:TerminalSpecification .

vec:SignalForm  rdf:type  owl:Class;
        rdfs:label       "SignalForm"@en;
        rdfs:subClassOf  vec:OpenEnumeration .

vec:AbstractSlot  rdf:type  owl:Class;
        rdfs:comment     "An AbstractSlot is a geometrical place in a connector housing, which can contain / group cavities. This can be either direct, if it is Slot and indirect if it is a ModularSlot .\nIf it is a Slot , than it is an inseparable part of the connector housing, which means it is created during the manufacturing process of the connector housing.\nIf it is a ModularSlot it is a place where one or more other connector housing can be place during the assembly.\n"@en;
        rdfs:label       "AbstractSlot"@en;
        rdfs:subClassOf  vec:ExtendableElement .

vec:topologySegmentEndNode
        rdf:type      owl:ObjectProperty;
        rdfs:comment  "References the TopologyNode where the TopologySegment ends. \n"@en;
        rdfs:domain   vec:TopologySegment;
        rdfs:label    "endNode"@en;
        rdfs:range    vec:TopologyNode .

vec:LanguageCode_Fr  rdf:type  vec:LanguageCode , owl:NamedIndividiual;
        vec:enumLiteral  "Fr" .

vec:transformation3DA22
        rdf:type     owl:DatatypeProperty;
        rdfs:domain  vec:Transformation3D;
        rdfs:label   "a22"@en;
        rdfs:range   xs:double .

vec:USUnitName_Quart  rdf:type  vec:USUnitName , owl:NamedIndividiual;
        vec:enumLiteral  "Quart" .

vec:ringTerminalSpecificationOutsideDimension
        rdf:type            owl:ObjectProperty;
        rdfs:comment        "Specifies the diameter of the circle around the center of the bolt which passes through the farthest outside point of the contact surface of the ring terminal. (see KBLFRM-311)\n"@en;
        rdfs:domain         vec:RingTerminalSpecification;
        rdfs:label          "outsideDimension"@en;
        rdfs:range          vec:NumericalValue;
        rdfs:subPropertyOf  vec:contains .

vec:SignalTransmissionMediumType_Hydraulic
        rdf:type         vec:SignalTransmissionMediumType , owl:NamedIndividiual;
        vec:enumLiteral  "hydraulic" .

vec:WireMounting  rdf:type  owl:Class;
        rdfs:comment     "A wire mouting defines the mouting of a wire end to terminal. If the contacting is required to be water proof a cavity seal can be mounted additionally.\n"@en;
        rdfs:label       "WireMounting"@en;
        rdfs:subClassOf  vec:ExtendableElement .

vec:wireElementSpecificationSize
        rdf:type            owl:ObjectProperty;
        rdfs:comment        "Defines the size of a WireElement if it has not the shape of circle. If it has the shape of a circle the size is normally defined by its outside diameter.\n"@en;
        rdfs:domain         vec:WireElementSpecification;
        rdfs:label          "size"@en;
        rdfs:range          vec:Size;
        rdfs:subPropertyOf  vec:contains .

vec:LanguageCode_Eo  rdf:type  vec:LanguageCode , owl:NamedIndividiual;
        vec:enumLiteral  "Eo" .

vec:segmentLocationAnchor
        rdf:type            owl:ObjectProperty;
        rdfs:comment        "Specifies if the location on the TopologySegment is defined as on offset relative to the startNode of the TopologySegment or the endNode."@en;
        rdfs:domain         vec:SegmentLocation;
        rdfs:label          "anchor"@en;
        rdfs:range          vec:AnchorType;
        rdfs:subPropertyOf  vec:contains .

vec:occurrenceOrUsageViewItem3DIdentification
        rdf:type      owl:DatatypeProperty;
        rdfs:comment  "Specifies a unique identification of the OccurrenceOrUsageViewItem. The identification is guaranteed to be unique within the BuildingBlockSpecification3D.\n"@en;
        rdfs:domain   vec:OccurrenceOrUsageViewItem3D;
        rdfs:label    "identification"@en;
        rdfs:range    xs:string .

vec:USUnitName  rdf:type     owl:Class;
        rdfs:comment         "Enumeration for the definition of US unit names.\n"@en;
        rdfs:label           "USUnitName"@en;
        rdfs:subClassOf      vec:ClosedEnumeration;
        owl:equivalentClass  [ rdf:type   owl:Class;
                               owl:oneOf  ( vec:USUnitName_Thou vec:USUnitName_Inch vec:USUnitName_Foot vec:USUnitName_Yard vec:USUnitName_Chain vec:USUnitName_Furlong vec:USUnitName_Mile vec:USUnitName_League vec:USUnitName_FluidOunce vec:USUnitName_Gill vec:USUnitName_Pint vec:USUnitName_Quart vec:USUnitName_Gallon vec:USUnitName_Grain vec:USUnitName_Drachm vec:USUnitName_Ounce vec:USUnitName_Pound vec:USUnitName_Stone vec:USUnitName_Quarter vec:USUnitName_HundredWeight vec:USUnitName_Ton vec:USUnitName_Perch vec:USUnitName_Rood vec:USUnitName_Acre vec:USUnitName_AWG )
                             ] .

vec:GrommetSpecification
        rdf:type         owl:Class;
        rdfs:comment     "Specification for the definition of grommets.\n"@en;
        rdfs:label       "GrommetSpecification"@en;
        rdfs:subClassOf  vec:PartOrUsageRelatedSpecification .

vec:slotCavity  rdf:type    owl:ObjectProperty;
        rdfs:comment        "Specifies the Cavities forming the Slot.\n"@en;
        rdfs:domain         vec:Slot;
        rdfs:label          "cavity"@en;
        rdfs:range          vec:Cavity;
        rdfs:subPropertyOf  vec:contains .

vec:connectorHousingSpecificationCoding
        rdf:type            owl:ObjectProperty;
        rdfs:comment        "Defines coding of the connector housing that is satisfied by the connector housing. \n"@en;
        rdfs:domain         vec:ConnectorHousingSpecification;
        rdfs:label          "coding"@en;
        rdfs:range          vec:Coding;
        rdfs:subPropertyOf  vec:contains .

vec:WireGroupingSpecification
        rdf:type         owl:Class;
        rdfs:comment     "Specification for the description of WireGroupings.\n"@en;
        rdfs:label       "WireGroupingSpecification"@en;
        rdfs:subClassOf  vec:Specification .

vec:ImperialUnitName_Quart
        rdf:type         vec:ImperialUnitName , owl:NamedIndividiual;
        vec:enumLiteral  "Quart" .

vec:conductorSpecificationMassInformation
        rdf:type            owl:ObjectProperty;
        rdfs:comment        "Specifies the mass information of the conductor. In most cases this mass information is known as copper weight and is normally specified as mass per length (e.g. gram per meter).\n"@en;
        rdfs:domain         vec:ConductorSpecification;
        rdfs:label          "massInformation"@en;
        rdfs:range          vec:MassInformation;
        rdfs:subPropertyOf  vec:contains .

vec:insulationSpecificationThickness
        rdf:type            owl:ObjectProperty;
        rdfs:comment        "Specifies the thickness of the insulation.\n"@en;
        rdfs:domain         vec:InsulationSpecification;
        rdfs:label          "thickness"@en;
        rdfs:range          vec:NumericalValue;
        rdfs:subPropertyOf  vec:contains .

vec:TopologySpecification
        rdf:type         owl:Class;
        rdfs:comment     "Specification for the definition of a topology. A topology consists of TopologyNodes, TopologySegments and Zones.\n"@en;
        rdfs:label       "TopologySpecification"@en;
        rdfs:subClassOf  vec:Specification .

vec:usageNodeAbbreviation
        rdf:type            owl:ObjectProperty;
        rdfs:comment        "Specifies an abbreviation of the UsageNode . Normally this a human readable short name.\n"@en;
        rdfs:domain         vec:UsageNode;
        rdfs:label          "abbreviation"@en;
        rdfs:range          vec:LocalizedString;
        rdfs:subPropertyOf  vec:contains .

vec:sealingClassDescription
        rdf:type            owl:ObjectProperty;
        rdfs:comment        "On optional human readable description of the sealing class (e.g. the name).\n"@en;
        rdfs:domain         vec:SealingClass;
        rdfs:label          "description"@en;
        rdfs:range          vec:AbstractLocalizedString;
        rdfs:subPropertyOf  vec:contains .

vec:changeDescriptionDescription
        rdf:type            owl:ObjectProperty;
        rdfs:comment        "Specifies additional, human readable, information about the ChangeDescription.\n"@en;
        rdfs:domain         vec:ChangeDescription;
        rdfs:label          "description"@en;
        rdfs:range          vec:AbstractLocalizedString;
        rdfs:subPropertyOf  vec:contains .

vec:SpecificRole  rdf:type  owl:Class;
        rdfs:comment     "A SpecificRole is the possibility to define instance specific properties with custom properties (see ExtendableElement). This is necessary, if the part is described by custom properties of a PartOrUsageRelatedSpecification.\n"@en;
        rdfs:label       "SpecificRole"@en;
        rdfs:subClassOf  vec:Role .

vec:SignalDirection_Out
        rdf:type         vec:SignalDirection , owl:NamedIndividiual;
        vec:enumLiteral  "Out" .

vec:Enumeration  rdf:type  owl:Class;
        rdfs:comment  "Classes in the model that can be enumerated, either closed or open (see VEC Specicification)"@en;
        rdfs:label    "Enumeration"@en .

vec:TerminalReceptionReference
        rdf:type      owl:Class;
        rdfs:comment  "A TerminalReceptionReference is an instance of a TerminalReception .\n"@en;
        rdfs:label    "TerminalReceptionReference"@en .

vec:Person  rdf:type  owl:Class;
        rdfs:comment  "Specifies all relevant data of a person.\n"@en;
        rdfs:label    "Person"@en .

vec:personEmailAddress
        rdf:type      owl:DatatypeProperty;
        rdfs:comment  "Specifies the person's email address.\n"@en;
        rdfs:domain   vec:Person;
        rdfs:label    "emailAddress"@en;
        rdfs:range    xs:string .

vec:ImperialUnitName_Pint
        rdf:type         vec:ImperialUnitName , owl:NamedIndividiual;
        vec:enumLiteral  "Pint" .

vec:terminalReceptionTerminalReceptionSpecification
        rdf:type      owl:ObjectProperty;
        rdfs:comment  "References the TerminalReceptionSpecification that specifies the TerminalReception.\n"@en;
        rdfs:domain   vec:TerminalReception;
        rdfs:label    "terminalReceptionSpecification"@en;
        rdfs:range    vec:TerminalReceptionSpecification .

vec:pathSegment  rdf:type   owl:ObjectProperty;
        rdfs:comment        "This association is defined as unique='false' and ordered='true'. This can not be represented efficiently directly in RDF/OWL. Therefore, this association references Wrappers as proxies to the actual elements, instead of the actual elements itself (like a regular association)." , "Specifies an ordered list of TopologySegments the routing goes through. \n"@en;
        rdfs:domain         vec:Path;
        rdfs:label          "segment"@en;
        rdfs:range          vec:TopologySegmentWrapper , vec:Ordered;
        rdfs:subPropertyOf  vec:contains .

vec:LanguageCode_Ja  rdf:type  vec:LanguageCode , owl:NamedIndividiual;
        vec:enumLiteral  "Ja" .

[ rdf:type     owl:AllDisjointClasses;
  owl:members  ( vec:CompatibilitySpecification vec:ContactSystemSpecification vec:ContactingSpecification vec:PartOrUsageRelatedSpecification vec:CavitySpecification vec:ConductorSpecification vec:FillerSpecification vec:InsulationSpecification vec:SlotSpecification vec:TerminalReceptionSpecification vec:WireElementSpecification vec:WireGroupSpecification vec:WireReceptionSpecification vec:ExternalMappingSpecification vec:BuildingBlockSpecification2D vec:HarnessDrawingSpecification2D vec:BuildingBlockSpecification3D vec:HarnessGeometrySpecification3D vec:WireGroupingSpecification vec:MappingSpecification vec:MatingSpecification vec:ModuleFamilySpecification vec:ModuleListSpecification vec:NetSpecification vec:CompositionSpecification vec:PartUsageSpecification vec:PlacementSpecification vec:RoutingSpecification vec:ConnectionSpecification vec:SignalSpecification vec:TopologySpecification vec:UsageConstraintSpecification vec:UsageNodeSpecification vec:VariantCodeSpecification vec:VariantConfigurationSpecification vec:VariantGroupSpecification )
] .

vec:wireTypeReferenceSystem
        rdf:type      owl:DatatypeProperty;
        rdfs:comment  "Specifies the reference system for the wire type.\n"@en;
        rdfs:domain   vec:WireType;
        rdfs:label    "referenceSystem"@en;
        rdfs:range    xs:string .

vec:pinComponentBehaviour
        rdf:type            owl:ObjectProperty;
        rdfs:comment        "Specifies the configuration dependent electrical behavior of the PinComponent.\n"@en;
        rdfs:domain         vec:PinComponent;
        rdfs:label          "behaviour"@en;
        rdfs:range          vec:PinComponentBehavior;
        rdfs:subPropertyOf  vec:contains .

vec:ImperialUnitName_Ounce
        rdf:type         vec:ImperialUnitName , owl:NamedIndividiual;
        vec:enumLiteral  "Ounce" .

vec:matingPointMatingDetail
        rdf:type            owl:ObjectProperty;
        rdfs:comment        "Specifies the MatingDetails, if a detailed description of the relationships between TerminalReceptions and TerminalReceptions is needed. \n"@en;
        rdfs:domain         vec:MatingPoint;
        rdfs:label          "matingDetail"@en;
        rdfs:range          vec:MatingDetail;
        rdfs:subPropertyOf  vec:contains .

vec:variantCodeDescription
        rdf:type            owl:ObjectProperty;
        rdfs:comment        "On optional human readable description of the variant code.\n"@en;
        rdfs:domain         vec:VariantCode;
        rdfs:label          "description"@en;
        rdfs:range          vec:AbstractLocalizedString;
        rdfs:subPropertyOf  vec:contains .

vec:VecContent  rdf:type  owl:Class;
        rdfs:comment     "The VecContent is the XML-Root node for any VEC-Document.\n"@en;
        rdfs:label       "VecContent"@en;
        rdfs:subClassOf  vec:ExtendableElement .

vec:SiUnitName_Candela
        rdf:type         vec:SiUnitName , owl:NamedIndividiual;
        vec:enumLiteral  "Candela" .

vec:TopologySegment  rdf:type  owl:Class;
        rdfs:comment     "A TopologySegment is a distance in the Topology where no intermediate electrical contacts appear. If a Topology contains routed wires, then the wire at the beginning of a TopologySegment have to be the same as in the ending.\n"@en;
        rdfs:label       "TopologySegment"@en;
        rdfs:subClassOf  vec:ConfigurableElement .

vec:terminalRoleWireReceptionReference
        rdf:type            owl:ObjectProperty;
        rdfs:comment        "Specifies the WireReceptionReferences of this TerminalRole.\n"@en;
        rdfs:domain         vec:TerminalRole;
        rdfs:label          "wireReceptionReference"@en;
        rdfs:range          vec:WireReceptionReference;
        rdfs:subPropertyOf  vec:contains .

vec:SlotGender  rdf:type  owl:Class;
        rdfs:comment     "Defines the gender of a slot.\n"@en;
        rdfs:label       "SlotGender"@en;
        rdfs:subClassOf  vec:OpenEnumeration .

vec:connectorHousingRoleSealState
        rdf:type            owl:ObjectProperty;
        rdfs:comment        "Specifies if this instance of a connector housing should be sealed (waterproof).\n"@en;
        rdfs:domain         vec:ConnectorHousingRole;
        rdfs:label          "sealState"@en;
        rdfs:range          vec:SealState;
        rdfs:subPropertyOf  vec:contains .

vec:terminalTypeName  rdf:type  owl:DatatypeProperty;
        rdfs:comment  "Specifies the type of the cavity (e.g. MQS, DFK, ...).\n"@en;
        rdfs:domain   vec:TerminalType;
        rdfs:label    "name"@en;
        rdfs:range    xs:string .

vec:PartRelationType  rdf:type  owl:Class;
        rdfs:comment         "Defines how the set of acessoryParts referenced by a PartRelation should be interpreted.\n"@en;
        rdfs:label           "PartRelationType"@en;
        rdfs:subClassOf      vec:ClosedEnumeration;
        owl:equivalentClass  [ rdf:type   owl:Class;
                               owl:oneOf  ( vec:PartRelationType_Mandatory vec:PartRelationType_Optional vec:PartRelationType_OneOfAll )
                             ] .

vec:GeometryType_Formboard
        rdf:type         vec:GeometryType , owl:NamedIndividiual;
        rdfs:comment     "The Geometry is a model of a Formboard.\n"@en;
        vec:enumLiteral  "Formboard" .

vec:HistoryEntryType_Derivation
        rdf:type         vec:HistoryEntryType , owl:NamedIndividiual;
        vec:enumLiteral  "Derivation" .

vec:netIdentification
        rdf:type      owl:DatatypeProperty;
        rdfs:comment  "Specifies a unique identification of the Net. The identification is guaranteed to be unique within the NetSpecification.\n"@en;
        rdfs:domain   vec:Net;
        rdfs:label    "identification"@en;
        rdfs:range    xs:string .

vec:ConformanceClass  rdf:type  owl:Class;
        rdfs:comment     "The ConformanceClass element represents a link to a ConformanceClass to which the vec-file is compliant.\n"@en;
        rdfs:label       "ConformanceClass"@en;
        rdfs:subClassOf  vec:ExtendableElement .

vec:internalTerminalConnectionTerminalReception
        rdf:type      owl:ObjectProperty;
        rdfs:comment  "References the TerminalReceptions that participate in the InternalTerminalConnection.\n"@en;
        rdfs:domain   vec:InternalTerminalConnection;
        rdfs:label    "terminalReception"@en;
        rdfs:range    vec:TerminalReception .

vec:PinComponentBehavior
        rdf:type         owl:Class;
        rdfs:comment     "A PinComponentBehavior specifies the electrical behavior of a PinComponent. Since the behavior of a pin is configuration dependent (e.g. the software deployed on an ECU) the PinComponentBehavior inherits from ConfigurableElement. Therefore a PinComponent can specify multiple PinComponentBehavior.\n"@en;
        rdfs:label       "PinComponentBehavior"@en;
        rdfs:subClassOf  vec:ConfigurableElement .

vec:PrimaryPartType_SpliceTerminal
        rdf:type         vec:PrimaryPartType , owl:NamedIndividiual;
        vec:enumLiteral  "SpliceTerminal" .

vec:netSpecificationNet
        rdf:type            owl:ObjectProperty;
        rdfs:comment        "Specifies the Nets defined in the NetSpecification.\n"@en;
        rdfs:domain         vec:NetSpecification;
        rdfs:label          "net"@en;
        rdfs:range          vec:Net;
        rdfs:subPropertyOf  vec:contains .

vec:InsulationState  rdf:type  owl:Class;
        rdfs:comment     "Enumeration for the definition of the insulation state of the splice.\n"@en;
        rdfs:label       "InsulationState"@en;
        rdfs:subClassOf  vec:OpenEnumeration .

vec:eEComponentRoleEEComponentSpecification
        rdf:type      owl:ObjectProperty;
        rdfs:comment  "References the EEComponentSpecification that is instanced by this EEComponentRole.\n"@en;
        rdfs:domain   vec:EEComponentRole;
        rdfs:label    "EEComponentSpecification"@en;
        rdfs:range    vec:EEComponentSpecification .

vec:buildingBlockSpecification2DBaseUnit
        rdf:type      owl:ObjectProperty;
        rdfs:comment  ""@en;
        rdfs:domain   vec:BuildingBlockSpecification2D;
        rdfs:label    "baseUnit"@en;
        rdfs:range    vec:Unit .

vec:LanguageCode_Et  rdf:type  vec:LanguageCode , owl:NamedIndividiual;
        vec:enumLiteral  "Et" .

vec:cartesianPoint2DY
        rdf:type      owl:DatatypeProperty;
        rdfs:comment  "Specifies the value of y-coordinate of the Cartesian point. The unit of this value is the baseUnit of containing BuildingBlockSpecification2D.\n"@en;
        rdfs:domain   vec:CartesianPoint2D;
        rdfs:label    "y"@en;
        rdfs:range    xs:double .

vec:SpliceTerminalRole
        rdf:type         owl:Class;
        rdfs:comment     "A SpliceTerminalRole defines the instance specific properties and relationships of a splice terminal.\n"@en;
        rdfs:label       "SpliceTerminalRole"@en;
        rdfs:subClassOf  vec:TerminalRole .

vec:partOccurrenceIsSecondaryAlternative
        rdf:type      owl:DatatypeProperty;
        rdfs:comment  "If a PartUsage is realized by more than one PartOccurrence it is possible to specify which one is the preferred. (see KBLFRM-264)\n"@en;
        rdfs:domain   vec:PartOccurrence;
        rdfs:label    "isSecondaryAlternative"@en;
        rdfs:range    xs:boolean .

vec:HoleMountedFixingSpecification
        rdf:type         owl:Class;
        rdfs:comment     "Specification for fixings that are mounted with a hole. This means, the fixing itself has got a hole, which is mounted onto a bolt.\n"@en;
        rdfs:label       "HoleMountedFixingSpecification"@en;
        rdfs:subClassOf  vec:FixingSpecification .

vec:BSplineCurve  rdf:type  owl:Class;
        rdfs:comment     "A B-spline curve is a piecewise parametric polynomial or rational curve described in terms of control points and basis functions. The B-spline curve has been selected as the most stable format to represent all types of polynomial or rational parametric curves. With appropriate attribute values it is capable of representing single span or spline curves of explicit polynomial, rational, Bezier or B-spline type.\nWithin the Harness Engineering Information Model the definition has been restricted to a uniform B_spline_curve, where the knots are evenly spaced. Suitable default values for the knots and knot multiplicities are derived in this case. A B-spline is uniform if and only if all knots are of multiplicity 1 and they differ by a positive constant from the preceding knot. In this case the knot spacing is 1.0, starting at -d, where d is the degree.\nNote: If the B-spline curve is uniform and degree=1, the B-spline is equivalent to a polyline.\n"@en;
        rdfs:label       "BSplineCurve"@en;
        rdfs:subClassOf  vec:ExtendableElement .

vec:LanguageCode_Mo  rdf:type  vec:LanguageCode , owl:NamedIndividiual;
        vec:enumLiteral  "Mo" .

vec:ImperialUnitName_Foot
        rdf:type         vec:ImperialUnitName , owl:NamedIndividiual;
        vec:enumLiteral  "Foot" .

vec:holeMountedFixingSpecificationPlateThickness
        rdf:type            owl:ObjectProperty;
        rdfs:comment        "Specifies the thickness of the plate in which the hole is positioned.\n"@en;
        rdfs:domain         vec:HoleMountedFixingSpecification;
        rdfs:label          "plateThickness"@en;
        rdfs:range          vec:ValueRange;
        rdfs:subPropertyOf  vec:contains .

vec:materialReferenceSystem
        rdf:type      owl:DatatypeProperty;
        rdfs:comment  "The identification of the material reference system, which is defining possible values and the semantic of material keys.\n"@en;
        rdfs:domain   vec:Material;
        rdfs:label    "referenceSystem"@en;
        rdfs:range    xs:string .

vec:SegmentCrossSectionArea
        rdf:type         owl:Class;
        rdfs:comment     "Specifies the cross section area of a segment. For the data exchange the cross section area is used and not the diameter, because the diameter is only a valid measure for circular segments. For circular segments, the diameter and the cross section area can be translated into each other without the loss of information. Attributes of the type SegmentCrossSectionArea normally have the multiplicity [0..*]. This means that such an attribute can have SegmentCrossSectionArea entries for different crossSectionAreaTypes and valueDeterminations. It must not have multiple entries with the same crossSectionAreaType and valueDetermination.\n"@en;
        rdfs:label       "SegmentCrossSectionArea"@en;
        rdfs:subClassOf  vec:ExtendableElement .

vec:PartUsage  rdf:type  owl:Class;
        rdfs:comment     "PartUsages shall be used for the specification of the elements on an electrical system wiring plan and for the specification of the elements on a pure geometry description. PartUsages shall more than ever be used in cases where it is necessary to describe a certain instance of a part or part group, possibly together with certain technical properties, but where it is at the same time yet not possible to define a concrete part number.\n"@en;
        rdfs:label       "PartUsage"@en;
        rdfs:subClassOf  vec:OccurrenceOrUsage .

vec:pinCurrentInformationType
        rdf:type            owl:ObjectProperty;
        rdfs:comment        "Defines the type of the current.\n"@en;
        rdfs:domain         vec:PinCurrentInformation;
        rdfs:label          "type"@en;
        rdfs:range          vec:PinCurrentType;
        rdfs:subPropertyOf  vec:contains .

vec:Transformation3D  rdf:type  owl:Class;
        rdfs:comment     "A Transformation is a geometric transformation and specifies a transformation matrix.\n"@en;
        rdfs:label       "Transformation3D"@en;
        rdfs:subClassOf  vec:ExtendableElement .

vec:LengthClassification
        rdf:type         owl:Class;
        rdfs:comment     "Enumeration for the definition of a LengthClassification.\n"@en;
        rdfs:label       "LengthClassification"@en;
        rdfs:subClassOf  vec:OpenEnumeration .

vec:sealingClassClassKey
        rdf:type      owl:DatatypeProperty;
        rdfs:comment  "Specifies a key for the sealing level defined in the specified sealing class (e.g. A, B, C).\n"@en;
        rdfs:domain   vec:SealingClass;
        rdfs:label    "classKey"@en;
        rdfs:range    xs:string .

vec:cavityMountingDetailEquippedCavityRef
        rdf:type      owl:ObjectProperty;
        rdfs:comment  "References the cavity that is used for the detailed description of the cavity mounting. \n"@en;
        rdfs:domain   vec:CavityMountingDetail;
        rdfs:label    "equippedCavityRef"@en;
        rdfs:range    vec:CavityReference .

vec:vecContentItemHistoryEntry
        rdf:type            owl:ObjectProperty;
        rdfs:comment        "Specifies the ItemVersionHistoryEntries for ItemVersions contained in the VEC-file. \n"@en;
        rdfs:domain         vec:VecContent;
        rdfs:label          "itemHistoryEntry"@en;
        rdfs:range          vec:ItemHistoryEntry;
        rdfs:subPropertyOf  vec:contains .

vec:grommetSpecificationHoleDiameter
        rdf:type            owl:ObjectProperty;
        rdfs:comment        "Specifies the valid diameter of a hole into which the grommet fits.\n"@en;
        rdfs:domain         vec:GrommetSpecification;
        rdfs:label          "holeDiameter"@en;
        rdfs:range          vec:NumericalValue;
        rdfs:subPropertyOf  vec:contains .

vec:LanguageCode_Tg  rdf:type  vec:LanguageCode , owl:NamedIndividiual;
        vec:enumLiteral  "Tg" .

vec:onPointPlacementLocation
        rdf:type            owl:ObjectProperty;
        rdfs:comment        "References the Locations where Placement places the reference points of the placed element. \n"@en;
        rdfs:domain         vec:OnPointPlacement;
        rdfs:label          "location"@en;
        rdfs:range          vec:Location;
        rdfs:subPropertyOf  vec:contains .

vec:DocumentBasedInstruction
        rdf:type         owl:Class;
        rdfs:comment     "A DocumentBasedInstruction is an Instruction to a SheetOrChapter in a DocumentVersion or to a complete DocumentVersion.\n"@en;
        rdfs:label       "DocumentBasedInstruction"@en;
        rdfs:subClassOf  vec:Instruction .

vec:GeneralTechnicalPartSpecification
        rdf:type         owl:Class;
        rdfs:comment     "Specification for the definition of common properties for technical parts.\n"@en;
        rdfs:label       "GeneralTechnicalPartSpecification"@en;
        rdfs:subClassOf  vec:PartOrUsageRelatedSpecification .

vec:cavityMountingEquippedCavityRef
        rdf:type      owl:ObjectProperty;
        rdfs:comment  "References the cavities that are used for the cavity mounting. \n"@en;
        rdfs:domain   vec:CavityMounting;
        rdfs:label    "equippedCavityRef"@en;
        rdfs:range    vec:CavityReference .

vec:GeometrySegment2D
        rdf:type         owl:Class;
        rdfs:comment     "A GeometrySegment2D is the geometric representation of a TopologySegment in 2D-space.\n"@en;
        rdfs:label       "GeometrySegment2D"@en;
        rdfs:subClassOf  vec:GeometrySegment .

vec:USUnitName_Pint  rdf:type  vec:USUnitName , owl:NamedIndividiual;
        vec:enumLiteral  "Pint" .

vec:contractContractRole
        rdf:type            owl:ObjectProperty;
        rdfs:comment        "The role the company takes in reference to the associated ItemVersion. Predefined are the values: Oem, Supplier and Manufacturer.\n"@en;
        rdfs:domain         vec:Contract;
        rdfs:label          "contractRole"@en;
        rdfs:range          vec:ContractRole;
        rdfs:subPropertyOf  vec:contains .

vec:networkPortSignal
        rdf:type      owl:ObjectProperty;
        rdfs:comment  "References the signal that is associated with the NetworkPort.\n"@en;
        rdfs:domain   vec:NetworkPort;
        rdfs:label    "signal"@en;
        rdfs:range    vec:Signal .

vec:LanguageCode_Sd  rdf:type  vec:LanguageCode , owl:NamedIndividiual;
        vec:enumLiteral  "Sd" .

vec:SiPrefix_Deca  rdf:type  vec:SiPrefix , owl:NamedIndividiual;
        vec:enumLiteral  "Deca" .

vec:PinCurrentInformation
        rdf:type      owl:Class;
        rdfs:comment  "Allows the definition of currents for a pin of an EEComponent. A current can be further specified by a duration. Attributes of the type PinCurrentInformation normally have the multiplicity [0..*]. This means that such an attribute can have PinCurrentInformation entries for different types and durations. It must not have multiple entries for the same type and duration.\n"@en;
        rdfs:label    "PinCurrentInformation"@en .

[ rdf:type     owl:AllDisjointClasses;
  owl:members  ( vec:PluggableTerminalRole vec:RingTerminalRole vec:SpliceTerminalRole )
] .

vec:geometrySegment3DBSplineCurve
        rdf:type            owl:ObjectProperty;
        rdfs:comment        "Specifies an ordered list of BSplineCurves defining the 3D appearance of the GeometrySegment3D. \n"@en;
        rdfs:domain         vec:GeometrySegment3D;
        rdfs:label          "bSplineCurve"@en;
        rdfs:range          vec:BSplineCurve , vec:Ordered;
        rdfs:subPropertyOf  vec:contains .

vec:ConnectorHousingRole
        rdf:type         owl:Class;
        rdfs:comment     "A ConnectorHousingRole defines the instance specific properties and relationships of a connector housing.\n"@en;
        rdfs:label       "ConnectorHousingRole"@en;
        rdfs:subClassOf  vec:Role .

vec:sIUnitSiUnitName  rdf:type  owl:ObjectProperty;
        rdfs:comment        "Specifies the name of SI unit (e.g. metre, second,...)\n"@en;
        rdfs:domain         vec:SIUnit;
        rdfs:label          "siUnitName"@en;
        rdfs:range          vec:SiUnitName;
        rdfs:subPropertyOf  vec:contains .

vec:IECPrefix_Yobi  rdf:type  vec:IECPrefix , owl:NamedIndividiual;
        vec:enumLiteral  "Yobi" .

vec:geometrySegment2DStartNode
        rdf:type      owl:ObjectProperty;
        rdfs:comment  "References the GeometryNode2D where the GeometrySegment2D starts. \n"@en;
        rdfs:domain   vec:GeometrySegment2D;
        rdfs:label    "startNode"@en;
        rdfs:range    vec:GeometryNode2D .

vec:variantConfigurationDescription
        rdf:type            owl:ObjectProperty;
        rdfs:comment        "On optional human readable description of the variant configuration.\n"@en;
        rdfs:domain         vec:VariantConfiguration;
        rdfs:label          "description"@en;
        rdfs:range          vec:AbstractLocalizedString;
        rdfs:subPropertyOf  vec:contains .

vec:connectorHousingSpecificationSlot
        rdf:type            owl:ObjectProperty;
        rdfs:comment        "Specifies the slots forming the ConnectorHousing. \n"@en;
        rdfs:domain         vec:ConnectorHousingSpecification;
        rdfs:label          "slot"@en;
        rdfs:range          vec:AbstractSlot;
        rdfs:subPropertyOf  vec:contains .

vec:approvalLevelOfApproval
        rdf:type      owl:DatatypeProperty;
        rdfs:comment  "Describes activities that can be started after release for example building pilot tools or production tools.\n"@en;
        rdfs:domain   vec:Approval;
        rdfs:label    "levelOfApproval"@en;
        rdfs:range    xs:string .

vec:grommetSpecificationHardness
        rdf:type            owl:ObjectProperty;
        rdfs:comment        "Specifies the hardness of the grommet.\n"@en;
        rdfs:domain         vec:GrommetSpecification;
        rdfs:label          "hardness"@en;
        rdfs:range          vec:NumericalValue;
        rdfs:subPropertyOf  vec:contains .

vec:CableDuctRole  rdf:type  owl:Class;
        rdfs:comment     "A GrommetRole defines the instance specific properties and relationships of a grommet.\n"@en;
        rdfs:label       "CableDuctRole"@en;
        rdfs:subClassOf  vec:Role .

vec:USUnitName_Yard  rdf:type  vec:USUnitName , owl:NamedIndividiual;
        vec:enumLiteral  "Yard" .

[ rdf:type     owl:AllDisjointClasses;
  owl:members  ( vec:CavityPlugSpecification vec:CavitySealSpecification vec:ConnectorHousingSpecification vec:EEComponentSpecification vec:GeneralTechnicalPartSpecification vec:TerminalSpecification vec:WireSpecification vec:CableDuctSpecification vec:FixingSpecification vec:GrommetSpecification vec:WireProtectionSpecification vec:PartStructureSpecification vec:PlaceableElementSpecification )
] .

vec:slotMappingIdentificationA
        rdf:type      owl:DatatypeProperty;
        rdfs:comment  "The identification of the Slot on side A\n"@en;
        rdfs:domain   vec:SlotMapping;
        rdfs:label    "identificationA"@en;
        rdfs:range    xs:string .

vec:RoutingSpecification
        rdf:type         owl:Class;
        rdfs:comment     "Specification for the description of Routings.\n"@en;
        rdfs:label       "RoutingSpecification"@en;
        rdfs:subClassOf  vec:Specification .

vec:boltMountedFixingSpecificationBoltHeight
        rdf:type            owl:ObjectProperty;
        rdfs:comment        "Specifies the height of the bolt of the fixing.\n"@en;
        rdfs:domain         vec:BoltMountedFixingSpecification;
        rdfs:label          "boltHeight"@en;
        rdfs:range          vec:NumericalValue;
        rdfs:subPropertyOf  vec:contains .

vec:topologyNodeNodeType
        rdf:type            owl:ObjectProperty;
        rdfs:comment        "Specifies the type of the TopologyNode. A Node can either be an EndNode, a Junction or an Inliner.\n"@en;
        rdfs:domain         vec:TopologyNode;
        rdfs:label          "nodeType"@en;
        rdfs:range          vec:NodeType;
        rdfs:subPropertyOf  vec:contains .

vec:topologyNodeAliasId
        rdf:type            owl:ObjectProperty;
        rdfs:comment        "Specifies additional identifiers for the TopologyNode.\nExample: TopologyNode Ids may vary from one CAD system export to another. Therefore the CAD system Id is improper for identification attribute. The identification shall have a value which is unique within the Topology. AliasId may be used for the CAD system Id.\n"@en;
        rdfs:domain         vec:TopologyNode;
        rdfs:label          "aliasId"@en;
        rdfs:range          vec:AliasIdentification;
        rdfs:subPropertyOf  vec:contains .

vec:CartesianPoint2DWrapper
        rdf:type      owl:Class;
        rdfs:comment  "Container class for CartesianPoint2D to participate in non-unique and/or ordered associations." .

vec:buildingBlockSpecification2DCartesianPoint
        rdf:type            owl:ObjectProperty;
        rdfs:comment        "Specifies the CartesianPoint2Ds that are used in the BuildingBlockSpecification2D.\n"@en;
        rdfs:domain         vec:BuildingBlockSpecification2D;
        rdfs:label          "cartesianPoint"@en;
        rdfs:range          vec:CartesianPoint2D;
        rdfs:subPropertyOf  vec:contains .

vec:housingComponentDescription
        rdf:type            owl:ObjectProperty;
        rdfs:comment        "Specifies additional, human readable information about the HousingComponent .\n"@en;
        rdfs:domain         vec:HousingComponent;
        rdfs:label          "description"@en;
        rdfs:range          vec:AbstractLocalizedString;
        rdfs:subPropertyOf  vec:contains .

vec:ContractRole  rdf:type  owl:Class;
        rdfs:comment     "Enumeration for the definition of roles a contractor has in a contract.\n"@en;
        rdfs:label       "ContractRole"@en;
        rdfs:subClassOf  vec:OpenEnumeration .

vec:pinComponentReferenceIdentification
        rdf:type      owl:DatatypeProperty;
        rdfs:comment  "Specifies a unique identification of the PinComponentReference. The identification is guaranteed to be unique within the HousingComponentReference.\n"@en;
        rdfs:domain   vec:PinComponentReference;
        rdfs:label    "identification"@en;
        rdfs:range    xs:string .

vec:LanguageCode_Mt  rdf:type  vec:LanguageCode , owl:NamedIndividiual;
        vec:enumLiteral  "Mt" .

vec:tubeSpecificationBendRadius
        rdf:type            owl:ObjectProperty;
        rdfs:comment        "Specifies the bend radius of the tube.\n"@en;
        rdfs:domain         vec:TubeSpecification;
        rdfs:label          "bendRadius"@en;
        rdfs:range          vec:NumericalValue;
        rdfs:subPropertyOf  vec:contains .

vec:GeometrySegment  rdf:type  owl:Class;
        rdfs:comment     "A GeometrySegment is the geometric representation of a TopologySegment. A TopologySegment may be represented by more than one GeometrySegment. A GeometrySegment is either a GeometrySegment2D or a GeometrySegment3D.\n"@en;
        rdfs:label       "GeometrySegment"@en;
        rdfs:subClassOf  vec:ConfigurableElement .

vec:    rdf:type        owl:Ontology;
        rdfs:comment    "\nThis file is provided under the terms of the MIT license reproduced here.\nCopyright ┬® 2021 prostep ivip association\n\nPermission is hereby granted, free of charge, to any person obtaining a copy of this software and associated documentation files (the \"Software\"), to deal in the Software without restriction, including without limitation the rights to use, copy, modify, merge, publish, distribute, sublicense, and/or sell copies of the Software, and to permit persons to whom the Software is furnished to do so, subject to the following conditions:\nThe above copyright notice and this permission notice shall be included in all copies or substantial portions of the Software.\nTHE SOFTWARE IS PROVIDED \"AS IS\", WITHOUT WARRANTY OF ANY KIND, EXPRESS OR IMPLIED, INCLUDING BUT NOT LIMITED TO THE WARRANTIES OF MERCHANTABILITY, FITNESS FOR A PARTICULAR PURPOSE AND NONINFRINGEMENT. IN NO EVENT SHALL THE AUTHORS OR COPYRIGHT HOLDERS BE LIABLE FOR ANY CLAIM, DAMAGES OR OTHER LIABILITY, WHETHER IN AN ACTION OF CONTRACT, TORT OR OTHERWISE, ARISING FROM, OUT OF OR IN CONNECTION WITH THE SOFTWARE OR THE USE OR OTHER DEALINGS IN THE SOFTWARE.\t\t\n\n---------------------------------------------------------------------------------------------------\n\nGenerated Ontology from VEC model. Changelog can be found at https://track.prostep.com/browse/KBLFRM.\nAttention: If this is a SNAPSHOT version, then this schema is produced by a nightly or preview build, \nis NO OFFICIAL RELEASE and can change at any time.\n\nVersion:   1.1.1\nRevision:  not-set\nTimestamp: not-set\n---------------------------------------------------------------------------------------------------                    \n                "@en;
        rdfs:label      "Vehicle Electric Container Ontology"@en;
        owl:versionIRI  <http://www.prostep.org/ontologies/ecad/2024/03/vec/1.1.1#> .

vec:signalSignalForm  rdf:type  owl:ObjectProperty;
        rdfs:comment        "Specifies the form of the signal.\n"@en;
        rdfs:domain         vec:Signal;
        rdfs:label          "signalForm"@en;
        rdfs:range          vec:SignalForm;
        rdfs:subPropertyOf  vec:contains .

vec:partVersionWrapperItem
        rdf:type      owl:ObjectProperty;
        rdfs:comment  "References the actual item for a Wrapper.";
        rdfs:domain   vec:PartVersionWrapper;
        rdfs:range    vec:PartVersion .

vec:eEComponentRoleMountingCavity
        rdf:type      owl:ObjectProperty;
        rdfs:comment  "Specifies the cavities to which into which the EE-component is mounted. \n"@en;
        rdfs:domain   vec:EEComponentRole;
        rdfs:label    "mountingCavity"@en;
        rdfs:range    vec:CavityReference .

vec:abstractSlotSlotNumber
        rdf:type      owl:DatatypeProperty;
        rdfs:comment  "Specifies the number of the slot. This must be unique within a ConnectorHousingSpecification.\n"@en;
        rdfs:domain   vec:AbstractSlot;
        rdfs:label    "slotNumber"@en;
        rdfs:range    xs:string .

vec:LanguageCode_Cs  rdf:type  vec:LanguageCode , owl:NamedIndividiual;
        vec:enumLiteral  "Cs" .

vec:LanguageCode_Tl  rdf:type  vec:LanguageCode , owl:NamedIndividiual;
        vec:enumLiteral  "Tl" .

[ rdf:type     owl:AllDisjointClasses;
  owl:members  ( vec:AliasIdentification vec:ExtendableElement vec:AbstractLocalizedString vec:CustomProperty vec:ConductorCurrentInformation vec:PartRelation vec:PinCurrentInformation vec:PinOpticalInformation vec:PinTiming vec:PinVoltageInformation vec:SealedCavitiesAssignment vec:SlotLayout vec:TerminalCurrentInformation vec:WireType vec:OpenCavitiesAssignment vec:PowerConsumption vec:HousingComponentReference vec:PinComponentReference vec:WireReceptionReference vec:TerminalReceptionReference vec:CavityMapping vec:SlotMapping vec:Person vec:AbrasionResistanceClass vec:Color vec:MassInformation vec:Material vec:RobustnessProperties vec:SealingClass vec:Size vec:SoundDampingClass vec:TemperatureInformation vec:Unit vec:ValueWithUnit vec:CartesianVector )
] .

vec:relaySpecificationRelaisType
        rdf:type      owl:DatatypeProperty;
        rdfs:comment  "The type of the relay. This should be an enumeration of values defined in a conformance class.\n"@en;
        rdfs:domain   vec:RelaySpecification;
        rdfs:label    "relaisType"@en;
        rdfs:range    xs:string .

vec:cavityWireAddOn  rdf:type  owl:ObjectProperty;
        rdfs:comment        "Specifies the wire length add on needed for the cavity.\n"@en;
        rdfs:domain         vec:Cavity;
        rdfs:label          "wireAddOn"@en;
        rdfs:range          vec:NumericalValue;
        rdfs:subPropertyOf  vec:contains .

vec:LanguageCode_Kn  rdf:type  vec:LanguageCode , owl:NamedIndividiual;
        vec:enumLiteral  "Kn" .

vec:SpliceType  rdf:type  owl:Class;
        rdfs:comment     "Enumeration for the definition of type of splice.\n"@en;
        rdfs:label       "SpliceType"@en;
        rdfs:subClassOf  vec:OpenEnumeration .

vec:SlotGender_Male  rdf:type  vec:SlotGender , owl:NamedIndividiual;
        vec:enumLiteral  "Male" .

vec:routingRoutedElement
        rdf:type      owl:ObjectProperty;
        rdfs:comment  "Specifies the Element that is routed. \n"@en;
        rdfs:domain   vec:Routing;
        rdfs:label    "routedElement"@en;
        rdfs:range    vec:RoutableElement .

vec:LanguageCode_Si  rdf:type  vec:LanguageCode , owl:NamedIndividiual;
        vec:enumLiteral  "Si" .

vec:mappingSpecificationMapping
        rdf:type            owl:ObjectProperty;
        rdfs:comment        ""@en;
        rdfs:domain         vec:MappingSpecification;
        rdfs:label          "mapping"@en;
        rdfs:range          vec:Mapping;
        rdfs:subPropertyOf  vec:contains .

[ rdf:type     owl:AllDisjointClasses;
  owl:members  ( vec:NumericalValue vec:ValueRange )
] .

vec:enumLiteral  rdf:type   owl:DatatypeProperty;
        rdfs:comment        "Defines the literal value of an enumeration as represented in the model."@en;
        rdfs:domain         vec:Enumeration;
        rdfs:label          "enumLiteral"@en;
        rdfs:range          xs:string;
        rdfs:subPropertyOf  rdfs:label .

vec:SignalTransmissionMediumType_Optical
        rdf:type         vec:SignalTransmissionMediumType , owl:NamedIndividiual;
        vec:enumLiteral  "optical" .

vec:LanguageCode_Am  rdf:type  vec:LanguageCode , owl:NamedIndividiual;
        vec:enumLiteral  "Am" .

vec:personDepartment  rdf:type  owl:DatatypeProperty;
        rdfs:comment  "Specifies the department the person belongs to.\n"@en;
        rdfs:domain   vec:Person;
        rdfs:label    "department"@en;
        rdfs:range    xs:string .

vec:wireMountingDetailContactedWireReception
        rdf:type      owl:ObjectProperty;
        rdfs:comment  "References the WireReception that is used for the WireMounting. \n"@en;
        rdfs:domain   vec:WireMountingDetail;
        rdfs:label    "contactedWireReception"@en;
        rdfs:range    vec:WireReceptionReference .

vec:PartRelationType_OneOfAll
        rdf:type         vec:PartRelationType , owl:NamedIndividiual;
        rdfs:comment     " OneOfAll means that in a usage of a component exactly one of the referenced acessoryParts must be selected.\n"@en;
        vec:enumLiteral  "OneOfAll" .

vec:ShieldSpecification
        rdf:type         owl:Class;
        rdfs:comment     "Specifies the properties of a shield.\n"@en;
        rdfs:label       "ShieldSpecification"@en;
        rdfs:subClassOf  vec:ConductorSpecification .

vec:LanguageCode_Za  rdf:type  vec:LanguageCode , owl:NamedIndividiual;
        vec:enumLiteral  "Za" .

vec:contactSystemReferencedCoreSpecification
        rdf:type      owl:ObjectProperty;
        rdfs:comment  "References the CoreSpecification that is used on both sides of the ContactSystem.\n"@en;
        rdfs:domain   vec:ContactSystem;
        rdfs:label    "referencedCoreSpecification"@en;
        rdfs:range    vec:ConductorSpecification .

vec:CableDuctOutlet  rdf:type  owl:Class;
        rdfs:comment     "Specifies one outlet of the cableduct.\n"@en;
        rdfs:label       "CableDuctOutlet"@en;
        rdfs:subClassOf  vec:ExtendableElement .

vec:OccurrenceOrUsageViewItem3D
        rdf:type         owl:Class;
        rdfs:comment     "An OccurrenceOrUsageViewItem3D specifies the representation of an OcurrenceOrUsage in a 3D-model.\n"@en;
        rdfs:label       "OccurrenceOrUsageViewItem3D"@en;
        rdfs:subClassOf  vec:ExtendableElement .

vec:CopyrightInformation
        rdf:type         owl:Class;
        rdfs:comment     "A CopyrightInformation-instance specifies copyright information for one or more Items.\n"@en;
        rdfs:label       "CopyrightInformation"@en;
        rdfs:subClassOf  vec:ExtendableElement .

vec:terminalReceptionSpecificationPullOutForce
        rdf:type            owl:ObjectProperty;
        rdfs:comment        "The force until the terminal is pulled out of the housing (normally a not intended case). KBLFRM-366\n"@en;
        rdfs:domain         vec:TerminalReceptionSpecification;
        rdfs:label          "pullOutForce"@en;
        rdfs:range          vec:NumericalValue;
        rdfs:subPropertyOf  vec:contains .

vec:connectionSpecificationConnection
        rdf:type            owl:ObjectProperty;
        rdfs:comment        "Specifies the Connection defined by the ConnectionSpecification.\n"@en;
        rdfs:domain         vec:ConnectionSpecification;
        rdfs:label          "connection"@en;
        rdfs:range          vec:Connection;
        rdfs:subPropertyOf  vec:contains .

vec:LanguageCode_He  rdf:type  vec:LanguageCode , owl:NamedIndividiual;
        vec:enumLiteral  "He" .

vec:SiUnitName_Second
        rdf:type         vec:SiUnitName , owl:NamedIndividiual;
        vec:enumLiteral  "Second" .

vec:PlacementType  rdf:type  owl:Class;
        rdfs:comment         "Defines the type for which a PlaceableElement can be used.\n"@en;
        rdfs:label           "PlacementType"@en;
        rdfs:subClassOf      vec:ClosedEnumeration;
        owl:equivalentClass  [ rdf:type   owl:Class;
                               owl:oneOf  ( vec:PlacementType_OnWay vec:PlacementType_OnPoint )
                             ] .

vec:networkPortSignalDirection
        rdf:type            owl:ObjectProperty;
        rdfs:comment        "Specifies the direction of the signal on this NetworkPort.\n"@en;
        rdfs:domain         vec:NetworkPort;
        rdfs:label          "signalDirection"@en;
        rdfs:range          vec:SignalDirection;
        rdfs:subPropertyOf  vec:contains .

vec:GeometryNode2D  rdf:type  owl:Class;
        rdfs:comment     "A GeometryNode2D is the geometric representation of a TopologyNode in 2D-space.\n"@en;
        rdfs:label       "GeometryNode2D"@en;
        rdfs:subClassOf  vec:GeometryNode .

vec:generalTechnicalPartSpecificationPartRelation
        rdf:type            owl:ObjectProperty;
        rdfs:comment        "Specifies possible relations (accessories) of the specified part with other PartVersion (e.g. caps, clips). "@en;
        rdfs:domain         vec:GeneralTechnicalPartSpecification;
        rdfs:label          "partRelation"@en;
        rdfs:range          vec:PartRelation;
        rdfs:subPropertyOf  vec:contains .

vec:BatterySpecification
        rdf:type         owl:Class;
        rdfs:comment     "Specification of the electrological aspects of a battery.\n"@en;
        rdfs:label       "BatterySpecification"@en;
        rdfs:subClassOf  vec:EEComponentSpecification .

vec:generalTechnicalPartSpecificationRobustnessProperties
        rdf:type            owl:ObjectProperty;
        rdfs:comment        "Specifies the robustness of a part.\n"@en;
        rdfs:domain         vec:GeneralTechnicalPartSpecification;
        rdfs:label          "robustnessProperties"@en;
        rdfs:range          vec:RobustnessProperties;
        rdfs:subPropertyOf  vec:contains .

vec:connectionSpecificationConnectionGroup
        rdf:type            owl:ObjectProperty;
        rdfs:comment        "Specifies the ConnectionGroup defined by the ConnectionSpecification.\n"@en;
        rdfs:domain         vec:ConnectionSpecification;
        rdfs:label          "connectionGroup"@en;
        rdfs:range          vec:ConnectionGroup;
        rdfs:subPropertyOf  vec:contains .

vec:Zone  rdf:type       owl:Class;
        rdfs:comment     "A Zone divides a topology in different sections / design spaces. A Zone may be subdivided in further zones.\n"@en;
        rdfs:label       "Zone"@en;
        rdfs:subClassOf  vec:ConfigurableElement .

vec:SiUnitName_Coulomb
        rdf:type         vec:SiUnitName , owl:NamedIndividiual;
        vec:enumLiteral  "Coulomb" .

vec:fittingSpecificationOutlet
        rdf:type            owl:ObjectProperty;
        rdfs:comment        ""@en;
        rdfs:domain         vec:FittingSpecification;
        rdfs:label          "outlet"@en;
        rdfs:range          vec:FittingOutlet;
        rdfs:subPropertyOf  vec:contains .

vec:WireSpecification
        rdf:type         owl:Class;
        rdfs:comment     "Specification for the definition of a wire. This can either be a complex multicore wire or a normal single core. In the VEC a wire is defined by one WireElement, which may be composed from other WireElements.\n"@en;
        rdfs:label       "WireSpecification"@en;
        rdfs:subClassOf  vec:PartOrUsageRelatedSpecification .

vec:SealedCavitiesAssignment
        rdf:type      owl:Class;
        rdfs:comment  "A SealedCavitiesAssignment groups the cavities of ONE connector that are sealed by a MultiCavityPlug. If a MultiCavityPlug fits into more than one connector, than there are as many SealedCavitiesAssignments .\n"@en;
        rdfs:label    "SealedCavitiesAssignment"@en .

vec:ModuleFamilySpecification
        rdf:type         owl:Class;
        rdfs:comment     "Specification for the description of module families (see ModuleFamily).\n"@en;
        rdfs:label       "ModuleFamilySpecification"@en;
        rdfs:subClassOf  vec:Specification .

vec:VariantConfigurationSpecification
        rdf:type         owl:Class;
        rdfs:comment     "Specification for the definition of variant configurations.\n"@en;
        rdfs:label       "VariantConfigurationSpecification"@en;
        rdfs:subClassOf  vec:Specification .

vec:connectorHousingSpecificationCoupleable
        rdf:type      owl:DatatypeProperty;
        rdfs:comment  "Defines whether the connector is coupleable or not. Connectors that are coupleable can be used in an inline position. Connectors that are not coupleable can be connected only to an ECU or something similar.\n"@en;
        rdfs:domain   vec:ConnectorHousingSpecification;
        rdfs:label    "coupleable"@en;
        rdfs:range    xs:boolean .

vec:LanguageCode_My  rdf:type  vec:LanguageCode , owl:NamedIndividiual;
        vec:enumLiteral  "My" .

vec:CavityMounting  rdf:type  owl:Class;
        rdfs:comment     "A CavityMounting defines the cavities (CavityReference) where the contacted elements (Terminal) will be mounted.\n"@en;
        rdfs:label       "CavityMounting"@en;
        rdfs:subClassOf  vec:ExtendableElement .

[ rdf:type     owl:AllDisjointClasses;
  owl:members  ( vec:BoltMountedFixingSpecification vec:EdgeMountedFixingSpecification vec:HoleMountedFixingSpecification )
] .

vec:SegmentForm_Circular
        rdf:type         vec:SegmentForm , owl:NamedIndividiual;
        vec:enumLiteral  "Circular" .

vec:PinType_Inductive
        rdf:type         vec:PinType , owl:NamedIndividiual;
        vec:enumLiteral  "inductive" .

vec:generalTechnicalPartSpecificationColorInformation
        rdf:type            owl:ObjectProperty;
        rdfs:comment        "Specifies the color of the part.\n"@en;
        rdfs:domain         vec:GeneralTechnicalPartSpecification;
        rdfs:label          "colorInformation"@en;
        rdfs:range          vec:Color;
        rdfs:subPropertyOf  vec:contains .

vec:WireGrouping  rdf:type  owl:Class;
        rdfs:comment     "A WireGrouping is the assignment of WireElementReferences to a WireGroupSpecification. A WireGrouping is needed if individual wire (e.g. with own part numbers) should be grouped (e.g. combined to a twisted pair) and the grouping is not have an individual part.\n"@en;
        rdfs:label       "WireGrouping"@en;
        rdfs:subClassOf  vec:ExtendableElement .

vec:StatusOfApproval_Approved
        rdf:type         vec:StatusOfApproval , owl:NamedIndividiual;
        vec:enumLiteral  "Approved" .

vec:PlacementPointReference
        rdf:type         owl:Class;
        rdfs:comment     "A PlacementPointReference is the instance of a PlacementPoint in the context of an OccurrenceOrUsage .\n"@en;
        rdfs:label       "PlacementPointReference"@en;
        rdfs:subClassOf  vec:ExtendableElement .

vec:itemVersionCreation
        rdf:type            owl:ObjectProperty;
        rdfs:comment        "Specifies the information about the creation of the ItemVersion. \n"@en;
        rdfs:domain         vec:ItemVersion;
        rdfs:label          "creation"@en;
        rdfs:range          vec:Creation;
        rdfs:subPropertyOf  vec:contains .

vec:Material  rdf:type  owl:Class;
        rdfs:comment  "Allows the definition of material information. Attributes of the type Material normally have the multiplicity [0..*]. This means that such an attribute can have material values for different referenceSystems . It must not have multiple values for the same referenceSystems .\n"@en;
        rdfs:label    "Material"@en .

vec:LanguageCode_Lv  rdf:type  vec:LanguageCode , owl:NamedIndividiual;
        vec:enumLiteral  "Lv" .

vec:vecContentUnit  rdf:type  owl:ObjectProperty;
        rdfs:comment        "Specifies the Units used in the VEC-file. \n"@en;
        rdfs:domain         vec:VecContent;
        rdfs:label          "unit"@en;
        rdfs:range          vec:Unit;
        rdfs:subPropertyOf  vec:contains .

vec:terminalSpecificationSealingClass
        rdf:type            owl:ObjectProperty;
        rdfs:comment        "Specifies the sealing class of the terminal.\n"@en;
        rdfs:domain         vec:TerminalSpecification;
        rdfs:label          "sealingClass"@en;
        rdfs:range          vec:SealingClass;
        rdfs:subPropertyOf  vec:contains .

vec:NetSpecification  rdf:type  owl:Class;
        rdfs:comment     "Specification for the description of electrological nets.\n"@en;
        rdfs:label       "NetSpecification"@en;
        rdfs:subClassOf  vec:Specification .

vec:variantCodeSpecificationVariantCode
        rdf:type            owl:ObjectProperty;
        rdfs:comment        "Specifies the individual VariantCodes defined in the VariantCodeSpecification.\n"@en;
        rdfs:domain         vec:VariantCodeSpecification;
        rdfs:label          "variantCode"@en;
        rdfs:range          vec:VariantCode;
        rdfs:subPropertyOf  vec:contains .

vec:LanguageCode_Ks  rdf:type  vec:LanguageCode , owl:NamedIndividiual;
        vec:enumLiteral  "Ks" .

vec:cavitySpecificationSealable
        rdf:type      owl:DatatypeProperty;
        rdfs:comment  "Specifies if the cavity is sealable.\n"@en;
        rdfs:domain   vec:CavitySpecification;
        rdfs:label    "sealable"@en;
        rdfs:range    xs:boolean .

vec:UsageConstraint  rdf:type  owl:Class;
        rdfs:comment     "Specifies a constraint of the possible usages for PartVersion or PartUsages. UsageContraints are of part master data information. UsageConstraints specify general restrictions for the application of a PartVersion or PartUsage (e.g. a certain period of time in which the part is allowed to be used). (see KBLFRM-229)\n"@en;
        rdfs:label       "UsageConstraint"@en;
        rdfs:subClassOf  vec:ExtendableElement .

vec:PrimaryPartType_Fuse
        rdf:type         vec:PrimaryPartType , owl:NamedIndividiual;
        vec:enumLiteral  "Fuse" .

vec:LanguageCode_Sn  rdf:type  vec:LanguageCode , owl:NamedIndividiual;
        vec:enumLiteral  "Sn" .

vec:PinCurrentType_MinCurrent
        rdf:type         vec:PinCurrentType , owl:NamedIndividiual;
        vec:enumLiteral  "minCurrent" .

vec:wireElementWireElementSpecification
        rdf:type      owl:ObjectProperty;
        rdfs:comment  "Reference the WireElementSpecification that is represented by the WireElement.\n"@en;
        rdfs:domain   vec:WireElement;
        rdfs:label    "wireElementSpecification"@en;
        rdfs:range    vec:WireElementSpecification .

vec:matingPointIdentification
        rdf:type      owl:DatatypeProperty;
        rdfs:comment  "Specifies a unique identification of the MatingPoint. The identification is guaranteed to be unique within the MatingSpecification.\n"@en;
        rdfs:domain   vec:MatingPoint;
        rdfs:label    "identification"@en;
        rdfs:range    xs:string .

vec:insulationSpecificationLabelIdentificationValue
        rdf:type      owl:DatatypeProperty;
        rdfs:comment  "Specifies the value of a label printed on the insulation of the wire.\n"@en;
        rdfs:domain   vec:InsulationSpecification;
        rdfs:label    "labelIdentificationValue"@en;
        rdfs:range    xs:string .

vec:LanguageCode_Ar  rdf:type  vec:LanguageCode , owl:NamedIndividiual;
        vec:enumLiteral  "Ar" .

vec:MatingPoint  rdf:type  owl:Class;
        rdfs:comment     "A MatingPoint defines the Mating of two terminals. This normally occurs when two inliners are connected. Then terminals of one side (female) are mated with terminals of the other side (male).\n"@en;
        rdfs:label       "MatingPoint"@en;
        rdfs:subClassOf  vec:ConfigurableElement .

vec:terminalRoleTerminalReceptionReference
        rdf:type            owl:ObjectProperty;
        rdfs:comment        "Specifies the TerminalReceptionReferences of this TerminalRole.\n"@en;
        rdfs:domain         vec:TerminalRole;
        rdfs:label          "terminalReceptionReference"@en;
        rdfs:range          vec:TerminalReceptionReference;
        rdfs:subPropertyOf  vec:contains .

vec:PinTimingType_Duration
        rdf:type         vec:PinTimingType , owl:NamedIndividiual;
        vec:enumLiteral  "duration" .

vec:Color  rdf:type   owl:Class;
        rdfs:comment  "Specifies a color value. A color is always defined by a key value. What color is meant by this key value is defined by a standard reference systems (e.g. RAL).\nFor example if a RAL color should be expressed in the terms of the VEC the referenceSystem would be \"RAL\", the key would be the RAL number defined by the standard (e.g. \"1003\" for signal yellow).\n"@en;
        rdfs:label    "Color"@en .

vec:IECUnit  rdf:type    owl:Class;
        rdfs:comment     "The IECUnit class can define quantities in the terms of the IEC-Unit-System by specifying the corresponding IEC prefix (optional) and an IEC unit name.\n"@en;
        rdfs:label       "IECUnit"@en;
        rdfs:subClassOf  vec:Unit .

vec:USUnitName_Inch  rdf:type  vec:USUnitName , owl:NamedIndividiual;
        vec:enumLiteral  "Inch" .

vec:holeMountedFixingSpecificationHoleDiameter
        rdf:type            owl:ObjectProperty;
        rdfs:comment        "Specifies the diameter of the hole in the fixing.\n"@en;
        rdfs:domain         vec:HoleMountedFixingSpecification;
        rdfs:label          "holeDiameter"@en;
        rdfs:range          vec:NumericalValue;
        rdfs:subPropertyOf  vec:contains .

vec:ShrinkableTubeSpecification
        rdf:type         owl:Class;
        rdfs:comment     "Specification of tubes that are shrinkable.\n"@en;
        rdfs:label       "ShrinkableTubeSpecification"@en;
        rdfs:subClassOf  vec:TubeSpecification .

vec:topologySegmentWrapperItem
        rdf:type      owl:ObjectProperty;
        rdfs:comment  "References the actual item for a Wrapper.";
        rdfs:domain   vec:TopologySegmentWrapper;
        rdfs:range    vec:TopologySegment .

vec:usageConstraintProjectPhase
        rdf:type      owl:DatatypeProperty;
        rdfs:comment  "Specifies the project phases to which the usage constraint applies.\n"@en;
        rdfs:domain   vec:UsageConstraint;
        rdfs:label    "projectPhase"@en;
        rdfs:range    xs:string .

vec:documentVersionRelatedDocument
        rdf:type      owl:ObjectProperty;
        rdfs:comment  "The association is an informative link which DocumentVersion are related to each other (e.g. by derivation, A Harness-Drawing is related to a 3D-Model). \n"@en;
        rdfs:domain   vec:DocumentVersion;
        rdfs:label    "relatedDocument"@en;
        rdfs:range    vec:DocumentVersion .

vec:SignalSpecification
        rdf:type         owl:Class;
        rdfs:comment     "Specification for the definition of a list of valid signals.\n"@en;
        rdfs:label       "SignalSpecification"@en;
        rdfs:subClassOf  vec:Specification .

vec:CustomProperty  rdf:type  owl:Class;
        rdfs:comment  "Abstract base class for custom properties. Basically a custom property is key / value pair. The key (propertyType) defines the meaning of the value. A custom property can either be a simple value (string), a numerical value or a value range.\n"@en;
        rdfs:label    "CustomProperty"@en .

vec:USUnitName_Quarter
        rdf:type         vec:USUnitName , owl:NamedIndividiual;
        vec:enumLiteral  "Quarter" .

vec:eEComponentRoleHousingComponentRef
        rdf:type            owl:ObjectProperty;
        rdfs:comment        "Specifies the HousingComponentReferences used in the EEComponentRole. \n(KBLFRM-401)\n"@en;
        rdfs:domain         vec:EEComponentRole;
        rdfs:label          "housingComponentRef"@en;
        rdfs:range          vec:HousingComponentReference;
        rdfs:subPropertyOf  vec:contains .

vec:connectorHousingSpecificationSegmentConnectionPoint
        rdf:type            owl:ObjectProperty;
        rdfs:comment        "Specifies the SegmentConnectionPoints the connector housing.\n"@en;
        rdfs:domain         vec:ConnectorHousingSpecification;
        rdfs:label          "segmentConnectionPoint"@en;
        rdfs:range          vec:SegmentConnectionPoint;
        rdfs:subPropertyOf  vec:contains .

vec:topologySpecificationZone
        rdf:type            owl:ObjectProperty;
        rdfs:comment        "Specifies the Zones that are part of the TopologySpecification.\n"@en;
        rdfs:domain         vec:TopologySpecification;
        rdfs:label          "zone"@en;
        rdfs:range          vec:Zone;
        rdfs:subPropertyOf  vec:contains .

vec:pinComponentBehaviorVoltageInformation
        rdf:type            owl:ObjectProperty;
        rdfs:comment        "Specifies the voltage information of the PinComponent in this PinComponentBehavior . Since the voltage values of a pin can be defined for different types and times it is possible to define multiple PinVoltageInformations for a PinComponentBehavior .\n"@en;
        rdfs:domain         vec:PinComponentBehavior;
        rdfs:label          "voltageInformation"@en;
        rdfs:range          vec:PinVoltageInformation;
        rdfs:subPropertyOf  vec:contains .

vec:usageNodeUsedInProject
        rdf:type      owl:ObjectProperty;
        rdfs:comment  "Specifies the Projects in which the UsageNode can be used.\n"@en;
        rdfs:domain   vec:UsageNode;
        rdfs:label    "usedInProject"@en;
        rdfs:range    vec:Project .

vec:Unit  rdf:type    owl:Class;
        rdfs:comment  "A precisely specified quantity in terms of which the magnitudes of other quantities of the same kind can be stated. The different systems to define units are represented by the subclasses of this class (e.g. SIUnit, ImperialUnit).\n"@en;
        rdfs:label    "Unit"@en .

vec:externalMappingMappedElement
        rdf:type      owl:ObjectProperty;
        rdfs:comment  ""@en;
        rdfs:domain   vec:ExternalMapping;
        rdfs:label    "mappedElement"@en;
        rdfs:range    vec:ExtendableElement .

vec:placeableElementRolePlaceableElementSpecification
        rdf:type      owl:ObjectProperty;
        rdfs:comment  "References the PlaceableElementSpecification that is instanced by this PlaceableElementRole.\n"@en;
        rdfs:domain   vec:PlaceableElementRole;
        rdfs:label    "placeableElementSpecification"@en;
        rdfs:range    vec:PlaceableElementSpecification .

vec:moduleListCompletionComponents
        rdf:type      owl:ObjectProperty;
        rdfs:comment  "References the components that are used as completition, if any of the Modules in the ModuleList appears in a configuration. \n"@en;
        rdfs:domain   vec:ModuleList;
        rdfs:label    "completionComponents"@en;
        rdfs:range    vec:PartOccurrence .

vec:matingDetailFirstTerminalReception
        rdf:type      owl:ObjectProperty;
        rdfs:comment  "References the first terminal reception that is mated.\n"@en;
        rdfs:domain   vec:MatingDetail;
        rdfs:label    "firstTerminalReception"@en;
        rdfs:range    vec:TerminalReceptionReference .

vec:externalMappingExternalReference
        rdf:type      owl:DatatypeProperty;
        rdfs:comment  "Defines the unique key of the external element. How this key shall be interpreted is dependent from the format of the external data source."@en;
        rdfs:domain   vec:ExternalMapping;
        rdfs:label    "externalReference"@en;
        rdfs:range    xs:string .

vec:componentPortSignal
        rdf:type      owl:ObjectProperty;
        rdfs:comment  "References the Signal that is associated with the ComponentPort .\n"@en;
        rdfs:domain   vec:ComponentPort;
        rdfs:label    "signal"@en;
        rdfs:range    vec:Signal .

vec:VecVersion_1.1.1  rdf:type  vec:VecVersion , owl:NamedIndividiual;
        vec:enumLiteral  "1.1.1" .

vec:SiPrefix_Exa  rdf:type  vec:SiPrefix , owl:NamedIndividiual;
        vec:enumLiteral  "Exa" .

vec:componentNodeIdentification
        rdf:type      owl:DatatypeProperty;
        rdfs:comment  "Specifies a unique identification of the ComponentNode. The identification is guaranteed to be unique within the ConnectionSpecification.\n"@en;
        rdfs:domain   vec:ComponentNode;
        rdfs:label    "identification"@en;
        rdfs:range    xs:string .

vec:PinTimingType_OverrunTime
        rdf:type         vec:PinTimingType , owl:NamedIndividiual;
        vec:enumLiteral  "overrunTime" .

vec:pinTimingTime  rdf:type  owl:ObjectProperty;
        rdfs:comment        "Specifies the time value of the timing.\n"@en;
        rdfs:domain         vec:PinTiming;
        rdfs:label          "time"@en;
        rdfs:range          vec:NumericalValue;
        rdfs:subPropertyOf  vec:contains .

vec:connectionInstallationInstruction
        rdf:type            owl:ObjectProperty;
        rdfs:comment        "Specifies installation instruction for the connection.\n"@en;
        rdfs:domain         vec:Connection;
        rdfs:label          "installationInstruction"@en;
        rdfs:range          vec:Instruction;
        rdfs:subPropertyOf  vec:contains .

vec:LanguageCode_Ss  rdf:type  vec:LanguageCode , owl:NamedIndividiual;
        vec:enumLiteral  "Ss" .

vec:RingTerminalRole  rdf:type  owl:Class;
        rdfs:comment     "A RingTerminalRole defines the instance specific properties and relationships of a ring terminal.\n"@en;
        rdfs:label       "RingTerminalRole"@en;
        rdfs:subClassOf  vec:TerminalRole .

vec:usageConstraintToDate
        rdf:type      owl:DatatypeProperty;
        rdfs:comment  "Specifies the upper bound of the time period to which the usage constraint applies.\n"@en;
        rdfs:domain   vec:UsageConstraint;
        rdfs:label    "toDate"@en;
        rdfs:range    xs:dateTime .

vec:SignalTransmissionMediumType
        rdf:type         owl:Class;
        rdfs:label       "SignalTransmissionMediumType"@en;
        rdfs:subClassOf  vec:OpenEnumeration .

vec:UsageConstraintType_Deny
        rdf:type         vec:UsageConstraintType , owl:NamedIndividiual;
        vec:enumLiteral  "Deny" .

vec:UsageNodeType_Fixing
        rdf:type         vec:UsageNodeType , owl:NamedIndividiual;
        vec:enumLiteral  "Fixing" .

vec:localizedTypedStringType
        rdf:type      owl:DatatypeProperty;
        rdfs:comment  "Defines the type of the LocalizedTypedString . This allows the definition of a more detailed semantic than the semantic of the attribute itself with the type LocalizedTypedString.\n"@en;
        rdfs:domain   vec:LocalizedTypedString;
        rdfs:label    "type"@en;
        rdfs:range    xs:string .

vec:variantConfigurationLogisticControlExpression
        rdf:type      owl:DatatypeProperty;
        rdfs:comment  "Specifies a logisticControlExpression expressed as boolean term.\n"@en;
        rdfs:domain   vec:VariantConfiguration;
        rdfs:label    "logisticControlExpression"@en;
        rdfs:range    xs:string .

vec:SiUnitName_Ampere
        rdf:type         vec:SiUnitName , owl:NamedIndividiual;
        vec:enumLiteral  "Ampere" .

vec:changeDescriptionResponsibleDesigner
        rdf:type            owl:ObjectProperty;
        rdfs:comment        "Specifies the design engineer who is/was responsible to perform the change.\n"@en;
        rdfs:domain         vec:ChangeDescription;
        rdfs:label          "responsibleDesigner"@en;
        rdfs:range          vec:Person;
        rdfs:subPropertyOf  vec:contains .

vec:dimensionIdentification
        rdf:type      owl:DatatypeProperty;
        rdfs:comment  "Specifies a unique identification of the Dimension. The identification is guaranteed to be unique within the containing PlacementSpecification.\n"@en;
        rdfs:domain   vec:Dimension;
        rdfs:label    "identification"@en;
        rdfs:range    xs:string .

vec:USUnitName_Pound  rdf:type  vec:USUnitName , owl:NamedIndividiual;
        vec:enumLiteral  "Pound" .

vec:InsulationState_Uninsulated
        rdf:type         vec:InsulationState , owl:NamedIndividiual;
        rdfs:comment     "The splice is not electrically insulated.\n"@en;
        vec:enumLiteral  "Uninsulated" .

vec:wireMountingReferencedWireEnd
        rdf:type      owl:ObjectProperty;
        rdfs:comment  "References the wire ends that are used for the wire mounting. The minimum cardinality is one, because a wire mounting without wire end makes no sense.\nThe maximum cardinality is * in order to support multi crimps.\n"@en;
        rdfs:domain   vec:WireMounting;
        rdfs:label    "referencedWireEnd"@en;
        rdfs:range    vec:WireEnd .

vec:batterySpecificationICool
        rdf:type            owl:ObjectProperty;
        rdfs:comment        "Specifies the battery's current in cool state.\n"@en;
        rdfs:domain         vec:BatterySpecification;
        rdfs:label          "iCool"@en;
        rdfs:range          vec:NumericalValue;
        rdfs:subPropertyOf  vec:contains .

vec:documentVersionSheetOrChapter
        rdf:type            owl:ObjectProperty;
        rdfs:comment        "Specifies SheetOrChapters defined in this DocumentVersion. These are especially useful if the DocumentVersion represents an external reference. \n"@en;
        rdfs:domain         vec:DocumentVersion;
        rdfs:label          "sheetOrChapter"@en;
        rdfs:range          vec:SheetOrChapter;
        rdfs:subPropertyOf  vec:contains .

vec:LanguageCode_Gl  rdf:type  vec:LanguageCode , owl:NamedIndividiual;
        vec:enumLiteral  "Gl" .

vec:Coding  rdf:type     owl:Class;
        rdfs:comment     "Specifies the coding of a slot or a connector housing.\n"@en;
        rdfs:label       "Coding"@en;
        rdfs:subClassOf  vec:ExtendableElement .

vec:TemperatureInformation
        rdf:type      owl:Class;
        rdfs:comment  "Defines the temperature information for a general technical part. It is necessary to define this in an external class and not as an attribute, since a part can have multiple different temperature information e.g. operating temperature, storage temperature, processing temperature, environment temperature. An additional constraint is that one GeneralTechnicalPartSpecification can own multiple TemperatureInformations, but must not have more than one TemperatureInformations of the same temperatureType.\n"@en;
        rdfs:label    "TemperatureInformation"@en .

vec:SiUnitName_Gray  rdf:type  vec:SiUnitName , owl:NamedIndividiual;
        vec:enumLiteral  "Gray" .

vec:OnWayPlacement  rdf:type  owl:Class;
        rdfs:comment     "An OnWayPlacement places an OccurrenceOrUsage onto an area of the Topology (e.g. a tape or a tube). The area is defined by a startLocation and an endLocation. If startLocation and endLocation are not located on the same TopologySegment it is possible to specify a Path of TopologySegments over which the OnWayPlacement goes.\n"@en;
        rdfs:label       "OnWayPlacement"@en;
        rdfs:subClassOf  vec:Placement .

vec:pinVoltageInformationTime
        rdf:type            owl:ObjectProperty;
        rdfs:comment        "Specifies the timing of the PinVoltageInformation .\n"@en;
        rdfs:domain         vec:PinVoltageInformation;
        rdfs:label          "time"@en;
        rdfs:range          vec:PinTiming;
        rdfs:subPropertyOf  vec:contains .

vec:LanguageCode_Fi  rdf:type  vec:LanguageCode , owl:NamedIndividiual;
        vec:enumLiteral  "Fi" .

vec:ImperialUnitName_Pound
        rdf:type         vec:ImperialUnitName , owl:NamedIndividiual;
        vec:enumLiteral  "Pound" .

vec:matingPointSecondTerminalRole
        rdf:type      owl:ObjectProperty;
        rdfs:comment  "References the second terminal that is mated.\n"@en;
        rdfs:domain   vec:MatingPoint;
        rdfs:label    "secondTerminalRole"@en;
        rdfs:range    vec:TerminalRole .

vec:Approval  rdf:type   owl:Class;
        rdfs:comment     "Defines the approval of an ItemVersion. This consists of the StatusOfApproval and the Permissions issued for the approval.\n"@en;
        rdfs:label       "Approval"@en;
        rdfs:subClassOf  vec:ExtendableElement .

vec:SiUnitName_Joule  rdf:type  vec:SiUnitName , owl:NamedIndividiual;
        vec:enumLiteral  "Joule" .

vec:ContactingSpecification
        rdf:type         owl:Class;
        rdfs:comment     "Specification for the description of the contacting. A contacting defines the relationships between Terminals, Seals, Plugs, Cavities and Wires. "@en;
        rdfs:label       "ContactingSpecification"@en;
        rdfs:subClassOf  vec:Specification .

vec:NodeType_Junction
        rdf:type         vec:NodeType , owl:NamedIndividiual;
        rdfs:comment     "A Junction is a TopologyNode where no electrical component is placed.\n"@en;
        vec:enumLiteral  "Junction" .

vec:ValueDetermination_Estimated
        rdf:type         vec:ValueDetermination , owl:NamedIndividiual;
        rdfs:comment     "The value is estimated by a person.\n"@en;
        vec:enumLiteral  "Estimated" .

vec:OtherUnitName_Piece
        rdf:type         vec:OtherUnitName , owl:NamedIndividiual;
        vec:enumLiteral  "Piece" .

vec:IECUnitName  rdf:type    owl:Class;
        rdfs:comment         "Enumeration for the definition of IEC unit names.\n"@en;
        rdfs:label           "IECUnitName"@en;
        rdfs:subClassOf      vec:ClosedEnumeration;
        owl:equivalentClass  [ rdf:type   owl:Class;
                               owl:oneOf  ( vec:IECUnitName_Bit vec:IECUnitName_Byte )
                             ] .

vec:PrimaryPartType_EEComponent
        rdf:type         vec:PrimaryPartType , owl:NamedIndividiual;
        vec:enumLiteral  "EEComponent" .

vec:PrimaryPartType_Relay
        rdf:type         vec:PrimaryPartType , owl:NamedIndividiual;
        vec:enumLiteral  "Relay" .

vec:segmentCrossSectionAreaArea
        rdf:type            owl:ObjectProperty;
        rdfs:comment        "Specifies the value of the cross section area of the segment.\n"@en;
        rdfs:domain         vec:SegmentCrossSectionArea;
        rdfs:label          "area"@en;
        rdfs:range          vec:NumericalValue;
        rdfs:subPropertyOf  vec:contains .

vec:PinVoltageType_OverrunVoltage
        rdf:type         vec:PinVoltageType , owl:NamedIndividiual;
        vec:enumLiteral  "overrunVoltage" .

vec:topologyNodeProcessingInstruction
        rdf:type            owl:ObjectProperty;
        rdfs:comment        "Specifies processing instructions for the TopologyNode.\n"@en;
        rdfs:domain         vec:TopologyNode;
        rdfs:label          "processingInstruction"@en;
        rdfs:range          vec:LocalizedString;
        rdfs:subPropertyOf  vec:contains .

vec:topologySegmentIdentification
        rdf:type      owl:DatatypeProperty;
        rdfs:comment  "Specifies a unique identification of the TopologySegment. The identification is guaranteed to be unique within the TopologySpecification. Over all VEC-documents a TopologySegment-instance can be trusted to be the same if the TopologySpecification-instance is the same (see TopologySpecification) and the identification of the TopologySegment is the same.\n"@en;
        rdfs:domain   vec:TopologySegment;
        rdfs:label    "identification"@en;
        rdfs:range    xs:string .

vec:LanguageCode_Ru  rdf:type  vec:LanguageCode , owl:NamedIndividiual;
        vec:enumLiteral  "Ru" .

vec:fillerSpecificationDiameter
        rdf:type            owl:ObjectProperty;
        rdfs:comment        "Specifies the diameter of the filler.\n"@en;
        rdfs:domain         vec:FillerSpecification;
        rdfs:label          "diameter"@en;
        rdfs:range          vec:NumericalValue;
        rdfs:subPropertyOf  vec:contains .

vec:externalMappingSpecificationMappedDocument
        rdf:type      owl:ObjectProperty;
        rdfs:comment  "Reference to the DocumentVersion that represents the external data source that connected to the VEC content by the ExternalMappingSpecification .\n"@en;
        rdfs:domain   vec:ExternalMappingSpecification;
        rdfs:label    "mappedDocument"@en;
        rdfs:range    vec:DocumentVersion .

vec:geometrySegmentReferenceSegment
        rdf:type      owl:ObjectProperty;
        rdfs:comment  "References the TopologySegment that is represented by the GeometrySegment. \n"@en;
        rdfs:domain   vec:GeometrySegment;
        rdfs:label    "referenceSegment"@en;
        rdfs:range    vec:TopologySegment .

vec:PrimaryPartType_CavitySeal
        rdf:type         vec:PrimaryPartType , owl:NamedIndividiual;
        vec:enumLiteral  "CavitySeal" .

vec:LanguageCode_Iw  rdf:type  vec:LanguageCode , owl:NamedIndividiual;
        vec:enumLiteral  "Iw" .

vec:specificationIdentification
        rdf:type      owl:DatatypeProperty;
        rdfs:comment  "Specifies a unique identification of the specification. The identification is guaranteed to be unique within the document containing the specification. Over all VEC-documents a Specification-instance can be trusted to be identical if the DocumentVersion-instance is the same (see DocumentVersion) and the identification of the Specification is the same.\n"@en;
        rdfs:domain   vec:Specification;
        rdfs:label    "identification"@en;
        rdfs:range    xs:string .

vec:ValueDetermination_Calculated
        rdf:type         vec:ValueDetermination , owl:NamedIndividiual;
        rdfs:comment     "The value is determined by a calculation algorithm.\n"@en;
        vec:enumLiteral  "Calculated" .

vec:RobustnessProperties
        rdf:type      owl:Class;
        rdfs:comment  "Allows the definition of robustness properties. Robustness of component is specified as a level of robustness against a specific influence (e.g. oil, water, UV-light). The influence is specified by the class and the level is specified by the classKey . Valid robustness classes and keys are specified by the reference system. Attributes of the type RobustnessProperties normally have the multiplicity [0..*]. This means that such an attribute can have RobustnessProperties entries for different classReferenceSystems and classes . It must not have multiple entries for the same class and classReferenceSystem .\n"@en;
        rdfs:label    "RobustnessProperties"@en .

vec:IECPrefix_Mebi  rdf:type  vec:IECPrefix , owl:NamedIndividiual;
        vec:enumLiteral  "Mebi" .

vec:batterySpecificationU
        rdf:type            owl:ObjectProperty;
        rdfs:comment        "Specifies the nominal voltage of the battery.\n"@en;
        rdfs:domain         vec:BatterySpecification;
        rdfs:label          "u"@en;
        rdfs:range          vec:NumericalValue;
        rdfs:subPropertyOf  vec:contains .

[ rdf:type     owl:AllDisjointClasses;
  owl:members  ( vec:CompatibilityStatement vec:ContactSystem vec:CavityMounting vec:CavityMountingDetail vec:WireMounting vec:WireMountingDetail vec:ConfigurableElement vec:ConformanceClass vec:ItemVersion vec:SheetOrChapter vec:Specification vec:VecContent vec:AbstractSlot vec:Cavity vec:Coding vec:HousingComponent vec:InternalTerminalConnection vec:PinComponent vec:SegmentConnectionPoint vec:TerminalReception vec:TerminalType vec:WireElement vec:WireReception vec:ExternalMapping vec:CartesianDimension vec:CartesianPoint2D vec:OccurrenceOrUsageViewItem2D vec:PathSegment vec:Transformation2D vec:BSplineCurve vec:CartesianPoint3D vec:OccurrenceOrUsageViewItem3D vec:Transformation3D vec:Role vec:AbstractSlotReference vec:CavityReference vec:WireEnd vec:WireGrouping vec:WireLength vec:Instruction vec:Mapping vec:MatingDetail vec:ModuleFamily vec:ModuleList vec:CableDuctOutlet vec:CableLeadThrough vec:FittingOutlet vec:Approval vec:ChangeDescription vec:Contract vec:CopyrightInformation vec:Creation vec:ItemEquivalence vec:ItemHistoryEntry vec:Permission vec:Project vec:Tolerance vec:MeasurementPoint vec:PlacementPoint vec:DimensionAnchor vec:PlacementPointReference vec:Signal vec:SegmentCrossSectionArea vec:SegmentLength vec:UsageConstraint vec:VariantCode vec:VariantConfiguration vec:VariantGroup )
] .

vec:wireElementSpecificationMinBendRadiusStatic
        rdf:type            owl:ObjectProperty;
        rdfs:comment        "Specifies the minimum bend radius for wire element, if it is used in a static environment, where it is bended once during installation. After that it remains unchanged in its bended position during usage. (see KLBFRM-311)\n"@en;
        rdfs:domain         vec:WireElementSpecification;
        rdfs:label          "minBendRadiusStatic"@en;
        rdfs:range          vec:NumericalValue;
        rdfs:subPropertyOf  vec:contains .

vec:variantGroupSpecificationVariantGroup
        rdf:type            owl:ObjectProperty;
        rdfs:comment        "Specifies the individual VariantGroups defined in the VariantGroupSpecification.\n"@en;
        rdfs:domain         vec:VariantGroupSpecification;
        rdfs:label          "variantGroup"@en;
        rdfs:range          vec:VariantGroup;
        rdfs:subPropertyOf  vec:contains .

vec:insulationSpecificationMaterial
        rdf:type            owl:ObjectProperty;
        rdfs:comment        "Specifies the material of the insulation.\n"@en;
        rdfs:domain         vec:InsulationSpecification;
        rdfs:label          "material"@en;
        rdfs:range          vec:Material;
        rdfs:subPropertyOf  vec:contains .

vec:Location  rdf:type   owl:Class;
        rdfs:comment     "A Location specifies a distinct position on a topology. Locations can be used for the placement of components or for the definition of Dimensions.\n"@en;
        rdfs:label       "Location"@en;
        rdfs:subClassOf  vec:DimensionAnchor .

vec:robustnessPropertiesDescription
        rdf:type            owl:ObjectProperty;
        rdfs:comment        "On optional human readable description of the robustnes (e.g. the name).\n"@en;
        rdfs:domain         vec:RobustnessProperties;
        rdfs:label          "description"@en;
        rdfs:range          vec:LocalizedString;
        rdfs:subPropertyOf  vec:contains .

vec:terminalSpecificationAngle
        rdf:type            owl:ObjectProperty;
        rdfs:comment        "Specifies the angle against two planes of the connector housing a terminal can be buckled.\n"@en;
        rdfs:domain         vec:TerminalSpecification;
        rdfs:label          "angle"@en;
        rdfs:range          vec:NumericalValue;
        rdfs:subPropertyOf  vec:contains .

vec:ContractRole_Supplier
        rdf:type         vec:ContractRole , owl:NamedIndividiual;
        vec:enumLiteral  "Supplier" .

vec:dimensionReferenceAnchor
        rdf:type      owl:ObjectProperty;
        rdfs:comment  "References the location that is used as reference point for the dimensioning (e.g. the location of a fixing as this relates to a fixpoint of the body in white).\nSee KBLFRM-329 and KBLFRM-391.\n"@en;
        rdfs:domain   vec:Dimension;
        rdfs:label    "referenceAnchor"@en;
        rdfs:range    vec:DimensionAnchor .

vec:transformation2DA12
        rdf:type     owl:DatatypeProperty;
        rdfs:domain  vec:Transformation2D;
        rdfs:label   "a12"@en;
        rdfs:range   xs:double .

vec:geometrySegmentAliasId
        rdf:type            owl:ObjectProperty;
        rdfs:comment        "Specifies additional identifiers for the GeometrySegment.\n"@en;
        rdfs:domain         vec:GeometrySegment;
        rdfs:label          "aliasId"@en;
        rdfs:range          vec:AliasIdentification;
        rdfs:subPropertyOf  vec:contains .

vec:transformation3DA31
        rdf:type     owl:DatatypeProperty;
        rdfs:domain  vec:Transformation3D;
        rdfs:label   "a31"@en;
        rdfs:range   xs:double .

vec:geometrySegment2DEndNode
        rdf:type      owl:ObjectProperty;
        rdfs:comment  "References the GeometryNode2D where the GeometrySegment2D ends. \n"@en;
        rdfs:domain   vec:GeometrySegment2D;
        rdfs:label    "endNode"@en;
        rdfs:range    vec:GeometryNode2D .

vec:tubeSpecificationIsSlit
        rdf:type      owl:DatatypeProperty;
        rdfs:comment  "Specifies whether the tube is slit or not.\n"@en;
        rdfs:domain   vec:TubeSpecification;
        rdfs:label    "isSlit"@en;
        rdfs:range    xs:boolean .

vec:ImperialUnitName_Rood
        rdf:type         vec:ImperialUnitName , owl:NamedIndividiual;
        vec:enumLiteral  "Rood" .

vec:pinTimingType  rdf:type  owl:ObjectProperty;
        rdfs:comment        "Specifies the type of the timing.\n"@en;
        rdfs:domain         vec:PinTiming;
        rdfs:label          "type"@en;
        rdfs:range          vec:PinTimingType;
        rdfs:subPropertyOf  vec:contains .

vec:networkNodePort  rdf:type  owl:ObjectProperty;
        rdfs:comment        "Specifies the NetworkPorts of a NetworkNode. \n"@en;
        rdfs:domain         vec:NetworkNode;
        rdfs:label          "port"@en;
        rdfs:range          vec:NetworkPort;
        rdfs:subPropertyOf  vec:contains .

vec:componentNodeChildNode
        rdf:type            owl:ObjectProperty;
        rdfs:comment        "Specifies the ComponentNodes that are a child of this ComponentNode.\n"@en;
        rdfs:domain         vec:ComponentNode;
        rdfs:label          "childNode"@en;
        rdfs:range          vec:ComponentNode;
        rdfs:subPropertyOf  vec:contains .

vec:placeableElementSpecificationValidPlacementTypes
        rdf:type            owl:ObjectProperty;
        rdfs:comment        "Defines the PlacementTypes that are valid for this element.\n"@en;
        rdfs:domain         vec:PlaceableElementSpecification;
        rdfs:label          "validPlacementTypes"@en;
        rdfs:range          vec:PlacementType;
        rdfs:subPropertyOf  vec:contains .

vec:buildingBlockSpecification3DZone
        rdf:type      owl:ObjectProperty;
        rdfs:comment  "References the Zone that is building block describes. \n"@en;
        rdfs:domain   vec:BuildingBlockSpecification3D;
        rdfs:label    "zone"@en;
        rdfs:range    vec:Zone .

vec:valueRangePropertyValue
        rdf:type            owl:ObjectProperty;
        rdfs:comment        "Defines the value of the CustomProperty.\n"@en;
        rdfs:domain         vec:ValueRangeProperty;
        rdfs:label          "value"@en;
        rdfs:range          vec:ValueRange;
        rdfs:subPropertyOf  vec:contains .

vec:CavitySpecification
        rdf:type         owl:Class;
        rdfs:comment     "Specification for the definition of cavities.\n"@en;
        rdfs:label       "CavitySpecification"@en;
        rdfs:subClassOf  vec:Specification .

[ rdf:type     owl:AllDisjointClasses;
  owl:members  ( vec:FittingSpecification vec:StripeSpecification vec:TapeSpecification vec:TubeSpecification )
] .

vec:compositionSpecificationComponent
        rdf:type            owl:ObjectProperty;
        rdfs:comment        "Specifies the PartOccurrences defined in the CompositionSpecification.\n"@en;
        rdfs:domain         vec:CompositionSpecification;
        rdfs:label          "component"@en;
        rdfs:range          vec:PartOccurrence;
        rdfs:subPropertyOf  vec:contains .

vec:wireProtectionSpecificationSoundDampingClass
        rdf:type            owl:ObjectProperty;
        rdfs:comment        "Specifies the class of sound damping. According to the VDA this is a value between A & E. KBLFRM-311\n"@en;
        rdfs:domain         vec:WireProtectionSpecification;
        rdfs:label          "soundDampingClass"@en;
        rdfs:range          vec:SoundDampingClass;
        rdfs:subPropertyOf  vec:contains .

vec:terminalReceptionSpecificationPlatingMaterial
        rdf:type            owl:ObjectProperty;
        rdfs:comment        "Specifies the plating material of the terminal reception.\n"@en;
        rdfs:domain         vec:TerminalReceptionSpecification;
        rdfs:label          "platingMaterial"@en;
        rdfs:range          vec:Material;
        rdfs:subPropertyOf  vec:contains .

vec:buildingBlockPositioning3DPositioning
        rdf:type            owl:ObjectProperty;
        rdfs:comment        "Specifies the positioning of the building block in the harness geometry.\n"@en;
        rdfs:domain         vec:BuildingBlockPositioning3D;
        rdfs:label          "positioning"@en;
        rdfs:range          vec:Transformation3D;
        rdfs:subPropertyOf  vec:contains .

vec:cavityCavityNumber
        rdf:type      owl:DatatypeProperty;
        rdfs:comment  "Provides an identifier for the cavity. The cavity number needs to be unique within a Slot .\n"@en;
        rdfs:domain   vec:Cavity;
        rdfs:label    "cavityNumber"@en;
        rdfs:range    xs:string .

vec:variantGroupVariantCode
        rdf:type      owl:ObjectProperty;
        rdfs:comment  "References the VariantCodes that are member of the VariantGroup. \n"@en;
        rdfs:domain   vec:VariantGroup;
        rdfs:label    "variantCode"@en;
        rdfs:range    vec:VariantCode .

vec:PinTimingType_BlockTime
        rdf:type         vec:PinTimingType , owl:NamedIndividiual;
        vec:enumLiteral  "blockTime" .

vec:PinTiming  rdf:type  owl:Class;
        rdfs:comment  "Specifies the timing for a PinCurrentInformation or a PinVoltageInformation .\n"@en;
        rdfs:label    "PinTiming"@en .

vec:UsageNodeType_Component
        rdf:type         vec:UsageNodeType , owl:NamedIndividiual;
        vec:enumLiteral  "Component" .

vec:TypeOfPermission_Released
        rdf:type         vec:TypeOfPermission , owl:NamedIndividiual;
        vec:enumLiteral  "Released" .

vec:partUsagePrimaryPartUsageType
        rdf:type            owl:ObjectProperty;
        rdfs:comment        "The primary type of the PartUsage defines the type of the described part (e.g. ConnectorHousing, Fixing, etc.) Since the VEC supports dual use parts (e.g. Fixing & WireProtection) there is no direct connection between the primaryPartUsageType and the allowed specifications for the description of a PartUsage.\n"@en;
        rdfs:domain         vec:PartUsage;
        rdfs:label          "primaryPartUsageType"@en;
        rdfs:range          vec:PrimaryPartType;
        rdfs:subPropertyOf  vec:contains .

vec:mappingB  rdf:type  owl:ObjectProperty;
        rdfs:comment  ""@en;
        rdfs:domain   vec:Mapping;
        rdfs:label    "B"@en;
        rdfs:range    vec:PartVersion .

vec:Connection  rdf:type  owl:Class;
        rdfs:comment     "A Connection is an electrological connection between two or more ComponentPorts.\n"@en;
        rdfs:label       "Connection"@en;
        rdfs:subClassOf  vec:RoutableElement .

vec:ConnectorHousingSpecification
        rdf:type         owl:Class;
        rdfs:comment     "Specification for the definition of connector housings. A connector housing consists of a one or more slots. In the means of the VEC, a connector housing can be a conventional connector housing, a contact module or a connector shell.\n"@en;
        rdfs:label       "ConnectorHousingSpecification"@en;
        rdfs:subClassOf  vec:PartOrUsageRelatedSpecification .

vec:placeableElementRolePlacementPointReference
        rdf:type            owl:ObjectProperty;
        rdfs:comment        ""@en;
        rdfs:domain         vec:PlaceableElementRole;
        rdfs:label          "placementPointReference"@en;
        rdfs:range          vec:PlacementPointReference;
        rdfs:subPropertyOf  vec:contains .

vec:moduleListDescription
        rdf:type            owl:ObjectProperty;
        rdfs:comment        "Room for additional, human readable information about the ModuleList.\n"@en;
        rdfs:domain         vec:ModuleList;
        rdfs:label          "description"@en;
        rdfs:range          vec:AbstractLocalizedString;
        rdfs:subPropertyOf  vec:contains .

vec:multiCavityPlugSpecificationAssignment
        rdf:type            owl:ObjectProperty;
        rdfs:comment        "References the SealedCavitiesAssignments that are valid for this MultiCavityPlug . One individual SealedCavitiesAssignment is used for each connector housing that matches witch this MultiCavityPlug.\n"@en;
        rdfs:domain         vec:MultiCavityPlugSpecification;
        rdfs:label          "assignment"@en;
        rdfs:range          vec:SealedCavitiesAssignment;
        rdfs:subPropertyOf  vec:contains .

vec:usageNodeIdentification
        rdf:type      owl:DatatypeProperty;
        rdfs:comment  "Specifies a unique identification of the UsageNode . The identification is guaranteed to be unique within the context. Over all VEC-documents a UsageNode-instance can be trusted to be the same if the context-instance is the same and the identification of the UsageNode is the same.\n"@en;
        rdfs:domain   vec:UsageNode;
        rdfs:label    "identification"@en;
        rdfs:range    xs:string .

vec:LanguageCode_Zu  rdf:type  vec:LanguageCode , owl:NamedIndividiual;
        rdfs:comment     "Zulu\n"@en;
        vec:enumLiteral  "Zu" .

vec:TapingDirection  rdf:type  owl:Class;
        rdfs:comment     "Defines the direction of a taping. Right means clockwise in the direction of the segment. Left means in the other direction.\n"@en;
        rdfs:label       "TapingDirection"@en;
        rdfs:subClassOf  vec:OpenEnumeration .

vec:TypeOfPermission  rdf:type  owl:Class;
        rdfs:comment     "Enumeration for the definition of the type of a permission.\n"@en;
        rdfs:label       "TypeOfPermission"@en;
        rdfs:subClassOf  vec:OpenEnumeration .

vec:VariantCodeSpecification
        rdf:type         owl:Class;
        rdfs:comment     "Specification for the definition of variant codes.\n"@en;
        rdfs:label       "VariantCodeSpecification"@en;
        rdfs:subClassOf  vec:Specification .

vec:pinVoltageInformationType
        rdf:type            owl:ObjectProperty;
        rdfs:comment        "Defines the type of the voltage.\n"@en;
        rdfs:domain         vec:PinVoltageInformation;
        rdfs:label          "type"@en;
        rdfs:range          vec:PinVoltageType;
        rdfs:subPropertyOf  vec:contains .

vec:TopologyNode  rdf:type  owl:Class;
        rdfs:comment     "A TopologyNode is a point in the Topology where TopologySegments are starting and ending.\n"@en;
        rdfs:label       "TopologyNode"@en;
        rdfs:subClassOf  vec:ConfigurableElement .

vec:LanguageCode_Hy  rdf:type  vec:LanguageCode , owl:NamedIndividiual;
        vec:enumLiteral  "Hy" .

vec:ContactSystemSpecification
        rdf:type         owl:Class;
        rdfs:comment     "Specification for the definition of ContactSystems.\n"@en;
        rdfs:label       "ContactSystemSpecification"@en;
        rdfs:subClassOf  vec:Specification .

vec:USUnitName_Stone  rdf:type  vec:USUnitName , owl:NamedIndividiual;
        vec:enumLiteral  "Stone" .

vec:ChangeDescription
        rdf:type         owl:Class;
        rdfs:comment     "A ChangeDescription describes the implemented issues that are reason for the aggregating ItemVersion to be either an initial or successor version. A ChangeDescription can optionally define the person who has approved the change.\n"@en;
        rdfs:label       "ChangeDescription"@en;
        rdfs:subClassOf  vec:ExtendableElement .

vec:LanguageCode_Pt  rdf:type  vec:LanguageCode , owl:NamedIndividiual;
        vec:enumLiteral  "Pt" .

vec:documentVersionNumberOfSheets
        rdf:type      owl:DatatypeProperty;
        rdfs:comment  "The number of sheets contained in the document.\n"@en;
        rdfs:domain   vec:DocumentVersion;
        rdfs:label    "numberOfSheets"@en;
        rdfs:range    xs:string .

vec:changeDescriptionIdentification
        rdf:type      owl:DatatypeProperty;
        rdfs:comment  "Specifies an identifier for the ChangeDescription. This can be the ID of a changeOrder or an ID which indicates model upgrading. (see KBLFRM-249)\n"@en;
        rdfs:domain   vec:ChangeDescription;
        rdfs:label    "identification"@en;
        rdfs:range    xs:string .

vec:aliasIdentificationScope
        rdf:type      owl:DatatypeProperty;
        rdfs:comment  "The scope in which the AliasIdentification is valid.\n"@en;
        rdfs:domain   vec:AliasIdentification;
        rdfs:label    "Scope"@en;
        rdfs:range    xs:string .

vec:ImperialUnitName_Stone
        rdf:type         vec:ImperialUnitName , owl:NamedIndividiual;
        vec:enumLiteral  "Stone" .

vec:compatibilitySpecificationCompatibilityStatement
        rdf:type            owl:ObjectProperty;
        rdfs:comment        "Specifies the CompatibilityStatements defined by this CompatibilitySpecification.\n"@en;
        rdfs:domain         vec:CompatibilitySpecification;
        rdfs:label          "compatibilityStatement"@en;
        rdfs:range          vec:CompatibilityStatement;
        rdfs:subPropertyOf  vec:contains .

vec:wireLengthLengthValue
        rdf:type            owl:ObjectProperty;
        rdfs:comment        "The length value for the type.\n"@en;
        rdfs:domain         vec:WireLength;
        rdfs:label          "lengthValue"@en;
        rdfs:range          vec:NumericalValue;
        rdfs:subPropertyOf  vec:contains .

vec:wireElementSpecificationConductorSpecification
        rdf:type      owl:ObjectProperty;
        rdfs:comment  "If the WireElement has a core then the specification of the core is referenced here.\n"@en;
        rdfs:domain   vec:WireElementSpecification;
        rdfs:label    "conductorSpecification"@en;
        rdfs:range    vec:ConductorSpecification .

vec:signalSignalName  rdf:type  owl:DatatypeProperty;
        rdfs:comment  "The name of the signal.\n"@en;
        rdfs:domain   vec:Signal;
        rdfs:label    "signalName"@en;
        rdfs:range    xs:string .

vec:ExtendableElement
        rdf:type      owl:Class;
        rdfs:comment  "Abstract base class for extendable elements. Extendable elements have the possibility to define non-standard custom properties.\n"@en;
        rdfs:label    "ExtendableElement"@en .

vec:transformation3DA23
        rdf:type     owl:DatatypeProperty;
        rdfs:domain  vec:Transformation3D;
        rdfs:label   "a23"@en;
        rdfs:range   xs:double .

vec:componentNodeAbbreviation
        rdf:type            owl:ObjectProperty;
        rdfs:comment        "Room for a short name of the ComponentNode.\n"@en;
        rdfs:domain         vec:ComponentNode;
        rdfs:label          "abbreviation"@en;
        rdfs:range          vec:LocalizedString;
        rdfs:subPropertyOf  vec:contains .

vec:USUnitName_FluidOunce
        rdf:type         vec:USUnitName , owl:NamedIndividiual;
        vec:enumLiteral  "FluidOunce" .

vec:cavityMappingIdentificationA
        rdf:type      owl:DatatypeProperty;
        rdfs:comment  "The identification of the Cavity on side A\n"@en;
        rdfs:domain   vec:CavityMapping;
        rdfs:label    "identificationA"@en;
        rdfs:range    xs:string .

vec:LanguageCode_Vi  rdf:type  vec:LanguageCode , owl:NamedIndividiual;
        vec:enumLiteral  "Vi" .

vec:wireElementSpecificationType
        rdf:type            owl:ObjectProperty;
        rdfs:comment        "Defines the type of the wire. A wire must not have more than one type. This attribute allows more than one value for the reason, that the same type can be expressed in multiple reference systems.\n"@en;
        rdfs:domain         vec:WireElementSpecification;
        rdfs:label          "type"@en;
        rdfs:range          vec:WireType;
        rdfs:subPropertyOf  vec:contains .

vec:MeasurementPoint  rdf:type  owl:Class;
        rdfs:comment     "Defines a reference point on a component that can be used to apply a Dimension. This is normally a significant point of the component e.g. an edge, a hole, a bolt or something similar.\n"@en;
        rdfs:label       "MeasurementPoint"@en;
        rdfs:subClassOf  vec:ExtendableElement .

vec:LanguageCode_Mk  rdf:type  vec:LanguageCode , owl:NamedIndividiual;
        vec:enumLiteral  "Mk" .

vec:PinCurrentType  rdf:type  owl:Class;
        rdfs:comment     "Defines the different available current types of a pin.\n"@en;
        rdfs:label       "PinCurrentType"@en;
        rdfs:subClassOf  vec:OpenEnumeration .

vec:PrimaryPartType_Terminal
        rdf:type         vec:PrimaryPartType , owl:NamedIndividiual;
        vec:enumLiteral  "Terminal" .

vec:PartVersionWrapper
        rdf:type      owl:Class;
        rdfs:comment  "Container class for PartVersion to participate in non-unique and/or ordered associations." .

vec:Tolerance  rdf:type  owl:Class;
        rdfs:comment     "Enables the specification of value ranges which can be tolerated.\n"@en;
        rdfs:label       "Tolerance"@en;
        rdfs:subClassOf  vec:ExtendableElement .

vec:USUnitName_Thou  rdf:type  vec:USUnitName , owl:NamedIndividiual;
        vec:enumLiteral  "Thou" .

vec:PrimaryPartType_CorrugatedPipe
        rdf:type         vec:PrimaryPartType , owl:NamedIndividiual;
        vec:enumLiteral  "CorrugatedPipe" .

vec:usageConstraintFromDate
        rdf:type      owl:DatatypeProperty;
        rdfs:comment  "Specifies the lower bound of the time period to which the usage constraint applies.\n"@en;
        rdfs:domain   vec:UsageConstraint;
        rdfs:label    "fromDate"@en;
        rdfs:range    xs:dateTime .

vec:tubeSpecificationNominalSize
        rdf:type      owl:DatatypeProperty;
        rdfs:comment  "Defines the nominal size of a tube. The nominal size is a name for the size of the tube that is somehow related to the inner diameter of the tube. However it is not the inner diameter (e.g. \"10.5\").\n"@en;
        rdfs:domain   vec:TubeSpecification;
        rdfs:label    "nominalSize"@en;
        rdfs:range    xs:string .

vec:TerminalSpecification
        rdf:type         owl:Class;
        rdfs:comment     "Specification for the definition of terminals. A terminal can own multiple WireReceptions & TerminalReceptions.\n"@en;
        rdfs:label       "TerminalSpecification"@en;
        rdfs:subClassOf  vec:PartOrUsageRelatedSpecification .

vec:measurementPointIdentification
        rdf:type      owl:DatatypeProperty;
        rdfs:comment  "Specifies a unique identification of the MeasurementPoint. The identification is guaranteed to be unique within a component.\n"@en;
        rdfs:domain   vec:MeasurementPoint;
        rdfs:label    "identification"@en;
        rdfs:range    xs:string .

vec:PrimaryPartType_PluggableTerminal
        rdf:type         vec:PrimaryPartType , owl:NamedIndividiual;
        vec:enumLiteral  "PluggableTerminal" .

vec:fixingRoleFixingSpecification
        rdf:type      owl:ObjectProperty;
        rdfs:comment  "References the FixingSpecification that is instanced by this FixingRole.\n"@en;
        rdfs:domain   vec:FixingRole;
        rdfs:label    "fixingSpecification"@en;
        rdfs:range    vec:FixingSpecification .

vec:matingDetailIdentification
        rdf:type     owl:DatatypeProperty;
        rdfs:domain  vec:MatingDetail;
        rdfs:label   "identification"@en;
        rdfs:range   xs:string .

vec:tapeSpecificationCoilCoreDiameter
        rdf:type            owl:ObjectProperty;
        rdfs:comment        "Specifies the inner diameter of the coil on which the tape is delivered.\n"@en;
        rdfs:domain         vec:TapeSpecification;
        rdfs:label          "coilCoreDiameter"@en;
        rdfs:range          vec:NumericalValue;
        rdfs:subPropertyOf  vec:contains .

vec:itemVersionCompanyName
        rdf:type      owl:DatatypeProperty;
        rdfs:comment  "Defines the publishing company of the ItemVersion. The companyName is part of the main identifier of an ItemVersion together with the corresponding number (partNumber or documentNumber) and version (partVersion or documentVersion).\n"@en;
        rdfs:domain   vec:ItemVersion;
        rdfs:label    "companyName"@en;
        rdfs:range    xs:string .

vec:occurrenceOrUsageViewItem2DAliasId
        rdf:type            owl:ObjectProperty;
        rdfs:comment        "Specifies additional identifiers for the OccurrenceOrUsageViewItem2D.\n"@en;
        rdfs:domain         vec:OccurrenceOrUsageViewItem2D;
        rdfs:label          "aliasId"@en;
        rdfs:range          vec:AliasIdentification;
        rdfs:subPropertyOf  vec:contains .

vec:LanguageCode_Bg  rdf:type  vec:LanguageCode , owl:NamedIndividiual;
        vec:enumLiteral  "Bg" .

vec:WireRole  rdf:type   owl:Class;
        rdfs:comment     "A WireRole defines the instance specific properties and relationships of a wire.\n"@en;
        rdfs:label       "WireRole"@en;
        rdfs:subClassOf  vec:Role .

vec:tapeSpecificationThickness
        rdf:type            owl:ObjectProperty;
        rdfs:comment        "Specifies the thickness of the tape (adhesive + backing).\n"@en;
        rdfs:domain         vec:TapeSpecification;
        rdfs:label          "thickness"@en;
        rdfs:range          vec:NumericalValue;
        rdfs:subPropertyOf  vec:contains .

vec:PrimaryPartType_ConnectorHousing
        rdf:type         vec:PrimaryPartType , owl:NamedIndividiual;
        vec:enumLiteral  "ConnectorHousing" .

vec:topologySegmentProcessingInstruction
        rdf:type            owl:ObjectProperty;
        rdfs:comment        "Specifies processing instructions for the TopologySegment.\n"@en;
        rdfs:domain         vec:TopologySegment;
        rdfs:label          "processingInstruction"@en;
        rdfs:range          vec:LocalizedString;
        rdfs:subPropertyOf  vec:contains .

vec:shrinkableTubeSpecificationWaterAbsorbtion
        rdf:type            owl:ObjectProperty;
        rdfs:comment        "Defines the water absorption of the shrinkable tube specification.\n"@en;
        rdfs:domain         vec:ShrinkableTubeSpecification;
        rdfs:label          "waterAbsorbtion"@en;
        rdfs:range          vec:NumericalValue;
        rdfs:subPropertyOf  vec:contains .

vec:componentPortSignalDirection
        rdf:type            owl:ObjectProperty;
        rdfs:comment        "Specifies the direction of the signal on this ComponentPort.\n"@en;
        rdfs:domain         vec:ComponentPort;
        rdfs:label          "signalDirection"@en;
        rdfs:range          vec:SignalDirection;
        rdfs:subPropertyOf  vec:contains .

vec:ModuleListSpecification
        rdf:type         owl:Class;
        rdfs:comment     "Specification for the description of module lists (see ModuleList).\n"@en;
        rdfs:label       "ModuleListSpecification"@en;
        rdfs:subClassOf  vec:Specification .

vec:contactSystemSpecificationContactSystem
        rdf:type            owl:ObjectProperty;
        rdfs:comment        "Specifies the ContactSystems described by the ContactSystemSpecification.\n"@en;
        rdfs:domain         vec:ContactSystemSpecification;
        rdfs:label          "contactSystem"@en;
        rdfs:range          vec:ContactSystem;
        rdfs:subPropertyOf  vec:contains .

vec:insulationSpecificationLabelIdentificationColor
        rdf:type            owl:ObjectProperty;
        rdfs:comment        "Specifies the color of a label printed on the insulation of the wire.\n"@en;
        rdfs:domain         vec:InsulationSpecification;
        rdfs:label          "labelIdentificationColor"@en;
        rdfs:range          vec:Color;
        rdfs:subPropertyOf  vec:contains .

vec:wireRoleWireSpecification
        rdf:type      owl:ObjectProperty;
        rdfs:comment  "References the WireSpecification that is instanced by this WireRole.\n"@en;
        rdfs:domain   vec:WireRole;
        rdfs:label    "wireSpecification"@en;
        rdfs:range    vec:WireSpecification .

vec:stripeSpecificationSegmentDiameter
        rdf:type            owl:ObjectProperty;
        rdfs:comment        "Specifies the valid segment diameter range for which the stripe can be used.\n"@en;
        rdfs:domain         vec:StripeSpecification;
        rdfs:label          "segmentDiameter"@en;
        rdfs:range          vec:ValueRange;
        rdfs:subPropertyOf  vec:contains .

vec:ringTerminalSpecificationBoltType
        rdf:type      owl:DatatypeProperty;
        rdfs:comment  "Specifies the type of the bolt. This should be an enumeration of values defined in a conformance class.\n"@en;
        rdfs:domain   vec:RingTerminalSpecification;
        rdfs:label    "boltType"@en;
        rdfs:range    xs:string .

vec:moduleFamilySpecificationModuleFamily
        rdf:type            owl:ObjectProperty;
        rdfs:comment        "Specifies the ModuleFamilies defined in the ModuleFamilySpecification.\n"@en;
        rdfs:domain         vec:ModuleFamilySpecification;
        rdfs:label          "moduleFamily"@en;
        rdfs:range          vec:ModuleFamily;
        rdfs:subPropertyOf  vec:contains .

vec:occurrenceOrUsageViewItem2DIdentification
        rdf:type      owl:DatatypeProperty;
        rdfs:comment  "Specifies a unique identification of the OccurrenceOrUsageViewItem. The identification is guaranteed to be unique within the BuildingBlockSpecification2D.\n"@en;
        rdfs:domain   vec:OccurrenceOrUsageViewItem2D;
        rdfs:label    "identification"@en;
        rdfs:range    xs:string .

vec:WireElementReference
        rdf:type         owl:Class;
        rdfs:comment     "A WireElementReference represents the usage of a WireElement in the context of a PartUsage or PartOccurrence. For contacting purposes a WireElementReference has WireEnds. KBLFRM-384\n"@en;
        rdfs:label       "WireElementReference"@en;
        rdfs:subClassOf  vec:RoutableElement .

vec:wireEndIdentification
        rdf:type      owl:DatatypeProperty;
        rdfs:comment  "Specifies a unique identification of the WireEnd. The identification is guaranteed to be unique within the WireElementReference.\n"@en;
        rdfs:domain   vec:WireEnd;
        rdfs:label    "identification"@en;
        rdfs:range    xs:string .

vec:OpenCavitiesAssignment
        rdf:type      owl:Class;
        rdfs:comment  "An OpenCavitiesAssignment groups the cavities of ONE connector that are open in a MultiCavitySeal. If a MultiCavitySeal fits into more than one connector, than there are as many OpenCavitiesAssignments.\n"@en;
        rdfs:label    "OpenCavitiesAssignment"@en .

vec:SiPrefix_Micro  rdf:type  vec:SiPrefix , owl:NamedIndividiual;
        vec:enumLiteral  "Micro" .

vec:vecContentGeneratingSystemVersion
        rdf:type      owl:DatatypeProperty;
        rdfs:comment  "Specifies the version of the system that has generated the VEC-file.\n"@en;
        rdfs:domain   vec:VecContent;
        rdfs:label    "generatingSystemVersion"@en;
        rdfs:range    xs:string .

vec:routingIdentification
        rdf:type      owl:DatatypeProperty;
        rdfs:comment  "Specifies a unique identification of the Routing. The identification is guaranteed to be unique within the RoutingSpecification.\n"@en;
        rdfs:domain   vec:Routing;
        rdfs:label    "identification"@en;
        rdfs:range    xs:string .

vec:LanguageCode_Eu  rdf:type  vec:LanguageCode , owl:NamedIndividiual;
        vec:enumLiteral  "Eu" .

vec:pinComponentBehaviorSignal
        rdf:type      owl:ObjectProperty;
        rdfs:comment  "Specifies the Signal associated with the pin in this behavior.\n"@en;
        rdfs:domain   vec:PinComponentBehavior;
        rdfs:label    "signal"@en;
        rdfs:range    vec:Signal .

vec:personPhoneNumber
        rdf:type      owl:DatatypeProperty;
        rdfs:comment  "Specifies the person's phone number.\n"@en;
        rdfs:domain   vec:Person;
        rdfs:label    "phoneNumber"@en;
        rdfs:range    xs:string .

vec:ModularSlot  rdf:type  owl:Class;
        rdfs:comment     "A ModularSlot is a place in a connector housing where different other connector housings can be placed during the assembly (e.g. by clicking them into the connector housing).\n"@en;
        rdfs:label       "ModularSlot"@en;
        rdfs:subClassOf  vec:AbstractSlot .

vec:AbstractSlotReference
        rdf:type         owl:Class;
        rdfs:comment     "An AbstractSlotReference represents the usage of an AbstractSlot in the context of PartUsage or PartOccurrence.\n"@en;
        rdfs:label       "AbstractSlotReference"@en;
        rdfs:subClassOf  vec:ExtendableElement .

vec:PinType_Capacitive
        rdf:type         vec:PinType , owl:NamedIndividiual;
        vec:enumLiteral  "capacitive" .

vec:LanguageCode_Uk  rdf:type  vec:LanguageCode , owl:NamedIndividiual;
        vec:enumLiteral  "Uk" .

vec:slotColorInformation
        rdf:type            owl:ObjectProperty;
        rdfs:comment        "Specifies the color of the slot.\n"@en;
        rdfs:domain         vec:Slot;
        rdfs:label          "colorInformation"@en;
        rdfs:range          vec:Color;
        rdfs:subPropertyOf  vec:contains .

vec:harnessDrawingSpecification2DBuildingBlockPositionings
        rdf:type            owl:ObjectProperty;
        rdfs:comment        "Specifies the BuildingBlockPositioning2Ds that are forming the 2D harness drawing. \n"@en;
        rdfs:domain         vec:HarnessDrawingSpecification2D;
        rdfs:label          "buildingBlockPositionings"@en;
        rdfs:range          vec:BuildingBlockPositioning2D;
        rdfs:subPropertyOf  vec:contains .

vec:LanguageCode_Co  rdf:type  vec:LanguageCode , owl:NamedIndividiual;
        vec:enumLiteral  "Co" .

vec:LanguageCode_Th  rdf:type  vec:LanguageCode , owl:NamedIndividiual;
        vec:enumLiteral  "Th" .

vec:shrinkableTubeSpecificationMaximumLongitudinalShrinkage
        rdf:type            owl:ObjectProperty;
        rdfs:comment        "Defines the shrinkage in longitudinal direction.\n"@en;
        rdfs:domain         vec:ShrinkableTubeSpecification;
        rdfs:label          "maximumLongitudinalShrinkage"@en;
        rdfs:range          vec:NumericalValue;
        rdfs:subPropertyOf  vec:contains .

vec:TopologyGroupSpecification
        rdf:type         owl:Class;
        rdfs:comment     "A TopologyGroupSpecification defines a new Topology based on the grouped Topologies. (see KBLFRM-240)\n"@en;
        rdfs:label       "TopologyGroupSpecification"@en;
        rdfs:subClassOf  vec:TopologySpecification .

vec:LanguageCode_Id  rdf:type  vec:LanguageCode , owl:NamedIndividiual;
        vec:enumLiteral  "Id" .

vec:cavitySpecificationMaxWireElementOutsideDiameter
        rdf:type            owl:ObjectProperty;
        rdfs:comment        "Specifies the maximum diameter a wire is allowed to have to fit into the cavity.\n"@en;
        rdfs:domain         vec:CavitySpecification;
        rdfs:label          "maxWireElementOutsideDiameter"@en;
        rdfs:range          vec:NumericalValue;
        rdfs:subPropertyOf  vec:contains .

vec:UsageNodeType_Grommet
        rdf:type         vec:UsageNodeType , owl:NamedIndividiual;
        vec:enumLiteral  "Grommet" .

vec:connectorHousingRoleSlotReference
        rdf:type            owl:ObjectProperty;
        rdfs:comment        "Specifies the SlotReferences used in the ConnectorHousingRole. \n"@en;
        rdfs:domain         vec:ConnectorHousingRole;
        rdfs:label          "slotReference"@en;
        rdfs:range          vec:AbstractSlotReference;
        rdfs:subPropertyOf  vec:contains .

vec:LanguageCode_Ha  rdf:type  vec:LanguageCode , owl:NamedIndividiual;
        vec:enumLiteral  "Ha" .

vec:SpliceType_InlineSplice
        rdf:type         vec:SpliceType , owl:NamedIndividiual;
        rdfs:comment     "An inlineSplice is a splice where wires from both sides are connected.\n"@en;
        vec:enumLiteral  "InlineSplice" .

vec:slotMappingIdentificationB
        rdf:type      owl:DatatypeProperty;
        rdfs:comment  "The identification of the Slot on side B\n"@en;
        rdfs:domain   vec:SlotMapping;
        rdfs:label    "identificationB"@en;
        rdfs:range    xs:string .

vec:PrimaryPartType_Tube
        rdf:type         vec:PrimaryPartType , owl:NamedIndividiual;
        vec:enumLiteral  "Tube" .

vec:SealState_Unsealed
        rdf:type         vec:SealState , owl:NamedIndividiual;
        rdfs:comment     "The splice is not waterproof.\n"@en;
        vec:enumLiteral  "Unsealed" .

vec:netSpecificationNetGroup
        rdf:type            owl:ObjectProperty;
        rdfs:comment        "Specifies the NetGroup defined in the NetSpecification.\n"@en;
        rdfs:domain         vec:NetSpecification;
        rdfs:label          "netGroup"@en;
        rdfs:range          vec:NetGroup;
        rdfs:subPropertyOf  vec:contains .

vec:approvalPermission
        rdf:type            owl:ObjectProperty;
        rdfs:comment        "Specifies the permission issued with the approval.\n"@en;
        rdfs:domain         vec:Approval;
        rdfs:label          "permission"@en;
        rdfs:range          vec:Permission;
        rdfs:subPropertyOf  vec:contains .

vec:documentVersionItemEquivalence
        rdf:type            owl:ObjectProperty;
        rdfs:comment        "Specifies ItemEquivalances defined by the DocumentVersion.\n"@en;
        rdfs:domain         vec:DocumentVersion;
        rdfs:label          "itemEquivalence"@en;
        rdfs:range          vec:ItemEquivalence;
        rdfs:subPropertyOf  vec:contains .

vec:approvalIdentification
        rdf:type      owl:DatatypeProperty;
        rdfs:comment  "Specifies a unique identification of the approval. The identification is guaranteed to be unique over all VEC-documents. Normally this would reference to a company specific approval number or something similar. KBLFRM-349\n"@en;
        rdfs:domain   vec:Approval;
        rdfs:label    "identification"@en;
        rdfs:range    xs:string .

vec:massInformationDeterminationType
        rdf:type            owl:ObjectProperty;
        rdfs:comment        "Specifies the determination type of the mass information.\n"@en;
        rdfs:domain         vec:MassInformation;
        rdfs:label          "determinationType"@en;
        rdfs:range          vec:ValueDetermination;
        rdfs:subPropertyOf  vec:contains .

vec:PinVoltageType_StartStopVoltage
        rdf:type         vec:PinVoltageType , owl:NamedIndividiual;
        vec:enumLiteral  "startStopVoltage" .

vec:shieldSpecificationOpticalTissueDensity
        rdf:type            owl:ObjectProperty;
        rdfs:comment        "Defines the optical tissue density of the strands of a shield. This is defined as a value in percentage.\n"@en;
        rdfs:domain         vec:ShieldSpecification;
        rdfs:label          "opticalTissueDensity"@en;
        rdfs:range          vec:NumericalValue;
        rdfs:subPropertyOf  vec:contains .

vec:FuseSpecification
        rdf:type         owl:Class;
        rdfs:comment     "Specification of the electrological aspects of a fuse.\n"@en;
        rdfs:label       "FuseSpecification"@en;
        rdfs:subClassOf  vec:EEComponentSpecification .

vec:PrimaryPartType_Fitting
        rdf:type         vec:PrimaryPartType , owl:NamedIndividiual;
        vec:enumLiteral  "Fitting" .

vec:insulationSpecificationSecondIdentificationColor
        rdf:type            owl:ObjectProperty;
        rdfs:comment        "Specifies the second identification color of the insulation.\n"@en;
        rdfs:domain         vec:InsulationSpecification;
        rdfs:label          "secondIdentificationColor"@en;
        rdfs:range          vec:Color;
        rdfs:subPropertyOf  vec:contains .

vec:wireElementReferenceWireLength
        rdf:type            owl:ObjectProperty;
        rdfs:comment        "Specifies the different length of a wire. \n"@en;
        rdfs:domain         vec:WireElementReference;
        rdfs:label          "wireLength"@en;
        rdfs:range          vec:WireLength;
        rdfs:subPropertyOf  vec:contains .

vec:PinTimingType_CurrentPeakDistances
        rdf:type         vec:PinTimingType , owl:NamedIndividiual;
        vec:enumLiteral  "currentPeakDistances" .

vec:wireRoleWireElementReference
        rdf:type            owl:ObjectProperty;
        rdfs:comment        "Specifies the WireElementReferences used in the WireRole. For multi core wires more than one WireElementReference is needed. \n"@en;
        rdfs:domain         vec:WireRole;
        rdfs:label          "wireElementReference"@en;
        rdfs:range          vec:WireElementReference;
        rdfs:subPropertyOf  vec:contains .

vec:ImperialUnitName_Gallon
        rdf:type         vec:ImperialUnitName , owl:NamedIndividiual;
        vec:enumLiteral  "Gallon" .

vec:UsageNodeType  rdf:type  owl:Class;
        rdfs:comment     "Enumeration for the different types of UsageNodes.\n"@en;
        rdfs:label       "UsageNodeType"@en;
        rdfs:subClassOf  vec:OpenEnumeration .

vec:SegmentConnectionPoint
        rdf:type         owl:Class;
        rdfs:comment     "Specifies a point where the connector can be attached to the topology (sometimes called bundle position point or insertion point).\n"@en;
        rdfs:label       "SegmentConnectionPoint"@en;
        rdfs:subClassOf  vec:ExtendableElement .

vec:copyrightInformationItem
        rdf:type      owl:ObjectProperty;
        rdfs:comment  "References all ItemVersions to which the copyright information applies to. \n"@en;
        rdfs:domain   vec:CopyrightInformation;
        rdfs:label    "item"@en;
        rdfs:range    vec:ItemVersion .

vec:connectionEndIdentification
        rdf:type      owl:DatatypeProperty;
        rdfs:comment  "Specifies a unique identification of the ConnectionEnd. The identification is guaranteed to be unique within the ConnectionSpecification.\n"@en;
        rdfs:domain   vec:ConnectionEnd;
        rdfs:label    "identification"@en;
        rdfs:range    xs:string .

vec:BuildingBlockSpecification2D
        rdf:type         owl:Class;
        rdfs:comment     "Specification for the description of a two dimensional building block. A building block is a reusable section of a geometry.\n"@en;
        rdfs:label       "BuildingBlockSpecification2D"@en;
        rdfs:subClassOf  vec:Specification .

vec:UsageNodeSpecification
        rdf:type         owl:Class;
        rdfs:comment     "A UsageNodeSpecification is a container for the specification of UsageNodes.\n"@en;
        rdfs:label       "UsageNodeSpecification"@en;
        rdfs:subClassOf  vec:Specification .

vec:InternalTerminalConnection
        rdf:type         owl:Class;
        rdfs:comment     "An InternalTerminalConnection represents an electrical connection within a terminal. For standard terminals all receptions (wire- and terminal-receptions) have an electrical connection. For non-standard terminals (e.g. coax) only some receptions have an electrical connection. The InternalTerminalConnection is modeled as a separate class and not as relationship between wire- and terminal-reception, since it is possible that a terminal has only one kind of reception (e.g. a parallel connector, a cavity bridge). (see KBLFRM-302)\n"@en;
        rdfs:label       "InternalTerminalConnection"@en;
        rdfs:subClassOf  vec:ExtendableElement .

vec:onWayPlacementPath
        rdf:type            owl:ObjectProperty;
        rdfs:comment        "Specifies the topology path defining the way the OnWayPlacement takes in the topology. \n"@en;
        rdfs:domain         vec:OnWayPlacement;
        rdfs:label          "path"@en;
        rdfs:range          vec:Path;
        rdfs:subPropertyOf  vec:contains .

vec:routingPath  rdf:type   owl:ObjectProperty;
        rdfs:comment        "Specifies a Path on the topology that is used for the routing. \n"@en;
        rdfs:domain         vec:Routing;
        rdfs:label          "path"@en;
        rdfs:range          vec:Path;
        rdfs:subPropertyOf  vec:contains .

vec:connectionDescription
        rdf:type            owl:ObjectProperty;
        rdfs:comment        "Specifies additional, human readable information about the Connection.\n"@en;
        rdfs:domain         vec:Connection;
        rdfs:label          "description"@en;
        rdfs:range          vec:AbstractLocalizedString;
        rdfs:subPropertyOf  vec:contains .

vec:topologyGroupSpecificationTopologySpecification
        rdf:type      owl:ObjectProperty;
        rdfs:comment  ""@en;
        rdfs:domain   vec:TopologyGroupSpecification;
        rdfs:label    "topologySpecification"@en;
        rdfs:range    vec:TopologySpecification .

vec:partOccurrenceReferenceElement
        rdf:type      owl:ObjectProperty;
        rdfs:comment  "References the PartOcurrence for which this PartOccurrence is an accessory.\n"@en;
        rdfs:domain   vec:PartOccurrence;
        rdfs:label    "referenceElement"@en;
        rdfs:range    vec:PartOccurrence .

vec:projectDescription
        rdf:type            owl:ObjectProperty;
        rdfs:comment        "Room for additional information about the item.\n"@en;
        rdfs:domain         vec:Project;
        rdfs:label          "description"@en;
        rdfs:range          vec:AbstractLocalizedString;
        rdfs:subPropertyOf  vec:contains .

vec:placementType  rdf:type  owl:DatatypeProperty;
        rdfs:comment  "Room to specify additional type information of the placement.\n"@en;
        rdfs:domain   vec:Placement;
        rdfs:label    "type"@en;
        rdfs:range    xs:string .

vec:wireLengthLengthType
        rdf:type      owl:DatatypeProperty;
        rdfs:comment  "The type of the length (e.g. DMU, CUT). This should be an enumeration of values defined in a conformance class.\n"@en;
        rdfs:domain   vec:WireLength;
        rdfs:label    "lengthType"@en;
        rdfs:range    xs:string .

vec:pinOpticalInformationFrequency
        rdf:type            owl:ObjectProperty;
        rdfs:comment        "The frequency of the optical signal.\n"@en;
        rdfs:domain         vec:PinOpticalInformation;
        rdfs:label          "frequency"@en;
        rdfs:range          vec:NumericalValue;
        rdfs:subPropertyOf  vec:contains .

vec:LanguageCode_Ko  rdf:type  vec:LanguageCode , owl:NamedIndividiual;
        vec:enumLiteral  "Ko" .

vec:PlaceableElementSpecification
        rdf:type         owl:Class;
        rdfs:comment     "Specification for the general aspects of a component that are enabling the component to be placed in a topology. All components that should have the ability to be placed on a certain position in the topology must have a PlaceableElementSpecification\n"@en;
        rdfs:label       "PlaceableElementSpecification"@en;
        rdfs:subClassOf  vec:PartOrUsageRelatedSpecification .

vec:pinComponentReferenceTerminalRole
        rdf:type            owl:ObjectProperty;
        rdfs:comment        "References the TerminalRole of PinComponentReference. This is required to specify a Mating for EEComponents with other EEComponents or a Harness. \n(KBLFRM-401)\n"@en;
        rdfs:domain         vec:PinComponentReference;
        rdfs:label          "terminalRole"@en;
        rdfs:range          vec:TerminalRole;
        rdfs:subPropertyOf  vec:contains .

vec:StripeSpecification
        rdf:type         owl:Class;
        rdfs:comment     "Specifies a stripe which has fixed length and width. Stripes can be used for example for sealing.\n"@en;
        rdfs:label       "StripeSpecification"@en;
        rdfs:subClassOf  vec:WireProtectionSpecification .

vec:NumericalValueProperty
        rdf:type         owl:Class;
        rdfs:comment     "A custom property with a numerical value. (see KBLFRM-319)\n"@en;
        rdfs:label       "NumericalValueProperty"@en;
        rdfs:subClassOf  vec:CustomProperty .

vec:changeDescriptionLabel
        rdf:type      owl:DatatypeProperty;
        rdfs:comment  "Specifies the label of the change on a drawing for example. If more than one change is issued with one ItemVersion (e.g. change 0001, 0002), in some cases the different changes are labeled on the drawing (e.g. A, B, C).\n"@en;
        rdfs:domain   vec:ChangeDescription;
        rdfs:label    "label"@en;
        rdfs:range    xs:string .

vec:OtherUnitName_Pi  rdf:type  vec:OtherUnitName , owl:NamedIndividiual;
        vec:enumLiteral  "Pi" .

vec:terminalCurrentInformationNominalVoltage
        rdf:type            owl:ObjectProperty;
        rdfs:comment        "Specifies the nominalVoltage for which the CurrentRangeInformation is valid.\n"@en;
        rdfs:domain         vec:TerminalCurrentInformation;
        rdfs:label          "nominalVoltage"@en;
        rdfs:range          vec:NumericalValue;
        rdfs:subPropertyOf  vec:contains .

vec:cartesianDimensionHeight
        rdf:type      owl:DatatypeProperty;
        rdfs:comment  "Specifies the height of the object. The unit of this value is the baseUnit of containing BuildingBlockSpecification2D.\n"@en;
        rdfs:domain   vec:CartesianDimension;
        rdfs:label    "height"@en;
        rdfs:range    xs:double .

vec:pinComponentReferencePinComponent
        rdf:type      owl:ObjectProperty;
        rdfs:comment  "Points to the PinComponent referenced by the PinComponent reference. \n(KBLFRM-401)\n"@en;
        rdfs:domain   vec:PinComponentReference;
        rdfs:label    "pinComponent"@en;
        rdfs:range    vec:PinComponent .

vec:vecContentProject
        rdf:type            owl:ObjectProperty;
        rdfs:comment        "Specifies the Projects used in the VEC-file. \n"@en;
        rdfs:domain         vec:VecContent;
        rdfs:label          "project"@en;
        rdfs:range          vec:Project;
        rdfs:subPropertyOf  vec:contains .

vec:harnessGeometrySpecification3DBuildingBlockPositionings
        rdf:type            owl:ObjectProperty;
        rdfs:comment        "Specifies the BuildingBlockPositioning3Ds that are forming the HarnessGeometrySpecification3D.\n"@en;
        rdfs:domain         vec:HarnessGeometrySpecification3D;
        rdfs:label          "buildingBlockPositionings"@en;
        rdfs:range          vec:BuildingBlockPositioning3D;
        rdfs:subPropertyOf  vec:contains .

vec:SiPrefix_Atto  rdf:type  vec:SiPrefix , owl:NamedIndividiual;
        vec:enumLiteral  "Atto" .

vec:iECUnitIecPrefix  rdf:type  owl:ObjectProperty;
        rdfs:comment        "Specifies the prefix of the IEC unit.\n"@en;
        rdfs:domain         vec:IECUnit;
        rdfs:label          "iecPrefix"@en;
        rdfs:range          vec:IECPrefix;
        rdfs:subPropertyOf  vec:contains .

vec:robustnessPropertiesHasRobustness
        rdf:type      owl:DatatypeProperty;
        rdfs:comment  "Specifies if the described element has a robustness in the specified robustness class. (see KBLFRM-260)\n"@en;
        rdfs:domain   vec:RobustnessProperties;
        rdfs:label    "hasRobustness"@en;
        rdfs:range    xs:boolean .

vec:abstractSlotReferenceReferencedSlot
        rdf:type      owl:ObjectProperty;
        rdfs:comment  "Points to the slot referenced by the slot reference. \n"@en;
        rdfs:domain   vec:AbstractSlotReference;
        rdfs:label    "referencedSlot"@en;
        rdfs:range    vec:AbstractSlot .
